<?xml version="1.0"?>
<!DOCTYPE rdf:RDF [
    <!ENTITY owl "http://www.w3.org/2002/07/owl#" >
    <!ENTITY obo "http://purl.obolibrary.org/obo/" >
    <!ENTITY dc "http://purl.org/dc/elements/1.1/" >
    <!ENTITY xsd "http://www.w3.org/2001/XMLSchema#" >
    <!ENTITY xml "http://www.w3.org/XML/1998/namespace" >
    <!ENTITY rdfs "http://www.w3.org/2000/01/rdf-schema#" >
    <!ENTITY taxon "http://purl.obolibrary.org/obo/NCBITaxon#" >
    <!ENTITY rdf "http://www.w3.org/1999/02/22-rdf-syntax-ns#" >
    <!ENTITY oboInOwl "http://www.geneontology.org/formats/oboInOwl#" >
]>

<rdf:RDF xmlns="http://purl.obolibrary.org/obo/FOODON/imports/product_type_import.owl#"
     xml:base="http://purl.obolibrary.org/obo/FOODON/imports/product_type_import.owl"
     xmlns:rdf="http://www.w3.org/1999/02/22-rdf-syntax-ns#"
     xmlns:owl="http://www.w3.org/2002/07/owl#"
     xmlns:oboInOwl="http://www.geneontology.org/formats/oboInOwl#"
     xmlns:xml="http://www.w3.org/XML/1998/namespace"
     xmlns:xsd="http://www.w3.org/2001/XMLSchema#"
     xmlns:rdfs="http://www.w3.org/2000/01/rdf-schema#"
     xmlns:taxon="http://purl.obolibrary.org/obo/NCBITaxon#"
     xmlns:obo="http://purl.obolibrary.org/obo/"
     xmlns:dc="http://purl.org/dc/elements/1.1/">
    <owl:Ontology rdf:about="http://purl.obolibrary.org/obo/FOODON/imports/product_type_import.owl">
        <dc:contributor xml:lang="en">Damion Dooley</dc:contributor>
    </owl:Ontology>
    


    <!-- 
    ///////////////////////////////////////////////////////////////////////////////////////
    //
    // Classes
    //
    ///////////////////////////////////////////////////////////////////////////////////////
     -->



<owl:Class rdf:about="&obo;FOODON_03400000">
	<rdfs:label xml:lang="en">langual thesaurus root</rdfs:label>
	<obo:IAO_0000412>http://langual.org</obo:IAO_0000412>
	<obo:IAO_0000115 xml:lang="en">2014</obo:IAO_0000115>
	<obo:IAO_0000114 rdf:resource="&obo;IAO_0000428"/>
	<rdfs:comment xml:lang="en">LanguaL curation note: This term is for CLASSIFICATION ONLY; DO NOT USE term in indexing. Use a more precise narrower term.</rdfs:comment>
	<oboInOwl:hasDbXref>LANGUAL:00000</oboInOwl:hasDbXref>
</owl:Class>

<owl:Class rdf:about="&obo;FOODON_03400001">
	<rdfs:label xml:lang="en">product type, not known</rdfs:label>
	<rdfs:subClassOf rdf:resource="&obo;FOODON_03400361"/>
	<obo:IAO_0000412>http://langual.org</obo:IAO_0000412>
	<owl:deprecated rdf:datatype="&xsd;boolean">true</owl:deprecated>
	<obo:IAO_0000114 rdf:resource="&obo;IAO_0000122"/>
	<rdfs:comment xml:lang="en">LanguaL curation note: Used when no product type is evident from the food product name, e.g., 'artificially sweetened food', 'food with herbs added', etc. [FDA CFSAN 1995]</rdfs:comment>
	<oboInOwl:hasDbXref>LANGUAL:A0001</oboInOwl:hasDbXref>
</owl:Class>

<owl:Class rdf:about="&obo;FOODON_03400004">
	<rdfs:label xml:lang="en">product type, other</rdfs:label>
	<rdfs:subClassOf rdf:resource="&obo;FOODON_03400361"/>
	<obo:IAO_0000412>http://langual.org</obo:IAO_0000412>
	<owl:deprecated rdf:datatype="&xsd;boolean">true</owl:deprecated>
	<obo:IAO_0000114 rdf:resource="&obo;IAO_0000122"/>
	<rdfs:comment xml:lang="en">LanguaL curation note: Used only if the product does not fall under any of the major product types listed. [FDA CFSAN 1995]</rdfs:comment>
	<oboInOwl:hasDbXref>LANGUAL:A0004</oboInOwl:hasDbXref>
</owl:Class>

<owl:Class rdf:about="&obo;FOODON_03400100">
	<rdfs:label xml:lang="en">pie, unsweetened, or pizza (us cfr)</rdfs:label>
	<rdfs:subClassOf rdf:resource="&obo;FOODON_03400102"/>
	<obo:IAO_0000412>http://langual.org</obo:IAO_0000412>
	<obo:IAO_0000114 rdf:resource="&obo;IAO_0000428"/>
	<rdfs:comment xml:lang="en">LanguaL curation note: Used only for unsweetened products; sweetened pies are indexed under *PIE, SWEETENED*.</rdfs:comment>
	<oboInOwl:hasSynonym xml:lang="en">pizza pie</oboInOwl:hasSynonym>
	<oboInOwl:hasDbXref>LANGUAL:A0100</oboInOwl:hasDbXref>
</owl:Class>

<owl:Class rdf:about="&obo;FOODON_03400101">
	<rdfs:label xml:lang="en">cultured milk product (us cfr)</rdfs:label>
	<rdfs:subClassOf rdf:resource="&obo;FOODON_03400148"/>
	<obo:IAO_0000412>http://langual.org</obo:IAO_0000412>
	<obo:IAO_0000115 xml:lang="en">Milk modified by adding acid-producing and/or flavor-producing bacteria under controlled conditions.</obo:IAO_0000115>
	<obo:IAO_0000114 rdf:resource="&obo;IAO_0000428"/>
	<oboInOwl:hasSynonym xml:lang="en">milk product, cultured</oboInOwl:hasSynonym>
	<oboInOwl:hasDbXref>LANGUAL:A0101</oboInOwl:hasDbXref>
</owl:Class>

<owl:Class rdf:about="&obo;FOODON_03400102">
	<rdfs:label xml:lang="en">prepared food product with bakery base or enclosure, unsweetened (us cfr)</rdfs:label>
	<rdfs:subClassOf rdf:resource="&obo;FOODON_03400172"/>
	<obo:IAO_0000412>http://langual.org</obo:IAO_0000412>
	<obo:IAO_0000114 rdf:resource="&obo;IAO_0000428"/>
	<oboInOwl:hasSynonym xml:lang="en">crepe, dinner</oboInOwl:hasSynonym>
	<oboInOwl:hasSynonym xml:lang="en">taco, prepared</oboInOwl:hasSynonym>
	<oboInOwl:hasDbXref>LANGUAL:A0102</oboInOwl:hasDbXref>
</owl:Class>

<owl:Class rdf:about="&obo;FOODON_03400103">
	<rdfs:label xml:lang="en">pastry, unsweetened, filled (us cfr)</rdfs:label>
	<rdfs:subClassOf rdf:resource="&obo;FOODON_03400102"/>
	<obo:IAO_0000412>http://langual.org</obo:IAO_0000412>
	<obo:IAO_0000114 rdf:resource="&obo;IAO_0000428"/>
	<oboInOwl:hasSynonym xml:lang="en">empanada</oboInOwl:hasSynonym>
	<oboInOwl:hasSynonym xml:lang="en">knish</oboInOwl:hasSynonym>
	<oboInOwl:hasSynonym xml:lang="en">turnover, unsweetened</oboInOwl:hasSynonym>
	<oboInOwl:hasDbXref>LANGUAL:A0103</oboInOwl:hasDbXref>
</owl:Class>

<owl:Class rdf:about="&obo;FOODON_03400104">
	<rdfs:label xml:lang="en">fruit juice or related product (us cfr)</rdfs:label>
	<rdfs:subClassOf rdf:resource="&obo;FOODON_03400143"/>
	<obo:IAO_0000412>http://langual.org</obo:IAO_0000412>
	<obo:IAO_0000115 xml:lang="en">Liquid food prepared from fruit (21 CFR 146). Products prepared from fruit juice by thickening with pectin are indexed under *FRUIT JELLY*; those thickened with gelatin are under *FRUIT BUTTER, JELLY, PRESERVE OR RELATED PRODUCT*.</obo:IAO_0000115>
	<obo:IAO_0000114 rdf:resource="&obo;IAO_0000428"/>
	<oboInOwl:hasDbXref>LANGUAL:A0104</oboInOwl:hasDbXref>
</owl:Class>

<owl:Class rdf:about="&obo;FOODON_03400105">
	<rdfs:label xml:lang="en">dressing, condiment, gravy or sauce (us cfr)</rdfs:label>
	<rdfs:subClassOf rdf:resource="&obo;FOODON_03401270"/>
	<obo:IAO_0000412>http://langual.org</obo:IAO_0000412>
	<obo:IAO_0000115 xml:lang="en">Seasoned product that contains multiple ingredients and that is used in limited amounts to accompany other foods; excludes flavors, spices and herbs.</obo:IAO_0000115>
	<obo:IAO_0000114 rdf:resource="&obo;IAO_0000428"/>
	<oboInOwl:hasSynonym xml:lang="en">condiment, dressing, gravy or sauce</oboInOwl:hasSynonym>
	<oboInOwl:hasSynonym xml:lang="en">gravy, condiment, dressing or sauce</oboInOwl:hasSynonym>
	<oboInOwl:hasSynonym xml:lang="en">sauce, condiment, dressing or gravy</oboInOwl:hasSynonym>
	<oboInOwl:hasDbXref>LANGUAL:A0105</oboInOwl:hasDbXref>
</owl:Class>

<owl:Class rdf:about="&obo;FOODON_03400106">
	<rdfs:label xml:lang="en">prepared grain or starch product (us cfr)</rdfs:label>
	<rdfs:subClassOf rdf:resource="&obo;FOODON_03400125"/>
	<obo:IAO_0000412>http://langual.org</obo:IAO_0000412>
	<obo:IAO_0000115 xml:lang="en">Food product prepared by drying and/or cooking a mixture of milled grain or non-grain starch with a liquid and usually other ingredients such as sweeteners or fats. Includes sweetened and unsweetened bakery products, macaroni or noodle products and breakfast cereals. Excludes *PUDDING, STARCH*, which is under *CUSTARD OR PUDDING*.</obo:IAO_0000115>
	<obo:IAO_0000114 rdf:resource="&obo;IAO_0000428"/>
	<oboInOwl:hasDbXref>LANGUAL:A0106</oboInOwl:hasDbXref>
</owl:Class>

<owl:Class rdf:about="&obo;FOODON_03400107">
	<rdfs:label xml:lang="en">bakery product, unsweetened (us cfr)</rdfs:label>
	<rdfs:subClassOf rdf:resource="&obo;FOODON_03400191"/>
	<obo:IAO_0000412>http://langual.org</obo:IAO_0000412>
	<obo:IAO_0000115 xml:lang="en">Includes breads, crackers, pie or pizza crusts and pretzels. Excludes glazed, filled or frosted bakery products, which fall under *BAKERY PRODUCT, SWEETENED* and unsweetened filled products that fall under *PREPARED FOOD PRODUCT WITH BAKERY BASE OR ENCLOSURE, UNSWEETENED* or the appropriate narrower term.  See 21 CFR for description of some subgroups.</obo:IAO_0000115>
	<obo:IAO_0000114 rdf:resource="&obo;IAO_0000428"/>
	<oboInOwl:hasSynonym xml:lang="en">crepe, unfilled</oboInOwl:hasSynonym>
	<oboInOwl:hasSynonym xml:lang="en">unfilled crepe</oboInOwl:hasSynonym>
	<oboInOwl:hasSynonym xml:lang="en">unsweetened bakery product</oboInOwl:hasSynonym>
	<oboInOwl:hasDbXref>LANGUAL:A0107</oboInOwl:hasDbXref>
</owl:Class>

<owl:Class rdf:about="&obo;FOODON_03400108">
	<rdfs:label xml:lang="en">pastry shell, unsweetened (us cfr)</rdfs:label>
	<rdfs:subClassOf rdf:resource="&obo;FOODON_03400107"/>
	<obo:IAO_0000412>http://langual.org</obo:IAO_0000412>
	<obo:IAO_0000114 rdf:resource="&obo;IAO_0000428"/>
	<oboInOwl:hasSynonym xml:lang="en">puff pastry</oboInOwl:hasSynonym>
	<oboInOwl:hasDbXref>LANGUAL:A0108</oboInOwl:hasDbXref>
</owl:Class>

<owl:Class rdf:about="&obo;FOODON_03400109">
	<rdfs:label xml:lang="en">pasteurized process cheese spread (us cfr)</rdfs:label>
	<rdfs:subClassOf rdf:resource="&obo;FOODON_03400117"/>
	<obo:IAO_0000412>http://langual.org</obo:IAO_0000412>
	<obo:IAO_0000115 xml:lang="en">Pasteurized cheese product made with mandatory emulsifier and optional dairy ingredients. Milkfat minimum 20% of total; moisture minimum 44%, maximum 60% (21 CFR 133.179, 133.180).</obo:IAO_0000115>
	<obo:IAO_0000114 rdf:resource="&obo;IAO_0000428"/>
	<oboInOwl:hasDbXref>LANGUAL:A0109</oboInOwl:hasDbXref>
</owl:Class>

<owl:Class rdf:about="&obo;FOODON_03400110">
	<rdfs:label xml:lang="en">pasteurized process cheese (us cfr)</rdfs:label>
	<rdfs:subClassOf rdf:resource="&obo;FOODON_03400117"/>
	<obo:IAO_0000412>http://langual.org</obo:IAO_0000412>
	<obo:IAO_0000115 xml:lang="en">Pasteurized cheese product made with mandatory emulsifier and optional milkfat or cream. Milkfat minimum 47% of solids (43% for swiss, 45% for gruyere); moisture maximum 51% (21 CFR 133.169, 133.170, 133.171).</obo:IAO_0000115>
	<obo:IAO_0000114 rdf:resource="&obo;IAO_0000428"/>
	<oboInOwl:hasDbXref>LANGUAL:A0110</oboInOwl:hasDbXref>
</owl:Class>

<owl:Class rdf:about="&obo;FOODON_03400111">
	<rdfs:label xml:lang="en">pasteurized process cheese food (us cfr)</rdfs:label>
	<rdfs:subClassOf rdf:resource="&obo;FOODON_03400117"/>
	<obo:IAO_0000412>http://langual.org</obo:IAO_0000412>
	<obo:IAO_0000115 xml:lang="en">Pasteurized cheese product made with optional emulsifier and optional dairy ingredients. Milkfat minimum 23% of total; moisture maximum 44%.</obo:IAO_0000115>
	<obo:IAO_0000114 rdf:resource="&obo;IAO_0000428"/>
	<oboInOwl:hasDbXref>LANGUAL:A0111</oboInOwl:hasDbXref>
</owl:Class>

<owl:Class rdf:about="&obo;FOODON_03400112">
	<rdfs:label xml:lang="en">nonalcoholic beverage (us cfr)</rdfs:label>
	<rdfs:subClassOf rdf:resource="&obo;FOODON_03400229"/>
	<obo:IAO_0000412>http://langual.org</obo:IAO_0000412>
	<obo:IAO_0000115 xml:lang="en">Beverage containing no more than 0.5% alcohol; it may be flavored, sweetened or carbonated; includes soft drinks and steeped beverages; excludes milk in all forms, fruit juices, diluted fruit juices and vegetable juices.</obo:IAO_0000115>
	<obo:IAO_0000114 rdf:resource="&obo;IAO_0000428"/>
	<oboInOwl:hasSynonym xml:lang="en">malt beverage, nonalcoholic</oboInOwl:hasSynonym>
	<oboInOwl:hasDbXref>LANGUAL:A0112</oboInOwl:hasDbXref>
</owl:Class>

<owl:Class rdf:about="&obo;FOODON_03400113">
	<rdfs:label xml:lang="en">spice or herb (us cfr)</rdfs:label>
	<rdfs:subClassOf rdf:resource="&obo;FOODON_03400133"/>
	<obo:IAO_0000412>http://langual.org</obo:IAO_0000412>
	<obo:IAO_0000115 xml:lang="en">Aromatic or pungent plant product used whole or ground as a seasoning in food products.</obo:IAO_0000115>
	<obo:IAO_0000114 rdf:resource="&obo;IAO_0000428"/>
	<oboInOwl:hasSynonym xml:lang="en">herb or spice</oboInOwl:hasSynonym>
	<oboInOwl:hasDbXref>LANGUAL:A0113</oboInOwl:hasDbXref>
</owl:Class>

<owl:Class rdf:about="&obo;FOODON_03400114">
	<rdfs:label xml:lang="en">frozen dairy dessert (us cfr)</rdfs:label>
	<rdfs:subClassOf rdf:resource="&obo;FOODON_03400164"/>
	<obo:IAO_0000412>http://langual.org</obo:IAO_0000412>
	<obo:IAO_0000115 xml:lang="en">A frozen dessert prepared from one or more dairy ingredients or their analogs, plus other ingredients. Includes frozen dairy items offered in a cone, a sandwich or as a cake or pie, such as frozen yogurt in a cone or an ice cream sandwich; these are also indexed under *GRAIN ADDED*.</obo:IAO_0000115>
	<obo:IAO_0000114 rdf:resource="&obo;IAO_0000428"/>
	<oboInOwl:hasSynonym xml:lang="en">dairy dessert, frozen</oboInOwl:hasSynonym>
	<oboInOwl:hasSynonym xml:lang="en">dessert, frozen dairy</oboInOwl:hasSynonym>
	<oboInOwl:hasDbXref>LANGUAL:A0114</oboInOwl:hasDbXref>
</owl:Class>

<owl:Class rdf:about="&obo;FOODON_03400115">
	<rdfs:label xml:lang="en">cheese or cheese product (us cfr)</rdfs:label>
	<rdfs:subClassOf rdf:resource="&obo;FOODON_03400164"/>
	<obo:IAO_0000412>http://langual.org</obo:IAO_0000412>
	<obo:IAO_0000115 xml:lang="en">Natural cheese, cured or uncured, cheese product (which is further processed), or cheese product analog.</obo:IAO_0000115>
	<obo:IAO_0000114 rdf:resource="&obo;IAO_0000428"/>
	<oboInOwl:hasDbXref>LANGUAL:A0115</oboInOwl:hasDbXref>
</owl:Class>

<owl:Class rdf:about="&obo;FOODON_03400116">
	<rdfs:label xml:lang="en">cold-pack cheese product (us cfr)</rdfs:label>
	<rdfs:subClassOf rdf:resource="&obo;FOODON_03400282"/>
	<obo:IAO_0000412>http://langual.org</obo:IAO_0000412>
	<obo:IAO_0000115 xml:lang="en">Cheese product made without the aid of heat. See 21 CFR 133.123-125 for lists of cheeses that cannot be used.</obo:IAO_0000115>
	<obo:IAO_0000114 rdf:resource="&obo;IAO_0000428"/>
	<oboInOwl:hasSynonym xml:lang="en">cheese product, cold-pack</oboInOwl:hasSynonym>
	<oboInOwl:hasDbXref>LANGUAL:A0116</oboInOwl:hasDbXref>
</owl:Class>

<owl:Class rdf:about="&obo;FOODON_03400117">
	<rdfs:label xml:lang="en">pasteurized cheese product (us cfr)</rdfs:label>
	<rdfs:subClassOf rdf:resource="&obo;FOODON_03400282"/>
	<obo:IAO_0000412>http://langual.org</obo:IAO_0000412>
	<obo:IAO_0000115 xml:lang="en">Food prepared by comminuting and mixing, with the aid of heat, one or more natural cheeses, with or without additional ingredients, into a homogeneous plastic mass; the product is packed while hot. See 21 CFR 133.167-180 for lists of cheeses that cannot be used.</obo:IAO_0000115>
	<obo:IAO_0000114 rdf:resource="&obo;IAO_0000428"/>
	<oboInOwl:hasDbXref>LANGUAL:A0117</oboInOwl:hasDbXref>
</owl:Class>

<owl:Class rdf:about="&obo;FOODON_03400118">
	<rdfs:label xml:lang="en">nutritive sweetener (us cfr)</rdfs:label>
	<rdfs:subClassOf rdf:resource="&obo;FOODON_03400237"/>
	<obo:IAO_0000412>http://langual.org</obo:IAO_0000412>
	<obo:IAO_0000115 xml:lang="en">A substance having greater than 2% of the caloric value of sucrose per equivalent unit of sweetening capacity. For example, the amount of such subtance having the sweetening capacity of 1 teaspoon of sucrose would have more than 0.4 calories (21 CFR 170.3(o)(21)).</obo:IAO_0000115>
	<obo:IAO_0000114 rdf:resource="&obo;IAO_0000428"/>
	<oboInOwl:hasSynonym xml:lang="en">nutritive carbohydrate sweetener</oboInOwl:hasSynonym>
	<oboInOwl:hasSynonym xml:lang="en">sweetener, nutritive</oboInOwl:hasSynonym>
	<oboInOwl:hasDbXref>LANGUAL:A0118</oboInOwl:hasDbXref>
</owl:Class>

<owl:Class rdf:about="&obo;FOODON_03400120">
	<rdfs:label xml:lang="en">neutral distilled spirits (us cfr)</rdfs:label>
	<rdfs:subClassOf rdf:resource="&obo;FOODON_03400277"/>
	<obo:IAO_0000412>http://langual.org</obo:IAO_0000412>
	<obo:IAO_0000115 xml:lang="en">Distilled spirits produced at or above 190 proof and, if bottled, bottled at not less than 80 proof (27 CFR 5.22(a)).</obo:IAO_0000115>
	<obo:IAO_0000114 rdf:resource="&obo;IAO_0000428"/>
	<oboInOwl:hasSynonym xml:lang="en">alcohol or neutral spirits</oboInOwl:hasSynonym>
	<oboInOwl:hasSynonym xml:lang="en">neutral spirits or alcohol</oboInOwl:hasSynonym>
	<oboInOwl:hasDbXref>LANGUAL:A0120</oboInOwl:hasDbXref>
</owl:Class>

<owl:Class rdf:about="&obo;FOODON_03400123">
	<rdfs:label xml:lang="en">cream product analog (us cfr)</rdfs:label>
	<rdfs:subClassOf rdf:resource="&obo;FOODON_03400147"/>
	<obo:IAO_0000412>http://langual.org</obo:IAO_0000412>
	<obo:IAO_0000115 xml:lang="en">Food product having functional characteristics similar to a cream product; it may be nutritionally equivalent or inferior to the product it purports to resemble. Includes nondairy coffee whitener and nondairy topping.</obo:IAO_0000115>
	<obo:IAO_0000114 rdf:resource="&obo;IAO_0000428"/>
	<oboInOwl:hasSynonym xml:lang="en">cream substitute</oboInOwl:hasSynonym>
	<oboInOwl:hasSynonym xml:lang="en">cream, imitation</oboInOwl:hasSynonym>
	<oboInOwl:hasSynonym xml:lang="en">imitation cream</oboInOwl:hasSynonym>
	<oboInOwl:hasSynonym xml:lang="en">whipped topping</oboInOwl:hasSynonym>
	<oboInOwl:hasDbXref>LANGUAL:A0123</oboInOwl:hasDbXref>
</owl:Class>

<owl:Class rdf:about="&obo;FOODON_03400125">
	<rdfs:label xml:lang="en">grain or starch product (us cfr)</rdfs:label>
	<rdfs:subClassOf rdf:resource="&obo;FOODON_03401270"/>
	<obo:IAO_0000412>http://langual.org</obo:IAO_0000412>
	<obo:IAO_0000115 xml:lang="en">Any form of whole or milled grain, prepared grain product or starch containing product derived from non-grain sources. [FDA CFSAN 1995]</obo:IAO_0000115>
	<obo:IAO_0000114 rdf:resource="&obo;IAO_0000428"/>
	<oboInOwl:hasDbXref>LANGUAL:A0125</oboInOwl:hasDbXref>
</owl:Class>

<owl:Class rdf:about="&obo;FOODON_03400126">
	<rdfs:label xml:lang="en">cold-pack cheese food (us cfr)</rdfs:label>
	<rdfs:subClassOf rdf:resource="&obo;FOODON_03400116"/>
	<obo:IAO_0000412>http://langual.org</obo:IAO_0000412>
	<obo:IAO_0000115 xml:lang="en">Cold-pack cheese product made with other dairy ingredients and without emulsifier. Milkfat minimum 23% of total; moisture maximum 44% (21 CFR 133.124, 133.125).</obo:IAO_0000115>
	<obo:IAO_0000114 rdf:resource="&obo;IAO_0000428"/>
	<oboInOwl:hasSynonym xml:lang="en">cheese food, cold-pack</oboInOwl:hasSynonym>
	<oboInOwl:hasSynonym xml:lang="en">cold cheese food</oboInOwl:hasSynonym>
	<oboInOwl:hasDbXref>LANGUAL:A0126</oboInOwl:hasDbXref>
</owl:Class>

<owl:Class rdf:about="&obo;FOODON_03400127">
	<rdfs:label xml:lang="en">fruit juice (us cfr)</rdfs:label>
	<rdfs:subClassOf rdf:resource="&obo;FOODON_03400104"/>
	<obo:IAO_0000412>http://langual.org</obo:IAO_0000412>
	<obo:IAO_0000115 xml:lang="en">The liquid extracted or expressed from mature fruit with or without the application of heat. Includes concentrated juice and single-strength juice. If the single-strength juice is prepared from concentrate, then *WATER ADDED* should be used. Carbonated fruit juices are indexed by *FRUIT JUICE* or *FRUIT JUICE, DILUTED* and *CARBONATED* or the appropriate narrower term.</obo:IAO_0000115>
	<obo:IAO_0000114 rdf:resource="&obo;IAO_0000428"/>
	<oboInOwl:hasSynonym xml:lang="en">juice, fruit</oboInOwl:hasSynonym>
	<oboInOwl:hasDbXref>LANGUAL:A0127</oboInOwl:hasDbXref>
</owl:Class>

<owl:Class rdf:about="&obo;FOODON_03400128">
	<rdfs:label xml:lang="en">cheese product analog (us cfr)</rdfs:label>
	<rdfs:subClassOf rdf:resource="&obo;FOODON_03400115"/>
	<obo:IAO_0000412>http://langual.org</obo:IAO_0000412>
	<obo:IAO_0000115 xml:lang="en">Food product having functional characteristics similar to those of cheese or cheese product; it may be nutritionally equivalent or inferior to the product it purports to resemble. The ingredients may or may not be milk-based. An example is a cheese-like product made from skim milk and vegetable oil.</obo:IAO_0000115>
	<obo:IAO_0000114 rdf:resource="&obo;IAO_0000428"/>
	<oboInOwl:hasSynonym xml:lang="en">cheese substitute</oboInOwl:hasSynonym>
	<oboInOwl:hasSynonym xml:lang="en">cheese, imitation</oboInOwl:hasSynonym>
	<oboInOwl:hasSynonym xml:lang="en">imitation cheese</oboInOwl:hasSynonym>
	<oboInOwl:hasDbXref>LANGUAL:A0128</oboInOwl:hasDbXref>
</owl:Class>

<owl:Class rdf:about="&obo;FOODON_03400129">
	<rdfs:label xml:lang="en">refined or partially-refined food product (us cfr)</rdfs:label>
	<rdfs:subClassOf rdf:resource="&obo;FOODON_03401270"/>
	<obo:IAO_0000412>http://langual.org</obo:IAO_0000412>
	<obo:IAO_0000115 xml:lang="en">Extract, concentrate or isolate derived from a food source through one or more refining steps (see *EXTRACT, CONCENTRATE OR ISOLATE OF PLANT OR ANIMAL*) and marketed as such. [FDA CFSAN 1995]</obo:IAO_0000115>
	<obo:IAO_0000114 rdf:resource="&obo;IAO_0000428"/>
	<oboInOwl:hasDbXref>LANGUAL:A0129</oboInOwl:hasDbXref>
</owl:Class>

<owl:Class rdf:about="&obo;FOODON_03400130">
	<rdfs:label xml:lang="en">fruit juice, diluted (us cfr)</rdfs:label>
	<rdfs:subClassOf rdf:resource="&obo;FOODON_03400104"/>
	<obo:IAO_0000412>http://langual.org</obo:IAO_0000412>
	<obo:IAO_0000115 xml:lang="en">Beverage prepared by diluting fruit juice to less than single strength, based upon accepted soluble solids values. Include beverages containing 15 to 99% fruit juice. *WATER ADDED* or the appropriate narrower term should be used to specify the degree of dilution.</obo:IAO_0000115>
	<obo:IAO_0000114 rdf:resource="&obo;IAO_0000428"/>
	<oboInOwl:hasSynonym xml:lang="en">diluted juice beverage</oboInOwl:hasSynonym>
	<oboInOwl:hasSynonym xml:lang="en">juice beverage, diluted</oboInOwl:hasSynonym>
	<oboInOwl:hasDbXref>LANGUAL:A0130</oboInOwl:hasDbXref>
</owl:Class>

<owl:Class rdf:about="&obo;FOODON_03400131">
	<rdfs:label xml:lang="en">poultry-based sausage or luncheon meat (us cfr)</rdfs:label>
	<rdfs:subClassOf rdf:resource="&obo;FOODON_03400273"/>
	<obo:IAO_0000412>http://langual.org</obo:IAO_0000412>
	<obo:IAO_0000115 xml:lang="en">Food product consisting of comminuted poultry meat, usually seasoned, pressed and/or encased.</obo:IAO_0000115>
	<obo:IAO_0000114 rdf:resource="&obo;IAO_0000428"/>
	<oboInOwl:hasDbXref>LANGUAL:A0131</oboInOwl:hasDbXref>
</owl:Class>

<owl:Class rdf:about="&obo;FOODON_03400132">
	<rdfs:label xml:lang="en">meat product analog (us cfr)</rdfs:label>
	<rdfs:subClassOf rdf:resource="&obo;FOODON_03400150"/>
	<obo:IAO_0000412>http://langual.org</obo:IAO_0000412>
	<obo:IAO_0000115 xml:lang="en">Food product having functional characteristics similar to a meat product; it may be nutritionally equivalent or inferior to the product it purports to resemble. Typically these products are soybean-based.</obo:IAO_0000115>
	<obo:IAO_0000114 rdf:resource="&obo;IAO_0000428"/>
	<oboInOwl:hasSynonym xml:lang="en">imitation meat</oboInOwl:hasSynonym>
	<oboInOwl:hasDbXref>LANGUAL:A0132</oboInOwl:hasDbXref>
</owl:Class>

<owl:Class rdf:about="&obo;FOODON_03400133">
	<rdfs:label xml:lang="en">flavoring or seasoning (us cfr)</rdfs:label>
	<rdfs:subClassOf rdf:resource="&obo;FOODON_03401270"/>
	<obo:IAO_0000412>http://langual.org</obo:IAO_0000412>
	<obo:IAO_0000115 xml:lang="en">Product that imparts or helps to impart a taste or aroma in food (21 CFR.170.3(n)(26). [FDA CFSAN 1995]</obo:IAO_0000115>
	<obo:IAO_0000114 rdf:resource="&obo;IAO_0000428"/>
	<oboInOwl:hasSynonym xml:lang="en">seasoning or flavoring</oboInOwl:hasSynonym>
	<oboInOwl:hasDbXref>LANGUAL:A0133</oboInOwl:hasDbXref>
</owl:Class>

<owl:Class rdf:about="&obo;FOODON_03400134">
	<rdfs:label xml:lang="en">salt or salt substitute (us cfr)</rdfs:label>
	<rdfs:subClassOf rdf:resource="&obo;FOODON_03400133"/>
	<obo:IAO_0000412>http://langual.org</obo:IAO_0000412>
	<obo:IAO_0000115 xml:lang="en">Table salt and its substitutes; also products combining other flavors or seasonings with salt when these are predominantly salt.</obo:IAO_0000115>
	<obo:IAO_0000114 rdf:resource="&obo;IAO_0000428"/>
	<oboInOwl:hasSynonym xml:lang="en">salt substitute or salt</oboInOwl:hasSynonym>
	<oboInOwl:hasDbXref>LANGUAL:A0134</oboInOwl:hasDbXref>
</owl:Class>

<owl:Class rdf:about="&obo;FOODON_03400135">
	<rdfs:label xml:lang="en">bakery product, sweetened (us cfr)</rdfs:label>
	<rdfs:subClassOf rdf:resource="&obo;FOODON_03400191"/>
	<obo:IAO_0000412>http://langual.org</obo:IAO_0000412>
	<obo:IAO_0000115 xml:lang="en">Includes cakes, cookies, pies, quick breads, doughnuts and related products, also bakery products that are glazed, frosted or have a sweetened filling. If sugar is not the first ingredient, *SUGAR OR SUGAR SYRUP ADDED* as well as *SWEETENER ADDED* (or the appropriate narrower term under each) should be indexed in *H. TREATMENT APPLIED*.</obo:IAO_0000115>
	<obo:IAO_0000114 rdf:resource="&obo;IAO_0000428"/>
	<oboInOwl:hasSynonym xml:lang="en">crepe, dessert</oboInOwl:hasSynonym>
	<oboInOwl:hasSynonym xml:lang="en">dessert crepe</oboInOwl:hasSynonym>
	<oboInOwl:hasSynonym xml:lang="en">sweetened bakery product</oboInOwl:hasSynonym>
	<oboInOwl:hasDbXref>LANGUAL:A0135</oboInOwl:hasDbXref>
</owl:Class>

<owl:Class rdf:about="&obo;FOODON_03400136">
	<rdfs:label xml:lang="en">nonstandardized dressing (us cfr)</rdfs:label>
	<rdfs:subClassOf rdf:resource="&obo;FOODON_03400276"/>
	<obo:IAO_0000412>http://langual.org</obo:IAO_0000412>
	<obo:IAO_0000115 xml:lang="en">Dressing for which no standards of identity are specified in the CFR.</obo:IAO_0000115>
	<obo:IAO_0000114 rdf:resource="&obo;IAO_0000428"/>
	<oboInOwl:hasDbXref>LANGUAL:A0136</oboInOwl:hasDbXref>
</owl:Class>

<owl:Class rdf:about="&obo;FOODON_03400137">
	<rdfs:label xml:lang="en">ice cream or frozen custard (us cfr)</rdfs:label>
	<rdfs:subClassOf rdf:resource="&obo;FOODON_03400114"/>
	<obo:IAO_0000412>http://langual.org</obo:IAO_0000412>
	<obo:IAO_0000115 xml:lang="en">A frozen dairy dessert prepared by freezing while stirring a mixture of pasteurized dairy ingredients and other optional ingredients specified in 21 CFR 135.110 (a). These exclude fats and nonnutritive sweeteners not derived from milk; the finished product has at least 10% milk fat and 10% nonfat milk solids.</obo:IAO_0000115>
	<obo:IAO_0000114 rdf:resource="&obo;IAO_0000428"/>
	<oboInOwl:hasSynonym xml:lang="en">frozen custard or ice cream</oboInOwl:hasSynonym>
	<oboInOwl:hasDbXref>LANGUAL:A0137</oboInOwl:hasDbXref>
</owl:Class>

<owl:Class rdf:about="&obo;FOODON_03400138">
	<rdfs:label xml:lang="en">soft cheese (us cfr)</rdfs:label>
	<rdfs:subClassOf rdf:resource="&obo;FOODON_03400316"/>
	<obo:IAO_0000412>http://langual.org</obo:IAO_0000412>
	<obo:IAO_0000115 xml:lang="en">The cheese is cured under conditions suitable for development of biological curing agents on the surface of the cheese, and the curing is conducted so that the cheese cures from the surface toward the center.</obo:IAO_0000115>
	<obo:IAO_0000114 rdf:resource="&obo;IAO_0000428"/>
	<rdfs:comment xml:lang="en">LanguaL curation note: Used for cheeses, which solids contain not less than 50 percent of milkfat [21 CFR Ch. I (4-1-99 Edition)]  -  moisture content not specified.</rdfs:comment>
	<oboInOwl:hasSynonym xml:lang="en">soft-ripened cheese (u.s.)</oboInOwl:hasSynonym>
	<oboInOwl:hasDbXref>LANGUAL:A0138</oboInOwl:hasDbXref>
</owl:Class>

<owl:Class rdf:about="&obo;FOODON_03400139">
	<rdfs:label xml:lang="en">multicomponent meal (us cfr)</rdfs:label>
	<rdfs:subClassOf rdf:resource="&obo;FOODON_03400172"/>
	<obo:IAO_0000412>http://langual.org</obo:IAO_0000412>
	<obo:IAO_0000115 xml:lang="en">A multiple-component food product typically containing a protein source, a vegetable, and a potato, rice or cereal-based component packaged to be served after heating, either as separate items or courses or mixed as recipe components; see 21 CFR 102.26, 102.28 and 104.47 for nutritional quality guidelines.</obo:IAO_0000115>
	<obo:IAO_0000114 rdf:resource="&obo;IAO_0000428"/>
	<oboInOwl:hasSynonym xml:lang="en">compartmentalized dinner</oboInOwl:hasSynonym>
	<oboInOwl:hasSynonym xml:lang="en">dinner with components separated in serving containers</oboInOwl:hasSynonym>
	<oboInOwl:hasSynonym xml:lang="en">dinner, compartmentalized</oboInOwl:hasSynonym>
	<oboInOwl:hasSynonym xml:lang="en">food packs with separate components</oboInOwl:hasSynonym>
	<oboInOwl:hasSynonym xml:lang="en">heat and serve dinner</oboInOwl:hasSynonym>
	<oboInOwl:hasSynonym xml:lang="en">multiple-course dinner</oboInOwl:hasSynonym>
	<oboInOwl:hasSynonym xml:lang="en">tv dinner</oboInOwl:hasSynonym>
	<oboInOwl:hasDbXref>LANGUAL:A0139</oboInOwl:hasDbXref>
</owl:Class>

<owl:Class rdf:about="&obo;FOODON_03400140">
	<rdfs:label xml:lang="en">pie crust, sweetened (us cfr)</rdfs:label>
	<rdfs:subClassOf rdf:resource="&obo;FOODON_03400135"/>
	<obo:IAO_0000412>http://langual.org</obo:IAO_0000412>
	<obo:IAO_0000115 xml:lang="en">Mixture of cookie crumbs or sweetened cracker crumbs and fat that is used as a base for fruit or other pie filling, e.g., graham cracker crust. Also includes ordinary pie crust that has been sweetened.</obo:IAO_0000115>
	<obo:IAO_0000114 rdf:resource="&obo;IAO_0000428"/>
	<oboInOwl:hasDbXref>LANGUAL:A0140</oboInOwl:hasDbXref>
</owl:Class>

<owl:Class rdf:about="&obo;FOODON_03400141">
	<rdfs:label xml:lang="en">aerated confectionery (us cfr)</rdfs:label>
	<rdfs:subClassOf rdf:resource="&obo;FOODON_03400293"/>
	<obo:IAO_0000412>http://langual.org</obo:IAO_0000412>
	<obo:IAO_0000115 xml:lang="en">Confectionery into which a substantial amount of air has been incorporated to produce a sponge-like or chewy texture. Examples are marshmallow and nougat.</obo:IAO_0000115>
	<obo:IAO_0000114 rdf:resource="&obo;IAO_0000428"/>
	<oboInOwl:hasSynonym xml:lang="en">confectionery, aerated</oboInOwl:hasSynonym>
	<oboInOwl:hasDbXref>LANGUAL:A0141</oboInOwl:hasDbXref>
</owl:Class>

<owl:Class rdf:about="&obo;FOODON_03400142">
	<rdfs:label xml:lang="en">nonnutritive sweetener (us cfr)</rdfs:label>
	<rdfs:subClassOf rdf:resource="&obo;FOODON_03400237"/>
	<obo:IAO_0000412>http://langual.org</obo:IAO_0000412>
	<obo:IAO_0000115 xml:lang="en">Substance having less than 2% of the caloric value of sucrose per equivalent unit of sweetening capacity. For example, the amount of such substance having the sweetening capacity of 1 teaspoon of sucrose would have no more than 0.4 calories (21 CFR 170.3(o)(19)).</obo:IAO_0000115>
	<obo:IAO_0000114 rdf:resource="&obo;IAO_0000428"/>
	<oboInOwl:hasSynonym xml:lang="en">sweetener, nonnutritive</oboInOwl:hasSynonym>
	<oboInOwl:hasDbXref>LANGUAL:A0142</oboInOwl:hasDbXref>
</owl:Class>

<owl:Class rdf:about="&obo;FOODON_03400143">
	<rdfs:label xml:lang="en">fruit or fruit product (us cfr)</rdfs:label>
	<rdfs:subClassOf rdf:resource="&obo;FOODON_03400257"/>
	<obo:IAO_0000412>http://langual.org</obo:IAO_0000412>
	<obo:IAO_0000115 xml:lang="en">Fruit in all forms; includes fruit juices and fruit juice drinks, fruit butters, jellies, preserves, and related products.</obo:IAO_0000115>
	<obo:IAO_0000114 rdf:resource="&obo;IAO_0000428"/>
	<oboInOwl:hasSynonym xml:lang="en">pie filling, fruit</oboInOwl:hasSynonym>
	<oboInOwl:hasDbXref>LANGUAL:A0143</oboInOwl:hasDbXref>
</owl:Class>

<owl:Class rdf:about="&obo;FOODON_03400145">
	<rdfs:label xml:lang="en">pasteurized blended cheese (us cfr)</rdfs:label>
	<rdfs:subClassOf rdf:resource="&obo;FOODON_03400117"/>
	<obo:IAO_0000412>http://langual.org</obo:IAO_0000412>
	<obo:IAO_0000115 xml:lang="en">Pasteurized cheese product made without emulsifier and with optional milkfat or cream. Milkfat minimum 47% of solids (43% for swiss, 45% for gruyere). Moisture maximum 51%. (21 CFR 133.167).</obo:IAO_0000115>
	<obo:IAO_0000114 rdf:resource="&obo;IAO_0000428"/>
	<oboInOwl:hasDbXref>LANGUAL:A0145</oboInOwl:hasDbXref>
</owl:Class>

<owl:Class rdf:about="&obo;FOODON_03400146">
	<rdfs:label xml:lang="en">jap or agar jelly candy (us cfr)</rdfs:label>
	<rdfs:subClassOf rdf:resource="&obo;FOODON_03400162"/>
	<obo:IAO_0000412>http://langual.org</obo:IAO_0000412>
	<obo:IAO_0000115 xml:lang="en">Jelly candy having agar as its principal jelling ingredient.</obo:IAO_0000115>
	<obo:IAO_0000114 rdf:resource="&obo;IAO_0000428"/>
	<oboInOwl:hasDbXref>LANGUAL:A0146</oboInOwl:hasDbXref>
</owl:Class>

<owl:Class rdf:about="&obo;FOODON_03400147">
	<rdfs:label xml:lang="en">milk or milk product analog (us cfr)</rdfs:label>
	<rdfs:subClassOf rdf:resource="&obo;FOODON_03400148"/>
	<obo:IAO_0000412>http://langual.org</obo:IAO_0000412>
	<obo:IAO_0000115 xml:lang="en">Food product having functional characteristics similar to milk or milk products, including cream product analogs, margarine, and milk analogs. Certain alternate ingredients are substituted for those components that are responsible for specific functional properties.</obo:IAO_0000115>
	<obo:IAO_0000114 rdf:resource="&obo;IAO_0000428"/>
	<oboInOwl:hasDbXref>LANGUAL:A0147</oboInOwl:hasDbXref>
</owl:Class>

<owl:Class rdf:about="&obo;FOODON_03400148">
	<rdfs:label xml:lang="en">milk or milk product (us cfr)</rdfs:label>
	<rdfs:subClassOf rdf:resource="&obo;FOODON_03400164"/>
	<obo:IAO_0000412>http://langual.org</obo:IAO_0000412>
	<obo:IAO_0000115 xml:lang="en">Milk in all forms, milk-based beverage, cultured milk product, or milk or milk product analog. Index infant formula under *MEAL REPLACEMENT*.</obo:IAO_0000115>
	<obo:IAO_0000114 rdf:resource="&obo;IAO_0000428"/>
	<oboInOwl:hasDbXref>LANGUAL:A0148</oboInOwl:hasDbXref>
</owl:Class>

<owl:Class rdf:about="&obo;FOODON_03400149">
	<rdfs:label xml:lang="en">milled grain or starch product (us cfr)</rdfs:label>
	<rdfs:subClassOf rdf:resource="&obo;FOODON_03400125"/>
	<obo:IAO_0000412>http://langual.org</obo:IAO_0000412>
	<obo:IAO_0000115 xml:lang="en">Food product prepared by milling a grain or by producing flour, meal or grits from a non-grain source such as beans, starchy roots or tubers. Refined starch is indexed under *REFINED OR PARTIALLY REFINED FOOD PRODUCT*.</obo:IAO_0000115>
	<obo:IAO_0000114 rdf:resource="&obo;IAO_0000428"/>
	<oboInOwl:hasDbXref>LANGUAL:A0149</oboInOwl:hasDbXref>
</owl:Class>

<owl:Class rdf:about="&obo;FOODON_03400150">
	<rdfs:label xml:lang="en">meat or meat product (from mammal) (us cfr)</rdfs:label>
	<rdfs:subClassOf rdf:resource="&obo;FOODON_03400217"/>
	<obo:IAO_0000412>http://langual.org</obo:IAO_0000412>
	<obo:IAO_0000115 xml:lang="en">Meat (flesh and organs including blood and bone marrow) from mammals. Used for meat in all forms including cured meat, sausage or luncheon meat and meat product analogs.</obo:IAO_0000115>
	<obo:IAO_0000114 rdf:resource="&obo;IAO_0000428"/>
	<oboInOwl:hasDbXref>LANGUAL:A0150</oboInOwl:hasDbXref>
</owl:Class>

<owl:Class rdf:about="&obo;FOODON_03400151">
	<rdfs:label xml:lang="en">sweet roll or sweet bun (us cfr)</rdfs:label>
	<rdfs:subClassOf rdf:resource="&obo;FOODON_03400135"/>
	<obo:IAO_0000412>http://langual.org</obo:IAO_0000412>
	<obo:IAO_0000115 xml:lang="en">Single-portion yeast-leavened sweetened bakery product.</obo:IAO_0000115>
	<obo:IAO_0000114 rdf:resource="&obo;IAO_0000428"/>
	<oboInOwl:hasSynonym xml:lang="en">roll, sweet</oboInOwl:hasSynonym>
	<oboInOwl:hasSynonym xml:lang="en">sweet bun</oboInOwl:hasSynonym>
	<oboInOwl:hasDbXref>LANGUAL:A0151</oboInOwl:hasDbXref>
</owl:Class>

<owl:Class rdf:about="&obo;FOODON_03400152">
	<rdfs:label xml:lang="en">vegetable or vegetable product (us cfr)</rdfs:label>
	<rdfs:subClassOf rdf:resource="&obo;FOODON_03400257"/>
	<obo:IAO_0000412>http://langual.org</obo:IAO_0000412>
	<obo:IAO_0000115 xml:lang="en">Vegetables in all forms except where a use-related product type descriptior (such as *PREPARED FOOD PRODUCT* or *SNACK FOOD*) takes precedence.</obo:IAO_0000115>
	<obo:IAO_0000114 rdf:resource="&obo;IAO_0000428"/>
	<oboInOwl:hasDbXref>LANGUAL:A0152</oboInOwl:hasDbXref>
</owl:Class>

<owl:Class rdf:about="&obo;FOODON_03400155">
	<rdfs:label xml:lang="en">fruit butter, jelly, preserve or related product (us cfr)</rdfs:label>
	<rdfs:subClassOf rdf:resource="&obo;FOODON_03400143"/>
	<obo:IAO_0000412>http://langual.org</obo:IAO_0000412>
	<obo:IAO_0000115 xml:lang="en">Semisolid or jelled food prepared from fruit or fruit juice and other ingredients prescribed for the individual products (21 CFR 150).</obo:IAO_0000115>
	<obo:IAO_0000114 rdf:resource="&obo;IAO_0000428"/>
	<oboInOwl:hasDbXref>LANGUAL:A0155</oboInOwl:hasDbXref>
</owl:Class>

<owl:Class rdf:about="&obo;FOODON_03400156">
	<rdfs:label xml:lang="en">seafood product analog (us cfr)</rdfs:label>
	<rdfs:subClassOf rdf:resource="&obo;FOODON_03400267"/>
	<obo:IAO_0000412>http://langual.org</obo:IAO_0000412>
	<obo:IAO_0000115 xml:lang="en">Food product having functional characteristics similar to a seafood product; it may be nutritionally equivalent or inferior to the product it purports to resemble.</obo:IAO_0000115>
	<obo:IAO_0000114 rdf:resource="&obo;IAO_0000428"/>
	<oboInOwl:hasSynonym xml:lang="en">engineered seafood</oboInOwl:hasSynonym>
	<oboInOwl:hasSynonym xml:lang="en">imitation seafood product</oboInOwl:hasSynonym>
	<oboInOwl:hasDbXref>LANGUAL:A0156</oboInOwl:hasDbXref>
</owl:Class>

<owl:Class rdf:about="&obo;FOODON_03400157">
	<rdfs:label xml:lang="en">poultry product analog (us cfr)</rdfs:label>
	<rdfs:subClassOf rdf:resource="&obo;FOODON_03400273"/>
	<obo:IAO_0000412>http://langual.org</obo:IAO_0000412>
	<obo:IAO_0000115 xml:lang="en">Food product having functional characteristics similar to a poultry product; it may be nutritionally equivalent or inferior to the product it purports to resemble.</obo:IAO_0000115>
	<obo:IAO_0000114 rdf:resource="&obo;IAO_0000428"/>
	<oboInOwl:hasSynonym xml:lang="en">imitation poultry product</oboInOwl:hasSynonym>
	<oboInOwl:hasSynonym xml:lang="en">poultry-like product</oboInOwl:hasSynonym>
	<oboInOwl:hasSynonym xml:lang="en">poultry-like vegetable protein food</oboInOwl:hasSynonym>
	<oboInOwl:hasSynonym xml:lang="en">simulated poultry meat</oboInOwl:hasSynonym>
	<oboInOwl:hasDbXref>LANGUAL:A0157</oboInOwl:hasDbXref>
</owl:Class>

<owl:Class rdf:about="&obo;FOODON_03400158">
	<rdfs:label xml:lang="en">cacao or chocolate product analog (us cfr)</rdfs:label>
	<rdfs:subClassOf rdf:resource="&obo;FOODON_03400272"/>
	<obo:IAO_0000412>http://langual.org</obo:IAO_0000412>
	<obo:IAO_0000115 xml:lang="en">Food product having functional characteristics, primarily taste, similar to those of a *CACAO OR CHOCOLATE PRODUCT*. Carob or artificial chocolate flavor may replace chocolate or cocoa in the product.</obo:IAO_0000115>
	<obo:IAO_0000114 rdf:resource="&obo;IAO_0000428"/>
	<oboInOwl:hasSynonym xml:lang="en">chocolate or cacao product analog</oboInOwl:hasSynonym>
	<oboInOwl:hasDbXref>LANGUAL:A0158</oboInOwl:hasDbXref>
</owl:Class>

<owl:Class rdf:about="&obo;FOODON_03400159">
	<rdfs:label xml:lang="en">ice cream product analog (us cfr)</rdfs:label>
	<rdfs:subClassOf rdf:resource="&obo;FOODON_03400114"/>
	<obo:IAO_0000412>http://langual.org</obo:IAO_0000412>
	<obo:IAO_0000115 xml:lang="en">Food product having functional characteristics similar to an ice cream product; it may be nutritionally equivalent or inferior to the product it purports to resemble.</obo:IAO_0000115>
	<obo:IAO_0000114 rdf:resource="&obo;IAO_0000428"/>
	<oboInOwl:hasSynonym xml:lang="en">imitation ice cream</oboInOwl:hasSynonym>
	<oboInOwl:hasDbXref>LANGUAL:A0159</oboInOwl:hasDbXref>
</owl:Class>

<owl:Class rdf:about="&obo;FOODON_03400160">
	<rdfs:label xml:lang="en">pie crust, unsweetened (us cfr)</rdfs:label>
	<rdfs:subClassOf rdf:resource="&obo;FOODON_03400107"/>
	<obo:IAO_0000412>http://langual.org</obo:IAO_0000412>
	<obo:IAO_0000115 xml:lang="en">Unsweetened, unleavened mixture of flour and fat that is used as a base for filling. Yeast-leavened pie crust is indexed under *PIZZA CRUST*.</obo:IAO_0000115>
	<obo:IAO_0000114 rdf:resource="&obo;IAO_0000428"/>
	<oboInOwl:hasSynonym xml:lang="en">pie shell</oboInOwl:hasSynonym>
	<oboInOwl:hasDbXref>LANGUAL:A0160</oboInOwl:hasDbXref>
</owl:Class>

<owl:Class rdf:about="&obo;FOODON_03400161">
	<rdfs:label xml:lang="en">fruit or nut candy (us cfr)</rdfs:label>
	<rdfs:subClassOf rdf:resource="&obo;FOODON_03400204"/>
	<obo:IAO_0000412>http://langual.org</obo:IAO_0000412>
	<obo:IAO_0000115 xml:lang="en">Candy in which fruit or nut is the first ingredient.</obo:IAO_0000115>
	<obo:IAO_0000114 rdf:resource="&obo;IAO_0000428"/>
	<oboInOwl:hasSynonym xml:lang="en">nut or fruit candy</oboInOwl:hasSynonym>
	<oboInOwl:hasDbXref>LANGUAL:A0161</oboInOwl:hasDbXref>
</owl:Class>

<owl:Class rdf:about="&obo;FOODON_03400162">
	<rdfs:label xml:lang="en">jelly candy (us cfr)</rdfs:label>
	<rdfs:subClassOf rdf:resource="&obo;FOODON_03400293"/>
	<obo:IAO_0000412>http://langual.org</obo:IAO_0000412>
	<obo:IAO_0000115 xml:lang="en">Candy prepared by cooking together a mixture of sweeteners, water, acids, flavoring agents, other ingredients and jelling agents to a temperature of 226-230 degrees F, which results in a soft-solid product.</obo:IAO_0000115>
	<obo:IAO_0000114 rdf:resource="&obo;IAO_0000428"/>
	<oboInOwl:hasDbXref>LANGUAL:A0162</oboInOwl:hasDbXref>
</owl:Class>

<owl:Class rdf:about="&obo;FOODON_03400164">
	<rdfs:label xml:lang="en">dairy product (us cfr)</rdfs:label>
	<rdfs:subClassOf rdf:resource="&obo;FOODON_03401270"/>
	<obo:IAO_0000412>http://langual.org</obo:IAO_0000412>
	<obo:IAO_0000115 xml:lang="en">Milk, a product derived from milk, or a dairy product analog; includes cheese and frozen dairy desserts. [FDA CFSAN 1995]</obo:IAO_0000115>
	<obo:IAO_0000114 rdf:resource="&obo;IAO_0000428"/>
	<oboInOwl:hasDbXref>LANGUAL:A0164</oboInOwl:hasDbXref>
</owl:Class>

<owl:Class rdf:about="&obo;FOODON_03400165">
	<rdfs:label xml:lang="en">frozen custard (us cfr)</rdfs:label>
	<rdfs:subClassOf rdf:resource="&obo;FOODON_03400137"/>
	<obo:IAO_0000412>http://langual.org</obo:IAO_0000412>
	<obo:IAO_0000115 xml:lang="en">Frozen custard, in comparison with ice cream, contains at least 1.4% egg yolk solids by weight of the finished product (21 CFR 135.110(a)).</obo:IAO_0000115>
	<obo:IAO_0000114 rdf:resource="&obo;IAO_0000428"/>
	<oboInOwl:hasSynonym xml:lang="en">custard, frozen</oboInOwl:hasSynonym>
	<oboInOwl:hasSynonym xml:lang="en">french custard ice cream</oboInOwl:hasSynonym>
	<oboInOwl:hasSynonym xml:lang="en">french ice cream</oboInOwl:hasSynonym>
	<oboInOwl:hasSynonym xml:lang="en">ice cream, french</oboInOwl:hasSynonym>
	<oboInOwl:hasDbXref>LANGUAL:A0165</oboInOwl:hasDbXref>
</owl:Class>

<owl:Class rdf:about="&obo;FOODON_03400166">
	<rdfs:label xml:lang="en">color additive (us cfr)</rdfs:label>
	<rdfs:subClassOf rdf:resource="&obo;FOODON_03400181"/>
	<obo:IAO_0000412>http://langual.org</obo:IAO_0000412>
	<obo:IAO_0000115 xml:lang="en">A substance added to food to impart, preserve, or enhance the color or shading of a food (21 CFR 170.3(0)).</obo:IAO_0000115>
	<obo:IAO_0000114 rdf:resource="&obo;IAO_0000428"/>
	<oboInOwl:hasDbXref>LANGUAL:A0166</oboInOwl:hasDbXref>
</owl:Class>

<owl:Class rdf:about="&obo;FOODON_03400167">
	<rdfs:label xml:lang="en">pizza crust (us cfr)</rdfs:label>
	<rdfs:subClassOf rdf:resource="&obo;FOODON_03400178"/>
	<obo:IAO_0000412>http://langual.org</obo:IAO_0000412>
	<obo:IAO_0000115 xml:lang="en">Yeast-leavened bread that is used as a base for filling, particularly to make pizza.</obo:IAO_0000115>
	<obo:IAO_0000114 rdf:resource="&obo;IAO_0000428"/>
	<oboInOwl:hasDbXref>LANGUAL:A0167</oboInOwl:hasDbXref>
</owl:Class>

<owl:Class rdf:about="&obo;FOODON_03400168">
	<rdfs:label xml:lang="en">cured cheese (us cfr)</rdfs:label>
	<rdfs:subClassOf rdf:resource="&obo;FOODON_03400187"/>
	<obo:IAO_0000412>http://langual.org</obo:IAO_0000412>
	<obo:IAO_0000115 xml:lang="en">Natural cheese that is cured; includes cheeses that are normally consumed cured but may be sold in an uncured or very lightly cured stage. The classification of cured cheeses is based on the method of curing, the moisture content, and the milk fat content measured as the proportion of solids. Scope notes given for the general classes give moisture and milkfat proportions that cover the entire range specified in the CFR for the individual cheeses included in a class; the class definition given in the CFR section cited may be more restrictive.</obo:IAO_0000115>
	<obo:IAO_0000114 rdf:resource="&obo;IAO_0000428"/>
	<oboInOwl:hasSynonym xml:lang="en">cheese, cured</oboInOwl:hasSynonym>
	<oboInOwl:hasDbXref>LANGUAL:A0168</oboInOwl:hasDbXref>
</owl:Class>

<owl:Class rdf:about="&obo;FOODON_03400169">
	<rdfs:label xml:lang="en">gelatin dessert (us cfr)</rdfs:label>
	<rdfs:subClassOf rdf:resource="&obo;FOODON_03400222"/>
	<obo:IAO_0000412>http://langual.org</obo:IAO_0000412>
	<obo:IAO_0000115 xml:lang="en">Sweetened product containing gelatin, flavoring and coloring.</obo:IAO_0000115>
	<obo:IAO_0000114 rdf:resource="&obo;IAO_0000428"/>
	<oboInOwl:hasDbXref>LANGUAL:A0169</oboInOwl:hasDbXref>
</owl:Class>

<owl:Class rdf:about="&obo;FOODON_03400172">
	<rdfs:label xml:lang="en">prepared food product (us cfr)</rdfs:label>
	<rdfs:subClassOf rdf:resource="&obo;FOODON_03401270"/>
	<obo:IAO_0000412>http://langual.org</obo:IAO_0000412>
	<obo:IAO_0000115 xml:lang="en">Food product that is 1) ready or nearly ready for consumption; 2) usually a composite of several foods or ingredients that often belong to distinct product types; 3) usually formulated, mixed and partially or fully cooked. Prepared foods often undergo several of the processes listed in *F. EXTENT OF HEAT TREATMENT* and *H. TREATMENT APPLIED*; these factors should be carefully considered in indexing. The classification of prepared food products emphasizes consumption characteristics. [FDA CFSAN 1995]</obo:IAO_0000115>
	<obo:IAO_0000114 rdf:resource="&obo;IAO_0000428"/>
	<oboInOwl:hasSynonym xml:lang="en">prepared dish</oboInOwl:hasSynonym>
	<oboInOwl:hasDbXref>LANGUAL:A0172</oboInOwl:hasDbXref>
</owl:Class>

<owl:Class rdf:about="&obo;FOODON_03400173">
	<rdfs:label xml:lang="en">caramel candy (us cfr)</rdfs:label>
	<rdfs:subClassOf rdf:resource="&obo;FOODON_03400293"/>
	<obo:IAO_0000412>http://langual.org</obo:IAO_0000412>
	<obo:IAO_0000115 xml:lang="en">Candy prepared by heating together sugar, corn syrup, fat and cream or milk to 240-250 degrees F.</obo:IAO_0000115>
	<obo:IAO_0000114 rdf:resource="&obo;IAO_0000428"/>
	<oboInOwl:hasSynonym xml:lang="en">candy, caramel</oboInOwl:hasSynonym>
	<oboInOwl:hasDbXref>LANGUAL:A0173</oboInOwl:hasDbXref>
</owl:Class>

<owl:Class rdf:about="&obo;FOODON_03400176">
	<rdfs:label xml:lang="en">chewing gum (us cfr)</rdfs:label>
	<rdfs:subClassOf rdf:resource="&obo;FOODON_03401270"/>
	<obo:IAO_0000412>http://langual.org</obo:IAO_0000412>
	<obo:IAO_0000115 xml:lang="en">An elastic substance flavored and used for chewing; it may be sweetened with a nutritive or nonnutritive sweetener. [FDA CFSAN 1995]</obo:IAO_0000115>
	<obo:IAO_0000114 rdf:resource="&obo;IAO_0000428"/>
	<oboInOwl:hasDbXref>LANGUAL:A0176</oboInOwl:hasDbXref>
</owl:Class>

<owl:Class rdf:about="&obo;FOODON_03400178">
	<rdfs:label xml:lang="en">bread (us cfr)</rdfs:label>
	<rdfs:subClassOf rdf:resource="&obo;FOODON_03400107"/>
	<obo:IAO_0000412>http://langual.org</obo:IAO_0000412>
	<obo:IAO_0000115 xml:lang="en">Unsweetened bakery product that may be unleavened or yeast-leavened and may be baked in various forms. Excludes pie crust.</obo:IAO_0000115>
	<obo:IAO_0000114 rdf:resource="&obo;IAO_0000428"/>
	<oboInOwl:hasSynonym xml:lang="en">bun, roll, or bread</oboInOwl:hasSynonym>
	<oboInOwl:hasSynonym xml:lang="en">roll, bun, or bread</oboInOwl:hasSynonym>
	<oboInOwl:hasDbXref>LANGUAL:A0178</oboInOwl:hasDbXref>
</owl:Class>

<owl:Class rdf:about="&obo;FOODON_03400179">
	<rdfs:label xml:lang="en">condiment or relish (us cfr)</rdfs:label>
	<rdfs:subClassOf rdf:resource="&obo;FOODON_03400105"/>
	<obo:IAO_0000412>http://langual.org</obo:IAO_0000412>
	<obo:IAO_0000115 xml:lang="en">Food product that is usually pungent, tart, salty, or spicy and is used to enhance the flavors of other foods; includes catsup, relish, prepared mustard, prepared horseradish, and condiment sauces.</obo:IAO_0000115>
	<obo:IAO_0000114 rdf:resource="&obo;IAO_0000428"/>
	<oboInOwl:hasSynonym xml:lang="en">relish or condiment</oboInOwl:hasSynonym>
	<oboInOwl:hasDbXref>LANGUAL:A0179</oboInOwl:hasDbXref>
</owl:Class>

<owl:Class rdf:about="&obo;FOODON_03400180">
	<rdfs:label xml:lang="en">soup, thick (us cfr)</rdfs:label>
	<rdfs:subClassOf rdf:resource="&obo;FOODON_03400198"/>
	<obo:IAO_0000412>http://langual.org</obo:IAO_0000412>
	<obo:IAO_0000115 xml:lang="en">A soup in which the liquid phase has high viscosity.</obo:IAO_0000115>
	<obo:IAO_0000114 rdf:resource="&obo;IAO_0000428"/>
	<oboInOwl:hasSynonym xml:lang="en">bisque</oboInOwl:hasSynonym>
	<oboInOwl:hasSynonym xml:lang="en">gumbo</oboInOwl:hasSynonym>
	<oboInOwl:hasSynonym xml:lang="en">soup, cream</oboInOwl:hasSynonym>
	<oboInOwl:hasDbXref>LANGUAL:A0180</oboInOwl:hasDbXref>
</owl:Class>

<owl:Class rdf:about="&obo;FOODON_03400181">
	<rdfs:label xml:lang="en">food additive (us cfr)</rdfs:label>
	<rdfs:subClassOf rdf:resource="&obo;FOODON_03401270"/>
	<obo:IAO_0000412>http://langual.org</obo:IAO_0000412>
	<obo:IAO_0000115 xml:lang="en">Substance that is added to food or that is used to treat food and that becomes a component of the food or otherwise affects the functional or nutritional characteristics of the food; for purposes of this vocabulary it excludes products that fall under other categories, such as flavors and sweeteners. [FDA CFSAN 1995]</obo:IAO_0000115>
	<obo:IAO_0000114 rdf:resource="&obo;IAO_0000428"/>
	<oboInOwl:hasDbXref>LANGUAL:A0181</oboInOwl:hasDbXref>
</owl:Class>

<owl:Class rdf:about="&obo;FOODON_03400182">
	<rdfs:label xml:lang="en">milk analog (us cfr)</rdfs:label>
	<rdfs:subClassOf rdf:resource="&obo;FOODON_03400147"/>
	<obo:IAO_0000412>http://langual.org</obo:IAO_0000412>
	<obo:IAO_0000115 xml:lang="en">Food product having functional characteristics similar to milk; it may be nutritionally equivalent or inferior to the product it purports to resemble.</obo:IAO_0000115>
	<obo:IAO_0000114 rdf:resource="&obo;IAO_0000428"/>
	<oboInOwl:hasSynonym xml:lang="en">imitation milk</oboInOwl:hasSynonym>
	<oboInOwl:hasDbXref>LANGUAL:A0182</oboInOwl:hasDbXref>
</owl:Class>

<owl:Class rdf:about="&obo;FOODON_03400183">
	<rdfs:label xml:lang="en">quick bread, sweetened (us cfr)</rdfs:label>
	<rdfs:subClassOf rdf:resource="&obo;FOODON_03400135"/>
	<obo:IAO_0000412>http://langual.org</obo:IAO_0000412>
	<obo:IAO_0000115 xml:lang="en">Chemically leavened sweetened bakery product that may contain other ingredients such as fruits, nuts or that may be filled.</obo:IAO_0000115>
	<obo:IAO_0000114 rdf:resource="&obo;IAO_0000428"/>
	<oboInOwl:hasSynonym xml:lang="en">fruit bread</oboInOwl:hasSynonym>
	<oboInOwl:hasSynonym xml:lang="en">nut bread</oboInOwl:hasSynonym>
	<oboInOwl:hasDbXref>LANGUAL:A0183</oboInOwl:hasDbXref>
</owl:Class>

<owl:Class rdf:about="&obo;FOODON_03400184">
	<rdfs:label xml:lang="en">fruit butter (us cfr)</rdfs:label>
	<rdfs:subClassOf rdf:resource="&obo;FOODON_03400155"/>
	<obo:IAO_0000412>http://langual.org</obo:IAO_0000412>
	<obo:IAO_0000115 xml:lang="en">Smooth semisolid fruit product prepared from a mixture of one or more fruit ingredients and specified optional ingredients. Skins, seeds, pits, and cores are screened out. Nutritive carbohydrate sweetener may be used, but the starting mixture of optional ingredients must contain at least five parts by weight of the fruit ingredient to each two parts by weight of the nutritive carbohydrate sweetener.  The soluble content of the finished fruit butter is not less than 43% solids (21 CFR 150.110).</obo:IAO_0000115>
	<obo:IAO_0000114 rdf:resource="&obo;IAO_0000428"/>
	<oboInOwl:hasDbXref>LANGUAL:A0184</oboInOwl:hasDbXref>
</owl:Class>

<owl:Class rdf:about="&obo;FOODON_03400185">
	<rdfs:label xml:lang="en">uncured cheese (us cfr)</rdfs:label>
	<rdfs:subClassOf rdf:resource="&obo;FOODON_03400187"/>
	<obo:IAO_0000412>http://langual.org</obo:IAO_0000412>
	<obo:IAO_0000115 xml:lang="en">Natural cheese that is not cured or is cured for less than 7 days. It may undergo some further processing, such as creaming. It is consumed fresh and has a mild acid flavor. Moisture max. 80%. Includes such products as cottage cheese, cream cheese and mozzarella cheese.</obo:IAO_0000115>
	<obo:IAO_0000114 rdf:resource="&obo;IAO_0000428"/>
	<oboInOwl:hasSynonym xml:lang="en">soft cheese</oboInOwl:hasSynonym>
	<oboInOwl:hasDbXref>LANGUAL:A0185</oboInOwl:hasDbXref>
</owl:Class>

<owl:Class rdf:about="&obo;FOODON_03400186">
	<rdfs:label xml:lang="en">hard cheese (us cfr)</rdfs:label>
	<rdfs:subClassOf rdf:resource="&obo;FOODON_03400316"/>
	<obo:IAO_0000412>http://langual.org</obo:IAO_0000412>
	<obo:IAO_0000115 xml:lang="en">Cured cheese ripened by bacteria.</obo:IAO_0000115>
	<obo:IAO_0000114 rdf:resource="&obo;IAO_0000428"/>
	<rdfs:comment xml:lang="en">LanguaL curation note: Used for cheeses, which contain not more than 39 percent of moisture, and their solids contain not less than 50 percent of milkfat [21 CFR Ch. I (4-1-99 Edition)]</rdfs:comment>
	<oboInOwl:hasDbXref>LANGUAL:A0186</oboInOwl:hasDbXref>
</owl:Class>

<owl:Class rdf:about="&obo;FOODON_03400187">
	<rdfs:label xml:lang="en">natural cheese (us cfr)</rdfs:label>
	<rdfs:subClassOf rdf:resource="&obo;FOODON_03400115"/>
	<obo:IAO_0000412>http://langual.org</obo:IAO_0000412>
	<obo:IAO_0000115 xml:lang="en">Cheese made from milk or milk components, such as cream, by the following process: (1) produce curd through coagulation of milk by bacterial action and/or enzymes and/or acidification and draining of whey. (2) For cured cheese only: cure the curd. Excludes products made through further processing, such as comminuting (see *CHEESE PRODUCT*).</obo:IAO_0000115>
	<obo:IAO_0000114 rdf:resource="&obo;IAO_0000428"/>
	<oboInOwl:hasDbXref>LANGUAL:A0187</oboInOwl:hasDbXref>
</owl:Class>

<owl:Class rdf:about="&obo;FOODON_03400188">
	<rdfs:label xml:lang="en">confectionery (us cfr)</rdfs:label>
	<rdfs:subClassOf rdf:resource="&obo;FOODON_03401270"/>
	<obo:IAO_0000412>http://langual.org</obo:IAO_0000412>
	<obo:IAO_0000115 xml:lang="en">Candy or other food product made with sweeteners and frequently containing nuts, fruits, starches, flavorings and other foods (21 CFR 170.3(n)(9). [FDA CFSAN 1995]</obo:IAO_0000115>
	<obo:IAO_0000114 rdf:resource="&obo;IAO_0000428"/>
	<oboInOwl:hasDbXref>LANGUAL:A0188</oboInOwl:hasDbXref>
</owl:Class>

<owl:Class rdf:about="&obo;FOODON_03400191">
	<rdfs:label xml:lang="en">bakery product (us cfr)</rdfs:label>
	<rdfs:subClassOf rdf:resource="&obo;FOODON_03400106"/>
	<obo:IAO_0000412>http://langual.org</obo:IAO_0000412>
	<obo:IAO_0000115 xml:lang="en">Prepared grain product made by baking or frying. Includes doughs, batters and mixes.</obo:IAO_0000115>
	<obo:IAO_0000114 rdf:resource="&obo;IAO_0000428"/>
	<oboInOwl:hasDbXref>LANGUAL:A0191</oboInOwl:hasDbXref>
</owl:Class>

<owl:Class rdf:about="&obo;FOODON_03400192">
	<rdfs:label xml:lang="en">pudding, starch (us cfr)</rdfs:label>
	<rdfs:subClassOf rdf:resource="&obo;FOODON_03400285"/>
	<obo:IAO_0000412>http://langual.org</obo:IAO_0000412>
	<obo:IAO_0000115 xml:lang="en">Cooked or uncooked mixture prepared with starch (tapioca starch, cornstarch, etc.) and other optional ingredients including sweeteners, eggs and flavorings.</obo:IAO_0000115>
	<obo:IAO_0000114 rdf:resource="&obo;IAO_0000428"/>
	<oboInOwl:hasSynonym xml:lang="en">starch pudding</oboInOwl:hasSynonym>
	<oboInOwl:hasDbXref>LANGUAL:A0192</oboInOwl:hasDbXref>
</owl:Class>

<owl:Class rdf:about="&obo;FOODON_03400194">
	<rdfs:label xml:lang="en">pancake or waffle (us cfr)</rdfs:label>
	<rdfs:subClassOf rdf:resource="&obo;FOODON_03400135"/>
	<obo:IAO_0000412>http://langual.org</obo:IAO_0000412>
	<obo:IAO_0000115 xml:lang="en">A thin, sweetened bakery product griddled or cooked in a heated mold.</obo:IAO_0000115>
	<obo:IAO_0000114 rdf:resource="&obo;IAO_0000428"/>
	<oboInOwl:hasSynonym xml:lang="en">waffle or pancake</oboInOwl:hasSynonym>
	<oboInOwl:hasDbXref>LANGUAL:A0194</oboInOwl:hasDbXref>
</owl:Class>

<owl:Class rdf:about="&obo;FOODON_03400195">
	<rdfs:label xml:lang="en">malt beverage (us cfr)</rdfs:label>
	<rdfs:subClassOf rdf:resource="&obo;FOODON_03400278"/>
	<obo:IAO_0000412>http://langual.org</obo:IAO_0000412>
	<obo:IAO_0000115 xml:lang="en">Alcoholic beverage prepared from water, malted grain and hops (humulus) by brewing. Examples are beer, ale and malt liquor (27 CFR 7.10).</obo:IAO_0000115>
	<obo:IAO_0000114 rdf:resource="&obo;IAO_0000428"/>
	<oboInOwl:hasDbXref>LANGUAL:A0195</oboInOwl:hasDbXref>
</owl:Class>

<owl:Class rdf:about="&obo;FOODON_03400196">
	<rdfs:label xml:lang="en">fruit nectar (us cfr)</rdfs:label>
	<rdfs:subClassOf rdf:resource="&obo;FOODON_03400104"/>
	<obo:IAO_0000412>http://langual.org</obo:IAO_0000412>
	<obo:IAO_0000115 xml:lang="en">Pulpy, liquid food prepared from fruit puree, pulp, juice or concentrates thereof, water, and optional ingredients. It contains finely divided insoluble fruit solids but not seeds, pits, or other coarse or hard substances. The proportion of fruit ingredient used on an equivalent single strength basis is not less than 40% by weight of the finished food. It may be sweetened (21 CFR 146.113).</obo:IAO_0000115>
	<obo:IAO_0000114 rdf:resource="&obo;IAO_0000428"/>
	<oboInOwl:hasDbXref>LANGUAL:A0196</oboInOwl:hasDbXref>
</owl:Class>

<owl:Class rdf:about="&obo;FOODON_03400197">
	<rdfs:label xml:lang="en">fruit spread or sauce (us cfr)</rdfs:label>
	<rdfs:subClassOf rdf:resource="&obo;FOODON_03400155"/>
	<obo:IAO_0000412>http://langual.org</obo:IAO_0000412>
	<obo:IAO_0000115 xml:lang="en">Nonstandardized fruit product prepared from a mixture of one or more fruit ingredients and optional ingredients including nutritive carbohydrate sweetener, spice or flavor; includes applesauce and cranberry sauce.</obo:IAO_0000115>
	<obo:IAO_0000114 rdf:resource="&obo;IAO_0000428"/>
	<oboInOwl:hasDbXref>LANGUAL:A0197</oboInOwl:hasDbXref>
</owl:Class>

<owl:Class rdf:about="&obo;FOODON_03400198">
	<rdfs:label xml:lang="en">soup (us cfr)</rdfs:label>
	<rdfs:subClassOf rdf:resource="&obo;FOODON_03400172"/>
	<obo:IAO_0000412>http://langual.org</obo:IAO_0000412>
	<obo:IAO_0000115 xml:lang="en">A liquid food made by simmering meat, poultry, seafood or vegetables, being clear or thickened to the consistency of a thin puree or having milk or cream added, and often containing pieces of solid food such as meat, shellfish, pasta or vegetables. Soup takes precedence over other food products.</obo:IAO_0000115>
	<obo:IAO_0000114 rdf:resource="&obo;IAO_0000428"/>
	<oboInOwl:hasDbXref>LANGUAL:A0198</oboInOwl:hasDbXref>
</owl:Class>

<owl:Class rdf:about="&obo;FOODON_03400200">
	<rdfs:label xml:lang="en">distinctive distilled spirits (us cfr)</rdfs:label>
	<rdfs:subClassOf rdf:resource="&obo;FOODON_03400277"/>
	<obo:IAO_0000412>http://langual.org</obo:IAO_0000412>
	<obo:IAO_0000115 xml:lang="en">Distilled spirits produced at less than 190 proof and having a distinctive flavor and aroma derived from the source (or from flavoring ingredients added) through a manufacturing process characteristic of the type. Includes whiskey, brandy, rum and similar products.</obo:IAO_0000115>
	<obo:IAO_0000114 rdf:resource="&obo;IAO_0000428"/>
	<oboInOwl:hasSynonym xml:lang="en">distilled spirits, distinctive</oboInOwl:hasSynonym>
	<oboInOwl:hasSynonym xml:lang="en">spirits, distinctive distilled</oboInOwl:hasSynonym>
	<oboInOwl:hasDbXref>LANGUAL:A0200</oboInOwl:hasDbXref>
</owl:Class>

<owl:Class rdf:about="&obo;FOODON_03400202">
	<rdfs:label xml:lang="en">pastry, sweetened (us cfr)</rdfs:label>
	<rdfs:subClassOf rdf:resource="&obo;FOODON_03400135"/>
	<obo:IAO_0000412>http://langual.org</obo:IAO_0000412>
	<obo:IAO_0000115 xml:lang="en">Sweetened bakery product consisting of a sweetened or unsweetened pastry shell or enclosure containing a sweetened filling, usually fruit, cheese or custard. Examples would be apple strudel, danish pastry or cream puff.</obo:IAO_0000115>
	<obo:IAO_0000114 rdf:resource="&obo;IAO_0000428"/>
	<oboInOwl:hasDbXref>LANGUAL:A0202</oboInOwl:hasDbXref>
</owl:Class>

<owl:Class rdf:about="&obo;FOODON_03400203">
	<rdfs:label xml:lang="en">cookie (us cfr)</rdfs:label>
	<rdfs:subClassOf rdf:resource="&obo;FOODON_03400135"/>
	<obo:IAO_0000412>http://langual.org</obo:IAO_0000412>
	<obo:IAO_0000115 xml:lang="en">Sweetened bakery product baked in individual portions that are usually small and flat.</obo:IAO_0000115>
	<obo:IAO_0000114 rdf:resource="&obo;IAO_0000428"/>
	<oboInOwl:hasDbXref>LANGUAL:A0203</oboInOwl:hasDbXref>
</owl:Class>

<owl:Class rdf:about="&obo;FOODON_03400204">
	<rdfs:label xml:lang="en">candy (us cfr)</rdfs:label>
	<rdfs:subClassOf rdf:resource="&obo;FOODON_03400188"/>
	<obo:IAO_0000412>http://langual.org</obo:IAO_0000412>
	<obo:IAO_0000115 xml:lang="en">Food product prepared by heating a mixture of sweeteners and other optional ingredients according to the specific formula for each subgroup.</obo:IAO_0000115>
	<obo:IAO_0000114 rdf:resource="&obo;IAO_0000428"/>
	<oboInOwl:hasDbXref>LANGUAL:A0204</oboInOwl:hasDbXref>
</owl:Class>

<owl:Class rdf:about="&obo;FOODON_03400205">
	<rdfs:label xml:lang="en">wine, 7-24% alcohol (us cfr)</rdfs:label>
	<rdfs:subClassOf rdf:resource="&obo;FOODON_03400297"/>
	<obo:IAO_0000412>http://langual.org</obo:IAO_0000412>
	<obo:IAO_0000115 xml:lang="en">Alcoholic beverage produced by the normal fermentation of the juice of grapes or other fruits or of the fermentable parts of plants or plant-related products; may contain certain optional ingredients. Contains between 7-24% alcohol by volume (27 CFR 4.10).</obo:IAO_0000115>
	<obo:IAO_0000114 rdf:resource="&obo;IAO_0000428"/>
	<oboInOwl:hasDbXref>LANGUAL:A0205</oboInOwl:hasDbXref>
</owl:Class>

<owl:Class rdf:about="&obo;FOODON_03400206">
	<rdfs:label xml:lang="en">frozen nondairy dessert (us cfr)</rdfs:label>
	<rdfs:subClassOf rdf:resource="&obo;FOODON_03400222"/>
	<obo:IAO_0000412>http://langual.org</obo:IAO_0000412>
	<obo:IAO_0000115 xml:lang="en">Frozen dessert prepared from nondairy ingredients.</obo:IAO_0000115>
	<obo:IAO_0000114 rdf:resource="&obo;IAO_0000428"/>
	<oboInOwl:hasSynonym xml:lang="en">dessert, frozen nondairy</oboInOwl:hasSynonym>
	<oboInOwl:hasSynonym xml:lang="en">nondairy dessert, frozen</oboInOwl:hasSynonym>
	<oboInOwl:hasDbXref>LANGUAL:A0206</oboInOwl:hasDbXref>
</owl:Class>

<owl:Class rdf:about="&obo;FOODON_03400208">
	<rdfs:label xml:lang="en">salad (us cfr)</rdfs:label>
	<rdfs:subClassOf rdf:resource="&obo;FOODON_03400172"/>
	<obo:IAO_0000412>http://langual.org</obo:IAO_0000412>
	<obo:IAO_0000115 xml:lang="en">A combination of one or more vegetable, fruit, herb, meat, poultry, seafood, egg, cereal or pasta, usually served with some kind of moist dressing; may be molded with a jelling agent. Salad takes precedence over other product types. Examples are egg salad, tuna salad, mixed vegetable salad, jelled fruit salad and macaroni salad.</obo:IAO_0000115>
	<obo:IAO_0000114 rdf:resource="&obo;IAO_0000428"/>
	<oboInOwl:hasDbXref>LANGUAL:A0208</oboInOwl:hasDbXref>
</owl:Class>

<owl:Class rdf:about="&obo;FOODON_03400209">
	<rdfs:label xml:lang="en">fruit jelly (us cfr)</rdfs:label>
	<rdfs:subClassOf rdf:resource="&obo;FOODON_03400155"/>
	<obo:IAO_0000412>http://langual.org</obo:IAO_0000412>
	<obo:IAO_0000115 xml:lang="en">Jelled product made from one or more fruit juices and optional ingredients. Includes both fruit jelly, which may be sweetened with nutritive carbohydrate sweeteners, (21 CFR 150.140), and artificially sweetened fruit jelly (21 CFR 150.141). The finished fruit jelly must have a soluble solid content of no less than 65% and the ratio by weight of the fruit ingredient to sweetener in the starting mixture must be no less than 45:55. Artificially sweetened fruit jelly must contain no less than 55% fruit ingredient by weight.</obo:IAO_0000115>
	<obo:IAO_0000114 rdf:resource="&obo;IAO_0000428"/>
	<oboInOwl:hasDbXref>LANGUAL:A0209</oboInOwl:hasDbXref>
</owl:Class>

<owl:Class rdf:about="&obo;FOODON_03400210">
	<rdfs:label xml:lang="en">cake (us cfr)</rdfs:label>
	<rdfs:subClassOf rdf:resource="&obo;FOODON_03400135"/>
	<obo:IAO_0000412>http://langual.org</obo:IAO_0000412>
	<obo:IAO_0000115 xml:lang="en">Sweetened bakery product that is leavened and baked.</obo:IAO_0000115>
	<obo:IAO_0000114 rdf:resource="&obo;IAO_0000428"/>
	<oboInOwl:hasDbXref>LANGUAL:A0210</oboInOwl:hasDbXref>
</owl:Class>

<owl:Class rdf:about="&obo;FOODON_03400211">
	<rdfs:label xml:lang="en">frozen yogurt (us cfr)</rdfs:label>
	<rdfs:subClassOf rdf:resource="&obo;FOODON_03400114"/>
	<obo:IAO_0000412>http://langual.org</obo:IAO_0000412>
	<obo:IAO_0000115 xml:lang="en">A frozen dessert prepared from yogurt and other ingredients.</obo:IAO_0000115>
	<obo:IAO_0000114 rdf:resource="&obo;IAO_0000428"/>
	<oboInOwl:hasSynonym xml:lang="en">yogurt, frozen</oboInOwl:hasSynonym>
	<oboInOwl:hasDbXref>LANGUAL:A0211</oboInOwl:hasDbXref>
</owl:Class>

<owl:Class rdf:about="&obo;FOODON_03400212">
	<rdfs:label xml:lang="en">stew or hash (us cfr)</rdfs:label>
	<rdfs:subClassOf rdf:resource="&obo;FOODON_03400172"/>
	<obo:IAO_0000412>http://langual.org</obo:IAO_0000412>
	<obo:IAO_0000115 xml:lang="en">Prepared dish consisting of a mixture of meat, poultry or seafood with one or more vegetables and possibly other ingredients. In contrast to soups, which are liquid or semiliquid, stews are thickened or have a larger proportion of solid ingredients.</obo:IAO_0000115>
	<obo:IAO_0000114 rdf:resource="&obo;IAO_0000428"/>
	<oboInOwl:hasSynonym xml:lang="en">hash or stew</oboInOwl:hasSynonym>
	<oboInOwl:hasDbXref>LANGUAL:A0212</oboInOwl:hasDbXref>
</owl:Class>

<owl:Class rdf:about="&obo;FOODON_03400213">
	<rdfs:label xml:lang="en">fudge (us cfr)</rdfs:label>
	<rdfs:subClassOf rdf:resource="&obo;FOODON_03400293"/>
	<obo:IAO_0000412>http://langual.org</obo:IAO_0000412>
	<obo:IAO_0000115 xml:lang="en">Soft candy prepared by boiling milk, sugar, salt and optional ingredients to the soft-ball stage (238 degrees F.).</obo:IAO_0000115>
	<obo:IAO_0000114 rdf:resource="&obo;IAO_0000428"/>
	<oboInOwl:hasDbXref>LANGUAL:A0213</oboInOwl:hasDbXref>
</owl:Class>

<owl:Class rdf:about="&obo;FOODON_03400214">
	<rdfs:label xml:lang="en">glaze (us cfr)</rdfs:label>
	<rdfs:subClassOf rdf:resource="&obo;FOODON_03401270"/>
	<obo:IAO_0000412>http://langual.org</obo:IAO_0000412>
	<obo:IAO_0000115 xml:lang="en">An edible coating used to enhance appearance and palatibility and to protect the food product. [FDA CFSAN 1995]</obo:IAO_0000115>
	<obo:IAO_0000114 rdf:resource="&obo;IAO_0000428"/>
	<oboInOwl:hasDbXref>LANGUAL:A0214</oboInOwl:hasDbXref>
</owl:Class>

<owl:Class rdf:about="&obo;FOODON_03400215">
	<rdfs:label xml:lang="en">flavoring (us cfr)</rdfs:label>
	<rdfs:subClassOf rdf:resource="&obo;FOODON_03400300"/>
	<obo:IAO_0000412>http://langual.org</obo:IAO_0000412>
	<obo:IAO_0000115 xml:lang="en">Natural or synthetic product, dissolved in a suitable solvent or carried on an appropriate dry base and added to a food product to enhance or impart taste and aroma.</obo:IAO_0000115>
	<obo:IAO_0000114 rdf:resource="&obo;IAO_0000428"/>
	<oboInOwl:hasSynonym xml:lang="en">aroma</oboInOwl:hasSynonym>
	<oboInOwl:hasDbXref>LANGUAL:A0215</oboInOwl:hasDbXref>
</owl:Class>

<owl:Class rdf:about="&obo;FOODON_03400216">
	<rdfs:label xml:lang="en">hard candy (us cfr)</rdfs:label>
	<rdfs:subClassOf rdf:resource="&obo;FOODON_03400204"/>
	<obo:IAO_0000412>http://langual.org</obo:IAO_0000412>
	<obo:IAO_0000115 xml:lang="en">Candy prepared by boiling a mixture of water, sugars, butter or margarine and optional ingredients to the hard-crack stage (300 degrees F.).</obo:IAO_0000115>
	<obo:IAO_0000114 rdf:resource="&obo;IAO_0000428"/>
	<oboInOwl:hasDbXref>LANGUAL:A0216</oboInOwl:hasDbXref>
</owl:Class>

<owl:Class rdf:about="&obo;FOODON_03400217">
	<rdfs:label xml:lang="en">meat, poultry, seafood or related product (us cfr)</rdfs:label>
	<rdfs:subClassOf rdf:resource="&obo;FOODON_03401270"/>
	<obo:IAO_0000412>http://langual.org</obo:IAO_0000412>
	<obo:IAO_0000115 xml:lang="en">Products of the flesh of animals. [FDA CFSAN 1995]</obo:IAO_0000115>
	<obo:IAO_0000114 rdf:resource="&obo;IAO_0000428"/>
	<oboInOwl:hasDbXref>LANGUAL:A0217</oboInOwl:hasDbXref>
</owl:Class>

<owl:Class rdf:about="&obo;FOODON_03400218">
	<rdfs:label xml:lang="en">sandwich (us cfr)</rdfs:label>
	<rdfs:subClassOf rdf:resource="&obo;FOODON_03400102"/>
	<obo:IAO_0000412>http://langual.org</obo:IAO_0000412>
	<obo:IAO_0000114 rdf:resource="&obo;IAO_0000428"/>
	<rdfs:comment xml:lang="en">LanguaL curation note: Sandwich takes precedent over other product types. Examples: peanut butter and jelly sandwich, tuna sandwich, egg salad sandwich or hamburger on roll. The filling of a sandwich is always indexed as the food source, even if the bread is the same weight or outweighs the filling ingredient(s). The bread would be indexed by *GRAIN ADDED* or the appropriate narrower term.</rdfs:comment>
	<oboInOwl:hasDbXref>LANGUAL:A0218</oboInOwl:hasDbXref>
</owl:Class>

<owl:Class rdf:about="&obo;FOODON_03400219">
	<rdfs:label xml:lang="en">custard, cooked (us cfr)</rdfs:label>
	<rdfs:subClassOf rdf:resource="&obo;FOODON_03400285"/>
	<obo:IAO_0000412>http://langual.org</obo:IAO_0000412>
	<obo:IAO_0000115 xml:lang="en">Cooked or baked mixture of milk, eggs and optional ingredients including nutritive and non-nutritive sweeteners.</obo:IAO_0000115>
	<obo:IAO_0000114 rdf:resource="&obo;IAO_0000428"/>
	<oboInOwl:hasSynonym xml:lang="en">cooked custard</oboInOwl:hasSynonym>
	<oboInOwl:hasDbXref>LANGUAL:A0219</oboInOwl:hasDbXref>
</owl:Class>

<owl:Class rdf:about="&obo;FOODON_03400220">
	<rdfs:label xml:lang="en">pasta dish (us cfr)</rdfs:label>
	<rdfs:subClassOf rdf:resource="&obo;FOODON_03400172"/>
	<obo:IAO_0000412>http://langual.org</obo:IAO_0000412>
	<obo:IAO_0000115 xml:lang="en">Prepared food product in which pasta in its cooked form is the first or second ingredient. Examples are spaghetti with meat balls, macaroni and cheese, beef stroganoff with noodles, etc. Excludes *SOUP* and *SALAD*.</obo:IAO_0000115>
	<obo:IAO_0000114 rdf:resource="&obo;IAO_0000428"/>
	<oboInOwl:hasDbXref>LANGUAL:A0220</oboInOwl:hasDbXref>
</owl:Class>

<owl:Class rdf:about="&obo;FOODON_03400221">
	<rdfs:label xml:lang="en">sausage or luncheon meat (us cfr)</rdfs:label>
	<rdfs:subClassOf rdf:resource="&obo;FOODON_03400150"/>
	<obo:IAO_0000412>http://langual.org</obo:IAO_0000412>
	<obo:IAO_0000115 xml:lang="en">This category includes a wide variety of products made from comminuted or chopped meat (skeletal and/or organ meat) that is usually salted and/or seasoned and often stuffed in an edible or inedible casing. Includes products such as pork sausage, pickle or pimiento loaf, meat spread and pate, and products made by binding meat chunks with gelatin or other binders, such as sectioned and formed ham, beef rolls, and headcheese. Excludes plain ground meat, meat loaf and products made by slicing intact muscle or other tissue, even if packaged and marketed like luncheon meat. Index all processes applied to the product at hand; examples: *FULLY HEAT TREATED*, *CURED FOR 2 MONTHS*, *SMOKED*, *FERMENTED*, *EMULSIFIED OR HOMOGENIZED*. Also consider *PARTICLE SIZE IN SOLID FORMED PRODUCTS* and *TYPEOF SAUSAGE CASING* in *Z. ADJUNCT CHARACTERISTICS OF FOOD*.</obo:IAO_0000115>
	<obo:IAO_0000114 rdf:resource="&obo;IAO_0000428"/>
	<oboInOwl:hasSynonym xml:lang="en">luncheon meat</oboInOwl:hasSynonym>
	<oboInOwl:hasDbXref>LANGUAL:A0221</oboInOwl:hasDbXref>
</owl:Class>

<owl:Class rdf:about="&obo;FOODON_03400222">
	<rdfs:label xml:lang="en">dessert (us cfr)</rdfs:label>
	<rdfs:subClassOf rdf:resource="&obo;FOODON_03400172"/>
	<obo:IAO_0000412>http://langual.org</obo:IAO_0000412>
	<obo:IAO_0000115 xml:lang="en">Sweetened prepared product usually consumed after the main course in a meal. Excludes fruit or fruit products, bakery products and confectionery.</obo:IAO_0000115>
	<obo:IAO_0000114 rdf:resource="&obo;IAO_0000428"/>
	<oboInOwl:hasDbXref>LANGUAL:A0222</oboInOwl:hasDbXref>
</owl:Class>

<owl:Class rdf:about="&obo;FOODON_03400224">
	<rdfs:label xml:lang="en">heavy wine, 14-24% alcohol (us cfr)</rdfs:label>
	<rdfs:subClassOf rdf:resource="&obo;FOODON_03400205"/>
	<obo:IAO_0000412>http://langual.org</obo:IAO_0000412>
	<obo:IAO_0000115 xml:lang="en">Wine containing 14-24% alcohol.</obo:IAO_0000115>
	<obo:IAO_0000114 rdf:resource="&obo;IAO_0000428"/>
	<oboInOwl:hasSynonym xml:lang="en">aperitif wine (u.s.)</oboInOwl:hasSynonym>
	<oboInOwl:hasSynonym xml:lang="en">dessert wine (u.s.)</oboInOwl:hasSynonym>
	<oboInOwl:hasDbXref>LANGUAL:A0224</oboInOwl:hasDbXref>
</owl:Class>

<owl:Class rdf:about="&obo;FOODON_03400225">
	<rdfs:label xml:lang="en">relish (us cfr)</rdfs:label>
	<rdfs:subClassOf rdf:resource="&obo;FOODON_03400179"/>
	<obo:IAO_0000412>http://langual.org</obo:IAO_0000412>
	<obo:IAO_0000115 xml:lang="en">Mixture of fruits, vegetables, or other ingredients, such as spices and sweeteners, used to enhance the flavor of other food products.</obo:IAO_0000115>
	<obo:IAO_0000114 rdf:resource="&obo;IAO_0000428"/>
	<oboInOwl:hasDbXref>LANGUAL:A0225</oboInOwl:hasDbXref>
</owl:Class>

<owl:Class rdf:about="&obo;FOODON_03400226">
	<rdfs:label xml:lang="en">brittle (us cfr)</rdfs:label>
	<rdfs:subClassOf rdf:resource="&obo;FOODON_03400216"/>
	<obo:IAO_0000412>http://langual.org</obo:IAO_0000412>
	<obo:IAO_0000115 xml:lang="en">Flat hard candy to which is added nuts, usually peanuts.</obo:IAO_0000115>
	<obo:IAO_0000114 rdf:resource="&obo;IAO_0000428"/>
	<oboInOwl:hasSynonym xml:lang="en">candy, brittle</oboInOwl:hasSynonym>
	<oboInOwl:hasDbXref>LANGUAL:A0226</oboInOwl:hasDbXref>
</owl:Class>

<owl:Class rdf:about="&obo;FOODON_03400227">
	<rdfs:label xml:lang="en">ice cream (us cfr)</rdfs:label>
	<rdfs:subClassOf rdf:resource="&obo;FOODON_03400137"/>
	<obo:IAO_0000412>http://langual.org</obo:IAO_0000412>
	<obo:IAO_0000115 xml:lang="en">Ice cream, in comparison with frozen custard, contains less than 1.4% egg yolk solids by weight of the finished product (21 CFR 135.110(a)).</obo:IAO_0000115>
	<obo:IAO_0000114 rdf:resource="&obo;IAO_0000428"/>
	<oboInOwl:hasDbXref>LANGUAL:A0227</oboInOwl:hasDbXref>
</owl:Class>

<owl:Class rdf:about="&obo;FOODON_03400228">
	<rdfs:label xml:lang="en">snack food (us cfr)</rdfs:label>
	<rdfs:subClassOf rdf:resource="&obo;FOODON_03401270"/>
	<obo:IAO_0000412>http://langual.org</obo:IAO_0000412>
	<obo:IAO_0000115 xml:lang="en">Unsweetened food product marketed for consumption between meals; excludes nuts, edible seeds, and sweetened products such as cakes, puddings and candies. [FDA CFSAN 1995]</obo:IAO_0000115>
	<obo:IAO_0000114 rdf:resource="&obo;IAO_0000428"/>
	<oboInOwl:hasDbXref>LANGUAL:A0228</oboInOwl:hasDbXref>
</owl:Class>

<owl:Class rdf:about="&obo;FOODON_03400229">
	<rdfs:label xml:lang="en">beverage (us cfr)</rdfs:label>
	<rdfs:subClassOf rdf:resource="&obo;FOODON_03401270"/>
	<obo:IAO_0000412>http://langual.org</obo:IAO_0000412>
	<obo:IAO_0000115 xml:lang="en">Alcoholic or nonalcoholic beverage; excludes milk and milk-based beverages, fruit juices and fruit juice drinks, and vegetable juices. [FDA CFSAN 1995]</obo:IAO_0000115>
	<obo:IAO_0000114 rdf:resource="&obo;IAO_0000428"/>
	<oboInOwl:hasDbXref>LANGUAL:A0229</oboInOwl:hasDbXref>
</owl:Class>

<owl:Class rdf:about="&obo;FOODON_03400230">
	<rdfs:label xml:lang="en">water ice (us cfr)</rdfs:label>
	<rdfs:subClassOf rdf:resource="&obo;FOODON_03400206"/>
	<obo:IAO_0000412>http://langual.org</obo:IAO_0000412>
	<obo:IAO_0000115 xml:lang="en">Frozen non-dairy dessert prepared by freezing, while stirring, a mixture of water, nutritive sweeteners and flavorings; the mix may or may not be pasteurized. Must not contain milk or milk-derived ingredients, egg yolk or food fats. The optional flavor ingredients are specified in 21 CFR 135.140(d) and (e).</obo:IAO_0000115>
	<obo:IAO_0000114 rdf:resource="&obo;IAO_0000428"/>
	<oboInOwl:hasDbXref>LANGUAL:A0230</oboInOwl:hasDbXref>
</owl:Class>

<owl:Class rdf:about="&obo;FOODON_03400231">
	<rdfs:label xml:lang="en">margarine (us cfr)</rdfs:label>
	<rdfs:subClassOf rdf:resource="&obo;FOODON_03400294"/>
	<obo:IAO_0000412>http://langual.org</obo:IAO_0000412>
	<obo:IAO_0000115 xml:lang="en">Food product having functional characteristics similar to those of butter; it is in plastic form or liquid emulsion and contains not less than 80% fat whose origin is vegetable or rendered animal carcass fats or a mixture of these as well as other optional ingredients specified by 21 CFR 166.110.</obo:IAO_0000115>
	<obo:IAO_0000114 rdf:resource="&obo;IAO_0000428"/>
	<oboInOwl:hasDbXref>LANGUAL:A0231</oboInOwl:hasDbXref>
</owl:Class>

<owl:Class rdf:about="&obo;FOODON_03400232">
	<rdfs:label xml:lang="en">mellorine (us cfr)</rdfs:label>
	<rdfs:subClassOf rdf:resource="&obo;FOODON_03400159"/>
	<obo:IAO_0000412>http://langual.org</obo:IAO_0000412>
	<obo:IAO_0000115 xml:lang="en">Frozen dairy dessert produced by freezing while stirring a pasteurized mix of ingredients including, but not limited to, milk derived nonfat solids, animal or vegetable fat or both, only part of which may be milkfat, and nutritive carbohydrate sweeteners.</obo:IAO_0000115>
	<obo:IAO_0000114 rdf:resource="&obo;IAO_0000428"/>
	<oboInOwl:hasDbXref>LANGUAL:A0232</oboInOwl:hasDbXref>
</owl:Class>

<owl:Class rdf:about="&obo;FOODON_03400233">
	<rdfs:label xml:lang="en">ice milk (us cfr)</rdfs:label>
	<rdfs:subClassOf rdf:resource="&obo;FOODON_03400114"/>
	<obo:IAO_0000412>http://langual.org</obo:IAO_0000412>
	<obo:IAO_0000115 xml:lang="en">Frozen dairy dessert similar to ice cream; it has between 2% and 7% milkfat and at least 11% total milk solids.</obo:IAO_0000115>
	<obo:IAO_0000114 rdf:resource="&obo;IAO_0000428"/>
	<oboInOwl:hasDbXref>LANGUAL:A0233</oboInOwl:hasDbXref>
</owl:Class>

<owl:Class rdf:about="&obo;FOODON_03400237">
	<rdfs:label xml:lang="en">sweetener (us cfr)</rdfs:label>
	<rdfs:subClassOf rdf:resource="&obo;FOODON_03400133"/>
	<obo:IAO_0000412>http://langual.org</obo:IAO_0000412>
	<obo:IAO_0000115 xml:lang="en">A product added to a food item to achieve some degree of sweet taste; it may be nutritive or nonnutritive.</obo:IAO_0000115>
	<obo:IAO_0000114 rdf:resource="&obo;IAO_0000428"/>
	<oboInOwl:hasDbXref>LANGUAL:A0237</oboInOwl:hasDbXref>
</owl:Class>

<owl:Class rdf:about="&obo;FOODON_03400240">
	<rdfs:label xml:lang="en">liqueur (us cfr)</rdfs:label>
	<rdfs:subClassOf rdf:resource="&obo;FOODON_03400200"/>
	<obo:IAO_0000412>http://langual.org</obo:IAO_0000412>
	<obo:IAO_0000115 xml:lang="en">Alcoholic beverage produced by combining a spirit (frequently brandy) with flavoring and sugar. May be grouped into five categories: fruits, seeds, herbs, peels and cremes. Examples of each include cherry heering, anisette, chartreuse, curacao and creme de menthe (27 CFR 5.22(h)).</obo:IAO_0000115>
	<obo:IAO_0000114 rdf:resource="&obo;IAO_0000428"/>
	<oboInOwl:hasSynonym xml:lang="en">cordial</oboInOwl:hasSynonym>
	<oboInOwl:hasDbXref>LANGUAL:A0240</oboInOwl:hasDbXref>
</owl:Class>

<owl:Class rdf:about="&obo;FOODON_03400241">
	<rdfs:label xml:lang="en">soft drink (us cfr)</rdfs:label>
	<rdfs:subClassOf rdf:resource="&obo;FOODON_03400112"/>
	<obo:IAO_0000412>http://langual.org</obo:IAO_0000412>
	<obo:IAO_0000115 xml:lang="en">Nonalcoholic beverage made from potable water by adding one or more of the following: carbon dioxide, flavoring ingredients or sweeteners. Naturally or artificially carbonated mineral waters are also considered soft drinks. Excludes products containing 15% or more fruit juice, which are indexed by the appropriate narrower term under *FRUIT JUICE OR RELATED PRODUCT*. Includes beverage bases to make soft drinks. Carbonated fruit juices are indexed by *FRUIT JUICE* or *FRUIT JUICE, DILUTED* and *CARBONATED* or the appropriate narrower term.</obo:IAO_0000115>
	<obo:IAO_0000114 rdf:resource="&obo;IAO_0000428"/>
	<oboInOwl:hasDbXref>LANGUAL:A0241</oboInOwl:hasDbXref>
</owl:Class>

<owl:Class rdf:about="&obo;FOODON_03400242">
	<rdfs:label xml:lang="en">cracker (us cfr)</rdfs:label>
	<rdfs:subClassOf rdf:resource="&obo;FOODON_03400107"/>
	<obo:IAO_0000412>http://langual.org</obo:IAO_0000412>
	<obo:IAO_0000115 xml:lang="en">Unsweetened bakery product baked in individual portions that are usually thin and crisp and may or may not be fat coated.</obo:IAO_0000115>
	<obo:IAO_0000114 rdf:resource="&obo;IAO_0000428"/>
	<oboInOwl:hasDbXref>LANGUAL:A0242</oboInOwl:hasDbXref>
</owl:Class>

<owl:Class rdf:about="&obo;FOODON_03400243">
	<rdfs:label xml:lang="en">soup, thin (us cfr)</rdfs:label>
	<rdfs:subClassOf rdf:resource="&obo;FOODON_03400198"/>
	<obo:IAO_0000412>http://langual.org</obo:IAO_0000412>
	<obo:IAO_0000115 xml:lang="en">A soup in which the liquid phase has low viscosity.</obo:IAO_0000115>
	<obo:IAO_0000114 rdf:resource="&obo;IAO_0000428"/>
	<oboInOwl:hasSynonym xml:lang="en">bouillon</oboInOwl:hasSynonym>
	<oboInOwl:hasSynonym xml:lang="en">consomme</oboInOwl:hasSynonym>
	<oboInOwl:hasDbXref>LANGUAL:A0243</oboInOwl:hasDbXref>
</owl:Class>

<owl:Class rdf:about="&obo;FOODON_03400244">
	<rdfs:label xml:lang="en">fondant (us cfr)</rdfs:label>
	<rdfs:subClassOf rdf:resource="&obo;FOODON_03400293"/>
	<obo:IAO_0000412>http://langual.org</obo:IAO_0000412>
	<obo:IAO_0000115 xml:lang="en">Candy prepared by cooking together sugar, water and ingredients to control crystal growth to a temperature of 238-246 degrees F. The product is then cooled approximately 100 degrees and agitated to promote a smooth, creamy texture.</obo:IAO_0000115>
	<obo:IAO_0000114 rdf:resource="&obo;IAO_0000428"/>
	<oboInOwl:hasSynonym xml:lang="en">candy, fondant</oboInOwl:hasSynonym>
	<oboInOwl:hasDbXref>LANGUAL:A0244</oboInOwl:hasDbXref>
</owl:Class>

<owl:Class rdf:about="&obo;FOODON_03400245">
	<rdfs:label xml:lang="en">sherbet (us cfr)</rdfs:label>
	<rdfs:subClassOf rdf:resource="&obo;FOODON_03400114"/>
	<obo:IAO_0000412>http://langual.org</obo:IAO_0000412>
	<obo:IAO_0000115 xml:lang="en">Frozen dairy dessert prepared by freezing, while stirring, a pasteurized mixture of one or more optional dairy ingredients, caseinates and other non-dairy ingredients, excluding other food fats; the milkfat content is not less than 1% nor more than 2%.</obo:IAO_0000115>
	<obo:IAO_0000114 rdf:resource="&obo;IAO_0000428"/>
	<oboInOwl:hasDbXref>LANGUAL:A0245</oboInOwl:hasDbXref>
</owl:Class>

<owl:Class rdf:about="&obo;FOODON_03400246">
	<rdfs:label xml:lang="en">decoration (us cfr)</rdfs:label>
	<rdfs:subClassOf rdf:resource="&obo;FOODON_03400188"/>
	<obo:IAO_0000412>http://langual.org</obo:IAO_0000412>
	<obo:IAO_0000115 xml:lang="en">Candy-like product shaped and/or colored to serve as a decoration.</obo:IAO_0000115>
	<obo:IAO_0000114 rdf:resource="&obo;IAO_0000428"/>
	<oboInOwl:hasDbXref>LANGUAL:A0246</oboInOwl:hasDbXref>
</owl:Class>

<owl:Class rdf:about="&obo;FOODON_03400248">
	<rdfs:label xml:lang="en">doughnut (us cfr)</rdfs:label>
	<rdfs:subClassOf rdf:resource="&obo;FOODON_03400135"/>
	<obo:IAO_0000412>http://langual.org</obo:IAO_0000412>
	<obo:IAO_0000115 xml:lang="en">Deep-fat fried sweetened bakery product that may be leavened with yeast or baking powder.</obo:IAO_0000115>
	<obo:IAO_0000114 rdf:resource="&obo;IAO_0000428"/>
	<oboInOwl:hasSynonym xml:lang="en">cruller</oboInOwl:hasSynonym>
	<oboInOwl:hasDbXref>LANGUAL:A0248</oboInOwl:hasDbXref>
</owl:Class>

<owl:Class rdf:about="&obo;FOODON_03400251">
	<rdfs:label xml:lang="en">fruit preserve or jam (us cfr)</rdfs:label>
	<rdfs:subClassOf rdf:resource="&obo;FOODON_03400155"/>
	<obo:IAO_0000412>http://langual.org</obo:IAO_0000412>
	<obo:IAO_0000115 xml:lang="en">Viscous or semisolid fruit product made from whole fruits or pieces of fruit of one or more varieties and optional ingredients.  Includes fruit preserve or jam (21 CFR 150.160) and artificially sweetened fruit preserve or jam (21 CFR 150.161).  The specifications of starting mixture and finished soluble solids are the same as for fruit jelly.</obo:IAO_0000115>
	<obo:IAO_0000114 rdf:resource="&obo;IAO_0000428"/>
	<oboInOwl:hasSynonym xml:lang="en">jam or fruit preserve</oboInOwl:hasSynonym>
	<oboInOwl:hasSynonym xml:lang="en">marmalade</oboInOwl:hasSynonym>
	<oboInOwl:hasDbXref>LANGUAL:A0251</oboInOwl:hasDbXref>
</owl:Class>

<owl:Class rdf:about="&obo;FOODON_03400253">
	<rdfs:label xml:lang="en">pie, sweetened (us cfr)</rdfs:label>
	<rdfs:subClassOf rdf:resource="&obo;FOODON_03400135"/>
	<obo:IAO_0000412>http://langual.org</obo:IAO_0000412>
	<obo:IAO_0000115 xml:lang="en">Sweetened bakery product consisting of a sweetened or unsweetened pie crust and a sweetened filling. The filling is always indexed as the food source, even if the crust is the same weight or greater weight than the filling ingredient.</obo:IAO_0000115>
	<obo:IAO_0000114 rdf:resource="&obo;IAO_0000428"/>
	<oboInOwl:hasSynonym xml:lang="en">tart</oboInOwl:hasSynonym>
	<oboInOwl:hasSynonym xml:lang="en">turnover, sweetened</oboInOwl:hasSynonym>
	<oboInOwl:hasDbXref>LANGUAL:A0253</oboInOwl:hasDbXref>
</owl:Class>

<owl:Class rdf:about="&obo;FOODON_03400254">
	<rdfs:label xml:lang="en">egg product analog (us cfr)</rdfs:label>
	<rdfs:subClassOf rdf:resource="&obo;FOODON_03400261"/>
	<obo:IAO_0000412>http://langual.org</obo:IAO_0000412>
	<obo:IAO_0000115 xml:lang="en">Food product having functional characteristics similar to an egg product; it may be nutritionally equivalent or inferior to the product it purports to resemble. Includes egg whites that have added ingredients, particularly vegetable oil.</obo:IAO_0000115>
	<obo:IAO_0000114 rdf:resource="&obo;IAO_0000428"/>
	<oboInOwl:hasSynonym xml:lang="en">egg product, imitation</oboInOwl:hasSynonym>
	<oboInOwl:hasSynonym xml:lang="en">egg substitute</oboInOwl:hasSynonym>
	<oboInOwl:hasSynonym xml:lang="en">imitation egg product</oboInOwl:hasSynonym>
	<oboInOwl:hasDbXref>LANGUAL:A0254</oboInOwl:hasDbXref>
</owl:Class>

<owl:Class rdf:about="&obo;FOODON_03400255">
	<rdfs:label xml:lang="en">pectin jelly candy (us cfr)</rdfs:label>
	<rdfs:subClassOf rdf:resource="&obo;FOODON_03400162"/>
	<obo:IAO_0000412>http://langual.org</obo:IAO_0000412>
	<obo:IAO_0000115 xml:lang="en">Jelly candy having pectin as its principal jelling ingredient.</obo:IAO_0000115>
	<obo:IAO_0000114 rdf:resource="&obo;IAO_0000428"/>
	<oboInOwl:hasDbXref>LANGUAL:A0255</oboInOwl:hasDbXref>
</owl:Class>

<owl:Class rdf:about="&obo;FOODON_03400256">
	<rdfs:label xml:lang="en">starch jelly candy (us cfr)</rdfs:label>
	<rdfs:subClassOf rdf:resource="&obo;FOODON_03400162"/>
	<obo:IAO_0000412>http://langual.org</obo:IAO_0000412>
	<obo:IAO_0000115 xml:lang="en">Jelly candy having starch as its principal jelling ingredient.</obo:IAO_0000115>
	<obo:IAO_0000114 rdf:resource="&obo;IAO_0000428"/>
	<oboInOwl:hasDbXref>LANGUAL:A0256</oboInOwl:hasDbXref>
</owl:Class>

<owl:Class rdf:about="&obo;FOODON_03400257">
	<rdfs:label xml:lang="en">fruit or vegetable product (us cfr)</rdfs:label>
	<rdfs:subClassOf rdf:resource="&obo;FOODON_03401270"/>
	<obo:IAO_0000412>http://langual.org</obo:IAO_0000412>
	<obo:IAO_0000115 xml:lang="en">Fruits and vegetables in all forms. [FDA CFSAN 1995]</obo:IAO_0000115>
	<obo:IAO_0000114 rdf:resource="&obo;IAO_0000428"/>
	<oboInOwl:hasDbXref>LANGUAL:A0257</oboInOwl:hasDbXref>
</owl:Class>

<owl:Class rdf:about="&obo;FOODON_03400258">
	<rdfs:label xml:lang="en">breakfast cereal (us cfr)</rdfs:label>
	<rdfs:subClassOf rdf:resource="&obo;FOODON_03400106"/>
	<obo:IAO_0000412>http://langual.org</obo:IAO_0000412>
	<obo:IAO_0000115 xml:lang="en">Prepared grain product ready or nearly ready for consumption and marketed primarily for breakfast use. Includes formulated breakfast cereals such as 'corn flakes' or 'cheerios' and simple breakfast cereals such as instant oatmeal. Excludes rolled oats, corn grits and similar products, which are indexed under *MILLED GRAIN OR STARCH PRODUCT*. See also *MILLED GRAIN OR STARCH PRODUCT*.</obo:IAO_0000115>
	<obo:IAO_0000114 rdf:resource="&obo;IAO_0000428"/>
	<oboInOwl:hasSynonym xml:lang="en">cereal, breakfast</oboInOwl:hasSynonym>
	<oboInOwl:hasDbXref>LANGUAL:A0258</oboInOwl:hasDbXref>
</owl:Class>

<owl:Class rdf:about="&obo;FOODON_03400260">
	<rdfs:label xml:lang="en">nut or nut product (us cfr)</rdfs:label>
	<rdfs:subClassOf rdf:resource="&obo;FOODON_03400306"/>
	<obo:IAO_0000412>http://langual.org</obo:IAO_0000412>
	<obo:IAO_0000115 xml:lang="en">Nuts in all forms, including nut butters and pastes.</obo:IAO_0000115>
	<obo:IAO_0000114 rdf:resource="&obo;IAO_0000428"/>
	<oboInOwl:hasDbXref>LANGUAL:A0260</oboInOwl:hasDbXref>
</owl:Class>

<owl:Class rdf:about="&obo;FOODON_03400261">
	<rdfs:label xml:lang="en">egg or egg product (us cfr)</rdfs:label>
	<rdfs:subClassOf rdf:resource="&obo;FOODON_03401270"/>
	<obo:IAO_0000412>http://langual.org</obo:IAO_0000412>
	<obo:IAO_0000115 xml:lang="en">Fresh egg in shell, liquid, frozen, dried egg or egg component, or egg product analog. Includes boiled, poached, scrambled, and fried eggs. Excludes prepared egg dishes, such as omelettes.</obo:IAO_0000115>
	<obo:IAO_0000114 rdf:resource="&obo;IAO_0000428"/>
	<oboInOwl:hasDbXref>LANGUAL:A0261</oboInOwl:hasDbXref>
</owl:Class>

<owl:Class rdf:about="&obo;FOODON_03400263">
	<rdfs:label xml:lang="en">condiment sauce (us cfr)</rdfs:label>
	<rdfs:subClassOf rdf:resource="&obo;FOODON_03400179"/>
	<obo:IAO_0000412>http://langual.org</obo:IAO_0000412>
	<obo:IAO_0000115 xml:lang="en">Pourable condiment that is usually applied after the food is prepared but can also be used in cooking. Examples are soy sauce, pepper sauce or barbeque sauce.</obo:IAO_0000115>
	<obo:IAO_0000114 rdf:resource="&obo;IAO_0000428"/>
	<oboInOwl:hasSynonym xml:lang="en">sauce, condiment</oboInOwl:hasSynonym>
	<oboInOwl:hasDbXref>LANGUAL:A0263</oboInOwl:hasDbXref>
</owl:Class>

<owl:Class rdf:about="&obo;FOODON_03400264">
	<rdfs:label xml:lang="en">vegetable juice (us cfr)</rdfs:label>
	<rdfs:subClassOf rdf:resource="&obo;FOODON_03400152"/>
	<obo:IAO_0000412>http://langual.org</obo:IAO_0000412>
	<obo:IAO_0000115 xml:lang="en">The liquid extracted or expressed from mature vegetables with or without optional ingredients such as seasoning or salt.  Products prepared from vegetable juice by thickening with gelatin or pectin are indexed under the broader term *VEGETABLE OR VEGETABLE PRODUCT*. For part or portion, index the part or the plant from which the juice was extracted, rather than *PLANT EXTRACT, CONCENTRATE, OR ISOLATE*.</obo:IAO_0000115>
	<obo:IAO_0000114 rdf:resource="&obo;IAO_0000428"/>
	<oboInOwl:hasSynonym xml:lang="en">juice, vegetable</oboInOwl:hasSynonym>
	<oboInOwl:hasDbXref>LANGUAL:A0264</oboInOwl:hasDbXref>
</owl:Class>

<owl:Class rdf:about="&obo;FOODON_03400266">
	<rdfs:label xml:lang="en">pasteurized cheese spread (us cfr)</rdfs:label>
	<rdfs:subClassOf rdf:resource="&obo;FOODON_03400117"/>
	<obo:IAO_0000412>http://langual.org</obo:IAO_0000412>
	<obo:IAO_0000115 xml:lang="en">Pasteurized cheese product made without emulsifier and with opional dairy ingredients. Milkfat minimum 20% of total; moisture minimum 44%, maximum 60% (21 CFR 133.175, 133.176).</obo:IAO_0000115>
	<obo:IAO_0000114 rdf:resource="&obo;IAO_0000428"/>
	<oboInOwl:hasDbXref>LANGUAL:A0266</oboInOwl:hasDbXref>
</owl:Class>

<owl:Class rdf:about="&obo;FOODON_03400267">
	<rdfs:label xml:lang="en">seafood or seafood product (us cfr)</rdfs:label>
	<rdfs:subClassOf rdf:resource="&obo;FOODON_03400217"/>
	<obo:IAO_0000412>http://langual.org</obo:IAO_0000412>
	<obo:IAO_0000115 xml:lang="en">Flesh from fish or shellfish. Includes seafood product analogs and seafood-based sausage or luncheon meat as well as such products as squid ink and clam juice.</obo:IAO_0000115>
	<obo:IAO_0000114 rdf:resource="&obo;IAO_0000428"/>
	<oboInOwl:hasDbXref>LANGUAL:A0267</oboInOwl:hasDbXref>
</owl:Class>

<owl:Class rdf:about="&obo;FOODON_03400268">
	<rdfs:label xml:lang="en">steeped beverage (us cfr)</rdfs:label>
	<rdfs:subClassOf rdf:resource="&obo;FOODON_03400112"/>
	<obo:IAO_0000412>http://langual.org</obo:IAO_0000412>
	<obo:IAO_0000115 xml:lang="en">Beverage prepared by extrcting flavor and other components from food sources by percolation and/or immersion in water, usually at near-boiling temperature.</obo:IAO_0000115>
	<obo:IAO_0000114 rdf:resource="&obo;IAO_0000428"/>
	<oboInOwl:hasDbXref>LANGUAL:A0268</oboInOwl:hasDbXref>
</owl:Class>

<owl:Class rdf:about="&obo;FOODON_03400269">
	<rdfs:label xml:lang="en">icing or frosting (us cfr)</rdfs:label>
	<rdfs:subClassOf rdf:resource="&obo;FOODON_03400188"/>
	<obo:IAO_0000412>http://langual.org</obo:IAO_0000412>
	<obo:IAO_0000115 xml:lang="en">Mixture of fat, sweetener and optional ingredients such as fruit juice, milk, flavorings, etc. used as a topping, coating or filling for bakery products.</obo:IAO_0000115>
	<obo:IAO_0000114 rdf:resource="&obo;IAO_0000428"/>
	<oboInOwl:hasSynonym xml:lang="en">frosting</oboInOwl:hasSynonym>
	<oboInOwl:hasDbXref>LANGUAL:A0269</oboInOwl:hasDbXref>
</owl:Class>

<owl:Class rdf:about="&obo;FOODON_03400271">
	<rdfs:label xml:lang="en">vegetable pickle (us cfr)</rdfs:label>
	<rdfs:subClassOf rdf:resource="&obo;FOODON_03400152"/>
	<obo:IAO_0000412>http://langual.org</obo:IAO_0000412>
	<obo:IAO_0000115 xml:lang="en">Vegetable product prepared by immersing vegetable in a brine or an acid solution. Often this treatment induces fermentation and/or other changes in the product.</obo:IAO_0000115>
	<obo:IAO_0000114 rdf:resource="&obo;IAO_0000428"/>
	<oboInOwl:hasSynonym xml:lang="en">pickle, vegetable</oboInOwl:hasSynonym>
	<oboInOwl:hasDbXref>LANGUAL:A0271</oboInOwl:hasDbXref>
</owl:Class>

<owl:Class rdf:about="&obo;FOODON_03400272">
	<rdfs:label xml:lang="en">cacao or chocolate product (us cfr)</rdfs:label>
	<rdfs:subClassOf rdf:resource="&obo;FOODON_03401270"/>
	<obo:IAO_0000412>http://langual.org</obo:IAO_0000412>
	<obo:IAO_0000115 xml:lang="en">Any form of cacao, cacao product, chocolate, chocolate product or chocolate product analog except chocolate candy; includes such products as cacao beans, cacao nibs, chocolate liquor, sweet or milk chocolate, and chocolate syrup; excludes flavors and extracts derived from cacao beans and chocolate- or cacao-flavored foods (21 CFR 163). [FDA CFSAN 1995]</obo:IAO_0000115>
	<obo:IAO_0000114 rdf:resource="&obo;IAO_0000428"/>
	<oboInOwl:hasSynonym xml:lang="en">chocolate or cacao product</oboInOwl:hasSynonym>
	<oboInOwl:hasDbXref>LANGUAL:A0272</oboInOwl:hasDbXref>
</owl:Class>

<owl:Class rdf:about="&obo;FOODON_03400273">
	<rdfs:label xml:lang="en">poultry or poultry product (us cfr)</rdfs:label>
	<rdfs:subClassOf rdf:resource="&obo;FOODON_03400217"/>
	<obo:IAO_0000412>http://langual.org</obo:IAO_0000412>
	<obo:IAO_0000115 xml:lang="en">Meat (flesh and organs including blood and bone marrow) from poultry. Used for poultry meat in all forms including poultry product analogs and poultry-based sausage or luncheon meat.</obo:IAO_0000115>
	<obo:IAO_0000114 rdf:resource="&obo;IAO_0000428"/>
	<oboInOwl:hasDbXref>LANGUAL:A0273</oboInOwl:hasDbXref>
</owl:Class>

<owl:Class rdf:about="&obo;FOODON_03400274">
	<rdfs:label xml:lang="en">meal replacement (us cfr)</rdfs:label>
	<rdfs:subClassOf rdf:resource="&obo;FOODON_03400309"/>
	<obo:IAO_0000412>http://langual.org</obo:IAO_0000412>
	<obo:IAO_0000115 xml:lang="en">Formulated and often nutritionally controlled product marketed for consumption in place of a conventional meal. The product may be used as the sole or major source of nourishment. It is frequently offered in a form convenient to use. Includes infant formula, products designed for weight loss, instant breakfast, interal and parenteral complete nutrition solutions, etc.</obo:IAO_0000115>
	<obo:IAO_0000114 rdf:resource="&obo;IAO_0000428"/>
	<oboInOwl:hasSynonym xml:lang="en">breakfast squares</oboInOwl:hasSynonym>
	<oboInOwl:hasSynonym xml:lang="en">energy food stick</oboInOwl:hasSynonym>
	<oboInOwl:hasSynonym xml:lang="en">instant breakfast</oboInOwl:hasSynonym>
	<oboInOwl:hasDbXref>LANGUAL:A0274</oboInOwl:hasDbXref>
</owl:Class>

<owl:Class rdf:about="&obo;FOODON_03400275">
	<rdfs:label xml:lang="en">macaroni or noodle product (us cfr)</rdfs:label>
	<rdfs:subClassOf rdf:resource="&obo;FOODON_03400106"/>
	<obo:IAO_0000412>http://langual.org</obo:IAO_0000412>
	<obo:IAO_0000115 xml:lang="en">A prepared grain or starch product made by forming units of dough composed of one or more flours, water and other ingredients. Macaroni, spaghetti and vermicelli may have *EGG WHITE ADDED*, but not egg yolk. Noodles, egg macaroni, egg spaghetti and egg vermicelli have *EGG YOLK ADDED* and should be so indexed. This refers to macaroni or noodles used as ingredients; excludes *PASTA DISH*, which is found under *PREPARED FOOD PRODUCT* (21 CFR 139).</obo:IAO_0000115>
	<obo:IAO_0000114 rdf:resource="&obo;IAO_0000428"/>
	<oboInOwl:hasDbXref>LANGUAL:A0275</oboInOwl:hasDbXref>
</owl:Class>

<owl:Class rdf:about="&obo;FOODON_03400276">
	<rdfs:label xml:lang="en">dressing for food (us cfr)</rdfs:label>
	<rdfs:subClassOf rdf:resource="&obo;FOODON_03400105"/>
	<obo:IAO_0000412>http://langual.org</obo:IAO_0000412>
	<obo:IAO_0000115 xml:lang="en">Standardized or nonstandardized mixture of edible fats or oils, acidifying agents and optional ingredients such as sweeteners (nutritive or nonnutritive), starch, egg and seasonings. Used in limited amounts to accompany salads and other foods.</obo:IAO_0000115>
	<obo:IAO_0000114 rdf:resource="&obo;IAO_0000428"/>
	<oboInOwl:hasSynonym xml:lang="en">food dressing</oboInOwl:hasSynonym>
	<oboInOwl:hasDbXref>LANGUAL:A0276</oboInOwl:hasDbXref>
</owl:Class>

<owl:Class rdf:about="&obo;FOODON_03400277">
	<rdfs:label xml:lang="en">distilled spirits (us cfr)</rdfs:label>
	<rdfs:subClassOf rdf:resource="&obo;FOODON_03400278"/>
	<obo:IAO_0000412>http://langual.org</obo:IAO_0000412>
	<obo:IAO_0000115 xml:lang="en">Alcoholic beverage prepared by fermentation of grain or plant-related products and subsequent distillation (27 CFR 5.11).</obo:IAO_0000115>
	<obo:IAO_0000114 rdf:resource="&obo;IAO_0000428"/>
	<oboInOwl:hasSynonym xml:lang="en">hard liquor</oboInOwl:hasSynonym>
	<oboInOwl:hasSynonym xml:lang="en">liquor, alcoholic</oboInOwl:hasSynonym>
	<oboInOwl:hasSynonym xml:lang="en">spirits, distilled</oboInOwl:hasSynonym>
	<oboInOwl:hasDbXref>LANGUAL:A0277</oboInOwl:hasDbXref>
</owl:Class>

<owl:Class rdf:about="&obo;FOODON_03400278">
	<rdfs:label xml:lang="en">alcoholic beverage (us cfr)</rdfs:label>
	<rdfs:subClassOf rdf:resource="&obo;FOODON_03400229"/>
	<obo:IAO_0000412>http://langual.org</obo:IAO_0000412>
	<obo:IAO_0000115 xml:lang="en">Beverage containing more than 0.5% alcohol; includes distilled spirits, malt beverage, and wine.</obo:IAO_0000115>
	<obo:IAO_0000114 rdf:resource="&obo;IAO_0000428"/>
	<oboInOwl:hasDbXref>LANGUAL:A0278</oboInOwl:hasDbXref>
</owl:Class>

<owl:Class rdf:about="&obo;FOODON_03400279">
	<rdfs:label xml:lang="en">cured meat (us cfr)</rdfs:label>
	<rdfs:subClassOf rdf:resource="&obo;FOODON_03400150"/>
	<obo:IAO_0000412>http://langual.org</obo:IAO_0000412>
	<obo:IAO_0000115 xml:lang="en">Meat product that has been preserved through treatment with salt (brining, dry salting or injection of salt solution), heating and drying.</obo:IAO_0000115>
	<obo:IAO_0000114 rdf:resource="&obo;IAO_0000428"/>
	<oboInOwl:hasSynonym xml:lang="en">meat, cured</oboInOwl:hasSynonym>
	<oboInOwl:hasDbXref>LANGUAL:A0279</oboInOwl:hasDbXref>
</owl:Class>

<owl:Class rdf:about="&obo;FOODON_03400280">
	<rdfs:label xml:lang="en">cold-pack cheese (us cfr)</rdfs:label>
	<rdfs:subClassOf rdf:resource="&obo;FOODON_03400116"/>
	<obo:IAO_0000412>http://langual.org</obo:IAO_0000412>
	<obo:IAO_0000115 xml:lang="en">Cold-pack cheese product made without other dairy ingredients and without emulsifiers. Milkfat minimum 47% of solids (43% for swiss, 45% for gruyere); moisture maximum 42% (21 CFR 133.123).</obo:IAO_0000115>
	<obo:IAO_0000114 rdf:resource="&obo;IAO_0000428"/>
	<oboInOwl:hasSynonym xml:lang="en">cheese, club</oboInOwl:hasSynonym>
	<oboInOwl:hasSynonym xml:lang="en">cheese, cold-pack</oboInOwl:hasSynonym>
	<oboInOwl:hasSynonym xml:lang="en">club cheese</oboInOwl:hasSynonym>
	<oboInOwl:hasDbXref>LANGUAL:A0280</oboInOwl:hasDbXref>
</owl:Class>

<owl:Class rdf:about="&obo;FOODON_03400281">
	<rdfs:label xml:lang="en">semisoft cheese (us cfr)</rdfs:label>
	<rdfs:subClassOf rdf:resource="&obo;FOODON_03400316"/>
	<obo:IAO_0000412>http://langual.org</obo:IAO_0000412>
	<obo:IAO_0000114 rdf:resource="&obo;IAO_0000428"/>
	<rdfs:comment xml:lang="en">LanguaL curation note: Used for cheeses, which contain more than 39 percent, but not more than 50 percent, of moisture, and their solids contain not less than 50 percent of milkfat [21 CFR Ch. I (4-1-99 Edition)]</rdfs:comment>
	<oboInOwl:hasDbXref>LANGUAL:A0281</oboInOwl:hasDbXref>
</owl:Class>

<owl:Class rdf:about="&obo;FOODON_03400282">
	<rdfs:label xml:lang="en">processed cheese product (us cfr)</rdfs:label>
	<rdfs:subClassOf rdf:resource="&obo;FOODON_03400115"/>
	<obo:IAO_0000412>http://langual.org</obo:IAO_0000412>
	<obo:IAO_0000115 xml:lang="en">Food made from natural cheese of one or more varieties or from cheese, other dairy ingredients and/or emulsifiers, and other optional ingredients by comminuting and possibly application of heat. The result is a homogeneous plastic mass, except for grated cheese product, which is powdered or granular.</obo:IAO_0000115>
	<obo:IAO_0000114 rdf:resource="&obo;IAO_0000428"/>
	<oboInOwl:hasDbXref>LANGUAL:A0282</oboInOwl:hasDbXref>
</owl:Class>

<owl:Class rdf:about="&obo;FOODON_03400283">
	<rdfs:label xml:lang="en">quick bread, unsweetened (us cfr)</rdfs:label>
	<rdfs:subClassOf rdf:resource="&obo;FOODON_03400107"/>
	<obo:IAO_0000412>http://langual.org</obo:IAO_0000412>
	<obo:IAO_0000115 xml:lang="en">Chemically leavened unsweetened bakery product such as biscuits or unsweetened cornbread.</obo:IAO_0000115>
	<obo:IAO_0000114 rdf:resource="&obo;IAO_0000428"/>
	<oboInOwl:hasDbXref>LANGUAL:A0283</oboInOwl:hasDbXref>
</owl:Class>

<owl:Class rdf:about="&obo;FOODON_03400284">
	<rdfs:label xml:lang="en">prepared egg dish (us cfr)</rdfs:label>
	<rdfs:subClassOf rdf:resource="&obo;FOODON_03400172"/>
	<obo:IAO_0000412>http://langual.org</obo:IAO_0000412>
	<obo:IAO_0000115 xml:lang="en">Prepared food product that contains egg as its principal ingredient. Examples include cheese souffle and quiche lorraine.</obo:IAO_0000115>
	<obo:IAO_0000114 rdf:resource="&obo;IAO_0000428"/>
	<oboInOwl:hasSynonym xml:lang="en">quiche</oboInOwl:hasSynonym>
	<oboInOwl:hasDbXref>LANGUAL:A0284</oboInOwl:hasDbXref>
</owl:Class>

<owl:Class rdf:about="&obo;FOODON_03400285">
	<rdfs:label xml:lang="en">custard or pudding (us cfr)</rdfs:label>
	<rdfs:subClassOf rdf:resource="&obo;FOODON_03400222"/>
	<obo:IAO_0000412>http://langual.org</obo:IAO_0000412>
	<obo:IAO_0000115 xml:lang="en">Sweetened or unsweetened custard or starch-based pudding; also non-fruit pie filling.</obo:IAO_0000115>
	<obo:IAO_0000114 rdf:resource="&obo;IAO_0000428"/>
	<oboInOwl:hasSynonym xml:lang="en">pie filling, non-fruit</oboInOwl:hasSynonym>
	<oboInOwl:hasSynonym xml:lang="en">pudding or custard</oboInOwl:hasSynonym>
	<oboInOwl:hasDbXref>LANGUAL:A0285</oboInOwl:hasDbXref>
</owl:Class>

<owl:Class rdf:about="&obo;FOODON_03400286">
	<rdfs:label xml:lang="en">gravy or sauce (us cfr)</rdfs:label>
	<rdfs:subClassOf rdf:resource="&obo;FOODON_03400105"/>
	<obo:IAO_0000412>http://langual.org</obo:IAO_0000412>
	<obo:IAO_0000115 xml:lang="en">Nonstandardized food product used as a meal accompaniment and consisting of a mixture of fats or oils, starch, liquid and other optional ingredients specified by the recipe; excludes condiment sauce (q.v.) and tomato or spaghetti sauce, which are vegetable products.</obo:IAO_0000115>
	<obo:IAO_0000114 rdf:resource="&obo;IAO_0000428"/>
	<oboInOwl:hasSynonym xml:lang="en">sauce or gravy</oboInOwl:hasSynonym>
	<oboInOwl:hasDbXref>LANGUAL:A0286</oboInOwl:hasDbXref>
</owl:Class>

<owl:Class rdf:about="&obo;FOODON_03400287">
	<rdfs:label xml:lang="en">sweet sauce or topping (us cfr)</rdfs:label>
	<rdfs:subClassOf rdf:resource="&obo;FOODON_03400188"/>
	<obo:IAO_0000412>http://langual.org</obo:IAO_0000412>
	<obo:IAO_0000115 xml:lang="en">Sweetened and flavored product that is used as an accompaniment to desserts.</obo:IAO_0000115>
	<obo:IAO_0000114 rdf:resource="&obo;IAO_0000428"/>
	<oboInOwl:hasDbXref>LANGUAL:A0287</oboInOwl:hasDbXref>
</owl:Class>

<owl:Class rdf:about="&obo;FOODON_03400288">
	<rdfs:label xml:lang="en">chocolate candy</rdfs:label>
	<rdfs:subClassOf rdf:resource="&obo;FOODON_03400293"/>
	<obo:IAO_0000412>http://langual.org</obo:IAO_0000412>
	<obo:IAO_0000115 xml:lang="en">Candy with the predominant ingredient chocolate; includes chocolate bars and other forms when these are marketed as candy (21 CFR 163).</obo:IAO_0000115>
	<obo:IAO_0000114 rdf:resource="&obo;IAO_0000428"/>
	<oboInOwl:hasSynonym xml:lang="en">candy, chocolate</oboInOwl:hasSynonym>
	<oboInOwl:hasDbXref>LANGUAL:A0288</oboInOwl:hasDbXref>
</owl:Class>

<owl:Class rdf:about="&obo;FOODON_03400289">
	<rdfs:label xml:lang="en">product type, usa</rdfs:label>
	<rdfs:subClassOf rdf:resource="&obo;FOODON_03400361"/>
	<obo:IAO_0000412>http://langual.org</obo:IAO_0000412>
	<obo:IAO_0000115 xml:lang="en">Food group having common consumption, functional or manufacturing characteristics, e.g. *FRUIT OR VEGETABLE PRODUCT*, *DAIRY PRODUCT*, *CONFECTIONARY*, *PREPARED FOOD PRODUCT*, etc. [FDA CFSAN 1995]</obo:IAO_0000115>
	<obo:IAO_0000114 rdf:resource="&obo;IAO_0000428"/>
	<rdfs:comment xml:lang="en">LanguaL curation note: This term is for CLASSIFICATION ONLY; DO NOT USE term in indexing. Use a more precise narrower term.</rdfs:comment>
	<oboInOwl:hasDbXref>LANGUAL:A0289</oboInOwl:hasDbXref>
</owl:Class>

<owl:Class rdf:about="&obo;FOODON_03400290">
	<rdfs:label xml:lang="en">hard grating cheese (us cfr)</rdfs:label>
	<rdfs:subClassOf rdf:resource="&obo;FOODON_03400316"/>
	<obo:IAO_0000412>http://langual.org</obo:IAO_0000412>
	<obo:IAO_0000114 rdf:resource="&obo;IAO_0000428"/>
	<rdfs:comment xml:lang="en">LanguaL curation note: Used for cheeses (cured cheeses), which contain not more than 34 percent of moisture, and their solids contain not less than 32 percent of milkfat [21 CFR Ch. I (4-1-99 Edition)].</rdfs:comment>
	<oboInOwl:hasDbXref>LANGUAL:A0290</oboInOwl:hasDbXref>
</owl:Class>

<owl:Class rdf:about="&obo;FOODON_03400291">
	<rdfs:label xml:lang="en">grated cheese food</rdfs:label>
	<rdfs:subClassOf rdf:resource="&obo;FOODON_03400282"/>
	<obo:IAO_0000412>http://langual.org</obo:IAO_0000412>
	<obo:IAO_0000115 xml:lang="en">Cheese product made with other dairy ingredients, with or without emulsifiers, with or without the aid of heat. It is a uniformly blended, partially dehydrated, powdered or granular mixture (adapted from 21 CFR 133.147 (grated american cheese food)).</obo:IAO_0000115>
	<obo:IAO_0000114 rdf:resource="&obo;IAO_0000428"/>
	<oboInOwl:hasDbXref>LANGUAL:A0291</oboInOwl:hasDbXref>
</owl:Class>

<owl:Class rdf:about="&obo;FOODON_03400292">
	<rdfs:label xml:lang="en">standardized dressing (us cfr)</rdfs:label>
	<rdfs:subClassOf rdf:resource="&obo;FOODON_03400276"/>
	<obo:IAO_0000412>http://langual.org</obo:IAO_0000412>
	<obo:IAO_0000115 xml:lang="en">Dressing for which standards of identity are specified in the CFR. Includes french dressing (21 CFR 169.115), mayonnaise (21 CFR 169.140) and salad dressing (21 CFR 169.150).</obo:IAO_0000115>
	<obo:IAO_0000114 rdf:resource="&obo;IAO_0000428"/>
	<oboInOwl:hasDbXref>LANGUAL:A0292</oboInOwl:hasDbXref>
</owl:Class>

<owl:Class rdf:about="&obo;FOODON_03400293">
	<rdfs:label xml:lang="en">soft candy (us cfr)</rdfs:label>
	<rdfs:subClassOf rdf:resource="&obo;FOODON_03400204"/>
	<obo:IAO_0000412>http://langual.org</obo:IAO_0000412>
	<obo:IAO_0000115 xml:lang="en">Candy prepared by cooking a mixture of water, sugars and optional ingredients to a temperature of 250 degrees F. or less.</obo:IAO_0000115>
	<obo:IAO_0000114 rdf:resource="&obo;IAO_0000428"/>
	<oboInOwl:hasDbXref>LANGUAL:A0293</oboInOwl:hasDbXref>
</owl:Class>

<owl:Class rdf:about="&obo;FOODON_03400294">
	<rdfs:label xml:lang="en">butter product analog (us cfr)</rdfs:label>
	<rdfs:subClassOf rdf:resource="&obo;FOODON_03400147"/>
	<obo:IAO_0000412>http://langual.org</obo:IAO_0000412>
	<obo:IAO_0000115 xml:lang="en">Food product having functional characteristics similar to a butter product; it may be nutritionally equivalent or inferior to the product it purports to resemble.</obo:IAO_0000115>
	<obo:IAO_0000114 rdf:resource="&obo;IAO_0000428"/>
	<oboInOwl:hasSynonym xml:lang="en">butter substitute</oboInOwl:hasSynonym>
	<oboInOwl:hasSynonym xml:lang="en">butter, imitation</oboInOwl:hasSynonym>
	<oboInOwl:hasSynonym xml:lang="en">imitation butter</oboInOwl:hasSynonym>
	<oboInOwl:hasDbXref>LANGUAL:A0294</oboInOwl:hasDbXref>
</owl:Class>

<owl:Class rdf:about="&obo;FOODON_03400295">
	<rdfs:label xml:lang="en">alcoholic beverage analog (us cfr)</rdfs:label>
	<rdfs:subClassOf rdf:resource="&obo;FOODON_03400112"/>
	<obo:IAO_0000412>http://langual.org</obo:IAO_0000412>
	<obo:IAO_0000115 xml:lang="en">Used for beverages marketed to resemble beer, wine or other alcoholic beverages but containing less than 0.5% alcohol by volume. Excludes unfermented fruit juices even if carbonated, for example, sparkling cider.</obo:IAO_0000115>
	<obo:IAO_0000114 rdf:resource="&obo;IAO_0000428"/>
	<oboInOwl:hasDbXref>LANGUAL:A0295</oboInOwl:hasDbXref>
</owl:Class>

<owl:Class rdf:about="&obo;FOODON_03400296">
	<rdfs:label xml:lang="en">seafood-based sausage or luncheon meat (us cfr)</rdfs:label>
	<rdfs:subClassOf rdf:resource="&obo;FOODON_03400267"/>
	<obo:IAO_0000412>http://langual.org</obo:IAO_0000412>
	<obo:IAO_0000115 xml:lang="en">Food product consisting of comminuted seafood, usually seasoned, pressed and/or encased.</obo:IAO_0000115>
	<obo:IAO_0000114 rdf:resource="&obo;IAO_0000428"/>
	<oboInOwl:hasDbXref>LANGUAL:A0296</oboInOwl:hasDbXref>
</owl:Class>

<owl:Class rdf:about="&obo;FOODON_03400297">
	<rdfs:label xml:lang="en">wine or wine-like product, .5-24% alcohol (us cfr)</rdfs:label>
	<rdfs:subClassOf rdf:resource="&obo;FOODON_03400278"/>
	<obo:IAO_0000412>http://langual.org</obo:IAO_0000412>
	<obo:IAO_0000115 xml:lang="en">Alcoholic beverage produced by the normal fermentation of the juice of grapes or other fruits or of the fermentable parts of plants or plant-related products; may contain certain optional ingredients. Contains between .5-24% alcohol.</obo:IAO_0000115>
	<obo:IAO_0000114 rdf:resource="&obo;IAO_0000428"/>
	<oboInOwl:hasDbXref>LANGUAL:A0297</oboInOwl:hasDbXref>
</owl:Class>

<owl:Class rdf:about="&obo;FOODON_03400298">
	<rdfs:label xml:lang="en">low-alcohol wine, .5-7% alcohol (us cfr)</rdfs:label>
	<rdfs:subClassOf rdf:resource="&obo;FOODON_03400297"/>
	<obo:IAO_0000412>http://langual.org</obo:IAO_0000412>
	<obo:IAO_0000115 xml:lang="en">Wine or wine-like product containing .5-7% alcohol.</obo:IAO_0000115>
	<obo:IAO_0000114 rdf:resource="&obo;IAO_0000428"/>
	<oboInOwl:hasDbXref>LANGUAL:A0298</oboInOwl:hasDbXref>
</owl:Class>

<owl:Class rdf:about="&obo;FOODON_03400299">
	<rdfs:label xml:lang="en">light wine, 7-14% alcohol (us cfr)</rdfs:label>
	<rdfs:subClassOf rdf:resource="&obo;FOODON_03400205"/>
	<obo:IAO_0000412>http://langual.org</obo:IAO_0000412>
	<obo:IAO_0000114 rdf:resource="&obo;IAO_0000428"/>
	<oboInOwl:hasSynonym xml:lang="en">sparkling wine (u.s.)</oboInOwl:hasSynonym>
	<oboInOwl:hasSynonym xml:lang="en">table wine (u.s.)</oboInOwl:hasSynonym>
	<oboInOwl:hasDbXref>LANGUAL:A0299</oboInOwl:hasDbXref>
</owl:Class>

<owl:Class rdf:about="&obo;FOODON_03400300">
	<rdfs:label xml:lang="en">flavoring or flavor enhancer (us cfr)</rdfs:label>
	<rdfs:subClassOf rdf:resource="&obo;FOODON_03400133"/>
	<obo:IAO_0000412>http://langual.org</obo:IAO_0000412>
	<obo:IAO_0000114 rdf:resource="&obo;IAO_0000428"/>
	<oboInOwl:hasSynonym xml:lang="en">flavor enhancer or flavoring</oboInOwl:hasSynonym>
	<oboInOwl:hasDbXref>LANGUAL:A0300</oboInOwl:hasDbXref>
</owl:Class>

<owl:Class rdf:about="&obo;FOODON_03400301">
	<rdfs:label xml:lang="en">flavor enhancer (us cfr)</rdfs:label>
	<rdfs:subClassOf rdf:resource="&obo;FOODON_03400300"/>
	<obo:IAO_0000412>http://langual.org</obo:IAO_0000412>
	<obo:IAO_0000115 xml:lang="en">Substance added to a food to supplement, enhance or modify the original taste and/or aroma of a food or any of its ingredients without imparting a pronounced characteristic taste or aroma of its own (modified from 21 CFR 170.3 (o) (11)).</obo:IAO_0000115>
	<obo:IAO_0000114 rdf:resource="&obo;IAO_0000428"/>
	<oboInOwl:hasSynonym xml:lang="en">taste enhancer</oboInOwl:hasSynonym>
	<oboInOwl:hasDbXref>LANGUAL:A0301</oboInOwl:hasDbXref>
</owl:Class>

<owl:Class rdf:about="&obo;FOODON_03400302">
	<rdfs:label xml:lang="en">vinegar (us cfr)</rdfs:label>
	<rdfs:subClassOf rdf:resource="&obo;FOODON_03400263"/>
	<obo:IAO_0000412>http://langual.org</obo:IAO_0000412>
	<obo:IAO_0000115 xml:lang="en">An acetic acid-containing liquid. Used as condiment or preservative in cooking, pickling and salad dressing preparation; may be flavored with herbs, vegetables or fruits. Natural vinegar is made by fermenting cider, wine, etc.</obo:IAO_0000115>
	<obo:IAO_0000114 rdf:resource="&obo;IAO_0000428"/>
	<oboInOwl:hasDbXref>LANGUAL:A0302</oboInOwl:hasDbXref>
</owl:Class>

<owl:Class rdf:about="&obo;FOODON_03400303">
	<rdfs:label xml:lang="en">reptile, amphibian, insect, etc. meat or meat product (us cfr)</rdfs:label>
	<rdfs:subClassOf rdf:resource="&obo;FOODON_03400217"/>
	<obo:IAO_0000412>http://langual.org</obo:IAO_0000412>
	<obo:IAO_0000115 xml:lang="en">Flesh or edible body part from reptile, amphibian, insect, or other nonmammal origin. Does not include poultry or seafood.</obo:IAO_0000115>
	<obo:IAO_0000114 rdf:resource="&obo;IAO_0000428"/>
	<oboInOwl:hasDbXref>LANGUAL:A0303</oboInOwl:hasDbXref>
</owl:Class>

<owl:Class rdf:about="&obo;FOODON_03400305">
	<rdfs:label xml:lang="en">seed or seed product (us cfr)</rdfs:label>
	<rdfs:subClassOf rdf:resource="&obo;FOODON_03400306"/>
	<obo:IAO_0000412>http://langual.org</obo:IAO_0000412>
	<obo:IAO_0000114 rdf:resource="&obo;IAO_0000428"/>
	<oboInOwl:hasDbXref>LANGUAL:A0305</oboInOwl:hasDbXref>
</owl:Class>

<owl:Class rdf:about="&obo;FOODON_03400306">
	<rdfs:label xml:lang="en">nut or seed product (us cfr)</rdfs:label>
	<rdfs:subClassOf rdf:resource="&obo;FOODON_03401270"/>
	<obo:IAO_0000412>http://langual.org</obo:IAO_0000412>
	<obo:IAO_0000114 rdf:resource="&obo;IAO_0000428"/>
	<oboInOwl:hasDbXref>LANGUAL:A0306</oboInOwl:hasDbXref>
</owl:Class>

<owl:Class rdf:about="&obo;FOODON_03400307">
	<rdfs:label xml:lang="en">frozen tofu dessert (us cfr)</rdfs:label>
	<rdfs:subClassOf rdf:resource="&obo;FOODON_03400206"/>
	<obo:IAO_0000412>http://langual.org</obo:IAO_0000412>
	<obo:IAO_0000115 xml:lang="en">Frozen dessert prepared from tofu ingredient and intended to resemble ice cream.</obo:IAO_0000115>
	<obo:IAO_0000114 rdf:resource="&obo;IAO_0000428"/>
	<oboInOwl:hasSynonym xml:lang="en">tofu dessert, frozen</oboInOwl:hasSynonym>
	<oboInOwl:hasSynonym xml:lang="en">tofu frozen dessert</oboInOwl:hasSynonym>
	<oboInOwl:hasDbXref>LANGUAL:A0307</oboInOwl:hasDbXref>
</owl:Class>

<owl:Class rdf:about="&obo;FOODON_03400308">
	<rdfs:label xml:lang="en">supplemental formulation (us cfr)</rdfs:label>
	<rdfs:subClassOf rdf:resource="&obo;FOODON_03400309"/>
	<obo:IAO_0000412>http://langual.org</obo:IAO_0000412>
	<obo:IAO_0000114 rdf:resource="&obo;IAO_0000428"/>
	<oboInOwl:hasDbXref>LANGUAL:A0308</oboInOwl:hasDbXref>
</owl:Class>

<owl:Class rdf:about="&obo;FOODON_03400309">
	<rdfs:label xml:lang="en">dietary or therapeutic formulation (us cfr)</rdfs:label>
	<rdfs:subClassOf rdf:resource="&obo;FOODON_03400172"/>
	<obo:IAO_0000412>http://langual.org</obo:IAO_0000412>
	<obo:IAO_0000114 rdf:resource="&obo;IAO_0000428"/>
	<oboInOwl:hasSynonym xml:lang="en">therapeutic formulation</oboInOwl:hasSynonym>
	<oboInOwl:hasDbXref>LANGUAL:A0309</oboInOwl:hasDbXref>
</owl:Class>

<owl:Class rdf:about="&obo;FOODON_03400310">
	<rdfs:label xml:lang="en">extra hard cheese (codex)</rdfs:label>
	<rdfs:subClassOf rdf:resource="&obo;FOODON_03400315"/>
	<obo:IAO_0000412>http://langual.org</obo:IAO_0000412>
	<obo:IAO_0000115 xml:lang="en">Cheese having less than 51% moisture on a fat- free basis (CODEX STAN A-6-1978, Rev.1-1999, Amended 2003).
Maximum moisture content 36%, minimum fat content in dry matter 32% (CODEX STAN C-35-1978).
Examples include parmesan, pecorino, romano cheese.</obo:IAO_0000115>
	<obo:IAO_0000114 rdf:resource="&obo;IAO_0000428"/>
	<oboInOwl:hasSynonym xml:lang="en">cheese, extra hard (codex)</oboInOwl:hasSynonym>
	<oboInOwl:hasSynonym xml:lang="en">grating cheese</oboInOwl:hasSynonym>
	<oboInOwl:hasDbXref>LANGUAL:A0310</oboInOwl:hasDbXref>
</owl:Class>

<owl:Class rdf:about="&obo;FOODON_03400311">
	<rdfs:label xml:lang="en">hard cheese (codex)</rdfs:label>
	<rdfs:subClassOf rdf:resource="&obo;FOODON_03400315"/>
	<obo:IAO_0000412>http://langual.org</obo:IAO_0000412>
	<obo:IAO_0000115 xml:lang="en">Cheese having 49-56% moisture on a fat- free basis (CODEX STAN A-6-1978, Rev.1-1999, Amended 2003).
Examples include gruyere, emmental, cheddar.</obo:IAO_0000115>
	<obo:IAO_0000114 rdf:resource="&obo;IAO_0000428"/>
	<oboInOwl:hasDbXref>LANGUAL:A0311</oboInOwl:hasDbXref>
</owl:Class>

<owl:Class rdf:about="&obo;FOODON_03400312">
	<rdfs:label xml:lang="en">semihard cheese (codex)</rdfs:label>
	<rdfs:subClassOf rdf:resource="&obo;FOODON_03400315"/>
	<obo:IAO_0000412>http://langual.org</obo:IAO_0000412>
	<obo:IAO_0000115 xml:lang="en">Cheese having 54-69% moisture on a fat- free basis (CODEX STAN A-6-1978, Rev.1-1999, Amended 2003).
Examples include younger emmental, cheddar, compté, edam, gouda, blue cheese.</obo:IAO_0000115>
	<obo:IAO_0000114 rdf:resource="&obo;IAO_0000428"/>
	<oboInOwl:hasSynonym xml:lang="en">firm cheese</oboInOwl:hasSynonym>
	<oboInOwl:hasSynonym xml:lang="en">semisoft cheese</oboInOwl:hasSynonym>
	<oboInOwl:hasDbXref>LANGUAL:A0312</oboInOwl:hasDbXref>
</owl:Class>

<owl:Class rdf:about="&obo;FOODON_03400313">
	<rdfs:label xml:lang="en">semisoft cheese (codex)</rdfs:label>
	<rdfs:subClassOf rdf:resource="&obo;FOODON_03400315"/>
	<obo:IAO_0000412>http://langual.org</obo:IAO_0000412>
	<obo:IAO_0000115 xml:lang="en">Cheese having between 61-69% moisture on a fat- free basis (Codex Alimentarius Standard A-6, Volume XVI, Ed. 1).</obo:IAO_0000115>
	<owl:deprecated rdf:datatype="&xsd;boolean">true</owl:deprecated>
	<obo:IAO_0000114 rdf:resource="&obo;IAO_0000122"/>
	<rdfs:comment xml:lang="en">LanguaL curation note: This term is only kept for backward compatibility. DO NOT USE for new indexing.</rdfs:comment>
	<oboInOwl:hasDbXref>LANGUAL:A0313</oboInOwl:hasDbXref>
</owl:Class>

<owl:Class rdf:about="&obo;FOODON_03400314">
	<rdfs:label xml:lang="en">soft cheese (codex)</rdfs:label>
	<rdfs:subClassOf rdf:resource="&obo;FOODON_03400315"/>
	<obo:IAO_0000412>http://langual.org</obo:IAO_0000412>
	<obo:IAO_0000115 xml:lang="en">Cheese having greater than 67% moisture on a fat-free basis (CODEX STAN A-6-1978, Rev.1-1999, Amended 2003). Examples include brie, camembert, coulommiers and feta.</obo:IAO_0000115>
	<obo:IAO_0000114 rdf:resource="&obo;IAO_0000428"/>
	<oboInOwl:hasDbXref>LANGUAL:A0314</oboInOwl:hasDbXref>
</owl:Class>

<owl:Class rdf:about="&obo;FOODON_03400315">
	<rdfs:label xml:lang="en">cheese hardness class (codex)</rdfs:label>
	<rdfs:subClassOf rdf:resource="&obo;FOODON_03401207"/>
	<obo:IAO_0000412>http://langual.org</obo:IAO_0000412>
	<obo:IAO_0000114 rdf:resource="&obo;IAO_0000428"/>
	<rdfs:comment xml:lang="en">LanguaL curation note: This term is for CLASSIFICATION ONLY; DO NOT USE term in indexing. Use a more precise narrower term.</rdfs:comment>
	<oboInOwl:hasSynonym xml:lang="en">designation according to cheese firmness</oboInOwl:hasSynonym>
	<oboInOwl:hasDbXref>LANGUAL:A0315</oboInOwl:hasDbXref>
</owl:Class>

<owl:Class rdf:about="&obo;FOODON_03400316">
	<rdfs:label xml:lang="en">cheese hardness class (us cfr)</rdfs:label>
	<rdfs:subClassOf rdf:resource="&obo;FOODON_03400168"/>
	<obo:IAO_0000412>http://langual.org</obo:IAO_0000412>
	<obo:IAO_0000114 rdf:resource="&obo;IAO_0000428"/>
	<oboInOwl:hasDbXref>LANGUAL:A0316</oboInOwl:hasDbXref>
</owl:Class>

<owl:Class rdf:about="&obo;FOODON_03400317">
	<rdfs:label xml:lang="en">preservative</rdfs:label>
	<rdfs:subClassOf rdf:resource="&obo;FOODON_03400181"/>
	<obo:IAO_0000412>http://langual.org</obo:IAO_0000412>
	<obo:IAO_0000115 xml:lang="en">Substance added to a product to prevent growth of contaminating microorganisms and subsequent spoilage of the product.</obo:IAO_0000115>
	<obo:IAO_0000114 rdf:resource="&obo;IAO_0000428"/>
	<oboInOwl:hasDbXref>LANGUAL:A0317</oboInOwl:hasDbXref>
</owl:Class>

<owl:Class rdf:about="&obo;FOODON_03400318">
	<rdfs:label xml:lang="en">antioxidant (us cfr)</rdfs:label>
	<rdfs:subClassOf rdf:resource="&obo;FOODON_03400181"/>
	<obo:IAO_0000412>http://langual.org</obo:IAO_0000412>
	<obo:IAO_0000115 xml:lang="en">Substance used to preserve food by retarding deterioration, rancidity or discoloration due to oxidation.</obo:IAO_0000115>
	<obo:IAO_0000114 rdf:resource="&obo;IAO_0000428"/>
	<oboInOwl:hasDbXref>LANGUAL:A0318</oboInOwl:hasDbXref>
</owl:Class>

<owl:Class rdf:about="&obo;FOODON_03400319">
	<rdfs:label xml:lang="en">stabilizer, thickener or gelling agent (us cfr)</rdfs:label>
	<rdfs:subClassOf rdf:resource="&obo;FOODON_03400181"/>
	<obo:IAO_0000412>http://langual.org</obo:IAO_0000412>
	<obo:IAO_0000115 xml:lang="en">Substance used to product viscous solutions or dispersions, to impart body, improve consistency, or stabilize emulsions. Includes suspending and bodying agents, setting agents, jelling agents, bulking agents, viscosity modifiers, etc.</obo:IAO_0000115>
	<obo:IAO_0000114 rdf:resource="&obo;IAO_0000428"/>
	<oboInOwl:hasSynonym xml:lang="en">gelling agent</oboInOwl:hasSynonym>
	<oboInOwl:hasSynonym xml:lang="en">jelling agent</oboInOwl:hasSynonym>
	<oboInOwl:hasSynonym xml:lang="en">thickener</oboInOwl:hasSynonym>
	<oboInOwl:hasDbXref>LANGUAL:A0319</oboInOwl:hasDbXref>
</owl:Class>

<owl:Class rdf:about="&obo;FOODON_03400321">
	<rdfs:label xml:lang="en">stabilizer (us cfr)</rdfs:label>
	<rdfs:subClassOf rdf:resource="&obo;FOODON_03400319"/>
	<obo:IAO_0000412>http://langual.org</obo:IAO_0000412>
	<obo:IAO_0000115 xml:lang="en">Substance used to produce viscous solutions or dispersions, to impart body, improve consistency, or stabilize emulsions.</obo:IAO_0000115>
	<obo:IAO_0000114 rdf:resource="&obo;IAO_0000428"/>
	<oboInOwl:hasDbXref>LANGUAL:A0321</oboInOwl:hasDbXref>
</owl:Class>

<owl:Class rdf:about="&obo;FOODON_03400322">
	<rdfs:label xml:lang="en">acidifier</rdfs:label>
	<rdfs:subClassOf rdf:resource="&obo;FOODON_03400181"/>
	<obo:IAO_0000412>http://langual.org</obo:IAO_0000412>
	<obo:IAO_0000114 rdf:resource="&obo;IAO_0000428"/>
	<oboInOwl:hasDbXref>LANGUAL:A0322</oboInOwl:hasDbXref>
</owl:Class>

<owl:Class rdf:about="&obo;FOODON_03400323">
	<rdfs:label xml:lang="en">food additives</rdfs:label>
	<rdfs:subClassOf rdf:resource="&obo;FOODON_03400361"/>
	<obo:IAO_0000412>http://langual.org</obo:IAO_0000412>
	<obo:IAO_0000114 rdf:resource="&obo;IAO_0000428"/>
	<rdfs:comment xml:lang="en">LanguaL curation note: This term is for CLASSIFICATION ONLY; DO NOT USE term in indexing. Use a more precise narrower term.</rdfs:comment>
	<oboInOwl:hasDbXref>LANGUAL:A0323</oboInOwl:hasDbXref>
</owl:Class>

<owl:Class rdf:about="&obo;FOODON_03400324">
	<rdfs:label xml:lang="en">food additive classification, european community</rdfs:label>
	<rdfs:subClassOf rdf:resource="&obo;FOODON_03400323"/>
	<obo:IAO_0000412>http://langual.org</obo:IAO_0000412>
	<obo:IAO_0000114 rdf:resource="&obo;IAO_0000428"/>
	<rdfs:comment xml:lang="en">LanguaL curation note: This term is for CLASSIFICATION ONLY; DO NOT USE term in indexing. Use a more precise narrower term.</rdfs:comment>
	<oboInOwl:hasDbXref>LANGUAL:A0324</oboInOwl:hasDbXref>
</owl:Class>

<owl:Class rdf:about="&obo;FOODON_03400325">
	<rdfs:label xml:lang="en">acid (ec)</rdfs:label>
	<rdfs:subClassOf rdf:resource="&obo;FOODON_03400324"/>
	<obo:IAO_0000412>http://langual.org</obo:IAO_0000412>
	<obo:IAO_0000115 xml:lang="en">Substance that increases the acidity of a food stuff and/or imparts to a sour taste to it. European Council Directive 95/2/EC.</obo:IAO_0000115>
	<obo:IAO_0000114 rdf:resource="&obo;IAO_0000428"/>
	<oboInOwl:hasDbXref>LANGUAL:A0325</oboInOwl:hasDbXref>
</owl:Class>

<owl:Class rdf:about="&obo;FOODON_03400326">
	<rdfs:label xml:lang="en">acidity regulator (ec)</rdfs:label>
	<rdfs:subClassOf rdf:resource="&obo;FOODON_03400324"/>
	<obo:IAO_0000412>http://langual.org</obo:IAO_0000412>
	<obo:IAO_0000115 xml:lang="en">Substance that alters or controls the acidity or alkalinity of a foodstuff. European Council Directive 95/2/EC.</obo:IAO_0000115>
	<obo:IAO_0000114 rdf:resource="&obo;IAO_0000428"/>
	<oboInOwl:hasDbXref>LANGUAL:A0326</oboInOwl:hasDbXref>
</owl:Class>

<owl:Class rdf:about="&obo;FOODON_03400327">
	<rdfs:label xml:lang="en">anticaking agent (ec)</rdfs:label>
	<rdfs:subClassOf rdf:resource="&obo;FOODON_03400324"/>
	<obo:IAO_0000412>http://langual.org</obo:IAO_0000412>
	<obo:IAO_0000115 xml:lang="en">Substance that reduces the tendency of individual particles of a foodstuff to adhere to one another. European Council Directive 95/2/EC</obo:IAO_0000115>
	<obo:IAO_0000114 rdf:resource="&obo;IAO_0000428"/>
	<oboInOwl:hasDbXref>LANGUAL:A0327</oboInOwl:hasDbXref>
</owl:Class>

<owl:Class rdf:about="&obo;FOODON_03400328">
	<rdfs:label xml:lang="en">antifoaming agent (ec)</rdfs:label>
	<rdfs:subClassOf rdf:resource="&obo;FOODON_03400324"/>
	<obo:IAO_0000412>http://langual.org</obo:IAO_0000412>
	<obo:IAO_0000115 xml:lang="en">Substance that prevents or reduces foaming. European Council Directive 95/2/EC.</obo:IAO_0000115>
	<obo:IAO_0000114 rdf:resource="&obo;IAO_0000428"/>
	<oboInOwl:hasDbXref>LANGUAL:A0328</oboInOwl:hasDbXref>
</owl:Class>

<owl:Class rdf:about="&obo;FOODON_03400329">
	<rdfs:label xml:lang="en">antioxidant (ec)</rdfs:label>
	<rdfs:subClassOf rdf:resource="&obo;FOODON_03400324"/>
	<obo:IAO_0000412>http://langual.org</obo:IAO_0000412>
	<obo:IAO_0000115 xml:lang="en">Substance that prolongs the shelf life of foodstuffs by protecting them against deterioration caused by oxidation, such as fat rancidity and colour changes. European Council Directive 95/2/EC.</obo:IAO_0000115>
	<obo:IAO_0000114 rdf:resource="&obo;IAO_0000428"/>
	<oboInOwl:hasDbXref>LANGUAL:A0329</oboInOwl:hasDbXref>
</owl:Class>

<owl:Class rdf:about="&obo;FOODON_03400330">
	<rdfs:label xml:lang="en">bulking agent (ec)</rdfs:label>
	<rdfs:subClassOf rdf:resource="&obo;FOODON_03400324"/>
	<obo:IAO_0000412>http://langual.org</obo:IAO_0000412>
	<obo:IAO_0000115 xml:lang="en">Substance that contributes to the volume of a foodstuff without contributing significantly to its available energy value. European Council Directive 95/2/EC.</obo:IAO_0000115>
	<obo:IAO_0000114 rdf:resource="&obo;IAO_0000428"/>
	<oboInOwl:hasDbXref>LANGUAL:A0330</oboInOwl:hasDbXref>
</owl:Class>

<owl:Class rdf:about="&obo;FOODON_03400331">
	<rdfs:label xml:lang="en">carrier, including carrier solvent (ec)</rdfs:label>
	<rdfs:subClassOf rdf:resource="&obo;FOODON_03400324"/>
	<obo:IAO_0000412>http://langual.org</obo:IAO_0000412>
	<obo:IAO_0000115 xml:lang="en">Substance used to dissolve, dilute, disperse or otherwise physically modify a food additive without altering its technological function (and without exerting any technological effect themselves) in order to facilitate its handling, application or use. European Council Directive 95/2/EC.</obo:IAO_0000115>
	<obo:IAO_0000114 rdf:resource="&obo;IAO_0000428"/>
	<oboInOwl:hasDbXref>LANGUAL:A0331</oboInOwl:hasDbXref>
</owl:Class>

<owl:Class rdf:about="&obo;FOODON_03400332">
	<rdfs:label xml:lang="en">colour (ec)</rdfs:label>
	<rdfs:subClassOf rdf:resource="&obo;FOODON_03400324"/>
	<obo:IAO_0000412>http://langual.org</obo:IAO_0000412>
	<obo:IAO_0000115 xml:lang="en">Substance that adds or restores the colour in a food, and includes natural constituents of foodstuffs and natural sources that are normally not consumed as foodstuffs as such and not normally used as characteristic ingredients of foods. European Council Directive 94/36/EC.</obo:IAO_0000115>
	<obo:IAO_0000114 rdf:resource="&obo;IAO_0000428"/>
	<oboInOwl:hasDbXref>LANGUAL:A0332</oboInOwl:hasDbXref>
</owl:Class>

<owl:Class rdf:about="&obo;FOODON_03400333">
	<rdfs:label xml:lang="en">emulsifier (ec)</rdfs:label>
	<rdfs:subClassOf rdf:resource="&obo;FOODON_03400324"/>
	<obo:IAO_0000412>http://langual.org</obo:IAO_0000412>
	<obo:IAO_0000115 xml:lang="en">Substance that makes it possible to form or maintain a homogenous mixture of two or more immiscible phases as oil and water in a foodstuff. European Council Directive 95/2/EC.</obo:IAO_0000115>
	<obo:IAO_0000114 rdf:resource="&obo;IAO_0000428"/>
	<oboInOwl:hasDbXref>LANGUAL:A0333</oboInOwl:hasDbXref>
</owl:Class>

<owl:Class rdf:about="&obo;FOODON_03400334">
	<rdfs:label xml:lang="en">emulsifying salt (ec)</rdfs:label>
	<rdfs:subClassOf rdf:resource="&obo;FOODON_03400324"/>
	<obo:IAO_0000412>http://langual.org</obo:IAO_0000412>
	<obo:IAO_0000115 xml:lang="en">Substance that converts proteins contained in cheese into a dispersed form and thereby brings about homogenous distribution of fat and other components. European Council Directive 95/2/EC.</obo:IAO_0000115>
	<obo:IAO_0000114 rdf:resource="&obo;IAO_0000428"/>
	<oboInOwl:hasDbXref>LANGUAL:A0334</oboInOwl:hasDbXref>
</owl:Class>

<owl:Class rdf:about="&obo;FOODON_03400335">
	<rdfs:label xml:lang="en">firming agent (ec)</rdfs:label>
	<rdfs:subClassOf rdf:resource="&obo;FOODON_03400324"/>
	<obo:IAO_0000412>http://langual.org</obo:IAO_0000412>
	<obo:IAO_0000115 xml:lang="en">Substance that makes or keeps tissues of fruit and vegetables firm or crisp, or interacts with gelling agents to produce or strengthen a gel. European Council Directive 95/2/EC.</obo:IAO_0000115>
	<obo:IAO_0000114 rdf:resource="&obo;IAO_0000428"/>
	<oboInOwl:hasDbXref>LANGUAL:A0335</oboInOwl:hasDbXref>
</owl:Class>

<owl:Class rdf:about="&obo;FOODON_03400336">
	<rdfs:label xml:lang="en">flavour enhancer (ec)</rdfs:label>
	<rdfs:subClassOf rdf:resource="&obo;FOODON_03400324"/>
	<obo:IAO_0000412>http://langual.org</obo:IAO_0000412>
	<obo:IAO_0000115 xml:lang="en">Substance that enhances the existing taste and/or odour of a foodstuff. European Council Directive 95/2/EC.</obo:IAO_0000115>
	<obo:IAO_0000114 rdf:resource="&obo;IAO_0000428"/>
	<oboInOwl:hasDbXref>LANGUAL:A0336</oboInOwl:hasDbXref>
</owl:Class>

<owl:Class rdf:about="&obo;FOODON_03400337">
	<rdfs:label xml:lang="en">flour treatment agent (ec)</rdfs:label>
	<rdfs:subClassOf rdf:resource="&obo;FOODON_03400324"/>
	<obo:IAO_0000412>http://langual.org</obo:IAO_0000412>
	<obo:IAO_0000115 xml:lang="en">Flour treatment agent other than emulsifier is a substance that is added to flour or dough to improve its baking quality. European Council Directive 95/2/EC.</obo:IAO_0000115>
	<obo:IAO_0000114 rdf:resource="&obo;IAO_0000428"/>
	<oboInOwl:hasDbXref>LANGUAL:A0337</oboInOwl:hasDbXref>
</owl:Class>

<owl:Class rdf:about="&obo;FOODON_03400338">
	<rdfs:label xml:lang="en">foaming agent (ec)</rdfs:label>
	<rdfs:subClassOf rdf:resource="&obo;FOODON_03400324"/>
	<obo:IAO_0000412>http://langual.org</obo:IAO_0000412>
	<obo:IAO_0000115 xml:lang="en">Substance that makes it possible to form a homogenous dispersion of a gaseous phase in a liquid or solid foodstuff. European Council Directive 95/2/EC.</obo:IAO_0000115>
	<obo:IAO_0000114 rdf:resource="&obo;IAO_0000428"/>
	<oboInOwl:hasDbXref>LANGUAL:A0338</oboInOwl:hasDbXref>
</owl:Class>

<owl:Class rdf:about="&obo;FOODON_03400339">
	<rdfs:label xml:lang="en">gelling agent (ec)</rdfs:label>
	<rdfs:subClassOf rdf:resource="&obo;FOODON_03400324"/>
	<obo:IAO_0000412>http://langual.org</obo:IAO_0000412>
	<obo:IAO_0000115 xml:lang="en">Substance that gives a foodstuff texture through formation of a gel. European Council Directive 95/2/EC.</obo:IAO_0000115>
	<obo:IAO_0000114 rdf:resource="&obo;IAO_0000428"/>
	<oboInOwl:hasDbXref>LANGUAL:A0339</oboInOwl:hasDbXref>
</owl:Class>

<owl:Class rdf:about="&obo;FOODON_03400340">
	<rdfs:label xml:lang="en">glazing agent (including lubricants) (ec)</rdfs:label>
	<rdfs:subClassOf rdf:resource="&obo;FOODON_03400324"/>
	<obo:IAO_0000412>http://langual.org</obo:IAO_0000412>
	<obo:IAO_0000115 xml:lang="en">Substance which, when applied to the external surface of a foodstuff, imparts a shiny appearance or provide a protective coating. European Council Directive 95/2/EC.</obo:IAO_0000115>
	<obo:IAO_0000114 rdf:resource="&obo;IAO_0000428"/>
	<oboInOwl:hasDbXref>LANGUAL:A0340</oboInOwl:hasDbXref>
</owl:Class>

<owl:Class rdf:about="&obo;FOODON_03400341">
	<rdfs:label xml:lang="en">humectant (ec)</rdfs:label>
	<rdfs:subClassOf rdf:resource="&obo;FOODON_03400324"/>
	<obo:IAO_0000412>http://langual.org</obo:IAO_0000412>
	<obo:IAO_0000115 xml:lang="en">Substance that prevents foodstuffs from drying out by counteracting the effect of an atmosphere having a low degree of humidity, or promote the dissolution of a powder in an aqueous medium. European Council Directive 95/2/EC.</obo:IAO_0000115>
	<obo:IAO_0000114 rdf:resource="&obo;IAO_0000428"/>
	<oboInOwl:hasDbXref>LANGUAL:A0341</oboInOwl:hasDbXref>
</owl:Class>

<owl:Class rdf:about="&obo;FOODON_03400342">
	<rdfs:label xml:lang="en">modified starch (ec)</rdfs:label>
	<rdfs:subClassOf rdf:resource="&obo;FOODON_03400324"/>
	<obo:IAO_0000412>http://langual.org</obo:IAO_0000412>
	<obo:IAO_0000115 xml:lang="en">Substance obtained by one or more chemical treatments of edible starches, which may have undergone a physical or enzymatic treatment, and may be acid or alkali thinned or bleached. European Council Directive 95/2/EC.</obo:IAO_0000115>
	<obo:IAO_0000114 rdf:resource="&obo;IAO_0000428"/>
	<oboInOwl:hasDbXref>LANGUAL:A0342</oboInOwl:hasDbXref>
</owl:Class>

<owl:Class rdf:about="&obo;FOODON_03400343">
	<rdfs:label xml:lang="en">packaging gas (ec)</rdfs:label>
	<rdfs:subClassOf rdf:resource="&obo;FOODON_03400324"/>
	<obo:IAO_0000412>http://langual.org</obo:IAO_0000412>
	<obo:IAO_0000115 xml:lang="en">Gas other than air, introduced into a container before, during or after the placing of a foodstuff in that container. European Council Directive 95/2/EC.</obo:IAO_0000115>
	<obo:IAO_0000114 rdf:resource="&obo;IAO_0000428"/>
	<oboInOwl:hasDbXref>LANGUAL:A0343</oboInOwl:hasDbXref>
</owl:Class>

<owl:Class rdf:about="&obo;FOODON_03400344">
	<rdfs:label xml:lang="en">preservative (ec)</rdfs:label>
	<rdfs:subClassOf rdf:resource="&obo;FOODON_03400324"/>
	<obo:IAO_0000412>http://langual.org</obo:IAO_0000412>
	<obo:IAO_0000115 xml:lang="en">Substance that prolongs the shelf life of foodstuffs by protecting them against deterioration caused by micro-organisms. European Council Directive 95/2/EC.</obo:IAO_0000115>
	<obo:IAO_0000114 rdf:resource="&obo;IAO_0000428"/>
	<oboInOwl:hasDbXref>LANGUAL:A0344</oboInOwl:hasDbXref>
</owl:Class>

<owl:Class rdf:about="&obo;FOODON_03400345">
	<rdfs:label xml:lang="en">propellant (ec)</rdfs:label>
	<rdfs:subClassOf rdf:resource="&obo;FOODON_03400324"/>
	<obo:IAO_0000412>http://langual.org</obo:IAO_0000412>
	<obo:IAO_0000115 xml:lang="en">Gas other than air, which expels a foodstuff from a container. European Council Directive 95/2/EC.</obo:IAO_0000115>
	<obo:IAO_0000114 rdf:resource="&obo;IAO_0000428"/>
	<oboInOwl:hasDbXref>LANGUAL:A0345</oboInOwl:hasDbXref>
</owl:Class>

<owl:Class rdf:about="&obo;FOODON_03400346">
	<rdfs:label xml:lang="en">raising agent (ec)</rdfs:label>
	<rdfs:subClassOf rdf:resource="&obo;FOODON_03400324"/>
	<obo:IAO_0000412>http://langual.org</obo:IAO_0000412>
	<obo:IAO_0000115 xml:lang="en">Substance or combinations of substances that liberate gas and thereby increase the volume of a dough or batter. European Council Directive 95/2/EC.</obo:IAO_0000115>
	<obo:IAO_0000114 rdf:resource="&obo;IAO_0000428"/>
	<oboInOwl:hasDbXref>LANGUAL:A0346</oboInOwl:hasDbXref>
</owl:Class>

<owl:Class rdf:about="&obo;FOODON_03400347">
	<rdfs:label xml:lang="en">sequestrant (ec)</rdfs:label>
	<rdfs:subClassOf rdf:resource="&obo;FOODON_03400324"/>
	<obo:IAO_0000412>http://langual.org</obo:IAO_0000412>
	<obo:IAO_0000115 xml:lang="en">Substance that forms chemical complexes with metallic ions. European Council Directive 95/2/EC.</obo:IAO_0000115>
	<obo:IAO_0000114 rdf:resource="&obo;IAO_0000428"/>
	<oboInOwl:hasDbXref>LANGUAL:A0347</oboInOwl:hasDbXref>
</owl:Class>

<owl:Class rdf:about="&obo;FOODON_03400348">
	<rdfs:label xml:lang="en">stabilizer (ec)</rdfs:label>
	<rdfs:subClassOf rdf:resource="&obo;FOODON_03400324"/>
	<obo:IAO_0000412>http://langual.org</obo:IAO_0000412>
	<obo:IAO_0000115 xml:lang="en">Substance that makes it possible to maintain the physico-chemical state of a foodstuff; stabilisers include substances that enable the maintenance of a homogenous dispersion of two or more immiscible substances in a foodstuff and include also substances that stabilise, retain or intensify an existing colour of a foodstuff. European Council Directive 95/2/EC.</obo:IAO_0000115>
	<obo:IAO_0000114 rdf:resource="&obo;IAO_0000428"/>
	<oboInOwl:hasDbXref>LANGUAL:A0348</oboInOwl:hasDbXref>
</owl:Class>

<owl:Class rdf:about="&obo;FOODON_03400349">
	<rdfs:label xml:lang="en">sweetener (ec)</rdfs:label>
	<rdfs:subClassOf rdf:resource="&obo;FOODON_03400324"/>
	<obo:IAO_0000412>http://langual.org</obo:IAO_0000412>
	<obo:IAO_0000115 xml:lang="en">Substance that is used to impart a sweet taste to foodstuffs or as tabletop sweetener. European Council Directive 94/35/EC.</obo:IAO_0000115>
	<obo:IAO_0000114 rdf:resource="&obo;IAO_0000428"/>
	<oboInOwl:hasDbXref>LANGUAL:A0349</oboInOwl:hasDbXref>
</owl:Class>

<owl:Class rdf:about="&obo;FOODON_03400350">
	<rdfs:label xml:lang="en">thickener (ec)</rdfs:label>
	<rdfs:subClassOf rdf:resource="&obo;FOODON_03400324"/>
	<obo:IAO_0000412>http://langual.org</obo:IAO_0000412>
	<obo:IAO_0000115 xml:lang="en">Substance that increases the viscosity of a foodstuff. European Council Directive 95/2/EC.</obo:IAO_0000115>
	<obo:IAO_0000114 rdf:resource="&obo;IAO_0000428"/>
	<oboInOwl:hasDbXref>LANGUAL:A0350</oboInOwl:hasDbXref>
</owl:Class>

<owl:Class rdf:about="&obo;FOODON_03400351">
	<rdfs:label xml:lang="en">codex alimentarius, functional classes</rdfs:label>
	<rdfs:subClassOf rdf:resource="&obo;FOODON_03400323"/>
	<obo:IAO_0000412>http://langual.org</obo:IAO_0000412>
	<obo:IAO_0000114 rdf:resource="&obo;IAO_0000428"/>
	<rdfs:comment xml:lang="en">LanguaL curation note: This term is for CLASSIFICATION ONLY; DO NOT USE term in indexing. Use a more precise narrower term.</rdfs:comment>
	<oboInOwl:hasDbXref>LANGUAL:A0351</oboInOwl:hasDbXref>
</owl:Class>

<owl:Class rdf:about="&obo;FOODON_03400352">
	<rdfs:label xml:lang="en">product type, international</rdfs:label>
	<rdfs:subClassOf rdf:resource="&obo;FOODON_03400361"/>
	<obo:IAO_0000412>http://langual.org</obo:IAO_0000412>
	<obo:IAO_0000115 xml:lang="en">Renamed from *PRODUCT TYPE, CODEX ALIMENTARIUS* in LanguaL 2008.</obo:IAO_0000115>
	<obo:IAO_0000114 rdf:resource="&obo;IAO_0000428"/>
	<rdfs:comment xml:lang="en">LanguaL curation note: This term is for CLASSIFICATION ONLY; DO NOT USE term in indexing. Use a more precise narrower term.</rdfs:comment>
	<oboInOwl:hasDbXref>LANGUAL:A0352</oboInOwl:hasDbXref>
</owl:Class>

<owl:Class rdf:about="&obo;FOODON_03400355">
	<rdfs:label xml:lang="en">food classification for food additives (codex alimentarius)</rdfs:label>
	<rdfs:subClassOf rdf:resource="&obo;FOODON_03400352"/>
	<obo:IAO_0000412>http://langual.org</obo:IAO_0000412>
	<obo:IAO_0000114 rdf:resource="&obo;IAO_0000428"/>
	<rdfs:comment xml:lang="en">LanguaL curation note: This term is for CLASSIFICATION ONLY; DO NOT USE term in indexing. Use a more precise narrower term.</rdfs:comment>
	<oboInOwl:hasDbXref>LANGUAL:A0355</oboInOwl:hasDbXref>
</owl:Class>

<owl:Class rdf:about="&obo;FOODON_03400356">
	<rdfs:label xml:lang="en">product type, european union</rdfs:label>
	<rdfs:subClassOf rdf:resource="&obo;FOODON_03400361"/>
	<obo:IAO_0000412>http://langual.org</obo:IAO_0000412>
	<obo:IAO_0000114 rdf:resource="&obo;IAO_0000428"/>
	<rdfs:comment xml:lang="en">LanguaL curation note: This term is for CLASSIFICATION ONLY; DO NOT USE term in indexing. Use a more precise narrower term.</rdfs:comment>
	<oboInOwl:hasDbXref>LANGUAL:A0356</oboInOwl:hasDbXref>
</owl:Class>

<owl:Class rdf:about="&obo;FOODON_03400357">
	<rdfs:label xml:lang="en">ciaa food classification for food additives</rdfs:label>
	<rdfs:subClassOf rdf:resource="&obo;FOODON_03400356"/>
	<obo:IAO_0000412>http://langual.org</obo:IAO_0000412>
	<obo:IAO_0000114 rdf:resource="&obo;IAO_0000428"/>
	<rdfs:comment xml:lang="en">LanguaL curation note: This term is for CLASSIFICATION ONLY; DO NOT USE term in indexing. Use a more precise narrower term.</rdfs:comment>
	<oboInOwl:hasDbXref>LANGUAL:A0357</oboInOwl:hasDbXref>
</owl:Class>

<owl:Class rdf:about="&obo;FOODON_03400361">
	<rdfs:label xml:lang="en">product type</rdfs:label>
	<obo:IAO_0000412>http://langual.org</obo:IAO_0000412>
	<obo:IAO_0000114 rdf:resource="&obo;IAO_0000428"/>
	<rdfs:comment xml:lang="en">LanguaL curation note: This term is for CLASSIFICATION ONLY; DO NOT USE term in indexing. Use a more precise narrower term.</rdfs:comment>
	<oboInOwl:hasDbXref>LANGUAL:A0361</oboInOwl:hasDbXref>
</owl:Class>

<owl:Class rdf:about="&obo;FOODON_03400362">
	<rdfs:label xml:lang="en">acid (codex)</rdfs:label>
	<rdfs:subClassOf rdf:resource="&obo;FOODON_03400351"/>
	<obo:IAO_0000412>http://langual.org</obo:IAO_0000412>
	<obo:IAO_0000115 xml:lang="en">FAO Food and Nutrition Paper 30/Rev. 1. FAO, Rome 1985. ISBN 92-5-102292-5</obo:IAO_0000115>
	<obo:IAO_0000114 rdf:resource="&obo;IAO_0000428"/>
	<oboInOwl:hasDbXref>LANGUAL:A0362</oboInOwl:hasDbXref>
</owl:Class>

<owl:Class rdf:about="&obo;FOODON_03400363">
	<rdfs:label xml:lang="en">acidifier (codex)</rdfs:label>
	<rdfs:subClassOf rdf:resource="&obo;FOODON_03400351"/>
	<obo:IAO_0000412>http://langual.org</obo:IAO_0000412>
	<obo:IAO_0000115 xml:lang="en">FAO Food and Nutrition Paper 30/Rev. 1. FAO, Rome 1985. ISBN 92-5-102292-5</obo:IAO_0000115>
	<obo:IAO_0000114 rdf:resource="&obo;IAO_0000428"/>
	<oboInOwl:hasDbXref>LANGUAL:A0363</oboInOwl:hasDbXref>
</owl:Class>

<owl:Class rdf:about="&obo;FOODON_03400364">
	<rdfs:label xml:lang="en">alkali (codex)</rdfs:label>
	<rdfs:subClassOf rdf:resource="&obo;FOODON_03400351"/>
	<obo:IAO_0000412>http://langual.org</obo:IAO_0000412>
	<obo:IAO_0000115 xml:lang="en">FAO Food and Nutrition Paper 30/Rev. 1. FAO, Rome 1985. ISBN 92-5-102292-5</obo:IAO_0000115>
	<obo:IAO_0000114 rdf:resource="&obo;IAO_0000428"/>
	<oboInOwl:hasDbXref>LANGUAL:A0364</oboInOwl:hasDbXref>
</owl:Class>

<owl:Class rdf:about="&obo;FOODON_03400365">
	<rdfs:label xml:lang="en">antibleaching agent (codex)</rdfs:label>
	<rdfs:subClassOf rdf:resource="&obo;FOODON_03400351"/>
	<obo:IAO_0000412>http://langual.org</obo:IAO_0000412>
	<obo:IAO_0000115 xml:lang="en">FAO Food and Nutrition Paper 30/Rev. 1. FAO, Rome 1985. ISBN 92-5-102292-5</obo:IAO_0000115>
	<obo:IAO_0000114 rdf:resource="&obo;IAO_0000428"/>
	<oboInOwl:hasDbXref>LANGUAL:A0365</oboInOwl:hasDbXref>
</owl:Class>

<owl:Class rdf:about="&obo;FOODON_03400366">
	<rdfs:label xml:lang="en">antibrowning agent (codex)</rdfs:label>
	<rdfs:subClassOf rdf:resource="&obo;FOODON_03400351"/>
	<obo:IAO_0000412>http://langual.org</obo:IAO_0000412>
	<obo:IAO_0000115 xml:lang="en">FAO Food and Nutrition Paper 30/Rev. 1. FAO, Rome 1985. ISBN 92-5-102292-5</obo:IAO_0000115>
	<obo:IAO_0000114 rdf:resource="&obo;IAO_0000428"/>
	<oboInOwl:hasDbXref>LANGUAL:A0366</oboInOwl:hasDbXref>
</owl:Class>

<owl:Class rdf:about="&obo;FOODON_03400367">
	<rdfs:label xml:lang="en">anticaking agent (codex)</rdfs:label>
	<rdfs:subClassOf rdf:resource="&obo;FOODON_03400351"/>
	<obo:IAO_0000412>http://langual.org</obo:IAO_0000412>
	<obo:IAO_0000115 xml:lang="en">FAO Food and Nutrition Paper 30/Rev. 1. FAO, Rome 1985. ISBN 92-5-102292-5</obo:IAO_0000115>
	<obo:IAO_0000114 rdf:resource="&obo;IAO_0000428"/>
	<oboInOwl:hasDbXref>LANGUAL:A0367</oboInOwl:hasDbXref>
</owl:Class>

<owl:Class rdf:about="&obo;FOODON_03400368">
	<rdfs:label xml:lang="en">antifoaming agent (codex)</rdfs:label>
	<rdfs:subClassOf rdf:resource="&obo;FOODON_03400351"/>
	<obo:IAO_0000412>http://langual.org</obo:IAO_0000412>
	<obo:IAO_0000115 xml:lang="en">FAO Food and Nutrition Paper 30/Rev. 1. FAO, Rome 1985. ISBN 92-5-102292-5</obo:IAO_0000115>
	<obo:IAO_0000114 rdf:resource="&obo;IAO_0000428"/>
	<oboInOwl:hasDbXref>LANGUAL:A0368</oboInOwl:hasDbXref>
</owl:Class>

<owl:Class rdf:about="&obo;FOODON_03400369">
	<rdfs:label xml:lang="en">antimicrobial preservative (codex)</rdfs:label>
	<rdfs:subClassOf rdf:resource="&obo;FOODON_03400351"/>
	<obo:IAO_0000412>http://langual.org</obo:IAO_0000412>
	<obo:IAO_0000115 xml:lang="en">FAO Food and Nutrition Paper 30/Rev. 1. FAO, Rome 1985. ISBN 92-5-102292-5</obo:IAO_0000115>
	<obo:IAO_0000114 rdf:resource="&obo;IAO_0000428"/>
	<oboInOwl:hasDbXref>LANGUAL:A0369</oboInOwl:hasDbXref>
</owl:Class>

<owl:Class rdf:about="&obo;FOODON_03400370">
	<rdfs:label xml:lang="en">antimould and antitrope agent (codex)</rdfs:label>
	<rdfs:subClassOf rdf:resource="&obo;FOODON_03400351"/>
	<obo:IAO_0000412>http://langual.org</obo:IAO_0000412>
	<obo:IAO_0000115 xml:lang="en">FAO Food and Nutrition Paper 30/Rev. 1. FAO, Rome 1985. ISBN 92-5-102292-5</obo:IAO_0000115>
	<obo:IAO_0000114 rdf:resource="&obo;IAO_0000428"/>
	<oboInOwl:hasDbXref>LANGUAL:A0370</oboInOwl:hasDbXref>
</owl:Class>

<owl:Class rdf:about="&obo;FOODON_03400371">
	<rdfs:label xml:lang="en">antioxidant (codex)</rdfs:label>
	<rdfs:subClassOf rdf:resource="&obo;FOODON_03400351"/>
	<obo:IAO_0000412>http://langual.org</obo:IAO_0000412>
	<obo:IAO_0000115 xml:lang="en">FAO Food and Nutrition Paper 30/Rev. 1. FAO, Rome 1985. ISBN 92-5-102292-5</obo:IAO_0000115>
	<obo:IAO_0000114 rdf:resource="&obo;IAO_0000428"/>
	<oboInOwl:hasDbXref>LANGUAL:A0371</oboInOwl:hasDbXref>
</owl:Class>

<owl:Class rdf:about="&obo;FOODON_03400372">
	<rdfs:label xml:lang="en">antioxidant synergist (codex)</rdfs:label>
	<rdfs:subClassOf rdf:resource="&obo;FOODON_03400351"/>
	<obo:IAO_0000412>http://langual.org</obo:IAO_0000412>
	<obo:IAO_0000115 xml:lang="en">FAO Food and Nutrition Paper 30/Rev. 1. FAO, Rome 1985. ISBN 92-5-102292-5</obo:IAO_0000115>
	<obo:IAO_0000114 rdf:resource="&obo;IAO_0000428"/>
	<oboInOwl:hasDbXref>LANGUAL:A0372</oboInOwl:hasDbXref>
</owl:Class>

<owl:Class rdf:about="&obo;FOODON_03400373">
	<rdfs:label xml:lang="en">antioxidants solubilizer (codex)</rdfs:label>
	<rdfs:subClassOf rdf:resource="&obo;FOODON_03400351"/>
	<obo:IAO_0000412>http://langual.org</obo:IAO_0000412>
	<obo:IAO_0000115 xml:lang="en">FAO Food and Nutrition Paper 30/Rev. 1. FAO, Rome 1985. ISBN 92-5-102292-5</obo:IAO_0000115>
	<obo:IAO_0000114 rdf:resource="&obo;IAO_0000428"/>
	<oboInOwl:hasDbXref>LANGUAL:A0373</oboInOwl:hasDbXref>
</owl:Class>

<owl:Class rdf:about="&obo;FOODON_03400374">
	<rdfs:label xml:lang="en">antitrope agent (codex)</rdfs:label>
	<rdfs:subClassOf rdf:resource="&obo;FOODON_03400351"/>
	<obo:IAO_0000412>http://langual.org</obo:IAO_0000412>
	<obo:IAO_0000115 xml:lang="en">FAO Food and Nutrition Paper 30/Rev. 1. FAO, Rome 1985. ISBN 92-5-102292-5</obo:IAO_0000115>
	<obo:IAO_0000114 rdf:resource="&obo;IAO_0000428"/>
	<oboInOwl:hasDbXref>LANGUAL:A0374</oboInOwl:hasDbXref>
</owl:Class>

<owl:Class rdf:about="&obo;FOODON_03400375">
	<rdfs:label xml:lang="en">antispattering agent (codex)</rdfs:label>
	<rdfs:subClassOf rdf:resource="&obo;FOODON_03400351"/>
	<obo:IAO_0000412>http://langual.org</obo:IAO_0000412>
	<obo:IAO_0000115 xml:lang="en">FAO Food and Nutrition Paper 30/Rev. 1. FAO, Rome 1985. ISBN 92-5-102292-5</obo:IAO_0000115>
	<obo:IAO_0000114 rdf:resource="&obo;IAO_0000428"/>
	<oboInOwl:hasDbXref>LANGUAL:A0375</oboInOwl:hasDbXref>
</owl:Class>

<owl:Class rdf:about="&obo;FOODON_03400376">
	<rdfs:label xml:lang="en">binder (codex)</rdfs:label>
	<rdfs:subClassOf rdf:resource="&obo;FOODON_03400351"/>
	<obo:IAO_0000412>http://langual.org</obo:IAO_0000412>
	<obo:IAO_0000115 xml:lang="en">FAO Food and Nutrition Paper 30/Rev. 1. FAO, Rome 1985. ISBN 92-5-102292-5</obo:IAO_0000115>
	<obo:IAO_0000114 rdf:resource="&obo;IAO_0000428"/>
	<oboInOwl:hasDbXref>LANGUAL:A0376</oboInOwl:hasDbXref>
</owl:Class>

<owl:Class rdf:about="&obo;FOODON_03400377">
	<rdfs:label xml:lang="en">bleaching agent (codex)</rdfs:label>
	<rdfs:subClassOf rdf:resource="&obo;FOODON_03400351"/>
	<obo:IAO_0000412>http://langual.org</obo:IAO_0000412>
	<obo:IAO_0000115 xml:lang="en">FAO Food and Nutrition Paper 30/Rev. 1. FAO, Rome 1985. ISBN 92-5-102292-5</obo:IAO_0000115>
	<obo:IAO_0000114 rdf:resource="&obo;IAO_0000428"/>
	<oboInOwl:hasDbXref>LANGUAL:A0377</oboInOwl:hasDbXref>
</owl:Class>

<owl:Class rdf:about="&obo;FOODON_03400378">
	<rdfs:label xml:lang="en">bodying agent (codex)</rdfs:label>
	<rdfs:subClassOf rdf:resource="&obo;FOODON_03400351"/>
	<obo:IAO_0000412>http://langual.org</obo:IAO_0000412>
	<obo:IAO_0000115 xml:lang="en">FAO Food and Nutrition Paper 30/Rev. 1. FAO, Rome 1985. ISBN 92-5-102292-5</obo:IAO_0000115>
	<obo:IAO_0000114 rdf:resource="&obo;IAO_0000428"/>
	<oboInOwl:hasDbXref>LANGUAL:A0378</oboInOwl:hasDbXref>
</owl:Class>

<owl:Class rdf:about="&obo;FOODON_03400379">
	<rdfs:label xml:lang="en">brown salt: nutrient, dietary supplement (codex)</rdfs:label>
	<rdfs:subClassOf rdf:resource="&obo;FOODON_03400351"/>
	<obo:IAO_0000412>http://langual.org</obo:IAO_0000412>
	<obo:IAO_0000115 xml:lang="en">FAO Food and Nutrition Paper 30/Rev. 1. FAO, Rome 1985. ISBN 92-5-102292-5</obo:IAO_0000115>
	<obo:IAO_0000114 rdf:resource="&obo;IAO_0000428"/>
	<oboInOwl:hasDbXref>LANGUAL:A0379</oboInOwl:hasDbXref>
</owl:Class>

<owl:Class rdf:about="&obo;FOODON_03400380">
	<rdfs:label xml:lang="en">buffering agent (codex)</rdfs:label>
	<rdfs:subClassOf rdf:resource="&obo;FOODON_03400351"/>
	<obo:IAO_0000412>http://langual.org</obo:IAO_0000412>
	<obo:IAO_0000115 xml:lang="en">FAO Food and Nutrition Paper 30/Rev. 1. FAO, Rome 1985. ISBN 92-5-102292-5</obo:IAO_0000115>
	<obo:IAO_0000114 rdf:resource="&obo;IAO_0000428"/>
	<oboInOwl:hasDbXref>LANGUAL:A0380</oboInOwl:hasDbXref>
</owl:Class>

<owl:Class rdf:about="&obo;FOODON_03400381">
	<rdfs:label xml:lang="en">bulking agent (codex)</rdfs:label>
	<rdfs:subClassOf rdf:resource="&obo;FOODON_03400351"/>
	<obo:IAO_0000412>http://langual.org</obo:IAO_0000412>
	<obo:IAO_0000115 xml:lang="en">FAO Food and Nutrition Paper 30/Rev. 1. FAO, Rome 1985. ISBN 92-5-102292-5</obo:IAO_0000115>
	<obo:IAO_0000114 rdf:resource="&obo;IAO_0000428"/>
	<oboInOwl:hasDbXref>LANGUAL:A0381</oboInOwl:hasDbXref>
</owl:Class>

<owl:Class rdf:about="&obo;FOODON_03400382">
	<rdfs:label xml:lang="en">carbonating agent (codex)</rdfs:label>
	<rdfs:subClassOf rdf:resource="&obo;FOODON_03400351"/>
	<obo:IAO_0000412>http://langual.org</obo:IAO_0000412>
	<obo:IAO_0000115 xml:lang="en">FAO Food and Nutrition Paper 30/Rev. 1. FAO, Rome 1985. ISBN 92-5-102292-5</obo:IAO_0000115>
	<obo:IAO_0000114 rdf:resource="&obo;IAO_0000428"/>
	<oboInOwl:hasDbXref>LANGUAL:A0382</oboInOwl:hasDbXref>
</owl:Class>

<owl:Class rdf:about="&obo;FOODON_03400383">
	<rdfs:label xml:lang="en">carrier (codex)</rdfs:label>
	<rdfs:subClassOf rdf:resource="&obo;FOODON_03400351"/>
	<obo:IAO_0000412>http://langual.org</obo:IAO_0000412>
	<obo:IAO_0000115 xml:lang="en">FAO Food and Nutrition Paper 30/Rev. 1. FAO, Rome 1985. ISBN 92-5-102292-5</obo:IAO_0000115>
	<obo:IAO_0000114 rdf:resource="&obo;IAO_0000428"/>
	<oboInOwl:hasDbXref>LANGUAL:A0383</oboInOwl:hasDbXref>
</owl:Class>

<owl:Class rdf:about="&obo;FOODON_03400384">
	<rdfs:label xml:lang="en">carrier solvent (codex)</rdfs:label>
	<rdfs:subClassOf rdf:resource="&obo;FOODON_03400351"/>
	<obo:IAO_0000412>http://langual.org</obo:IAO_0000412>
	<obo:IAO_0000115 xml:lang="en">FAO Food and Nutrition Paper 30/Rev. 1. FAO, Rome 1985. ISBN 92-5-102292-5</obo:IAO_0000115>
	<obo:IAO_0000114 rdf:resource="&obo;IAO_0000428"/>
	<oboInOwl:hasDbXref>LANGUAL:A0384</oboInOwl:hasDbXref>
</owl:Class>

<owl:Class rdf:about="&obo;FOODON_03400385">
	<rdfs:label xml:lang="en">chewing gum base (codex)</rdfs:label>
	<rdfs:subClassOf rdf:resource="&obo;FOODON_03400351"/>
	<obo:IAO_0000412>http://langual.org</obo:IAO_0000412>
	<obo:IAO_0000115 xml:lang="en">FAO Food and Nutrition Paper 30/Rev. 1. FAO, Rome 1985. ISBN 92-5-102292-5</obo:IAO_0000115>
	<obo:IAO_0000114 rdf:resource="&obo;IAO_0000428"/>
	<oboInOwl:hasDbXref>LANGUAL:A0385</oboInOwl:hasDbXref>
</owl:Class>

<owl:Class rdf:about="&obo;FOODON_03400386">
	<rdfs:label xml:lang="en">clarifying agent (codex)</rdfs:label>
	<rdfs:subClassOf rdf:resource="&obo;FOODON_03400351"/>
	<obo:IAO_0000412>http://langual.org</obo:IAO_0000412>
	<obo:IAO_0000115 xml:lang="en">FAO Food and Nutrition Paper 30/Rev. 1. FAO, Rome 1985. ISBN 92-5-102292-5</obo:IAO_0000115>
	<obo:IAO_0000114 rdf:resource="&obo;IAO_0000428"/>
	<oboInOwl:hasDbXref>LANGUAL:A0386</oboInOwl:hasDbXref>
</owl:Class>

<owl:Class rdf:about="&obo;FOODON_03400387">
	<rdfs:label xml:lang="en">cloud producing agent (codex)</rdfs:label>
	<rdfs:subClassOf rdf:resource="&obo;FOODON_03400351"/>
	<obo:IAO_0000412>http://langual.org</obo:IAO_0000412>
	<obo:IAO_0000115 xml:lang="en">FAO Food and Nutrition Paper 30/Rev. 1. FAO, Rome 1985. ISBN 92-5-102292-5</obo:IAO_0000115>
	<obo:IAO_0000114 rdf:resource="&obo;IAO_0000428"/>
	<oboInOwl:hasDbXref>LANGUAL:A0387</oboInOwl:hasDbXref>
</owl:Class>

<owl:Class rdf:about="&obo;FOODON_03400388">
	<rdfs:label xml:lang="en">cloud producing agent in non-alcoholic beverages (codex)</rdfs:label>
	<rdfs:subClassOf rdf:resource="&obo;FOODON_03400351"/>
	<obo:IAO_0000412>http://langual.org</obo:IAO_0000412>
	<obo:IAO_0000115 xml:lang="en">FAO Food and Nutrition Paper 30/Rev. 1. FAO, Rome 1985. ISBN 92-5-102292-5</obo:IAO_0000115>
	<obo:IAO_0000114 rdf:resource="&obo;IAO_0000428"/>
	<oboInOwl:hasDbXref>LANGUAL:A0388</oboInOwl:hasDbXref>
</owl:Class>

<owl:Class rdf:about="&obo;FOODON_03400389">
	<rdfs:label xml:lang="en">colloidal stabilizers (codex)</rdfs:label>
	<rdfs:subClassOf rdf:resource="&obo;FOODON_03400351"/>
	<obo:IAO_0000412>http://langual.org</obo:IAO_0000412>
	<obo:IAO_0000115 xml:lang="en">FAO Food and Nutrition Paper 30/Rev. 1. FAO, Rome 1985. ISBN 92-5-102292-5</obo:IAO_0000115>
	<obo:IAO_0000114 rdf:resource="&obo;IAO_0000428"/>
	<oboInOwl:hasDbXref>LANGUAL:A0389</oboInOwl:hasDbXref>
</owl:Class>

<owl:Class rdf:about="&obo;FOODON_03400390">
	<rdfs:label xml:lang="en">colour adjunct (codex)</rdfs:label>
	<rdfs:subClassOf rdf:resource="&obo;FOODON_03400351"/>
	<obo:IAO_0000412>http://langual.org</obo:IAO_0000412>
	<obo:IAO_0000115 xml:lang="en">FAO Food and Nutrition Paper 30/Rev. 1. FAO, Rome 1985. ISBN 92-5-102292-5</obo:IAO_0000115>
	<obo:IAO_0000114 rdf:resource="&obo;IAO_0000428"/>
	<oboInOwl:hasDbXref>LANGUAL:A0390</oboInOwl:hasDbXref>
</owl:Class>

<owl:Class rdf:about="&obo;FOODON_03400391">
	<rdfs:label xml:lang="en">colour fixative (codex)</rdfs:label>
	<rdfs:subClassOf rdf:resource="&obo;FOODON_03400351"/>
	<obo:IAO_0000412>http://langual.org</obo:IAO_0000412>
	<obo:IAO_0000115 xml:lang="en">FAO Food and Nutrition Paper 30/Rev. 1. FAO, Rome 1985. ISBN 92-5-102292-5</obo:IAO_0000115>
	<obo:IAO_0000114 rdf:resource="&obo;IAO_0000428"/>
	<oboInOwl:hasDbXref>LANGUAL:A0391</oboInOwl:hasDbXref>
</owl:Class>

<owl:Class rdf:about="&obo;FOODON_03400392">
	<rdfs:label xml:lang="en">colour retention agent (codex)</rdfs:label>
	<rdfs:subClassOf rdf:resource="&obo;FOODON_03400351"/>
	<obo:IAO_0000412>http://langual.org</obo:IAO_0000412>
	<obo:IAO_0000115 xml:lang="en">FAO Food and Nutrition Paper 30/Rev. 1. FAO, Rome 1985. ISBN 92-5-102292-5</obo:IAO_0000115>
	<obo:IAO_0000114 rdf:resource="&obo;IAO_0000428"/>
	<oboInOwl:hasDbXref>LANGUAL:A0392</oboInOwl:hasDbXref>
</owl:Class>

<owl:Class rdf:about="&obo;FOODON_03400393">
	<rdfs:label xml:lang="en">colour stabilizer (codex)</rdfs:label>
	<rdfs:subClassOf rdf:resource="&obo;FOODON_03400351"/>
	<obo:IAO_0000412>http://langual.org</obo:IAO_0000412>
	<obo:IAO_0000115 xml:lang="en">FAO Food and Nutrition Paper 30/Rev. 1. FAO, Rome 1985. ISBN 92-5-102292-5</obo:IAO_0000115>
	<obo:IAO_0000114 rdf:resource="&obo;IAO_0000428"/>
	<oboInOwl:hasDbXref>LANGUAL:A0393</oboInOwl:hasDbXref>
</owl:Class>

<owl:Class rdf:about="&obo;FOODON_03400394">
	<rdfs:label xml:lang="en">contaminant (codex)</rdfs:label>
	<rdfs:subClassOf rdf:resource="&obo;FOODON_03400351"/>
	<obo:IAO_0000412>http://langual.org</obo:IAO_0000412>
	<obo:IAO_0000115 xml:lang="en">FAO Food and Nutrition Paper 30/Rev. 1. FAO, Rome 1985. ISBN 92-5-102292-5</obo:IAO_0000115>
	<obo:IAO_0000114 rdf:resource="&obo;IAO_0000428"/>
	<oboInOwl:hasDbXref>LANGUAL:A0394</oboInOwl:hasDbXref>
</owl:Class>

<owl:Class rdf:about="&obo;FOODON_03400395">
	<rdfs:label xml:lang="en">decolourizing agent (codex)</rdfs:label>
	<rdfs:subClassOf rdf:resource="&obo;FOODON_03400351"/>
	<obo:IAO_0000412>http://langual.org</obo:IAO_0000412>
	<obo:IAO_0000115 xml:lang="en">FAO Food and Nutrition Paper 30/Rev. 1. FAO, Rome 1985. ISBN 92-5-102292-5</obo:IAO_0000115>
	<obo:IAO_0000114 rdf:resource="&obo;IAO_0000428"/>
	<oboInOwl:hasDbXref>LANGUAL:A0395</oboInOwl:hasDbXref>
</owl:Class>

<owl:Class rdf:about="&obo;FOODON_03400396">
	<rdfs:label xml:lang="en">defoaming agent (codex)</rdfs:label>
	<rdfs:subClassOf rdf:resource="&obo;FOODON_03400351"/>
	<obo:IAO_0000412>http://langual.org</obo:IAO_0000412>
	<obo:IAO_0000115 xml:lang="en">FAO Food and Nutrition Paper 30/Rev. 1. FAO, Rome 1985. ISBN 92-5-102292-5</obo:IAO_0000115>
	<obo:IAO_0000114 rdf:resource="&obo;IAO_0000428"/>
	<oboInOwl:hasDbXref>LANGUAL:A0396</oboInOwl:hasDbXref>
</owl:Class>

<owl:Class rdf:about="&obo;FOODON_03400397">
	<rdfs:label xml:lang="en">density adjusting agent (codex)</rdfs:label>
	<rdfs:subClassOf rdf:resource="&obo;FOODON_03400351"/>
	<obo:IAO_0000412>http://langual.org</obo:IAO_0000412>
	<obo:IAO_0000115 xml:lang="en">FAO Food and Nutrition Paper 30/Rev. 1. FAO, Rome 1985. ISBN 92-5-102292-5</obo:IAO_0000115>
	<obo:IAO_0000114 rdf:resource="&obo;IAO_0000428"/>
	<oboInOwl:hasDbXref>LANGUAL:A0397</oboInOwl:hasDbXref>
</owl:Class>

<owl:Class rdf:about="&obo;FOODON_03400398">
	<rdfs:label xml:lang="en">dietary supplement (codex)</rdfs:label>
	<rdfs:subClassOf rdf:resource="&obo;FOODON_03400351"/>
	<obo:IAO_0000412>http://langual.org</obo:IAO_0000412>
	<obo:IAO_0000115 xml:lang="en">FAO Food and Nutrition Paper 30/Rev. 1. FAO, Rome 1985. ISBN 92-5-102292-5</obo:IAO_0000115>
	<obo:IAO_0000114 rdf:resource="&obo;IAO_0000428"/>
	<oboInOwl:hasDbXref>LANGUAL:A0398</oboInOwl:hasDbXref>
</owl:Class>

<owl:Class rdf:about="&obo;FOODON_03400399">
	<rdfs:label xml:lang="en">diluent of colour and other food additives (codex)</rdfs:label>
	<rdfs:subClassOf rdf:resource="&obo;FOODON_03400351"/>
	<obo:IAO_0000412>http://langual.org</obo:IAO_0000412>
	<obo:IAO_0000115 xml:lang="en">FAO Food and Nutrition Paper 30/Rev. 1. FAO, Rome 1985. ISBN 92-5-102292-5</obo:IAO_0000115>
	<obo:IAO_0000114 rdf:resource="&obo;IAO_0000428"/>
	<oboInOwl:hasDbXref>LANGUAL:A0399</oboInOwl:hasDbXref>
</owl:Class>

<owl:Class rdf:about="&obo;FOODON_03400400">
	<rdfs:label xml:lang="en">dispersing agent (codex)</rdfs:label>
	<rdfs:subClassOf rdf:resource="&obo;FOODON_03400351"/>
	<obo:IAO_0000412>http://langual.org</obo:IAO_0000412>
	<obo:IAO_0000115 xml:lang="en">FAO Food and Nutrition Paper 30/Rev. 1. FAO, Rome 1985. ISBN 92-5-102292-5</obo:IAO_0000115>
	<obo:IAO_0000114 rdf:resource="&obo;IAO_0000428"/>
	<oboInOwl:hasDbXref>LANGUAL:A0400</oboInOwl:hasDbXref>
</owl:Class>

<owl:Class rdf:about="&obo;FOODON_03400401">
	<rdfs:label xml:lang="en">dough conditioner (codex)</rdfs:label>
	<rdfs:subClassOf rdf:resource="&obo;FOODON_03400351"/>
	<obo:IAO_0000412>http://langual.org</obo:IAO_0000412>
	<obo:IAO_0000115 xml:lang="en">FAO Food and Nutrition Paper 30/Rev. 1. FAO, Rome 1985. ISBN 92-5-102292-5</obo:IAO_0000115>
	<obo:IAO_0000114 rdf:resource="&obo;IAO_0000428"/>
	<oboInOwl:hasDbXref>LANGUAL:A0401</oboInOwl:hasDbXref>
</owl:Class>

<owl:Class rdf:about="&obo;FOODON_03400402">
	<rdfs:label xml:lang="en">drying agent (codex)</rdfs:label>
	<rdfs:subClassOf rdf:resource="&obo;FOODON_03400351"/>
	<obo:IAO_0000412>http://langual.org</obo:IAO_0000412>
	<obo:IAO_0000115 xml:lang="en">FAO Food and Nutrition Paper 30/Rev. 1. FAO, Rome 1985. ISBN 92-5-102292-5</obo:IAO_0000115>
	<obo:IAO_0000114 rdf:resource="&obo;IAO_0000428"/>
	<oboInOwl:hasDbXref>LANGUAL:A0402</oboInOwl:hasDbXref>
</owl:Class>

<owl:Class rdf:about="&obo;FOODON_03400403">
	<rdfs:label xml:lang="en">dusting powder (codex)</rdfs:label>
	<rdfs:subClassOf rdf:resource="&obo;FOODON_03400351"/>
	<obo:IAO_0000412>http://langual.org</obo:IAO_0000412>
	<obo:IAO_0000115 xml:lang="en">FAO Food and Nutrition Paper 30/Rev. 1. FAO, Rome 1985. ISBN 92-5-102292-5</obo:IAO_0000115>
	<obo:IAO_0000114 rdf:resource="&obo;IAO_0000428"/>
	<oboInOwl:hasDbXref>LANGUAL:A0403</oboInOwl:hasDbXref>
</owl:Class>

<owl:Class rdf:about="&obo;FOODON_03400404">
	<rdfs:label xml:lang="en">emulsifier (codex)</rdfs:label>
	<rdfs:subClassOf rdf:resource="&obo;FOODON_03400351"/>
	<obo:IAO_0000412>http://langual.org</obo:IAO_0000412>
	<obo:IAO_0000115 xml:lang="en">FAO Food and Nutrition Paper 30/Rev. 1. FAO, Rome 1985. ISBN 92-5-102292-5</obo:IAO_0000115>
	<obo:IAO_0000114 rdf:resource="&obo;IAO_0000428"/>
	<oboInOwl:hasDbXref>LANGUAL:A0404</oboInOwl:hasDbXref>
</owl:Class>

<owl:Class rdf:about="&obo;FOODON_03400405">
	<rdfs:label xml:lang="en">emulsion stabilizer (codex)</rdfs:label>
	<rdfs:subClassOf rdf:resource="&obo;FOODON_03400351"/>
	<obo:IAO_0000412>http://langual.org</obo:IAO_0000412>
	<obo:IAO_0000115 xml:lang="en">FAO Food and Nutrition Paper 30/Rev. 1. FAO, Rome 1985. ISBN 92-5-102292-5</obo:IAO_0000115>
	<obo:IAO_0000114 rdf:resource="&obo;IAO_0000428"/>
	<oboInOwl:hasDbXref>LANGUAL:A0405</oboInOwl:hasDbXref>
</owl:Class>

<owl:Class rdf:about="&obo;FOODON_03400406">
	<rdfs:label xml:lang="en">enzyme preparation (codex)</rdfs:label>
	<rdfs:subClassOf rdf:resource="&obo;FOODON_03400351"/>
	<obo:IAO_0000412>http://langual.org</obo:IAO_0000412>
	<obo:IAO_0000115 xml:lang="en">FAO Food and Nutrition Paper 30/Rev. 1. FAO, Rome 1985. ISBN 92-5-102292-5</obo:IAO_0000115>
	<obo:IAO_0000114 rdf:resource="&obo;IAO_0000428"/>
	<oboInOwl:hasDbXref>LANGUAL:A0406</oboInOwl:hasDbXref>
</owl:Class>

<owl:Class rdf:about="&obo;FOODON_03400407">
	<rdfs:label xml:lang="en">extraction solvent (codex)</rdfs:label>
	<rdfs:subClassOf rdf:resource="&obo;FOODON_03400351"/>
	<obo:IAO_0000412>http://langual.org</obo:IAO_0000412>
	<obo:IAO_0000115 xml:lang="en">FAO Food and Nutrition Paper 30/Rev. 1. FAO, Rome 1985. ISBN 92-5-102292-5</obo:IAO_0000115>
	<obo:IAO_0000114 rdf:resource="&obo;IAO_0000428"/>
	<oboInOwl:hasDbXref>LANGUAL:A0407</oboInOwl:hasDbXref>
</owl:Class>

<owl:Class rdf:about="&obo;FOODON_03400408">
	<rdfs:label xml:lang="en">filler (codex)</rdfs:label>
	<rdfs:subClassOf rdf:resource="&obo;FOODON_03400351"/>
	<obo:IAO_0000412>http://langual.org</obo:IAO_0000412>
	<obo:IAO_0000115 xml:lang="en">FAO Food and Nutrition Paper 30/Rev. 1. FAO, Rome 1985. ISBN 92-5-102292-5</obo:IAO_0000115>
	<obo:IAO_0000114 rdf:resource="&obo;IAO_0000428"/>
	<oboInOwl:hasDbXref>LANGUAL:A0408</oboInOwl:hasDbXref>
</owl:Class>

<owl:Class rdf:about="&obo;FOODON_03400409">
	<rdfs:label xml:lang="en">filtering aid (codex)</rdfs:label>
	<rdfs:subClassOf rdf:resource="&obo;FOODON_03400351"/>
	<obo:IAO_0000412>http://langual.org</obo:IAO_0000412>
	<obo:IAO_0000115 xml:lang="en">FAO Food and Nutrition Paper 30/Rev. 1. FAO, Rome 1985. ISBN 92-5-102292-5</obo:IAO_0000115>
	<obo:IAO_0000114 rdf:resource="&obo;IAO_0000428"/>
	<oboInOwl:hasDbXref>LANGUAL:A0409</oboInOwl:hasDbXref>
</owl:Class>

<owl:Class rdf:about="&obo;FOODON_03400410">
	<rdfs:label xml:lang="en">firming agent (codex)</rdfs:label>
	<rdfs:subClassOf rdf:resource="&obo;FOODON_03400351"/>
	<obo:IAO_0000412>http://langual.org</obo:IAO_0000412>
	<obo:IAO_0000115 xml:lang="en">FAO Food and Nutrition Paper 30/Rev. 1. FAO, Rome 1985. ISBN 92-5-102292-5</obo:IAO_0000115>
	<obo:IAO_0000114 rdf:resource="&obo;IAO_0000428"/>
	<oboInOwl:hasDbXref>LANGUAL:A0410</oboInOwl:hasDbXref>
</owl:Class>

<owl:Class rdf:about="&obo;FOODON_03400411">
	<rdfs:label xml:lang="en">flavour adjunct (codex)</rdfs:label>
	<rdfs:subClassOf rdf:resource="&obo;FOODON_03400351"/>
	<obo:IAO_0000412>http://langual.org</obo:IAO_0000412>
	<obo:IAO_0000115 xml:lang="en">FAO Food and Nutrition Paper 30/Rev. 1. FAO, Rome 1985. ISBN 92-5-102292-5</obo:IAO_0000115>
	<obo:IAO_0000114 rdf:resource="&obo;IAO_0000428"/>
	<oboInOwl:hasDbXref>LANGUAL:A0411</oboInOwl:hasDbXref>
</owl:Class>

<owl:Class rdf:about="&obo;FOODON_03400412">
	<rdfs:label xml:lang="en">flavour enhancer (codex)</rdfs:label>
	<rdfs:subClassOf rdf:resource="&obo;FOODON_03400351"/>
	<obo:IAO_0000412>http://langual.org</obo:IAO_0000412>
	<obo:IAO_0000115 xml:lang="en">FAO Food and Nutrition Paper 30/Rev. 1. FAO, Rome 1985. ISBN 92-5-102292-5</obo:IAO_0000115>
	<obo:IAO_0000114 rdf:resource="&obo;IAO_0000428"/>
	<oboInOwl:hasDbXref>LANGUAL:A0412</oboInOwl:hasDbXref>
</owl:Class>

<owl:Class rdf:about="&obo;FOODON_03400413">
	<rdfs:label xml:lang="en">flavouring agent (codex)</rdfs:label>
	<rdfs:subClassOf rdf:resource="&obo;FOODON_03400351"/>
	<obo:IAO_0000412>http://langual.org</obo:IAO_0000412>
	<obo:IAO_0000115 xml:lang="en">FAO Food and Nutrition Paper 30/Rev. 1. FAO, Rome 1985. ISBN 92-5-102292-5</obo:IAO_0000115>
	<obo:IAO_0000114 rdf:resource="&obo;IAO_0000428"/>
	<oboInOwl:hasDbXref>LANGUAL:A0413</oboInOwl:hasDbXref>
</owl:Class>

<owl:Class rdf:about="&obo;FOODON_03400414">
	<rdfs:label xml:lang="en">flavours solubilizer (codex)</rdfs:label>
	<rdfs:subClassOf rdf:resource="&obo;FOODON_03400351"/>
	<obo:IAO_0000412>http://langual.org</obo:IAO_0000412>
	<obo:IAO_0000115 xml:lang="en">FAO Food and Nutrition Paper 30/Rev. 1. FAO, Rome 1985. ISBN 92-5-102292-5</obo:IAO_0000115>
	<obo:IAO_0000114 rdf:resource="&obo;IAO_0000428"/>
	<oboInOwl:hasDbXref>LANGUAL:A0414</oboInOwl:hasDbXref>
</owl:Class>

<owl:Class rdf:about="&obo;FOODON_03400415">
	<rdfs:label xml:lang="en">flour treatment agent (codex)</rdfs:label>
	<rdfs:subClassOf rdf:resource="&obo;FOODON_03400351"/>
	<obo:IAO_0000412>http://langual.org</obo:IAO_0000412>
	<obo:IAO_0000115 xml:lang="en">FAO Food and Nutrition Paper 30/Rev. 1. FAO, Rome 1985. ISBN 92-5-102292-5</obo:IAO_0000115>
	<obo:IAO_0000114 rdf:resource="&obo;IAO_0000428"/>
	<oboInOwl:hasDbXref>LANGUAL:A0415</oboInOwl:hasDbXref>
</owl:Class>

<owl:Class rdf:about="&obo;FOODON_03400416">
	<rdfs:label xml:lang="en">foaming agent (codex)</rdfs:label>
	<rdfs:subClassOf rdf:resource="&obo;FOODON_03400351"/>
	<obo:IAO_0000412>http://langual.org</obo:IAO_0000412>
	<obo:IAO_0000115 xml:lang="en">FAO Food and Nutrition Paper 30/Rev. 1. FAO, Rome 1985. ISBN 92-5-102292-5</obo:IAO_0000115>
	<obo:IAO_0000114 rdf:resource="&obo;IAO_0000428"/>
	<oboInOwl:hasDbXref>LANGUAL:A0416</oboInOwl:hasDbXref>
</owl:Class>

<owl:Class rdf:about="&obo;FOODON_03400417">
	<rdfs:label xml:lang="en">food colour (codex)</rdfs:label>
	<rdfs:subClassOf rdf:resource="&obo;FOODON_03400351"/>
	<obo:IAO_0000412>http://langual.org</obo:IAO_0000412>
	<obo:IAO_0000115 xml:lang="en">FAO Food and Nutrition Paper 30/Rev. 1. FAO, Rome 1985. ISBN 92-5-102292-5</obo:IAO_0000115>
	<obo:IAO_0000114 rdf:resource="&obo;IAO_0000428"/>
	<oboInOwl:hasDbXref>LANGUAL:A0417</oboInOwl:hasDbXref>
</owl:Class>

<owl:Class rdf:about="&obo;FOODON_03400418">
	<rdfs:label xml:lang="en">food preservative (codex)</rdfs:label>
	<rdfs:subClassOf rdf:resource="&obo;FOODON_03400351"/>
	<obo:IAO_0000412>http://langual.org</obo:IAO_0000412>
	<obo:IAO_0000115 xml:lang="en">FAO Food and Nutrition Paper 30/Rev. 1. FAO, Rome 1985. ISBN 92-5-102292-5</obo:IAO_0000115>
	<obo:IAO_0000114 rdf:resource="&obo;IAO_0000428"/>
	<oboInOwl:hasDbXref>LANGUAL:A0418</oboInOwl:hasDbXref>
</owl:Class>

<owl:Class rdf:about="&obo;FOODON_03400419">
	<rdfs:label xml:lang="en">formulation agent (codex)</rdfs:label>
	<rdfs:subClassOf rdf:resource="&obo;FOODON_03400351"/>
	<obo:IAO_0000412>http://langual.org</obo:IAO_0000412>
	<obo:IAO_0000115 xml:lang="en">FAO Food and Nutrition Paper 30/Rev. 1. FAO, Rome 1985. ISBN 92-5-102292-5</obo:IAO_0000115>
	<obo:IAO_0000114 rdf:resource="&obo;IAO_0000428"/>
	<oboInOwl:hasDbXref>LANGUAL:A0419</oboInOwl:hasDbXref>
</owl:Class>

<owl:Class rdf:about="&obo;FOODON_03400420">
	<rdfs:label xml:lang="en">formulation aid (codex)</rdfs:label>
	<rdfs:subClassOf rdf:resource="&obo;FOODON_03400351"/>
	<obo:IAO_0000412>http://langual.org</obo:IAO_0000412>
	<obo:IAO_0000115 xml:lang="en">FAO Food and Nutrition Paper 30/Rev. 1. FAO, Rome 1985. ISBN 92-5-102292-5</obo:IAO_0000115>
	<obo:IAO_0000114 rdf:resource="&obo;IAO_0000428"/>
	<oboInOwl:hasDbXref>LANGUAL:A0420</oboInOwl:hasDbXref>
</owl:Class>

<owl:Class rdf:about="&obo;FOODON_03400421">
	<rdfs:label xml:lang="en">freezant (codex)</rdfs:label>
	<rdfs:subClassOf rdf:resource="&obo;FOODON_03400351"/>
	<obo:IAO_0000412>http://langual.org</obo:IAO_0000412>
	<obo:IAO_0000115 xml:lang="en">FAO Food and Nutrition Paper 30/Rev. 1. FAO, Rome 1985. ISBN 92-5-102292-5</obo:IAO_0000115>
	<obo:IAO_0000114 rdf:resource="&obo;IAO_0000428"/>
	<oboInOwl:hasDbXref>LANGUAL:A0421</oboInOwl:hasDbXref>
</owl:Class>

<owl:Class rdf:about="&obo;FOODON_03400422">
	<rdfs:label xml:lang="en">fumigant (codex)</rdfs:label>
	<rdfs:subClassOf rdf:resource="&obo;FOODON_03400351"/>
	<obo:IAO_0000412>http://langual.org</obo:IAO_0000412>
	<obo:IAO_0000115 xml:lang="en">FAO Food and Nutrition Paper 30/Rev. 1. FAO, Rome 1985. ISBN 92-5-102292-5</obo:IAO_0000115>
	<obo:IAO_0000114 rdf:resource="&obo;IAO_0000428"/>
	<oboInOwl:hasDbXref>LANGUAL:A0422</oboInOwl:hasDbXref>
</owl:Class>

<owl:Class rdf:about="&obo;FOODON_03400423">
	<rdfs:label xml:lang="en">fungicidal preservative (codex)</rdfs:label>
	<rdfs:subClassOf rdf:resource="&obo;FOODON_03400351"/>
	<obo:IAO_0000412>http://langual.org</obo:IAO_0000412>
	<obo:IAO_0000115 xml:lang="en">FAO Food and Nutrition Paper 30/Rev. 1. FAO, Rome 1985. ISBN 92-5-102292-5</obo:IAO_0000115>
	<obo:IAO_0000114 rdf:resource="&obo;IAO_0000428"/>
	<oboInOwl:hasDbXref>LANGUAL:A0423</oboInOwl:hasDbXref>
</owl:Class>

<owl:Class rdf:about="&obo;FOODON_03400424">
	<rdfs:label xml:lang="en">fungistatic agent (codex)</rdfs:label>
	<rdfs:subClassOf rdf:resource="&obo;FOODON_03400351"/>
	<obo:IAO_0000412>http://langual.org</obo:IAO_0000412>
	<obo:IAO_0000115 xml:lang="en">FAO Food and Nutrition Paper 30/Rev. 1. FAO, Rome 1985. ISBN 92-5-102292-5</obo:IAO_0000115>
	<obo:IAO_0000114 rdf:resource="&obo;IAO_0000428"/>
	<oboInOwl:hasDbXref>LANGUAL:A0424</oboInOwl:hasDbXref>
</owl:Class>

<owl:Class rdf:about="&obo;FOODON_03400425">
	<rdfs:label xml:lang="en">humectant (codex)</rdfs:label>
	<rdfs:subClassOf rdf:resource="&obo;FOODON_03400351"/>
	<obo:IAO_0000412>http://langual.org</obo:IAO_0000412>
	<obo:IAO_0000115 xml:lang="en">FAO Food and Nutrition Paper 30/Rev. 1. FAO, Rome 1985. ISBN 92-5-102292-5</obo:IAO_0000115>
	<obo:IAO_0000114 rdf:resource="&obo;IAO_0000428"/>
	<oboInOwl:hasDbXref>LANGUAL:A0425</oboInOwl:hasDbXref>
</owl:Class>

<owl:Class rdf:about="&obo;FOODON_03400426">
	<rdfs:label xml:lang="en">gelling agent (codex)</rdfs:label>
	<rdfs:subClassOf rdf:resource="&obo;FOODON_03400351"/>
	<obo:IAO_0000412>http://langual.org</obo:IAO_0000412>
	<obo:IAO_0000115 xml:lang="en">FAO Food and Nutrition Paper 30/Rev. 1. FAO, Rome 1985. ISBN 92-5-102292-5</obo:IAO_0000115>
	<obo:IAO_0000114 rdf:resource="&obo;IAO_0000428"/>
	<oboInOwl:hasDbXref>LANGUAL:A0426</oboInOwl:hasDbXref>
</owl:Class>

<owl:Class rdf:about="&obo;FOODON_03400427">
	<rdfs:label xml:lang="en">green: nutrient, diet supplement, anti-caking agent (codex)</rdfs:label>
	<rdfs:subClassOf rdf:resource="&obo;FOODON_03400351"/>
	<obo:IAO_0000412>http://langual.org</obo:IAO_0000412>
	<obo:IAO_0000115 xml:lang="en">FAO Food and Nutrition Paper 30/Rev. 1. FAO, Rome 1985. ISBN 92-5-102292-5</obo:IAO_0000115>
	<obo:IAO_0000114 rdf:resource="&obo;IAO_0000428"/>
	<oboInOwl:hasDbXref>LANGUAL:A0427</oboInOwl:hasDbXref>
</owl:Class>

<owl:Class rdf:about="&obo;FOODON_03400428">
	<rdfs:label xml:lang="en">leavening agent (codex)</rdfs:label>
	<rdfs:subClassOf rdf:resource="&obo;FOODON_03400351"/>
	<obo:IAO_0000412>http://langual.org</obo:IAO_0000412>
	<obo:IAO_0000115 xml:lang="en">FAO Food and Nutrition Paper 30/Rev. 1. FAO, Rome 1985. ISBN 92-5-102292-5</obo:IAO_0000115>
	<obo:IAO_0000114 rdf:resource="&obo;IAO_0000428"/>
	<oboInOwl:hasDbXref>LANGUAL:A0428</oboInOwl:hasDbXref>
</owl:Class>

<owl:Class rdf:about="&obo;FOODON_03400429">
	<rdfs:label xml:lang="en">liquid freezant (codex)</rdfs:label>
	<rdfs:subClassOf rdf:resource="&obo;FOODON_03400351"/>
	<obo:IAO_0000412>http://langual.org</obo:IAO_0000412>
	<obo:IAO_0000115 xml:lang="en">FAO Food and Nutrition Paper 30/Rev. 1. FAO, Rome 1985. ISBN 92-5-102292-5</obo:IAO_0000115>
	<obo:IAO_0000114 rdf:resource="&obo;IAO_0000428"/>
	<oboInOwl:hasDbXref>LANGUAL:A0429</oboInOwl:hasDbXref>
</owl:Class>

<owl:Class rdf:about="&obo;FOODON_03400430">
	<rdfs:label xml:lang="en">moisture retaining agent (codex)</rdfs:label>
	<rdfs:subClassOf rdf:resource="&obo;FOODON_03400351"/>
	<obo:IAO_0000412>http://langual.org</obo:IAO_0000412>
	<obo:IAO_0000115 xml:lang="en">FAO Food and Nutrition Paper 30/Rev. 1. FAO, Rome 1985. ISBN 92-5-102292-5</obo:IAO_0000115>
	<obo:IAO_0000114 rdf:resource="&obo;IAO_0000428"/>
	<oboInOwl:hasDbXref>LANGUAL:A0430</oboInOwl:hasDbXref>
</owl:Class>

<owl:Class rdf:about="&obo;FOODON_03400431">
	<rdfs:label xml:lang="en">neutralizing agent (codex)</rdfs:label>
	<rdfs:subClassOf rdf:resource="&obo;FOODON_03400351"/>
	<obo:IAO_0000412>http://langual.org</obo:IAO_0000412>
	<obo:IAO_0000115 xml:lang="en">FAO Food and Nutrition Paper 30/Rev. 1. FAO, Rome 1985. ISBN 92-5-102292-5</obo:IAO_0000115>
	<obo:IAO_0000114 rdf:resource="&obo;IAO_0000428"/>
	<oboInOwl:hasDbXref>LANGUAL:A0431</oboInOwl:hasDbXref>
</owl:Class>

<owl:Class rdf:about="&obo;FOODON_03400432">
	<rdfs:label xml:lang="en">nutrient (codex)</rdfs:label>
	<rdfs:subClassOf rdf:resource="&obo;FOODON_03400351"/>
	<obo:IAO_0000412>http://langual.org</obo:IAO_0000412>
	<obo:IAO_0000115 xml:lang="en">FAO Food and Nutrition Paper 30/Rev. 1. FAO, Rome 1985. ISBN 92-5-102292-5</obo:IAO_0000115>
	<obo:IAO_0000114 rdf:resource="&obo;IAO_0000428"/>
	<oboInOwl:hasDbXref>LANGUAL:A0432</oboInOwl:hasDbXref>
</owl:Class>

<owl:Class rdf:about="&obo;FOODON_03400433">
	<rdfs:label xml:lang="en">odour removing agent (codex)</rdfs:label>
	<rdfs:subClassOf rdf:resource="&obo;FOODON_03400351"/>
	<obo:IAO_0000412>http://langual.org</obo:IAO_0000412>
	<obo:IAO_0000115 xml:lang="en">FAO Food and Nutrition Paper 30/Rev. 1. FAO, Rome 1985. ISBN 92-5-102292-5</obo:IAO_0000115>
	<obo:IAO_0000114 rdf:resource="&obo;IAO_0000428"/>
	<oboInOwl:hasDbXref>LANGUAL:A0433</oboInOwl:hasDbXref>
</owl:Class>

<owl:Class rdf:about="&obo;FOODON_03400434">
	<rdfs:label xml:lang="en">oxidizing agent (codex)</rdfs:label>
	<rdfs:subClassOf rdf:resource="&obo;FOODON_03400351"/>
	<obo:IAO_0000412>http://langual.org</obo:IAO_0000412>
	<obo:IAO_0000115 xml:lang="en">FAO Food and Nutrition Paper 30/Rev. 1. FAO, Rome 1985. ISBN 92-5-102292-5</obo:IAO_0000115>
	<obo:IAO_0000114 rdf:resource="&obo;IAO_0000428"/>
	<oboInOwl:hasDbXref>LANGUAL:A0434</oboInOwl:hasDbXref>
</owl:Class>

<owl:Class rdf:about="&obo;FOODON_03400435">
	<rdfs:label xml:lang="en">packing gas (codex)</rdfs:label>
	<rdfs:subClassOf rdf:resource="&obo;FOODON_03400351"/>
	<obo:IAO_0000412>http://langual.org</obo:IAO_0000412>
	<obo:IAO_0000115 xml:lang="en">FAO Food and Nutrition Paper 30/Rev. 1. FAO, Rome 1985. ISBN 92-5-102292-5</obo:IAO_0000115>
	<obo:IAO_0000114 rdf:resource="&obo;IAO_0000428"/>
	<oboInOwl:hasDbXref>LANGUAL:A0435</oboInOwl:hasDbXref>
</owl:Class>

<owl:Class rdf:about="&obo;FOODON_03400436">
	<rdfs:label xml:lang="en">propellant (codex)</rdfs:label>
	<rdfs:subClassOf rdf:resource="&obo;FOODON_03400351"/>
	<obo:IAO_0000412>http://langual.org</obo:IAO_0000412>
	<obo:IAO_0000115 xml:lang="en">FAO Food and Nutrition Paper 30/Rev. 1. FAO, Rome 1985. ISBN 92-5-102292-5</obo:IAO_0000115>
	<obo:IAO_0000114 rdf:resource="&obo;IAO_0000428"/>
	<oboInOwl:hasDbXref>LANGUAL:A0436</oboInOwl:hasDbXref>
</owl:Class>

<owl:Class rdf:about="&obo;FOODON_03400437">
	<rdfs:label xml:lang="en">release agent (codex)</rdfs:label>
	<rdfs:subClassOf rdf:resource="&obo;FOODON_03400351"/>
	<obo:IAO_0000412>http://langual.org</obo:IAO_0000412>
	<obo:IAO_0000115 xml:lang="en">FAO Food and Nutrition Paper 30/Rev. 1. FAO, Rome 1985. ISBN 92-5-102292-5</obo:IAO_0000115>
	<obo:IAO_0000114 rdf:resource="&obo;IAO_0000428"/>
	<oboInOwl:hasDbXref>LANGUAL:A0437</oboInOwl:hasDbXref>
</owl:Class>

<owl:Class rdf:about="&obo;FOODON_03400438">
	<rdfs:label xml:lang="en">residue (codex)</rdfs:label>
	<rdfs:subClassOf rdf:resource="&obo;FOODON_03400351"/>
	<obo:IAO_0000412>http://langual.org</obo:IAO_0000412>
	<obo:IAO_0000115 xml:lang="en">FAO Food and Nutrition Paper 30/Rev. 1. FAO, Rome 1985. ISBN 92-5-102292-5</obo:IAO_0000115>
	<obo:IAO_0000114 rdf:resource="&obo;IAO_0000428"/>
	<oboInOwl:hasDbXref>LANGUAL:A0438</oboInOwl:hasDbXref>
</owl:Class>

<owl:Class rdf:about="&obo;FOODON_03400439">
	<rdfs:label xml:lang="en">salt substitute (codex)</rdfs:label>
	<rdfs:subClassOf rdf:resource="&obo;FOODON_03400351"/>
	<obo:IAO_0000412>http://langual.org</obo:IAO_0000412>
	<obo:IAO_0000115 xml:lang="en">FAO Food and Nutrition Paper 30/Rev. 1. FAO, Rome 1985. ISBN 92-5-102292-5</obo:IAO_0000115>
	<obo:IAO_0000114 rdf:resource="&obo;IAO_0000428"/>
	<oboInOwl:hasDbXref>LANGUAL:A0439</oboInOwl:hasDbXref>
</owl:Class>

<owl:Class rdf:about="&obo;FOODON_03400440">
	<rdfs:label xml:lang="en">sealing agent (codex)</rdfs:label>
	<rdfs:subClassOf rdf:resource="&obo;FOODON_03400351"/>
	<obo:IAO_0000412>http://langual.org</obo:IAO_0000412>
	<obo:IAO_0000115 xml:lang="en">FAO Food and Nutrition Paper 30/Rev. 1. FAO, Rome 1985. ISBN 92-5-102292-5</obo:IAO_0000115>
	<obo:IAO_0000114 rdf:resource="&obo;IAO_0000428"/>
	<oboInOwl:hasDbXref>LANGUAL:A0440</oboInOwl:hasDbXref>
</owl:Class>

<owl:Class rdf:about="&obo;FOODON_03400441">
	<rdfs:label xml:lang="en">seasoning agent (codex)</rdfs:label>
	<rdfs:subClassOf rdf:resource="&obo;FOODON_03400351"/>
	<obo:IAO_0000412>http://langual.org</obo:IAO_0000412>
	<obo:IAO_0000115 xml:lang="en">FAO Food and Nutrition Paper 30/Rev. 1. FAO, Rome 1985. ISBN 92-5-102292-5</obo:IAO_0000115>
	<obo:IAO_0000114 rdf:resource="&obo;IAO_0000428"/>
	<oboInOwl:hasDbXref>LANGUAL:A0441</oboInOwl:hasDbXref>
</owl:Class>

<owl:Class rdf:about="&obo;FOODON_03400442">
	<rdfs:label xml:lang="en">sequestrant (codex)</rdfs:label>
	<rdfs:subClassOf rdf:resource="&obo;FOODON_03400351"/>
	<obo:IAO_0000412>http://langual.org</obo:IAO_0000412>
	<obo:IAO_0000115 xml:lang="en">FAO Food and Nutrition Paper 30/Rev. 1. FAO, Rome 1985. ISBN 92-5-102292-5</obo:IAO_0000115>
	<obo:IAO_0000114 rdf:resource="&obo;IAO_0000428"/>
	<oboInOwl:hasDbXref>LANGUAL:A0442</oboInOwl:hasDbXref>
</owl:Class>

<owl:Class rdf:about="&obo;FOODON_03400443">
	<rdfs:label xml:lang="en">stabilizer (codex)</rdfs:label>
	<rdfs:subClassOf rdf:resource="&obo;FOODON_03400351"/>
	<obo:IAO_0000412>http://langual.org</obo:IAO_0000412>
	<obo:IAO_0000115 xml:lang="en">FAO Food and Nutrition Paper 30/Rev. 1. FAO, Rome 1985. ISBN 92-5-102292-5</obo:IAO_0000115>
	<obo:IAO_0000114 rdf:resource="&obo;IAO_0000428"/>
	<oboInOwl:hasDbXref>LANGUAL:A0443</oboInOwl:hasDbXref>
</owl:Class>

<owl:Class rdf:about="&obo;FOODON_03400444">
	<rdfs:label xml:lang="en">suspending agent (codex)</rdfs:label>
	<rdfs:subClassOf rdf:resource="&obo;FOODON_03400351"/>
	<obo:IAO_0000412>http://langual.org</obo:IAO_0000412>
	<obo:IAO_0000115 xml:lang="en">FAO Food and Nutrition Paper 30/Rev. 1. FAO, Rome 1985. ISBN 92-5-102292-5</obo:IAO_0000115>
	<obo:IAO_0000114 rdf:resource="&obo;IAO_0000428"/>
	<oboInOwl:hasDbXref>LANGUAL:A0444</oboInOwl:hasDbXref>
</owl:Class>

<owl:Class rdf:about="&obo;FOODON_03400445">
	<rdfs:label xml:lang="en">sweetening agent (codex)</rdfs:label>
	<rdfs:subClassOf rdf:resource="&obo;FOODON_03400351"/>
	<obo:IAO_0000412>http://langual.org</obo:IAO_0000412>
	<obo:IAO_0000115 xml:lang="en">FAO Food and Nutrition Paper 30/Rev. 1. FAO, Rome 1985. ISBN 92-5-102292-5</obo:IAO_0000115>
	<obo:IAO_0000114 rdf:resource="&obo;IAO_0000428"/>
	<oboInOwl:hasDbXref>LANGUAL:A0445</oboInOwl:hasDbXref>
</owl:Class>

<owl:Class rdf:about="&obo;FOODON_03400446">
	<rdfs:label xml:lang="en">tableting aid (codex)</rdfs:label>
	<rdfs:subClassOf rdf:resource="&obo;FOODON_03400351"/>
	<obo:IAO_0000412>http://langual.org</obo:IAO_0000412>
	<obo:IAO_0000115 xml:lang="en">FAO Food and Nutrition Paper 30/Rev. 1. FAO, Rome 1985. ISBN 92-5-102292-5</obo:IAO_0000115>
	<obo:IAO_0000114 rdf:resource="&obo;IAO_0000428"/>
	<oboInOwl:hasDbXref>LANGUAL:A0446</oboInOwl:hasDbXref>
</owl:Class>

<owl:Class rdf:about="&obo;FOODON_03400447">
	<rdfs:label xml:lang="en">taste removing agent (codex)</rdfs:label>
	<rdfs:subClassOf rdf:resource="&obo;FOODON_03400351"/>
	<obo:IAO_0000412>http://langual.org</obo:IAO_0000412>
	<obo:IAO_0000115 xml:lang="en">FAO Food and Nutrition Paper 30/Rev. 1. FAO, Rome 1985. ISBN 92-5-102292-5</obo:IAO_0000115>
	<obo:IAO_0000114 rdf:resource="&obo;IAO_0000428"/>
	<oboInOwl:hasDbXref>LANGUAL:A0447</oboInOwl:hasDbXref>
</owl:Class>

<owl:Class rdf:about="&obo;FOODON_03400448">
	<rdfs:label xml:lang="en">texturizer (codex)</rdfs:label>
	<rdfs:subClassOf rdf:resource="&obo;FOODON_03400351"/>
	<obo:IAO_0000412>http://langual.org</obo:IAO_0000412>
	<obo:IAO_0000115 xml:lang="en">FAO Food and Nutrition Paper 30/Rev. 1. FAO, Rome 1985. ISBN 92-5-102292-5</obo:IAO_0000115>
	<obo:IAO_0000114 rdf:resource="&obo;IAO_0000428"/>
	<oboInOwl:hasDbXref>LANGUAL:A0448</oboInOwl:hasDbXref>
</owl:Class>

<owl:Class rdf:about="&obo;FOODON_03400449">
	<rdfs:label xml:lang="en">thickening agent (codex)</rdfs:label>
	<rdfs:subClassOf rdf:resource="&obo;FOODON_03400351"/>
	<obo:IAO_0000412>http://langual.org</obo:IAO_0000412>
	<obo:IAO_0000115 xml:lang="en">FAO Food and Nutrition Paper 30/Rev. 1. FAO, Rome 1985. ISBN 92-5-102292-5</obo:IAO_0000115>
	<obo:IAO_0000114 rdf:resource="&obo;IAO_0000428"/>
	<oboInOwl:hasDbXref>LANGUAL:A0449</oboInOwl:hasDbXref>
</owl:Class>

<owl:Class rdf:about="&obo;FOODON_03400450">
	<rdfs:label xml:lang="en">wetting agent (codex)</rdfs:label>
	<rdfs:subClassOf rdf:resource="&obo;FOODON_03400351"/>
	<obo:IAO_0000412>http://langual.org</obo:IAO_0000412>
	<obo:IAO_0000115 xml:lang="en">FAO Food and Nutrition Paper 30/Rev. 1. FAO, Rome 1985. ISBN 92-5-102292-5</obo:IAO_0000115>
	<obo:IAO_0000114 rdf:resource="&obo;IAO_0000428"/>
	<oboInOwl:hasDbXref>LANGUAL:A0450</oboInOwl:hasDbXref>
</owl:Class>

<owl:Class rdf:about="&obo;FOODON_03400451">
	<rdfs:label xml:lang="en">yeast food (codex)</rdfs:label>
	<rdfs:subClassOf rdf:resource="&obo;FOODON_03400351"/>
	<obo:IAO_0000412>http://langual.org</obo:IAO_0000412>
	<obo:IAO_0000115 xml:lang="en">FAO Food and Nutrition Paper 30/Rev. 1. FAO, Rome 1985. ISBN 92-5-102292-5</obo:IAO_0000115>
	<obo:IAO_0000114 rdf:resource="&obo;IAO_0000428"/>
	<oboInOwl:hasDbXref>LANGUAL:A0451</oboInOwl:hasDbXref>
</owl:Class>

<owl:Class rdf:about="&obo;FOODON_03400452">
	<rdfs:label xml:lang="en">dairy products (ciaa)</rdfs:label>
	<rdfs:subClassOf rdf:resource="&obo;FOODON_03400357"/>
	<obo:IAO_0000412>http://langual.org</obo:IAO_0000412>
	<obo:IAO_0000115 xml:lang="en">CIAA ADD/385/90E Rev 5</obo:IAO_0000115>
	<obo:IAO_0000114 rdf:resource="&obo;IAO_0000428"/>
	<oboInOwl:hasDbXref>LANGUAL:A0452</oboInOwl:hasDbXref>
</owl:Class>

<owl:Class rdf:about="&obo;FOODON_03400453">
	<rdfs:label xml:lang="en">fats and oils (ciaa)</rdfs:label>
	<rdfs:subClassOf rdf:resource="&obo;FOODON_03400357"/>
	<obo:IAO_0000412>http://langual.org</obo:IAO_0000412>
	<obo:IAO_0000115 xml:lang="en">CIAA ADD/385/90E Rev 5</obo:IAO_0000115>
	<obo:IAO_0000114 rdf:resource="&obo;IAO_0000428"/>
	<oboInOwl:hasDbXref>LANGUAL:A0453</oboInOwl:hasDbXref>
</owl:Class>

<owl:Class rdf:about="&obo;FOODON_03400454">
	<rdfs:label xml:lang="en">edible ices (ciaa)</rdfs:label>
	<rdfs:subClassOf rdf:resource="&obo;FOODON_03400357"/>
	<obo:IAO_0000412>http://langual.org</obo:IAO_0000412>
	<obo:IAO_0000115 xml:lang="en">CIAA ADD/385/90E Rev 5</obo:IAO_0000115>
	<obo:IAO_0000114 rdf:resource="&obo;IAO_0000428"/>
	<oboInOwl:hasDbXref>LANGUAL:A0454</oboInOwl:hasDbXref>
</owl:Class>

<owl:Class rdf:about="&obo;FOODON_03400455">
	<rdfs:label xml:lang="en">fruits and vegetables (ciaa)</rdfs:label>
	<rdfs:subClassOf rdf:resource="&obo;FOODON_03400357"/>
	<obo:IAO_0000412>http://langual.org</obo:IAO_0000412>
	<obo:IAO_0000115 xml:lang="en">CIAA ADD/385/90E Rev 5</obo:IAO_0000115>
	<obo:IAO_0000114 rdf:resource="&obo;IAO_0000428"/>
	<oboInOwl:hasDbXref>LANGUAL:A0455</oboInOwl:hasDbXref>
</owl:Class>

<owl:Class rdf:about="&obo;FOODON_03400456">
	<rdfs:label xml:lang="en">confectionary (ciaa)</rdfs:label>
	<rdfs:subClassOf rdf:resource="&obo;FOODON_03400357"/>
	<obo:IAO_0000412>http://langual.org</obo:IAO_0000412>
	<obo:IAO_0000115 xml:lang="en">CIAA ADD/385/90E Rev 5</obo:IAO_0000115>
	<obo:IAO_0000114 rdf:resource="&obo;IAO_0000428"/>
	<oboInOwl:hasDbXref>LANGUAL:A0456</oboInOwl:hasDbXref>
</owl:Class>

<owl:Class rdf:about="&obo;FOODON_03400457">
	<rdfs:label xml:lang="en">cereals and cereal products (ciaa)</rdfs:label>
	<rdfs:subClassOf rdf:resource="&obo;FOODON_03400357"/>
	<obo:IAO_0000412>http://langual.org</obo:IAO_0000412>
	<obo:IAO_0000115 xml:lang="en">CIAA ADD/385/90E Rev 5</obo:IAO_0000115>
	<obo:IAO_0000114 rdf:resource="&obo;IAO_0000428"/>
	<oboInOwl:hasDbXref>LANGUAL:A0457</oboInOwl:hasDbXref>
</owl:Class>

<owl:Class rdf:about="&obo;FOODON_03400458">
	<rdfs:label xml:lang="en">bakery wares (ciaa)</rdfs:label>
	<rdfs:subClassOf rdf:resource="&obo;FOODON_03400357"/>
	<obo:IAO_0000412>http://langual.org</obo:IAO_0000412>
	<obo:IAO_0000115 xml:lang="en">CIAA ADD/385/90E Rev 5</obo:IAO_0000115>
	<obo:IAO_0000114 rdf:resource="&obo;IAO_0000428"/>
	<oboInOwl:hasDbXref>LANGUAL:A0458</oboInOwl:hasDbXref>
</owl:Class>

<owl:Class rdf:about="&obo;FOODON_03400459">
	<rdfs:label xml:lang="en">meat and meat products (ciaa)</rdfs:label>
	<rdfs:subClassOf rdf:resource="&obo;FOODON_03400357"/>
	<obo:IAO_0000412>http://langual.org</obo:IAO_0000412>
	<obo:IAO_0000115 xml:lang="en">CIAA ADD/385/90E Rev 5</obo:IAO_0000115>
	<obo:IAO_0000114 rdf:resource="&obo;IAO_0000428"/>
	<oboInOwl:hasDbXref>LANGUAL:A0459</oboInOwl:hasDbXref>
</owl:Class>

<owl:Class rdf:about="&obo;FOODON_03400460">
	<rdfs:label xml:lang="en">fish and fish products (ciaa)</rdfs:label>
	<rdfs:subClassOf rdf:resource="&obo;FOODON_03400357"/>
	<obo:IAO_0000412>http://langual.org</obo:IAO_0000412>
	<obo:IAO_0000115 xml:lang="en">CIAA ADD/385/90E Rev 5</obo:IAO_0000115>
	<obo:IAO_0000114 rdf:resource="&obo;IAO_0000428"/>
	<oboInOwl:hasDbXref>LANGUAL:A0460</oboInOwl:hasDbXref>
</owl:Class>

<owl:Class rdf:about="&obo;FOODON_03400461">
	<rdfs:label xml:lang="en">egg and egg products (ciaa)</rdfs:label>
	<rdfs:subClassOf rdf:resource="&obo;FOODON_03400357"/>
	<obo:IAO_0000412>http://langual.org</obo:IAO_0000412>
	<obo:IAO_0000115 xml:lang="en">CIAA ADD/385/90E Rev 5</obo:IAO_0000115>
	<obo:IAO_0000114 rdf:resource="&obo;IAO_0000428"/>
	<oboInOwl:hasDbXref>LANGUAL:A0461</oboInOwl:hasDbXref>
</owl:Class>

<owl:Class rdf:about="&obo;FOODON_03400462">
	<rdfs:label xml:lang="en">sugar and honey (ciaa)</rdfs:label>
	<rdfs:subClassOf rdf:resource="&obo;FOODON_03400357"/>
	<obo:IAO_0000412>http://langual.org</obo:IAO_0000412>
	<obo:IAO_0000115 xml:lang="en">CIAA ADD/385/90E Rev 5</obo:IAO_0000115>
	<obo:IAO_0000114 rdf:resource="&obo;IAO_0000428"/>
	<oboInOwl:hasDbXref>LANGUAL:A0462</oboInOwl:hasDbXref>
</owl:Class>

<owl:Class rdf:about="&obo;FOODON_03400463">
	<rdfs:label xml:lang="en">salts and spices, soups, sauces and salads, protein products etc. (ciaa)</rdfs:label>
	<rdfs:subClassOf rdf:resource="&obo;FOODON_03400357"/>
	<obo:IAO_0000412>http://langual.org</obo:IAO_0000412>
	<obo:IAO_0000115 xml:lang="en">CIAA ADD/385/90E Rev 5</obo:IAO_0000115>
	<obo:IAO_0000114 rdf:resource="&obo;IAO_0000428"/>
	<oboInOwl:hasDbXref>LANGUAL:A0463</oboInOwl:hasDbXref>
</owl:Class>

<owl:Class rdf:about="&obo;FOODON_03400464">
	<rdfs:label xml:lang="en">foodstuffs intended for particular nutritional uses (ciaa)</rdfs:label>
	<rdfs:subClassOf rdf:resource="&obo;FOODON_03400357"/>
	<obo:IAO_0000412>http://langual.org</obo:IAO_0000412>
	<obo:IAO_0000115 xml:lang="en">CIAA ADD/385/90E Rev 5</obo:IAO_0000115>
	<obo:IAO_0000114 rdf:resource="&obo;IAO_0000428"/>
	<oboInOwl:hasDbXref>LANGUAL:A0464</oboInOwl:hasDbXref>
</owl:Class>

<owl:Class rdf:about="&obo;FOODON_03400465">
	<rdfs:label xml:lang="en">beverages (ciaa)</rdfs:label>
	<rdfs:subClassOf rdf:resource="&obo;FOODON_03400357"/>
	<obo:IAO_0000412>http://langual.org</obo:IAO_0000412>
	<obo:IAO_0000115 xml:lang="en">CIAA ADD/385/90E Rev 5</obo:IAO_0000115>
	<obo:IAO_0000114 rdf:resource="&obo;IAO_0000428"/>
	<oboInOwl:hasDbXref>LANGUAL:A0465</oboInOwl:hasDbXref>
</owl:Class>

<owl:Class rdf:about="&obo;FOODON_03400466">
	<rdfs:label xml:lang="en">ready-to-eat savories (ciaa)</rdfs:label>
	<rdfs:subClassOf rdf:resource="&obo;FOODON_03400357"/>
	<obo:IAO_0000412>http://langual.org</obo:IAO_0000412>
	<obo:IAO_0000115 xml:lang="en">CIAA ADD/385/90E Rev 5</obo:IAO_0000115>
	<obo:IAO_0000114 rdf:resource="&obo;IAO_0000428"/>
	<oboInOwl:hasDbXref>LANGUAL:A0466</oboInOwl:hasDbXref>
</owl:Class>

<owl:Class rdf:about="&obo;FOODON_03400467">
	<rdfs:label xml:lang="en">other foods (ciaa)</rdfs:label>
	<rdfs:subClassOf rdf:resource="&obo;FOODON_03400357"/>
	<obo:IAO_0000412>http://langual.org</obo:IAO_0000412>
	<obo:IAO_0000115 xml:lang="en">CIAA ADD/385/90E Rev 5</obo:IAO_0000115>
	<obo:IAO_0000114 rdf:resource="&obo;IAO_0000428"/>
	<oboInOwl:hasDbXref>LANGUAL:A0467</oboInOwl:hasDbXref>
</owl:Class>

<owl:Class rdf:about="&obo;FOODON_03400626">
	<rdfs:label xml:lang="en">dairy products, excluding fats and oils, fat emulsions (ccfac)</rdfs:label>
	<rdfs:subClassOf rdf:resource="&obo;FOODON_03400355"/>
	<obo:IAO_0000412>http://langual.org</obo:IAO_0000412>
	<obo:IAO_0000115 xml:lang="en">CL 1996/14-FAC, May 1996</obo:IAO_0000115>
	<obo:IAO_0000114 rdf:resource="&obo;IAO_0000428"/>
	<oboInOwl:hasDbXref>LANGUAL:A0626</oboInOwl:hasDbXref>
</owl:Class>

<owl:Class rdf:about="&obo;FOODON_03400627">
	<rdfs:label xml:lang="en">fats and oils, and fat emulsions (type water-in-oil) (ccfac)</rdfs:label>
	<rdfs:subClassOf rdf:resource="&obo;FOODON_03400355"/>
	<obo:IAO_0000412>http://langual.org</obo:IAO_0000412>
	<obo:IAO_0000115 xml:lang="en">CL 1996/14-FAC, May 1996</obo:IAO_0000115>
	<obo:IAO_0000114 rdf:resource="&obo;IAO_0000428"/>
	<oboInOwl:hasDbXref>LANGUAL:A0627</oboInOwl:hasDbXref>
</owl:Class>

<owl:Class rdf:about="&obo;FOODON_03400628">
	<rdfs:label xml:lang="en">edible ices, including sherbet and sorbet (ccfac)</rdfs:label>
	<rdfs:subClassOf rdf:resource="&obo;FOODON_03400355"/>
	<obo:IAO_0000412>http://langual.org</obo:IAO_0000412>
	<obo:IAO_0000115 xml:lang="en">CL 1996/14-FAC, May 1996</obo:IAO_0000115>
	<obo:IAO_0000114 rdf:resource="&obo;IAO_0000428"/>
	<oboInOwl:hasDbXref>LANGUAL:A0628</oboInOwl:hasDbXref>
</owl:Class>

<owl:Class rdf:about="&obo;FOODON_03400629">
	<rdfs:label xml:lang="en">fruits and vegetables (ccfac)</rdfs:label>
	<rdfs:subClassOf rdf:resource="&obo;FOODON_03400355"/>
	<obo:IAO_0000412>http://langual.org</obo:IAO_0000412>
	<obo:IAO_0000115 xml:lang="en">CL 1996/14-FAC, May 1996</obo:IAO_0000115>
	<obo:IAO_0000114 rdf:resource="&obo;IAO_0000428"/>
	<oboInOwl:hasDbXref>LANGUAL:A0629</oboInOwl:hasDbXref>
</owl:Class>

<owl:Class rdf:about="&obo;FOODON_03400630">
	<rdfs:label xml:lang="en">confectionary (ccfac)</rdfs:label>
	<rdfs:subClassOf rdf:resource="&obo;FOODON_03400355"/>
	<obo:IAO_0000412>http://langual.org</obo:IAO_0000412>
	<obo:IAO_0000115 xml:lang="en">CL 1996/14-FAC, May 1996</obo:IAO_0000115>
	<obo:IAO_0000114 rdf:resource="&obo;IAO_0000428"/>
	<oboInOwl:hasDbXref>LANGUAL:A0630</oboInOwl:hasDbXref>
</owl:Class>

<owl:Class rdf:about="&obo;FOODON_03400631">
	<rdfs:label xml:lang="en">cereals and cereal products (ccfac)</rdfs:label>
	<rdfs:subClassOf rdf:resource="&obo;FOODON_03400355"/>
	<obo:IAO_0000412>http://langual.org</obo:IAO_0000412>
	<obo:IAO_0000115 xml:lang="en">CL 1996/14-FAC, May 1996</obo:IAO_0000115>
	<obo:IAO_0000114 rdf:resource="&obo;IAO_0000428"/>
	<oboInOwl:hasDbXref>LANGUAL:A0631</oboInOwl:hasDbXref>
</owl:Class>

<owl:Class rdf:about="&obo;FOODON_03400632">
	<rdfs:label xml:lang="en">bakery wares (ccfac)</rdfs:label>
	<rdfs:subClassOf rdf:resource="&obo;FOODON_03400355"/>
	<obo:IAO_0000412>http://langual.org</obo:IAO_0000412>
	<obo:IAO_0000115 xml:lang="en">CL 1996/14-FAC, May 1996</obo:IAO_0000115>
	<obo:IAO_0000114 rdf:resource="&obo;IAO_0000428"/>
	<oboInOwl:hasDbXref>LANGUAL:A0632</oboInOwl:hasDbXref>
</owl:Class>

<owl:Class rdf:about="&obo;FOODON_03400633">
	<rdfs:label xml:lang="en">meat and meat products (ccfac)</rdfs:label>
	<rdfs:subClassOf rdf:resource="&obo;FOODON_03400355"/>
	<obo:IAO_0000412>http://langual.org</obo:IAO_0000412>
	<obo:IAO_0000115 xml:lang="en">CL 1996/14-FAC, May 1996</obo:IAO_0000115>
	<obo:IAO_0000114 rdf:resource="&obo;IAO_0000428"/>
	<oboInOwl:hasDbXref>LANGUAL:A0633</oboInOwl:hasDbXref>
</owl:Class>

<owl:Class rdf:about="&obo;FOODON_03400634">
	<rdfs:label xml:lang="en">fish and fish products (ccfac)</rdfs:label>
	<rdfs:subClassOf rdf:resource="&obo;FOODON_03400355"/>
	<obo:IAO_0000412>http://langual.org</obo:IAO_0000412>
	<obo:IAO_0000115 xml:lang="en">CL 1996/14-FAC, May 1996</obo:IAO_0000115>
	<obo:IAO_0000114 rdf:resource="&obo;IAO_0000428"/>
	<oboInOwl:hasDbXref>LANGUAL:A0634</oboInOwl:hasDbXref>
</owl:Class>

<owl:Class rdf:about="&obo;FOODON_03400635">
	<rdfs:label xml:lang="en">egg and egg products (ccfac)</rdfs:label>
	<rdfs:subClassOf rdf:resource="&obo;FOODON_03400355"/>
	<obo:IAO_0000412>http://langual.org</obo:IAO_0000412>
	<obo:IAO_0000115 xml:lang="en">CL 1996/14-FAC, May 1996</obo:IAO_0000115>
	<obo:IAO_0000114 rdf:resource="&obo;IAO_0000428"/>
	<oboInOwl:hasDbXref>LANGUAL:A0635</oboInOwl:hasDbXref>
</owl:Class>

<owl:Class rdf:about="&obo;FOODON_03400636">
	<rdfs:label xml:lang="en">sweeteners (ccfac)</rdfs:label>
	<rdfs:subClassOf rdf:resource="&obo;FOODON_03400355"/>
	<obo:IAO_0000412>http://langual.org</obo:IAO_0000412>
	<obo:IAO_0000115 xml:lang="en">CL 1996/14-FAC, May 1996</obo:IAO_0000115>
	<obo:IAO_0000114 rdf:resource="&obo;IAO_0000428"/>
	<oboInOwl:hasDbXref>LANGUAL:A0636</oboInOwl:hasDbXref>
</owl:Class>

<owl:Class rdf:about="&obo;FOODON_03400637">
	<rdfs:label xml:lang="en">salts and spices, soups, sauces and salads, protein products etc. (ccfac)</rdfs:label>
	<rdfs:subClassOf rdf:resource="&obo;FOODON_03400355"/>
	<obo:IAO_0000412>http://langual.org</obo:IAO_0000412>
	<obo:IAO_0000115 xml:lang="en">CL 1996/14-FAC, May 1996</obo:IAO_0000115>
	<obo:IAO_0000114 rdf:resource="&obo;IAO_0000428"/>
	<oboInOwl:hasDbXref>LANGUAL:A0637</oboInOwl:hasDbXref>
</owl:Class>

<owl:Class rdf:about="&obo;FOODON_03400638">
	<rdfs:label xml:lang="en">foodstuffs intended for particular nutritional uses (ccfac)</rdfs:label>
	<rdfs:subClassOf rdf:resource="&obo;FOODON_03400355"/>
	<obo:IAO_0000412>http://langual.org</obo:IAO_0000412>
	<obo:IAO_0000115 xml:lang="en">CL 1996/14-FAC, May 1996</obo:IAO_0000115>
	<obo:IAO_0000114 rdf:resource="&obo;IAO_0000428"/>
	<oboInOwl:hasDbXref>LANGUAL:A0638</oboInOwl:hasDbXref>
</owl:Class>

<owl:Class rdf:about="&obo;FOODON_03400639">
	<rdfs:label xml:lang="en">beverages, excluding dairy products (ccfac)</rdfs:label>
	<rdfs:subClassOf rdf:resource="&obo;FOODON_03400355"/>
	<obo:IAO_0000412>http://langual.org</obo:IAO_0000412>
	<obo:IAO_0000115 xml:lang="en">CL 1996/14-FAC, May 1996</obo:IAO_0000115>
	<obo:IAO_0000114 rdf:resource="&obo;IAO_0000428"/>
	<oboInOwl:hasDbXref>LANGUAL:A0639</oboInOwl:hasDbXref>
</owl:Class>

<owl:Class rdf:about="&obo;FOODON_03400640">
	<rdfs:label xml:lang="en">ready-to-eat savories (ccfac)</rdfs:label>
	<rdfs:subClassOf rdf:resource="&obo;FOODON_03400355"/>
	<obo:IAO_0000412>http://langual.org</obo:IAO_0000412>
	<obo:IAO_0000115 xml:lang="en">CL 1996/14-FAC, May 1996</obo:IAO_0000115>
	<obo:IAO_0000114 rdf:resource="&obo;IAO_0000428"/>
	<oboInOwl:hasDbXref>LANGUAL:A0640</oboInOwl:hasDbXref>
</owl:Class>

<owl:Class rdf:about="&obo;FOODON_03400641">
	<rdfs:label xml:lang="en">composite foods (ccfac)</rdfs:label>
	<rdfs:subClassOf rdf:resource="&obo;FOODON_03400355"/>
	<obo:IAO_0000412>http://langual.org</obo:IAO_0000412>
	<obo:IAO_0000115 xml:lang="en">CL 1996/14-FAC, May 1996</obo:IAO_0000115>
	<obo:IAO_0000114 rdf:resource="&obo;IAO_0000428"/>
	<oboInOwl:hasDbXref>LANGUAL:A0641</oboInOwl:hasDbXref>
</owl:Class>

<owl:Class rdf:about="&obo;FOODON_03400642">
	<rdfs:label xml:lang="en">eurocode 2 food classification</rdfs:label>
	<rdfs:subClassOf rdf:resource="&obo;FOODON_03400356"/>
	<obo:IAO_0000412>http://langual.org</obo:IAO_0000412>
	<obo:IAO_0000114 rdf:resource="&obo;IAO_0000428"/>
	<rdfs:comment xml:lang="en">LanguaL curation note: This term is for CLASSIFICATION ONLY; DO NOT USE term in indexing. Use a more precise narrower term.</rdfs:comment>
	<oboInOwl:hasDbXref>LANGUAL:A0642</oboInOwl:hasDbXref>
</owl:Class>

<owl:Class rdf:about="&obo;FOODON_03400643">
	<rdfs:label xml:lang="en">classification of food and feed commodities (codex alimentarius)</rdfs:label>
	<rdfs:subClassOf rdf:resource="&obo;FOODON_03400352"/>
	<obo:IAO_0000412>http://langual.org</obo:IAO_0000412>
	<obo:IAO_0000115 xml:lang="en">Codex Alimentarius, Volume 2 - 1993, Section 2:  Pesticide Residues in Food.

The Codex Classification of food and animal feed commodities moving in trade and the description of the various items and groups of food and animal feedstuffs included in the present document have been developed by the Codex Committee on Pesticide Residues. It was first adopted by the 18th Session of the Codex Alimentarius Commission, (1989).

The Codex Classification includes food commodities and animal feedstuffs for which Codex maximum residue limits will not necessarily be established. The Classification is intended to be as complete a listing of food commodities in trade as possible, classified into groups on the basis of the commodity's similar potential for pesticide residues.

The Classification may also be appropriate for other purposes such as setting maximum levels for other types of residues or for other contaminants in food. The Codex Classification should be consulted in order to obtain a precise description of the food or animal feed commodities and, especially, in cases where Codex maximum residue limits have been set for groups of food and groups of animal feedstuffs. The Codex Classification is intended to promote harmonization of the terms used to describe commodities which are subject to maximum residue limits and of the approach to grouping commodities with similar potential for residue for which a common group maximum residue limit can be set.</obo:IAO_0000115>
	<obo:IAO_0000114 rdf:resource="&obo;IAO_0000428"/>
	<rdfs:comment xml:lang="en">LanguaL curation note: This term is for CLASSIFICATION ONLY; DO NOT USE term in indexing. Use a more precise narrower term.</rdfs:comment>
	<oboInOwl:hasDbXref>LANGUAL:A0643</oboInOwl:hasDbXref>
</owl:Class>

<owl:Class rdf:about="&obo;FOODON_03400644">
	<rdfs:label xml:lang="en">a.  primary food commodities of plant origin (ccpr)</rdfs:label>
	<rdfs:subClassOf rdf:resource="&obo;FOODON_03400643"/>
	<obo:IAO_0000412>http://langual.org</obo:IAO_0000412>
	<obo:IAO_0000114 rdf:resource="&obo;IAO_0000428"/>
	<rdfs:comment xml:lang="en">LanguaL curation note: This term is for CLASSIFICATION ONLY; DO NOT USE term in indexing. Use a more precise narrower term.</rdfs:comment>
	<oboInOwl:hasDbXref>LANGUAL:A0644</oboInOwl:hasDbXref>
</owl:Class>

<owl:Class rdf:about="&obo;FOODON_03400645">
	<rdfs:label xml:lang="en">b.  primary food commodities of animal origin (ccpr)</rdfs:label>
	<rdfs:subClassOf rdf:resource="&obo;FOODON_03400643"/>
	<obo:IAO_0000412>http://langual.org</obo:IAO_0000412>
	<obo:IAO_0000114 rdf:resource="&obo;IAO_0000428"/>
	<rdfs:comment xml:lang="en">LanguaL curation note: This term is for CLASSIFICATION ONLY; DO NOT USE term in indexing. Use a more precise narrower term.</rdfs:comment>
	<oboInOwl:hasDbXref>LANGUAL:A0645</oboInOwl:hasDbXref>
</owl:Class>

<owl:Class rdf:about="&obo;FOODON_03400646">
	<rdfs:label xml:lang="en">c.  primary feed commodities (ccpr)</rdfs:label>
	<rdfs:subClassOf rdf:resource="&obo;FOODON_03400643"/>
	<obo:IAO_0000412>http://langual.org</obo:IAO_0000412>
	<obo:IAO_0000115 xml:lang="en">Four the purpose of the Codex Alimentarius the term "primary feed commodity" means the product in or nearly in its natura1 state intended for sale to:

1.  the stock farmer as feed which is used without further processing for livestock animals or after silaging or similar farm processes;

2.  the animal feed industry as a raw material for preparing compounded feeds;</obo:IAO_0000115>
	<obo:IAO_0000114 rdf:resource="&obo;IAO_0000428"/>
	<rdfs:comment xml:lang="en">LanguaL curation note: This term is for CLASSIFICATION ONLY; DO NOT USE term in indexing. Use a more precise narrower term.</rdfs:comment>
	<oboInOwl:hasDbXref>LANGUAL:A0646</oboInOwl:hasDbXref>
</owl:Class>

<owl:Class rdf:about="&obo;FOODON_03400647">
	<rdfs:label xml:lang="en">d.  processed food of plant origin (ccpr)</rdfs:label>
	<rdfs:subClassOf rdf:resource="&obo;FOODON_03400643"/>
	<obo:IAO_0000412>http://langual.org</obo:IAO_0000412>
	<obo:IAO_0000114 rdf:resource="&obo;IAO_0000428"/>
	<rdfs:comment xml:lang="en">LanguaL curation note: This term is for CLASSIFICATION ONLY; DO NOT USE term in indexing. Use a more precise narrower term.</rdfs:comment>
	<oboInOwl:hasDbXref>LANGUAL:A0647</oboInOwl:hasDbXref>
</owl:Class>

<owl:Class rdf:about="&obo;FOODON_03400648">
	<rdfs:label xml:lang="en">e.  processed food of animal origin (ccpr)</rdfs:label>
	<rdfs:subClassOf rdf:resource="&obo;FOODON_03400643"/>
	<obo:IAO_0000412>http://langual.org</obo:IAO_0000412>
	<obo:IAO_0000114 rdf:resource="&obo;IAO_0000428"/>
	<rdfs:comment xml:lang="en">LanguaL curation note: This term is for CLASSIFICATION ONLY; DO NOT USE term in indexing. Use a more precise narrower term.</rdfs:comment>
	<oboInOwl:hasDbXref>LANGUAL:A0648</oboInOwl:hasDbXref>
</owl:Class>

<owl:Class rdf:about="&obo;FOODON_03400649">
	<rdfs:label xml:lang="en">01  fruits (ccpr)</rdfs:label>
	<rdfs:subClassOf rdf:resource="&obo;FOODON_03400644"/>
	<obo:IAO_0000412>http://langual.org</obo:IAO_0000412>
	<obo:IAO_0000115 xml:lang="en">Fruits are derived from many different kinds of perennial plants, trees and shrubs, usually cultivated. They consist mostly of the ripe, often sweet, succulent or pulpy developed plant ovary and its accessory parts, commonly and traditionally known as fruit.
Exposure to pesticides is dependent on the particular part of the fruit used for food. Fruits may be consumed whole, after the removal of the peel, or in part, and in the form of fresh, dried or processed products.</obo:IAO_0000115>
	<obo:IAO_0000114 rdf:resource="&obo;IAO_0000428"/>
	<oboInOwl:hasDbXref>LANGUAL:A0649</oboInOwl:hasDbXref>
</owl:Class>

<owl:Class rdf:about="&obo;FOODON_03400650">
	<rdfs:label xml:lang="en">02  vegetables (ccpr)</rdfs:label>
	<rdfs:subClassOf rdf:resource="&obo;FOODON_03400644"/>
	<obo:IAO_0000412>http://langual.org</obo:IAO_0000412>
	<obo:IAO_0000115 xml:lang="en">Vegetables are foods derived from many different kinds of plants mostly annual and usually cultivated, commonly known by custom and tradition as "vegetables".
In several countries, some of these commodities grown on large areas are distinguished as "field crops" or arable crops e.g. sugar beet. For the sake of convenience in this guide such crops are classified under Type 2 Vegetables.
Exposure to pesticides is dependent on the particular part of the plant used for food and the growing practices.
Vegetables may be consumed in whole or in part and in the form of fresh, dried or processed foods.</obo:IAO_0000115>
	<obo:IAO_0000114 rdf:resource="&obo;IAO_0000428"/>
	<oboInOwl:hasDbXref>LANGUAL:A0650</oboInOwl:hasDbXref>
</owl:Class>

<owl:Class rdf:about="&obo;FOODON_03400651">
	<rdfs:label xml:lang="en">03  grasses (ccpr)</rdfs:label>
	<rdfs:subClassOf rdf:resource="&obo;FOODON_03400644"/>
	<obo:IAO_0000412>http://langual.org</obo:IAO_0000412>
	<obo:IAO_0000115 xml:lang="en">TYPE 03 - GRASSES

Grasses are herbaceous annual and perennial monocotyledonous plants of different kinds, cultivated extensively for their ears (heads) of starchy seeds used directly for the production of food. Grasses used for animal feed are classified under Class C; Primary Animal feed commodities, Group 051.

The plants are fully exposed to pesticides applied during the growing season.</obo:IAO_0000115>
	<obo:IAO_0000114 rdf:resource="&obo;IAO_0000428"/>
	<oboInOwl:hasDbXref>LANGUAL:A0651</oboInOwl:hasDbXref>
</owl:Class>

<owl:Class rdf:about="&obo;FOODON_03400652">
	<rdfs:label xml:lang="en">04  nuts and seeds (ccpr)</rdfs:label>
	<rdfs:subClassOf rdf:resource="&obo;FOODON_03400644"/>
	<obo:IAO_0000412>http://langual.org</obo:IAO_0000412>
	<obo:IAO_0000115 xml:lang="en">TYPE 04  -  NUTS AND SEEDS

Nuts and seeds are derived from a large variety of trees, shrubs and herbaceous plants, mostly cultivated.

The mature seeds or nuts are used as human food, for the production of beverages or edible vegetable oils and for the production of seed meals and cakes for animal feed.</obo:IAO_0000115>
	<obo:IAO_0000114 rdf:resource="&obo;IAO_0000428"/>
	<oboInOwl:hasDbXref>LANGUAL:A0652</oboInOwl:hasDbXref>
</owl:Class>

<owl:Class rdf:about="&obo;FOODON_03400653">
	<rdfs:label xml:lang="en">05  herbs and spices (ccpr)</rdfs:label>
	<rdfs:subClassOf rdf:resource="&obo;FOODON_03400644"/>
	<obo:IAO_0000412>http://langual.org</obo:IAO_0000412>
	<obo:IAO_0000115 xml:lang="en">TYPE 05  -  HERBS AND SPICES

Herbs and spices are the flavoursome or aromatic leaves, stems, roots, flowers or fruits of a variety of plants used to impart special flavours to food and beverages.</obo:IAO_0000115>
	<obo:IAO_0000114 rdf:resource="&obo;IAO_0000428"/>
	<oboInOwl:hasDbXref>LANGUAL:A0653</oboInOwl:hasDbXref>
</owl:Class>

<owl:Class rdf:about="&obo;FOODON_03400654">
	<rdfs:label xml:lang="en">06  mammalian products (ccpr)</rdfs:label>
	<rdfs:subClassOf rdf:resource="&obo;FOODON_03400645"/>
	<obo:IAO_0000412>http://langual.org</obo:IAO_0000412>
	<obo:IAO_0000115 xml:lang="en">TYPE 06  -  MAMMALIAN PRODUCTS

Mammalian products are derived from the edible parts of various mammals, primarily herbivorous, slaughtered for food. These mammals are usually domesticated, or to a lesser extent obtained as game animals.

This type does not include edible products from marine mammals, for which see Group 044.</obo:IAO_0000115>
	<obo:IAO_0000114 rdf:resource="&obo;IAO_0000428"/>
	<oboInOwl:hasDbXref>LANGUAL:A0654</oboInOwl:hasDbXref>
</owl:Class>

<owl:Class rdf:about="&obo;FOODON_03400655">
	<rdfs:label xml:lang="en">07  poultry products (ccpr)</rdfs:label>
	<rdfs:subClassOf rdf:resource="&obo;FOODON_03400645"/>
	<obo:IAO_0000412>http://langual.org</obo:IAO_0000412>
	<obo:IAO_0000114 rdf:resource="&obo;IAO_0000428"/>
	<oboInOwl:hasDbXref>LANGUAL:A0655</oboInOwl:hasDbXref>
</owl:Class>

<owl:Class rdf:about="&obo;FOODON_03400656">
	<rdfs:label xml:lang="en">08  aquatic animal products (ccpr)</rdfs:label>
	<rdfs:subClassOf rdf:resource="&obo;FOODON_03400645"/>
	<obo:IAO_0000412>http://langual.org</obo:IAO_0000412>
	<obo:IAO_0000115 xml:lang="en">Type 08  -  Aquatic animal products

Aquatic animal products are derived from the edible parts of various aquatic animals, usually wild, harvested for food.</obo:IAO_0000115>
	<obo:IAO_0000114 rdf:resource="&obo;IAO_0000428"/>
	<oboInOwl:hasDbXref>LANGUAL:A0656</oboInOwl:hasDbXref>
</owl:Class>

<owl:Class rdf:about="&obo;FOODON_03400657">
	<rdfs:label xml:lang="en">09  amphibians and reptiles (ccpr)</rdfs:label>
	<rdfs:subClassOf rdf:resource="&obo;FOODON_03400645"/>
	<obo:IAO_0000412>http://langual.org</obo:IAO_0000412>
	<obo:IAO_0000114 rdf:resource="&obo;IAO_0000428"/>
	<oboInOwl:hasDbXref>LANGUAL:A0657</oboInOwl:hasDbXref>
</owl:Class>

<owl:Class rdf:about="&obo;FOODON_03400658">
	<rdfs:label xml:lang="en">10  invertebrate animals (ccpr)</rdfs:label>
	<rdfs:subClassOf rdf:resource="&obo;FOODON_03400645"/>
	<obo:IAO_0000412>http://langual.org</obo:IAO_0000412>
	<obo:IAO_0000114 rdf:resource="&obo;IAO_0000428"/>
	<oboInOwl:hasDbXref>LANGUAL:A0658</oboInOwl:hasDbXref>
</owl:Class>

<owl:Class rdf:about="&obo;FOODON_03400659">
	<rdfs:label xml:lang="en">11  primary food commodities of plant origin (ccpr)</rdfs:label>
	<rdfs:subClassOf rdf:resource="&obo;FOODON_03400646"/>
	<obo:IAO_0000412>http://langual.org</obo:IAO_0000412>
	<obo:IAO_0000115 xml:lang="en">Type 11  -  Primary feed commodities of plant origin

The primary feed commodities of plant origin include products after removal of certain parts of the plants.

Some types of the primary feed commodities are grown and used exclusively for animal feeding purposes, e.g. alfalfa vetch and maize forage. Other types are derived from crops of which the edible parts are used directly or after processing as food, whereas the "waste" parts of these crops are generally used for feeding purposes, e.g. cereal straws, pea vines (fresh = green), pea hay, maize fodder, sugar beet tops or -leaves.</obo:IAO_0000115>
	<obo:IAO_0000114 rdf:resource="&obo;IAO_0000428"/>
	<oboInOwl:hasDbXref>LANGUAL:A0659</oboInOwl:hasDbXref>
</owl:Class>

<owl:Class rdf:about="&obo;FOODON_03400660">
	<rdfs:label xml:lang="en">12  secondary food commodities of plant origin (ccpr)</rdfs:label>
	<rdfs:subClassOf rdf:resource="&obo;FOODON_03400647"/>
	<obo:IAO_0000412>http://langual.org</obo:IAO_0000412>
	<obo:IAO_0000115 xml:lang="en">The term "secondary food commodity" means a "primary food commodity" which has undergone simple processing, such as removal of certain portions, drying (except natural drying), husking, and comminution, which do not basically alter the composition or identity of the product. Natural field dried mature crops or parts of crops such as pulses, bulb onions or cereal grains are not considered as secondary food commodities.

Secondary food commodities may be processed further or used as ingredients in the manufacture of food or sold directly to the consumer.</obo:IAO_0000115>
	<obo:IAO_0000114 rdf:resource="&obo;IAO_0000428"/>
	<oboInOwl:hasDbXref>LANGUAL:A0660</oboInOwl:hasDbXref>
</owl:Class>

<owl:Class rdf:about="&obo;FOODON_03400661">
	<rdfs:label xml:lang="en">13  derived products of plant origin (ccpr)</rdfs:label>
	<rdfs:subClassOf rdf:resource="&obo;FOODON_03400647"/>
	<obo:IAO_0000412>http://langual.org</obo:IAO_0000412>
	<obo:IAO_0000115 xml:lang="en">Type 13  -  Derived edible products of plant origin

"Derived edible products" are foods or edible substances isolated from primary food commodities or raw agricultural commodities, not intended for human consumption as such, using physical, biological or chemical processing.

This type of processed food includes groups such as vegetable oils (crude and refined), by-products of the fractionation of cereals fruit juices, teas (fermented and dried), cocoa powder and by-products of cocoa manufacturing, and extracts of various plants.</obo:IAO_0000115>
	<obo:IAO_0000114 rdf:resource="&obo;IAO_0000428"/>
	<oboInOwl:hasDbXref>LANGUAL:A0661</oboInOwl:hasDbXref>
</owl:Class>

<owl:Class rdf:about="&obo;FOODON_03400662">
	<rdfs:label xml:lang="en">14  manufactured foods (single ingredient) of plant origin (ccpr)</rdfs:label>
	<rdfs:subClassOf rdf:resource="&obo;FOODON_03400647"/>
	<obo:IAO_0000412>http://langual.org</obo:IAO_0000412>
	<obo:IAO_0000115 xml:lang="en">Type 14 - Manufactured Foods (single-ingredient) of plant origin

The term "single-ingredient manufactured food" means a "processed food" which consists of one identifiable food ingredient, with or without packing medium or minor ingredients, such as flavouring agents, spices and condiments, and which is normally pre-packaged and ready for consumption with or without cooking.</obo:IAO_0000115>
	<obo:IAO_0000114 rdf:resource="&obo;IAO_0000428"/>
	<oboInOwl:hasDbXref>LANGUAL:A0662</oboInOwl:hasDbXref>
</owl:Class>

<owl:Class rdf:about="&obo;FOODON_03400663">
	<rdfs:label xml:lang="en">15  manufactured foods (multi-ingredient) of plant origin (ccpr)</rdfs:label>
	<rdfs:subClassOf rdf:resource="&obo;FOODON_03400647"/>
	<obo:IAO_0000412>http://langual.org</obo:IAO_0000412>
	<obo:IAO_0000115 xml:lang="en">The term "multi-ingredient manufactured food" means a processed food, consisting of more than one major ingredient.

A multi-ingredient food consisting of ingredients of both plant and animal origin will be included in this type if the ingredient(s) of plant origin is (are) predominant.</obo:IAO_0000115>
	<obo:IAO_0000114 rdf:resource="&obo;IAO_0000428"/>
	<oboInOwl:hasDbXref>LANGUAL:A0663</oboInOwl:hasDbXref>
</owl:Class>

<owl:Class rdf:about="&obo;FOODON_03400664">
	<rdfs:label xml:lang="en">16  secondary food commodities of animal origin (ccpr)</rdfs:label>
	<rdfs:subClassOf rdf:resource="&obo;FOODON_03400648"/>
	<obo:IAO_0000412>http://langual.org</obo:IAO_0000412>
	<obo:IAO_0000115 xml:lang="en">Type 16 - Secondary food commodities of animal origin

The term "secondary food commodity" means a "primary food commodity" which has undergone simple processing, such as removal of certain portions, drying, and comminution, which do not basically alter the composition or identity of the commodity.

Secondary food commodities may be processed further, or used as ingredients in the manufacture of food, or sold directly to the consumer.

This type of processed food includes groups of processed primary food commodities of animal origin which have undergone simple processing, such as processed mammalian meat and poultry meat, fishes and other aquatic animals, e.g. dried meat, dried fish.</obo:IAO_0000115>
	<obo:IAO_0000114 rdf:resource="&obo;IAO_0000428"/>
	<oboInOwl:hasDbXref>LANGUAL:A0664</oboInOwl:hasDbXref>
</owl:Class>

<owl:Class rdf:about="&obo;FOODON_03400665">
	<rdfs:label xml:lang="en">17  derived edible products of animal origin (ccpr)</rdfs:label>
	<rdfs:subClassOf rdf:resource="&obo;FOODON_03400648"/>
	<obo:IAO_0000412>http://langual.org</obo:IAO_0000412>
	<obo:IAO_0000115 xml:lang="en">Type 17 - Derived edible products of animal origin

The term "Derived edible products" means foods or edible substances isolated from primary food commodities or raw agricultural commodities not intended for human consumption as such, using physical, biological and chemical processes.

This type includes processed (rendered or extracted, possibly refined and/or clarified) fats from mammals, including aquatic mammals, poultry and aquatic organisms such as fishes</obo:IAO_0000115>
	<obo:IAO_0000114 rdf:resource="&obo;IAO_0000428"/>
	<oboInOwl:hasDbXref>LANGUAL:A0665</oboInOwl:hasDbXref>
</owl:Class>

<owl:Class rdf:about="&obo;FOODON_03400666">
	<rdfs:label xml:lang="en">18  manufactured food (single-ingredient) of animal origin (ccpr)</rdfs:label>
	<rdfs:subClassOf rdf:resource="&obo;FOODON_03400648"/>
	<obo:IAO_0000412>http://langual.org</obo:IAO_0000412>
	<obo:IAO_0000115 xml:lang="en">The term "single ingredient manufactured food" means a processed food which consists of one identifiable food ingredient, with or without packing medium or minor ingredients such as flavouring agents, spices and condiments, and which is normally pre-packaged and ready for consumption, with or without cooking.</obo:IAO_0000115>
	<obo:IAO_0000114 rdf:resource="&obo;IAO_0000428"/>
	<oboInOwl:hasDbXref>LANGUAL:A0666</oboInOwl:hasDbXref>
</owl:Class>

<owl:Class rdf:about="&obo;FOODON_03400667">
	<rdfs:label xml:lang="en">19  manufactured food (multi-ingredient) of animal origin (ccpr)</rdfs:label>
	<rdfs:subClassOf rdf:resource="&obo;FOODON_03400648"/>
	<obo:IAO_0000412>http://langual.org</obo:IAO_0000412>
	<obo:IAO_0000115 xml:lang="en">19  Manufactured food (multi-ingredient) of animal origin

The term "multi-ingredient manufactured food" means a processed food consisting of more than one major ingredient.
A multi-ingredient food consisting of ingredients of both animal and plant origin will be included in this type if the ingredient(s) of animal origin is (are) predominant</obo:IAO_0000115>
	<obo:IAO_0000114 rdf:resource="&obo;IAO_0000428"/>
	<oboInOwl:hasDbXref>LANGUAL:A0667</oboInOwl:hasDbXref>
</owl:Class>

<owl:Class rdf:about="&obo;FOODON_03400668">
	<rdfs:label xml:lang="en">001  citrus fruits (fc) (ccpr)</rdfs:label>
	<rdfs:subClassOf rdf:resource="&obo;FOODON_03400649"/>
	<obo:IAO_0000412>http://langual.org</obo:IAO_0000412>
	<obo:IAO_0000115 xml:lang="en">Citrus fruits are produced on trees or shrubs of the family Rutaceae. These fruits are characterized by aromatic oily peel, globular form and interior segments of juice-filled vesicles. The fruit is fully exposed to pesticides during the growing season. Post-harvest treatments with pesticides and liquid waxes are often carried out to avoid deterioration during transport and distribution due to fungal diseases, insect pests or loss of moisture.
The fruit pulp may be consumed in succulent form and as a juice. The entire fruit may be used for preserves.</obo:IAO_0000115>
	<obo:IAO_0000114 rdf:resource="&obo;IAO_0000428"/>
	<oboInOwl:hasDbXref>LANGUAL:A0668</oboInOwl:hasDbXref>
</owl:Class>

<owl:Class rdf:about="&obo;FOODON_03400669">
	<rdfs:label xml:lang="en">002  pome fruits (fp) (ccpr)</rdfs:label>
	<rdfs:subClassOf rdf:resource="&obo;FOODON_03400649"/>
	<obo:IAO_0000412>http://langual.org</obo:IAO_0000412>
	<obo:IAO_0000115 xml:lang="en">Pome fruits are produced on trees and shrubs belonging to certain genera of the rose family (Rosaceae), especially the genera Malus and Pyrus. They are characterized by fleshy tissue surrounding a core consisting of parchment-like carpels enclosing the seeds.
Pome fruits are fully exposed to pesticides applied during the growing season. Post-harvest treatments directly after harvest may also occur. The entire fruit, except the core, may be consumed in the succulent form or after processing.</obo:IAO_0000115>
	<obo:IAO_0000114 rdf:resource="&obo;IAO_0000428"/>
	<oboInOwl:hasDbXref>LANGUAL:A0669</oboInOwl:hasDbXref>
</owl:Class>

<owl:Class rdf:about="&obo;FOODON_03400670">
	<rdfs:label xml:lang="en">003  stone fruits (fs) (ccpr)</rdfs:label>
	<rdfs:subClassOf rdf:resource="&obo;FOODON_03400649"/>
	<obo:IAO_0000412>http://langual.org</obo:IAO_0000412>
	<obo:IAO_0000115 xml:lang="en">Stone fruits are produced on trees belonging to the genus Prunus of the rose family (Rosaceae). They are characterized by fleshy tissue surrounding a single hard shelled seed. The fruit is fully exposed to pesticides applied during the growing season (fruit setting until harvest). Dipping of fruit immediately after harvest, especially with fungicides, may also occur.
The entire fruit, except the seed, may be consumed in a succulent or processed form.</obo:IAO_0000115>
	<obo:IAO_0000114 rdf:resource="&obo;IAO_0000428"/>
	<oboInOwl:hasDbXref>LANGUAL:A0670</oboInOwl:hasDbXref>
</owl:Class>

<owl:Class rdf:about="&obo;FOODON_03400671">
	<rdfs:label xml:lang="en">004  berries and other small fruits (fb) (ccpr)</rdfs:label>
	<rdfs:subClassOf rdf:resource="&obo;FOODON_03400649"/>
	<obo:IAO_0000412>http://langual.org</obo:IAO_0000412>
	<obo:IAO_0000115 xml:lang="en">Berries and other small fruits are derived from a variety of perennial plants and shrubs having fruit characterized by a high surface: weight ratio. The fruits are fully exposed to pesticides applied during the growing season (blossoming until harvest).
The entire fruit, often including seed, may be consumed in a succulent or processed form.</obo:IAO_0000115>
	<obo:IAO_0000114 rdf:resource="&obo;IAO_0000428"/>
	<oboInOwl:hasDbXref>LANGUAL:A0671</oboInOwl:hasDbXref>
</owl:Class>

<owl:Class rdf:about="&obo;FOODON_03400672">
	<rdfs:label xml:lang="en">005  assorted tropical and sub-tropical fruit - edible peel (ft) (ccpr)</rdfs:label>
	<rdfs:subClassOf rdf:resource="&obo;FOODON_03400649"/>
	<obo:IAO_0000412>http://langual.org</obo:IAO_0000412>
	<obo:IAO_0000115 xml:lang="en">The assorted tropical and sub-tropical fruits - edible peel are derived from the immature or mature fruits of a large variety of perennial plants, usually shrubs or trees. The fruits are fully exposed to pesticides during the growing season (period of fruit development).
The whole fruit may be consumed in a succulent or processed form.</obo:IAO_0000115>
	<obo:IAO_0000114 rdf:resource="&obo;IAO_0000428"/>
	<oboInOwl:hasDbXref>LANGUAL:A0672</oboInOwl:hasDbXref>
</owl:Class>

<owl:Class rdf:about="&obo;FOODON_03400673">
	<rdfs:label xml:lang="en">006  assorted tropical and sub-tropical fruit - inedible peel (fi) (ccpr)</rdfs:label>
	<rdfs:subClassOf rdf:resource="&obo;FOODON_03400649"/>
	<obo:IAO_0000412>http://langual.org</obo:IAO_0000412>
	<obo:IAO_0000115 xml:lang="en">The assorted tropical and sub-tropical fruits - inedible peel are derived from the immature or mature fruits of a large variety of perennial plants, usually shrubs or trees. Fruits are fully exposed to pesticides applied during the growing season (period of fruit development) but the edible portion is protected by skin, peel or husk. The edible part of the fruits may be consumed in a fresh or processed form.</obo:IAO_0000115>
	<obo:IAO_0000114 rdf:resource="&obo;IAO_0000428"/>
	<oboInOwl:hasDbXref>LANGUAL:A0673</oboInOwl:hasDbXref>
</owl:Class>

<owl:Class rdf:about="&obo;FOODON_03400674">
	<rdfs:label xml:lang="en">009  bulb vegetables (va) (ccpr)</rdfs:label>
	<rdfs:subClassOf rdf:resource="&obo;FOODON_03400650"/>
	<obo:IAO_0000412>http://langual.org</obo:IAO_0000412>
	<obo:IAO_0000115 xml:lang="en">Bulb vegetables are pungent highly flavoured foods derived from fleshy scale bulbs in some commodities including stem and leaves, of the genus Allium of the lily family (Lilaceae). Bulb fennel is included in this group; the bulb-like growth of this commodity gives rise to similar residues.
The subterranean parts of the bulbs and shoots are protected from direct exposure to pesticides during the growing season.
The entire bulb may be consumed after removal of the parchment-like skin. The leaves and stems of some species or cultivars may also be consumed.</obo:IAO_0000115>
	<obo:IAO_0000114 rdf:resource="&obo;IAO_0000428"/>
	<oboInOwl:hasDbXref>LANGUAL:A0674</oboInOwl:hasDbXref>
</owl:Class>

<owl:Class rdf:about="&obo;FOODON_03400675">
	<rdfs:label xml:lang="en">010  brassica (cole or cabbage) vegetables, head cabbage, flowerhead brassicas (vb) (ccpr)</rdfs:label>
	<rdfs:subClassOf rdf:resource="&obo;FOODON_03400650"/>
	<obo:IAO_0000412>http://langual.org</obo:IAO_0000412>
	<obo:IAO_0000115 xml:lang="en">Brassica (cole or cabbage) vegetables and flowerhead brassicas are foods derived from the leafy heads, stems and immature inflorescences of plants belonging to the genus Brassica or the family Cruciferae. Although Kohlrabi does not comply fully with the description above, for convenience and because of the similarity in residue behaviour the commodity is classified in this group. Koblrabi is a tuber-like enlargement of the stem.
The edible part of the crop is partly protected from pesticides applied during the growing season by outer leaves, or skin (Kohlrabi).
The entire vegetable after discarding obviously decomposed or withered leaves may be consumed.</obo:IAO_0000115>
	<obo:IAO_0000114 rdf:resource="&obo;IAO_0000428"/>
	<oboInOwl:hasDbXref>LANGUAL:A0675</oboInOwl:hasDbXref>
</owl:Class>

<owl:Class rdf:about="&obo;FOODON_03400676">
	<rdfs:label xml:lang="en">011 fruiting vegetables, cucurbits (vc) (ccpr)</rdfs:label>
	<rdfs:subClassOf rdf:resource="&obo;FOODON_03400650"/>
	<obo:IAO_0000412>http://langual.org</obo:IAO_0000412>
	<obo:IAO_0000115 xml:lang="en">Fruiting vegetables, Cucurbits are derived from the immature or mature fruits of various plants, belonging to the botanical family Cucurbitaceae; usually these are annual vines or bushes.
These vegetables are fully exposed to pesticides during the period of fruit development.
The edible portion of those fruits of which the inedible peel is discarded before consumption is protected from most pesticides, by the skin or peel, except from pesticides with a systemic action.
The entire fruiting vegetables or the edible portion after discarding the inedible peel may be consumed in the fresh form or after processing.The entire immature fruit of some of the fruiting vegetables species may be consumed, whereas only the edible portion of the mature fruit of the same species, after discarding the then inedible peel, is consumed.</obo:IAO_0000115>
	<obo:IAO_0000114 rdf:resource="&obo;IAO_0000428"/>
	<oboInOwl:hasDbXref>LANGUAL:A0676</oboInOwl:hasDbXref>
</owl:Class>

<owl:Class rdf:about="&obo;FOODON_03400677">
	<rdfs:label xml:lang="en">012  fruiting vegetables, other than cucurbits (vo) (ccpr)</rdfs:label>
	<rdfs:subClassOf rdf:resource="&obo;FOODON_03400650"/>
	<obo:IAO_0000412>http://langual.org</obo:IAO_0000412>
	<obo:IAO_0000115 xml:lang="en">Fruiting vegetables, other than Cucurbits are derived from the immature and mature fruits of various plants, usually annual vines or bushes. The group includes edible fungi and mushrooms, being comparable organs of lower plants. Many plants of this group belong to the botanical family Solanaceae.
This group does not include fruits of vegetables of the botanical family Cucurbitaceae or the pods of vegetables of the Leguminosae-family.
The vegetables of this group are fully exposed to pesticides applied during the period of fruit development, except those of which the edible portion is covered by husks, such as sweet corn, ground cherries (Physalis spp.). The latter fruiting vegetables are protected from most pesticides by the husk except from pesticides with a systemic action.
The entire fruiting vegetable or the edible portion after discarding husks or peels may be consumed in a fresh form or after processing.</obo:IAO_0000115>
	<obo:IAO_0000114 rdf:resource="&obo;IAO_0000428"/>
	<oboInOwl:hasDbXref>LANGUAL:A0677</oboInOwl:hasDbXref>
</owl:Class>

<owl:Class rdf:about="&obo;FOODON_03400678">
	<rdfs:label xml:lang="en">013  leafy vegetables (including brassica leafy vegetables) (vl) (ccpr)</rdfs:label>
	<rdfs:subClassOf rdf:resource="&obo;FOODON_03400650"/>
	<obo:IAO_0000412>http://langual.org</obo:IAO_0000412>
	<obo:IAO_0000115 xml:lang="en">Leafy vegetables are foods derived from the leaves of a wide variety of edible plants, usually annuals or biennials. They are characterized by a high surface:weight ratio. The leaves are fully exposed to pesticides applied during the growing season.
The entire leaf may be consumed, either fresh or after processing or household cooking.</obo:IAO_0000115>
	<obo:IAO_0000114 rdf:resource="&obo;IAO_0000428"/>
	<oboInOwl:hasDbXref>LANGUAL:A0678</oboInOwl:hasDbXref>
</owl:Class>

<owl:Class rdf:about="&obo;FOODON_03400679">
	<rdfs:label xml:lang="en">014  legume vegetables (vp) (ccpr)</rdfs:label>
	<rdfs:subClassOf rdf:resource="&obo;FOODON_03400650"/>
	<obo:IAO_0000412>http://langual.org</obo:IAO_0000412>
	<obo:IAO_0000115 xml:lang="en">Legume vegetables are derived from the succulent seed and immature pods of leguminous plants commonly known as beans and peas.
Pods are fully exposed to pesticides during the growing season, whereas the succulent seed is protected within the pod from most pesticides, except pesticides with systemic action.
The succulent forms may be consumed as whole pods or as the shelled product.</obo:IAO_0000115>
	<obo:IAO_0000114 rdf:resource="&obo;IAO_0000428"/>
	<oboInOwl:hasDbXref>LANGUAL:A0679</oboInOwl:hasDbXref>
</owl:Class>

<owl:Class rdf:about="&obo;FOODON_03400680">
	<rdfs:label xml:lang="en">015  pulses (vd) (ccpr)</rdfs:label>
	<rdfs:subClassOf rdf:resource="&obo;FOODON_03400650"/>
	<obo:IAO_0000412>http://langual.org</obo:IAO_0000412>
	<obo:IAO_0000115 xml:lang="en">Pulses are derived from the mature seeds naturally or artificially dried, of leguminous plants known as beans (dry) and peas (dry).
The seeds in the pods are protected from most pesticides applied during the growing season except pesticides which show a systemic action. The dried beans and peas however are often exposed to post-harvest treatments.
The dry pulses are consumed after processing or household cooking.</obo:IAO_0000115>
	<obo:IAO_0000114 rdf:resource="&obo;IAO_0000428"/>
	<oboInOwl:hasDbXref>LANGUAL:A0680</oboInOwl:hasDbXref>
</owl:Class>

<owl:Class rdf:about="&obo;FOODON_03400681">
	<rdfs:label xml:lang="en">016  root and tuber vegetables (vr) (ccpr)</rdfs:label>
	<rdfs:subClassOf rdf:resource="&obo;FOODON_03400650"/>
	<obo:IAO_0000412>http://langual.org</obo:IAO_0000412>
	<obo:IAO_0000115 xml:lang="en">Root and tuber vegetables are the starchy enlarged solid roots, tubers, corms or rhizomes, mostly subterranean, of various species of plants, mostly annuals.
The underground location protects the edible portion from pesticides applied to the aerial parts of the crop during the growing season; however the commodities in this group are exposed to pesticide residues from soil treatments.
The entire vegetable may be consumed in the form of fresh or processed foods.</obo:IAO_0000115>
	<obo:IAO_0000114 rdf:resource="&obo;IAO_0000428"/>
	<oboInOwl:hasDbXref>LANGUAL:A0681</oboInOwl:hasDbXref>
</owl:Class>

<owl:Class rdf:about="&obo;FOODON_03400682">
	<rdfs:label xml:lang="en">017  stalk and stem vegetables (vs) (ccpr)</rdfs:label>
	<rdfs:subClassOf rdf:resource="&obo;FOODON_03400650"/>
	<obo:IAO_0000412>http://langual.org</obo:IAO_0000412>
	<obo:IAO_0000115 xml:lang="en">Stalk and stem vegetables are the edible stalks, leaf stems or immature shoots, from a variety of annual or perennial plants. Although not actually belonging to this group, globe artichoke (the immature flowerhead) of the family Compositae is included in this group.
Depending upon the part of the crop used for consumption and the growing practices, stalk and stem vegetables are exposed, in varying degrees, to pesticides applied during the growing season.
Stalk and stem vegetables may be consumed in whole or in part and in the form of fresh, dried or processed foods.</obo:IAO_0000115>
	<obo:IAO_0000114 rdf:resource="&obo;IAO_0000428"/>
	<oboInOwl:hasDbXref>LANGUAL:A0682</oboInOwl:hasDbXref>
</owl:Class>

<owl:Class rdf:about="&obo;FOODON_03400683">
	<rdfs:label xml:lang="en">020  cereal grains (gc) (ccpr)</rdfs:label>
	<rdfs:subClassOf rdf:resource="&obo;FOODON_03400651"/>
	<obo:IAO_0000412>http://langual.org</obo:IAO_0000412>
	<obo:IAO_0000115 xml:lang="en">Cereal grains are derived from the ears (heads) of starchy seeds produced by a variety of plants, primarily of the grass family (Grainineae)
Buckwheat, a dicotyledonous crop belonging to the botanical family Polygonaceae and two Chenopodium species, belonging to the botanical family Chenopodiaceae are included in this group, because of similarities in size and type of the seed, residue pattern and the use of the commodity.
The edible seeds are protected to varying degrees from pesticides applied during flee growing season by husks. Husks are removed before processing and/or consumption.
Cereal grains are often exposed to post-harvest treatments with pesticides.</obo:IAO_0000115>
	<obo:IAO_0000114 rdf:resource="&obo;IAO_0000428"/>
	<oboInOwl:hasDbXref>LANGUAL:A0683</oboInOwl:hasDbXref>
</owl:Class>

<owl:Class rdf:about="&obo;FOODON_03400684">
	<rdfs:label xml:lang="en">021  grasses for sugar and syrup production (gs) (ccpr)</rdfs:label>
	<rdfs:subClassOf rdf:resource="&obo;FOODON_03400651"/>
	<obo:IAO_0000412>http://langual.org</obo:IAO_0000412>
	<obo:IAO_0000115 xml:lang="en">Grasses For sugar or syrup production, includes species of grasses with a high sugar content especially in the stem. The stems are mainly used for sugar or syrup production, and to a small extent as vegetables or sweets. The leaves, ears and several wastes of the sugar or syrup manufacturing process are used, among others, as animal feed see Group 052: Miscellaneous fodder and forage crops).</obo:IAO_0000115>
	<obo:IAO_0000114 rdf:resource="&obo;IAO_0000428"/>
	<oboInOwl:hasDbXref>LANGUAL:A0684</oboInOwl:hasDbXref>
</owl:Class>

<owl:Class rdf:about="&obo;FOODON_03400685">
	<rdfs:label xml:lang="en">022  tree nuts (tn) (ccpr)</rdfs:label>
	<rdfs:subClassOf rdf:resource="&obo;FOODON_03400652"/>
	<obo:IAO_0000412>http://langual.org</obo:IAO_0000412>
	<obo:IAO_0000115 xml:lang="en">Tree nuts are the seeds of a variety of trees and shrubs which are characterized by a hard inedible shell enclosing an oily seed.
The seed is protected from pesticides applied during the growing season by the shell and other parts of the fruit.
The edible portion of the nut is consumed in succulent, dried or processed forms.</obo:IAO_0000115>
	<obo:IAO_0000114 rdf:resource="&obo;IAO_0000428"/>
	<oboInOwl:hasDbXref>LANGUAL:A0685</oboInOwl:hasDbXref>
</owl:Class>

<owl:Class rdf:about="&obo;FOODON_03400686">
	<rdfs:label xml:lang="en">023  oilseed (so) (ccpr)</rdfs:label>
	<rdfs:subClassOf rdf:resource="&obo;FOODON_03400652"/>
	<obo:IAO_0000412>http://langual.org</obo:IAO_0000412>
	<obo:IAO_0000115 xml:lang="en">Oilseed consists of seeds from a variety of plants used in the production of edible vegetable oils, seed meals and cakes for animal feed. Some important vegetable oil seeds are by-products of fibre or fruit crops (e.g. cotton seed, olives).
Some of the oilseeds are, directly or after slight processing (e.g. roasting), used as food (e.g. peanuts) or for food flavouring (e.g. poppy seed, sesame seed).
Oilseeds are protected from pesticides applied during the growing season by the shell or husk.</obo:IAO_0000115>
	<obo:IAO_0000114 rdf:resource="&obo;IAO_0000428"/>
	<oboInOwl:hasDbXref>LANGUAL:A0686</oboInOwl:hasDbXref>
</owl:Class>

<owl:Class rdf:about="&obo;FOODON_03400687">
	<rdfs:label xml:lang="en">024  seed for beverages and sweets (sb) (ccpr)</rdfs:label>
	<rdfs:subClassOf rdf:resource="&obo;FOODON_03400652"/>
	<obo:IAO_0000412>http://langual.org</obo:IAO_0000412>
	<obo:IAO_0000115 xml:lang="en">The seeds for beverages and sweets are derived from tropical and sub-tropical trees and shrubs. After processing the seeds are used in the production of beverages and sweets.
These seeds are protected from pesticides applied during the growing season by the shell or other parts of the fruit.</obo:IAO_0000115>
	<obo:IAO_0000114 rdf:resource="&obo;IAO_0000428"/>
	<oboInOwl:hasDbXref>LANGUAL:A0687</oboInOwl:hasDbXref>
</owl:Class>

<owl:Class rdf:about="&obo;FOODON_03400688">
	<rdfs:label xml:lang="en">027  herbs (hh) (ccpr)</rdfs:label>
	<rdfs:subClassOf rdf:resource="&obo;FOODON_03400653"/>
	<obo:IAO_0000412>http://langual.org</obo:IAO_0000412>
	<obo:IAO_0000115 xml:lang="en">Herbs consist of leaves, flowers, stems and roots from a variety of herbaceous plants, used in relatively small amounts as condiments to flavour foods or beverages. They are used either in fresh or naturally dried form.
Herbs are fully exposed to pesticides applied during the growing season. Post-harvest treatments are often carried out on dried herbs.
Herbs are consumed as components of other foods in succulent and dried forms or as extracts of the succulent products.</obo:IAO_0000115>
	<obo:IAO_0000114 rdf:resource="&obo;IAO_0000428"/>
	<oboInOwl:hasDbXref>LANGUAL:A0688</oboInOwl:hasDbXref>
</owl:Class>

<owl:Class rdf:about="&obo;FOODON_03400689">
	<rdfs:label xml:lang="en">028  spices (hs) (codex)</rdfs:label>
	<rdfs:subClassOf rdf:resource="&obo;FOODON_03400653"/>
	<obo:IAO_0000412>http://langual.org</obo:IAO_0000412>
	<obo:IAO_0000115 xml:lang="en">Spices consist of the aromatic seeds roots, berries or other fruits from a variety of plants, which are used in relatively small quantities to flavour foods.
Spices are exposed in varying degrees to pesticides applied during the growing season. Also post-harvest treatments may be applied to spices in the dried form.
They are consumed primarily in the dried form as condiment.</obo:IAO_0000115>
	<obo:IAO_0000114 rdf:resource="&obo;IAO_0000428"/>
	<oboInOwl:hasDbXref>LANGUAL:A0689</oboInOwl:hasDbXref>
</owl:Class>

<owl:Class rdf:about="&obo;FOODON_03400690">
	<rdfs:label xml:lang="en">european food groups (efg)</rdfs:label>
	<rdfs:subClassOf rdf:resource="&obo;FOODON_03400356"/>
	<obo:IAO_0000412>http://langual.org</obo:IAO_0000412>
	<obo:IAO_0000115 xml:lang="en">The European Food Groups (EFG) classification system was developed, as a project of COST Action 99/Eurofoods, in an attempt to evaluate the level of food description and classification that would permit international comparisons of the results of available food consumption and food availability surveys. In order to formulate the EFG system, several classification schemes used for recording food intake at the international and national classification schemes were compared:  International - FAO Food Balance Sheet, WHO GEMS/FOODS regional diets, DAFNE classification system for Household Budget Survey (HBS) data, and Eurocode 2 core classification (levels 1 and 2); National  -   French National Food Consumption Survey (1999), Dutch National Food Consumption Survey (1998), and British National Food Survey.
In the process of comparing food intake data from various European countries, it became evident that such comparisons are feasible only when results are expressed at the raw ingredient level. Since the DAFNE classification system groups food items at the raw level, it was one of the international classification schemes used to create the EFG food grouping system.
Ref.:  Ireland, J., Van Erp-Baart, A.M.J., Charrondière, U.R., Møller, A., Smithers, G., and Trichopoulou, A.: Selection of food classification system and food composition database for future food consumption surveys. European Journal of Clinical Nutrition, 56, Suppl. 2, S33 - S45, 2002.</obo:IAO_0000115>
	<obo:IAO_0000114 rdf:resource="&obo;IAO_0000428"/>
	<rdfs:comment xml:lang="en">LanguaL curation note: This term is for CLASSIFICATION ONLY; DO NOT USE term in indexing. Use a more precise narrower term.</rdfs:comment>
	<oboInOwl:hasDbXref>LANGUAL:A0690</oboInOwl:hasDbXref>
</owl:Class>

<owl:Class rdf:about="&obo;FOODON_03400691">
	<rdfs:label xml:lang="en">01  bread and rolls (efg)</rdfs:label>
	<rdfs:subClassOf rdf:resource="&obo;FOODON_03400690"/>
	<obo:IAO_0000412>http://langual.org</obo:IAO_0000412>
	<obo:IAO_0000114 rdf:resource="&obo;IAO_0000428"/>
	<oboInOwl:hasDbXref>LANGUAL:A0691</oboInOwl:hasDbXref>
</owl:Class>

<owl:Class rdf:about="&obo;FOODON_03400692">
	<rdfs:label xml:lang="en">02  breakfast cereals (efg)</rdfs:label>
	<rdfs:subClassOf rdf:resource="&obo;FOODON_03400690"/>
	<obo:IAO_0000412>http://langual.org</obo:IAO_0000412>
	<obo:IAO_0000114 rdf:resource="&obo;IAO_0000428"/>
	<oboInOwl:hasDbXref>LANGUAL:A0692</oboInOwl:hasDbXref>
</owl:Class>

<owl:Class rdf:about="&obo;FOODON_03400693">
	<rdfs:label xml:lang="en">03  flour (efg)</rdfs:label>
	<rdfs:subClassOf rdf:resource="&obo;FOODON_03400690"/>
	<obo:IAO_0000412>http://langual.org</obo:IAO_0000412>
	<obo:IAO_0000114 rdf:resource="&obo;IAO_0000428"/>
	<oboInOwl:hasDbXref>LANGUAL:A0693</oboInOwl:hasDbXref>
</owl:Class>

<owl:Class rdf:about="&obo;FOODON_03400694">
	<rdfs:label xml:lang="en">04  pasta (efg)</rdfs:label>
	<rdfs:subClassOf rdf:resource="&obo;FOODON_03400690"/>
	<obo:IAO_0000412>http://langual.org</obo:IAO_0000412>
	<obo:IAO_0000114 rdf:resource="&obo;IAO_0000428"/>
	<oboInOwl:hasDbXref>LANGUAL:A0694</oboInOwl:hasDbXref>
</owl:Class>

<owl:Class rdf:about="&obo;FOODON_03400695">
	<rdfs:label xml:lang="en">05  bakery products (efg)</rdfs:label>
	<rdfs:subClassOf rdf:resource="&obo;FOODON_03400690"/>
	<obo:IAO_0000412>http://langual.org</obo:IAO_0000412>
	<obo:IAO_0000114 rdf:resource="&obo;IAO_0000428"/>
	<oboInOwl:hasDbXref>LANGUAL:A0695</oboInOwl:hasDbXref>
</owl:Class>

<owl:Class rdf:about="&obo;FOODON_03400696">
	<rdfs:label xml:lang="en">06  rice and other cereal products (efg)</rdfs:label>
	<rdfs:subClassOf rdf:resource="&obo;FOODON_03400690"/>
	<obo:IAO_0000412>http://langual.org</obo:IAO_0000412>
	<obo:IAO_0000114 rdf:resource="&obo;IAO_0000428"/>
	<oboInOwl:hasDbXref>LANGUAL:A0696</oboInOwl:hasDbXref>
</owl:Class>

<owl:Class rdf:about="&obo;FOODON_03400697">
	<rdfs:label xml:lang="en">07  sugar (efg)</rdfs:label>
	<rdfs:subClassOf rdf:resource="&obo;FOODON_03400690"/>
	<obo:IAO_0000412>http://langual.org</obo:IAO_0000412>
	<obo:IAO_0000114 rdf:resource="&obo;IAO_0000428"/>
	<oboInOwl:hasDbXref>LANGUAL:A0697</oboInOwl:hasDbXref>
</owl:Class>

<owl:Class rdf:about="&obo;FOODON_03400698">
	<rdfs:label xml:lang="en">08 sugar products, excluding chocolate (efg)</rdfs:label>
	<rdfs:subClassOf rdf:resource="&obo;FOODON_03400690"/>
	<obo:IAO_0000412>http://langual.org</obo:IAO_0000412>
	<obo:IAO_0000114 rdf:resource="&obo;IAO_0000428"/>
	<oboInOwl:hasDbXref>LANGUAL:A0698</oboInOwl:hasDbXref>
</owl:Class>

<owl:Class rdf:about="&obo;FOODON_03400699">
	<rdfs:label xml:lang="en">09  chocolate (efg)</rdfs:label>
	<rdfs:subClassOf rdf:resource="&obo;FOODON_03400690"/>
	<obo:IAO_0000412>http://langual.org</obo:IAO_0000412>
	<obo:IAO_0000114 rdf:resource="&obo;IAO_0000428"/>
	<oboInOwl:hasDbXref>LANGUAL:A0699</oboInOwl:hasDbXref>
</owl:Class>

<owl:Class rdf:about="&obo;FOODON_03400700">
	<rdfs:label xml:lang="en">10  vegetable oils (efg)</rdfs:label>
	<rdfs:subClassOf rdf:resource="&obo;FOODON_03400690"/>
	<obo:IAO_0000412>http://langual.org</obo:IAO_0000412>
	<obo:IAO_0000114 rdf:resource="&obo;IAO_0000428"/>
	<oboInOwl:hasDbXref>LANGUAL:A0700</oboInOwl:hasDbXref>
</owl:Class>

<owl:Class rdf:about="&obo;FOODON_03400701">
	<rdfs:label xml:lang="en">11  margarine and lipids of mixed origin (efg)</rdfs:label>
	<rdfs:subClassOf rdf:resource="&obo;FOODON_03400690"/>
	<obo:IAO_0000412>http://langual.org</obo:IAO_0000412>
	<obo:IAO_0000114 rdf:resource="&obo;IAO_0000428"/>
	<oboInOwl:hasDbXref>LANGUAL:A0701</oboInOwl:hasDbXref>
</owl:Class>

<owl:Class rdf:about="&obo;FOODON_03400702">
	<rdfs:label xml:lang="en">12  butter and animal fats (efg)</rdfs:label>
	<rdfs:subClassOf rdf:resource="&obo;FOODON_03400690"/>
	<obo:IAO_0000412>http://langual.org</obo:IAO_0000412>
	<obo:IAO_0000114 rdf:resource="&obo;IAO_0000428"/>
	<oboInOwl:hasDbXref>LANGUAL:A0702</oboInOwl:hasDbXref>
</owl:Class>

<owl:Class rdf:about="&obo;FOODON_03400703">
	<rdfs:label xml:lang="en">13  nuts (efg)</rdfs:label>
	<rdfs:subClassOf rdf:resource="&obo;FOODON_03400690"/>
	<obo:IAO_0000412>http://langual.org</obo:IAO_0000412>
	<obo:IAO_0000114 rdf:resource="&obo;IAO_0000428"/>
	<oboInOwl:hasDbXref>LANGUAL:A0703</oboInOwl:hasDbXref>
</owl:Class>

<owl:Class rdf:about="&obo;FOODON_03400704">
	<rdfs:label xml:lang="en">14  pulses (efg)</rdfs:label>
	<rdfs:subClassOf rdf:resource="&obo;FOODON_03400690"/>
	<obo:IAO_0000412>http://langual.org</obo:IAO_0000412>
	<obo:IAO_0000114 rdf:resource="&obo;IAO_0000428"/>
	<oboInOwl:hasDbXref>LANGUAL:A0704</oboInOwl:hasDbXref>
</owl:Class>

<owl:Class rdf:about="&obo;FOODON_03400705">
	<rdfs:label xml:lang="en">15  vegetables, excluding potatoes (efg)</rdfs:label>
	<rdfs:subClassOf rdf:resource="&obo;FOODON_03400690"/>
	<obo:IAO_0000412>http://langual.org</obo:IAO_0000412>
	<obo:IAO_0000114 rdf:resource="&obo;IAO_0000428"/>
	<oboInOwl:hasDbXref>LANGUAL:A0705</oboInOwl:hasDbXref>
</owl:Class>

<owl:Class rdf:about="&obo;FOODON_03400706">
	<rdfs:label xml:lang="en">16  starchy roots and potatoes (efg)</rdfs:label>
	<rdfs:subClassOf rdf:resource="&obo;FOODON_03400690"/>
	<obo:IAO_0000412>http://langual.org</obo:IAO_0000412>
	<obo:IAO_0000114 rdf:resource="&obo;IAO_0000428"/>
	<oboInOwl:hasDbXref>LANGUAL:A0706</oboInOwl:hasDbXref>
</owl:Class>

<owl:Class rdf:about="&obo;FOODON_03400707">
	<rdfs:label xml:lang="en">17  fruits (efg)</rdfs:label>
	<rdfs:subClassOf rdf:resource="&obo;FOODON_03400690"/>
	<obo:IAO_0000412>http://langual.org</obo:IAO_0000412>
	<obo:IAO_0000114 rdf:resource="&obo;IAO_0000428"/>
	<oboInOwl:hasDbXref>LANGUAL:A0707</oboInOwl:hasDbXref>
</owl:Class>

<owl:Class rdf:about="&obo;FOODON_03400708">
	<rdfs:label xml:lang="en">18  fruit juices (efg)</rdfs:label>
	<rdfs:subClassOf rdf:resource="&obo;FOODON_03400690"/>
	<obo:IAO_0000412>http://langual.org</obo:IAO_0000412>
	<obo:IAO_0000114 rdf:resource="&obo;IAO_0000428"/>
	<oboInOwl:hasDbXref>LANGUAL:A0708</oboInOwl:hasDbXref>
</owl:Class>

<owl:Class rdf:about="&obo;FOODON_03400709">
	<rdfs:label xml:lang="en">19  non-alcoholic beverages (efg)</rdfs:label>
	<rdfs:subClassOf rdf:resource="&obo;FOODON_03400690"/>
	<obo:IAO_0000412>http://langual.org</obo:IAO_0000412>
	<obo:IAO_0000114 rdf:resource="&obo;IAO_0000428"/>
	<oboInOwl:hasDbXref>LANGUAL:A0709</oboInOwl:hasDbXref>
</owl:Class>

<owl:Class rdf:about="&obo;FOODON_03400710">
	<rdfs:label xml:lang="en">20  coffee, tea, cocoa powder (efg)</rdfs:label>
	<rdfs:subClassOf rdf:resource="&obo;FOODON_03400690"/>
	<obo:IAO_0000412>http://langual.org</obo:IAO_0000412>
	<obo:IAO_0000114 rdf:resource="&obo;IAO_0000428"/>
	<oboInOwl:hasDbXref>LANGUAL:A0710</oboInOwl:hasDbXref>
</owl:Class>

<owl:Class rdf:about="&obo;FOODON_03400711">
	<rdfs:label xml:lang="en">21  beer (efg)</rdfs:label>
	<rdfs:subClassOf rdf:resource="&obo;FOODON_03400690"/>
	<obo:IAO_0000412>http://langual.org</obo:IAO_0000412>
	<obo:IAO_0000114 rdf:resource="&obo;IAO_0000428"/>
	<oboInOwl:hasDbXref>LANGUAL:A0711</oboInOwl:hasDbXref>
</owl:Class>

<owl:Class rdf:about="&obo;FOODON_03400712">
	<rdfs:label xml:lang="en">22  wine (efg)</rdfs:label>
	<rdfs:subClassOf rdf:resource="&obo;FOODON_03400690"/>
	<obo:IAO_0000412>http://langual.org</obo:IAO_0000412>
	<obo:IAO_0000114 rdf:resource="&obo;IAO_0000428"/>
	<oboInOwl:hasDbXref>LANGUAL:A0712</oboInOwl:hasDbXref>
</owl:Class>

<owl:Class rdf:about="&obo;FOODON_03400713">
	<rdfs:label xml:lang="en">23  other alcoholic beverages (efg)</rdfs:label>
	<rdfs:subClassOf rdf:resource="&obo;FOODON_03400690"/>
	<obo:IAO_0000412>http://langual.org</obo:IAO_0000412>
	<obo:IAO_0000114 rdf:resource="&obo;IAO_0000428"/>
	<oboInOwl:hasDbXref>LANGUAL:A0713</oboInOwl:hasDbXref>
</owl:Class>

<owl:Class rdf:about="&obo;FOODON_03400714">
	<rdfs:label xml:lang="en">24  red meat and meat products (efg)</rdfs:label>
	<rdfs:subClassOf rdf:resource="&obo;FOODON_03400690"/>
	<obo:IAO_0000412>http://langual.org</obo:IAO_0000412>
	<obo:IAO_0000114 rdf:resource="&obo;IAO_0000428"/>
	<oboInOwl:hasDbXref>LANGUAL:A0714</oboInOwl:hasDbXref>
</owl:Class>

<owl:Class rdf:about="&obo;FOODON_03400715">
	<rdfs:label xml:lang="en">25  poultry and poultry products (efg)</rdfs:label>
	<rdfs:subClassOf rdf:resource="&obo;FOODON_03400690"/>
	<obo:IAO_0000412>http://langual.org</obo:IAO_0000412>
	<obo:IAO_0000114 rdf:resource="&obo;IAO_0000428"/>
	<oboInOwl:hasDbXref>LANGUAL:A0715</oboInOwl:hasDbXref>
</owl:Class>

<owl:Class rdf:about="&obo;FOODON_03400716">
	<rdfs:label xml:lang="en">26  offals (efg)</rdfs:label>
	<rdfs:subClassOf rdf:resource="&obo;FOODON_03400690"/>
	<obo:IAO_0000412>http://langual.org</obo:IAO_0000412>
	<obo:IAO_0000114 rdf:resource="&obo;IAO_0000428"/>
	<oboInOwl:hasDbXref>LANGUAL:A0716</oboInOwl:hasDbXref>
</owl:Class>

<owl:Class rdf:about="&obo;FOODON_03400717">
	<rdfs:label xml:lang="en">27  fish and seafood (efg)</rdfs:label>
	<rdfs:subClassOf rdf:resource="&obo;FOODON_03400690"/>
	<obo:IAO_0000412>http://langual.org</obo:IAO_0000412>
	<obo:IAO_0000114 rdf:resource="&obo;IAO_0000428"/>
	<oboInOwl:hasDbXref>LANGUAL:A0717</oboInOwl:hasDbXref>
</owl:Class>

<owl:Class rdf:about="&obo;FOODON_03400718">
	<rdfs:label xml:lang="en">28  eggs (efg)</rdfs:label>
	<rdfs:subClassOf rdf:resource="&obo;FOODON_03400690"/>
	<obo:IAO_0000412>http://langual.org</obo:IAO_0000412>
	<obo:IAO_0000114 rdf:resource="&obo;IAO_0000428"/>
	<oboInOwl:hasDbXref>LANGUAL:A0718</oboInOwl:hasDbXref>
</owl:Class>

<owl:Class rdf:about="&obo;FOODON_03400719">
	<rdfs:label xml:lang="en">29  milk (efg)</rdfs:label>
	<rdfs:subClassOf rdf:resource="&obo;FOODON_03400690"/>
	<obo:IAO_0000412>http://langual.org</obo:IAO_0000412>
	<obo:IAO_0000114 rdf:resource="&obo;IAO_0000428"/>
	<oboInOwl:hasDbXref>LANGUAL:A0719</oboInOwl:hasDbXref>
</owl:Class>

<owl:Class rdf:about="&obo;FOODON_03400720">
	<rdfs:label xml:lang="en">30  cheese (efg)</rdfs:label>
	<rdfs:subClassOf rdf:resource="&obo;FOODON_03400690"/>
	<obo:IAO_0000412>http://langual.org</obo:IAO_0000412>
	<obo:IAO_0000114 rdf:resource="&obo;IAO_0000428"/>
	<oboInOwl:hasDbXref>LANGUAL:A0720</oboInOwl:hasDbXref>
</owl:Class>

<owl:Class rdf:about="&obo;FOODON_03400721">
	<rdfs:label xml:lang="en">31  other milk products (efg)</rdfs:label>
	<rdfs:subClassOf rdf:resource="&obo;FOODON_03400690"/>
	<obo:IAO_0000412>http://langual.org</obo:IAO_0000412>
	<obo:IAO_0000114 rdf:resource="&obo;IAO_0000428"/>
	<oboInOwl:hasDbXref>LANGUAL:A0721</oboInOwl:hasDbXref>
</owl:Class>

<owl:Class rdf:about="&obo;FOODON_03400722">
	<rdfs:label xml:lang="en">32  miscellaneous foods (efg)</rdfs:label>
	<rdfs:subClassOf rdf:resource="&obo;FOODON_03400690"/>
	<obo:IAO_0000412>http://langual.org</obo:IAO_0000412>
	<obo:IAO_0000114 rdf:resource="&obo;IAO_0000428"/>
	<oboInOwl:hasDbXref>LANGUAL:A0722</oboInOwl:hasDbXref>
</owl:Class>

<owl:Class rdf:about="&obo;FOODON_03400723">
	<rdfs:label xml:lang="en">33  products for special nutritional use (efg)</rdfs:label>
	<rdfs:subClassOf rdf:resource="&obo;FOODON_03400690"/>
	<obo:IAO_0000412>http://langual.org</obo:IAO_0000412>
	<obo:IAO_0000114 rdf:resource="&obo;IAO_0000428"/>
	<oboInOwl:hasDbXref>LANGUAL:A0723</oboInOwl:hasDbXref>
</owl:Class>

<owl:Class rdf:about="&obo;FOODON_03400724">
	<rdfs:label xml:lang="en">01  milk and milk products (eurocode2)</rdfs:label>
	<rdfs:subClassOf rdf:resource="&obo;FOODON_03400642"/>
	<obo:IAO_0000412>http://langual.org</obo:IAO_0000412>
	<obo:IAO_0000114 rdf:resource="&obo;IAO_0000428"/>
	<oboInOwl:hasDbXref>LANGUAL:A0724</oboInOwl:hasDbXref>
</owl:Class>

<owl:Class rdf:about="&obo;FOODON_03400725">
	<rdfs:label xml:lang="en">02  egg and egg products (eurocode2)</rdfs:label>
	<rdfs:subClassOf rdf:resource="&obo;FOODON_03400642"/>
	<obo:IAO_0000412>http://langual.org</obo:IAO_0000412>
	<obo:IAO_0000114 rdf:resource="&obo;IAO_0000428"/>
	<oboInOwl:hasDbXref>LANGUAL:A0725</oboInOwl:hasDbXref>
</owl:Class>

<owl:Class rdf:about="&obo;FOODON_03400726">
	<rdfs:label xml:lang="en">03  meat and meat products (eurocode2)</rdfs:label>
	<rdfs:subClassOf rdf:resource="&obo;FOODON_03400642"/>
	<obo:IAO_0000412>http://langual.org</obo:IAO_0000412>
	<obo:IAO_0000114 rdf:resource="&obo;IAO_0000428"/>
	<oboInOwl:hasDbXref>LANGUAL:A0726</oboInOwl:hasDbXref>
</owl:Class>

<owl:Class rdf:about="&obo;FOODON_03400727">
	<rdfs:label xml:lang="en">04  fish and fish products (eurocode2)</rdfs:label>
	<rdfs:subClassOf rdf:resource="&obo;FOODON_03400642"/>
	<obo:IAO_0000412>http://langual.org</obo:IAO_0000412>
	<obo:IAO_0000114 rdf:resource="&obo;IAO_0000428"/>
	<oboInOwl:hasDbXref>LANGUAL:A0727</oboInOwl:hasDbXref>
</owl:Class>

<owl:Class rdf:about="&obo;FOODON_03400728">
	<rdfs:label xml:lang="en">05  fats and oils (eurocode2)</rdfs:label>
	<rdfs:subClassOf rdf:resource="&obo;FOODON_03400642"/>
	<obo:IAO_0000412>http://langual.org</obo:IAO_0000412>
	<obo:IAO_0000114 rdf:resource="&obo;IAO_0000428"/>
	<oboInOwl:hasDbXref>LANGUAL:A0728</oboInOwl:hasDbXref>
</owl:Class>

<owl:Class rdf:about="&obo;FOODON_03400729">
	<rdfs:label xml:lang="en">06  grains and grain products (eurocode2)</rdfs:label>
	<rdfs:subClassOf rdf:resource="&obo;FOODON_03400642"/>
	<obo:IAO_0000412>http://langual.org</obo:IAO_0000412>
	<obo:IAO_0000114 rdf:resource="&obo;IAO_0000428"/>
	<oboInOwl:hasDbXref>LANGUAL:A0729</oboInOwl:hasDbXref>
</owl:Class>

<owl:Class rdf:about="&obo;FOODON_03400730">
	<rdfs:label xml:lang="en">07  pulses, seeds, kernels, nuts and products (eurocode2)</rdfs:label>
	<rdfs:subClassOf rdf:resource="&obo;FOODON_03400642"/>
	<obo:IAO_0000412>http://langual.org</obo:IAO_0000412>
	<obo:IAO_0000114 rdf:resource="&obo;IAO_0000428"/>
	<oboInOwl:hasDbXref>LANGUAL:A0730</oboInOwl:hasDbXref>
</owl:Class>

<owl:Class rdf:about="&obo;FOODON_03400731">
	<rdfs:label xml:lang="en">08  vegetables and vegetable products (eurocode2)</rdfs:label>
	<rdfs:subClassOf rdf:resource="&obo;FOODON_03400642"/>
	<obo:IAO_0000412>http://langual.org</obo:IAO_0000412>
	<obo:IAO_0000114 rdf:resource="&obo;IAO_0000428"/>
	<oboInOwl:hasDbXref>LANGUAL:A0731</oboInOwl:hasDbXref>
</owl:Class>

<owl:Class rdf:about="&obo;FOODON_03400732">
	<rdfs:label xml:lang="en">09  fruit and fruit products (eurocode2)</rdfs:label>
	<rdfs:subClassOf rdf:resource="&obo;FOODON_03400642"/>
	<obo:IAO_0000412>http://langual.org</obo:IAO_0000412>
	<obo:IAO_0000114 rdf:resource="&obo;IAO_0000428"/>
	<oboInOwl:hasDbXref>LANGUAL:A0732</oboInOwl:hasDbXref>
</owl:Class>

<owl:Class rdf:about="&obo;FOODON_03400733">
	<rdfs:label xml:lang="en">10  sugar, chocolate and related products (eurocode2)</rdfs:label>
	<rdfs:subClassOf rdf:resource="&obo;FOODON_03400642"/>
	<obo:IAO_0000412>http://langual.org</obo:IAO_0000412>
	<obo:IAO_0000114 rdf:resource="&obo;IAO_0000428"/>
	<oboInOwl:hasDbXref>LANGUAL:A0733</oboInOwl:hasDbXref>
</owl:Class>

<owl:Class rdf:about="&obo;FOODON_03400734">
	<rdfs:label xml:lang="en">11  beverages (non-milk) (eurocode2)</rdfs:label>
	<rdfs:subClassOf rdf:resource="&obo;FOODON_03400642"/>
	<obo:IAO_0000412>http://langual.org</obo:IAO_0000412>
	<obo:IAO_0000114 rdf:resource="&obo;IAO_0000428"/>
	<oboInOwl:hasDbXref>LANGUAL:A0734</oboInOwl:hasDbXref>
</owl:Class>

<owl:Class rdf:about="&obo;FOODON_03400735">
	<rdfs:label xml:lang="en">12  miscellaneous foods (eurocode2)</rdfs:label>
	<rdfs:subClassOf rdf:resource="&obo;FOODON_03400642"/>
	<obo:IAO_0000412>http://langual.org</obo:IAO_0000412>
	<obo:IAO_0000114 rdf:resource="&obo;IAO_0000428"/>
	<oboInOwl:hasDbXref>LANGUAL:A0735</oboInOwl:hasDbXref>
</owl:Class>

<owl:Class rdf:about="&obo;FOODON_03400736">
	<rdfs:label xml:lang="en">13  products for special nutritional use (eurocode2)</rdfs:label>
	<rdfs:subClassOf rdf:resource="&obo;FOODON_03400642"/>
	<obo:IAO_0000412>http://langual.org</obo:IAO_0000412>
	<obo:IAO_0000114 rdf:resource="&obo;IAO_0000428"/>
	<oboInOwl:hasDbXref>LANGUAL:A0736</oboInOwl:hasDbXref>
</owl:Class>

<owl:Class rdf:about="&obo;FOODON_03400737">
	<rdfs:label xml:lang="en">030  meat (from mammals other than marine mammals) (mm) (ccpr)</rdfs:label>
	<rdfs:subClassOf rdf:resource="&obo;FOODON_03400654"/>
	<obo:IAO_0000412>http://langual.org</obo:IAO_0000412>
	<obo:IAO_0000115 xml:lang="en">Meats are the muscular tissues, including adhering fatty tissues such as intramuscular and subcutaneous fat from animal carcases or cuts of these as prepared for wholesale or retail distribution in a "fresh" state. The cuts offered to the consumer may include bones, connective tissues and tendons as well as nerves and lymph nodes.
The cornrnodity description of "fresh" meat includes meat which has been quick-frozen or quick-frozen and thawed.
The Group does not include edible offal as defined in Group 032.
Exposures to pesticides is through animal metabolism following oral intake with feed or through dermal intake as a consequence of external use of pesticides against ectoparasites.
The entire commodity except bones may be consumed.</obo:IAO_0000115>
	<obo:IAO_0000114 rdf:resource="&obo;IAO_0000428"/>
	<oboInOwl:hasDbXref>LANGUAL:A0737</oboInOwl:hasDbXref>
</owl:Class>

<owl:Class rdf:about="&obo;FOODON_03400738">
	<rdfs:label xml:lang="en">031  mammalian fats (mf) (ccpr)</rdfs:label>
	<rdfs:subClassOf rdf:resource="&obo;FOODON_03400654"/>
	<obo:IAO_0000412>http://langual.org</obo:IAO_0000412>
	<obo:IAO_0000115 xml:lang="en">Mammalian fats, excluding milk fats are derived from the fatty tissues of animals (not processed). For processed animal fats see Group 085.
Exposure to pesticides is through animal metabolism following oral intake with feed or through dermal intake as a consequence of external use of the pesticides against ectoparasites.
The entire commodity may be consumed.</obo:IAO_0000115>
	<obo:IAO_0000114 rdf:resource="&obo;IAO_0000428"/>
	<oboInOwl:hasDbXref>LANGUAL:A0738</oboInOwl:hasDbXref>
</owl:Class>

<owl:Class rdf:about="&obo;FOODON_03400739">
	<rdfs:label xml:lang="en">032  edible offal (mammalian) (mo) (ccpr)</rdfs:label>
	<rdfs:subClassOf rdf:resource="&obo;FOODON_03400654"/>
	<obo:IAO_0000412>http://langual.org</obo:IAO_0000412>
	<obo:IAO_0000115 xml:lang="en">Edible offal are edible tissue and organs other than muscles (= meat) and animal fat from slaughtered animals as prepared for wholesale or retail distribution.
Examples: liver, kidney, tongue, heart, stomach, sweetbread (thymus gland), braln, etc.
The group name and definitions are in conformity with those recorded in the Codex Standards 89-1981 and 98-1981, Codex Standard for Luncheon Meat and Codex Standard for Cooked Cured Chopped Meat respectively: "Edible offal" means such offal as have been passed as fit for human consumption, but not including lungs, ears, scalp, snout (including lips and muzzle), mucous membranes, sinews, genital system, udders, intestines and urinary bladder". In the former Classification of Food and Food Groups in the Guide to Codex Maximum Limits for Pesticide Residues 1978; CAC/PR 1-1978 the name Meat by-products was used for this group.
Exposure to pesticides is through animal metabolism following oral intake with feed or through dermal intake as a consequence of external use of pesticides on livestock animals against ectoparasites.
The entire commodity may be consumed.</obo:IAO_0000115>
	<obo:IAO_0000114 rdf:resource="&obo;IAO_0000428"/>
	<oboInOwl:hasDbXref>LANGUAL:A0739</oboInOwl:hasDbXref>
</owl:Class>

<owl:Class rdf:about="&obo;FOODON_03400740">
	<rdfs:label xml:lang="en">033  milks (ml) (ccpr)</rdfs:label>
	<rdfs:subClassOf rdf:resource="&obo;FOODON_03400654"/>
	<obo:IAO_0000412>http://langual.org</obo:IAO_0000412>
	<obo:IAO_0000115 xml:lang="en">Milks are the mammary secretions of various species of lactating herbivorous ruminant animals, usually domesticated.
In conformity with the Codex Alimentarius Code of Principles concerning Milk and Milk Products the term "Milk" shall mean exclusively the normal mammary excretion obtained from one or more milkings without either addition thereto or extraction therefrom.
Notwithstanding the provisions in the preceding paragraph, "the term "Milk" may be used for milk treated without altering its composition, or for milk, the fat content of which has been standardized under domestic legislation".
The entire commodity may be consumed.</obo:IAO_0000115>
	<obo:IAO_0000114 rdf:resource="&obo;IAO_0000428"/>
	<oboInOwl:hasDbXref>LANGUAL:A0740</oboInOwl:hasDbXref>
</owl:Class>

<owl:Class rdf:about="&obo;FOODON_03400741">
	<rdfs:label xml:lang="en">036  poultry meat (including pigeon meat) (pm) (ccpr)</rdfs:label>
	<rdfs:subClassOf rdf:resource="&obo;FOODON_03400655"/>
	<obo:IAO_0000412>http://langual.org</obo:IAO_0000412>
	<obo:IAO_0000115 xml:lang="en">Poultry meats are the muscular tissues including adhering fat and skin from poultry carcases as prepared for wholesale or retail distribution.
Exposure to pesticides may result from external treatment of animals or poultry houses or through animal metabolism following oral intake of pesticides with feed.
The entire product may be consumed.</obo:IAO_0000115>
	<obo:IAO_0000114 rdf:resource="&obo;IAO_0000428"/>
	<oboInOwl:hasDbXref>LANGUAL:A0741</oboInOwl:hasDbXref>
</owl:Class>

<owl:Class rdf:about="&obo;FOODON_03400742">
	<rdfs:label xml:lang="en">037  poultry fats (pf) (ccpr)</rdfs:label>
	<rdfs:subClassOf rdf:resource="&obo;FOODON_03400655"/>
	<obo:IAO_0000412>http://langual.org</obo:IAO_0000412>
	<obo:IAO_0000115 xml:lang="en">Poultry fats are derived from the fatty tissues of poultry. Exposure to pesticides may result from external treatment of animals or poultry houses or through animal metabolism following oral intake of pesticides with feed.
The entire product may be consumed.</obo:IAO_0000115>
	<obo:IAO_0000114 rdf:resource="&obo;IAO_0000428"/>
	<oboInOwl:hasDbXref>LANGUAL:A0742</oboInOwl:hasDbXref>
</owl:Class>

<owl:Class rdf:about="&obo;FOODON_03400743">
	<rdfs:label xml:lang="en">038 - poultry, edible offal of (po) (ccpr)</rdfs:label>
	<rdfs:subClassOf rdf:resource="&obo;FOODON_03400655"/>
	<obo:IAO_0000412>http://langual.org</obo:IAO_0000412>
	<obo:IAO_0000115 xml:lang="en">Poultry edible offal are such edible tissues and organs, other than poultry meat and poultry fat, from slaughtered poultry as have been passed as fit for human consumption. Examples: liver, gizzard, heart, skin etc. In the former Classification of Food and Feed Groups in the Guide to Codex Maximum Limits for Pesticide Residues 1978: CAC/PR 1-1978 the name Poultry by-products was used for this group.
Exposure to pesticides is through animal metabolism following oral intake of pesticides with feed or may result from external treatment of animals or poultry houses.
The entire product may be consumed.</obo:IAO_0000115>
	<obo:IAO_0000114 rdf:resource="&obo;IAO_0000428"/>
	<oboInOwl:hasDbXref>LANGUAL:A0743</oboInOwl:hasDbXref>
</owl:Class>

<owl:Class rdf:about="&obo;FOODON_03400744">
	<rdfs:label xml:lang="en">039  eggs (pe) (ccpr)</rdfs:label>
	<rdfs:subClassOf rdf:resource="&obo;FOODON_03400655"/>
	<obo:IAO_0000412>http://langual.org</obo:IAO_0000412>
	<obo:IAO_0000115 xml:lang="en">Eggs are the fresh edible portion of the body produced by female birds, especially domestic fowl.
The edible portion includes egg yolk and egg white after removal of the shell.</obo:IAO_0000115>
	<obo:IAO_0000114 rdf:resource="&obo;IAO_0000428"/>
	<oboInOwl:hasDbXref>LANGUAL:A0744</oboInOwl:hasDbXref>
</owl:Class>

<owl:Class rdf:about="&obo;FOODON_03400745">
	<rdfs:label xml:lang="en">040  freshwater fish (wf) (ccpr)</rdfs:label>
	<rdfs:subClassOf rdf:resource="&obo;FOODON_03400656"/>
	<obo:IAO_0000412>http://langual.org</obo:IAO_0000412>
	<obo:IAO_0000115 xml:lang="en">The freshwater fishes generally remain lifelong,including flee spawning period,in fresh water (lakes, ponds, rivers and brooks).
Several species of freshwater fish are domesticated and bred in fish farms. Exposure of the latter species to pesticides is mainly through compounded fish feed and can also be through water pollution.</obo:IAO_0000115>
	<obo:IAO_0000114 rdf:resource="&obo;IAO_0000428"/>
	<oboInOwl:hasDbXref>LANGUAL:A0745</oboInOwl:hasDbXref>
</owl:Class>

<owl:Class rdf:about="&obo;FOODON_03400746">
	<rdfs:label xml:lang="en">041  diadromoous fish (wd) (ccpr)</rdfs:label>
	<rdfs:subClassOf rdf:resource="&obo;FOODON_03400656"/>
	<obo:IAO_0000412>http://langual.org</obo:IAO_0000412>
	<obo:IAO_0000115 xml:lang="en">The diadromous fishes in general migrate from the sea to brackish and/or freshwater and in the opposite direction.
The anadromous species spawn in fresh water (streams, small rivers and brooks) e.g. several salmon species, whereas eels spawn in the ocean. Some species, such as trout, are domesticated and do not migrate. They are bred in fish farms in ponds, mountain streams etc. The latter species especially may be exposed to pesticides through compounded fish feed and also through water pollution.
The fleshy parts of the animals and, to a lesser extent, roe and milt are consumed.</obo:IAO_0000115>
	<obo:IAO_0000114 rdf:resource="&obo;IAO_0000428"/>
	<oboInOwl:hasDbXref>LANGUAL:A0746</oboInOwl:hasDbXref>
</owl:Class>

<owl:Class rdf:about="&obo;FOODON_03400747">
	<rdfs:label xml:lang="en">042  marine fish (ws) (ccpr)</rdfs:label>
	<rdfs:subClassOf rdf:resource="&obo;FOODON_03400656"/>
	<obo:IAO_0000412>http://langual.org</obo:IAO_0000412>
	<obo:IAO_0000115 xml:lang="en">The marine fishes generally live in open seas. They are all or nearly all wild species, caught and prepared (often deep-frozen) for wholesale and retail distribution. Exposure to pesticides is mainly through water pollution and animal metabolism.
Especially the fleshy parts of the animals and to a lesser extent roe and milt are consumed.</obo:IAO_0000115>
	<obo:IAO_0000114 rdf:resource="&obo;IAO_0000428"/>
	<oboInOwl:hasDbXref>LANGUAL:A0747</oboInOwl:hasDbXref>
</owl:Class>

<owl:Class rdf:about="&obo;FOODON_03400748">
	<rdfs:label xml:lang="en">043  fish roe (including milt = soft roe) and edible offal of fish (wr) (ccpr)</rdfs:label>
	<rdfs:subClassOf rdf:resource="&obo;FOODON_03400656"/>
	<obo:IAO_0000412>http://langual.org</obo:IAO_0000412>
	<obo:IAO_0000115 xml:lang="en">Fish roes are the edible reproductive bodies of several species of fish. Of some of these only the "hard roe", the female reproductive body, is used whereas both the "hard" and "soft" roe (milt) of other species is marketed.
The term roe used in flee commodity description includes if relevant both types of roe.
The liver of some species is used as such for human consumption or for production of liver oils (e.g. cod liver oil).
Exposure to pesticides is through animal metabolism.</obo:IAO_0000115>
	<obo:IAO_0000114 rdf:resource="&obo;IAO_0000428"/>
	<oboInOwl:hasDbXref>LANGUAL:A0748</oboInOwl:hasDbXref>
</owl:Class>

<owl:Class rdf:about="&obo;FOODON_03400749">
	<rdfs:label xml:lang="en">044  marine mammals (wm) (ccpr)</rdfs:label>
	<rdfs:subClassOf rdf:resource="&obo;FOODON_03400656"/>
	<obo:IAO_0000412>http://langual.org</obo:IAO_0000412>
	<obo:IAO_0000115 xml:lang="en">Several sea mammals are caught on a large scale. The meat of various species is used as food or feed in some areas of the world. The blubber (=whale or seal fat) fat and train oil (oil derived from whale fat) is used after processing as raw material in food or feed manufacture; the sperm oil, as well as the spermaceti (a waxy substance from the head of sperm whales) is mainly used in cosmetics and some other industrial products.
Exposure to pesticides is by consumption of contaminated prey or through water pollution.
The entire commodity except the bones and other inedible parts may be consumed.</obo:IAO_0000115>
	<obo:IAO_0000114 rdf:resource="&obo;IAO_0000428"/>
	<oboInOwl:hasDbXref>LANGUAL:A0749</oboInOwl:hasDbXref>
</owl:Class>

<owl:Class rdf:about="&obo;FOODON_03400750">
	<rdfs:label xml:lang="en">045  crustaceans (wc) (ccpr)</rdfs:label>
	<rdfs:subClassOf rdf:resource="&obo;FOODON_03400656"/>
	<obo:IAO_0000412>http://langual.org</obo:IAO_0000412>
	<obo:IAO_0000115 xml:lang="en">Crustaceans are aquatic animals of various species, wild or cultivated, which have an inedible chitinous outer shell.
A small number of species live in fresh water but most species live in brackish water and/or in the sea.
Exposure to pesticides is through animal metabolism or water pollution.
Crustaceans are prepared for wholesale or retail distribution at a "raw" stage, often still alive, "raw" and deep-frozen or cooked directly after catching and deep-frozen. Shrimps or prawns may also be parboiled and thereafter deep-frozen.
Although the cooked or parboiled crustaceans should be regarded as processed foods, the animals of this group are primarily classified in the Chapter on Primary food commodities, Type 8: Aquatic animal products, since several crustaceans are also-marketed in a "raw" form, i.e. not exposed to temperatures sufficiently high to coagulate the protein at the surface. A short reference to processed Crustaceans is given in Type 17: Derived edible products of animal origin, Group 084 Crustaceans, processed.
The entire commodity except the shell may be consumed: the "raw" commodities, in general, after cooking.

In some countries, species such as the Norway lobster (Nephrops norvegicus) are included in the commodity "Prawns" with some qualifying designation, such as Dublin Bay Prawn or Prawn of Bantry Bay (both Ireland).The Codex Stan. 92-1981 on Quick Frozen Shrimps and Prawns does not prevent this practice, provided that the designation on the label ensures that the consumer will not be misled.
There is no clear-cut distinction between Shrimps and Prawns. In several countries the commodity name-Shrimps is used for the small species whereas the slightly larger ones are called Prawns. However, a species marked in certain regions of the world as "Prawn" may be called in the local English language in other areas a shrimp and visa versa, e.g., Pandalus borcalis is called Northern prawn or Deepwater prawn in the United Kingdom and the same species is named Pink shrimp in Canada. In Australia only the name Prawn is used for animals included in this commodity.
Not including the Freshwater species of the Palaemonidae.</obo:IAO_0000115>
	<obo:IAO_0000114 rdf:resource="&obo;IAO_0000428"/>
	<oboInOwl:hasDbXref>LANGUAL:A0750</oboInOwl:hasDbXref>
</owl:Class>

<owl:Class rdf:about="&obo;FOODON_03400751">
	<rdfs:label xml:lang="en">048  frogs, lizards, snakes and turtles (ar) (ccpr)</rdfs:label>
	<rdfs:subClassOf rdf:resource="&obo;FOODON_03400657"/>
	<obo:IAO_0000412>http://langual.org</obo:IAO_0000412>
	<obo:IAO_0000115 xml:lang="en">Frog, lizard, snake and turtle products are the edible parts from various animal species of the zoological classes Amphibia and Reptilia, usually wild, harvested for food. Some frog species are cultivated in a few European and Asian countries and to a small extent in the USA and "marketed" in the form of deep-frozen frog legs. The wild species are marketed in the same manner.
A few turtle species are raised from eggs or hatchlings in some tropical countries, especially the Green Turtle.
Exposure to pesticides is through animal metabolism.
The entire product, except the bones and the bony or horny outer shell (turtles), may be consumed.</obo:IAO_0000115>
	<obo:IAO_0000114 rdf:resource="&obo;IAO_0000428"/>
	<oboInOwl:hasDbXref>LANGUAL:A0751</oboInOwl:hasDbXref>
</owl:Class>

<owl:Class rdf:about="&obo;FOODON_03400752">
	<rdfs:label xml:lang="en">049  molluscs (including cephalopods) and other invertebrate animals (im) (ccpr)</rdfs:label>
	<rdfs:subClassOf rdf:resource="&obo;FOODON_03400658"/>
	<obo:IAO_0000412>http://langual.org</obo:IAO_0000412>
	<obo:IAO_0000115 xml:lang="en">Molluscs are aquatic or land animals or various species, wild or cultivated, which have an inedible outer or inner shell.
The edible aquatic Molluscs live mainly in brackish water or in the sea; several species are cultivated. A few edible species of land snails are cultivated.
Exposure to pesticides is through animal metabolism: the aquatic species also through water contamination.
The entire commodity except the outer or inner shell may be consumed.</obo:IAO_0000115>
	<obo:IAO_0000114 rdf:resource="&obo;IAO_0000428"/>
	<oboInOwl:hasDbXref>LANGUAL:A0752</oboInOwl:hasDbXref>
</owl:Class>

<owl:Class rdf:about="&obo;FOODON_03400753">
	<rdfs:label xml:lang="en">050  legume animal feeds (al) (ccpr)</rdfs:label>
	<rdfs:subClassOf rdf:resource="&obo;FOODON_03400659"/>
	<obo:IAO_0000412>http://langual.org</obo:IAO_0000412>
	<obo:IAO_0000115 xml:lang="en">Legume animal feeds include various species of leguminous plants used for animal forage, grazing, fodder hay or silage, with or without seed. Several species are grown exclusively for animal feeding purposes, whereas some others are grown primarily as food crops. The "waste" parts of the latter crops are often used as animal feed, either in the fresh form or as hay.
The entire commodity may be consumed by livestock animals.</obo:IAO_0000115>
	<obo:IAO_0000114 rdf:resource="&obo;IAO_0000428"/>
	<oboInOwl:hasDbXref>LANGUAL:A0753</oboInOwl:hasDbXref>
</owl:Class>

<owl:Class rdf:about="&obo;FOODON_03400754">
	<rdfs:label xml:lang="en">051  straw, fodder and forage of cereal grains and grasses, except grasses for sugar production (including buckwheat fooder) (as/af) (ccpr)</rdfs:label>
	<rdfs:subClassOf rdf:resource="&obo;FOODON_03400659"/>
	<obo:IAO_0000412>http://langual.org</obo:IAO_0000412>
	<obo:IAO_0000115 xml:lang="en">The straw, fodder and forage of cereal grains are derived from various plants of the grass family (Gramineae).
Cereal grains are grown to a limited extent as a forage crop. The immature crop is fed to livestock animals as succulent forage or as silage.
The cereal grain crops are mainly grown for human food or raw material for preparing food products. The "waste" parts remaining after harvest of the grain kernels (stems, stalks, leaves and empty ears) are extensively used and distributed for animal feeding purposes, in the form of dry fodder or straw.
Several other species of the grass family are exclusively grown as forage crops. These crops are either used for grazing or are prepared for wholesale or retail distribution in the form of grass silage (in general one or more cuttings from immature plants), as artificially dried grass or as hay.
The entire conimodity may be consumed by livestock animals.</obo:IAO_0000115>
	<obo:IAO_0000114 rdf:resource="&obo;IAO_0000428"/>
	<oboInOwl:hasDbXref>LANGUAL:A0754</oboInOwl:hasDbXref>
</owl:Class>

<owl:Class rdf:about="&obo;FOODON_03400755">
	<rdfs:label xml:lang="en">052  miscellaneous fodder and forage crops (am) (ccpr)</rdfs:label>
	<rdfs:subClassOf rdf:resource="&obo;FOODON_03400659"/>
	<obo:IAO_0000412>http://langual.org</obo:IAO_0000412>
	<obo:IAO_0000115 xml:lang="en">Miscellaneous Fodder and Forage crops, are derived from various kinds of plants except leguminous and grassy plants (family Gramineae). However, for convenience, the fodders and forage of grasses for sugar production are included in this group. Some of the crops listed in this group are primarily grown for human food or as raw material for preparing food (e.g. sugar beet) and the "waste" material of such crops is used as animal feed.
The entire commodity may be consumed by livestock animals, either in a succulent form, as silage or in the form of dry fodder.</obo:IAO_0000115>
	<obo:IAO_0000114 rdf:resource="&obo;IAO_0000428"/>
	<oboInOwl:hasDbXref>LANGUAL:A0755</oboInOwl:hasDbXref>
</owl:Class>

<owl:Class rdf:about="&obo;FOODON_03400756">
	<rdfs:label xml:lang="en">055  dried fruits (df) (ccpr)</rdfs:label>
	<rdfs:subClassOf rdf:resource="&obo;FOODON_03400660"/>
	<obo:IAO_0000412>http://langual.org</obo:IAO_0000412>
	<obo:IAO_0000115 xml:lang="en">Dried fruits. The commodities of this group are in general artificially dried. They may or may not be preserved or candied with addition of sugars.
Exposure to pesticides may arise from pre-harvest applications, post-harvest treatment of the fruits before processing, or treatment of the dried fruit to avoid losses during transport and wholesale or retail distribution.</obo:IAO_0000115>
	<obo:IAO_0000114 rdf:resource="&obo;IAO_0000428"/>
	<oboInOwl:hasDbXref>LANGUAL:A0756</oboInOwl:hasDbXref>
</owl:Class>

<owl:Class rdf:about="&obo;FOODON_03400757">
	<rdfs:label xml:lang="en">056  dried vegetables (dv) (ccpr)</rdfs:label>
	<rdfs:subClassOf rdf:resource="&obo;FOODON_03400660"/>
	<obo:IAO_0000412>http://langual.org</obo:IAO_0000412>
	<obo:IAO_0000115 xml:lang="en">Dried vegetables. The commodities of this group are in general artificially dried and often comminuted. Exposure to pesticides is from pre-harvest applications and or treatment of the dry commodities.
The entire commodity may be consumed after soaking or boiling.</obo:IAO_0000115>
	<obo:IAO_0000114 rdf:resource="&obo;IAO_0000428"/>
	<oboInOwl:hasDbXref>LANGUAL:A0757</oboInOwl:hasDbXref>
</owl:Class>

<owl:Class rdf:about="&obo;FOODON_03400758">
	<rdfs:label xml:lang="en">057 dried herbs (dh) (ccpr)</rdfs:label>
	<rdfs:subClassOf rdf:resource="&obo;FOODON_03400660"/>
	<obo:IAO_0000412>http://langual.org</obo:IAO_0000412>
	<obo:IAO_0000115 xml:lang="en">Dried herbs. The commodities of this group are in general artificially dried and often comminuted. For the commodities on the "fresh" state see Group 027 Herbs. Exposure to pesticides is from pre-harvest applications and/or treatment of the dry commodities.
They are often consumed in the dried form or soaked as a condiment in food commodities of plant or animal origin or in drinks, generally in small amounts</obo:IAO_0000115>
	<obo:IAO_0000114 rdf:resource="&obo;IAO_0000428"/>
	<oboInOwl:hasDbXref>LANGUAL:A0758</oboInOwl:hasDbXref>
</owl:Class>

<owl:Class rdf:about="&obo;FOODON_03400759">
	<rdfs:label xml:lang="en">058  milled cereal products (early milling stages) (cm) (ccpr)</rdfs:label>
	<rdfs:subClassOf rdf:resource="&obo;FOODON_03400660"/>
	<obo:IAO_0000412>http://langual.org</obo:IAO_0000412>
	<obo:IAO_0000115 xml:lang="en">Milled cereal products (early milling stages). The group includes the early milling fractions of cereal grains, except buckwheat, cañihua and quinoa such as husked rice, polished rice and the unprocessed cereal grain brans.
Exposure to pesticides is through pre-harvest treatments of the growing cereal grain crop and especially through post-harvest treatment of cereal grains.
The entire commodity may be consumed after further processing or household preparation.</obo:IAO_0000115>
	<obo:IAO_0000114 rdf:resource="&obo;IAO_0000428"/>
	<oboInOwl:hasDbXref>LANGUAL:A0759</oboInOwl:hasDbXref>
</owl:Class>

<owl:Class rdf:about="&obo;FOODON_03400760">
	<rdfs:label xml:lang="en">059  miscellaneaous secondary food commodities of plant origin (sm) (ccpr)</rdfs:label>
	<rdfs:subClassOf rdf:resource="&obo;FOODON_03400660"/>
	<obo:IAO_0000412>http://langual.org</obo:IAO_0000412>
	<obo:IAO_0000114 rdf:resource="&obo;IAO_0000428"/>
	<oboInOwl:hasDbXref>LANGUAL:A0760</oboInOwl:hasDbXref>
</owl:Class>

<owl:Class rdf:about="&obo;FOODON_03400761">
	<rdfs:label xml:lang="en">065  cereal grain milling fractions (cf) (ccpr)</rdfs:label>
	<rdfs:subClassOf rdf:resource="&obo;FOODON_03400661"/>
	<obo:IAO_0000412>http://langual.org</obo:IAO_0000412>
	<obo:IAO_0000115 xml:lang="en">Cereal grain milling fractions includes milling fractions of cereal grains at the final stage of milling and separation in the fractions. The group also includes the processed brans, as prepared for direct consumption.</obo:IAO_0000115>
	<obo:IAO_0000114 rdf:resource="&obo;IAO_0000428"/>
	<oboInOwl:hasDbXref>LANGUAL:A0761</oboInOwl:hasDbXref>
</owl:Class>

<owl:Class rdf:about="&obo;FOODON_03400762">
	<rdfs:label xml:lang="en">066  teas (dt) (ccpr)</rdfs:label>
	<rdfs:subClassOf rdf:resource="&obo;FOODON_03400661"/>
	<obo:IAO_0000412>http://langual.org</obo:IAO_0000412>
	<obo:IAO_0000115 xml:lang="en">Teas are derived from the leaves of several plants, principally Camellia sinensis.
They are used mainly in a fermented and dried form or only as dry leaves for the preparation of infusions, which are used as beverages.
Newly grown vegetative shoots (terminal bud and 2-3 leaves) of tea are plucked, withered, twisted and comminuted and thereafter, in general, fermented and dried.
Teas made from other plants are often prepared in a similar way.</obo:IAO_0000115>
	<obo:IAO_0000114 rdf:resource="&obo;IAO_0000428"/>
	<oboInOwl:hasDbXref>LANGUAL:A0762</oboInOwl:hasDbXref>
</owl:Class>

<owl:Class rdf:about="&obo;FOODON_03400763">
	<rdfs:label xml:lang="en">067  vegetable oils, crude (oc) (ccpr)</rdfs:label>
	<rdfs:subClassOf rdf:resource="&obo;FOODON_03400661"/>
	<obo:IAO_0000412>http://langual.org</obo:IAO_0000412>
	<obo:IAO_0000115 xml:lang="en">Vegetable oils, crude, includes the crude vegetable oils derived from oil seed Group 023, tropical and sub-tropical oil-containing fruits such as olives, and some pulses (e.g. soya bean, dry). For the definition and characteristics of Olive oil, crude see Codex Stan. 33-1981. The crude oils are used as constituents of compounded animal feeds or further processed (refined, clarified). See Group 068, Vegetable oils, edible (or refined).
Exposure to pesticides is through pre-harvest treatment of the relevant crops or post-harvest treatment of the oilseeds or oil-containing pulses.</obo:IAO_0000115>
	<obo:IAO_0000114 rdf:resource="&obo;IAO_0000428"/>
	<oboInOwl:hasDbXref>LANGUAL:A0763</oboInOwl:hasDbXref>
</owl:Class>

<owl:Class rdf:about="&obo;FOODON_03400764">
	<rdfs:label xml:lang="en">068  vegetable oils, edible (or refined) (or) (ccpr)</rdfs:label>
	<rdfs:subClassOf rdf:resource="&obo;FOODON_03400661"/>
	<obo:IAO_0000412>http://langual.org</obo:IAO_0000412>
	<obo:IAO_0000115 xml:lang="en">Vegetable oils, edible (or refined) includes the vegetable oil derived from oil seed, Group 023, tropical and sub-tropical oil-containing fruits such as olives, and some pulses with a high oil content. The edible oils are derived from the crude oils though a refining and/or clarifying process. For definitions and characteristics of the edible oils listed below, see Codex Stan. 20-27 (inclusive), 33,124 and 126 (inclusive) - 1981.
Exposure to pesticides is through pre-harvest treatment of the relevant crops, or post-harvest treatment of the oilseeds and oil containing pulses.</obo:IAO_0000115>
	<obo:IAO_0000114 rdf:resource="&obo;IAO_0000428"/>
	<oboInOwl:hasDbXref>LANGUAL:A0764</oboInOwl:hasDbXref>
</owl:Class>

<owl:Class rdf:about="&obo;FOODON_03400765">
	<rdfs:label xml:lang="en">069  miscellaneous derived edible products of plant origin (dm) (ccpr)</rdfs:label>
	<rdfs:subClassOf rdf:resource="&obo;FOODON_03400661"/>
	<obo:IAO_0000412>http://langual.org</obo:IAO_0000412>
	<obo:IAO_0000115 xml:lang="en">Miscellaneous derived edible products include various intermediate products in the manufacture of edible food products. Some of these are used for further processing and not consumed as food or feed as such.</obo:IAO_0000115>
	<obo:IAO_0000114 rdf:resource="&obo;IAO_0000428"/>
	<oboInOwl:hasDbXref>LANGUAL:A0765</oboInOwl:hasDbXref>
</owl:Class>

<owl:Class rdf:about="&obo;FOODON_03400766">
	<rdfs:label xml:lang="en">070  fruit juices (jf) (ccpr)</rdfs:label>
	<rdfs:subClassOf rdf:resource="&obo;FOODON_03400661"/>
	<obo:IAO_0000412>http://langual.org</obo:IAO_0000412>
	<obo:IAO_0000115 xml:lang="en">Fruit juices are pressed from various mature fruits, either from the whole fruits or from the pulp (Type 1 and fruits from fruiting vegetables, Groups 011 and 012). A small amount of preserving agent(s) may be added to the juices during processing. The juices are often prepared for international trade in a concentrated form which is reconstituted for wholesale or retail distribution to about the original juice concentration as obtained by the pressing process.</obo:IAO_0000115>
	<obo:IAO_0000114 rdf:resource="&obo;IAO_0000428"/>
	<oboInOwl:hasDbXref>LANGUAL:A0766</oboInOwl:hasDbXref>
</owl:Class>

<owl:Class rdf:about="&obo;FOODON_03400767">
	<rdfs:label xml:lang="en">071  by-products, used for animal feeding purposes, derived from fruit and vegetable processing (ab) (ccpr)</rdfs:label>
	<rdfs:subClassOf rdf:resource="&obo;FOODON_03400661"/>
	<obo:IAO_0000412>http://langual.org</obo:IAO_0000412>
	<obo:IAO_0000115 xml:lang="en">The commodities of this group are by-products derived from fruit and vegetable processing which are mainly used for animal feeding purposes either as a part of the ration of livestock animals as such, or as an element in the manufacture of compounded feeds. The commodities are prepared, in general, in a dry form for wholesale or retail distribution.</obo:IAO_0000115>
	<obo:IAO_0000114 rdf:resource="&obo;IAO_0000428"/>
	<oboInOwl:hasDbXref>LANGUAL:A0767</oboInOwl:hasDbXref>
</owl:Class>

<owl:Class rdf:about="&obo;FOODON_03400768">
	<rdfs:label xml:lang="en">078  manufactured multi-ingredient cereal products (cp) (ccpr)</rdfs:label>
	<rdfs:subClassOf rdf:resource="&obo;FOODON_03400663"/>
	<obo:IAO_0000412>http://langual.org</obo:IAO_0000412>
	<obo:IAO_0000115 xml:lang="en">The commodities of this group are manufactured with several ingredients; products derived from cereal grains however form the major ingredient.</obo:IAO_0000115>
	<obo:IAO_0000114 rdf:resource="&obo;IAO_0000428"/>
	<oboInOwl:hasDbXref>LANGUAL:A0768</oboInOwl:hasDbXref>
</owl:Class>

<owl:Class rdf:about="&obo;FOODON_03400769">
	<rdfs:label xml:lang="en">080  dried meat and fish products (md) (ccpr)</rdfs:label>
	<rdfs:subClassOf rdf:resource="&obo;FOODON_03400664"/>
	<obo:IAO_0000412>http://langual.org</obo:IAO_0000412>
	<obo:IAO_0000115 xml:lang="en">Dried meat and fish products, includes natural or artificial dried meat products and dried fishes, mainly marine fishes. Most of the dried fishes are naturally dried (wind and sun). For convenience other marine animals, whether or not fishes or Crustaceans, are classified in this group.
The entire commodity may be consumed, either as such or after processing (c.q. dried fish).</obo:IAO_0000115>
	<obo:IAO_0000114 rdf:resource="&obo;IAO_0000428"/>
	<oboInOwl:hasDbXref>LANGUAL:A0769</oboInOwl:hasDbXref>
</owl:Class>

<owl:Class rdf:about="&obo;FOODON_03400770">
	<rdfs:label xml:lang="en">082  secondary milk products (ls) (ccpr)</rdfs:label>
	<rdfs:subClassOf rdf:resource="&obo;FOODON_03400665"/>
	<obo:IAO_0000412>http://langual.org</obo:IAO_0000412>
	<obo:IAO_0000115 xml:lang="en">Secondary milk products include milk products which have undergone simple processing such as removal or part removal of certain ingredients e.g. water, milk fat etc. The group and the commodities therein will only be used for pesticides which are not partitioned exclusively or nearly exclusively into the milk fat.
The group includes among others the following commodities as defined in the relevant Codex Standards, see CAC/VOL. XVI-Ed. 1 (1984). The reference no. of the standard is indicated between brackets.
Milk powders (whole, skimmed and partly skimmed) (Standard A-5 1971); evaporated milks (whole, skimmed) (Standard A-3 1971); skimmed milk.
Specific commodities will be listed in this group with their code nos. accordingly as the necessity for this arises.</obo:IAO_0000115>
	<obo:IAO_0000114 rdf:resource="&obo;IAO_0000428"/>
	<oboInOwl:hasDbXref>LANGUAL:A0770</oboInOwl:hasDbXref>
</owl:Class>

<owl:Class rdf:about="&obo;FOODON_03400771">
	<rdfs:label xml:lang="en">084  crustaceans, processed (sc) (ccpr)</rdfs:label>
	<rdfs:subClassOf rdf:resource="&obo;FOODON_03400665"/>
	<obo:IAO_0000412>http://langual.org</obo:IAO_0000412>
	<obo:IAO_0000115 xml:lang="en">Crustaceans are processed to a large extent before entering the national or international trade channels.
Crabs, lobsters and shrimps or prawns are in general cooked directly after catching. Thereafter either the animals are deep frozen with or without shell, or the meat without shell is canned, with or without a packing medium. The latter may consist of water, salt, lemon juice and sugars.
Shrimps or prawns may also be "parboiled" and thereafter deep-frozen.
According to the relevant Codex Standards, namely 92-1981, and 95-1981 "cooked" means heated for a period of time such that the thermal centre reaches a temperature adequate to coagulate the protein and "parboiled" means heated for a period of such time that the surface of the product Codex Alimentarius reaches a temperature adequate to coagulate the protein at the surface but inadequate to coagulate the protein at the thermal centre.
The cooked commodities are in general subjected to deep-freezing directly after cooking or the cooking is part of the canning process.
The designation cooked after the commodity may include any of the processes mentioned except the parboiled and deep-frozen shrimps or prawns.
The entire commodity except the shell may be consumed.</obo:IAO_0000115>
	<obo:IAO_0000114 rdf:resource="&obo;IAO_0000428"/>
	<oboInOwl:hasDbXref>LANGUAL:A0771</oboInOwl:hasDbXref>
</owl:Class>

<owl:Class rdf:about="&obo;FOODON_03400772">
	<rdfs:label xml:lang="en">085  animal fats, processed (fa) (ccpr)</rdfs:label>
	<rdfs:subClassOf rdf:resource="&obo;FOODON_03400665"/>
	<obo:IAO_0000412>http://langual.org</obo:IAO_0000412>
	<obo:IAO_0000115 xml:lang="en">The processed animal fats include rendered or extracted (possibly refined and/or clarified) fats from land and aquatic mammals and poultry and fats and oils derived from fishes.</obo:IAO_0000115>
	<obo:IAO_0000114 rdf:resource="&obo;IAO_0000428"/>
	<oboInOwl:hasDbXref>LANGUAL:A0772</oboInOwl:hasDbXref>
</owl:Class>

<owl:Class rdf:about="&obo;FOODON_03400773">
	<rdfs:label xml:lang="en">086  milk fats (fm) (ccpr)</rdfs:label>
	<rdfs:subClassOf rdf:resource="&obo;FOODON_03400665"/>
	<obo:IAO_0000412>http://langual.org</obo:IAO_0000412>
	<obo:IAO_0000115 xml:lang="en">Milk fats are the fatty ingredients derived from the milk of various mammals</obo:IAO_0000115>
	<obo:IAO_0000114 rdf:resource="&obo;IAO_0000428"/>
	<oboInOwl:hasDbXref>LANGUAL:A0773</oboInOwl:hasDbXref>
</owl:Class>

<owl:Class rdf:about="&obo;FOODON_03400774">
	<rdfs:label xml:lang="en">087  derived milk products (ld) (ccpr)</rdfs:label>
	<rdfs:subClassOf rdf:resource="&obo;FOODON_03400665"/>
	<obo:IAO_0000412>http://langual.org</obo:IAO_0000412>
	<obo:IAO_0000115 xml:lang="en">Derived milk products include food or edible substances isolated from the primary food commodity cattle milk, or milks from other mammals, using physical, biological and chemical processes. This group and the commodities therein will only be used if necessary for pesticides which are not partitioned exclusively or nearly exclusively into the milk fat. For further explanation, see Group 082.
This group includes among others the following food commodities, as defined in the relevant Codex Standards, see CAC/VOL. XXI, Ed-1 (1984): Butter, whey butter, both in Standard A-1 (1971), Butteroil, anhydrous butteroil, both in Standard A-2 (1973); Cream, Standard A-9 (1976); Cream powders (half cream, high fat), Standard A-10 (1971); Edible acid casein, Standard A-12 (1976): Edible caseinates, Standard A-13 (1976).
Specific commodities will be listed in this group with their code nos. accordingly as the necessity for this arises.</obo:IAO_0000115>
	<obo:IAO_0000114 rdf:resource="&obo;IAO_0000428"/>
	<oboInOwl:hasDbXref>LANGUAL:A0774</oboInOwl:hasDbXref>
</owl:Class>

<owl:Class rdf:about="&obo;FOODON_03400775">
	<rdfs:label xml:lang="en">090  manufactured milk products (single ingredient) of animal origin (li) (ccpr)</rdfs:label>
	<rdfs:subClassOf rdf:resource="&obo;FOODON_03400666"/>
	<obo:IAO_0000412>http://langual.org</obo:IAO_0000412>
	<obo:IAO_0000115 xml:lang="en">This group and the commodities therein will only be used, if the necessity arises, for pesticides which are not partitioned exclusively or nearly exclusively into the milk fat. For further explanation see Group 0 82.
This group includes among others the following food commodities, as defined in the relevant Codex Standards (indicated between brackets); Yoghurt (Codex Standard A-11(a) 1975); Cheeses, individually named (Codex Standard A-6 1978 and Standard Standard C-1 (1966-1978).
Specific commodities will be listed in this group with their code nos. accordingly as the necessity for this arises</obo:IAO_0000115>
	<obo:IAO_0000114 rdf:resource="&obo;IAO_0000428"/>
	<oboInOwl:hasDbXref>LANGUAL:A0775</oboInOwl:hasDbXref>
</owl:Class>

<owl:Class rdf:about="&obo;FOODON_03400776">
	<rdfs:label xml:lang="en">092  manufactured milk products (multi-ingredient) of animal origin (lm) (ccpr)</rdfs:label>
	<rdfs:subClassOf rdf:resource="&obo;FOODON_03400667"/>
	<obo:IAO_0000412>http://langual.org</obo:IAO_0000412>
	<obo:IAO_0000115 xml:lang="en">This group and the commodities therein will only be used in the classification if necessary for pesticides which are not partitioned exclusively or nearly exclusively into the milk fat. For further explanation see Group 082.
This group includes among others the following commodities, as defined in the relevant Codex Standards, see CAC/VOL.XVI, Ed-1 (1984); Processed Cheese Products, Codex Standard A-8(a) and A-8(b) (1978) Processed Cheese Preparations, Standard A-8(c) (1978); Flavoured Yoghurt, Standard A-11(b) (1976); Sweetened Condensed Milk, Standard A-4 (1971).
Specific commodities will be listed in this group with their code nos. accordingly as the necessity for this arises.</obo:IAO_0000115>
	<obo:IAO_0000114 rdf:resource="&obo;IAO_0000428"/>
	<oboInOwl:hasDbXref>LANGUAL:A0776</oboInOwl:hasDbXref>
</owl:Class>

<owl:Class rdf:about="&obo;FOODON_03400777">
	<rdfs:label xml:lang="en">eurofir food classification</rdfs:label>
	<rdfs:subClassOf rdf:resource="&obo;FOODON_03400356"/>
	<obo:IAO_0000412>http://langual.org</obo:IAO_0000412>
	<obo:IAO_0000114 rdf:resource="&obo;IAO_0000428"/>
	<rdfs:comment xml:lang="en">LanguaL curation note: This term is for CLASSIFICATION ONLY; DO NOT USE term in indexing. Use a more precise narrower term.</rdfs:comment>
	<oboInOwl:hasDbXref>LANGUAL:A0777</oboInOwl:hasDbXref>
</owl:Class>

<owl:Class rdf:about="&obo;FOODON_03400778">
	<rdfs:label xml:lang="en">milk, milk product or milk substitute (eurofir)</rdfs:label>
	<rdfs:subClassOf rdf:resource="&obo;FOODON_03400777"/>
	<obo:IAO_0000412>http://langual.org</obo:IAO_0000412>
	<obo:IAO_0000115 xml:lang="en">This category includes: liquid milks and processed milks; cream; milk products including fermented milk products, yoghurts and cheeses; milk product substitutes (e.g. made from soya); milk beverage powders; dairy ice cream. The category does not include butter and butter spreads (under *FAT OR OIL*); sauces and soups with a milk product as the main ingredient (under *PREPARED FOOD PRODUCT*). Index infant formula under *FOOD FOR SPECIAL NUTRITIONAL USE*.</obo:IAO_0000115>
	<obo:IAO_0000114 rdf:resource="&obo;IAO_0000428"/>
	<oboInOwl:hasSynonym xml:lang="en">dairy product</oboInOwl:hasSynonym>
	<oboInOwl:hasDbXref>LANGUAL:A0778</oboInOwl:hasDbXref>
</owl:Class>

<owl:Class rdf:about="&obo;FOODON_03400779">
	<rdfs:label xml:lang="en">milk (eurofir)</rdfs:label>
	<rdfs:subClassOf rdf:resource="&obo;FOODON_03400778"/>
	<obo:IAO_0000412>http://langual.org</obo:IAO_0000412>
	<obo:IAO_0000115 xml:lang="en">Milk in all forms, milk-based beverage, cultured milk product, or milk.</obo:IAO_0000115>
	<obo:IAO_0000114 rdf:resource="&obo;IAO_0000428"/>
	<rdfs:comment xml:lang="en">LanguaL curation note: Index also * MILK OR MILK COMPONENT* or underlying term in facet C.</rdfs:comment>
	<oboInOwl:hasDbXref>LANGUAL:A0779</oboInOwl:hasDbXref>
</owl:Class>

<owl:Class rdf:about="&obo;FOODON_03400780">
	<rdfs:label xml:lang="en">liquid milk (eurofir)</rdfs:label>
	<rdfs:subClassOf rdf:resource="&obo;FOODON_03400779"/>
	<obo:IAO_0000412>http://langual.org</obo:IAO_0000412>
	<obo:IAO_0000115 xml:lang="en">Liquid milks are the secretion of the mammary gland of animals such as cow, sheep, goat, buffalo and camel, and include Human milk. The category includes milks that have only been processed for reasons of food safety (e.g. pasteurisation), preservation (e.g. UHT) or skimming to reduce fat content.</obo:IAO_0000115>
	<obo:IAO_0000114 rdf:resource="&obo;IAO_0000428"/>
	<rdfs:comment xml:lang="en">LanguaL curation note: Index also *MILK* in facet C.</rdfs:comment>
	<oboInOwl:hasDbXref>LANGUAL:A0780</oboInOwl:hasDbXref>
</owl:Class>

<owl:Class rdf:about="&obo;FOODON_03400781">
	<rdfs:label xml:lang="en">processed milk (eurofir)</rdfs:label>
	<rdfs:subClassOf rdf:resource="&obo;FOODON_03400779"/>
	<obo:IAO_0000412>http://langual.org</obo:IAO_0000412>
	<obo:IAO_0000115 xml:lang="en">Processed milks are milks that have been subject to processing that modifies their consistency (e.g. evaporated milk) and/or composition other than fat content (e.g. whey). The group also includes milk-based drinks like milkshakes.</obo:IAO_0000115>
	<obo:IAO_0000114 rdf:resource="&obo;IAO_0000428"/>
	<rdfs:comment xml:lang="en">LanguaL curation note: Index also *MILK OR MILK COMPONENT* or underlying term in facet C.</rdfs:comment>
	<oboInOwl:hasDbXref>LANGUAL:A0781</oboInOwl:hasDbXref>
</owl:Class>

<owl:Class rdf:about="&obo;FOODON_03400782">
	<rdfs:label xml:lang="en">cream (eurofir)</rdfs:label>
	<rdfs:subClassOf rdf:resource="&obo;FOODON_03400779"/>
	<obo:IAO_0000412>http://langual.org</obo:IAO_0000412>
	<obo:IAO_0000115 xml:lang="en">Includes fresh cream, crème fraîche and sour cream.</obo:IAO_0000115>
	<obo:IAO_0000114 rdf:resource="&obo;IAO_0000428"/>
	<rdfs:comment xml:lang="en">LanguaL curation note: Index also *CREAM* or underlying terms in facet C.</rdfs:comment>
	<oboInOwl:hasDbXref>LANGUAL:A0782</oboInOwl:hasDbXref>
</owl:Class>

<owl:Class rdf:about="&obo;FOODON_03400783">
	<rdfs:label xml:lang="en">fermented milk product (eurofir)</rdfs:label>
	<rdfs:subClassOf rdf:resource="&obo;FOODON_03400778"/>
	<obo:IAO_0000412>http://langual.org</obo:IAO_0000412>
	<obo:IAO_0000115 xml:lang="en">Fermented milk is a milk product obtained by fermentation of milk, which milk may have been manufactured from products obtained from milk with or without compositional modification as limited by the provision in Section 3.3, by the action of suitable microorganisms and resulting in reduction of pH with or without coagulation (CODEX STAN 243-2003).  Fermented milk products include a range of foods commonly referred to as yogurt (or yoghurt), plus sour milk drinks produced by fermentation. A few of these are alcoholic as they are made with combined lactic and yeast ferments (e.g. kefir, koumiss); others are lactic fermented milk products (e.g. cieddu, kaeder milk, skyr, taette). In some traditional fermented milk products, such as Stragisto (strained yoghurt), Labneh, Ymer and Ylette, Milk the protein has been increased to minimum 5.6%.  .</obo:IAO_0000115>
	<obo:IAO_0000114 rdf:resource="&obo;IAO_0000428"/>
	<oboInOwl:hasSynonym xml:lang="en">cultured milk product</oboInOwl:hasSynonym>
	<oboInOwl:hasDbXref>LANGUAL:A0783</oboInOwl:hasDbXref>
</owl:Class>

<owl:Class rdf:about="&obo;FOODON_03400784">
	<rdfs:label xml:lang="en">cheese (eurofir)</rdfs:label>
	<rdfs:subClassOf rdf:resource="&obo;FOODON_03400778"/>
	<obo:IAO_0000412>http://langual.org</obo:IAO_0000412>
	<obo:IAO_0000115 xml:lang="en">Cheese is the ripened or unripened soft or semi-hard, hard and extra hard product, which may be coated, and in which the whey protein/casein ratio does not exceed that of milk, obtained by : coagulating wholly or partly  through the action of rennet or other suitable coagulating agents, and by partially draining the whey resulting from such coagulation; and/or processing techniques involving coagulation of the protein of milk and/or products obtained from milk which give an end-product with similar physical, chemical and organoleptic characteristics (CODEX STAN A-6-1978, Rev.1-1999, Amended 2003). The group includes goat and sheep cheeses, and cheeses made from sour milk, whey or buttermilk.</obo:IAO_0000115>
	<obo:IAO_0000114 rdf:resource="&obo;IAO_0000428"/>
	<rdfs:comment xml:lang="en">LanguaL curation note: Index also * MILK OR MILK COMPONENT* or underlying term in facet C.</rdfs:comment>
	<oboInOwl:hasDbXref>LANGUAL:A0784</oboInOwl:hasDbXref>
</owl:Class>

<owl:Class rdf:about="&obo;FOODON_03400785">
	<rdfs:label xml:lang="en">cured cheese (eurofir)</rdfs:label>
	<rdfs:subClassOf rdf:resource="&obo;FOODON_03400784"/>
	<obo:IAO_0000412>http://langual.org</obo:IAO_0000412>
	<obo:IAO_0000115 xml:lang="en">Ripened cheese is cheese which is not ready for consumption shortly after manufacture but which must be held for such time, at such temperature, and under such other conditions as will result in the necessary biochemical and physical changes characterizing the cheese in question. (CODEX STAN A-6-1978, Rev.1-1999, Amended 2003). The group includes cheeses that are normally consumed cured but may be sold in an uncured or very lightly cured stage.</obo:IAO_0000115>
	<obo:IAO_0000114 rdf:resource="&obo;IAO_0000428"/>
	<rdfs:comment xml:lang="en">LanguaL curation note: Cheeses are classified here according to their consistency (Codex Alimentarius Standard). Cheeses can be further distinguished according to fat content and rind type in facet Z.</rdfs:comment>
	<oboInOwl:hasSynonym xml:lang="en">ripened cheese</oboInOwl:hasSynonym>
	<oboInOwl:hasDbXref>LANGUAL:A0785</oboInOwl:hasDbXref>
</owl:Class>

<owl:Class rdf:about="&obo;FOODON_03400786">
	<rdfs:label xml:lang="en">uncured cheese (eurofir)</rdfs:label>
	<rdfs:subClassOf rdf:resource="&obo;FOODON_03400784"/>
	<obo:IAO_0000412>http://langual.org</obo:IAO_0000412>
	<obo:IAO_0000115 xml:lang="en">Unripened cheese including fresh cheese is cheese which is ready for consumption shortly after manufacture (CODEX STAN A-6-1978, Rev.1-1999, Amended 2003). It is consumed fresh and has a mild acid flavour, moisture max. 80%. Includes such products as cream cheese and mozzarella cheese.</obo:IAO_0000115>
	<obo:IAO_0000114 rdf:resource="&obo;IAO_0000428"/>
	<oboInOwl:hasSynonym xml:lang="en">unripened cheese</oboInOwl:hasSynonym>
	<oboInOwl:hasDbXref>LANGUAL:A0786</oboInOwl:hasDbXref>
</owl:Class>

<owl:Class rdf:about="&obo;FOODON_03400787">
	<rdfs:label xml:lang="en">processed cheese (eurofir)</rdfs:label>
	<rdfs:subClassOf rdf:resource="&obo;FOODON_03400784"/>
	<obo:IAO_0000412>http://langual.org</obo:IAO_0000412>
	<obo:IAO_0000115 xml:lang="en">Process(ed) cheese and spreadable process(ed) cheese are made by grinding, mixing, melting and emulsifying with the aid of heat and emulsifying agents one or more varieties of cheese, with or without the addition of milk components and/or other foodstuffs (CODEX STAN A-8(b)-1978). The result is a homogeneous plastic mass, except for grated cheese product, which is powdered or granular.</obo:IAO_0000115>
	<obo:IAO_0000114 rdf:resource="&obo;IAO_0000428"/>
	<oboInOwl:hasDbXref>LANGUAL:A0787</oboInOwl:hasDbXref>
</owl:Class>

<owl:Class rdf:about="&obo;FOODON_03400788">
	<rdfs:label xml:lang="en">immitation milk products (eurofir)</rdfs:label>
	<rdfs:subClassOf rdf:resource="&obo;FOODON_03400778"/>
	<obo:IAO_0000412>http://langual.org</obo:IAO_0000412>
	<obo:IAO_0000115 xml:lang="en">The group includes soya milk, soya cheese, non-dairy coffee creamer.</obo:IAO_0000115>
	<obo:IAO_0000114 rdf:resource="&obo;IAO_0000428"/>
	<oboInOwl:hasSynonym xml:lang="en">milk product analog</oboInOwl:hasSynonym>
	<oboInOwl:hasDbXref>LANGUAL:A0788</oboInOwl:hasDbXref>
</owl:Class>

<owl:Class rdf:about="&obo;FOODON_03400789">
	<rdfs:label xml:lang="en">frozen dairy dessert (eurofir)</rdfs:label>
	<rdfs:subClassOf rdf:resource="&obo;FOODON_03400778"/>
	<obo:IAO_0000412>http://langual.org</obo:IAO_0000412>
	<obo:IAO_0000115 xml:lang="en">A frozen dessert prepared from one or more dairy ingredients plus other ingredients.</obo:IAO_0000115>
	<obo:IAO_0000114 rdf:resource="&obo;IAO_0000428"/>
	<rdfs:comment xml:lang="en">LanguaL curation note: Includes frozen dairy items offered in a cone, a sandwich or as a cake or pie, such as frozen yogurt in a cone or an ice cream sandwich; these are also indexed under *GRAIN ADDED*. Non-dairy ices (e.g. Water ices, granitas, sorbets) are classified under *DESSERT*.</rdfs:comment>
	<oboInOwl:hasDbXref>LANGUAL:A0789</oboInOwl:hasDbXref>
</owl:Class>

<owl:Class rdf:about="&obo;FOODON_03400790">
	<rdfs:label xml:lang="en">egg or egg product (eurofir)</rdfs:label>
	<rdfs:subClassOf rdf:resource="&obo;FOODON_03400777"/>
	<obo:IAO_0000412>http://langual.org</obo:IAO_0000412>
	<obo:IAO_0000115 xml:lang="en">The group includes bird eggs, food product whose predominant constituent is eggs, recipe dishes whose main ingredient is considered to be eggs. It does not include fish roe (under Fish).</obo:IAO_0000115>
	<obo:IAO_0000114 rdf:resource="&obo;IAO_0000428"/>
	<oboInOwl:hasDbXref>LANGUAL:A0790</oboInOwl:hasDbXref>
</owl:Class>

<owl:Class rdf:about="&obo;FOODON_03400791">
	<rdfs:label xml:lang="en">fresh or processed egg (eurofir)</rdfs:label>
	<rdfs:subClassOf rdf:resource="&obo;FOODON_03400790"/>
	<obo:IAO_0000412>http://langual.org</obo:IAO_0000412>
	<obo:IAO_0000115 xml:lang="en">e.g. chicken eggs, duck eggs, egg yolk, egg products such as dried eggs</obo:IAO_0000115>
	<obo:IAO_0000114 rdf:resource="&obo;IAO_0000428"/>
	<oboInOwl:hasDbXref>LANGUAL:A0791</oboInOwl:hasDbXref>
</owl:Class>

<owl:Class rdf:about="&obo;FOODON_03400792">
	<rdfs:label xml:lang="en">egg dish (eurofir)</rdfs:label>
	<rdfs:subClassOf rdf:resource="&obo;FOODON_03400790"/>
	<rdfs:subClassOf rdf:resource="&obo;FOODON_03400861"/>
	<obo:IAO_0000412>http://langual.org</obo:IAO_0000412>
	<obo:IAO_0000115 xml:lang="en">Dishes whose predominant ingredient is seen to be eggs, e.g. omelette, soufflé, meringue, eggnog.</obo:IAO_0000115>
	<obo:IAO_0000114 rdf:resource="&obo;IAO_0000428"/>
	<oboInOwl:hasDbXref>LANGUAL:A0792</oboInOwl:hasDbXref>
</owl:Class>

<owl:Class rdf:about="&obo;FOODON_03400793">
	<rdfs:label xml:lang="en">meat or meat product (eurofir)</rdfs:label>
	<rdfs:subClassOf rdf:resource="&obo;FOODON_03400777"/>
	<obo:IAO_0000412>http://langual.org</obo:IAO_0000412>
	<obo:IAO_0000115 xml:lang="en">This category includes: carcass meat of mammals and birds; offal of mammals and birds; a food product whose predominant constituent is meat; a recipe dish whose main ingredient is considered to be meat.</obo:IAO_0000115>
	<obo:IAO_0000114 rdf:resource="&obo;IAO_0000428"/>
	<oboInOwl:hasDbXref>LANGUAL:A0793</oboInOwl:hasDbXref>
</owl:Class>

<owl:Class rdf:about="&obo;FOODON_03400794">
	<rdfs:label xml:lang="en">red meat (eurofir)</rdfs:label>
	<rdfs:subClassOf rdf:resource="&obo;FOODON_03400793"/>
	<obo:IAO_0000412>http://langual.org</obo:IAO_0000412>
	<obo:IAO_0000115 xml:lang="en">The group includes carcass meat of domestic animals (e.g. beef, veal, pork, mutton / lamb, horse, rabbit) and game (e.g. wild pig, boar, venison, whale).</obo:IAO_0000115>
	<obo:IAO_0000114 rdf:resource="&obo;IAO_0000428"/>
	<oboInOwl:hasDbXref>LANGUAL:A0794</oboInOwl:hasDbXref>
</owl:Class>

<owl:Class rdf:about="&obo;FOODON_03400795">
	<rdfs:label xml:lang="en">poultry meat (eurofir)</rdfs:label>
	<rdfs:subClassOf rdf:resource="&obo;FOODON_03400793"/>
	<obo:IAO_0000412>http://langual.org</obo:IAO_0000412>
	<obo:IAO_0000115 xml:lang="en">The group includes carcass meat of domestic poultry (e.g. chicken, turkey, duck, goose) and game birds (e.g. pheasant, partridge, sea birds)</obo:IAO_0000115>
	<obo:IAO_0000114 rdf:resource="&obo;IAO_0000428"/>
	<oboInOwl:hasDbXref>LANGUAL:A0795</oboInOwl:hasDbXref>
</owl:Class>

<owl:Class rdf:about="&obo;FOODON_03400796">
	<rdfs:label xml:lang="en">offal (eurofir)</rdfs:label>
	<rdfs:subClassOf rdf:resource="&obo;FOODON_03400793"/>
	<obo:IAO_0000412>http://langual.org</obo:IAO_0000412>
	<obo:IAO_0000115 xml:lang="en">e.g. liver, kidney, tongue, heart, trotters, giblets.</obo:IAO_0000115>
	<obo:IAO_0000114 rdf:resource="&obo;IAO_0000428"/>
	<rdfs:comment xml:lang="en">LanguaL curation note: Index also *ORGAN MEAT* or underlying terms in facet C.</rdfs:comment>
	<oboInOwl:hasDbXref>LANGUAL:A0796</oboInOwl:hasDbXref>
</owl:Class>

<owl:Class rdf:about="&obo;FOODON_03400797">
	<rdfs:label xml:lang="en">preserved meat (eurofir)</rdfs:label>
	<rdfs:subClassOf rdf:resource="&obo;FOODON_03400793"/>
	<obo:IAO_0000412>http://langual.org</obo:IAO_0000412>
	<obo:IAO_0000115 xml:lang="en">e.g. ham, bacon, corned beef</obo:IAO_0000115>
	<obo:IAO_0000114 rdf:resource="&obo;IAO_0000428"/>
	<oboInOwl:hasSynonym xml:lang="en">cured meat</oboInOwl:hasSynonym>
	<oboInOwl:hasDbXref>LANGUAL:A0797</oboInOwl:hasDbXref>
</owl:Class>

<owl:Class rdf:about="&obo;FOODON_03400798">
	<rdfs:label xml:lang="en">sausage or similar meat product (eurofir)</rdfs:label>
	<rdfs:subClassOf rdf:resource="&obo;FOODON_03400793"/>
	<obo:IAO_0000412>http://langual.org</obo:IAO_0000412>
	<obo:IAO_0000115 xml:lang="en">includes: pastes, pâtés and terrines; sausage meat; dry, smoked sausages (rohwurst); fresh and lightly cooked sausages (bratwurst); cooked sausages (kochwurst); blood &amp; blood products (e.g. haggis, black pudding); other meat products (e.g. galantine, brawn).</obo:IAO_0000115>
	<obo:IAO_0000114 rdf:resource="&obo;IAO_0000428"/>
	<oboInOwl:hasDbXref>LANGUAL:A0798</oboInOwl:hasDbXref>
</owl:Class>

<owl:Class rdf:about="&obo;FOODON_03400799">
	<rdfs:label xml:lang="en">meat dish (eurofir)</rdfs:label>
	<rdfs:subClassOf rdf:resource="&obo;FOODON_03400793"/>
	<rdfs:subClassOf rdf:resource="&obo;FOODON_03400861"/>
	<obo:IAO_0000412>http://langual.org</obo:IAO_0000412>
	<obo:IAO_0000115 xml:lang="en">Dishes whose predominant ingredient is seen to be meat; e.g. stew, meat burger, meat balls, meat pie or pasty</obo:IAO_0000115>
	<obo:IAO_0000114 rdf:resource="&obo;IAO_0000428"/>
	<oboInOwl:hasDbXref>LANGUAL:A0799</oboInOwl:hasDbXref>
</owl:Class>

<owl:Class rdf:about="&obo;FOODON_03400800">
	<rdfs:label xml:lang="en">meat analogue (eurofir)</rdfs:label>
	<rdfs:subClassOf rdf:resource="&obo;FOODON_03400793"/>
	<obo:IAO_0000412>http://langual.org</obo:IAO_0000412>
	<obo:IAO_0000115 xml:lang="en">e.g. textured vegetable protein.</obo:IAO_0000115>
	<obo:IAO_0000114 rdf:resource="&obo;IAO_0000428"/>
	<rdfs:comment xml:lang="en">LanguaL curation note: Index the food source (e.g. soy) in facet B.</rdfs:comment>
	<oboInOwl:hasDbXref>LANGUAL:A0800</oboInOwl:hasDbXref>
</owl:Class>

<owl:Class rdf:about="&obo;FOODON_03400801">
	<rdfs:label xml:lang="en">seafood or related product (eurofir)</rdfs:label>
	<rdfs:subClassOf rdf:resource="&obo;FOODON_03400777"/>
	<obo:IAO_0000412>http://langual.org</obo:IAO_0000412>
	<obo:IAO_0000115 xml:lang="en">The group includes marine or freshwater fish, molluscs, crustaceans, and other fauna such as reptiles, insects or frogs not in the Meats group. The group also includes seafood product analogs and seafood-based sausage or luncheon meat as well as such products as squid ink and clam juice.</obo:IAO_0000115>
	<obo:IAO_0000114 rdf:resource="&obo;IAO_0000428"/>
	<oboInOwl:hasDbXref>LANGUAL:A0801</oboInOwl:hasDbXref>
</owl:Class>

<owl:Class rdf:about="&obo;FOODON_03400802">
	<rdfs:label xml:lang="en">fish or related organism (eurofir)</rdfs:label>
	<rdfs:subClassOf rdf:resource="&obo;FOODON_03400801"/>
	<obo:IAO_0000412>http://langual.org</obo:IAO_0000412>
	<obo:IAO_0000115 xml:lang="en">Flesh from marine or freshwater fish, molluscs, crustaceans, and other fauna such as reptiles, insects or frogs not in the Meats group..</obo:IAO_0000115>
	<obo:IAO_0000114 rdf:resource="&obo;IAO_0000428"/>
	<oboInOwl:hasDbXref>LANGUAL:A0802</oboInOwl:hasDbXref>
</owl:Class>

<owl:Class rdf:about="&obo;FOODON_03400803">
	<rdfs:label xml:lang="en">seafood product (eurofir)</rdfs:label>
	<rdfs:subClassOf rdf:resource="&obo;FOODON_03400801"/>
	<obo:IAO_0000412>http://langual.org</obo:IAO_0000412>
	<obo:IAO_0000115 xml:lang="en">includes fish offal; a food product whose predominant constituent is fish (e.g. dried and salted fish, smoked fish, canned fish, pickled fish, restructured fish and fish analogues, surimi; fish paste, pâté).</obo:IAO_0000115>
	<obo:IAO_0000114 rdf:resource="&obo;IAO_0000428"/>
	<oboInOwl:hasDbXref>LANGUAL:A0803</oboInOwl:hasDbXref>
</owl:Class>

<owl:Class rdf:about="&obo;FOODON_03400804">
	<rdfs:label xml:lang="en">seafood dish (eurofir)</rdfs:label>
	<rdfs:subClassOf rdf:resource="&obo;FOODON_03400861"/>
	<rdfs:subClassOf rdf:resource="&obo;FOODON_03400803"/>
	<obo:IAO_0000412>http://langual.org</obo:IAO_0000412>
	<obo:IAO_0000115 xml:lang="en">A recipe dish whose main ingredient is considered to be fish</obo:IAO_0000115>
	<obo:IAO_0000114 rdf:resource="&obo;IAO_0000428"/>
	<oboInOwl:hasDbXref>LANGUAL:A0804</oboInOwl:hasDbXref>
</owl:Class>

<owl:Class rdf:about="&obo;FOODON_03400805">
	<rdfs:label xml:lang="en">fat or oil (eurofir)</rdfs:label>
	<rdfs:subClassOf rdf:resource="&obo;FOODON_03400777"/>
	<obo:IAO_0000412>http://langual.org</obo:IAO_0000412>
	<obo:IAO_0000115 xml:lang="en">Food substance or component consisting predominantly of mixed glycerol esters of fatty acids and, in far lesser amounts, of fatty acids, sterols and pigments. A fat is solid at room temperature; an oil is liquid at room temperature (20 degrees C). Excludes essential oils.</obo:IAO_0000115>
	<obo:IAO_0000114 rdf:resource="&obo;IAO_0000428"/>
	<rdfs:comment xml:lang="en">LanguaL curation note: Index also *FAT OR OIL* or subgroups in facet C.</rdfs:comment>
	<oboInOwl:hasDbXref>LANGUAL:A0805</oboInOwl:hasDbXref>
</owl:Class>

<owl:Class rdf:about="&obo;FOODON_03400806">
	<rdfs:label xml:lang="en">vegetable fat or oil (eurofir)</rdfs:label>
	<rdfs:subClassOf rdf:resource="&obo;FOODON_03400805"/>
	<obo:IAO_0000412>http://langual.org</obo:IAO_0000412>
	<obo:IAO_0000115 xml:lang="en">In this context, vegetable fats are oils that are solid at room temperature (e.g. palm oil, cocoa butter). It may also apply to hydrogenated (hardened) vegetable fats.</obo:IAO_0000115>
	<obo:IAO_0000114 rdf:resource="&obo;IAO_0000428"/>
	<oboInOwl:hasDbXref>LANGUAL:A0806</oboInOwl:hasDbXref>
</owl:Class>

<owl:Class rdf:about="&obo;FOODON_03400807">
	<rdfs:label xml:lang="en">margarine or lipid of mixed origin (eurofir)</rdfs:label>
	<rdfs:subClassOf rdf:resource="&obo;FOODON_03400805"/>
	<obo:IAO_0000412>http://langual.org</obo:IAO_0000412>
	<obo:IAO_0000115 xml:lang="en">Food product having functional characteristics similar to a butter product; it may be nutritionally equivalent or inferior to the product it purports to resemble.</obo:IAO_0000115>
	<obo:IAO_0000114 rdf:resource="&obo;IAO_0000428"/>
	<oboInOwl:hasDbXref>LANGUAL:A0807</oboInOwl:hasDbXref>
</owl:Class>

<owl:Class rdf:about="&obo;FOODON_03400808">
	<rdfs:label xml:lang="en">butter or other animal fat (eurofir)</rdfs:label>
	<rdfs:subClassOf rdf:resource="&obo;FOODON_03400805"/>
	<obo:IAO_0000412>http://langual.org</obo:IAO_0000412>
	<obo:IAO_0000115 xml:lang="en">EFG group 12.</obo:IAO_0000115>
	<obo:IAO_0000114 rdf:resource="&obo;IAO_0000428"/>
	<oboInOwl:hasDbXref>LANGUAL:A0808</oboInOwl:hasDbXref>
</owl:Class>

<owl:Class rdf:about="&obo;FOODON_03400809">
	<rdfs:label xml:lang="en">butter (eurofir)</rdfs:label>
	<rdfs:subClassOf rdf:resource="&obo;FOODON_03400808"/>
	<obo:IAO_0000412>http://langual.org</obo:IAO_0000412>
	<obo:IAO_0000115 xml:lang="en">e.g. butter, butter oil, ghee</obo:IAO_0000115>
	<obo:IAO_0000114 rdf:resource="&obo;IAO_0000428"/>
	<oboInOwl:hasDbXref>LANGUAL:A0809</oboInOwl:hasDbXref>
</owl:Class>

<owl:Class rdf:about="&obo;FOODON_03400810">
	<rdfs:label xml:lang="en">other animal fats (eurofir)</rdfs:label>
	<rdfs:subClassOf rdf:resource="&obo;FOODON_03400808"/>
	<obo:IAO_0000412>http://langual.org</obo:IAO_0000412>
	<obo:IAO_0000115 xml:lang="en">e.g. beef fat, goose fat</obo:IAO_0000115>
	<obo:IAO_0000114 rdf:resource="&obo;IAO_0000428"/>
	<oboInOwl:hasDbXref>LANGUAL:A0810</oboInOwl:hasDbXref>
</owl:Class>

<owl:Class rdf:about="&obo;FOODON_03400811">
	<rdfs:label xml:lang="en">fish oils (eurofir)</rdfs:label>
	<rdfs:subClassOf rdf:resource="&obo;FOODON_03400808"/>
	<obo:IAO_0000412>http://langual.org</obo:IAO_0000412>
	<obo:IAO_0000115 xml:lang="en">e.g. herring oil, sardine oil</obo:IAO_0000115>
	<obo:IAO_0000114 rdf:resource="&obo;IAO_0000428"/>
	<oboInOwl:hasDbXref>LANGUAL:A0811</oboInOwl:hasDbXref>
</owl:Class>

<owl:Class rdf:about="&obo;FOODON_03400812">
	<rdfs:label xml:lang="en">grain or grain product (eurofir)</rdfs:label>
	<rdfs:subClassOf rdf:resource="&obo;FOODON_03400777"/>
	<obo:IAO_0000412>http://langual.org</obo:IAO_0000412>
	<obo:IAO_0000115 xml:lang="en">This group includes: grains and their milled products obtained from members of the grass family; dough products obtained from grain, such as pasta and breads; breakfast cereals; savoury and sweet products and dishes in which grain products are considered the predominant constituent; substitute flours and other starch products obtained from non-cereal sources. It excludes sweet corn when eaten as a vegetable.</obo:IAO_0000115>
	<obo:IAO_0000114 rdf:resource="&obo;IAO_0000428"/>
	<oboInOwl:hasSynonym xml:lang="en">cereal product</oboInOwl:hasSynonym>
	<oboInOwl:hasDbXref>LANGUAL:A0812</oboInOwl:hasDbXref>
</owl:Class>

<owl:Class rdf:about="&obo;FOODON_03400813">
	<rdfs:label xml:lang="en">cereal or cereal-like milling products and derivatives (eurofir)</rdfs:label>
	<rdfs:subClassOf rdf:resource="&obo;FOODON_03400812"/>
	<obo:IAO_0000412>http://langual.org</obo:IAO_0000412>
	<obo:IAO_0000115 xml:lang="en">Examples: wheat flour, wholemeal, substitute flours and starches, wheat flour, patent, soya flour, rye flour, whole, potato flour, cornflour, carob flour, rice flour, arrowroot, buckwheat flour, tapioca</obo:IAO_0000115>
	<obo:IAO_0000114 rdf:resource="&obo;IAO_0000428"/>
	<rdfs:comment xml:lang="en">LanguaL curation note: Renamed from *FLOUR OR STARCH (EUROFIR)* (LanguaL 2010).</rdfs:comment>
	<oboInOwl:hasSynonym xml:lang="en">flour or starch</oboInOwl:hasSynonym>
	<oboInOwl:hasSynonym xml:lang="en">milled grain or starch product</oboInOwl:hasSynonym>
	<oboInOwl:hasDbXref>LANGUAL:A0813</oboInOwl:hasDbXref>
</owl:Class>

<owl:Class rdf:about="&obo;FOODON_03400814">
	<rdfs:label xml:lang="en">rice or other grain (eurofir)</rdfs:label>
	<rdfs:subClassOf rdf:resource="&obo;FOODON_03400812"/>
	<obo:IAO_0000412>http://langual.org</obo:IAO_0000412>
	<obo:IAO_0000115 xml:lang="en">Examples are whole grain wheat, brown rice, bulgur, parboiled rice, rolled oats, wild rice, pearl barley, millet, rolled oats, corn grits and similar products.</obo:IAO_0000115>
	<obo:IAO_0000114 rdf:resource="&obo;IAO_0000428"/>
	<oboInOwl:hasSynonym xml:lang="en">cereal grains</oboInOwl:hasSynonym>
	<oboInOwl:hasDbXref>LANGUAL:A0814</oboInOwl:hasDbXref>
</owl:Class>

<owl:Class rdf:about="&obo;FOODON_03400815">
	<rdfs:label xml:lang="en">pasta and similar products (eurofir)</rdfs:label>
	<rdfs:subClassOf rdf:resource="&obo;FOODON_03400812"/>
	<obo:IAO_0000412>http://langual.org</obo:IAO_0000412>
	<obo:IAO_0000115 xml:lang="en">Eurocode-2 group 06.30. Pasta can be either dried or fresh, and as main-dish (pasta asciutta) or miniature pasta (e.g. to add to soups). Although pasta is usually made from durum wheat flour, it can also be made from wholemeal flour or buckwheat flour. Noodles contain egg unless specifically referred to as plain noodles. Asian transparent noodles can made from a wide range of flours, many of them non-cereal.</obo:IAO_0000115>
	<obo:IAO_0000114 rdf:resource="&obo;IAO_0000428"/>
	<rdfs:comment xml:lang="en">LanguaL curation note: Renamed from *PASTA (EUROFIR)* (LanguaL 2010).</rdfs:comment>
	<oboInOwl:hasSynonym xml:lang="en">pasta</oboInOwl:hasSynonym>
	<oboInOwl:hasDbXref>LANGUAL:A0815</oboInOwl:hasDbXref>
</owl:Class>

<owl:Class rdf:about="&obo;FOODON_03400816">
	<rdfs:label xml:lang="en">breakfast cereal (eurofir)</rdfs:label>
	<rdfs:subClassOf rdf:resource="&obo;FOODON_03400812"/>
	<obo:IAO_0000412>http://langual.org</obo:IAO_0000412>
	<obo:IAO_0000115 xml:lang="en">Prepared grain product ready or nearly ready for consumption and marketed primarily for breakfast use. Includes formulated breakfast cereals such as 'corn flakes' or "muesli" and simple breakfast cereals such as instant oatmeal.</obo:IAO_0000115>
	<obo:IAO_0000114 rdf:resource="&obo;IAO_0000428"/>
	<rdfs:comment xml:lang="en">LanguaL curation note: Excludes rolled oats, corn grits and similar products, which are indexed under *RICE OR OTHER GRAIN *.</rdfs:comment>
	<oboInOwl:hasDbXref>LANGUAL:A0816</oboInOwl:hasDbXref>
</owl:Class>

<owl:Class rdf:about="&obo;FOODON_03400817">
	<rdfs:label xml:lang="en">bread and similar products (eurofir)</rdfs:label>
	<rdfs:subClassOf rdf:resource="&obo;FOODON_03400812"/>
	<obo:IAO_0000412>http://langual.org</obo:IAO_0000412>
	<obo:IAO_0000115 xml:lang="en">Products in the Bread categories normally have contents of sugars and fat neither exceeding 5% on a dry weight basis.</obo:IAO_0000115>
	<obo:IAO_0000114 rdf:resource="&obo;IAO_0000428"/>
	<rdfs:comment xml:lang="en">LanguaL curation note: Renamed from *BREAD (EUROFIR)* (LanguaL 2010).</rdfs:comment>
	<oboInOwl:hasSynonym xml:lang="en">bread</oboInOwl:hasSynonym>
	<oboInOwl:hasDbXref>LANGUAL:A0817</oboInOwl:hasDbXref>
</owl:Class>

<owl:Class rdf:about="&obo;FOODON_03400818">
	<rdfs:label xml:lang="en">leavened bread (eurofir)</rdfs:label>
	<rdfs:subClassOf rdf:resource="&obo;FOODON_03400817"/>
	<obo:IAO_0000412>http://langual.org</obo:IAO_0000412>
	<obo:IAO_0000115 xml:lang="en">includes wholemeal wheat bread, soda bread, rye bread</obo:IAO_0000115>
	<obo:IAO_0000114 rdf:resource="&obo;IAO_0000428"/>
	<oboInOwl:hasDbXref>LANGUAL:A0818</oboInOwl:hasDbXref>
</owl:Class>

<owl:Class rdf:about="&obo;FOODON_03400819">
	<rdfs:label xml:lang="en">unleavened bread, crisp bread and rusk (eurofir)</rdfs:label>
	<rdfs:subClassOf rdf:resource="&obo;FOODON_03400817"/>
	<obo:IAO_0000412>http://langual.org</obo:IAO_0000412>
	<obo:IAO_0000115 xml:lang="en">A flatbread, or unleavened bread, is a simple bread made with flour, water, and salt and then thoroughly rolled into flattened dough. Many flatbreads are unleavened-made without yeast or sourdough culture-although some flatbread is made with yeast, such as pita bread. There are many other optional ingredients that flatbreads may contain, such as curry powder, diced jalapeños, chili powder, or black pepper. Olive oil or sesame oil may be added as well. Flatbreads can range from one millimeter to a few centimeters thick. [Wikipedia].
Includes pitta bread, matzo, tortilla.</obo:IAO_0000115>
	<obo:IAO_0000114 rdf:resource="&obo;IAO_0000428"/>
	<rdfs:comment xml:lang="en">LanguaL curation note: Renamed from *FLATBREAD (EUROFIR)* (LanguaL 2010).</rdfs:comment>
	<oboInOwl:hasSynonym xml:lang="en">crisp bread</oboInOwl:hasSynonym>
	<oboInOwl:hasSynonym xml:lang="en">flatbread</oboInOwl:hasSynonym>
	<oboInOwl:hasSynonym xml:lang="en">unleavened bread</oboInOwl:hasSynonym>
	<oboInOwl:hasDbXref>LANGUAL:A0819</oboInOwl:hasDbXref>
</owl:Class>

<owl:Class rdf:about="&obo;FOODON_03400820">
	<rdfs:label xml:lang="en">bread product (eurofir)</rdfs:label>
	<rdfs:subClassOf rdf:resource="&obo;FOODON_03400817"/>
	<obo:IAO_0000412>http://langual.org</obo:IAO_0000412>
	<obo:IAO_0000115 xml:lang="en">includes breadcrumbs, bread stuffing</obo:IAO_0000115>
	<obo:IAO_0000114 rdf:resource="&obo;IAO_0000428"/>
	<oboInOwl:hasDbXref>LANGUAL:A0820</oboInOwl:hasDbXref>
</owl:Class>

<owl:Class rdf:about="&obo;FOODON_03400821">
	<rdfs:label xml:lang="en">fine bakery ware (eurofir)</rdfs:label>
	<rdfs:subClassOf rdf:resource="&obo;FOODON_03400812"/>
	<obo:IAO_0000412>http://langual.org</obo:IAO_0000412>
	<obo:IAO_0000115 xml:lang="en">Products in the *BREAD* category normally have contents of sugars and fat neither exceeding 5% on a dry weight basis. Bakery products exceeding either of these limits are termed "Fine bakery ware". Savoury fine bakery wares will tend to be higher in fat and sweet products in sugars. However, some products, for example scones, may be considered savoury or sweet. Therefore, all of these products are categorised as "Fine bakery wares", rather than using separate categories for savoury and sweet products. Some examples are: biscuits, cookies, dry pastry (e.g. savoury biscuits, sweet biscuits and cookies); sweet breads (e.g. croissants, currant bun, dough cakes like muffins or brioche, scone, doughnut); pastry (e.g. danish pastry, baclava); tart, pie (e.g. custard tart, mince pie); cakes (e.g. fruit cake, cream cake, sponge cake.</obo:IAO_0000115>
	<obo:IAO_0000114 rdf:resource="&obo;IAO_0000428"/>
	<oboInOwl:hasDbXref>LANGUAL:A0821</oboInOwl:hasDbXref>
</owl:Class>

<owl:Class rdf:about="&obo;FOODON_03400822">
	<rdfs:label xml:lang="en">savoury cereal dish (eurofir)</rdfs:label>
	<rdfs:subClassOf rdf:resource="&obo;FOODON_03400812"/>
	<rdfs:subClassOf rdf:resource="&obo;FOODON_03400861"/>
	<obo:IAO_0000412>http://langual.org</obo:IAO_0000412>
	<obo:IAO_0000115 xml:lang="en">includes dumpling, risotto, savoury pancake, pizza, couscous, savoury pie, sandwich.</obo:IAO_0000115>
	<obo:IAO_0000114 rdf:resource="&obo;IAO_0000428"/>
	<oboInOwl:hasDbXref>LANGUAL:A0822</oboInOwl:hasDbXref>
</owl:Class>

<owl:Class rdf:about="&obo;FOODON_03400823">
	<rdfs:label xml:lang="en">nut, seed or kernel (eurofir)</rdfs:label>
	<rdfs:subClassOf rdf:resource="&obo;FOODON_03400777"/>
	<obo:IAO_0000412>http://langual.org</obo:IAO_0000412>
	<obo:IAO_0000115 xml:lang="en">Nuts, seeds and kernels in all forms, including pastes. Examples: walnut, hazelnut, sweet chestnut, sunflower seed, olive seed, pine nut, apricot kernel, peanuts.</obo:IAO_0000115>
	<obo:IAO_0000114 rdf:resource="&obo;IAO_0000428"/>
	<oboInOwl:hasDbXref>LANGUAL:A0823</oboInOwl:hasDbXref>
</owl:Class>

<owl:Class rdf:about="&obo;FOODON_03400824">
	<rdfs:label xml:lang="en">nut or seed product (eurofir)</rdfs:label>
	<rdfs:subClassOf rdf:resource="&obo;FOODON_03400823"/>
	<obo:IAO_0000412>http://langual.org</obo:IAO_0000412>
	<obo:IAO_0000115 xml:lang="en">e.g. coconut milk, chestnut purée, tahini paste, peanut butter.</obo:IAO_0000115>
	<obo:IAO_0000114 rdf:resource="&obo;IAO_0000428"/>
	<oboInOwl:hasDbXref>LANGUAL:A0824</oboInOwl:hasDbXref>
</owl:Class>

<owl:Class rdf:about="&obo;FOODON_03400825">
	<rdfs:label xml:lang="en">vegetable or vegetable product (eurofir)</rdfs:label>
	<rdfs:subClassOf rdf:resource="&obo;FOODON_03400777"/>
	<obo:IAO_0000412>http://langual.org</obo:IAO_0000412>
	<obo:IAO_0000115 xml:lang="en">includes: plants and parts of plants eaten as vegetables (i.e. normally consumed as a savoury and usually with other foods as sources of protein and/or grain starch), including immature pulses; edible fungi and seaweed; a food product whose predominant constituent is vegetables; a recipe dish whose main ingredient is considered to be vegetables. The group excludes: fruiting body of a plant when this is consumed as a dessert fruit (under *FRUIT*); seeds, kernels and nuts (under *NUT, SEED OR KERNEL PRODUCT*); oils produced from vegetable plants (under *FAT OR OIL*); herbs, spices, chutney and pickles produced from vegetables (under *SPICE, CONDIMENT OR OTHER INGREDIENT*); food products produced wholly or partially from vegetables but used as a substitute for a food assigned to another main group (for example, potato flour is a substitute flour under *FLOUR OR STARCH*).</obo:IAO_0000115>
	<obo:IAO_0000114 rdf:resource="&obo;IAO_0000428"/>
	<oboInOwl:hasDbXref>LANGUAL:A0825</oboInOwl:hasDbXref>
</owl:Class>

<owl:Class rdf:about="&obo;FOODON_03400826">
	<rdfs:label xml:lang="en">vegetable (excluding potato) (eurofir)</rdfs:label>
	<rdfs:subClassOf rdf:resource="&obo;FOODON_03400825"/>
	<obo:IAO_0000412>http://langual.org</obo:IAO_0000412>
	<obo:IAO_0000115 xml:lang="en">In EFG, Potatoes were excluded distinguished from other vegetables because of their high starch content. Herbs have been included where these may be consumed in significant amounts as vegetables, either raw or cooked (e.g. parsley, chives). A vegetable fruit is usually consumed as a vegetable when the starch content is high (e.g. avocado, olive). Some examples of foods classified here would be lettuce, cabbage, rhubarb, asparagus, onion, carrot.</obo:IAO_0000115>
	<obo:IAO_0000114 rdf:resource="&obo;IAO_0000428"/>
	<oboInOwl:hasDbXref>LANGUAL:A0826</oboInOwl:hasDbXref>
</owl:Class>

<owl:Class rdf:about="&obo;FOODON_03400827">
	<rdfs:label xml:lang="en">vegetable product (eurofir)</rdfs:label>
	<rdfs:subClassOf rdf:resource="&obo;FOODON_03400826"/>
	<obo:IAO_0000412>http://langual.org</obo:IAO_0000412>
	<obo:IAO_0000115 xml:lang="en">e.g. tomato purée, sun-dried tomatoes, pickled red cabbage, sauerkraut.</obo:IAO_0000115>
	<obo:IAO_0000114 rdf:resource="&obo;IAO_0000428"/>
	<oboInOwl:hasDbXref>LANGUAL:A0827</oboInOwl:hasDbXref>
</owl:Class>

<owl:Class rdf:about="&obo;FOODON_03400828">
	<rdfs:label xml:lang="en">vegetable dish (eurofir)</rdfs:label>
	<rdfs:subClassOf rdf:resource="&obo;FOODON_03400827"/>
	<rdfs:subClassOf rdf:resource="&obo;FOODON_03400861"/>
	<obo:IAO_0000412>http://langual.org</obo:IAO_0000412>
	<obo:IAO_0000115 xml:lang="en">A recipe dish whose main ingredient is considered to be vegetables.</obo:IAO_0000115>
	<obo:IAO_0000114 rdf:resource="&obo;IAO_0000428"/>
	<oboInOwl:hasDbXref>LANGUAL:A0828</oboInOwl:hasDbXref>
</owl:Class>

<owl:Class rdf:about="&obo;FOODON_03400829">
	<rdfs:label xml:lang="en">starchy root or potato (eurofir)</rdfs:label>
	<rdfs:subClassOf rdf:resource="&obo;FOODON_03400825"/>
	<obo:IAO_0000412>http://langual.org</obo:IAO_0000412>
	<obo:IAO_0000115 xml:lang="en">In EFG, Potatoes were excluded distinguished from other vegetables because of their high starch content. Some examples of foods classified here would be new potato, main-crop potato, jerusalem artichoke, sweet potato, yam</obo:IAO_0000115>
	<obo:IAO_0000114 rdf:resource="&obo;IAO_0000428"/>
	<oboInOwl:hasDbXref>LANGUAL:A0829</oboInOwl:hasDbXref>
</owl:Class>

<owl:Class rdf:about="&obo;FOODON_03400830">
	<rdfs:label xml:lang="en">potato dish (eurofir)</rdfs:label>
	<rdfs:subClassOf rdf:resource="&obo;FOODON_03400829"/>
	<rdfs:subClassOf rdf:resource="&obo;FOODON_03400861"/>
	<obo:IAO_0000412>http://langual.org</obo:IAO_0000412>
	<obo:IAO_0000114 rdf:resource="&obo;IAO_0000428"/>
	<oboInOwl:hasDbXref>LANGUAL:A0830</oboInOwl:hasDbXref>
</owl:Class>

<owl:Class rdf:about="&obo;FOODON_03400831">
	<rdfs:label xml:lang="en">pulse or pulse product (eurofir)</rdfs:label>
	<rdfs:subClassOf rdf:resource="&obo;FOODON_03400825"/>
	<obo:IAO_0000412>http://langual.org</obo:IAO_0000412>
	<obo:IAO_0000115 xml:lang="en">EFG group 14. Eurocode-2 group 7.10-20</obo:IAO_0000115>
	<obo:IAO_0000114 rdf:resource="&obo;IAO_0000428"/>
	<oboInOwl:hasDbXref>LANGUAL:A0831</oboInOwl:hasDbXref>
</owl:Class>

<owl:Class rdf:about="&obo;FOODON_03400832">
	<rdfs:label xml:lang="en">pulse dish (eurofir)</rdfs:label>
	<rdfs:subClassOf rdf:resource="&obo;FOODON_03400831"/>
	<rdfs:subClassOf rdf:resource="&obo;FOODON_03400861"/>
	<obo:IAO_0000412>http://langual.org</obo:IAO_0000412>
	<obo:IAO_0000114 rdf:resource="&obo;IAO_0000428"/>
	<oboInOwl:hasDbXref>LANGUAL:A0832</oboInOwl:hasDbXref>
</owl:Class>

<owl:Class rdf:about="&obo;FOODON_03400833">
	<rdfs:label xml:lang="en">fruit or fruit product (eurofir)</rdfs:label>
	<rdfs:subClassOf rdf:resource="&obo;FOODON_03400777"/>
	<obo:IAO_0000412>http://langual.org</obo:IAO_0000412>
	<obo:IAO_0000115 xml:lang="en">The group includes: fruits when consumed as a dessert; food products whose predominant constituent is fruit; recipe dishes whose main ingredient is considered to be fruit. A fruit is usually consumed as a dessert when the starch content has been reduced by conversion during ripening to sugars. The group excludes: vegetable fruits (under Vegetable); nuts, seeds and kernels (under *NUT, SEED OR KERNEL PRODUCT*); oils produced from fruits (under *FAT OR OIL*); chutney and pickles (under Miscellaneous foods).</obo:IAO_0000115>
	<obo:IAO_0000114 rdf:resource="&obo;IAO_0000428"/>
	<oboInOwl:hasDbXref>LANGUAL:A0833</oboInOwl:hasDbXref>
</owl:Class>

<owl:Class rdf:about="&obo;FOODON_03400834">
	<rdfs:label xml:lang="en">processed fruit product (eurofir)</rdfs:label>
	<rdfs:subClassOf rdf:resource="&obo;FOODON_03400833"/>
	<obo:IAO_0000412>http://langual.org</obo:IAO_0000412>
	<obo:IAO_0000115 xml:lang="en">Examples are dried fruits (e.g. dried mixed fruit), compotes, canned, stewed fruit (e.g. apple sauce, fruit cocktail).</obo:IAO_0000115>
	<obo:IAO_0000114 rdf:resource="&obo;IAO_0000428"/>
	<oboInOwl:hasDbXref>LANGUAL:A0834</oboInOwl:hasDbXref>
</owl:Class>

<owl:Class rdf:about="&obo;FOODON_03400835">
	<rdfs:label xml:lang="en">sugar or sugar product (eurofir)</rdfs:label>
	<rdfs:subClassOf rdf:resource="&obo;FOODON_03400777"/>
	<obo:IAO_0000412>http://langual.org</obo:IAO_0000412>
	<obo:IAO_0000115 xml:lang="en">This group includes sucrose and other sugars, sugar substitutes, honey and syrups; fruit jams, marmalades and other spreads; dessert jellies and toppings; chocolate and non-chocolate confectionery; a food product whose predominant constituent is sugar or chocolate; a recipe dish whose main ingredient is considered to be sugar or chocolate.</obo:IAO_0000115>
	<obo:IAO_0000114 rdf:resource="&obo;IAO_0000428"/>
	<oboInOwl:hasSynonym xml:lang="en">confectionery</oboInOwl:hasSynonym>
	<oboInOwl:hasDbXref>LANGUAL:A0835</oboInOwl:hasDbXref>
</owl:Class>

<owl:Class rdf:about="&obo;FOODON_03400836">
	<rdfs:label xml:lang="en">sugar, honey or syrup (eurofir)</rdfs:label>
	<rdfs:subClassOf rdf:resource="&obo;FOODON_03400835"/>
	<obo:IAO_0000412>http://langual.org</obo:IAO_0000412>
	<obo:IAO_0000115 xml:lang="en">This group includes sugars (e.g. white sugar, brown sugar, fructose), sugar substitutes (non-nutritive sweeteners like aspartame &amp; saccharine, nutritive sweeteners like sorbitol &amp; mannitol), honey, syrups (e.g. molasses, maple syrup, corn syrup).</obo:IAO_0000115>
	<obo:IAO_0000114 rdf:resource="&obo;IAO_0000428"/>
	<oboInOwl:hasDbXref>LANGUAL:A0836</oboInOwl:hasDbXref>
</owl:Class>

<owl:Class rdf:about="&obo;FOODON_03400837">
	<rdfs:label xml:lang="en">jam or marmalade (eurofir)</rdfs:label>
	<rdfs:subClassOf rdf:resource="&obo;FOODON_03400835"/>
	<obo:IAO_0000412>http://langual.org</obo:IAO_0000412>
	<obo:IAO_0000115 xml:lang="en">Semisolid or jelled food prepared from fruit or fruit juice and other ingredients. The group includes fruit jam, fruit jelly preserve, marmalade.</obo:IAO_0000115>
	<obo:IAO_0000114 rdf:resource="&obo;IAO_0000428"/>
	<oboInOwl:hasDbXref>LANGUAL:A0837</oboInOwl:hasDbXref>
</owl:Class>

<owl:Class rdf:about="&obo;FOODON_03400838">
	<rdfs:label xml:lang="en">non-chocolate confectionery or other sugar product (eurofir)</rdfs:label>
	<rdfs:subClassOf rdf:resource="&obo;FOODON_03400835"/>
	<obo:IAO_0000412>http://langual.org</obo:IAO_0000412>
	<obo:IAO_0000115 xml:lang="en">Some examples are boiled sweet, gum sweet, nougat, turkish delight, chewing gum, marzipan, candied fruit.</obo:IAO_0000115>
	<obo:IAO_0000114 rdf:resource="&obo;IAO_0000428"/>
	<oboInOwl:hasDbXref>LANGUAL:A0838</oboInOwl:hasDbXref>
</owl:Class>

<owl:Class rdf:about="&obo;FOODON_03400839">
	<rdfs:label xml:lang="en">chocolate or chocolate product (eurofir)</rdfs:label>
	<rdfs:subClassOf rdf:resource="&obo;FOODON_03400835"/>
	<obo:IAO_0000412>http://langual.org</obo:IAO_0000412>
	<obo:IAO_0000115 xml:lang="en">Some examples are chocolate slab or bar (e.g. milk chocolate bar, white chocolate bar), filled chocolate candy, chocolate-coated confectionery bars.</obo:IAO_0000115>
	<obo:IAO_0000114 rdf:resource="&obo;IAO_0000428"/>
	<oboInOwl:hasSynonym xml:lang="en">chocolate confectionery</oboInOwl:hasSynonym>
	<oboInOwl:hasDbXref>LANGUAL:A0839</oboInOwl:hasDbXref>
</owl:Class>

<owl:Class rdf:about="&obo;FOODON_03400840">
	<rdfs:label xml:lang="en">beverage (non-milk) (eurofir)</rdfs:label>
	<rdfs:subClassOf rdf:resource="&obo;FOODON_03400777"/>
	<obo:IAO_0000412>http://langual.org</obo:IAO_0000412>
	<obo:IAO_0000115 xml:lang="en">Alcoholic or non-alcoholic beverage; excludes milk and milk-based beverages.</obo:IAO_0000115>
	<obo:IAO_0000114 rdf:resource="&obo;IAO_0000428"/>
	<oboInOwl:hasDbXref>LANGUAL:A0840</oboInOwl:hasDbXref>
</owl:Class>

<owl:Class rdf:about="&obo;FOODON_03400841">
	<rdfs:label xml:lang="en">juice or nectar (eurofir)</rdfs:label>
	<rdfs:subClassOf rdf:resource="&obo;FOODON_03400840"/>
	<obo:IAO_0000412>http://langual.org</obo:IAO_0000412>
	<obo:IAO_0000115 xml:lang="en">The members of the work group in Action COST 99/Eurofoods considered it important to be able to separate fruit juices from both *NON-ALCOHOLIC BEVERAGE* and *FRUIT* in the EFG classification, in order to evaluate and compare consumption patterns across countries. Examples are orange juice, apple juice, tomato juice, fruit and vegetable nectars.</obo:IAO_0000115>
	<obo:IAO_0000114 rdf:resource="&obo;IAO_0000428"/>
	<oboInOwl:hasDbXref>LANGUAL:A0841</oboInOwl:hasDbXref>
</owl:Class>

<owl:Class rdf:about="&obo;FOODON_03400842">
	<rdfs:label xml:lang="en">non alcoholic beverage (eurofir)</rdfs:label>
	<rdfs:subClassOf rdf:resource="&obo;FOODON_03400840"/>
	<obo:IAO_0000412>http://langual.org</obo:IAO_0000412>
	<obo:IAO_0000115 xml:lang="en">Beverage containing no more than 0.5% alcohol; it may be flavoured, sweetened or carbonated; includes soft drinks and steeped beverages; excludes milk in all forms, fruit juices and vegetable juices.</obo:IAO_0000115>
	<obo:IAO_0000114 rdf:resource="&obo;IAO_0000428"/>
	<oboInOwl:hasDbXref>LANGUAL:A0842</oboInOwl:hasDbXref>
</owl:Class>

<owl:Class rdf:about="&obo;FOODON_03400843">
	<rdfs:label xml:lang="en">soft drink (eurofir)</rdfs:label>
	<rdfs:subClassOf rdf:resource="&obo;FOODON_03400842"/>
	<obo:IAO_0000412>http://langual.org</obo:IAO_0000412>
	<obo:IAO_0000115 xml:lang="en">Includes carbonated soft drinks (e.g. soda water, carbonated lemonade, cola, tonic), non-dilution still drinks (e.g. still lemonade), dilution drinks (concentrates which are diluted with water prior to consumption , e.g. rosehip syrup, fruit squash, lime cordial).</obo:IAO_0000115>
	<obo:IAO_0000114 rdf:resource="&obo;IAO_0000428"/>
	<oboInOwl:hasDbXref>LANGUAL:A0843</oboInOwl:hasDbXref>
</owl:Class>

<owl:Class rdf:about="&obo;FOODON_03400844">
	<rdfs:label xml:lang="en">water (eurofir)</rdfs:label>
	<rdfs:subClassOf rdf:resource="&obo;FOODON_03400842"/>
	<obo:IAO_0000412>http://langual.org</obo:IAO_0000412>
	<obo:IAO_0000115 xml:lang="en">Includes tap water, carbonated mineral water, still mineral water.</obo:IAO_0000115>
	<obo:IAO_0000114 rdf:resource="&obo;IAO_0000428"/>
	<oboInOwl:hasDbXref>LANGUAL:A0844</oboInOwl:hasDbXref>
</owl:Class>

<owl:Class rdf:about="&obo;FOODON_03400845">
	<rdfs:label xml:lang="en">coffee, tea, cocoa or infusion (eurofir)</rdfs:label>
	<rdfs:subClassOf rdf:resource="&obo;FOODON_03400842"/>
	<obo:IAO_0000412>http://langual.org</obo:IAO_0000412>
	<obo:IAO_0000115 xml:lang="en">Beverage prepared by extracting flavour and other components from food sources by percolation and/or immersion in water, usually at near-boiling temperature. The group includes coffee (e.g. instant coffee, coffee and chicory essence), tea, herbal tea (e.g. green tea, black tea, tisane), cocoa beverage and beverage powder.</obo:IAO_0000115>
	<obo:IAO_0000114 rdf:resource="&obo;IAO_0000428"/>
	<rdfs:comment xml:lang="en">LanguaL curation note: Renamed from *COFFEE, TEA, COCOA (EUROFIR)* (LanguaL 2010).</rdfs:comment>
	<oboInOwl:hasSynonym xml:lang="en">infusion</oboInOwl:hasSynonym>
	<oboInOwl:hasSynonym xml:lang="en">steeped beverage</oboInOwl:hasSynonym>
	<oboInOwl:hasDbXref>LANGUAL:A0845</oboInOwl:hasDbXref>
</owl:Class>

<owl:Class rdf:about="&obo;FOODON_03400846">
	<rdfs:label xml:lang="en">alcoholic beverage (eurofir)</rdfs:label>
	<rdfs:subClassOf rdf:resource="&obo;FOODON_03400840"/>
	<obo:IAO_0000412>http://langual.org</obo:IAO_0000412>
	<obo:IAO_0000115 xml:lang="en">Beverage containing more than 0.5% alcohol; includes distilled spirits, malt beverage, and wine. Alcohol-free varieties are included in the appropriate categories together with their alcohol-containing forms and distinguished in facets H and P.</obo:IAO_0000115>
	<obo:IAO_0000114 rdf:resource="&obo;IAO_0000428"/>
	<rdfs:comment xml:lang="en">LanguaL curation note: Alcoholic content can be indexed in facet Z.</rdfs:comment>
	<oboInOwl:hasDbXref>LANGUAL:A0846</oboInOwl:hasDbXref>
</owl:Class>

<owl:Class rdf:about="&obo;FOODON_03400847">
	<rdfs:label xml:lang="en">beer or beer-like beverage (eurofir)</rdfs:label>
	<rdfs:subClassOf rdf:resource="&obo;FOODON_03400846"/>
	<obo:IAO_0000412>http://langual.org</obo:IAO_0000412>
	<obo:IAO_0000115 xml:lang="en">includes beer, barley beer.</obo:IAO_0000115>
	<obo:IAO_0000114 rdf:resource="&obo;IAO_0000428"/>
	<rdfs:comment xml:lang="en">LanguaL curation note: Renamed from *BEER OR OTHER MALT BEVERAGE (EUROFIR)* (LanguaL 2010).</rdfs:comment>
	<oboInOwl:hasSynonym xml:lang="en">beer or other malt beverage</oboInOwl:hasSynonym>
	<oboInOwl:hasDbXref>LANGUAL:A0847</oboInOwl:hasDbXref>
</owl:Class>

<owl:Class rdf:about="&obo;FOODON_03400848">
	<rdfs:label xml:lang="en">cider, perry or similar drink (eurofir)</rdfs:label>
	<rdfs:subClassOf rdf:resource="&obo;FOODON_03400846"/>
	<obo:IAO_0000412>http://langual.org</obo:IAO_0000412>
	<obo:IAO_0000115 xml:lang="en">includes apple cider, perry (made by fermenting pear juice)</obo:IAO_0000115>
	<obo:IAO_0000114 rdf:resource="&obo;IAO_0000428"/>
	<oboInOwl:hasDbXref>LANGUAL:A0848</oboInOwl:hasDbXref>
</owl:Class>

<owl:Class rdf:about="&obo;FOODON_03400849">
	<rdfs:label xml:lang="en">wine, fortified wine or wine-like beverage (eurofir)</rdfs:label>
	<rdfs:subClassOf rdf:resource="&obo;FOODON_03400846"/>
	<obo:IAO_0000412>http://langual.org</obo:IAO_0000412>
	<obo:IAO_0000115 xml:lang="en">Alcoholic beverage produced by the normal fermentation of the juice of grapes or other fruits or of the fermentable parts of plants or plant-related products. The group includes table wine, dessert wine, elderberry wine, fortified and liqueur wines (e.g. port, sherry, vermouth).</obo:IAO_0000115>
	<obo:IAO_0000114 rdf:resource="&obo;IAO_0000428"/>
	<oboInOwl:hasDbXref>LANGUAL:A0849</oboInOwl:hasDbXref>
</owl:Class>

<owl:Class rdf:about="&obo;FOODON_03400850">
	<rdfs:label xml:lang="en">liqueur or spirits (eurofir)</rdfs:label>
	<rdfs:subClassOf rdf:resource="&obo;FOODON_03400846"/>
	<obo:IAO_0000412>http://langual.org</obo:IAO_0000412>
	<obo:IAO_0000115 xml:lang="en">Alcoholic beverage prepared by fermentation of grain or plant-related products and subsequent distillation. Includes liqueurs (e.g. calvados, kahlua, advocaat) and spirits (e.g. brandy, whisk(e)y, rum).</obo:IAO_0000115>
	<obo:IAO_0000114 rdf:resource="&obo;IAO_0000428"/>
	<oboInOwl:hasDbXref>LANGUAL:A0850</oboInOwl:hasDbXref>
</owl:Class>

<owl:Class rdf:about="&obo;FOODON_03400851">
	<rdfs:label xml:lang="en">alcoholic mixed drink (eurofir)</rdfs:label>
	<rdfs:subClassOf rdf:resource="&obo;FOODON_03400846"/>
	<obo:IAO_0000412>http://langual.org</obo:IAO_0000412>
	<obo:IAO_0000115 xml:lang="en">includes cocktails, punch, shandy.</obo:IAO_0000115>
	<obo:IAO_0000114 rdf:resource="&obo;IAO_0000428"/>
	<oboInOwl:hasDbXref>LANGUAL:A0851</oboInOwl:hasDbXref>
</owl:Class>

<owl:Class rdf:about="&obo;FOODON_03400852">
	<rdfs:label xml:lang="en">miscellaneous food product (eurofir)</rdfs:label>
	<rdfs:subClassOf rdf:resource="&obo;FOODON_03400777"/>
	<obo:IAO_0000412>http://langual.org</obo:IAO_0000412>
	<obo:IAO_0000115 xml:lang="en">EFG group 32, Eurocode-2 group 12.</obo:IAO_0000115>
	<obo:IAO_0000114 rdf:resource="&obo;IAO_0000428"/>
	<rdfs:comment xml:lang="en">LanguaL curation note: Use for foods and ingredients that could not fit into any of the above classes.</rdfs:comment>
	<oboInOwl:hasDbXref>LANGUAL:A0852</oboInOwl:hasDbXref>
</owl:Class>

<owl:Class rdf:about="&obo;FOODON_03400853">
	<rdfs:label xml:lang="en">spice, condiment or other ingredient (eurofir)</rdfs:label>
	<rdfs:subClassOf rdf:resource="&obo;FOODON_03400852"/>
	<obo:IAO_0000412>http://langual.org</obo:IAO_0000412>
	<obo:IAO_0000115 xml:lang="en">This subgroup includes baking goods and other ingredients such as flavourings, essences, seasonings and extracts which are difficult to assign to other main groups; herbs and spices; dressings, condiments and mixed accompaniments such as chutneys and pickles. The group does not include starches (under *GRAIN OR GRAIN PRODUCT*); plant products that may be used in significant amounts as vegetables as well as herbs, like chives and parsley (under *VEGETABLE*).</obo:IAO_0000115>
	<obo:IAO_0000114 rdf:resource="&obo;IAO_0000428"/>
	<oboInOwl:hasDbXref>LANGUAL:A0853</oboInOwl:hasDbXref>
</owl:Class>

<owl:Class rdf:about="&obo;FOODON_03400854">
	<rdfs:label xml:lang="en">baking ingredient (eurofir)</rdfs:label>
	<rdfs:subClassOf rdf:resource="&obo;FOODON_03400853"/>
	<obo:IAO_0000412>http://langual.org</obo:IAO_0000412>
	<obo:IAO_0000115 xml:lang="en">includes yeast, baking powder, pectin, additives.</obo:IAO_0000115>
	<obo:IAO_0000114 rdf:resource="&obo;IAO_0000428"/>
	<oboInOwl:hasDbXref>LANGUAL:A0854</oboInOwl:hasDbXref>
</owl:Class>

<owl:Class rdf:about="&obo;FOODON_03400855">
	<rdfs:label xml:lang="en">flavouring or essence (eurofir)</rdfs:label>
	<rdfs:subClassOf rdf:resource="&obo;FOODON_03400853"/>
	<obo:IAO_0000412>http://langual.org</obo:IAO_0000412>
	<obo:IAO_0000115 xml:lang="en">includes almond essence, vanilla essence.</obo:IAO_0000115>
	<obo:IAO_0000114 rdf:resource="&obo;IAO_0000428"/>
	<oboInOwl:hasDbXref>LANGUAL:A0855</oboInOwl:hasDbXref>
</owl:Class>

<owl:Class rdf:about="&obo;FOODON_03400856">
	<rdfs:label xml:lang="en">seasoning or extract (eurofir)</rdfs:label>
	<rdfs:subClassOf rdf:resource="&obo;FOODON_03400853"/>
	<obo:IAO_0000412>http://langual.org</obo:IAO_0000412>
	<obo:IAO_0000115 xml:lang="en">includes salt, stock cubes, gravy thickener, beef extract, marmite, vinegar.</obo:IAO_0000115>
	<obo:IAO_0000114 rdf:resource="&obo;IAO_0000428"/>
	<oboInOwl:hasDbXref>LANGUAL:A0856</oboInOwl:hasDbXref>
</owl:Class>

<owl:Class rdf:about="&obo;FOODON_03400857">
	<rdfs:label xml:lang="en">herb or spice (eurofir)</rdfs:label>
	<rdfs:subClassOf rdf:resource="&obo;FOODON_03400853"/>
	<obo:IAO_0000412>http://langual.org</obo:IAO_0000412>
	<obo:IAO_0000115 xml:lang="en">Aromatic or pungent plant product used whole or ground as a seasoning in food products, e.g. basil, oregano, thyme, allspice, clove, paprika, curry powder. Herbs may be considered to be plants whose non-woody parts are consumed in small amounts for their flavouring properties rather than in amounts significant to the intake of major nutrients. Spices are usually a dried part, or parts, of aromatic plants used either whole or ground to add flavour and for preservative properties. Some such as coriander and fenugreek are the ground seeds of plants whose leaves are used as herbs or vegetables. Others are dried fruits or berries.</obo:IAO_0000115>
	<obo:IAO_0000114 rdf:resource="&obo;IAO_0000428"/>
	<oboInOwl:hasSynonym xml:lang="en">spice or herb</oboInOwl:hasSynonym>
	<oboInOwl:hasDbXref>LANGUAL:A0857</oboInOwl:hasDbXref>
</owl:Class>

<owl:Class rdf:about="&obo;FOODON_03400858">
	<rdfs:label xml:lang="en">condiment (eurofir)</rdfs:label>
	<rdfs:subClassOf rdf:resource="&obo;FOODON_03400853"/>
	<obo:IAO_0000412>http://langual.org</obo:IAO_0000412>
	<obo:IAO_0000115 xml:lang="en">Food product that is usually pungent, tart, salty, or spicy and is used to enhance the flavours of other foods; includes ketchup, tabasco sauce, barbeque sauce, vinegar, soy sauce, prepared mustard, prepared horseradish, mint sauce and tartar sauce.</obo:IAO_0000115>
	<obo:IAO_0000114 rdf:resource="&obo;IAO_0000428"/>
	<oboInOwl:hasSynonym xml:lang="en">condiment sauce</oboInOwl:hasSynonym>
	<oboInOwl:hasDbXref>LANGUAL:A0858</oboInOwl:hasDbXref>
</owl:Class>

<owl:Class rdf:about="&obo;FOODON_03400859">
	<rdfs:label xml:lang="en">dressing, mayonnaise (eurofir)</rdfs:label>
	<rdfs:subClassOf rdf:resource="&obo;FOODON_03400853"/>
	<obo:IAO_0000412>http://langual.org</obo:IAO_0000412>
	<obo:IAO_0000115 xml:lang="en">Mixture of edible fats or oils, acidifying agents and optional ingredients such as sweeteners (nutritive or non-nutritive), starch, egg and seasonings. Used in limited amounts to accompany salads and other foods. Includes salad dressings &amp; other vinegar and oil based cold sauces, mayonnaise &amp; other egg and oil based cold sauces.</obo:IAO_0000115>
	<obo:IAO_0000114 rdf:resource="&obo;IAO_0000428"/>
	<oboInOwl:hasDbXref>LANGUAL:A0859</oboInOwl:hasDbXref>
</owl:Class>

<owl:Class rdf:about="&obo;FOODON_03400860">
	<rdfs:label xml:lang="en">chutney or pickle (eurofir)</rdfs:label>
	<rdfs:subClassOf rdf:resource="&obo;FOODON_03400858"/>
	<rdfs:subClassOf rdf:resource="&obo;FOODON_03400827"/>
	<obo:IAO_0000412>http://langual.org</obo:IAO_0000412>
	<obo:IAO_0000115 xml:lang="en">Product prepared by immersing fruits, vegetables, or other ingredients, such as spices and sweeteners, in a brine or an acid solution. Used to enhance the flavour of other food products. Examples are mango chutney, dill pickle, mixed pickle, relish.</obo:IAO_0000115>
	<obo:IAO_0000114 rdf:resource="&obo;IAO_0000428"/>
	<oboInOwl:hasSynonym xml:lang="en">pickle; relish</oboInOwl:hasSynonym>
	<oboInOwl:hasDbXref>LANGUAL:A0860</oboInOwl:hasDbXref>
</owl:Class>

<owl:Class rdf:about="&obo;FOODON_03400861">
	<rdfs:label xml:lang="en">prepared food product (eurofir)</rdfs:label>
	<rdfs:subClassOf rdf:resource="&obo;FOODON_03400852"/>
	<obo:IAO_0000412>http://langual.org</obo:IAO_0000412>
	<obo:IAO_0000115 xml:lang="en">This subgroup includes multicomponent meals, sauces, retail salads, desserts, soups, snacks and other foods where similarity of the product type is more significant than the source of the principal ingredient(s).</obo:IAO_0000115>
	<obo:IAO_0000114 rdf:resource="&obo;IAO_0000428"/>
	<oboInOwl:hasSynonym xml:lang="en">soup, sauce or miscellaneous food product</oboInOwl:hasSynonym>
	<oboInOwl:hasDbXref>LANGUAL:A0861</oboInOwl:hasDbXref>
</owl:Class>

<owl:Class rdf:about="&obo;FOODON_03400862">
	<rdfs:label xml:lang="en">savoury sauce (eurofir)</rdfs:label>
	<rdfs:subClassOf rdf:resource="&obo;FOODON_03400861"/>
	<obo:IAO_0000412>http://langual.org</obo:IAO_0000412>
	<obo:IAO_0000115 xml:lang="en">Nonstandardized food product used as a meal accompaniment and consisting of a mixture of fats or oils, starch, liquid and other optional ingredients specified by the recipe; excludes condiments. Includes. bolognese sauce , white sauce, brown sauce, butter sauce, tomato sauce.</obo:IAO_0000115>
	<obo:IAO_0000114 rdf:resource="&obo;IAO_0000428"/>
	<rdfs:comment xml:lang="en">LanguaL curation note: Sauce is a very general term for a liquid or semiliquid seasoning or other accompaniment for food. When sauces are cooked as part of, or adjuncts to, dishes (including starters, main courses and desserts), they have been assigned to the *SAVOURY SAUCE* or</rdfs:comment>
	<oboInOwl:hasSynonym xml:lang="en">gravy or sauce</oboInOwl:hasSynonym>
	<oboInOwl:hasDbXref>LANGUAL:A0862</oboInOwl:hasDbXref>
</owl:Class>

<owl:Class rdf:about="&obo;FOODON_03400863">
	<rdfs:label xml:lang="en">dessert sauce (eurofir)</rdfs:label>
	<rdfs:subClassOf rdf:resource="&obo;FOODON_03400861"/>
	<obo:IAO_0000412>http://langual.org</obo:IAO_0000412>
	<obo:IAO_0000115 xml:lang="en">Sweetened and flavored product that is used as an accompaniment to desserts, e.g. fruit sauce, fudge sauce, brandy sauce.</obo:IAO_0000115>
	<obo:IAO_0000114 rdf:resource="&obo;IAO_0000428"/>
	<rdfs:comment xml:lang="en">LanguaL curation note: Sauce is a very general term for a liquid or semiliquid seasoning or other accompaniment for food. When sauces are cooked as part of, or adjuncts to, dishes (including starters, main courses and desserts), they have been assigned to the *SAVOURY SAUCE* or</rdfs:comment>
	<oboInOwl:hasSynonym xml:lang="en">sweet sauce</oboInOwl:hasSynonym>
	<oboInOwl:hasDbXref>LANGUAL:A0863</oboInOwl:hasDbXref>
</owl:Class>

<owl:Class rdf:about="&obo;FOODON_03400864">
	<rdfs:label xml:lang="en">dessert (eurofir)</rdfs:label>
	<rdfs:subClassOf rdf:resource="&obo;FOODON_03400861"/>
	<obo:IAO_0000412>http://langual.org</obo:IAO_0000412>
	<obo:IAO_0000115 xml:lang="en">Sweetened prepared product usually consumed after the main course in a meal. Excludes fruit or fruit products, bakery products and confectionery. Includes sweet puddings (custards, starch puddings), non-dairy ices (e.g. water ices, granitas, sorbets) and gelatine desserts.</obo:IAO_0000115>
	<obo:IAO_0000114 rdf:resource="&obo;IAO_0000428"/>
	<oboInOwl:hasDbXref>LANGUAL:A0864</oboInOwl:hasDbXref>
</owl:Class>

<owl:Class rdf:about="&obo;FOODON_03400865">
	<rdfs:label xml:lang="en">soup (eurofir)</rdfs:label>
	<rdfs:subClassOf rdf:resource="&obo;FOODON_03400861"/>
	<obo:IAO_0000412>http://langual.org</obo:IAO_0000412>
	<obo:IAO_0000115 xml:lang="en">A liquid food made by simmering meat, poultry, seafood or vegetables, being clear or thickened to the consistency of a thin puree or having milk or cream added, and often containing pieces of solid food such as meat, shellfish, pasta or vegetables. Soup takes precedence over other food products. Examples are egg and lemon soup, oxtail soup, fish soup, rice soup, lentil soup, minestrone, cherry soup.</obo:IAO_0000115>
	<obo:IAO_0000114 rdf:resource="&obo;IAO_0000428"/>
	<oboInOwl:hasDbXref>LANGUAL:A0865</oboInOwl:hasDbXref>
</owl:Class>

<owl:Class rdf:about="&obo;FOODON_03400866">
	<rdfs:label xml:lang="en">prepared salad (eurofir)</rdfs:label>
	<rdfs:subClassOf rdf:resource="&obo;FOODON_03400861"/>
	<obo:IAO_0000412>http://langual.org</obo:IAO_0000412>
	<obo:IAO_0000115 xml:lang="en">A combination of one or more vegetable, fruit, herb, meat, poultry, seafood, egg, cereal or pasta, usually served with some kind of moist dressing; may be moulded with a jellying agent. Salad takes precedence over other product types. Examples are egg salad, tuna salad, mixed vegetable salad, jelled fruit salad, macaroni salad, potato salad, rice salad, mayonnaise salad.</obo:IAO_0000115>
	<obo:IAO_0000114 rdf:resource="&obo;IAO_0000428"/>
	<oboInOwl:hasDbXref>LANGUAL:A0866</oboInOwl:hasDbXref>
</owl:Class>

<owl:Class rdf:about="&obo;FOODON_03400867">
	<rdfs:label xml:lang="en">sandwich filling (eurofir)</rdfs:label>
	<rdfs:subClassOf rdf:resource="&obo;FOODON_03400861"/>
	<obo:IAO_0000412>http://langual.org</obo:IAO_0000412>
	<obo:IAO_0000115 xml:lang="en">includes cheese-based sandwich filling, fish-based sandwich filling.</obo:IAO_0000115>
	<obo:IAO_0000114 rdf:resource="&obo;IAO_0000428"/>
	<oboInOwl:hasDbXref>LANGUAL:A0867</oboInOwl:hasDbXref>
</owl:Class>

<owl:Class rdf:about="&obo;FOODON_03400868">
	<rdfs:label xml:lang="en">savoury snack (eurofir)</rdfs:label>
	<rdfs:subClassOf rdf:resource="&obo;FOODON_03400861"/>
	<obo:IAO_0000412>http://langual.org</obo:IAO_0000412>
	<obo:IAO_0000115 xml:lang="en">Unsweetened food product marketed for consumption between meals; excludes nuts, edible seeds, and sweetened products such as cakes, puddings and candies. Examples are potato crisps, maize-based snacks, pretzels, popcorn.</obo:IAO_0000115>
	<obo:IAO_0000114 rdf:resource="&obo;IAO_0000428"/>
	<oboInOwl:hasSynonym xml:lang="en">snack food</oboInOwl:hasSynonym>
	<oboInOwl:hasDbXref>LANGUAL:A0868</oboInOwl:hasDbXref>
</owl:Class>

<owl:Class rdf:about="&obo;FOODON_03400869">
	<rdfs:label xml:lang="en">product for special nutritional use or dietary supplement (eurofir)</rdfs:label>
	<rdfs:subClassOf rdf:resource="&obo;FOODON_03400777"/>
	<obo:IAO_0000412>http://langual.org</obo:IAO_0000412>
	<obo:IAO_0000115 xml:lang="en">This group includes products for dietetic use that are not typically regarded as food. It excludes normal foods that are prepared or processed in a special way to suit dietetic purposes; these are indexed as the normal food with the addition of appropriate terms available from the thesaurus (facet P).</obo:IAO_0000115>
	<obo:IAO_0000114 rdf:resource="&obo;IAO_0000428"/>
	<oboInOwl:hasDbXref>LANGUAL:A0869</oboInOwl:hasDbXref>
</owl:Class>

<owl:Class rdf:about="&obo;FOODON_03400870">
	<rdfs:label xml:lang="en">dietary supplement (eurofir)</rdfs:label>
	<rdfs:subClassOf rdf:resource="&obo;FOODON_03400869"/>
	<obo:IAO_0000412>http://langual.org</obo:IAO_0000412>
	<obo:IAO_0000115 xml:lang="en">includes vitamin/mineral products, tonics, supplements. Vitamin and mineral food supplements are sources in concentrated forms of those nutrients alone or in combinations, marketed in forms such as capsules, tablets, powders, solutions etc., that are designed to be taken in measured small-unit quantities but are not in a conventional food form and whose purpose is to supplement the intake of vitamins and/or minerals from the normal diet (Codex CAC/GL 55 - 2005).</obo:IAO_0000115>
	<obo:IAO_0000114 rdf:resource="&obo;IAO_0000428"/>
	<oboInOwl:hasSynonym xml:lang="en">vitamin and mineral food supplements</oboInOwl:hasSynonym>
	<oboInOwl:hasDbXref>LANGUAL:A0870</oboInOwl:hasDbXref>
</owl:Class>

<owl:Class rdf:about="&obo;FOODON_03400871">
	<rdfs:label xml:lang="en">food for special nutritional use (eurofir)</rdfs:label>
	<rdfs:subClassOf rdf:resource="&obo;FOODON_03400869"/>
	<obo:IAO_0000412>http://langual.org</obo:IAO_0000412>
	<obo:IAO_0000115 xml:lang="en">Foods for Special Dietary Uses are those foods that are specially processed or formulated to satisfy particular dietary requirements that exist because of a particular physical or physiological condition and/or specific diseases and disorders and that are presented as such. The composition of these foodstuffs must differ significantly from the composition of ordinary foods of comparable nature, if such ordinary foods exist (CODEX STAN 146-1985).  The product may be used as the sole or major source of nourishment. It is frequently offered in a form convenient to use. The group includes infant formula, products designed for weight loss, instant breakfast, energy food stick, interal and parenteral complete nutrition solutions, etc.</obo:IAO_0000115>
	<obo:IAO_0000114 rdf:resource="&obo;IAO_0000428"/>
	<oboInOwl:hasSynonym xml:lang="en">food for special dietary use</oboInOwl:hasSynonym>
	<oboInOwl:hasSynonym xml:lang="en">meal replacement</oboInOwl:hasSynonym>
	<oboInOwl:hasDbXref>LANGUAL:A0871</oboInOwl:hasDbXref>
</owl:Class>

<owl:Class rdf:about="&obo;FOODON_03400872">
	<rdfs:label xml:lang="en">medical food (eurofir)</rdfs:label>
	<rdfs:subClassOf rdf:resource="&obo;FOODON_03400871"/>
	<obo:IAO_0000412>http://langual.org</obo:IAO_0000412>
	<obo:IAO_0000115 xml:lang="en">Foods for special medical purposes are a category of foods for special dietary uses that are specially processed or formulated and presented for the dietary management of patients and may be used only under medical supervision. They are intended for the exclusive or partial feeding of patients with limited or impaired capacity to take, digest, absorb or metabolize ordinary foodstuffs or certain nutrients contained therein, or who have other special medically-determined nutrient requirements, whose dietary management cannot be achieved only by modification of the normal diet, by other foods for special dietary uses, or by a combination of the two (CODEX STAN 180-1991).</obo:IAO_0000115>
	<obo:IAO_0000114 rdf:resource="&obo;IAO_0000428"/>
	<oboInOwl:hasSynonym xml:lang="en">dietary foods for special medical purposes</oboInOwl:hasSynonym>
	<oboInOwl:hasSynonym xml:lang="en">food for special medical purposes</oboInOwl:hasSynonym>
	<oboInOwl:hasDbXref>LANGUAL:A0872</oboInOwl:hasDbXref>
</owl:Class>

<owl:Class rdf:about="&obo;FOODON_03400873">
	<rdfs:label xml:lang="en">food for infants (eurofir)</rdfs:label>
	<rdfs:subClassOf rdf:resource="&obo;FOODON_03400871"/>
	<obo:IAO_0000412>http://langual.org</obo:IAO_0000412>
	<obo:IAO_0000115 xml:lang="en">Eurocode-2 group 13.60.</obo:IAO_0000115>
	<obo:IAO_0000114 rdf:resource="&obo;IAO_0000428"/>
	<rdfs:comment xml:lang="en">LanguaL curation note: Use for Infant formulae and follow-on formulae. Index Processed cereal-based foods and baby foods for infants and young children as the corresponding normal food (e.g. soup, fruit product). For both infant and baby foods, also index *INFANT OR TODDLER FOOD* in facet P.</rdfs:comment>
	<oboInOwl:hasSynonym xml:lang="en">infant formula</oboInOwl:hasSynonym>
	<oboInOwl:hasDbXref>LANGUAL:A0873</oboInOwl:hasDbXref>
</owl:Class>

<owl:Class rdf:about="&obo;FOODON_03400874">
	<rdfs:label xml:lang="en">global product classification (gs1 gpc)</rdfs:label>
	<rdfs:subClassOf rdf:resource="&obo;FOODON_03400352"/>
	<obo:IAO_0000412>http://langual.org</obo:IAO_0000412>
	<obo:IAO_0000115 xml:lang="en">The Global System 1 (GS1) Global Product Classification (GPC) is a system that gives buyers and sellers a common language for grouping products in the same way, everywhere in the world [http://gpcbrowser.gs1.org/].</obo:IAO_0000115>
	<obo:IAO_0000114 rdf:resource="&obo;IAO_0000428"/>
	<oboInOwl:hasDbXref>LANGUAL:A0874</oboInOwl:hasDbXref>
</owl:Class>

<owl:Class rdf:about="&obo;FOODON_03400875">
	<rdfs:label xml:lang="en">50200000 - beverages (gs1 gpc)</rdfs:label>
	<rdfs:subClassOf rdf:resource="&obo;FOODON_03400874"/>
	<obo:IAO_0000412>http://langual.org</obo:IAO_0000412>
	<obo:IAO_0000114 rdf:resource="&obo;IAO_0000428"/>
	<oboInOwl:hasDbXref>LANGUAL:A0875</oboInOwl:hasDbXref>
</owl:Class>

<owl:Class rdf:about="&obo;FOODON_03400876">
	<rdfs:label xml:lang="en">50202200 - alcoholic beverages (gs1 gpc)</rdfs:label>
	<rdfs:subClassOf rdf:resource="&obo;FOODON_03400875"/>
	<obo:IAO_0000412>http://langual.org</obo:IAO_0000412>
	<obo:IAO_0000114 rdf:resource="&obo;IAO_0000428"/>
	<oboInOwl:hasDbXref>LANGUAL:A0876</oboInOwl:hasDbXref>
</owl:Class>

<owl:Class rdf:about="&obo;FOODON_03400877">
	<rdfs:label xml:lang="en">10000142 - alcohol making kits (gs1 gpc)</rdfs:label>
	<rdfs:subClassOf rdf:resource="&obo;FOODON_03400876"/>
	<obo:IAO_0000412>http://langual.org</obo:IAO_0000412>
	<obo:IAO_0000115 xml:lang="en">Includes any products that can be described/observed as an alcoholic drink making kit. These products are total units that include all the necessary ingredients and equipment required to brew various flavours of beer, wine or spirits. Excludes products such as Alcohol Making Accessories sold separately, Non-Alcoholic Drink Making Kits and Pre-Made Alcohol.</obo:IAO_0000115>
	<obo:IAO_0000114 rdf:resource="&obo;IAO_0000428"/>
	<oboInOwl:hasDbXref>LANGUAL:A0877</oboInOwl:hasDbXref>
</owl:Class>

<owl:Class rdf:about="&obo;FOODON_03400878">
	<rdfs:label xml:lang="en">10000143 - alcohol making supplies (gs1 gpc)</rdfs:label>
	<rdfs:subClassOf rdf:resource="&obo;FOODON_03400876"/>
	<obo:IAO_0000412>http://langual.org</obo:IAO_0000412>
	<obo:IAO_0000115 xml:lang="en">Includes any products that can be described/observed as alcoholic drink making supplies; extra or replacement components for alcohol making kits or components for home put together kits. These products are individual pieces of hardware such as, siphons and fermentation locks and separately packaged ingredients such as brewers yeast.  These products can either be disposable or re-usable. Excludes products such as Alcohol Making Kits and Pre-Made Alcohol.</obo:IAO_0000115>
	<obo:IAO_0000114 rdf:resource="&obo;IAO_0000428"/>
	<oboInOwl:hasDbXref>LANGUAL:A0878</oboInOwl:hasDbXref>
</owl:Class>

<owl:Class rdf:about="&obo;FOODON_03400879">
	<rdfs:label xml:lang="en">10000591 - alcoholic beverages variety packs (gs1 gpc)</rdfs:label>
	<rdfs:subClassOf rdf:resource="&obo;FOODON_03400876"/>
	<obo:IAO_0000412>http://langual.org</obo:IAO_0000412>
	<obo:IAO_0000115 xml:lang="en">Includes any products that can be described/observed as two or more distinct Alcoholic Beverages sold together, which exist within the schema belonging to different bricks but to the same class, that is two or more products contained within the same pack which cross bricks within the Alcoholic Beverages class. Includes products such as Still and Sparkling Wine sold together. Items that are received free with purchases should be removed from the classification decision-making process. Excludes products such as Wine and Chocolate variety packs.</obo:IAO_0000115>
	<obo:IAO_0000114 rdf:resource="&obo;IAO_0000428"/>
	<oboInOwl:hasDbXref>LANGUAL:A0879</oboInOwl:hasDbXref>
</owl:Class>

<owl:Class rdf:about="&obo;FOODON_03400880">
	<rdfs:label xml:lang="en">10000589 - alcoholic cordials/syrups (gs1 gpc)</rdfs:label>
	<rdfs:subClassOf rdf:resource="&obo;FOODON_03400876"/>
	<obo:IAO_0000412>http://langual.org</obo:IAO_0000412>
	<obo:IAO_0000115 xml:lang="en">Includes any products than can be described/observed as an alcoholic liquid distilled from herbs, spices and fruits. These products contain less than 100 grams of sugar per litre. Their most common use is to add colour and/or flavour to cocktails and other long drinks. Includes products such as alcoholic Grenadine. Specifically excludes Spirits such as Brandy and Vodka, that typically have an alcohol content of around 35-40%. Excludes products such as Liqueurs and Spirits and Non Alcoholic Cordials and Syrups.</obo:IAO_0000115>
	<obo:IAO_0000114 rdf:resource="&obo;IAO_0000428"/>
	<rdfs:comment xml:lang="en">LanguaL curation note: If low alcohol claim, index in facet P. Index in facet B the type of product on which the cordial/syrup is based (i.e. fruit, dairy).</rdfs:comment>
	<oboInOwl:hasDbXref>LANGUAL:A0880</oboInOwl:hasDbXref>
</owl:Class>

<owl:Class rdf:about="&obo;FOODON_03400881">
	<rdfs:label xml:lang="en">10000144 - alcoholic pre-mixed drinks (gs1 gpc)</rdfs:label>
	<rdfs:subClassOf rdf:resource="&obo;FOODON_03400876"/>
	<obo:IAO_0000412>http://langual.org</obo:IAO_0000412>
	<obo:IAO_0000115 xml:lang="en">Includes any products that can be described/observed as a flavoured alcoholic beverage that is pre-mixed with another drink, usually a soft drink. Also includes soft or milk based drinks which have spirits added during the production process. Includes pre mixed cocktails, such as Vodka Martini and mixed wine drinks such as Spritzers and Bucks Fizz. Excludes products such as Spirits, Non-alcoholic Mixers/Coolers, Liqueurs and Alcoholic Jellies.</obo:IAO_0000115>
	<obo:IAO_0000114 rdf:resource="&obo;IAO_0000428"/>
	<rdfs:comment xml:lang="en">LanguaL curation note: Index added ingredients or flavours in facet H.</rdfs:comment>
	<oboInOwl:hasDbXref>LANGUAL:A0881</oboInOwl:hasDbXref>
</owl:Class>

<owl:Class rdf:about="&obo;FOODON_03400882">
	<rdfs:label xml:lang="en">10000159 - beer (gs1 gpc)</rdfs:label>
	<rdfs:subClassOf rdf:resource="&obo;FOODON_03400876"/>
	<obo:IAO_0000412>http://langual.org</obo:IAO_0000412>
	<obo:IAO_0000115 xml:lang="en">Includes any products that can be described/observed as a beer made by the fermentation of cereals, usually barley or hops but also maize, wheat, rice and sorghum, by the addition of yeast and water. These products are differentiated by various brewing techniques and include products described as lager, bitter, ale, stout, lambic and specialty beers. Excludes products such as Soft drinks that may be labelled as beer, such as Ginger Beer/Ale and Root Beer.</obo:IAO_0000115>
	<obo:IAO_0000114 rdf:resource="&obo;IAO_0000428"/>
	<rdfs:comment xml:lang="en">LanguaL curation note: If ingredient or flavouring added, index in facet H. If low or no alcohol claim, index in facet P. Index geographical origin in facet R.</rdfs:comment>
	<oboInOwl:hasDbXref>LANGUAL:A0882</oboInOwl:hasDbXref>
</owl:Class>

<owl:Class rdf:about="&obo;FOODON_03400883">
	<rdfs:label xml:lang="en">10000181 - cider/perry (gs1 gpc)</rdfs:label>
	<rdfs:subClassOf rdf:resource="&obo;FOODON_03400876"/>
	<obo:IAO_0000412>http://langual.org</obo:IAO_0000412>
	<obo:IAO_0000115 xml:lang="en">Includes any products that can be described/observed as a beverage that is produced by fermenting the pulp of apples or the juice of pears, with or without the addition of water and/or sugar. These products can be carbonated or non carbonated, sweet or dry, cloudy or clear. Excludes products such as Beers, Apple Wines and Non Fermented Apple/Pear Drinks and Juices.</obo:IAO_0000115>
	<obo:IAO_0000114 rdf:resource="&obo;IAO_0000428"/>
	<rdfs:comment xml:lang="en">LanguaL curation note: Index main ingredient in facet B to indicate whether the product is cider (apple) or perry (pear). Index in facet H if the product has been made effervescent by the addition of carbon dioxide gas, or if flavour or ingredient added. If low or no alcohol claim, index in facet P. Index geographical origin in facet R.</rdfs:comment>
	<oboInOwl:hasDbXref>LANGUAL:A0883</oboInOwl:hasDbXref>
</owl:Class>

<owl:Class rdf:about="&obo;FOODON_03400884">
	<rdfs:label xml:lang="en">10000227 - liqueurs (gs1 gpc)</rdfs:label>
	<rdfs:subClassOf rdf:resource="&obo;FOODON_03400876"/>
	<obo:IAO_0000412>http://langual.org</obo:IAO_0000412>
	<obo:IAO_0000115 xml:lang="en">Includes any products that can be described/observed as a strong often sweet, spirit based alcoholic beverage, which is infused with herb, fruit or nut extracts. Liqueurs are not aged for any great period of time, may use syrups, honey or cane sugar as sweeteners and may be blended with cream. Includes products which are based on various spirits such as Cognac, Brandy, Whisky, Rum and other finished spirits. Excludes products such as Spirits or Wine based alcoholic pre-mixed drinks.</obo:IAO_0000115>
	<obo:IAO_0000114 rdf:resource="&obo;IAO_0000428"/>
	<rdfs:comment xml:lang="en">LanguaL curation note: If flavouring or cream added, index in facet H.</rdfs:comment>
	<oboInOwl:hasDbXref>LANGUAL:A0884</oboInOwl:hasDbXref>
</owl:Class>

<owl:Class rdf:about="&obo;FOODON_03400885">
	<rdfs:label xml:lang="en">10000263 - spirits (gs1 gpc)</rdfs:label>
	<rdfs:subClassOf rdf:resource="&obo;FOODON_03400876"/>
	<obo:IAO_0000412>http://langual.org</obo:IAO_0000412>
	<obo:IAO_0000115 xml:lang="en">Includes any products that can be described/observed as an alcoholic beverage distilled from fermented fruit juice, fruit, grains or sugar. Products will normally have a high alcohol content of around 35-40%. Includes products such as brandy, schnapps, gin, rum, tequila, vodka and whisky. Excludes products such as Fortified Wines, Liqueurs, Non Alcoholic Bitters/Mixers, Wine.</obo:IAO_0000115>
	<obo:IAO_0000114 rdf:resource="&obo;IAO_0000428"/>
	<rdfs:comment xml:lang="en">LanguaL curation note: Index age of product under CURED OR AGED in facet H. If flavouring or ingredient added, index also in facet H. Index geographical origin in facet R.</rdfs:comment>
	<oboInOwl:hasDbXref>LANGUAL:A0885</oboInOwl:hasDbXref>
</owl:Class>

<owl:Class rdf:about="&obo;FOODON_03400886">
	<rdfs:label xml:lang="en">10000273 - wine - fortified (gs1 gpc)</rdfs:label>
	<rdfs:subClassOf rdf:resource="&obo;FOODON_03400876"/>
	<obo:IAO_0000412>http://langual.org</obo:IAO_0000412>
	<obo:IAO_0000115 xml:lang="en">Includes any products that can be described/observed as an alcoholic beverage made by the fermentation of the juice of the grape which then has the fermentation arrested by the addition of a spirit. These wines can be made in any region or country and may have a particular style of production. Includes fortified sweet wines such as Port, Madeira, Marsala and Vermouth. Excludes products such as Pineau, Pommeau and Unfortified Wines and Spirits.</obo:IAO_0000115>
	<obo:IAO_0000114 rdf:resource="&obo;IAO_0000428"/>
	<rdfs:comment xml:lang="en">LanguaL curation note: Index geographical origin in facet R.</rdfs:comment>
	<oboInOwl:hasDbXref>LANGUAL:A0886</oboInOwl:hasDbXref>
</owl:Class>

<owl:Class rdf:about="&obo;FOODON_03400887">
	<rdfs:label xml:lang="en">10000275 - wine - sparkling (gs1 gpc)</rdfs:label>
	<rdfs:subClassOf rdf:resource="&obo;FOODON_03400876"/>
	<obo:IAO_0000412>http://langual.org</obo:IAO_0000412>
	<obo:IAO_0000115 xml:lang="en">Includes any products that can be described/observed as an alcoholic beverage made by the fermentation of the juice of the grape and contains carbon dioxide gas. These products include all types of sparkling wine, Champagne, Cava and Semi-Sparkling Wine. Excludes products such as Still and Fortified Wines.</obo:IAO_0000115>
	<obo:IAO_0000114 rdf:resource="&obo;IAO_0000428"/>
	<rdfs:comment xml:lang="en">LanguaL curation note: Grape can be indexed in facet B. If low or no alcohol, index in facet P. Index in facet H if the beverage product has been made effervescent by the addition of carbon dioxide gas. Index geographical origin in facet R.</rdfs:comment>
	<oboInOwl:hasDbXref>LANGUAL:A0887</oboInOwl:hasDbXref>
</owl:Class>

<owl:Class rdf:about="&obo;FOODON_03400888">
	<rdfs:label xml:lang="en">10000276 - wine - still (gs1 gpc)</rdfs:label>
	<rdfs:subClassOf rdf:resource="&obo;FOODON_03400876"/>
	<obo:IAO_0000412>http://langual.org</obo:IAO_0000412>
	<obo:IAO_0000115 xml:lang="en">Includes any products that can be described/observed as an alcoholic beverage made by the fermentation of the juice of the grapes, usually having an alcoholic content of 14 percent or less. These products are non carbonated and can be White, Red or Rosé in colour as well as dry, sweet or medium in flavour and maybe described as 'Vintage' or 'Non Vintage'. Excludes products such as Champagne, Sparkling Wine.</obo:IAO_0000115>
	<obo:IAO_0000114 rdf:resource="&obo;IAO_0000428"/>
	<rdfs:comment xml:lang="en">LanguaL curation note: Grape can be indexed in facet B. If low or no alcohol, index in facet P. Index geographical origin in facet R. Status of food name (APPELLATION CONTROLEE, DENOMINACION DE ORIGEN CALIFICADA) can be indexed in facet Z.</rdfs:comment>
	<oboInOwl:hasDbXref>LANGUAL:A0888</oboInOwl:hasDbXref>
</owl:Class>

<owl:Class rdf:about="&obo;FOODON_03400889">
	<rdfs:label xml:lang="en">10003689 - non grape fermented alcoholic beverages - sparkling (gs1 gpc)</rdfs:label>
	<rdfs:subClassOf rdf:resource="&obo;FOODON_03400876"/>
	<obo:IAO_0000412>http://langual.org</obo:IAO_0000412>
	<obo:IAO_0000115 xml:lang="en">Includes any products than can be described/observed as an alcoholic beverage made by the fermentation of products other than grapes. These products can be fruit-based, vegetable-based, grain-based or plant-based and contain carbon dioxide gas. Includes products such as Sparkling Mead Wine. Excludes products such as Grape Based Wine, Still Non Grape Fermented Wines, Spirits, Liqueurs and Fruit/Vegetable and Grain Based Spirits.</obo:IAO_0000115>
	<obo:IAO_0000114 rdf:resource="&obo;IAO_0000428"/>
	<rdfs:comment xml:lang="en">LanguaL curation note: If low or no alcohol, index in facet P. Index the type (fruit, grain) in Facet B.</rdfs:comment>
	<oboInOwl:hasDbXref>LANGUAL:A0889</oboInOwl:hasDbXref>
</owl:Class>

<owl:Class rdf:about="&obo;FOODON_03400890">
	<rdfs:label xml:lang="en">10000588 - non grape fermented alcoholic beverages - still (gs1 gpc)</rdfs:label>
	<rdfs:subClassOf rdf:resource="&obo;FOODON_03400876"/>
	<obo:IAO_0000412>http://langual.org</obo:IAO_0000412>
	<obo:IAO_0000115 xml:lang="en">Includes any products than can be described/observed as an alcoholic beverage made by the fermentation of products other than grapes. These products can be fruit-based, vegetable-based, grain-based or plant-based and are not carbonated. Includes products such as Sake, Saki, Rhubarb Wine, Plum Wine, Mead and Hydromel. Excludes products such as Grape Based Wine, Sparkling Non Grape Fermented Wines, Spirits, Liqueurs and Fruit/Vegetable and Grain Based Spirits.</obo:IAO_0000115>
	<obo:IAO_0000114 rdf:resource="&obo;IAO_0000428"/>
	<rdfs:comment xml:lang="en">LanguaL curation note: If low or no alcohol, index in facet P. Index the type (fruit, grain) in Facet B.</rdfs:comment>
	<oboInOwl:hasDbXref>LANGUAL:A0890</oboInOwl:hasDbXref>
</owl:Class>

<owl:Class rdf:about="&obo;FOODON_03400891">
	<rdfs:label xml:lang="en">50201700 - coffee/tea/substitutes (gs1 gpc)</rdfs:label>
	<rdfs:subClassOf rdf:resource="&obo;FOODON_03400875"/>
	<obo:IAO_0000412>http://langual.org</obo:IAO_0000412>
	<obo:IAO_0000114 rdf:resource="&obo;IAO_0000428"/>
	<oboInOwl:hasDbXref>LANGUAL:A0891</oboInOwl:hasDbXref>
</owl:Class>

<owl:Class rdf:about="&obo;FOODON_03400892">
	<rdfs:label xml:lang="en">10000111 - coffee/coffee substitutes - beans/ground (gs1 gpc)</rdfs:label>
	<rdfs:subClassOf rdf:resource="&obo;FOODON_03400891"/>
	<obo:IAO_0000412>http://langual.org</obo:IAO_0000412>
	<obo:IAO_0000115 xml:lang="en">Includes any products that can be described/observed as a whole/ground bean of coffee or a coffee substitute. Whole beans must be ground by the user prior to consumption and can be used pure or blended with different coffee bean types, whereas ground coffee is prepared for consumption by the addition of water and/or milk. Includes all varieties of coffee beans such as arabica and robusta, and those from various countries such as Columbia, Ethiopia and Costa Rica Excludes products such as Coffee Beans that are consumed as confectionery and Instant Coffee.</obo:IAO_0000115>
	<obo:IAO_0000114 rdf:resource="&obo;IAO_0000428"/>
	<rdfs:comment xml:lang="en">LanguaL curation note: Index botanical variety (ARABICA , BARLEY) in facet B. Index geographical origin in facet R. Index in facet E the state in which the product is sold (whole bean, ground). Index in facet H if decaffinated or flavoured. If an industry recognized organic certification is claimed, index ORGANIC FOOD CLAIM OR USE in facet P.</rdfs:comment>
	<oboInOwl:hasDbXref>LANGUAL:A0892</oboInOwl:hasDbXref>
</owl:Class>

<owl:Class rdf:about="&obo;FOODON_03400893">
	<rdfs:label xml:lang="en">10000115 - coffee/coffee substitutes - instant (gs1 gpc)</rdfs:label>
	<rdfs:subClassOf rdf:resource="&obo;FOODON_03400891"/>
	<obo:IAO_0000412>http://langual.org</obo:IAO_0000412>
	<obo:IAO_0000115 xml:lang="en">Includes any products that can be described/observed as a substance made from the ground beans of the coffee tree and/or the root of the Chicory plant or other coffee substitute which makes coffee instantly on the addition of hot water and/or hot milk. Includes products with added dry milk or whitener and both decaffeinated and with caffeine varieties. Excludes products such as Ground Coffee, Liquid Coffee and Iced Coffee.</obo:IAO_0000115>
	<obo:IAO_0000114 rdf:resource="&obo;IAO_0000428"/>
	<rdfs:comment xml:lang="en">LanguaL curation note: Index botanical variety (ARABICA , BARLEY) in facet B. Index geographical origin in facet R. Index in facet E the state in which the product is sold (liquid, powder). Index in facet H if decaffinated or flavoured, or if coffee whitener (POWDERED MILK, POWDERED MILK SUBSTITUTE) has been added. If an industry recognized organic certification is claimed, index ORGANIC FOOD CLAIM OR USE in facet P.</rdfs:comment>
	<oboInOwl:hasDbXref>LANGUAL:A0893</oboInOwl:hasDbXref>
</owl:Class>

<owl:Class rdf:about="&obo;FOODON_03400894">
	<rdfs:label xml:lang="en">10000114 - coffee/coffee substitutes - ready to drink (gs1 gpc)</rdfs:label>
	<rdfs:subClassOf rdf:resource="&obo;FOODON_03400891"/>
	<obo:IAO_0000412>http://langual.org</obo:IAO_0000412>
	<obo:IAO_0000115 xml:lang="en">Includes any products that can be described/observed as a ready to drink non-carbonated beverage made from coffee beans or coffee substitutes such as chicory. Includes products that are consumed cold and those sold in 'self heating' cans, which allow the consumer to heat the coffee prior to consumption. Includes black coffee and coffees with added flavourings (such as mocha), milk or sweeteners. Excludes products such as Not Ready to Drink Coffees and Ready to Drink Teas.</obo:IAO_0000115>
	<obo:IAO_0000114 rdf:resource="&obo;IAO_0000428"/>
	<rdfs:comment xml:lang="en">LanguaL curation note: Index in facet H if decaffinated or flavoured or if coffee whitener (POWDERED MILK, POWDERED MILK SUBSTITUTE) has been added. If an industry recognized organic certification is claimed, index ORGANIC FOOD CLAIM OR USE in facet P.</rdfs:comment>
	<oboInOwl:hasDbXref>LANGUAL:A0894</oboInOwl:hasDbXref>
</owl:Class>

<owl:Class rdf:about="&obo;FOODON_03400895">
	<rdfs:label xml:lang="en">10000592 - coffee/tea/substitutes variety packs (gs1 gpc)</rdfs:label>
	<rdfs:subClassOf rdf:resource="&obo;FOODON_03400891"/>
	<obo:IAO_0000412>http://langual.org</obo:IAO_0000412>
	<obo:IAO_0000115 xml:lang="en">Includes any products that can be described/observed as two or more distinct Coffee, Tea or Substitutes sold together, which exist within the schema belonging to different bricks but to the same class, that is two or more products contained within the same pack which cross bricks within the Coffee, Tea and Substitutes class. Includes products such as Ground Coffee and Tea Bags sold together. Excludes products such as Coffee and Cream variety packs.</obo:IAO_0000115>
	<obo:IAO_0000114 rdf:resource="&obo;IAO_0000428"/>
	<oboInOwl:hasDbXref>LANGUAL:A0895</oboInOwl:hasDbXref>
</owl:Class>

<owl:Class rdf:about="&obo;FOODON_03400896">
	<rdfs:label xml:lang="en">10000119 - fruit herbal infusions - bags/loose (gs1 gpc)</rdfs:label>
	<rdfs:subClassOf rdf:resource="&obo;FOODON_03400891"/>
	<obo:IAO_0000412>http://langual.org</obo:IAO_0000412>
	<obo:IAO_0000115 xml:lang="en">Includes any products that can be described/observed as loose fruit or herbal tea, which is derived from the dried leaves of an infusion of dried fruits, herbs, spices and flowers, used specifically to make a long drink. Includes herbal teas of various flavours such as apple, ginseng, jasmine and cinnamon, and bags which contain blends of any of these such as apple and cinnamon. Specifically includes herbal infusions and fruit teas contained in tea bags. Excludes products such as Instant Fruit or Herbal Tea, and Bouquet Garni.</obo:IAO_0000115>
	<obo:IAO_0000114 rdf:resource="&obo;IAO_0000428"/>
	<rdfs:comment xml:lang="en">LanguaL curation note: Index the Variety of Fruit Herbal Infusion in facet B and the part of plant (fruit, leaves) in facet C. Index in facet H if the product is Naturally Flavoured. If the product is sold in bags, index in facet M. If an industry recognized organic certification is claimed, index ORGANIC FOOD CLAIM OR USE in facet P.</rdfs:comment>
	<oboInOwl:hasDbXref>LANGUAL:A0896</oboInOwl:hasDbXref>
</owl:Class>

<owl:Class rdf:about="&obo;FOODON_03400897">
	<rdfs:label xml:lang="en">10000210 - fruit herbal infusions - instant (gs1 gpc)</rdfs:label>
	<rdfs:subClassOf rdf:resource="&obo;FOODON_03400891"/>
	<obo:IAO_0000412>http://langual.org</obo:IAO_0000412>
	<obo:IAO_0000115 xml:lang="en">Includes any products that can be described/observed as a fruit or herbal tea, which is prepared for consumption by the addition of hot water and/or hot milk and is derived in part or in total from one or more species of fruit, herb, spice or flower and does not require straining. Includes herbal teas of various flavours such as apple, ginseng, jasmine and cinnamon, and blends of any of these such as apple and cinnamon. Excludes products such as Fruit/Herbal Tea which is Loose or in Bags, all other types of Powdered Tea, Ready-to-Drink Teas and Tea Substitutes.</obo:IAO_0000115>
	<obo:IAO_0000114 rdf:resource="&obo;IAO_0000428"/>
	<rdfs:comment xml:lang="en">LanguaL curation note: Index the Variety of Fruit Herbal Infusion in facet B. If an industry recognized organic certification is claimed, index ORGANIC FOOD CLAIM OR USE in facet P. Index in facet E the state in which the product is sold (liquid, powder). Index in facet H if creamer/whitener (POWDERED MILK, POWDERED MILK SUBSTITUTE) or flavoring has been added.</rdfs:comment>
	<oboInOwl:hasDbXref>LANGUAL:A0897</oboInOwl:hasDbXref>
</owl:Class>

<owl:Class rdf:about="&obo;FOODON_03400898">
	<rdfs:label xml:lang="en">10000313 - fruit herbal infusions - ready to drink (gs1 gpc)</rdfs:label>
	<rdfs:subClassOf rdf:resource="&obo;FOODON_03400891"/>
	<obo:IAO_0000412>http://langual.org</obo:IAO_0000412>
	<obo:IAO_0000115 xml:lang="en">Includes any products that can be described/observed as a ready to drink beverage, which is derived in part or in total from one or more species of fruit, herb, spice or flower and does not require any further preparation. Includes products sold in containers with a self-heating mechanism and those with added flavourings and milk or sweeteners. Excludes products such as Not Ready To Drink Fruit Herbal Infusions and all Teas.</obo:IAO_0000115>
	<obo:IAO_0000114 rdf:resource="&obo;IAO_0000428"/>
	<rdfs:comment xml:lang="en">LanguaL curation note: Index the Variety of Fruit Herbal Infusion in facet B. If an industry recognized organic certification is claimed, index ORGANIC FOOD CLAIM OR USE in facet P.</rdfs:comment>
	<oboInOwl:hasDbXref>LANGUAL:A0898</oboInOwl:hasDbXref>
</owl:Class>

<owl:Class rdf:about="&obo;FOODON_03400899">
	<rdfs:label xml:lang="en">10000116 - tea - bags/loose (gs1 gpc)</rdfs:label>
	<rdfs:subClassOf rdf:resource="&obo;FOODON_03400891"/>
	<obo:IAO_0000412>http://langual.org</obo:IAO_0000412>
	<obo:IAO_0000115 xml:lang="en">Includes any products that can be described/observed as loose tea that is derived from the dried leaves of the tea plant, Camellia Sinensis. Specifically includes tea contained in tea bags. Excludes products such as Ready-to-Drink Teas, Instant Teas and Herbal Infusions.</obo:IAO_0000115>
	<obo:IAO_0000114 rdf:resource="&obo;IAO_0000428"/>
	<rdfs:comment xml:lang="en">LanguaL curation note: If the product is sold in bags; index in facet M. Index in facet H if the product is flavoured. If an industry recognized organic certification is claimed, index ORGANIC FOOD CLAIM OR USE in facet P. Index the geographical origin of the tea in facet R.</rdfs:comment>
	<oboInOwl:hasDbXref>LANGUAL:A0899</oboInOwl:hasDbXref>
</owl:Class>

<owl:Class rdf:about="&obo;FOODON_03400900">
	<rdfs:label xml:lang="en">10000117 - tea - instant (gs1 gpc)</rdfs:label>
	<rdfs:subClassOf rdf:resource="&obo;FOODON_03400891"/>
	<obo:IAO_0000412>http://langual.org</obo:IAO_0000412>
	<obo:IAO_0000115 xml:lang="en">Includes any products that can be described/observed as a beverage, which is prepared for consumption by the addition of hot water and/or hot milk and is derived in part or in total from the dried leaves of the tea plant, Camellia Sinensis and does not require straining. Includes both flavoured (such as with lemon) and non-flavoured varieties. Excludes products such as Tea Bags or Loose Tea, Ready-to-Drink Teas and Tea Substitutes.</obo:IAO_0000115>
	<obo:IAO_0000114 rdf:resource="&obo;IAO_0000428"/>
	<rdfs:comment xml:lang="en">LanguaL curation note: Index in facet E the state in which the product is sold (liquid, powder). Index in facet H if creamer/whitener (POWDERED MILK, POWDERED MILK SUBSTITUTE) or flavoring has been added. If an industry recognized organic certification is claimed, index ORGANIC FOOD CLAIM OR USE in facet P. Index the geographical origin of the tea in facet R.</rdfs:comment>
	<oboInOwl:hasDbXref>LANGUAL:A0900</oboInOwl:hasDbXref>
</owl:Class>

<owl:Class rdf:about="&obo;FOODON_03400901">
	<rdfs:label xml:lang="en">10000118 - tea - ready to drink (gs1 gpc)</rdfs:label>
	<rdfs:subClassOf rdf:resource="&obo;FOODON_03400891"/>
	<obo:IAO_0000412>http://langual.org</obo:IAO_0000412>
	<obo:IAO_0000115 xml:lang="en">Includes any products that can be described/observed as a ready to drink beverage made from the dried leaves of the tea plant, Camellia Sinensis. Includes self-heating products and teas from single tea types such as Assam and Ceylon, and those, which are blends of various teas. Products may also have added flavourings such as lemon and milk or sweeteners. Excludes products such as Not Ready To Drink Teas, Ready to Drink Fruit Herbal Infusions, Instant Tea and Ready To Drink Coffees.</obo:IAO_0000115>
	<obo:IAO_0000114 rdf:resource="&obo;IAO_0000428"/>
	<rdfs:comment xml:lang="en">LanguaL curation note: Index in facet H if creamer/whitener (POWDERED MILK, POWDERED MILK SUBSTITUTE) or flavoring has been added. If an industry recognized organic certification is claimed, index ORGANIC FOOD CLAIM OR USE in facet P. Index the geographical origin of the tea in facet R.</rdfs:comment>
	<oboInOwl:hasDbXref>LANGUAL:A0901</oboInOwl:hasDbXref>
</owl:Class>

<owl:Class rdf:about="&obo;FOODON_03400902">
	<rdfs:label xml:lang="en">50202400 - non alcoholic beverages - not ready to drink (gs1 gpc)</rdfs:label>
	<rdfs:subClassOf rdf:resource="&obo;FOODON_03400875"/>
	<obo:IAO_0000412>http://langual.org</obo:IAO_0000412>
	<obo:IAO_0000114 rdf:resource="&obo;IAO_0000428"/>
	<oboInOwl:hasDbXref>LANGUAL:A0902</oboInOwl:hasDbXref>
</owl:Class>

<owl:Class rdf:about="&obo;FOODON_03400903">
	<rdfs:label xml:lang="en">10000178 - chocolate/cocoa/malt - not ready to drink (gs1 gpc)</rdfs:label>
	<rdfs:subClassOf rdf:resource="&obo;FOODON_03400902"/>
	<obo:IAO_0000412>http://langual.org</obo:IAO_0000412>
	<obo:IAO_0000115 xml:lang="en">Includes any products that can be described/observed as a liquid, powder or granules made from either cocoa beans, malted barley, corn starch or other grain extracts, which when diluted by hot water/hot milk, makes an instant drink. These products may also require the addition of sugar. Specifically excludes flavoured milk and dairy based drinks to which chocolate flavouring has been added, and those that are not based on cocoa beans/powder. Excludes products such as Ready to Drink Chocolate, Malt and Cocoa, Chocolate Flavoured Milk and Dairy Based Drinks such as Chocolate Flavoured Milk Shakes, Baby &amp; Infant Specialised Beverages</obo:IAO_0000115>
	<obo:IAO_0000114 rdf:resource="&obo;IAO_0000428"/>
	<rdfs:comment xml:lang="en">LanguaL curation note: Index consumer lifestage (child, any age) and label claims (diet/lite) in facet P. Index in facet E the state in which the product is sold (liquid, powder). Index main ingredient in facet B. If instantized or if ingredients added (milk, malt), index in facet H.</rdfs:comment>
	<oboInOwl:hasDbXref>LANGUAL:A0903</oboInOwl:hasDbXref>
</owl:Class>

<owl:Class rdf:about="&obo;FOODON_03400904">
	<rdfs:label xml:lang="en">10000310 - dairy/dairy substitute based drinks - not ready to drink (shelf stable) (gs1 gpc)</rdfs:label>
	<rdfs:subClassOf rdf:resource="&obo;FOODON_03400902"/>
	<obo:IAO_0000412>http://langual.org</obo:IAO_0000412>
	<obo:IAO_0000115 xml:lang="en">Includes any products that can be described/observed as not ready to drink dairy or dairy substitute-based products, which are specifically designed to be consumed as a beverage and may often be flavoured. Products include both fermented, such as drinking yogurt, laban, kefir, yger, airag, kumis, kvass and non-fermented, such as milkshake, dairy and dairy substitutes drinks. These products have been treated or packaged in such a way as to extend their consumable life. Specifically excludes Chocolate, Cocoa and Malt Drinks. Excludes products such as Ready to Drink Dairy and Dairy Substitutes Based Drinks, all Milk and Milk Substitutes, Spoonable Yogurt and Dairy Based beverages specifically designed for babies and infants.</obo:IAO_0000115>
	<obo:IAO_0000114 rdf:resource="&obo;IAO_0000428"/>
	<rdfs:comment xml:lang="en">LanguaL curation note: Index consumer lifestage (child, any age) and label claims (diet, probiotic) in facet P. Index in facet E the state in which the product is sold (liquid, powder). Index main ingredient in facet B. If fermented or if ingredients (fruit, flavouring) added, index in facet H.</rdfs:comment>
	<oboInOwl:hasDbXref>LANGUAL:A0904</oboInOwl:hasDbXref>
</owl:Class>

<owl:Class rdf:about="&obo;FOODON_03400905">
	<rdfs:label xml:lang="en">10000202 - drinks flavoured - not ready to drink (gs1 gpc)</rdfs:label>
	<rdfs:subClassOf rdf:resource="&obo;FOODON_03400902"/>
	<obo:IAO_0000412>http://langual.org</obo:IAO_0000412>
	<obo:IAO_0000115 xml:lang="en">Includes any products that can be described/observed as a sweet powder or concentrate that, when diluted by water, makes a carbonated or non-carbonated beverage that includes no juice or dairy/dairy-substitute ingredients. These products are usually artificially flavoured and coloured. Products include carbonated drinks, which contain caffeine and those sweetened with sugar or artificial sweeteners. Excludes products such as Ready to Drink Flavoured Drinks, all Juice Drinks and Dairy and Dairy Substitute Drinks.</obo:IAO_0000115>
	<obo:IAO_0000114 rdf:resource="&obo;IAO_0000428"/>
	<rdfs:comment xml:lang="en">LanguaL curation note: Index added ingredients (vitamins, fruit) in facet H. Index added preservatives in facet J. Index in facet E the state in which the product is sold (powder, liquid). Index Cafeine and Diet/Lite claims in facet P.</rdfs:comment>
	<oboInOwl:hasDbXref>LANGUAL:A0905</oboInOwl:hasDbXref>
</owl:Class>

<owl:Class rdf:about="&obo;FOODON_03400906">
	<rdfs:label xml:lang="en">10000307 - juice - not ready to drink (frozen) (gs1 gpc)</rdfs:label>
	<rdfs:subClassOf rdf:resource="&obo;FOODON_03400902"/>
	<obo:IAO_0000412>http://langual.org</obo:IAO_0000412>
	<obo:IAO_0000115 xml:lang="en">Includes any products that can be described/observed as a frozen concentrate that is made exclusively from the extracted fluid content of a fruit or vegetable and that, when diluted with water, makes an instant juice beverage. These products must be frozen to extend their consumable life. Products include individual and blended pure juice varieties. Excludes products such as Shelf Stable and Perishable Ready to Drink Juices and Not Ready to Drink Juices, Baby &amp; Infant Specialized Beverages.</obo:IAO_0000115>
	<obo:IAO_0000114 rdf:resource="&obo;IAO_0000428"/>
	<rdfs:comment xml:lang="en">LanguaL curation note: Index type of juice in facet B. If an industry recognized organic certification is claimed, index ORGANIC FOOD CLAIM OR USE in facet P. Index Diet/Lite claim in facet P.</rdfs:comment>
	<oboInOwl:hasDbXref>LANGUAL:A0906</oboInOwl:hasDbXref>
</owl:Class>

<owl:Class rdf:about="&obo;FOODON_03400907">
	<rdfs:label xml:lang="en">10000308 - juice - not ready to drink (shelf stable) (gs1 gpc)</rdfs:label>
	<rdfs:subClassOf rdf:resource="&obo;FOODON_03400902"/>
	<obo:IAO_0000412>http://langual.org</obo:IAO_0000412>
	<obo:IAO_0000115 xml:lang="en">Includes any products that can be described/observed as a powder or a concentrate that is made exclusively from the extracted fluid content of a fruit or vegetable and that, when diluted with water, makes an instant juice beverage. These products have been treated or packaged in such a way as to extend their consumable life. Products include individual and blended pure juice varieties. Excludes products such as Perishable and Frozen Not Ready to Drink Juices and Ready to Drink Juices, Baby &amp; Infant Specialized Beverages.</obo:IAO_0000115>
	<obo:IAO_0000114 rdf:resource="&obo;IAO_0000428"/>
	<rdfs:comment xml:lang="en">LanguaL curation note: Index type of juice in facet B. Index in facet E the state in which the product is sold (powder, liquid). If an industry recognized organic certification is claimed, index ORGANIC FOOD CLAIM OR USE in facet P. Index Diet/Lite claim in facet P.</rdfs:comment>
	<oboInOwl:hasDbXref>LANGUAL:A0907</oboInOwl:hasDbXref>
</owl:Class>

<owl:Class rdf:about="&obo;FOODON_03400908">
	<rdfs:label xml:lang="en">10000309 - juice drinks - not ready to drink (shelf stable) (gs1 gpc)</rdfs:label>
	<rdfs:subClassOf rdf:resource="&obo;FOODON_03400902"/>
	<obo:IAO_0000412>http://langual.org</obo:IAO_0000412>
	<obo:IAO_0000115 xml:lang="en">Includes any products that can be described/observed as a powder or concentrate that contains some fruit or vegetable juice together with additional ingredients, such as water, sugar, colourings and flavourings that, when diluted by water, makes an instant juice drink. These products have been treated or packaged in such a way as to extend their consumable life. Products include individual and blended juice drink varieties. Excludes products such as Ready to Drink Juice Drinks and all 100% Juices, Baby &amp; Infant Specialized Beverages.</obo:IAO_0000115>
	<obo:IAO_0000114 rdf:resource="&obo;IAO_0000428"/>
	<rdfs:comment xml:lang="en">LanguaL curation note: Index type of juice in facet B. Index in facet E the state in which the product is sold (powder, liquid). Index consumer lifestage (child, any age) and label claims (diet) in facet P.</rdfs:comment>
	<oboInOwl:hasDbXref>LANGUAL:A0908</oboInOwl:hasDbXref>
</owl:Class>

<owl:Class rdf:about="&obo;FOODON_03400909">
	<rdfs:label xml:lang="en">10000593 - non alcoholic beverages variety packs - not ready to drink (gs1 gpc)</rdfs:label>
	<rdfs:subClassOf rdf:resource="&obo;FOODON_03400902"/>
	<obo:IAO_0000412>http://langual.org</obo:IAO_0000412>
	<obo:IAO_0000115 xml:lang="en">Includes any products that can be described/observed as two or more distinct Non Alcoholic Beverages Not Ready to Drink sold together, which exist within the schema belonging to different bricks but to the same class, that is two or more products contained within the same pack which cross bricks within the Non Alcoholic Beverages - Not Ready to Drink class. Includes products such as powdered Malt and Milkshakes sold together. Items that are received free with purchases should be removed from the classification decision-making process. Excludes products such as powdered Milkshakes and Sugar Candy variety packs.</obo:IAO_0000115>
	<obo:IAO_0000114 rdf:resource="&obo;IAO_0000428"/>
	<oboInOwl:hasDbXref>LANGUAL:A0909</oboInOwl:hasDbXref>
</owl:Class>

<owl:Class rdf:about="&obo;FOODON_03400910">
	<rdfs:label xml:lang="en">10000264 - sports drinks - rehydration (not ready to drink) (gs1 gpc)</rdfs:label>
	<rdfs:subClassOf rdf:resource="&obo;FOODON_03400902"/>
	<obo:IAO_0000412>http://langual.org</obo:IAO_0000412>
	<obo:IAO_0000115 xml:lang="en">Includes any products that can be described/observed as a beverage, which contains carbohydrates and electrolytes, designed to accelerate rehydration of cells by osmosis, normally consumed after a sporting activity. These products require the addition of water or other liquids prior to consumption and may be sold in liquid, powder or granular form. Includes products of various flavours such as orange and lemon. Excludes products such as Sports Drinks - Rehydration - Ready to Drink and all Stimulants/Energy Drinks.</obo:IAO_0000115>
	<obo:IAO_0000114 rdf:resource="&obo;IAO_0000428"/>
	<rdfs:comment xml:lang="en">LanguaL curation note: Index in facet E the state in which the product is sold (powder, liquid). Index in facet H if it has been made effervescent by the addition of carbon dioxide gas. Index cafeine and diet claims in facet P.</rdfs:comment>
	<oboInOwl:hasDbXref>LANGUAL:A0910</oboInOwl:hasDbXref>
</owl:Class>

<owl:Class rdf:about="&obo;FOODON_03400911">
	<rdfs:label xml:lang="en">10000311 - stimulants/energy drinks - not ready to drink (gs1 gpc)</rdfs:label>
	<rdfs:subClassOf rdf:resource="&obo;FOODON_03400902"/>
	<obo:IAO_0000412>http://langual.org</obo:IAO_0000412>
	<obo:IAO_0000115 xml:lang="en">Includes any products that can be described/observed as a powder or concentrate that, when diluted by water, makes an instant beverage containing taurine, guaranine, caffeine or other stimulants designed to give the consumer a short term boost of energy. Includes products of various flavours such as orange and lemon. Specifically excludes flavoured drink powders or concentrates that contain caffeine (such as Cola) but are not labelled and marketed with energy enhancing properties. Excludes products such as Stimulants/Energy Drinks - Ready to Drink and all Rehydration Sports Drinks.</obo:IAO_0000115>
	<obo:IAO_0000114 rdf:resource="&obo;IAO_0000428"/>
	<rdfs:comment xml:lang="en">LanguaL curation note: Index in facet E the state in which the product is sold (powder, liquid). Index cafeine and diet claims in facet P.</rdfs:comment>
	<oboInOwl:hasDbXref>LANGUAL:A0911</oboInOwl:hasDbXref>
</owl:Class>

<owl:Class rdf:about="&obo;FOODON_03400912">
	<rdfs:label xml:lang="en">50202300 - non alcoholic beverages - ready to drink (gs1 gpc)</rdfs:label>
	<rdfs:subClassOf rdf:resource="&obo;FOODON_03400875"/>
	<obo:IAO_0000412>http://langual.org</obo:IAO_0000412>
	<obo:IAO_0000114 rdf:resource="&obo;IAO_0000428"/>
	<oboInOwl:hasDbXref>LANGUAL:A0912</oboInOwl:hasDbXref>
</owl:Class>

<owl:Class rdf:about="&obo;FOODON_03400913">
	<rdfs:label xml:lang="en">10000179 - chocolate/cocoa/malt - ready to drink (gs1 gpc)</rdfs:label>
	<rdfs:subClassOf rdf:resource="&obo;FOODON_03400912"/>
	<obo:IAO_0000412>http://langual.org</obo:IAO_0000412>
	<obo:IAO_0000115 xml:lang="en">Includes any products that can be described/observed as a ready to drink liquid made from either cocoa beans/powder, malted barley, corn starch or other grain extracts, and sometimes incorporating milk, sugar, egg extract or other ingredients. Specifically excludes flavoured milk and dairy based drinks to which chocolate flavouring has been added, and those that are not based on cocoa beans/powder. Excludes products such as Not Ready to Drink Chocolate, Malt and Cocoa, Chocolate Flavoured Milk and Dairy Based Drinks such as Chocolate Flavoured Milk Shakes, Baby and Infant Specialized Beverages.</obo:IAO_0000115>
	<obo:IAO_0000114 rdf:resource="&obo;IAO_0000428"/>
	<rdfs:comment xml:lang="en">LanguaL curation note: Index consumer lifestage (child, any age) and label claims (diet/lite) in facet P. Index main ingredient in facet B. If fermented or homogenized, or if milk added, index in facet H. Index preservation method (pasteurised, sterilized) in facet J.</rdfs:comment>
	<oboInOwl:hasDbXref>LANGUAL:A0913</oboInOwl:hasDbXref>
</owl:Class>

<owl:Class rdf:about="&obo;FOODON_03400914">
	<rdfs:label xml:lang="en">10000191 - dairy/dairy substitute based drinks - ready to drink (perishable) (gs1 gpc)</rdfs:label>
	<rdfs:subClassOf rdf:resource="&obo;FOODON_03400912"/>
	<obo:IAO_0000412>http://langual.org</obo:IAO_0000412>
	<obo:IAO_0000115 xml:lang="en">Includes any products that can be described/observed as ready to drink dairy or dairy substitute-based products, which are specifically designed to be consumed as a beverage and may often be flavoured. Products include both fermented, such as buttermilk, drinking yogurt, laban, kefir, yger, airag, kumis, kvass and non-fermented, such as milkshake, dairy and dairy substitute drinks. Products specifically include those marketed as health drinks. These products must be refrigerated to extend their consumable life. Specifically excludes Chocolate, Cocoa and Malt Drinks. Excludes products such as Shelf Stable Ready to Drink Dairy and Dairy Substitutes Based Drinks, Not Ready to Drink Dairy and Dairy Substitutes Based Drinks all Milk and Milk Substitutes, Spoonable Yogurt and Dairy Based beverages specifically designed for babies and infants.</obo:IAO_0000115>
	<obo:IAO_0000114 rdf:resource="&obo;IAO_0000428"/>
	<rdfs:comment xml:lang="en">LanguaL curation note: Index consumer lifestage (child, any age) and label claims (diet, probiotic) in facet P. Index main ingredient in facet B. If fermented or if ingredients (fruit, flavouring) added, index in facet H. Index preservation method (refrigerated) in facet J.</rdfs:comment>
	<oboInOwl:hasDbXref>LANGUAL:A0914</oboInOwl:hasDbXref>
</owl:Class>

<owl:Class rdf:about="&obo;FOODON_03400915">
	<rdfs:label xml:lang="en">10000192 - dairy/dairy substitute based drinks - ready to drink (shelf stable) (gs1 gpc)</rdfs:label>
	<rdfs:subClassOf rdf:resource="&obo;FOODON_03400912"/>
	<obo:IAO_0000412>http://langual.org</obo:IAO_0000412>
	<obo:IAO_0000115 xml:lang="en">Includes any products that can be described/observed as ready to drink dairy or dairy substitute-based products, which are specifically designed to be consumed as a beverage and may often be flavoured. Products include both fermented, such as buttermilk, drinking yogurt, laban, kefir, yger, airag, kumis, kvass and non-fermented, such as milkshake or whey drink. Products specifically include those marketed as health drinks. These products have been treated or packaged in such a way as to extend their consumable life. Specifically excludes Chocolate, Cocoa and Malt Drinks. Excludes products such as Perishable Ready to Drink Dairy and Dairy Substitutes Based Drinks, Not Ready to Drink Dairy and Dairy Substitutes Based Drinks, all Milk and Milk Substitutes, Spoonable Yogurt and Dairy Based beverages specifically designed for babies and infants.</obo:IAO_0000115>
	<obo:IAO_0000114 rdf:resource="&obo;IAO_0000428"/>
	<rdfs:comment xml:lang="en">LanguaL curation note: Index consumer lifestage (child, any age) and label claims (diet, probiotic) in facet P. Index main ingredient in facet B. If fermented or if ingredients (fruit, flavouring) added, index in facet H. Index preservation method (pasteurised, sterilized) in facet J.</rdfs:comment>
	<oboInOwl:hasDbXref>LANGUAL:A0915</oboInOwl:hasDbXref>
</owl:Class>

<owl:Class rdf:about="&obo;FOODON_03400916">
	<rdfs:label xml:lang="en">10000201 - drinks flavoured - ready to drink (gs1 gpc)</rdfs:label>
	<rdfs:subClassOf rdf:resource="&obo;FOODON_03400912"/>
	<obo:IAO_0000412>http://langual.org</obo:IAO_0000412>
	<obo:IAO_0000115 xml:lang="en">Includes any products that can be described/observed as a sweet, ready to drink, carbonated or non-carbonated beverage that includes no dairy/dairy-substitute ingredients. These products are usually artificially flavoured and coloured. Products include carbonated drinks which contain caffeine and those sweetened with sugar or artificial sweeteners. Also includes fruit based carbonated drinks. Specifically excludes all non-carbonated juice based drinks and 100% juices. Excludes products such as Not Ready to Drink Flavoured Drinks, all Juice Drinks and Dairy and Dairy Substitute Drinks.</obo:IAO_0000115>
	<obo:IAO_0000114 rdf:resource="&obo;IAO_0000428"/>
	<rdfs:comment xml:lang="en">LanguaL curation note: In facet H index addition of ingredients (vitamins, fruit) or carbon dioxide gas. Index cafeine and diet claims in facet P. Index preservatives added in facet J.</rdfs:comment>
	<oboInOwl:hasDbXref>LANGUAL:A0916</oboInOwl:hasDbXref>
</owl:Class>

<owl:Class rdf:about="&obo;FOODON_03400917">
	<rdfs:label xml:lang="en">10000214 - ice (gs1 gpc)</rdfs:label>
	<rdfs:subClassOf rdf:resource="&obo;FOODON_03400912"/>
	<obo:IAO_0000412>http://langual.org</obo:IAO_0000412>
	<obo:IAO_0000115 xml:lang="en">Includes any products that can be described/observed as frozen water formed into shapes such as cubes or blocks, which are usually used to chill beverages. These products must be frozen to extend their consumable life. Excludes products such as Frozen Flavoured Ice Pops or Lollies.</obo:IAO_0000115>
	<obo:IAO_0000114 rdf:resource="&obo;IAO_0000428"/>
	<rdfs:comment xml:lang="en">LanguaL curation note: Index physical state (cube, crushed) in facet E.</rdfs:comment>
	<oboInOwl:hasDbXref>LANGUAL:A0917</oboInOwl:hasDbXref>
</owl:Class>

<owl:Class rdf:about="&obo;FOODON_03400918">
	<rdfs:label xml:lang="en">10000219 - juice - ready to drink (perishable) (gs1 gpc)</rdfs:label>
	<rdfs:subClassOf rdf:resource="&obo;FOODON_03400912"/>
	<obo:IAO_0000412>http://langual.org</obo:IAO_0000412>
	<obo:IAO_0000115 xml:lang="en">Includes any products that can be described/observed as a ready to drink, non-carbonated beverage that is made exclusively from the extracted fluid content of a fruit or vegetable. These products must be refrigerated to extend their consumable life. Products include individual and blended pure juice varieties. Excludes products such as Shelf Stable and Frozen Ready to Drink Juices and Not Ready to Drink Juices, Baby &amp; Infant Specialized Beverages.</obo:IAO_0000115>
	<obo:IAO_0000114 rdf:resource="&obo;IAO_0000428"/>
	<rdfs:comment xml:lang="en">LanguaL curation note: Index type of juice in facet B. If reconstituted from concentrate, index in facet H. If an industry recognized organic certification is claimed, index ORGANIC FOOD CLAIM OR USE in facet P. Index Diet/Lite claim in facet P. Index preservation method (refrigerated) in facet J.</rdfs:comment>
	<oboInOwl:hasDbXref>LANGUAL:A0918</oboInOwl:hasDbXref>
</owl:Class>

<owl:Class rdf:about="&obo;FOODON_03400919">
	<rdfs:label xml:lang="en">10000220 - juice - ready to drink (shelf stable) (gs1 gpc)</rdfs:label>
	<rdfs:subClassOf rdf:resource="&obo;FOODON_03400912"/>
	<obo:IAO_0000412>http://langual.org</obo:IAO_0000412>
	<obo:IAO_0000115 xml:lang="en">Includes any products that can be described/observed as a ready to drink, carbonated or non-carbonated beverage that is made exclusively from the extracted fluid content of a fruit or vegetable. These products have been treated or packaged in such a way as to extend their consumable life. Products include individual and blended pure juice varieties. Excludes products such as Perishable and Frozen Ready to Drink Juices and Not Ready to Drink Juices, Baby Specialized Beverages.</obo:IAO_0000115>
	<obo:IAO_0000114 rdf:resource="&obo;IAO_0000428"/>
	<rdfs:comment xml:lang="en">LanguaL curation note: Index type of juice in facet B. If reconstituted from concentrate or if carbonated, index in facet H. If an industry recognized organic certification is claimed, index ORGANIC FOOD CLAIM OR USE in facet P. Index Diet/Lite claim in facet P. Index preservation method (pasteurised, sterilized) in facet J.</rdfs:comment>
	<oboInOwl:hasDbXref>LANGUAL:A0919</oboInOwl:hasDbXref>
</owl:Class>

<owl:Class rdf:about="&obo;FOODON_03400920">
	<rdfs:label xml:lang="en">10000222 - juice drinks - ready to drink (perishable) (gs1 gpc)</rdfs:label>
	<rdfs:subClassOf rdf:resource="&obo;FOODON_03400912"/>
	<obo:IAO_0000412>http://langual.org</obo:IAO_0000412>
	<obo:IAO_0000115 xml:lang="en">Includes any products that can be described/observed as a perishable, ready to drink non-carbonated beverage, that contains some fruit or vegetable juice together with additional ingredients such as water, sugar, colourings and flavourings. These products must be refrigerated to extend their consumable life. Includes products that may be described as Nectar, Fruit Drink or Juice Drink and available in single flavours such as carrot, tomato, orange and apple or they may be blends of more than one such as orange &amp; apricot, cranberry &amp; raspberry. Excludes products such as Frozen and Shelf Stable Juice Drinks, Juice, Syrups, Juice Concentrate, 100% Juices, Flavoured Mixers, Mineral Water, Baby &amp; Infant Specialized Beverages.</obo:IAO_0000115>
	<obo:IAO_0000114 rdf:resource="&obo;IAO_0000428"/>
	<rdfs:comment xml:lang="en">LanguaL curation note: Index consumer lifestage (child, any age) and label claims (diet/lite) in facet P. Index main ingredient in facet B. Index added ingredients (fruit, flavouring) in facet H. Index preservation method (refrigerated) in facet J.</rdfs:comment>
	<oboInOwl:hasDbXref>LANGUAL:A0920</oboInOwl:hasDbXref>
</owl:Class>

<owl:Class rdf:about="&obo;FOODON_03400921">
	<rdfs:label xml:lang="en">10000223 - juice drinks - ready to drink (shelf stable) (gs1 gpc)</rdfs:label>
	<rdfs:subClassOf rdf:resource="&obo;FOODON_03400912"/>
	<obo:IAO_0000412>http://langual.org</obo:IAO_0000412>
	<obo:IAO_0000115 xml:lang="en">Includes any products that can be described/observed as a shelf stable ready to drink, non-carbonated beverage that contains some fruit or vegetable juice together with additional ingredients, such as water, sugar, colourings and flavourings. These products have been specially treated or packaged in such a way as to extend their consumable life. Products include individual and blended juice drink varieties. Excludes products such as Frozen and Perishable Juice Drinks and all 100% Juices.</obo:IAO_0000115>
	<obo:IAO_0000114 rdf:resource="&obo;IAO_0000428"/>
	<rdfs:comment xml:lang="en">LanguaL curation note: Index consumer lifestage (child, any age) and label claims (diet/lite) in facet P. Index main ingredient in facet B. Index added ingredients (fruit, flavouring) in facet H.</rdfs:comment>
	<oboInOwl:hasDbXref>LANGUAL:A0921</oboInOwl:hasDbXref>
</owl:Class>

<owl:Class rdf:about="&obo;FOODON_03400922">
	<rdfs:label xml:lang="en">10000594 - non alcoholic beverages variety packs - ready to drink (gs1 gpc)</rdfs:label>
	<rdfs:subClassOf rdf:resource="&obo;FOODON_03400912"/>
	<obo:IAO_0000412>http://langual.org</obo:IAO_0000412>
	<obo:IAO_0000115 xml:lang="en">Includes any products that can be described/observed as two or more distinct Non Alcoholic Beverages Ready to Drink sold together, which exist within the schema belonging to different bricks but to the same class, that is two or more products contained within the same pack which cross bricks within the Non Alcoholic Beverages - Ready to Drink class. Includes products such as ready to drink Cola and Ice sold together. Items that are received free with purchases should be removed from the classification decision-making process. Excludes products such as ready to drink Cola and Crisps variety packs.</obo:IAO_0000115>
	<obo:IAO_0000114 rdf:resource="&obo;IAO_0000428"/>
	<oboInOwl:hasDbXref>LANGUAL:A0922</oboInOwl:hasDbXref>
</owl:Class>

<owl:Class rdf:about="&obo;FOODON_03400923">
	<rdfs:label xml:lang="en">10000232 - packaged water (gs1 gpc)</rdfs:label>
	<rdfs:subClassOf rdf:resource="&obo;FOODON_03400912"/>
	<obo:IAO_0000412>http://langual.org</obo:IAO_0000412>
	<obo:IAO_0000115 xml:lang="en">Includes any products that can be described/observed as water that has been specifically packaged for human consumption, and which may contain additional minerals or other trace elements including a natural or artificial source of carbon dioxide. Includes slightly flavoured products that are labelled and marketed as water and all mineral waters originating from both natural and drilled sources. These mineral waters are characterized by a guaranteed content of certain mineral salts and original microbiological purity. Also includes waters with added calcium. Specifically excludes products that contain sugars or sweeteners. Excludes products such as Tonic Water and Juice Drinks.</obo:IAO_0000115>
	<obo:IAO_0000114 rdf:resource="&obo;IAO_0000428"/>
	<rdfs:comment xml:lang="en">LanguaL curation note: If flavouring or carvonation added, index in facet H.</rdfs:comment>
	<oboInOwl:hasDbXref>LANGUAL:A0923</oboInOwl:hasDbXref>
</owl:Class>

<owl:Class rdf:about="&obo;FOODON_03400924">
	<rdfs:label xml:lang="en">10000265 - sports drinks - rehydration (ready to drink) (gs1 gpc)</rdfs:label>
	<rdfs:subClassOf rdf:resource="&obo;FOODON_03400912"/>
	<obo:IAO_0000412>http://langual.org</obo:IAO_0000412>
	<obo:IAO_0000115 xml:lang="en">Includes any products that can be described/observed as a ready to drink, liquid beverage which contains carbohydrates and electrolytes, designed to accelerate the re-hydration of cells by osmosis, normally consumed after a sporting activity. Includes products of various flavours such as orange and lemon. Excludes products such as Sports - Rehydration Drinks - Not Ready to Drink and all Stimulants/Energy Drinks.</obo:IAO_0000115>
	<obo:IAO_0000114 rdf:resource="&obo;IAO_0000428"/>
	<rdfs:comment xml:lang="en">LanguaL curation note: Index in facet H if it has been made effervescent by the addition of carbon dioxide gas. Index cafeine and diet claims in facet P.</rdfs:comment>
	<oboInOwl:hasDbXref>LANGUAL:A0924</oboInOwl:hasDbXref>
</owl:Class>

<owl:Class rdf:about="&obo;FOODON_03400925">
	<rdfs:label xml:lang="en">10000266 - stimulants/energy drinks - ready to drink (gs1 gpc)</rdfs:label>
	<rdfs:subClassOf rdf:resource="&obo;FOODON_03400912"/>
	<obo:IAO_0000412>http://langual.org</obo:IAO_0000412>
	<obo:IAO_0000115 xml:lang="en">Includes any products that can be described/observed as a ready to drink beverage containing glucose, caffeine or other stimulant designed to give the consumer a short-term boost of energy. Products are available in a variety of flavours. Specifically excludes flavoured drinks that contain caffeine (such as Cola) but are not labelled and marketed with energy enhancing properties. Excludes products such as Stimulants/Energy Drinks - Not Ready to Drink and all Rehydration Sport Drinks.</obo:IAO_0000115>
	<obo:IAO_0000114 rdf:resource="&obo;IAO_0000428"/>
	<rdfs:comment xml:lang="en">LanguaL curation note: Index in facet H if it has been made effervescent by the addition of carbon dioxide gas. Index cafeine and diet claims in facet P.</rdfs:comment>
	<oboInOwl:hasDbXref>LANGUAL:A0925</oboInOwl:hasDbXref>
</owl:Class>

<owl:Class rdf:about="&obo;FOODON_03400926">
	<rdfs:label xml:lang="en">50202500 - beverages variety packs (gs1 gpc)</rdfs:label>
	<rdfs:subClassOf rdf:resource="&obo;FOODON_03400875"/>
	<obo:IAO_0000412>http://langual.org</obo:IAO_0000412>
	<obo:IAO_0000115 xml:lang="en">Includes any products that can be described/observed as two or more distinct Beverages sold together which exist within the schema but belong to different classes, that is two or more products contained within the same pack which cross classes within the Beverages Family. Includes products such as Gin with Tonic Water variety packs.  Excludes products such as Still and Sparkling Wine variety packs and Wine and Chocolate variety packs.</obo:IAO_0000115>
	<obo:IAO_0000114 rdf:resource="&obo;IAO_0000428"/>
	<oboInOwl:hasDbXref>LANGUAL:A0926</oboInOwl:hasDbXref>
</owl:Class>

<owl:Class rdf:about="&obo;FOODON_03400927">
	<rdfs:label xml:lang="en">50180000 - bread/bakery products (gs1 gpc)</rdfs:label>
	<rdfs:subClassOf rdf:resource="&obo;FOODON_03400874"/>
	<obo:IAO_0000412>http://langual.org</obo:IAO_0000412>
	<obo:IAO_0000114 rdf:resource="&obo;IAO_0000428"/>
	<oboInOwl:hasDbXref>LANGUAL:A0927</oboInOwl:hasDbXref>
</owl:Class>

<owl:Class rdf:about="&obo;FOODON_03400928">
	<rdfs:label xml:lang="en">50181700 - baking/cooking mixes/supplies (gs1 gpc)</rdfs:label>
	<rdfs:subClassOf rdf:resource="&obo;FOODON_03400927"/>
	<obo:IAO_0000412>http://langual.org</obo:IAO_0000412>
	<obo:IAO_0000114 rdf:resource="&obo;IAO_0000428"/>
	<oboInOwl:hasDbXref>LANGUAL:A0928</oboInOwl:hasDbXref>
</owl:Class>

<owl:Class rdf:about="&obo;FOODON_03400929">
	<rdfs:label xml:lang="en">10000155 - baking/cooking mixes (frozen) (gs1 gpc)</rdfs:label>
	<rdfs:subClassOf rdf:resource="&obo;FOODON_03400928"/>
	<obo:IAO_0000412>http://langual.org</obo:IAO_0000412>
	<obo:IAO_0000115 xml:lang="en">Includes any products that can be described/observed as a quantity of frozen, pre-mixed dough, batter or powder that is specifically intended to produce bread, cakes, biscuits, desserts, or other products. Products may be ready to use (where no additional ingredients need to be added to the mix prior to use) or require the addition of wet ingredients such as water, milk, oil, fat or egg. These products must be frozen to extend their consumable life. Excludes products such as Perishable or Shelf-Stable Baking Mixes, all Part Baked and Baked Products.</obo:IAO_0000115>
	<obo:IAO_0000114 rdf:resource="&obo;IAO_0000428"/>
	<rdfs:comment xml:lang="en">LanguaL curation note: Index use (diabetic, vegetarian/vegan), diet and organic claims in facet P.</rdfs:comment>
	<oboInOwl:hasDbXref>LANGUAL:A0929</oboInOwl:hasDbXref>
</owl:Class>

<owl:Class rdf:about="&obo;FOODON_03400930">
	<rdfs:label xml:lang="en">10000068 - baking/cooking mixes (perishable) (gs1 gpc)</rdfs:label>
	<rdfs:subClassOf rdf:resource="&obo;FOODON_03400928"/>
	<obo:IAO_0000412>http://langual.org</obo:IAO_0000412>
	<obo:IAO_0000115 xml:lang="en">Includes any products that can be described/observed as a quantity of perishable, pre-mixed dough, batter or powder or other ingredients that is specifically intended to produce bread, cakes, biscuits, desserts, or other products. Products may be ready to use (where no additional ingredients need to be added to the mix prior to use) or require the addition of wet ingredients such as water, milk, oil, fat or egg. These products must be refrigerated to extend their consumable life. Excludes products such as Frozen or Shelf-Stable Baking Mixes, all Part Baked and Baked Products.</obo:IAO_0000115>
	<obo:IAO_0000114 rdf:resource="&obo;IAO_0000428"/>
	<rdfs:comment xml:lang="en">LanguaL curation note: Index use (diabetic, vegetarian/vegan), diet and organic claims in facet P.</rdfs:comment>
	<oboInOwl:hasDbXref>LANGUAL:A0930</oboInOwl:hasDbXref>
</owl:Class>

<owl:Class rdf:about="&obo;FOODON_03400931">
	<rdfs:label xml:lang="en">10000156 - baking/cooking mixes (shelf stable) (gs1 gpc)</rdfs:label>
	<rdfs:subClassOf rdf:resource="&obo;FOODON_03400928"/>
	<obo:IAO_0000412>http://langual.org</obo:IAO_0000412>
	<obo:IAO_0000115 xml:lang="en">Includes any products that can be described/observed as a quantity of shelf-stable, pre-mixed dough, batter or powder that is specifically intended to produce bread, cakes, biscuits, desserts, or other products. Products may be ready to use (where no additional ingredients need to be added to the mix prior to use) or require the addition of wet ingredients such as water, milk, oil, fat or egg. These products have been treated or packaged in such a way as to extend their consumable life. Excludes products such as Frozen or Perishable Baking Mixes, all Part Baked and Baked Products.</obo:IAO_0000115>
	<obo:IAO_0000114 rdf:resource="&obo;IAO_0000428"/>
	<rdfs:comment xml:lang="en">LanguaL curation note: Index use (diabetic, vegetarian/vegan), diet and organic claims in facet P.</rdfs:comment>
	<oboInOwl:hasDbXref>LANGUAL:A0931</oboInOwl:hasDbXref>
</owl:Class>

<owl:Class rdf:about="&obo;FOODON_03400932">
	<rdfs:label xml:lang="en">10000595 - baking/cooking mixes/supplies variety packs (gs1 gpc)</rdfs:label>
	<rdfs:subClassOf rdf:resource="&obo;FOODON_03400928"/>
	<obo:IAO_0000412>http://langual.org</obo:IAO_0000412>
	<obo:IAO_0000115 xml:lang="en">Includes any products that can be described/observed as two or more distinct Baking/Cooking Mixes and Supplies sold together, which exist within the schema belonging to different bricks but to the same class, that is two or more products contained within the same pack which cross bricks within the Baking/Cooking Mixes and Supplies class. Includes products such as cake mixes with edible decorations sold together. Items that are received free with purchases should be removed from the classification decision-making process. Excludes products such as Cake Mixes with Ground Coffee variety packs.</obo:IAO_0000115>
	<obo:IAO_0000114 rdf:resource="&obo;IAO_0000428"/>
	<oboInOwl:hasDbXref>LANGUAL:A0932</oboInOwl:hasDbXref>
</owl:Class>

<owl:Class rdf:about="&obo;FOODON_03400933">
	<rdfs:label xml:lang="en">10000157 - baking/cooking supplies (frozen) (gs1 gpc)</rdfs:label>
	<rdfs:subClassOf rdf:resource="&obo;FOODON_03400928"/>
	<obo:IAO_0000412>http://langual.org</obo:IAO_0000412>
	<obo:IAO_0000115 xml:lang="en">Includes any products that can be described/observed as items specifically designed to be used when baking or cooking. Products include yeast, breadcrumbs and part meal kits. They may/may not require the addition of other ingredients, and may/may not need further baking or cooking. These products must be frozen to extend their consumable life. Excludes products such as Perishable and Shelf-Stable Baking Supplies, Flour, Butter, Margarine, Lard, Sugar, Dried Fruit, Nuts.</obo:IAO_0000115>
	<obo:IAO_0000114 rdf:resource="&obo;IAO_0000428"/>
	<rdfs:comment xml:lang="en">LanguaL curation note: Index use (vegetarian/vegan) claim in facet P.</rdfs:comment>
	<oboInOwl:hasDbXref>LANGUAL:A0933</oboInOwl:hasDbXref>
</owl:Class>

<owl:Class rdf:about="&obo;FOODON_03400934">
	<rdfs:label xml:lang="en">10000069 - baking/cooking supplies (perishable) (gs1 gpc)</rdfs:label>
	<rdfs:subClassOf rdf:resource="&obo;FOODON_03400928"/>
	<obo:IAO_0000412>http://langual.org</obo:IAO_0000412>
	<obo:IAO_0000115 xml:lang="en">Includes any products that can be described/observed as items specifically designed to be used when baking or cooking. Products include yeast and part meal kits. They may/may not require the addition of other ingredients, and may/may not need further baking or cooking. These products can be/must be refrigerated to extend their consumable life. Excludes products such as Shelf Stable and Frozen Baking Supplies, Butter, Margarine, Lard, Sugar, Dried Fruit, Nuts.</obo:IAO_0000115>
	<obo:IAO_0000114 rdf:resource="&obo;IAO_0000428"/>
	<rdfs:comment xml:lang="en">LanguaL curation note: Index use (vegetarian/vegan) claim in facet P.</rdfs:comment>
	<oboInOwl:hasDbXref>LANGUAL:A0934</oboInOwl:hasDbXref>
</owl:Class>

<owl:Class rdf:about="&obo;FOODON_03400935">
	<rdfs:label xml:lang="en">10000158 - baking/cooking supplies (shelf stable) (gs1 gpc)</rdfs:label>
	<rdfs:subClassOf rdf:resource="&obo;FOODON_03400928"/>
	<obo:IAO_0000412>http://langual.org</obo:IAO_0000412>
	<obo:IAO_0000115 xml:lang="en">Includes any products that can be described/observed as items specifically designed to be used when baking or cooking. Products include cornflour, yeast, baking powder, cooking chocolate and confectionary style beverage toppings. Also includes Host, which forms a thin pastry intended to be used for layers of a cake, in between which different sorts of fillings are layered. These products have been treated or packaged in such a way as to extend their consumable life. Excludes products such as Perishable and Frozen Baking Supplies, Butter, Margarine, Lard, Sugar, Dried Fruit and Nuts.</obo:IAO_0000115>
	<obo:IAO_0000114 rdf:resource="&obo;IAO_0000428"/>
	<rdfs:comment xml:lang="en">LanguaL curation note: Index use (vegetarian/vegan) claim in facet P. Index main ingredient (almond, sodium bicarbonate) in facet B.</rdfs:comment>
	<oboInOwl:hasDbXref>LANGUAL:A0935</oboInOwl:hasDbXref>
</owl:Class>

<owl:Class rdf:about="&obo;FOODON_03400936">
	<rdfs:label xml:lang="en">50182100 - biscuits/cookies (gs1 gpc)</rdfs:label>
	<rdfs:subClassOf rdf:resource="&obo;FOODON_03400927"/>
	<obo:IAO_0000412>http://langual.org</obo:IAO_0000412>
	<obo:IAO_0000114 rdf:resource="&obo;IAO_0000428"/>
	<oboInOwl:hasDbXref>LANGUAL:A0936</oboInOwl:hasDbXref>
</owl:Class>

<owl:Class rdf:about="&obo;FOODON_03400937">
	<rdfs:label xml:lang="en">10000304 - biscuits/cookies (frozen) (gs1 gpc)</rdfs:label>
	<rdfs:subClassOf rdf:resource="&obo;FOODON_03400936"/>
	<obo:IAO_0000412>http://langual.org</obo:IAO_0000412>
	<obo:IAO_0000115 xml:lang="en">Includes any products that can be described/observed as a thin, unleavened, baked, cereal-based product. Products may be sweet or savoury and are available in a variety of shapes and sizes. These products must be frozen to extend their consumable life. Includes products such as crackers, cookies, oatcakes. Excludes products such as Perishable and Shelf Stable Biscuits and Cookies and all Dried Breads.</obo:IAO_0000115>
	<obo:IAO_0000114 rdf:resource="&obo;IAO_0000428"/>
	<rdfs:comment xml:lang="en">LanguaL curation note: Index use (diabetic) and fat level claims in facet P. Index Type of Cereal/Grain in facet B. Index added ingredients (sugar, chocolate) and filling/coating in facet H.</rdfs:comment>
	<oboInOwl:hasDbXref>LANGUAL:A0937</oboInOwl:hasDbXref>
</owl:Class>

<owl:Class rdf:about="&obo;FOODON_03400938">
	<rdfs:label xml:lang="en">10000160 - biscuits/cookies (perishable) (gs1 gpc)</rdfs:label>
	<rdfs:subClassOf rdf:resource="&obo;FOODON_03400936"/>
	<obo:IAO_0000412>http://langual.org</obo:IAO_0000412>
	<obo:IAO_0000115 xml:lang="en">Includes any products that can be described/observed as a thin, unleavened, baked, cereal-based product. Products may be sweet or savoury and are available in a variety of shapes and sizes These products can be refrigerated to extend their consumable life. Includes products such as crackers, cookies, oatcakes. Excludes products such as Frozen and Shelf-Stable Biscuits and Cookies, all Dried Breads.</obo:IAO_0000115>
	<obo:IAO_0000114 rdf:resource="&obo;IAO_0000428"/>
	<rdfs:comment xml:lang="en">LanguaL curation note: Index use (diabetic) and fat level claims in facet P. Index Type of Cereal/Grain in facet B. Index added ingredients (sugar, chocolate) and filling/coating in facet H.</rdfs:comment>
	<oboInOwl:hasDbXref>LANGUAL:A0938</oboInOwl:hasDbXref>
</owl:Class>

<owl:Class rdf:about="&obo;FOODON_03400939">
	<rdfs:label xml:lang="en">10000161 - biscuits/cookies (shelf stable) (gs1 gpc)</rdfs:label>
	<rdfs:subClassOf rdf:resource="&obo;FOODON_03400936"/>
	<obo:IAO_0000412>http://langual.org</obo:IAO_0000412>
	<obo:IAO_0000115 xml:lang="en">Includes any products that can be described/observed as a thin, unleavened, baked, cereal-based product. Products may be sweet or savoury and are available in a variety of shapes and sizes. These products have been treated or packaged in such a way as to extend their consumable life. Includes products such as crackers, cookies, oatcakes. Excludes products such as Frozen and Perishable Biscuits and Cookies, all Dried Breads.</obo:IAO_0000115>
	<obo:IAO_0000114 rdf:resource="&obo;IAO_0000428"/>
	<rdfs:comment xml:lang="en">LanguaL curation note: Index use (diabetic) and fat level claims in facet P. Index Type of Cereal/Grain in facet B. Index added ingredients (sugar, chocolate) and filling/coating in facet H.</rdfs:comment>
	<oboInOwl:hasDbXref>LANGUAL:A0939</oboInOwl:hasDbXref>
</owl:Class>

<owl:Class rdf:about="&obo;FOODON_03400940">
	<rdfs:label xml:lang="en">10000596 - biscuits/cookies variety packs (gs1 gpc)</rdfs:label>
	<rdfs:subClassOf rdf:resource="&obo;FOODON_03400936"/>
	<obo:IAO_0000412>http://langual.org</obo:IAO_0000412>
	<obo:IAO_0000115 xml:lang="en">Includes any products that can be described/observed as two or more distinct Biscuits, Cookies or Dried Breads sold together, which exist within the schema belonging to different bricks but to the same class, that is two or more products contained within the same pack which cross bricks within the Biscuits and Cookies class. Includes products such as Cookies and Breadsticks sold together. Items that are received free with purchases should be removed from the classification decision-making process. Excludes products such as Cookies and Chocolate variety packs.</obo:IAO_0000115>
	<obo:IAO_0000114 rdf:resource="&obo;IAO_0000428"/>
	<oboInOwl:hasDbXref>LANGUAL:A0940</oboInOwl:hasDbXref>
</owl:Class>

<owl:Class rdf:about="&obo;FOODON_03400941">
	<rdfs:label xml:lang="en">10000305 - dried breads (frozen) (gs1 gpc)</rdfs:label>
	<rdfs:subClassOf rdf:resource="&obo;FOODON_03400936"/>
	<obo:IAO_0000412>http://langual.org</obo:IAO_0000412>
	<obo:IAO_0000115 xml:lang="en">Includes any products that can be described/observed as a leavened or unleavened, flour-based baked, fried, dried or extruded product, typically designed to be used as an ingredient or accompaniment in another dish. These products must be frozen to extend their consumable life. Includes such products as Breadsticks, Tortillas and Croutons. Excludes products such as Shelf Stable Dried Breads, Biscuits, all types of Shelf Stable Baking Mixes and Baking Supplies, Sweet Products, Crackers and Oatcakes.</obo:IAO_0000115>
	<obo:IAO_0000114 rdf:resource="&obo;IAO_0000428"/>
	<rdfs:comment xml:lang="en">LanguaL curation note: Index fat level or organic claims in facet P.</rdfs:comment>
	<oboInOwl:hasDbXref>LANGUAL:A0941</oboInOwl:hasDbXref>
</owl:Class>

<owl:Class rdf:about="&obo;FOODON_03400942">
	<rdfs:label xml:lang="en">10000166 - dried breads (shelf stable) (gs1 gpc)</rdfs:label>
	<rdfs:subClassOf rdf:resource="&obo;FOODON_03400936"/>
	<obo:IAO_0000412>http://langual.org</obo:IAO_0000412>
	<obo:IAO_0000115 xml:lang="en">Includes any products that can be described/observed as a leavened or unleavened, flour-based baked, fried, dried or extruded product, typically designed to be used as an ingredient or accompaniment in another dish. These products have been treated or packaged in such a way as to extend their consumable life. Includes such products as Breadsticks, Croutons and Crispbreads. Excludes products such as Frozen Dried Breads, all types of Shelf Stable Baking Mixes and Baking Supplies, Sweet Products, Crackers and Oatcakes.</obo:IAO_0000115>
	<obo:IAO_0000114 rdf:resource="&obo;IAO_0000428"/>
	<rdfs:comment xml:lang="en">LanguaL curation note: Index fat level or organic claims in facet P.</rdfs:comment>
	<oboInOwl:hasDbXref>LANGUAL:A0942</oboInOwl:hasDbXref>
</owl:Class>

<owl:Class rdf:about="&obo;FOODON_03400943">
	<rdfs:label xml:lang="en">50181900 - bread (gs1 gpc)</rdfs:label>
	<rdfs:subClassOf rdf:resource="&obo;FOODON_03400927"/>
	<obo:IAO_0000412>http://langual.org</obo:IAO_0000412>
	<obo:IAO_0000114 rdf:resource="&obo;IAO_0000428"/>
	<oboInOwl:hasDbXref>LANGUAL:A0943</oboInOwl:hasDbXref>
</owl:Class>

<owl:Class rdf:about="&obo;FOODON_03400944">
	<rdfs:label xml:lang="en">10000163 - bread (frozen) (gs1 gpc)</rdfs:label>
	<rdfs:subClassOf rdf:resource="&obo;FOODON_03400943"/>
	<obo:IAO_0000412>http://langual.org</obo:IAO_0000412>
	<obo:IAO_0000115 xml:lang="en">Includes any products that can be described/observed as a leavened or unleavened, dough-based baked product. These products do not typically contain eggs and tend to have lower fat content than other dough products such as pastry. These products must be frozen to extend their consumable life. Includes such products as naan, chapatti, loaves, rolls, bagels, focaccia, ciabatta, baguette. Also includes rye bread, bread made from rice flour and part baked bread products. Excludes products such as Shelf-Stable and Perishable Bread Products, Dried Breads, Frozen Baking Mixes and Baking Supplies, and Pies and Pastries.</obo:IAO_0000115>
	<obo:IAO_0000114 rdf:resource="&obo;IAO_0000428"/>
	<rdfs:comment xml:lang="en">LanguaL curation note: Index use (gluten free), fat level or organic claims in facet P. Index Type of Cereal/Grain in facet B. Index added flavours or ingredients in facet H. If partly baked/heat treated, index in facet F.</rdfs:comment>
	<oboInOwl:hasDbXref>LANGUAL:A0944</oboInOwl:hasDbXref>
</owl:Class>

<owl:Class rdf:about="&obo;FOODON_03400945">
	<rdfs:label xml:lang="en">10000164 - bread (perishable) (gs1 gpc)</rdfs:label>
	<rdfs:subClassOf rdf:resource="&obo;FOODON_03400943"/>
	<obo:IAO_0000412>http://langual.org</obo:IAO_0000412>
	<obo:IAO_0000115 xml:lang="en">Includes any products that can be described/observed as a leavened or unleavened, dough-based baked product. These products do not typically contain eggs and tend to have lower fat content than other dough products such as pastry. These products can be refrigerated to extend their consumable life. Includes such products as naan, chapatti, loaves, rolls, bagels, focaccia, ciabatta, baguette. Also includes rye bread, bread made from rice flour and part baked bread products. Excludes products such as Shelf-Stable and Frozen Bread Products, Dried Breads, Perishable Baking Mixes and Baking Supplies, and Pies and Pastries.</obo:IAO_0000115>
	<obo:IAO_0000114 rdf:resource="&obo;IAO_0000428"/>
	<rdfs:comment xml:lang="en">LanguaL curation note: Index use (gluten free), fat level or organic claims in facet P. Index Type of Cereal/Grain in facet B. Index added flavours or ingredients in facet H. If partly baked/heat treated, index in facet F.</rdfs:comment>
	<oboInOwl:hasDbXref>LANGUAL:A0945</oboInOwl:hasDbXref>
</owl:Class>

<owl:Class rdf:about="&obo;FOODON_03400946">
	<rdfs:label xml:lang="en">10000165 - bread (shelf stable) (gs1 gpc)</rdfs:label>
	<rdfs:subClassOf rdf:resource="&obo;FOODON_03400943"/>
	<obo:IAO_0000412>http://langual.org</obo:IAO_0000412>
	<obo:IAO_0000115 xml:lang="en">Includes any products that can be described/observed as a leavened or unleavened, dough-based baked product. These products do not typically contain eggs and tend to have lower fat content than other dough products such as pastry. These products have been treated or packaged in such a way as to extend their consumable life. Includes such products as naan, chapatti, loaves, rolls, bagels, focaccia, ciabatta, baguette. Also includes rye bread, bread made from rice flour and part baked bread products. Excludes products such as Frozen and Perishable Bread Products, Dried Breads, Shelf-Stable Baking Mixes and Baking Supplies, and Pies and Pastries.</obo:IAO_0000115>
	<obo:IAO_0000114 rdf:resource="&obo;IAO_0000428"/>
	<rdfs:comment xml:lang="en">LanguaL curation note: Index use (gluten free), fat level or organic claims in facet P. Index Type of Cereal/Grain in facet B. Index added flavours or ingredients in facet H.</rdfs:comment>
	<oboInOwl:hasDbXref>LANGUAL:A0946</oboInOwl:hasDbXref>
</owl:Class>

<owl:Class rdf:about="&obo;FOODON_03400947">
	<rdfs:label xml:lang="en">50182200 - savoury bakery products (gs1 gpc)</rdfs:label>
	<rdfs:subClassOf rdf:resource="&obo;FOODON_03400927"/>
	<obo:IAO_0000412>http://langual.org</obo:IAO_0000412>
	<obo:IAO_0000114 rdf:resource="&obo;IAO_0000428"/>
	<oboInOwl:hasDbXref>LANGUAL:A0947</oboInOwl:hasDbXref>
</owl:Class>

<owl:Class rdf:about="&obo;FOODON_03400948">
	<rdfs:label xml:lang="en">10000248 - pies/pastries/pizzas/quiches - savoury (frozen) (gs1 gpc)</rdfs:label>
	<rdfs:subClassOf rdf:resource="&obo;FOODON_03400947"/>
	<obo:IAO_0000412>http://langual.org</obo:IAO_0000412>
	<obo:IAO_0000115 xml:lang="en">Includes any products that can be described/observed as a pastry based product consisting of a butter, egg and flour dough. Products may use shortcrust, puff, filo or flaky pastry and be filled or topped with a combination or mixture of shredded/sliced savoury ingredients, commonly including meat, vegetables, eggs or other additives, then baked, and sold ready for immediate consumption. Products specifically include Pizza. Products must be frozen to extend their consumable life. Excludes products such as Perishable and Shelf Stable Savoury Pies, Pastries, Pizzas and Quiches, Sweet Pies/Tarts, and Potato Topped Meat Pies.</obo:IAO_0000115>
	<obo:IAO_0000114 rdf:resource="&obo;IAO_0000428"/>
	<rdfs:comment xml:lang="en">LanguaL curation note: Index added ingredients (dairy, meat) in facet H. Index use (Vegetarians/Vegans), fat level or organic claims in facet P.</rdfs:comment>
	<oboInOwl:hasDbXref>LANGUAL:A0948</oboInOwl:hasDbXref>
</owl:Class>

<owl:Class rdf:about="&obo;FOODON_03400949">
	<rdfs:label xml:lang="en">10000249 - pies/pastries/pizzas/quiches - savoury (perishable) (gs1 gpc)</rdfs:label>
	<rdfs:subClassOf rdf:resource="&obo;FOODON_03400947"/>
	<obo:IAO_0000412>http://langual.org</obo:IAO_0000412>
	<obo:IAO_0000115 xml:lang="en">Includes any products that can be described/observed as a pastry based product consisting of a butter, egg and flour dough. Products may use shortcrust, puff, filo or flaky pastry and be filled or topped with a combination or mixture of shredded/sliced savoury ingredients, commonly including meat, vegetables, eggs or other additives, then baked, and sold ready for immediate consumption. Specifically includes Pizza. Products must be refrigerated to extend their consumable life. Excludes products such as Frozen and Shelf Stable Savoury Pies, Pastries, Pizzas and Quiches, Sweet Pies/Tarts, and Potato Topped Meat Pies.</obo:IAO_0000115>
	<obo:IAO_0000114 rdf:resource="&obo;IAO_0000428"/>
	<rdfs:comment xml:lang="en">LanguaL curation note: Index added ingredients (dairy, meat) in facet H. Index use (Vegetarians/Vegans), fat level or organic claims in facet P.</rdfs:comment>
	<oboInOwl:hasDbXref>LANGUAL:A0949</oboInOwl:hasDbXref>
</owl:Class>

<owl:Class rdf:about="&obo;FOODON_03400950">
	<rdfs:label xml:lang="en">10000250 - pies/pastries/pizzas/quiches - savoury (shelf stable) (gs1 gpc)</rdfs:label>
	<rdfs:subClassOf rdf:resource="&obo;FOODON_03400947"/>
	<obo:IAO_0000412>http://langual.org</obo:IAO_0000412>
	<obo:IAO_0000115 xml:lang="en">Includes any products that can be described/observed as a pastry based product consisting of a butter, egg and flour dough. Products may use shortcrust, puff, filo or flaky pastry and be filled or topped with a combination or mixture of shredded/sliced savoury ingredients, commonly including meat, vegetables, eggs or other additives, then baked, and sold ready for immediate consumption. Products specifically include pizza. These products have been treated or packaged in such a way as to extend their consumable life. Excludes products such as Perishable and Frozen Savoury Pies, Pastries, Pizzas and Quiches, Sweet Pies/Tarts, and Potato Topped Meat Pies.</obo:IAO_0000115>
	<obo:IAO_0000114 rdf:resource="&obo;IAO_0000428"/>
	<rdfs:comment xml:lang="en">LanguaL curation note: Index added ingredients (dairy, meat) in facet H. Index use (Vegetarians/Vegans), fat level or organic claims in facet P.</rdfs:comment>
	<oboInOwl:hasDbXref>LANGUAL:A0950</oboInOwl:hasDbXref>
</owl:Class>

<owl:Class rdf:about="&obo;FOODON_03400951">
	<rdfs:label xml:lang="en">50182000 - sweet bakery products (gs1 gpc)</rdfs:label>
	<rdfs:subClassOf rdf:resource="&obo;FOODON_03400927"/>
	<obo:IAO_0000412>http://langual.org</obo:IAO_0000412>
	<obo:IAO_0000114 rdf:resource="&obo;IAO_0000428"/>
	<oboInOwl:hasDbXref>LANGUAL:A0951</oboInOwl:hasDbXref>
</owl:Class>

<owl:Class rdf:about="&obo;FOODON_03400952">
	<rdfs:label xml:lang="en">10000170 - cakes - sweet (frozen) (gs1 gpc)</rdfs:label>
	<rdfs:subClassOf rdf:resource="&obo;FOODON_03400951"/>
	<obo:IAO_0000412>http://langual.org</obo:IAO_0000412>
	<obo:IAO_0000115 xml:lang="en">Includes any products that can be described/observed as a sweet prepared food, usually made from flour, sugar, shortening/fat and eggs mixed with other ingredients and baked or fried. These products must be frozen to extend their consumable life. Excludes products such as Perishable and Shelf Stable Cakes, Cake Mixes, all Bread Products.</obo:IAO_0000115>
	<obo:IAO_0000114 rdf:resource="&obo;IAO_0000428"/>
	<rdfs:comment xml:lang="en">LanguaL curation note: Index coating, added flavours or ingredients in facet H. Index fat level or organic claims in facet P.</rdfs:comment>
	<oboInOwl:hasDbXref>LANGUAL:A0952</oboInOwl:hasDbXref>
</owl:Class>

<owl:Class rdf:about="&obo;FOODON_03400953">
	<rdfs:label xml:lang="en">10000171 - cakes - sweet (perishable) (gs1 gpc)</rdfs:label>
	<rdfs:subClassOf rdf:resource="&obo;FOODON_03400951"/>
	<obo:IAO_0000412>http://langual.org</obo:IAO_0000412>
	<obo:IAO_0000115 xml:lang="en">Includes any products that can be described/observed as a sweet prepared food, usually made from flour, sugar, shortening/fat and eggs mixed with other ingredients and baked or fried. These products can be/must be refrigerated to extend their consumable life. Excludes products such as Frozen and Shelf Stable Cakes, Cake Mixes, all Bread Products.</obo:IAO_0000115>
	<obo:IAO_0000114 rdf:resource="&obo;IAO_0000428"/>
	<rdfs:comment xml:lang="en">LanguaL curation note: Index coating, added flavours or ingredients in facet H. Index fat level or organic claims in facet P.</rdfs:comment>
	<oboInOwl:hasDbXref>LANGUAL:A0953</oboInOwl:hasDbXref>
</owl:Class>

<owl:Class rdf:about="&obo;FOODON_03400954">
	<rdfs:label xml:lang="en">10000172 - cakes - sweet (shelf stable) (gs1 gpc)</rdfs:label>
	<rdfs:subClassOf rdf:resource="&obo;FOODON_03400951"/>
	<obo:IAO_0000412>http://langual.org</obo:IAO_0000412>
	<obo:IAO_0000115 xml:lang="en">Includes any products that can be described/observed as a sweet prepared food, usually made from flour, sugar, shortening/fat and eggs mixed with other ingredients and baked or fried. These products have been treated or packaged in such a way as to extend their consumable life. Excludes products such as Perishable and Frozen Cakes, Cake Mixes, all Bread Products.</obo:IAO_0000115>
	<obo:IAO_0000114 rdf:resource="&obo;IAO_0000428"/>
	<rdfs:comment xml:lang="en">LanguaL curation note: Index coating, added flavours or ingredients in facet H. Index fat level or organic claims in facet P.</rdfs:comment>
	<oboInOwl:hasDbXref>LANGUAL:A0954</oboInOwl:hasDbXref>
</owl:Class>

<owl:Class rdf:about="&obo;FOODON_03400955">
	<rdfs:label xml:lang="en">10000245 - pies/pastries - sweet (frozen) (gs1 gpc)</rdfs:label>
	<rdfs:subClassOf rdf:resource="&obo;FOODON_03400951"/>
	<obo:IAO_0000412>http://langual.org</obo:IAO_0000412>
	<obo:IAO_0000115 xml:lang="en">Includes any products that can be described/observed as a pastry based sweet product consisting of a butter, flour and egg dough. Products may use shortcrust, puff, filo or flaky pastry and must contain a filling. Generally, these products have a high fat content. Products must be frozen to extend their consumable life. Products include pies and tarts, croissants, Danish and other breakfast pastries. Excludes products such as Perishable and Shelf Stable Pies and Pastries, Savoury Pies, Pastries and Tarts, and Bread.</obo:IAO_0000115>
	<obo:IAO_0000114 rdf:resource="&obo;IAO_0000428"/>
	<rdfs:comment xml:lang="en">LanguaL curation note: Index added flavours or ingredients (chocolate, fruit) in facet H. Index use (diabetic, vegetarian/vegan), fat level or organic claims in facet P.</rdfs:comment>
	<oboInOwl:hasDbXref>LANGUAL:A0955</oboInOwl:hasDbXref>
</owl:Class>

<owl:Class rdf:about="&obo;FOODON_03400956">
	<rdfs:label xml:lang="en">10000246 - pies/pastries - sweet (perishable) (gs1 gpc)</rdfs:label>
	<rdfs:subClassOf rdf:resource="&obo;FOODON_03400951"/>
	<obo:IAO_0000412>http://langual.org</obo:IAO_0000412>
	<obo:IAO_0000115 xml:lang="en">Includes any products that can be described/observed as a pastry based sweet product consisting of a butter, flour and egg dough. Products may use shortcrust, puff, filo or flaky pastry and must contain a filling. Generally, these products have a high fat content. Products can be refrigerated to extend their consumable life. Products include pies and tarts, croissants, Danish and other breakfast pastries. Excludes products such as Frozen and Shelf Stable Pies and Pastries, Savoury Pies and Pastries.</obo:IAO_0000115>
	<obo:IAO_0000114 rdf:resource="&obo;IAO_0000428"/>
	<rdfs:comment xml:lang="en">LanguaL curation note: Index added flavours or ingredients (chocolate, fruit) in facet H. Index use (diabetic, vegetarian/vegan), fat level or organic claims in facet P.</rdfs:comment>
	<oboInOwl:hasDbXref>LANGUAL:A0956</oboInOwl:hasDbXref>
</owl:Class>

<owl:Class rdf:about="&obo;FOODON_03400957">
	<rdfs:label xml:lang="en">10000247 - pies/pastries - sweet (shelf stable) (gs1 gpc)</rdfs:label>
	<rdfs:subClassOf rdf:resource="&obo;FOODON_03400951"/>
	<obo:IAO_0000412>http://langual.org</obo:IAO_0000412>
	<obo:IAO_0000115 xml:lang="en">Includes any products that can be described/observed as a pastry based sweet product consisting of a butter, flour and egg dough. Products may use shortcrust, puff, filo or flaky pastry and must contain a filling. Generally, these products have a high fat content. These products have been treated or packaged in such a way as to extend their consumable life. Products include pies and tarts, croissants, Danish and other breakfast pastries. Excludes products such as Perishable and Frozen Pies and Pastries, Savoury Pies and Pastries.</obo:IAO_0000115>
	<obo:IAO_0000114 rdf:resource="&obo;IAO_0000428"/>
	<rdfs:comment xml:lang="en">LanguaL curation note: Index added flavours or ingredients (chocolate, fruit) in facet H. Index use (diabetic, vegetarian/vegan), fat level or organic claims in facet P.</rdfs:comment>
	<oboInOwl:hasDbXref>LANGUAL:A0957</oboInOwl:hasDbXref>
</owl:Class>

<owl:Class rdf:about="&obo;FOODON_03400958">
	<rdfs:label xml:lang="en">10000597 - sweet bakery products variety packs (gs1 gpc)</rdfs:label>
	<rdfs:subClassOf rdf:resource="&obo;FOODON_03400951"/>
	<obo:IAO_0000412>http://langual.org</obo:IAO_0000412>
	<obo:IAO_0000115 xml:lang="en">Includes any products that can be described/observed as two or more distinct sweet cakes, pies or pastries sold together, which exist within the schema belonging to different bricks but to the same class, that is two or more products contained within the same pack which cross bricks within the Sweet Bakery Products class. Includes products such as sponge cakes and danish pastries sold together. Items that are received free with purchases should be removed from the classification decision-making process. Excludes products such as Sponge Cakes and Ice Cream variety packs.</obo:IAO_0000115>
	<obo:IAO_0000114 rdf:resource="&obo;IAO_0000428"/>
	<oboInOwl:hasDbXref>LANGUAL:A0958</oboInOwl:hasDbXref>
</owl:Class>

<owl:Class rdf:about="&obo;FOODON_03400959">
	<rdfs:label xml:lang="en">50182300 - bread/bakery products variety packs (gs1 gpc)</rdfs:label>
	<rdfs:subClassOf rdf:resource="&obo;FOODON_03400927"/>
	<obo:IAO_0000412>http://langual.org</obo:IAO_0000412>
	<obo:IAO_0000115 xml:lang="en">Includes any products that can be described/observed as two or more distinct Bread and Bakery Products sold together which exist within the schema but belong to different classes, that is two or more products contained within the same pack which cross classes within the Bread and Bakery Products Family. Includes products such as Pizza with Garlic Bread variety packs. Items that are received free with purchases should be removed from the classification decision-making process. Excludes products such as Sponge Cakes and Danish Pastries variety packs and Breadsticks and Dips variety packs.</obo:IAO_0000115>
	<obo:IAO_0000114 rdf:resource="&obo;IAO_0000428"/>
	<oboInOwl:hasDbXref>LANGUAL:A0959</oboInOwl:hasDbXref>
</owl:Class>

<owl:Class rdf:about="&obo;FOODON_03400960">
	<rdfs:label xml:lang="en">50220000 - cereal/grain/pulse products (gs1 gpc)</rdfs:label>
	<rdfs:subClassOf rdf:resource="&obo;FOODON_03400874"/>
	<obo:IAO_0000412>http://langual.org</obo:IAO_0000412>
	<obo:IAO_0000114 rdf:resource="&obo;IAO_0000428"/>
	<oboInOwl:hasDbXref>LANGUAL:A0960</oboInOwl:hasDbXref>
</owl:Class>

<owl:Class rdf:about="&obo;FOODON_03400961">
	<rdfs:label xml:lang="en">50221000 - grains/flour (gs1 gpc)</rdfs:label>
	<rdfs:subClassOf rdf:resource="&obo;FOODON_03400960"/>
	<obo:IAO_0000412>http://langual.org</obo:IAO_0000412>
	<obo:IAO_0000114 rdf:resource="&obo;IAO_0000428"/>
	<oboInOwl:hasDbXref>LANGUAL:A0961</oboInOwl:hasDbXref>
</owl:Class>

<owl:Class rdf:about="&obo;FOODON_03400962">
	<rdfs:label xml:lang="en">10000203 - flour - cereal/pulse (shelf stable) (gs1 gpc)</rdfs:label>
	<rdfs:subClassOf rdf:resource="&obo;FOODON_03400961"/>
	<obo:IAO_0000412>http://langual.org</obo:IAO_0000412>
	<obo:IAO_0000115 xml:lang="en">Includes any products that can be described/observed as a fine powder derived from grains, roots or tubers. These products have been treated or packaged in such a way as to extend their consumable life. Specifically excludes products such as Cornflour. Excludes products such as Whole Grains, Bread and Baking Mixes.</obo:IAO_0000115>
	<obo:IAO_0000114 rdf:resource="&obo;IAO_0000428"/>
	<rdfs:comment xml:lang="en">LanguaL curation note: Index type of flour (wholdmeal, soy) in facet B. Index claims (organic, gluten free) in facet P. If the flour contains raising agent, index the added ingredient in facet H.</rdfs:comment>
	<oboInOwl:hasDbXref>LANGUAL:A0962</oboInOwl:hasDbXref>
</owl:Class>

<owl:Class rdf:about="&obo;FOODON_03400963">
	<rdfs:label xml:lang="en">10000314 - grains/cereal - not ready to eat - (frozen) (gs1 gpc)</rdfs:label>
	<rdfs:subClassOf rdf:resource="&obo;FOODON_03400961"/>
	<obo:IAO_0000412>http://langual.org</obo:IAO_0000412>
	<obo:IAO_0000115 xml:lang="en">Includes any products that can be described/observed as a savoury grain not ready to eat product, such as Rice, Polenta, Couscous. These products must not include any additional ingredients and are not part of a recipe prior to sale. These products are not ready to eat and require cooking prior to consumption. These products must be frozen to extend their consumable life. Specifically excludes all grain based prepared products such as Risotto and Cereal Products. Excludes products such as Perishable and Shelf Stable Not Ready to Eat and Ready to Eat Grain and all Grain Based Prepared Recipe Products.</obo:IAO_0000115>
	<obo:IAO_0000114 rdf:resource="&obo;IAO_0000428"/>
	<rdfs:comment xml:lang="en">LanguaL curation note: Index type of cereal/grain (barley, rice) in facet B.  If an industry recognized organic certification is claimed, index ORGANIC FOOD CLAIM OR USE in facet P.</rdfs:comment>
	<oboInOwl:hasDbXref>LANGUAL:A0963</oboInOwl:hasDbXref>
</owl:Class>

<owl:Class rdf:about="&obo;FOODON_03400964">
	<rdfs:label xml:lang="en">10000315 - grains/cereal - not ready to eat - (perishable) (gs1 gpc)</rdfs:label>
	<rdfs:subClassOf rdf:resource="&obo;FOODON_03400961"/>
	<obo:IAO_0000412>http://langual.org</obo:IAO_0000412>
	<obo:IAO_0000115 xml:lang="en">Includes any products that can be described/observed as a savoury grain not ready to eat product, such as Rice, Polenta, Couscous. These products must not include any additional ingredients and are not part of a recipe prior to sale. These products are not ready to eat and require cooking prior to consumption. These products must be refrigerated to extend their consumable life. Specifically excludes all grain based prepared products such as Risotto and Cereal Products. Excludes products such as Frozen and Shelf Stable Not Ready to Eat and Ready to Eat Grain and all Grain Based Prepared Recipe Products.</obo:IAO_0000115>
	<obo:IAO_0000114 rdf:resource="&obo;IAO_0000428"/>
	<rdfs:comment xml:lang="en">LanguaL curation note: Index type of cereal/grain (barley, rice) in facet B.  If an industry recognized organic certification is claimed, index ORGANIC FOOD CLAIM OR USE in facet P. Index preservation method (refrigeration) in facet J.</rdfs:comment>
	<oboInOwl:hasDbXref>LANGUAL:A0964</oboInOwl:hasDbXref>
</owl:Class>

<owl:Class rdf:about="&obo;FOODON_03400965">
	<rdfs:label xml:lang="en">10000211 - grains/cereal - not ready to eat - (shelf stable) (gs1 gpc)</rdfs:label>
	<rdfs:subClassOf rdf:resource="&obo;FOODON_03400961"/>
	<obo:IAO_0000412>http://langual.org</obo:IAO_0000412>
	<obo:IAO_0000115 xml:lang="en">Includes any products that can be described/observed as a savoury grain not ready to eat product, such as Rice, Polenta, Couscous. These products must not include any additional ingredients and are not part of a recipe prior to sale. These products are not ready to eat and require cooking prior to consumption. These products have been treated or packaged in such a way as to extend their consumable life. Specifically excludes all grain based prepared products such as Risotto and Cereal Products. Excludes products such as Perishable and Frozen Not Ready to Eat and Ready to Eat Grain and all Grain Based Prepared Recipe Products.</obo:IAO_0000115>
	<obo:IAO_0000114 rdf:resource="&obo;IAO_0000428"/>
	<rdfs:comment xml:lang="en">LanguaL curation note: Index type of cereal/grain (barley, rice) in facet B.  If an industry recognized organic certification is claimed, index ORGANIC FOOD CLAIM OR USE in facet P.</rdfs:comment>
	<oboInOwl:hasDbXref>LANGUAL:A0965</oboInOwl:hasDbXref>
</owl:Class>

<owl:Class rdf:about="&obo;FOODON_03400966">
	<rdfs:label xml:lang="en">10000316 - grains/cereal - ready to eat - (perishable) (gs1 gpc)</rdfs:label>
	<rdfs:subClassOf rdf:resource="&obo;FOODON_03400961"/>
	<obo:IAO_0000412>http://langual.org</obo:IAO_0000412>
	<obo:IAO_0000115 xml:lang="en">Includes any products that can be described/observed as a grain, ready to eat product, such as Rice, Polenta, Couscous. These products must not include any additional ingredients and are not part of a recipe prior to sale. These products do not require cooking prior to consumption, but some products can be reheated. These products must be refrigerated to extend their consumable life. Specifically excludes all grain based prepared products such as Rice Salad and Cereal Products. Excludes products such as Shelf Stable Ready to Eat and Not Ready to Eat Grain and all Grain Based Prepared Recipe Products.</obo:IAO_0000115>
	<obo:IAO_0000114 rdf:resource="&obo;IAO_0000428"/>
	<rdfs:comment xml:lang="en">LanguaL curation note: Index type of cereal/grain (barley, rice) in facet B.  If an industry recognized organic certification is claimed, index ORGANIC FOOD CLAIM OR USE in facet P. Index preservation method (refrigeration) in facet J.</rdfs:comment>
	<oboInOwl:hasDbXref>LANGUAL:A0966</oboInOwl:hasDbXref>
</owl:Class>

<owl:Class rdf:about="&obo;FOODON_03400967">
	<rdfs:label xml:lang="en">10000319 - grains/cereal - ready to eat - (shelf stable) (gs1 gpc)</rdfs:label>
	<rdfs:subClassOf rdf:resource="&obo;FOODON_03400961"/>
	<obo:IAO_0000412>http://langual.org</obo:IAO_0000412>
	<obo:IAO_0000115 xml:lang="en">Includes any products that can be described/observed as a grain, ready to eat product, such as Rice, Polenta, Couscous. These products must not include any additional ingredients and are not part of a recipe prior to sale. These products do not require cooking prior to consumption, but some products can be reheated. These products have been treated or packaged in such a way as to extend their consumable life. Specifically excludes all grain based prepared products such as Shelf Stable Rice Salad and Cereal Products. Excludes products such as Perishable Ready to Eat and Not Ready to Eat Grain and all Grain Based Prepared Recipe Products.</obo:IAO_0000115>
	<obo:IAO_0000114 rdf:resource="&obo;IAO_0000428"/>
	<rdfs:comment xml:lang="en">LanguaL curation note: Index type of cereal/grain (barley, rice) in facet B.  If an industry recognized organic certification is claimed, index ORGANIC FOOD CLAIM OR USE in facet P.</rdfs:comment>
	<oboInOwl:hasDbXref>LANGUAL:A0967</oboInOwl:hasDbXref>
</owl:Class>

<owl:Class rdf:about="&obo;FOODON_03400968">
	<rdfs:label xml:lang="en">10000599 - grains/flour variety packs (gs1 gpc)</rdfs:label>
	<rdfs:subClassOf rdf:resource="&obo;FOODON_03400961"/>
	<obo:IAO_0000412>http://langual.org</obo:IAO_0000412>
	<obo:IAO_0000115 xml:lang="en">Includes any products that can be described/observed as two or more distinct Grains or Flour sold together, which exist within the schema belonging to different bricks but to the same class, that is two or more products contained within the same pack which cross bricks within the Grains and Flour class. Includes products such as Semolina and not ready to eat Polenta sold together. Items that are received free with purchases should be removed from the classification decision-making process. Excludes products such as Rice and Cooking Sauces variety packs.</obo:IAO_0000115>
	<obo:IAO_0000114 rdf:resource="&obo;IAO_0000428"/>
	<oboInOwl:hasDbXref>LANGUAL:A0968</oboInOwl:hasDbXref>
</owl:Class>

<owl:Class rdf:about="&obo;FOODON_03400969">
	<rdfs:label xml:lang="en">50221200 - processed cereal products (gs1 gpc)</rdfs:label>
	<rdfs:subClassOf rdf:resource="&obo;FOODON_03400960"/>
	<obo:IAO_0000412>http://langual.org</obo:IAO_0000412>
	<obo:IAO_0000114 rdf:resource="&obo;IAO_0000428"/>
	<oboInOwl:hasDbXref>LANGUAL:A0969</oboInOwl:hasDbXref>
</owl:Class>

<owl:Class rdf:about="&obo;FOODON_03400970">
	<rdfs:label xml:lang="en">10000285 - cereals products - not ready to eat (shelf stable) (gs1 gpc)</rdfs:label>
	<rdfs:subClassOf rdf:resource="&obo;FOODON_03400969"/>
	<obo:IAO_0000412>http://langual.org</obo:IAO_0000412>
	<obo:IAO_0000115 xml:lang="en">Includes any products that can be described/observed as a cereal produced from wheat, rye, barley, oats, or other types of grain, which has gone through further manufacturing processes such as cooking, milling, drying and reforming, which will require preparation/cooking prior to consumption. Includes products such as porridge oats, couscous and tapioca. These products have been treated or packaged in such a way as to extend their consumable life. Excludes products such as whole Unprocessed Grains, Flour, Ready to Eat Cereal, Cereal Bars.</obo:IAO_0000115>
	<obo:IAO_0000114 rdf:resource="&obo;IAO_0000428"/>
	<rdfs:comment xml:lang="en">LanguaL curation note: Index type of cereal/grain (barley, rice) in facet B.  Index claims (organic, low calorie, sugar free or low) in facet P. If ingredient added (sugar), index in facet H.</rdfs:comment>
	<oboInOwl:hasDbXref>LANGUAL:A0970</oboInOwl:hasDbXref>
</owl:Class>

<owl:Class rdf:about="&obo;FOODON_03400971">
	<rdfs:label xml:lang="en">10000284 - cereals products - ready to eat (shelf stable) (gs1 gpc)</rdfs:label>
	<rdfs:subClassOf rdf:resource="&obo;FOODON_03400969"/>
	<obo:IAO_0000412>http://langual.org</obo:IAO_0000412>
	<obo:IAO_0000115 xml:lang="en">Includes any products that can be described/observed as a cereal produced from wheat, rye, barley, oats, or other types of grain, which has gone through further manufacturing processes such as cooking and milling, which does not require cooking and is usually consumed as a breakfast food, served with hot or cold milk. These products have been treated or packaged in such a way as to extend their consumable life. Includes single grain cereals, mixed grain cereals, and cereals containing additional ingredients such as fruit, nuts, or chocolate. Excludes products such as Perishable Ready to Eat Cereals, Whole Unprocessed Grains, Flour, Cereals that require cooking and Cereal Bars.</obo:IAO_0000115>
	<obo:IAO_0000114 rdf:resource="&obo;IAO_0000428"/>
	<rdfs:comment xml:lang="en">LanguaL curation note: Index type of cereal/grain (barley, rice) in facet B.  Index claims (organic, low calorie, sugar free or low) in facet P. If ingredient added (sugar), index in facet H.</rdfs:comment>
	<oboInOwl:hasDbXref>LANGUAL:A0971</oboInOwl:hasDbXref>
</owl:Class>

<owl:Class rdf:about="&obo;FOODON_03400972">
	<rdfs:label xml:lang="en">10000286 - cereal products - ready to eat (perishable) (gs1 gpc)</rdfs:label>
	<rdfs:subClassOf rdf:resource="&obo;FOODON_03400969"/>
	<obo:IAO_0000412>http://langual.org</obo:IAO_0000412>
	<obo:IAO_0000115 xml:lang="en">Includes any products that can be described/observed as a processed cereal produced from wheat, rye, barley, oats, or other types of grain, which has gone through further manufacturing processes such as cooking and milling, which does not require cooking and is usually consumed as a breakfast food, served with hot or cold milk. These products must be refrigerated to extend their consumable life. Includes single grain cereals, mixed grain cereals, and cereals containing additional ingredients such as fruit, nuts, or chocolate. Excludes products such as Whole Unprocessed Grains, Flour, Cereal that requires cooking, Cereal Bars.</obo:IAO_0000115>
	<obo:IAO_0000114 rdf:resource="&obo;IAO_0000428"/>
	<rdfs:comment xml:lang="en">LanguaL curation note: Index type of cereal/grain (barley, rice) in facet B.  Index claims (organic, low calorie, sugar free or low) in facet P. If ingredient added (sugar), index in facet H. Index preservation method (refrigeration) in facet J.</rdfs:comment>
	<oboInOwl:hasDbXref>LANGUAL:A0972</oboInOwl:hasDbXref>
</owl:Class>

<owl:Class rdf:about="&obo;FOODON_03400973">
	<rdfs:label xml:lang="en">10000287 - cereal/muesli bars (gs1 gpc)</rdfs:label>
	<rdfs:subClassOf rdf:resource="&obo;FOODON_03400969"/>
	<obo:IAO_0000412>http://langual.org</obo:IAO_0000412>
	<obo:IAO_0000115 xml:lang="en">Includes any products that can be described/observed as a block or bar combining all or some of the following ingredients; oats, muesli, wheat, rice, bran, fruit, nuts, cereal and honey. Products may contain chocolate or be fully or partially chocolate coated. These products have been treated or packaged in such a way as to extend their consumable life. These products will sometimes refer to benefits such as natural ingredients, high in fibre, vitamins, protein or energy or low in fat. Excludes products such as Cereals, Chocolate Bars, Cakes, Biscuits and Cookies.</obo:IAO_0000115>
	<obo:IAO_0000114 rdf:resource="&obo;IAO_0000428"/>
	<rdfs:comment xml:lang="en">LanguaL curation note: Index claims (organic, low calorie, sugar free or low) in facet P. If ingredient added (fruit, sugar) or surface coated/filled, index in facet H.</rdfs:comment>
	<oboInOwl:hasDbXref>LANGUAL:A0973</oboInOwl:hasDbXref>
</owl:Class>

<owl:Class rdf:about="&obo;FOODON_03400974">
	<rdfs:label xml:lang="en">10000600 - processed cereal products variety packs (gs1 gpc)</rdfs:label>
	<rdfs:subClassOf rdf:resource="&obo;FOODON_03400969"/>
	<obo:IAO_0000412>http://langual.org</obo:IAO_0000412>
	<obo:IAO_0000115 xml:lang="en">Includes any products that can be described/observed as two or more distinct Processed Cereals sold together, which exist within the schema belonging to different bricks but to the same class, that is two or more products contained within the same pack which cross bricks within the Processed Cereal Products class. Includes products such as ready to eat Packet Cereal and Cereal Bars sold together. Items that are received free with purchases should be removed from the classification decision-making process. Excludes products such as Cereal Bars and ready to drink Milkshake variety packs.</obo:IAO_0000115>
	<obo:IAO_0000114 rdf:resource="&obo;IAO_0000428"/>
	<oboInOwl:hasDbXref>LANGUAL:A0974</oboInOwl:hasDbXref>
</owl:Class>

<owl:Class rdf:about="&obo;FOODON_03400975">
	<rdfs:label xml:lang="en">50221300 - cereal/grain/pulse products variety packs (gs1 gpc)</rdfs:label>
	<rdfs:subClassOf rdf:resource="&obo;FOODON_03400960"/>
	<obo:IAO_0000412>http://langual.org</obo:IAO_0000412>
	<obo:IAO_0000115 xml:lang="en">Includes any products that can be described/observed as two or more distinct Cereal, Grain and Pulse Products sold together which exist within the schema but belong to different classes, that is two or more products contained within the same pack which cross classes within the Cereal, Grain and Pulse Products Family. Includes products such as Cereal Bars and ready to eat Couscous variety packs. Items that are received free with purchases should be removed from the classification decision-making process. Excludes products such as Semolina and not ready to eat Polenta variety packs and Cereal Bars and ready to drink Milkshake variety packs.</obo:IAO_0000115>
	<obo:IAO_0000114 rdf:resource="&obo;IAO_0000428"/>
	<oboInOwl:hasDbXref>LANGUAL:A0975</oboInOwl:hasDbXref>
</owl:Class>

<owl:Class rdf:about="&obo;FOODON_03400976">
	<rdfs:label xml:lang="en">50160000 - confectionery/sugar sweetening products (gs1 gpc)</rdfs:label>
	<rdfs:subClassOf rdf:resource="&obo;FOODON_03400874"/>
	<obo:IAO_0000412>http://langual.org</obo:IAO_0000412>
	<obo:IAO_0000114 rdf:resource="&obo;IAO_0000428"/>
	<oboInOwl:hasDbXref>LANGUAL:A0976</oboInOwl:hasDbXref>
</owl:Class>

<owl:Class rdf:about="&obo;FOODON_03400977">
	<rdfs:label xml:lang="en">50161800 - confectionery products (gs1 gpc)</rdfs:label>
	<rdfs:subClassOf rdf:resource="&obo;FOODON_03400976"/>
	<obo:IAO_0000412>http://langual.org</obo:IAO_0000412>
	<obo:IAO_0000114 rdf:resource="&obo;IAO_0000428"/>
	<oboInOwl:hasDbXref>LANGUAL:A0977</oboInOwl:hasDbXref>
</owl:Class>

<owl:Class rdf:about="&obo;FOODON_03400978">
	<rdfs:label xml:lang="en">10000045 - chocolate/chocolate substitutes confectionery (gs1 gpc)</rdfs:label>
	<rdfs:subClassOf rdf:resource="&obo;FOODON_03400977"/>
	<obo:IAO_0000412>http://langual.org</obo:IAO_0000412>
	<obo:IAO_0000115 xml:lang="en">Includes any products that can be described/observed as a portion of chocolate or chocolate substitute confectionery that may contain additional ingredients such as nuts, coconut, dried fruits, and soft filling. These products may be sold individually, or packaged to provide a quantity of similar items. Excludes products such as Sugar Candy Specialty Products covered in chocolate and Cooking Chocolate.</obo:IAO_0000115>
	<obo:IAO_0000114 rdf:resource="&obo;IAO_0000428"/>
	<rdfs:comment xml:lang="en">LanguaL curation note: Index use (diabetic) and sugar level claims in facet P.</rdfs:comment>
	<oboInOwl:hasDbXref>LANGUAL:A0978</oboInOwl:hasDbXref>
</owl:Class>

<owl:Class rdf:about="&obo;FOODON_03400979">
	<rdfs:label xml:lang="en">10000046 - chocolate/sugar candy combination - confectionery (gs1 gpc)</rdfs:label>
	<rdfs:subClassOf rdf:resource="&obo;FOODON_03400977"/>
	<obo:IAO_0000412>http://langual.org</obo:IAO_0000412>
	<obo:IAO_0000115 xml:lang="en">Includes any products that can be described/observed as a specific confectionery item that is covered in chocolate, such as toffee, marshmallow, liquorice and fudge. Excludes products such as pure Chocolate products with a sweet filling such as liqueur or fondant, pure Sugar Candy Products with no chocolate coating.</obo:IAO_0000115>
	<obo:IAO_0000114 rdf:resource="&obo;IAO_0000428"/>
	<rdfs:comment xml:lang="en">LanguaL curation note: Index use (diabetic) and sugar level claims in facet P. Index main ingredient in facet B and added ingredients in facet H.</rdfs:comment>
	<oboInOwl:hasDbXref>LANGUAL:A0979</oboInOwl:hasDbXref>
</owl:Class>

<owl:Class rdf:about="&obo;FOODON_03400980">
	<rdfs:label xml:lang="en">10000047 - sugar candy/sugar candy substitutes confectionery (gs1 gpc)</rdfs:label>
	<rdfs:subClassOf rdf:resource="&obo;FOODON_03400977"/>
	<obo:IAO_0000412>http://langual.org</obo:IAO_0000412>
	<obo:IAO_0000115 xml:lang="en">Includes any products that can be described/observed as a hard or soft confection made mostly from sugar, with added flavourings that may or may not contain gelatine. These products may be individually wrapped, packaged loose in a bag or container, or tightly packaged in a roll or tube. Products include toffees, chewing and bubble gum. Excludes products such as Sugar Candy Products covered in chocolate.</obo:IAO_0000115>
	<obo:IAO_0000114 rdf:resource="&obo;IAO_0000428"/>
	<rdfs:comment xml:lang="en">LanguaL curation note: Index use (diabetic) and sugar level claims in facet P.</rdfs:comment>
	<oboInOwl:hasDbXref>LANGUAL:A0980</oboInOwl:hasDbXref>
</owl:Class>

<owl:Class rdf:about="&obo;FOODON_03400981">
	<rdfs:label xml:lang="en">10000602 - confectionery products variety packs (gs1 gpc)</rdfs:label>
	<rdfs:subClassOf rdf:resource="&obo;FOODON_03400977"/>
	<obo:IAO_0000412>http://langual.org</obo:IAO_0000412>
	<obo:IAO_0000115 xml:lang="en">Includes any products that can be described/observed as two or more distinct Confectionery Products sold together, which exist within the schema belonging to different bricks but to the same class, that is two or more products contained within the same pack which cross bricks within the Confectionery Products class. Includes products such as Chocolate and Chewing Gum sold together. Items that are received free with purchases should be removed from the classification decision-making process. Excludes products such as Chocolate and Wine variety packs.</obo:IAO_0000115>
	<obo:IAO_0000114 rdf:resource="&obo;IAO_0000428"/>
	<oboInOwl:hasDbXref>LANGUAL:A0981</oboInOwl:hasDbXref>
</owl:Class>

<owl:Class rdf:about="&obo;FOODON_03400982">
	<rdfs:label xml:lang="en">50161500 - sugars/sugar substitute products (gs1 gpc)</rdfs:label>
	<rdfs:subClassOf rdf:resource="&obo;FOODON_03400976"/>
	<obo:IAO_0000412>http://langual.org</obo:IAO_0000412>
	<obo:IAO_0000114 rdf:resource="&obo;IAO_0000428"/>
	<oboInOwl:hasDbXref>LANGUAL:A0982</oboInOwl:hasDbXref>
</owl:Class>

<owl:Class rdf:about="&obo;FOODON_03400983">
	<rdfs:label xml:lang="en">10000043 - sugar/sugar substitutes (shelf stable) (gs1 gpc)</rdfs:label>
	<rdfs:subClassOf rdf:resource="&obo;FOODON_03400982"/>
	<obo:IAO_0000412>http://langual.org</obo:IAO_0000412>
	<obo:IAO_0000115 xml:lang="en">Includes any products that can be described/observed as a sweet substance, obtained from the different stages of refining the juice of the sugar cane/sugar beet/molasses, or an artificial sweet substance that is specifically labelled and marketed to replace natural sugar, which is used as a sweetener and preservative of food and drinks. Products include white sugars such as castor, cubes, loaf, granulated, icing and preserving, coloured sugars such as brown, barbados, demerara and artificial sweeteners, such as saccharin, sorbitol and xylitol. Excludes products such as Syrups, Treacle and Molasses, Sugar Candy and Sugar Candy Substitute Confectionery.</obo:IAO_0000115>
	<obo:IAO_0000114 rdf:resource="&obo;IAO_0000428"/>
	<rdfs:comment xml:lang="en">LanguaL curation note: Index diabetic use and organic claims in facet P. Index physical form (granulated, liquid) in facet E. If sugar, index source (cane, sugar beet) in facet B and type of sugar (destrose, brown sugar) in facet C. If sugar substitute (xylitol, sorbitol), index under FOOD ADDITIVE, EUROPEAN COMMUNITY/CODEX ALIMENTARIUS in facet C.</rdfs:comment>
	<oboInOwl:hasDbXref>LANGUAL:A0983</oboInOwl:hasDbXref>
</owl:Class>

<owl:Class rdf:about="&obo;FOODON_03400984">
	<rdfs:label xml:lang="en">10000044 - syrup/treacle/molasses (shelf stable) (gs1 gpc)</rdfs:label>
	<rdfs:subClassOf rdf:resource="&obo;FOODON_03400982"/>
	<obo:IAO_0000412>http://langual.org</obo:IAO_0000412>
	<obo:IAO_0000115 xml:lang="en">Includes any products that can be described/observed as a sweet thick liquid that is a derivative of the sugar crystallization process, such as molasses (the residue left after the first stage), treacle (the residue from the second stage that is sweeter and less viscous than molasses), syrup (prepared from molasses, glucose and often flavourings or a solution of sugar which may be from a variety of sources, such as maple). Products include corn syrups, fruit syrups, golden syrups, maple syrups and molasses. Excludes products such as Sugar and Sugar Substitutes.</obo:IAO_0000115>
	<obo:IAO_0000114 rdf:resource="&obo;IAO_0000428"/>
	<rdfs:comment xml:lang="en">LanguaL curation note: Index diabetic use and organic claims in facet P. Index type of syrup in facet C (MOLASSES, HIGH FRUCTOSE SYRUP).</rdfs:comment>
	<oboInOwl:hasDbXref>LANGUAL:A0984</oboInOwl:hasDbXref>
</owl:Class>

<owl:Class rdf:about="&obo;FOODON_03400985">
	<rdfs:label xml:lang="en">10000603 - sugars/sugar substitute products variety packs (gs1 gpc)</rdfs:label>
	<rdfs:subClassOf rdf:resource="&obo;FOODON_03400982"/>
	<obo:IAO_0000412>http://langual.org</obo:IAO_0000412>
	<obo:IAO_0000115 xml:lang="en">Includes any products that can be described/observed as two or more distinct Sugars or Sugar Substitutes sold together, which exist within the schema belonging to different bricks but to the same class, that is two or more products contained within the same pack which cross bricks within the Sugars and Sugar Substitutes Products class. Includes products such as Golden Syrup and Dark Brown Sugar sold together. Items that are received free with purchases should be removed from the classification decision-making process. Excludes products such as Golden Syrup and Sponge Cake variety packs.</obo:IAO_0000115>
	<obo:IAO_0000114 rdf:resource="&obo;IAO_0000428"/>
	<oboInOwl:hasDbXref>LANGUAL:A0985</oboInOwl:hasDbXref>
</owl:Class>

<owl:Class rdf:about="&obo;FOODON_03400986">
	<rdfs:label xml:lang="en">50161900 - confectionery/sugar sweetening products variety packs (gs1 gpc)</rdfs:label>
	<rdfs:subClassOf rdf:resource="&obo;FOODON_03400976"/>
	<obo:IAO_0000412>http://langual.org</obo:IAO_0000412>
	<obo:IAO_0000115 xml:lang="en">Includes any products that can be described/observed as two or more distinct Confectionery and Sugar Sweeteners sold together which exist within the schema but belong to different classes, that is two or more products contained within the same pack which cross classes within the Confectionery and Sugar Sweetening Products Family. Includes products such as Chocolate with Treacle variety packs. Items that are received free with purchases should be removed from the classification decision-making process. Excludes products such as Chocolate and Chewing Gum variety packs and Chocolate and Wine variety packs.</obo:IAO_0000115>
	<obo:IAO_0000114 rdf:resource="&obo;IAO_0000428"/>
	<oboInOwl:hasDbXref>LANGUAL:A0986</oboInOwl:hasDbXref>
</owl:Class>

<owl:Class rdf:about="&obo;FOODON_03400987">
	<rdfs:label xml:lang="en">50100000 - fruits/vegetables/nuts/seeds (gs1 gpc)</rdfs:label>
	<rdfs:subClassOf rdf:resource="&obo;FOODON_03400874"/>
	<obo:IAO_0000412>http://langual.org</obo:IAO_0000412>
	<obo:IAO_0000114 rdf:resource="&obo;IAO_0000428"/>
	<oboInOwl:hasDbXref>LANGUAL:A0987</oboInOwl:hasDbXref>
</owl:Class>

<owl:Class rdf:about="&obo;FOODON_03400988">
	<rdfs:label xml:lang="en">50102000 - fruit - prepared/processed (gs1 gpc)</rdfs:label>
	<rdfs:subClassOf rdf:resource="&obo;FOODON_03400987"/>
	<obo:IAO_0000412>http://langual.org</obo:IAO_0000412>
	<obo:IAO_0000114 rdf:resource="&obo;IAO_0000428"/>
	<oboInOwl:hasDbXref>LANGUAL:A0988</oboInOwl:hasDbXref>
</owl:Class>

<owl:Class rdf:about="&obo;FOODON_03400989">
	<rdfs:label xml:lang="en">10000204 - fruit - prepared/processed (frozen) (gs1 gpc)</rdfs:label>
	<rdfs:subClassOf rdf:resource="&obo;FOODON_03400988"/>
	<obo:IAO_0000412>http://langual.org</obo:IAO_0000412>
	<obo:IAO_0000115 xml:lang="en">Includes any products that can be described/observed as any variety of fruit or combination of fruits, which may be whole or stoned, pitted, chopped, cored and/or peeled, and which have gone through further manufacturing processes, such as reformed, cooked or dried, however these products can also be coated, in sauce, stuffed or filled. These products must be frozen to extend their consumable life. Specifically excludes tomatoes. Excludes products such as Unprepared and Unprocessed Fruit and Prepared and Processed Shelf Stable &amp; Perishable Fruit.</obo:IAO_0000115>
	<obo:IAO_0000114 rdf:resource="&obo;IAO_0000428"/>
	<rdfs:comment xml:lang="en">LanguaL curation note: Index type of fruit (apple, watermellon) in facet B. Index physical form (whole, sliced) in facet E. If an industry recognized organic certification is claimed, index ORGANIC FOOD CLAIM OR USE in facet P. Index whether pitted or stoned in facet C. Index manufacturer's treatments (sugared, dried) in facet H and heat treatment (cooked, pasteurised) in facet F.</rdfs:comment>
	<oboInOwl:hasDbXref>LANGUAL:A0989</oboInOwl:hasDbXref>
</owl:Class>

<owl:Class rdf:about="&obo;FOODON_03400990">
	<rdfs:label xml:lang="en">10000205 - fruit - prepared/processed (perishable) (gs1 gpc)</rdfs:label>
	<rdfs:subClassOf rdf:resource="&obo;FOODON_03400988"/>
	<obo:IAO_0000412>http://langual.org</obo:IAO_0000412>
	<obo:IAO_0000115 xml:lang="en">Includes any products that can be described/observed as any variety of fruit or combination of fruits, which may be whole or stoned, pitted, chopped, cored and/or peeled, and which have gone through further manufacturing processes, such as reformed, cooked or dried, however these products can also be coated, in sauce, stuffed or filled. Specifically excludes tomatoes. Excludes products such as Unprepared and Unprocessed Fruit and Prepared and Processed Shelf Stable &amp; Frozen Fruit.</obo:IAO_0000115>
	<obo:IAO_0000114 rdf:resource="&obo;IAO_0000428"/>
	<rdfs:comment xml:lang="en">LanguaL curation note: Index type of fruit (apple, watermellon) in facet B. Index physical form (whole, sliced) in facet E. If an industry recognized organic certification is claimed, index ORGANIC FOOD CLAIM OR USE in facet P. Index whether pitted or stoned in facet C. Index manufacturer's treatments (sugared, dried) in facet H and heat treatment (cooked, pasteurised) in facet F.</rdfs:comment>
	<oboInOwl:hasDbXref>LANGUAL:A0990</oboInOwl:hasDbXref>
</owl:Class>

<owl:Class rdf:about="&obo;FOODON_03400991">
	<rdfs:label xml:lang="en">10000206 - fruit - prepared/processed (shelf stable) (gs1 gpc)</rdfs:label>
	<rdfs:subClassOf rdf:resource="&obo;FOODON_03400988"/>
	<obo:IAO_0000412>http://langual.org</obo:IAO_0000412>
	<obo:IAO_0000115 xml:lang="en">Includes any products that can be described/observed as any variety of fruit or combination of fruits, which may be whole or stoned, pitted, chopped, cored and/or peeled, and which have gone through further manufacturing processes, such as reformed, cooked or dried, however these products can also be coated, in sauce, stuffed or filled. These products have been treated or packaged in such a way as to extend their consumable life. Specifically excludes tomatoes. Excludes products such as Unprepared and Unprocessed Fruit and Prepared and Processed Frozen &amp; Perishable Fruit.</obo:IAO_0000115>
	<obo:IAO_0000114 rdf:resource="&obo;IAO_0000428"/>
	<rdfs:comment xml:lang="en">LanguaL curation note: Index type of fruit (apple, watermellon) in facet B. Index physical form (whole, sliced) in facet E. If an industry recognized organic certification is claimed, index ORGANIC FOOD CLAIM OR USE in facet P. Index whether pitted or stoned in facet C. Index manufacturer's treatments (sugared, dried) in facet H and heat treatment (cooked, pasteurised) in facet F.</rdfs:comment>
	<oboInOwl:hasDbXref>LANGUAL:A0991</oboInOwl:hasDbXref>
</owl:Class>

<owl:Class rdf:about="&obo;FOODON_03400992">
	<rdfs:label xml:lang="en">50101600 - fruit - unprepared/unprocessed (gs1 gpc)</rdfs:label>
	<rdfs:subClassOf rdf:resource="&obo;FOODON_03400987"/>
	<obo:IAO_0000412>http://langual.org</obo:IAO_0000412>
	<obo:IAO_0000114 rdf:resource="&obo;IAO_0000428"/>
	<oboInOwl:hasDbXref>LANGUAL:A0992</oboInOwl:hasDbXref>
</owl:Class>

<owl:Class rdf:about="&obo;FOODON_03400993">
	<rdfs:label xml:lang="en">10000002 - fruit - unprepared/unprocessed (frozen) (gs1 gpc)</rdfs:label>
	<rdfs:subClassOf rdf:resource="&obo;FOODON_03400992"/>
	<obo:IAO_0000412>http://langual.org</obo:IAO_0000412>
	<obo:IAO_0000115 xml:lang="en">Includes any products that can be described/observed as any variety of frozen fruit or combination of fruits, which may be whole or stoned, pitted, chopped, cored and/or peeled, but has not gone through any further manufacturing processes, such as reformed or cooked, however these products can be coated, in sauce, stuffed or filled. These products must be frozen to extend their consumable life. Specifically excludes tomatoes. Excludes products such as Prepared and Processed Fruit and Perishable and Shelf Stable Unprepared and Unprocessed Fruits.</obo:IAO_0000115>
	<obo:IAO_0000114 rdf:resource="&obo;IAO_0000428"/>
	<rdfs:comment xml:lang="en">LanguaL curation note: Index type of fruit (apple, watermellon) in facet B. Index physical form (whole, sliced) in facet E. If an industry recognized organic certification is claimed, index ORGANIC FOOD CLAIM OR USE in facet P. Index whether pitted or stoned in facet C.</rdfs:comment>
	<oboInOwl:hasDbXref>LANGUAL:A0993</oboInOwl:hasDbXref>
</owl:Class>

<owl:Class rdf:about="&obo;FOODON_03400994">
	<rdfs:label xml:lang="en">10000001 - fruit - unprepared/unprocessed (perishable) (gs1 gpc)</rdfs:label>
	<rdfs:subClassOf rdf:resource="&obo;FOODON_03400992"/>
	<obo:IAO_0000412>http://langual.org</obo:IAO_0000412>
	<obo:IAO_0000115 xml:lang="en">Includes any products that can be described/observed as any variety of fresh fruit or combination of fruits, which may be whole or stoned, pitted, chopped, cored and/or peeled, but has not gone through any further manufacturing processes, such as reformed, cooked or dried, however these products can be coated, in sauce, stuffed or filled. These products can be/must be refrigerated to extend their consumable life. Specifically excludes tomatoes. Excludes products such as Prepared and Processed Fruit and Frozen and Shelf Stable Unprepared and Unprocessed Fruits.</obo:IAO_0000115>
	<obo:IAO_0000114 rdf:resource="&obo;IAO_0000428"/>
	<rdfs:comment xml:lang="en">LanguaL curation note: Index type of fruit (apple, watermellon) in facet B. Index physical form (whole, sliced) in facet E. If an industry recognized organic certification is claimed, index ORGANIC FOOD CLAIM OR USE in facet P. Index whether pitted or stoned in facet C.</rdfs:comment>
	<oboInOwl:hasDbXref>LANGUAL:A0994</oboInOwl:hasDbXref>
</owl:Class>

<owl:Class rdf:about="&obo;FOODON_03400995">
	<rdfs:label xml:lang="en">10000003 - fruit - unprepared/unprocessed (shelf stable) (gs1 gpc)</rdfs:label>
	<rdfs:subClassOf rdf:resource="&obo;FOODON_03400992"/>
	<obo:IAO_0000412>http://langual.org</obo:IAO_0000412>
	<obo:IAO_0000115 xml:lang="en">Includes any products that can be described/observed as any variety of fruit or combination of fruits, which may be whole or stoned, pitted, chopped, cored and/or peeled, but has not gone through any further manufacturing processes, such as reformed, cooked or dried, however these products can be coated, in sauce, stuffed or filled. These products have been treated or packaged in such a way as to extend their consumable life. Specifically excludes tomatoes. Excludes products such as Prepared and Processed Fruit and Perishable and Frozen Unprepared and Unprocessed Fruits.</obo:IAO_0000115>
	<obo:IAO_0000114 rdf:resource="&obo;IAO_0000428"/>
	<rdfs:comment xml:lang="en">LanguaL curation note: Index type of fruit (apple, watermellon) in facet B. Index physical form (whole, sliced) in facet E. If an industry recognized organic certification is claimed, index ORGANIC FOOD CLAIM OR USE in facet P. Index whether pitted or stoned in facet C.</rdfs:comment>
	<oboInOwl:hasDbXref>LANGUAL:A0995</oboInOwl:hasDbXref>
</owl:Class>

<owl:Class rdf:about="&obo;FOODON_03400996">
	<rdfs:label xml:lang="en">50101900 - fruit/nuts/seeds combination (gs1 gpc)</rdfs:label>
	<rdfs:subClassOf rdf:resource="&obo;FOODON_03400987"/>
	<obo:IAO_0000412>http://langual.org</obo:IAO_0000412>
	<obo:IAO_0000114 rdf:resource="&obo;IAO_0000428"/>
	<oboInOwl:hasDbXref>LANGUAL:A0996</oboInOwl:hasDbXref>
</owl:Class>

<owl:Class rdf:about="&obo;FOODON_03400997">
	<rdfs:label xml:lang="en">10000207 - fruit/nuts/seeds mixes - prepared/processed (shelf stable) (gs1 gpc)</rdfs:label>
	<rdfs:subClassOf rdf:resource="&obo;FOODON_03400996"/>
	<obo:IAO_0000412>http://langual.org</obo:IAO_0000412>
	<obo:IAO_0000115 xml:lang="en">Includes any products that can be described/observed as any variety of fruit mixed either with nuts or seeds or both, that have gone through further manufacturing processes, such as reformed, cooked or dried, however these products can also be coated, in sauce, stuffed or filled. These products have been treated or packaged in such a way as to extend their consumable life. Excludes products such as Fruit, Nuts and Seeds sold separately, Unprepared and Unprocessed Fruit and Nuts and/or Seeds Mixes.</obo:IAO_0000115>
	<obo:IAO_0000114 rdf:resource="&obo;IAO_0000428"/>
	<rdfs:comment xml:lang="en">LanguaL curation note: Index type of main ingredient (fruit, seed) and whether peeled or shelled in facet C. Index other ingredients (fruit added, nut or seed added) in facet H. Index physical form (whole, sliced) in facet E. If an industry recognized organic certification is claimed, index ORGANIC FOOD CLAIM OR USE in facet P.  Index manufacturer's treatments (sugared, dried) in facet H and heat treatment (cooked) in facet F.</rdfs:comment>
	<oboInOwl:hasDbXref>LANGUAL:A0997</oboInOwl:hasDbXref>
</owl:Class>

<owl:Class rdf:about="&obo;FOODON_03400998">
	<rdfs:label xml:lang="en">10000209 - fruit/nuts/seeds mixes - unprepared/unprocessed (shelf stable) (gs1 gpc)</rdfs:label>
	<rdfs:subClassOf rdf:resource="&obo;FOODON_03400996"/>
	<obo:IAO_0000412>http://langual.org</obo:IAO_0000412>
	<obo:IAO_0000115 xml:lang="en">Includes any products that can be described/observed as any variety of fruit mixed either with nuts or seeds or both, that has not gone through any further manufacturing processes, such as reformed, cooked or dried, however these products can be coated, in sauce, stuffed or filled. These products have been treated or packaged in such a way as to extend their consumable life. Excludes products such as Fruit, Nuts and Seeds sold separately, Prepared and Processed Fruit and Nuts and/or Seeds Mixes.</obo:IAO_0000115>
	<obo:IAO_0000114 rdf:resource="&obo;IAO_0000428"/>
	<rdfs:comment xml:lang="en">LanguaL curation note: Index type of main ingredient (fruit, seed) and whether peeled or shelled in facet C. Index other ingredients (fruit added, nut or seed added) in facet H. Index physical form (whole, sliced) in facet E. If an industry recognized organic certification is claimed, index ORGANIC FOOD CLAIM OR USE in facet P.</rdfs:comment>
	<oboInOwl:hasDbXref>LANGUAL:A0998</oboInOwl:hasDbXref>
</owl:Class>

<owl:Class rdf:about="&obo;FOODON_03400999">
	<rdfs:label xml:lang="en">10000604 - fruit/nuts/seeds combination variety packs (gs1 gpc)</rdfs:label>
	<rdfs:subClassOf rdf:resource="&obo;FOODON_03400996"/>
	<obo:IAO_0000412>http://langual.org</obo:IAO_0000412>
	<obo:IAO_0000115 xml:lang="en">Includes any products that can be described/observed as two or more distinct Fruit, Nut and/or Seed Combination sold together, which exist within the schema belonging to different bricks but to the same class, that is two or more products contained within the same pack which cross bricks within the Fruit and Nuts and/or Seeds Combination class. Includes products such as packets of dried fruit and unshelled nuts sold together. Items that are received free with purchases should be removed from the classification decision-making process. Excludes products such as Dried Fruit and Yogurt variety packs.</obo:IAO_0000115>
	<obo:IAO_0000114 rdf:resource="&obo;IAO_0000428"/>
	<oboInOwl:hasDbXref>LANGUAL:A0999</oboInOwl:hasDbXref>
</owl:Class>

<owl:Class rdf:about="&obo;FOODON_03401000">
	<rdfs:label xml:lang="en">50101800 - nuts/seeds - prepared/processed (gs1 gpc)</rdfs:label>
	<rdfs:subClassOf rdf:resource="&obo;FOODON_03400987"/>
	<obo:IAO_0000412>http://langual.org</obo:IAO_0000412>
	<obo:IAO_0000114 rdf:resource="&obo;IAO_0000428"/>
	<oboInOwl:hasDbXref>LANGUAL:A1000</oboInOwl:hasDbXref>
</owl:Class>

<owl:Class rdf:about="&obo;FOODON_03401001">
	<rdfs:label xml:lang="en">10000235 - nuts/seeds - prepared/processed (perishable) (gs1 gpc)</rdfs:label>
	<rdfs:subClassOf rdf:resource="&obo;FOODON_03401000"/>
	<obo:IAO_0000412>http://langual.org</obo:IAO_0000412>
	<obo:IAO_0000115 xml:lang="en">Includes any products that can be described/observed as any variety of fresh nuts and seeds that has gone through further manufacturing processes, such as reformed or cooked, however these products can also be coated, in sauce, stuffed or filled.. These products can be/must be refrigerated to extend their consumable life. Products include nuts and seeds sold on their own or a combination of both. Excludes products such as Shelf Stable Nuts and Seeds, Unprepared and Unprocessed Nuts and Seeds, Fruit and Nuts and/or Seeds Mixes.</obo:IAO_0000115>
	<obo:IAO_0000114 rdf:resource="&obo;IAO_0000428"/>
	<rdfs:comment xml:lang="en">LanguaL curation note: Index type of nut or seed (almond, walnut) in facet B and if shelled/peeled in facet C. Index physical form (whole, chopped) in facet E. If an industry recognized organic certification is claimed, index ORGANIC FOOD CLAIM OR USE in facet P.  Index manufacturer's treatments (sugared, dried) in facet H and heat treatment (cooked) in facet F. Index preservation method (refrigeration) in facet J.</rdfs:comment>
	<oboInOwl:hasDbXref>LANGUAL:A1001</oboInOwl:hasDbXref>
</owl:Class>

<owl:Class rdf:about="&obo;FOODON_03401002">
	<rdfs:label xml:lang="en">10000236 - nuts/seeds - prepared/processed (shelf stable) (gs1 gpc)</rdfs:label>
	<rdfs:subClassOf rdf:resource="&obo;FOODON_03401000"/>
	<obo:IAO_0000412>http://langual.org</obo:IAO_0000412>
	<obo:IAO_0000115 xml:lang="en">Includes any products that can be described/observed as any variety of nuts and seeds that has gone through further manufacturing processes, such as reformed, cooked or dried, however these products can also be coated, in sauce, stuffed or filled. These products have been treated or packaged in such a way as to extend their consumable life. Products include nuts and seeds sold on their own or a combination of both. Excludes products such as Perishable Nuts and Seeds, Unprepared and Unprocessed Nuts and Seeds, Fruit and Nuts and/or Seeds Mixes.</obo:IAO_0000115>
	<obo:IAO_0000114 rdf:resource="&obo;IAO_0000428"/>
	<rdfs:comment xml:lang="en">LanguaL curation note: Index type of nut or seed (almond, walnut) in facet B and if shelled/peeled in facet C. Index physical form (whole, chopped) in facet E. If an industry recognized organic certification is claimed, index ORGANIC FOOD CLAIM OR USE in facet P.  Index manufacturer's treatments (sugared, dried) in facet H and heat treatment (cooked) in facet F.</rdfs:comment>
	<oboInOwl:hasDbXref>LANGUAL:A1002</oboInOwl:hasDbXref>
</owl:Class>

<owl:Class rdf:about="&obo;FOODON_03401003">
	<rdfs:label xml:lang="en">50101700 - nuts/seeds - unprepared/unprocessed (gs1 gpc)</rdfs:label>
	<rdfs:subClassOf rdf:resource="&obo;FOODON_03400987"/>
	<obo:IAO_0000412>http://langual.org</obo:IAO_0000412>
	<obo:IAO_0000114 rdf:resource="&obo;IAO_0000428"/>
	<oboInOwl:hasDbXref>LANGUAL:A1003</oboInOwl:hasDbXref>
</owl:Class>

<owl:Class rdf:about="&obo;FOODON_03401004">
	<rdfs:label xml:lang="en">10000007 - nuts/seeds - unprepared/unprocessed (perishable) (gs1 gpc)</rdfs:label>
	<rdfs:subClassOf rdf:resource="&obo;FOODON_03401003"/>
	<obo:IAO_0000412>http://langual.org</obo:IAO_0000412>
	<obo:IAO_0000115 xml:lang="en">Includes any products that can be described/observed as any variety of fresh nuts and seeds that has not gone through any further manufacturing processes, such as reformed, cooked or dried, however these products can be coated, in sauce, stuffed or filled. These products can be/must be refrigerated to extend their consumable life. Products include nuts and seeds sold on their own or a combination of both. Excludes products such as Shelf Stable Nuts and Seeds, Prepared and Processed Nuts and Seeds, Fruit and Nuts and/or Seeds Mixes.</obo:IAO_0000115>
	<obo:IAO_0000114 rdf:resource="&obo;IAO_0000428"/>
	<rdfs:comment xml:lang="en">LanguaL curation note: Index type of nut or seed (almond, walnut) in facet B and if shelled/peeled in facet C. Index physical form (whole, chopped) in facet E. If an industry recognized organic certification is claimed, index ORGANIC FOOD CLAIM OR USE in facet P. Index preservation method (refrigeration) in facet J.</rdfs:comment>
	<oboInOwl:hasDbXref>LANGUAL:A1004</oboInOwl:hasDbXref>
</owl:Class>

<owl:Class rdf:about="&obo;FOODON_03401005">
	<rdfs:label xml:lang="en">10000008 - nuts/seeds - unprepared/unprocessed (shelf stable) (gs1 gpc)</rdfs:label>
	<rdfs:subClassOf rdf:resource="&obo;FOODON_03401003"/>
	<obo:IAO_0000412>http://langual.org</obo:IAO_0000412>
	<obo:IAO_0000115 xml:lang="en">Includes any products that can be described/observed as any variety of nuts and seeds that has not gone through any further manufacturing processes, such as reformed, cooked or dried, however these products can be coated, in sauce, stuffed or filled. These products have been treated or packaged in such a way as to extend their consumable life. Products include nuts and seeds sold on their own or a combination of both. Excludes products such as Perishable Nuts and Seeds, Prepared and Processed Nuts and Seeds, Fruit and Nuts and/or Seeds Mixes.</obo:IAO_0000115>
	<obo:IAO_0000114 rdf:resource="&obo;IAO_0000428"/>
	<rdfs:comment xml:lang="en">LanguaL curation note: Index type of nut or seed (almond, walnut) in facet B and if shelled/peeled in facet C. Index physical form (whole, chopped) in facet E. If an industry recognized organic certification is claimed, index ORGANIC FOOD CLAIM OR USE in facet P.</rdfs:comment>
	<oboInOwl:hasDbXref>LANGUAL:A1005</oboInOwl:hasDbXref>
</owl:Class>

<owl:Class rdf:about="&obo;FOODON_03401006">
	<rdfs:label xml:lang="en">50102100 - vegetables - prepared/processed (gs1 gpc)</rdfs:label>
	<rdfs:subClassOf rdf:resource="&obo;FOODON_03400987"/>
	<obo:IAO_0000412>http://langual.org</obo:IAO_0000412>
	<obo:IAO_0000114 rdf:resource="&obo;IAO_0000428"/>
	<oboInOwl:hasDbXref>LANGUAL:A1006</oboInOwl:hasDbXref>
</owl:Class>

<owl:Class rdf:about="&obo;FOODON_03401007">
	<rdfs:label xml:lang="en">10000270 - vegetables - prepared/processed (frozen) (gs1 gpc)</rdfs:label>
	<rdfs:subClassOf rdf:resource="&obo;FOODON_03401006"/>
	<obo:IAO_0000412>http://langual.org</obo:IAO_0000412>
	<obo:IAO_0000115 xml:lang="en">Includes any products that can be described/observed as any variety of vegetables, combination of vegetables or fruit vegetables, which may be whole, chopped, cleaned and trimmed, that have gone through further manufacturing processes, such as reformed, cooked, dried, salted or smoked, however these products can also be coated, in sauce, stuffed or filled. Specifically excludes products that have added ingredients included such as rice, couscous and pasta. These products must be frozen to extend their consumable life. Excludes products such as Vegetables with additional dough or grains, Shelf Stable and Perishable Prepared and Processed Vegetables, all Unprepared and Unprocessed Vegetables, all Fruit, Nuts and Seeds.</obo:IAO_0000115>
	<obo:IAO_0000114 rdf:resource="&obo;IAO_0000428"/>
	<rdfs:comment xml:lang="en">LanguaL curation note: Index type of vegetable (alfalfa, yuca) in facet B. Index physical form (whole, chopped) in facet E. If an industry recognized organic certification is claimed, index ORGANIC FOOD CLAIM OR USE in facet P. Index manufacturer's treatments (seasoned, dried) in facet H and heat treatment (cooked) in facet F.</rdfs:comment>
	<oboInOwl:hasDbXref>LANGUAL:A1007</oboInOwl:hasDbXref>
</owl:Class>

<owl:Class rdf:about="&obo;FOODON_03401008">
	<rdfs:label xml:lang="en">10000271 - vegetables - prepared/processed (perishable) (gs1 gpc)</rdfs:label>
	<rdfs:subClassOf rdf:resource="&obo;FOODON_03401006"/>
	<obo:IAO_0000412>http://langual.org</obo:IAO_0000412>
	<obo:IAO_0000115 xml:lang="en">Includes any products that can be described/observed as any variety of fresh vegetables, combination of vegetables or fruit vegetables, which may be whole, chopped, cleaned and trimmed, that have gone through further manufacturing processes, such as reformed, cooked, salted or smoked, however these products can also be coated, in sauce, stuffed or filled. Specifically excludes products that have added ingredients included such as rice, couscous and pasta. These products can be/must be refrigerated to extend their consumable life. Excludes products such as Vegetables with additional dough or grains, Frozen and Shelf Stable Prepared and Processed Vegetables, all Unprepared and Unprocessed Vegetables, all Fruit, Nuts and Seeds.</obo:IAO_0000115>
	<obo:IAO_0000114 rdf:resource="&obo;IAO_0000428"/>
	<rdfs:comment xml:lang="en">LanguaL curation note: Index type of vegetable (alfalfa, yuca) in facet B. Index physical form (whole, chopped) in facet E. If an industry recognized organic certification is claimed, index ORGANIC FOOD CLAIM OR USE in facet P. Index manufacturer's treatments (seasoned, dried) in facet H and heat treatment (cooked) in facet F. Index preservation method (refrigeration) in facet J.</rdfs:comment>
	<oboInOwl:hasDbXref>LANGUAL:A1008</oboInOwl:hasDbXref>
</owl:Class>

<owl:Class rdf:about="&obo;FOODON_03401009">
	<rdfs:label xml:lang="en">10000272 - vegetables - prepared/processed (shelf stable) (gs1 gpc)</rdfs:label>
	<rdfs:subClassOf rdf:resource="&obo;FOODON_03401006"/>
	<obo:IAO_0000412>http://langual.org</obo:IAO_0000412>
	<obo:IAO_0000115 xml:lang="en">Includes any products that can be described/observed as any variety of vegetables combination of vegetables or fruit vegetables, which may be whole, chopped, cleaned and trimmed, that have gone through further manufacturing processes, such as reformed, cooked, dried, salted or smoked, however these products can also be coated, in sauce, stuffed or filled. Specifically excludes products that have added ingredients included such as rice, couscous and pasta. These products have been treated or packaged in such a way as to extend their consumable life. Excludes products such as Vegetables with additional dough or grains, Frozen and Perishable Prepared and Processed Vegetables, all Unprepared and Unprocessed Vegetables, all Fruit, Nuts and Seeds.</obo:IAO_0000115>
	<obo:IAO_0000114 rdf:resource="&obo;IAO_0000428"/>
	<rdfs:comment xml:lang="en">LanguaL curation note: Index type of vegetable (alfalfa, yuca) in facet B. Index physical form (whole, chopped) in facet E. If an industry recognized organic certification is claimed, index ORGANIC FOOD CLAIM OR USE in facet P. Index manufacturer's treatments (seasoned, dried) in facet H and heat treatment (cooked) in facet F.</rdfs:comment>
	<oboInOwl:hasDbXref>LANGUAL:A1009</oboInOwl:hasDbXref>
</owl:Class>

<owl:Class rdf:about="&obo;FOODON_03401010">
	<rdfs:label xml:lang="en">50101500 - vegetables - unprepared/unprocessed (gs1 gpc)</rdfs:label>
	<rdfs:subClassOf rdf:resource="&obo;FOODON_03400987"/>
	<obo:IAO_0000412>http://langual.org</obo:IAO_0000412>
	<obo:IAO_0000114 rdf:resource="&obo;IAO_0000428"/>
	<oboInOwl:hasDbXref>LANGUAL:A1010</oboInOwl:hasDbXref>
</owl:Class>

<owl:Class rdf:about="&obo;FOODON_03401011">
	<rdfs:label xml:lang="en">10000005 - vegetables - unprepared/unprocessed (frozen) (gs1 gpc)</rdfs:label>
	<rdfs:subClassOf rdf:resource="&obo;FOODON_03401010"/>
	<obo:IAO_0000412>http://langual.org</obo:IAO_0000412>
	<obo:IAO_0000115 xml:lang="en">Includes any products that can be described/observed as any variety of frozen vegetables, combination of vegetables or fruit vegetables, which may be whole, chopped, cleaned and trimmed, but has not gone through any further manufacturing processes, such as reformed, cooked, dried, salted or smoked, however these products can be coated, in sauce, stuffed or filled. Specifically excludes products that have added ingredients included such as rice, couscous and pasta. These products must be frozen to extend their consumable life. Excludes products such as Vegetables with additional dough or grains, Perishable and Shelf Stable Unprepared and Unprocessed Vegetable, all Prepared and Processed Vegetables.</obo:IAO_0000115>
	<obo:IAO_0000114 rdf:resource="&obo;IAO_0000428"/>
	<rdfs:comment xml:lang="en">LanguaL curation note: Index type of vegetable (alfalfa, yuca) in facet B. Index physical form (whole, chopped) in facet E. If an industry recognized organic certification is claimed, index ORGANIC FOOD CLAIM OR USE in facet P.</rdfs:comment>
	<oboInOwl:hasDbXref>LANGUAL:A1011</oboInOwl:hasDbXref>
</owl:Class>

<owl:Class rdf:about="&obo;FOODON_03401012">
	<rdfs:label xml:lang="en">10000004 - vegetables - unprepared/unprocessed (perishable) (gs1 gpc)</rdfs:label>
	<rdfs:subClassOf rdf:resource="&obo;FOODON_03401010"/>
	<obo:IAO_0000412>http://langual.org</obo:IAO_0000412>
	<obo:IAO_0000115 xml:lang="en">Includes any products that can be described/observed as any variety of fresh vegetables, combination of vegetables or fruit vegetables, which may be whole, chopped, cleaned and trimmed, but has not gone through any further manufacturing processes, such as reformed, cooked, dried, salted or smoked, however these products can be coated, in sauce, stuffed or filled. Specifically excludes products that have added ingredients included such as rice, couscous and pasta. These products can be/must be refrigerated to extend their consumable life. Excludes products such as Vegetables with additional dough or grains, Frozen and Shelf Stable Unprepared and Unprocessed Vegetable, all Prepared and Processed Vegetables.</obo:IAO_0000115>
	<obo:IAO_0000114 rdf:resource="&obo;IAO_0000428"/>
	<rdfs:comment xml:lang="en">LanguaL curation note: Index type of vegetable (alfalfa, yuca) in facet B. Index physical form (whole, chopped) in facet E. If an industry recognized organic certification is claimed, index ORGANIC FOOD CLAIM OR USE in facet P. Index preservation method (refrigeration) in facet J.</rdfs:comment>
	<oboInOwl:hasDbXref>LANGUAL:A1012</oboInOwl:hasDbXref>
</owl:Class>

<owl:Class rdf:about="&obo;FOODON_03401013">
	<rdfs:label xml:lang="en">10000006 - vegetables - unprepared/unprocessed (shelf stable) (gs1 gpc)</rdfs:label>
	<rdfs:subClassOf rdf:resource="&obo;FOODON_03401010"/>
	<obo:IAO_0000412>http://langual.org</obo:IAO_0000412>
	<obo:IAO_0000115 xml:lang="en">Includes any products that can be described/observed as any variety of vegetables, combination of vegetables or fruit vegetables, which may be whole, chopped, cleaned and trimmed, but has not gone through any further manufacturing processes, such as reformed, cooked, dried, salted or smoked, however these products can be coated, in sauce, stuffed or filled. Specifically excludes products that have added ingredients included such as rice, couscous and pasta. These products have been treated or packaged in such a way as to extend their consumable life. Excludes products such as Vegetables with additional dough or grains, Frozen and Perishable Unprepared and Unprocessed Vegetables, all Prepared and Processed Vegetables.</obo:IAO_0000115>
	<obo:IAO_0000114 rdf:resource="&obo;IAO_0000428"/>
	<rdfs:comment xml:lang="en">LanguaL curation note: Index type of vegetable (alfalfa, yuca) in facet B. Index physical form (whole, chopped) in facet E. If an industry recognized organic certification is claimed, index ORGANIC FOOD CLAIM OR USE in facet P.</rdfs:comment>
	<oboInOwl:hasDbXref>LANGUAL:A1013</oboInOwl:hasDbXref>
</owl:Class>

<owl:Class rdf:about="&obo;FOODON_03401014">
	<rdfs:label xml:lang="en">50102200 - fruits/vegetables/nuts/seeds variety packs (gs1 gpc)</rdfs:label>
	<rdfs:subClassOf rdf:resource="&obo;FOODON_03400987"/>
	<obo:IAO_0000412>http://langual.org</obo:IAO_0000412>
	<obo:IAO_0000115 xml:lang="en">Includes any products that can be described/observed as two or more distinct Fruits, Vegetables, Nuts and Seeds sold together which exist within the schema but belong to different classes, that is two or more products contained within the same pack which cross classes within the Fruits, Vegetables, Nuts and Seeds Family. Includes products such as Salad and Nuts variety packs. Items that are received free with purchases should be removed from the classification decision-making process. Excludes products such as Strawberries and Cream variety packs.</obo:IAO_0000115>
	<obo:IAO_0000114 rdf:resource="&obo;IAO_0000428"/>
	<oboInOwl:hasDbXref>LANGUAL:A1014</oboInOwl:hasDbXref>
</owl:Class>

<owl:Class rdf:about="&obo;FOODON_03401015">
	<rdfs:label xml:lang="en">50110000 - meat/poultry/game/batrachian (gs1 gpc)</rdfs:label>
	<rdfs:subClassOf rdf:resource="&obo;FOODON_03400874"/>
	<obo:IAO_0000412>http://langual.org</obo:IAO_0000412>
	<obo:IAO_0000114 rdf:resource="&obo;IAO_0000428"/>
	<oboInOwl:hasDbXref>LANGUAL:A1015</oboInOwl:hasDbXref>
</owl:Class>

<owl:Class rdf:about="&obo;FOODON_03401016">
	<rdfs:label xml:lang="en">50112000 - meat/poultry/game/batrachian - prepared/processed (gs1 gpc)</rdfs:label>
	<rdfs:subClassOf rdf:resource="&obo;FOODON_03401015"/>
	<obo:IAO_0000412>http://langual.org</obo:IAO_0000412>
	<obo:IAO_0000114 rdf:resource="&obo;IAO_0000428"/>
	<oboInOwl:hasDbXref>LANGUAL:A1016</oboInOwl:hasDbXref>
</owl:Class>

<owl:Class rdf:about="&obo;FOODON_03401017">
	<rdfs:label xml:lang="en">10000013 - meat/poultry/game/batrachian - prepared/processed (frozen) (gs1 gpc)</rdfs:label>
	<rdfs:subClassOf rdf:resource="&obo;FOODON_03401016"/>
	<obo:IAO_0000412>http://langual.org</obo:IAO_0000412>
	<obo:IAO_0000115 xml:lang="en">Includes any products that can be described/observed as meat, poultry, game, batrachian and protein-based alternatives to meat, often consisting of a soy or nut mixture, that has gone through further manufacturing processes such as, reformed, cooked and dried, however these products can also be coated, in sauce, stuffed or filled. Products include land snails but specifically exclude products that have added ingredients included such as rice, couscous and pasta. However products may contain a small quantity of vegetables such as those in a sauce or stuffing/filling. These products must be frozen to extend their consumable life. Excludes products such as Meat, Poultry, Game and Batrachian with additional vegetables, dough or grains, Shelf Stable and Perishable Prepared and Processed Meat, Poultry, Game, Batrachian and Substitutes, all Unprepared and Unprocessed Meat, Poultry, Game, Batrachian and Substitutes.</obo:IAO_0000115>
	<obo:IAO_0000114 rdf:resource="&obo;IAO_0000428"/>
	<rdfs:comment xml:lang="en">LanguaL curation note: Index type of meat (chicken, venison) in facet B. If an industry recognized organic certification is claimed, index ORGANIC FOOD CLAIM OR USE in facet P. Index part of animal (meat, offal) in facet C. Index meat cut (brisket, entrecote) in facet Z. Index packing medium (sauce) in facet K. Index manufacturer's treatments (stuffed, smoked) in facet H and heat treatment (cooked) in facet F.</rdfs:comment>
	<oboInOwl:hasDbXref>LANGUAL:A1017</oboInOwl:hasDbXref>
</owl:Class>

<owl:Class rdf:about="&obo;FOODON_03401018">
	<rdfs:label xml:lang="en">10000012 - meat/poultry/game/batrachian - prepared/processed (perishable) (gs1 gpc)</rdfs:label>
	<rdfs:subClassOf rdf:resource="&obo;FOODON_03401016"/>
	<obo:IAO_0000412>http://langual.org</obo:IAO_0000412>
	<obo:IAO_0000115 xml:lang="en">Includes any products that can be described/observed as meat, poultry, game, batrachian and protein-based alternatives to meat, often consisting of a soy or nut mixture, that has gone through further manufacturing processes such as, reformed, cooked, dried and cured, however these products can also be coated, in sauce, stuffed or filled. Products include land snails but specifically exclude products that have added ingredients included such as rice, couscous and pasta. However products may contain a small quantity of vegetables such as those in a sauce or stuffing/filling. These products must be refrigerated to extend their consumable life. Excludes products such as Meat, Poultry, Game and Batrachian with additional vegetables, dough or grains, Frozen and Shelf Stable Prepared and Processed Meat, Poultry, Game, Batrachian and Substitutes, all Unprepared and Unprocessed Meat, Poultry, Game, Batrachian and Substitutes.</obo:IAO_0000115>
	<obo:IAO_0000114 rdf:resource="&obo;IAO_0000428"/>
	<rdfs:comment xml:lang="en">LanguaL curation note: Index type of meat (chicken, venison) in facet B. If an industry recognized organic certification is claimed, index ORGANIC FOOD CLAIM OR USE in facet P. Index part of animal (meat, offal) in facet C. Index meat cut (brisket, entrecote) in facet Z. Index packing medium (sauce) in facet K. Index manufacturer's treatments (stuffed, smoked) in facet H and heat treatment (cooked) in facet F. Index preservation method (refrigeration) in facet J.</rdfs:comment>
	<oboInOwl:hasDbXref>LANGUAL:A1018</oboInOwl:hasDbXref>
</owl:Class>

<owl:Class rdf:about="&obo;FOODON_03401019">
	<rdfs:label xml:lang="en">10000014 - meat/poultry/game/batrachian - prepared/processed (shelf stable) (gs1 gpc)</rdfs:label>
	<rdfs:subClassOf rdf:resource="&obo;FOODON_03401016"/>
	<obo:IAO_0000412>http://langual.org</obo:IAO_0000412>
	<obo:IAO_0000115 xml:lang="en">Includes any products that can be described/observed as meat, poultry, game, batrachian and protein-based alternatives to meat, often consisting of a soy or nut mixture, that has gone through further manufacturing processes such as, reformed, cooked, dried and cured, however these products can also be coated, in sauce, stuffed or filled. Products include land snails but specifically exclude products that have added ingredients included such as rice, couscous and pasta. However products may contain a small quantity of vegetables such as those in a sauce or stuffing/filling. These products have been treated or packaged in such a way as to extend their consumable life. Excludes products such as Meat, Poultry, Game and Batrachian with additional vegetables, dough or grains, Frozen and Perishable Prepared and Processed Meat, Poultry, Game, Batrachian and Substitutes, all Unprepared and Unprocessed Meat, Poultry, Game, Batrachian and Substitutes.</obo:IAO_0000115>
	<obo:IAO_0000114 rdf:resource="&obo;IAO_0000428"/>
	<rdfs:comment xml:lang="en">LanguaL curation note: Index type of meat (chicken, venison) in facet B. If an industry recognized organic certification is claimed, index ORGANIC FOOD CLAIM OR USE in facet P. Index part of animal (meat, offal) in facet C. Index meat cut (brisket, entrecote) in facet Z. Index packing medium (sauce) in facet K. Index manufacturer's treatments (stuffed, smoked) in facet H and heat treatment (cooked) in facet F.</rdfs:comment>
	<oboInOwl:hasDbXref>LANGUAL:A1019</oboInOwl:hasDbXref>
</owl:Class>

<owl:Class rdf:about="&obo;FOODON_03401020">
	<rdfs:label xml:lang="en">50111500 - meat/poultry/game/batrachian - unprepared/unprocessed (gs1 gpc)</rdfs:label>
	<rdfs:subClassOf rdf:resource="&obo;FOODON_03401015"/>
	<obo:IAO_0000412>http://langual.org</obo:IAO_0000412>
	<obo:IAO_0000114 rdf:resource="&obo;IAO_0000428"/>
	<oboInOwl:hasDbXref>LANGUAL:A1020</oboInOwl:hasDbXref>
</owl:Class>

<owl:Class rdf:about="&obo;FOODON_03401021">
	<rdfs:label xml:lang="en">10000010 - meat/poultry/game/batrachian - unprepared/unprocessed (frozen) (gs1 gpc)</rdfs:label>
	<rdfs:subClassOf rdf:resource="&obo;FOODON_03401020"/>
	<obo:IAO_0000412>http://langual.org</obo:IAO_0000412>
	<obo:IAO_0000115 xml:lang="en">Includes any products that can be described/observed as meat, poultry, game, batrachian and protein-based alternatives to meat, often consisting of a soy or nut mixture, that has not gone through any further manufacturing process such as, reformed, cooked, dried and cured, however these products can be coated, in sauce, stuffed or filled. Products include land snails but specifically exclude products that have added ingredients included such as rice, couscous and pasta. However products may contain a small quantity of vegetables such as those in a sauce or stuffing/filling. These products must be frozen to extend their consumable life. Excludes products such as Meat, Poultry, Game and Batrachian with additional vegetables, dough or grains, Shelf Stable and Perishable Unprepared and Unprocessed Meat, Poultry, Game, Batrachian and Substitutes, all Prepared and Processed Meat, Poultry, Game, Batrachian and Substitutes.</obo:IAO_0000115>
	<obo:IAO_0000114 rdf:resource="&obo;IAO_0000428"/>
	<rdfs:comment xml:lang="en">LanguaL curation note: Index type of meat (chicken, venison) in facet B. If an industry recognized organic certification is claimed, index ORGANIC FOOD CLAIM OR USE in facet P. Index part of animal (meat with bone or boneless, offal) in facet C. Index meat cut (brisket, entrecote) in facet Z.</rdfs:comment>
	<oboInOwl:hasDbXref>LANGUAL:A1021</oboInOwl:hasDbXref>
</owl:Class>

<owl:Class rdf:about="&obo;FOODON_03401022">
	<rdfs:label xml:lang="en">10000009 - meat/poultry/game/batrachian - unprepared/unprocessed (perishable) (gs1 gpc)</rdfs:label>
	<rdfs:subClassOf rdf:resource="&obo;FOODON_03401020"/>
	<obo:IAO_0000412>http://langual.org</obo:IAO_0000412>
	<obo:IAO_0000115 xml:lang="en">Includes any products that can be described/observed as meat, poultry, game, batrachian and protein-based alternatives to meat, often consisting of a soy or nut mixture, that has not gone through any further manufacturing processes such as, reformed, cooked, dried and cured, however these products can be coated, in sauce, stuffed or filled. Products include land snails but specifically exclude products that have added ingredients included such as rice, couscous and pasta. However products may contain a small quantity of vegetables such as those in a sauce or stuffing/filling. These products must be refrigerated to extend their consumable life. Excludes products such as Meat, Poultry, Game and Batrachian with additional vegetables, dough or grains, Shelf Stable and Frozen Unprepared and Unprocessed Meat, Poultry, Game, Batrachian and Substitutes, all Prepared and Processed Meat, Poultry, Game, Batrachian and Substitutes.</obo:IAO_0000115>
	<obo:IAO_0000114 rdf:resource="&obo;IAO_0000428"/>
	<rdfs:comment xml:lang="en">LanguaL curation note: Index type of meat (chicken, venison) in facet B. If an industry recognized organic certification is claimed, index ORGANIC FOOD CLAIM OR USE in facet P. Index part of animal (meat with bone or boneless, offal) in facet C. Index meat cut (brisket, entrecote) in facet Z.  Index preservation method (refrigeration) in facet J.</rdfs:comment>
	<oboInOwl:hasDbXref>LANGUAL:A1022</oboInOwl:hasDbXref>
</owl:Class>

<owl:Class rdf:about="&obo;FOODON_03401023">
	<rdfs:label xml:lang="en">10000011 - meat/poultry/game/batrachian - unprepared/unprocessed (shelf stable) (gs1 gpc)</rdfs:label>
	<rdfs:subClassOf rdf:resource="&obo;FOODON_03401020"/>
	<obo:IAO_0000412>http://langual.org</obo:IAO_0000412>
	<obo:IAO_0000115 xml:lang="en">Includes any products that can be described/observed as meat, poultry, game, batrachian and protein-based alternatives to meat, often consisting of a soy or nut mixture, that has not gone through any further manufacturing processes such as, reformed, cooked, dried and cured, however these products can be coated, in sauce, stuffed or filled. Products include land snails but specifically exclude products that have added ingredients included such as rice, couscous and pasta. However products may contain a small quantity of vegetables such as those in a sauce or stuffing/filling. These products have been treated or packaged in such a way as to extend their consumable life. Excludes products such as Meat, Poultry, Game and Batrachian with additional vegetables, dough or grains, Frozen and Perishable Unprepared and Unprocessed Meat, Poultry, Game, Batrachian and Substitutes, all Prepared and Processed Meat, Poultry, Game, Batrachian and Substitutes.</obo:IAO_0000115>
	<obo:IAO_0000114 rdf:resource="&obo;IAO_0000428"/>
	<rdfs:comment xml:lang="en">LanguaL curation note: Index type of meat (chicken, venison) in facet B. If an industry recognized organic certification is claimed, index ORGANIC FOOD CLAIM OR USE in facet P. Index part of animal (meat with bone or boneless, offal) in facet C. Index meat cut (brisket, entrecote) in facet Z.</rdfs:comment>
	<oboInOwl:hasDbXref>LANGUAL:A1023</oboInOwl:hasDbXref>
</owl:Class>

<owl:Class rdf:about="&obo;FOODON_03401024">
	<rdfs:label xml:lang="en">50112100 - meat/poultry/game/batrachian variety packs (gs1 gpc)</rdfs:label>
	<rdfs:subClassOf rdf:resource="&obo;FOODON_03401015"/>
	<obo:IAO_0000412>http://langual.org</obo:IAO_0000412>
	<obo:IAO_0000115 xml:lang="en">Includes any products that can be described/observed as two or more distinct Meat, Poultry, Game and Batrachian products sold together which exist within the schema but belong to different classes, that is two or more products contained within the same pack which cross classes within the Meat, Poultry, Game and Batrachian Family. Includes products such as hampers of cooked red meats with unprepared and unprocessed Game. Items that are received free with purchases should be removed from the classification decision-making process. Excludes products such as Meat and Relish variety packs.</obo:IAO_0000115>
	<obo:IAO_0000114 rdf:resource="&obo;IAO_0000428"/>
	<oboInOwl:hasDbXref>LANGUAL:A1024</oboInOwl:hasDbXref>
</owl:Class>

<owl:Class rdf:about="&obo;FOODON_03401025">
	<rdfs:label xml:lang="en">50130000 - milk/butter/cream/yoghurts/cheese/eggs/substitutes (gs1 gpc)</rdfs:label>
	<rdfs:subClassOf rdf:resource="&obo;FOODON_03400874"/>
	<obo:IAO_0000412>http://langual.org</obo:IAO_0000412>
	<obo:IAO_0000114 rdf:resource="&obo;IAO_0000428"/>
	<oboInOwl:hasDbXref>LANGUAL:A1025</oboInOwl:hasDbXref>
</owl:Class>

<owl:Class rdf:about="&obo;FOODON_03401026">
	<rdfs:label xml:lang="en">50131900 - butter/butter substitutes (gs1 gpc)</rdfs:label>
	<rdfs:subClassOf rdf:resource="&obo;FOODON_03401025"/>
	<obo:IAO_0000412>http://langual.org</obo:IAO_0000412>
	<obo:IAO_0000114 rdf:resource="&obo;IAO_0000428"/>
	<oboInOwl:hasDbXref>LANGUAL:A1026</oboInOwl:hasDbXref>
</owl:Class>

<owl:Class rdf:about="&obo;FOODON_03401027">
	<rdfs:label xml:lang="en">10000167 - butter/butter substitutes (frozen) (gs1 gpc)</rdfs:label>
	<rdfs:subClassOf rdf:resource="&obo;FOODON_03401026"/>
	<obo:IAO_0000412>http://langual.org</obo:IAO_0000412>
	<obo:IAO_0000115 xml:lang="en">Includes any products that can be described/observed as either the fatty portion of animal milk, separated when milk or cream is agitated or churned, or a spread made from vegetable or a combination of vegetable and animal fats that is specifically marketed and labelled as margarine. These products must be frozen to extend their consumable life. Excludes products such as Shelf Stable or Perishable Butter and Butter Substitutes and all Vegetable and Animal Cooking Oils and Fats.</obo:IAO_0000115>
	<obo:IAO_0000114 rdf:resource="&obo;IAO_0000428"/>
	<rdfs:comment xml:lang="en">LanguaL curation note: Index the source of the product (animal, vegetable, combination, unidentified) in facet B. Index physical form (liquid/spray, solid) in facet E. Index the types of manufacturers treatment/cooking process the product has undergone (flavoured, salted) in facet H. Index the fat claim (full fat, reduced fat, low fat) and organic claim in Facet P.</rdfs:comment>
	<oboInOwl:hasDbXref>LANGUAL:A1027</oboInOwl:hasDbXref>
</owl:Class>

<owl:Class rdf:about="&obo;FOODON_03401028">
	<rdfs:label xml:lang="en">10000168 - butter/butter substitutes (perishable) (gs1 gpc)</rdfs:label>
	<rdfs:subClassOf rdf:resource="&obo;FOODON_03401026"/>
	<obo:IAO_0000412>http://langual.org</obo:IAO_0000412>
	<obo:IAO_0000115 xml:lang="en">Includes any products that can be described/observed as either the fatty portion of animal milk, separated when milk or cream is agitated or churned, or a spread made from vegetable or a combination of vegetable and animal fats that is specifically marketed and labelled as margarine. These products must be refrigerated to extend their consumable life. Excludes products such as Shelf Stable or Frozen Butter and Butter Based Substitutes, and all Vegetable and Animal Cooking Oils and Fats.</obo:IAO_0000115>
	<obo:IAO_0000114 rdf:resource="&obo;IAO_0000428"/>
	<rdfs:comment xml:lang="en">LanguaL curation note: Index the source of the product (animal, vegetable, combination, unidentified) in facet B. Index physical form (liquid/spray, solid) in facet E. Index the types of manufacturers treatment/cooking process the product has undergone (flavoured, salted) in facet H. Index the fat claim (full fat, reduced fat, low fat) and organic claim in Facet P. Index preservation method (refrigeration) in facet J.</rdfs:comment>
	<oboInOwl:hasDbXref>LANGUAL:A1028</oboInOwl:hasDbXref>
</owl:Class>

<owl:Class rdf:about="&obo;FOODON_03401029">
	<rdfs:label xml:lang="en">10000169 - butter/butter substitutes (shelf stable) (gs1 gpc)</rdfs:label>
	<rdfs:subClassOf rdf:resource="&obo;FOODON_03401026"/>
	<obo:IAO_0000412>http://langual.org</obo:IAO_0000412>
	<obo:IAO_0000115 xml:lang="en">Includes any products that can be described/observed as either the fatty portion of animal milk, separated when milk or cream is agitated or churned, or a spread made from vegetable or a combination of vegetable and animal fats that is specifically marketed and labelled as margarine. These products have been treated or packaged in such a way as to extend their consumable life. Excludes products such as Perishable or Frozen Butter and Butter Substitutes, and all Vegetable and Animal Cooking Oils and Fats.</obo:IAO_0000115>
	<obo:IAO_0000114 rdf:resource="&obo;IAO_0000428"/>
	<rdfs:comment xml:lang="en">LanguaL curation note: Index the source of the product (animal, vegetable, combination, unidentified) in facet B. Index physical form (liquid/spray, solid) in facet E. Index the types of manufacturers treatment/cooking process the product has undergone (flavoured, salted) in facet H. Index the fat claim (full fat, reduced fat, low fat) and organic claim in Facet P.</rdfs:comment>
	<oboInOwl:hasDbXref>LANGUAL:A1029</oboInOwl:hasDbXref>
</owl:Class>

<owl:Class rdf:about="&obo;FOODON_03401030">
	<rdfs:label xml:lang="en">50131800 - cheese/cheese substitutes (gs1 gpc)</rdfs:label>
	<rdfs:subClassOf rdf:resource="&obo;FOODON_03401025"/>
	<obo:IAO_0000412>http://langual.org</obo:IAO_0000412>
	<obo:IAO_0000114 rdf:resource="&obo;IAO_0000428"/>
	<oboInOwl:hasDbXref>LANGUAL:A1030</oboInOwl:hasDbXref>
</owl:Class>

<owl:Class rdf:about="&obo;FOODON_03401031">
	<rdfs:label xml:lang="en">10000030 - cheese/cheese substitutes (frozen) (gs1 gpc)</rdfs:label>
	<rdfs:subClassOf rdf:resource="&obo;FOODON_03401030"/>
	<obo:IAO_0000412>http://langual.org</obo:IAO_0000412>
	<obo:IAO_0000115 xml:lang="en">Includes any products that can be described/observed as frozen food made from the curd of milk, separated from the whey, sometimes fermented, and usually pressed, cooked, smoked, matured, or heated and mixed with artificial ingredients, such as emulsifiers, colourings and flavourings. These products must be frozen to extend their consumable life. These products include natural, processed cheese and substitutes, cheese with added ingredients, such as herbs and nuts, in blocks, rolls, slices, grated, cubes, spreadable and portions. Excludes products such as Shelf Stable and Perishable Cheeses and Cheese Substitutes and Cheese-Based/Flavoured Meals and Fromage Frais.</obo:IAO_0000115>
	<obo:IAO_0000114 rdf:resource="&obo;IAO_0000428"/>
	<rdfs:comment xml:lang="en">LanguaL curation note: Index the source of the product (cow, soy, etc.) in facet B.  Index the fat claim (full fat, reduced fat, low fat) and organic claim in Facet P. Index in facet H the type of manufacturers treatment the product has undergone. Index the geographical origin of the cheese in Facet R. Cheese may be further indexed using Codex classification of cheese by hardness (SOFT CHEESE, HARAD CHEESE, etc.) in facet A.</rdfs:comment>
	<oboInOwl:hasDbXref>LANGUAL:A1031</oboInOwl:hasDbXref>
</owl:Class>

<owl:Class rdf:about="&obo;FOODON_03401032">
	<rdfs:label xml:lang="en">10000028 - cheese/cheese substitutes (perishable) (gs1 gpc)</rdfs:label>
	<rdfs:subClassOf rdf:resource="&obo;FOODON_03401030"/>
	<obo:IAO_0000412>http://langual.org</obo:IAO_0000412>
	<obo:IAO_0000115 xml:lang="en">Includes any products that can be described/observed as food made from the curd of milk, separated from the whey, sometimes fermented, and usually pressed, cooked, smoked, matured, or heated and mixed with artificial ingredients, such as emulsifiers, colourings and flavourings. These products must be refrigerated to extend their consumable life. These products include natural, processed cheese and substitutes, cheese with added ingredients, such as herbs and nuts, in blocks, rolls, slices, grated, cubes, spreadable and portions. Excludes products such as Shelf Stable and Frozen Cheeses and Cheese Substitutes and Cheese-Based/Flavoured Meals and Fromage Frais.</obo:IAO_0000115>
	<obo:IAO_0000114 rdf:resource="&obo;IAO_0000428"/>
	<rdfs:comment xml:lang="en">LanguaL curation note: Index the source of the product (cow, soy, etc.) in facet B.  Index the fat claim (full fat, reduced fat, low fat) and organic claim in Facet P. Index in facet H the type of manufacturers treatment the product has undergone. Index the geographical origin of the cheese in Facet R. Index preservation method (refrigeration) in facet J. Cheese may be further indexed using Codex classification of cheese by hardness (SOFT CHEESE, HARAD CHEESE, etc.) in facet A.</rdfs:comment>
	<oboInOwl:hasDbXref>LANGUAL:A1032</oboInOwl:hasDbXref>
</owl:Class>

<owl:Class rdf:about="&obo;FOODON_03401033">
	<rdfs:label xml:lang="en">10000029 - cheese/cheese substitutes (shelf stable) (gs1 gpc)</rdfs:label>
	<rdfs:subClassOf rdf:resource="&obo;FOODON_03401030"/>
	<obo:IAO_0000412>http://langual.org</obo:IAO_0000412>
	<obo:IAO_0000115 xml:lang="en">Includes any products that can be described/observed as food made from the curd of milk, separated from the whey, sometimes fermented, and usually pressed, cooked, smoked, matured, or heated and mixed with artificial ingredients, such as emulsifiers, colourings and flavourings. These products have been treated or packaged in such a way as to extend their consumable life. These products include natural, processed cheese and substitutes, cheese with added ingredients, such as herbs and nuts, in blocks, rolls, slices, grated, cubes, spreadable and portions. Excludes products such as Frozen and Perishable Cheeses and Cheese Substitutes and Cheese-Based/Flavoured Meals and Fromage Frais.</obo:IAO_0000115>
	<obo:IAO_0000114 rdf:resource="&obo;IAO_0000428"/>
	<rdfs:comment xml:lang="en">LanguaL curation note: Index the source of the product (cow, soy, etc.) in facet B.  Index the fat claim (full fat, reduced fat, low fat) and organic claim in Facet P. Index in facet H the type of manufacturers treatment the product has undergone. Index the geographical origin of the cheese in Facet R. Cheese may be further indexed using Codex classification of cheese by hardness (SOFT CHEESE, HARAD CHEESE, etc.) in facet A.</rdfs:comment>
	<oboInOwl:hasDbXref>LANGUAL:A1033</oboInOwl:hasDbXref>
</owl:Class>

<owl:Class rdf:about="&obo;FOODON_03401034">
	<rdfs:label xml:lang="en">50132000 - cream/cream substitutes (gs1 gpc)</rdfs:label>
	<rdfs:subClassOf rdf:resource="&obo;FOODON_03401025"/>
	<obo:IAO_0000412>http://langual.org</obo:IAO_0000412>
	<obo:IAO_0000114 rdf:resource="&obo;IAO_0000428"/>
	<oboInOwl:hasDbXref>LANGUAL:A1034</oboInOwl:hasDbXref>
</owl:Class>

<owl:Class rdf:about="&obo;FOODON_03401035">
	<rdfs:label xml:lang="en">10000188 - cream/cream substitutes (frozen) (gs1 gpc)</rdfs:label>
	<rdfs:subClassOf rdf:resource="&obo;FOODON_03401034"/>
	<obo:IAO_0000412>http://langual.org</obo:IAO_0000412>
	<obo:IAO_0000115 xml:lang="en">Includes any products that can be described/observed as frozen dairy cream (the fatty part of fresh milk that rises to the top if allowed to stand), or non-dairy cream, usually made from vegetable oils and buttermilk, with stabilizers and emulsifiers, which is specifically designed and marketed to replicate natural cream. These products must be frozen to extend their consumable life. Products include cream with added flavouring or ingredients, such as fruit and chocolate. Excludes products such as Shelf Stable and Perishable Cream and Cream Substitutes.</obo:IAO_0000115>
	<obo:IAO_0000114 rdf:resource="&obo;IAO_0000428"/>
	<rdfs:comment xml:lang="en">LanguaL curation note: Index the source of the product (cow, soy, etc.) in facet B. Index fat claim (full fat, reduced fat, low fat) and organic claim in Facet P. Index in facet H the types of manufacturers treatment the product has undergone (fermented, homogenised).</rdfs:comment>
	<oboInOwl:hasDbXref>LANGUAL:A1035</oboInOwl:hasDbXref>
</owl:Class>

<owl:Class rdf:about="&obo;FOODON_03401036">
	<rdfs:label xml:lang="en">10000189 - cream/cream substitutes (perishable) (gs1 gpc)</rdfs:label>
	<rdfs:subClassOf rdf:resource="&obo;FOODON_03401034"/>
	<obo:IAO_0000412>http://langual.org</obo:IAO_0000412>
	<obo:IAO_0000115 xml:lang="en">Includes any products that can be described/observed as dairy cream (the fatty part of fresh milk that rises to the top if allowed to stand), or non-dairy cream, usually made from vegetable oils and buttermilk, with stabilisers and emulsifiers, which is specifically designed and marketed to replicate natural cream. These products must be refrigerated to extend their consumable life. These products can have added flavour or ingredients, such as fruit and chocolate. Excludes products such as Frozen and Shelf Stable Cream and Cream Substitutes.</obo:IAO_0000115>
	<obo:IAO_0000114 rdf:resource="&obo;IAO_0000428"/>
	<rdfs:comment xml:lang="en">LanguaL curation note: Index the source of the product (cow, soy, etc.) in facet B. Index fat claim (full fat, reduced fat, low fat) and organic claim in Facet P. Index in facet H the types of manufacturers treatment the product has undergone (fermented, homogenised). Index preservation method (refrigeration) in facet J.</rdfs:comment>
	<oboInOwl:hasDbXref>LANGUAL:A1036</oboInOwl:hasDbXref>
</owl:Class>

<owl:Class rdf:about="&obo;FOODON_03401037">
	<rdfs:label xml:lang="en">10000190 - cream/cream substitutes (shelf stable) (gs1 gpc)</rdfs:label>
	<rdfs:subClassOf rdf:resource="&obo;FOODON_03401034"/>
	<obo:IAO_0000412>http://langual.org</obo:IAO_0000412>
	<obo:IAO_0000115 xml:lang="en">Includes any products that can be described/observed as dairy cream (the fatty part of fresh milk that rises to the top if allowed to stand), or non-dairy cream, usually made from vegetable oils and buttermilk, with stabilizers and emulsifiers, which is specifically designed and marketed to replicate natural cream. These products have been treated or packaged in such a way as to extend their consumable life. Products include cream with added flavouring or ingredients, such as fruit and chocolate and frothy style beverage toppings Excludes products such as Frozen and Perishable Cream and Cream Substitutes.</obo:IAO_0000115>
	<obo:IAO_0000114 rdf:resource="&obo;IAO_0000428"/>
	<rdfs:comment xml:lang="en">LanguaL curation note: Index the source of the product (cow, soy, etc.) in facet B. Index fat claim (full fat, reduced fat, low fat) and organic claim in Facet P. Index in facet H the types of manufacturers treatment the product has undergone (fermented, homogenised).</rdfs:comment>
	<oboInOwl:hasDbXref>LANGUAL:A1037</oboInOwl:hasDbXref>
</owl:Class>

<owl:Class rdf:about="&obo;FOODON_03401038">
	<rdfs:label xml:lang="en">50131600 - eggs/egg substitutes (gs1 gpc)</rdfs:label>
	<rdfs:subClassOf rdf:resource="&obo;FOODON_03401025"/>
	<obo:IAO_0000412>http://langual.org</obo:IAO_0000412>
	<obo:IAO_0000114 rdf:resource="&obo;IAO_0000428"/>
	<oboInOwl:hasDbXref>LANGUAL:A1038</oboInOwl:hasDbXref>
</owl:Class>

<owl:Class rdf:about="&obo;FOODON_03401039">
	<rdfs:label xml:lang="en">10000582 - eggs/eggs substitutes (frozen) (gs1 gpc)</rdfs:label>
	<rdfs:subClassOf rdf:resource="&obo;FOODON_03401038"/>
	<obo:IAO_0000412>http://langual.org</obo:IAO_0000412>
	<obo:IAO_0000115 xml:lang="en">Includes any products that can be described/observed as an egg produced by female fowl of various shell sizes and colours or an egg substitute that is specifically labelled and marketed to replicate natural eggs. These products must be frozen to extend their consumable life. Products include whole frozen eggs, frozen whites and yolks sold separately. Excludes products such as Shelf Stable and Perishable Eggs and Eggs Substitutes and Egg-Based Meals.</obo:IAO_0000115>
	<obo:IAO_0000114 rdf:resource="&obo;IAO_0000428"/>
	<rdfs:comment xml:lang="en">LanguaL curation note: Index the source of the product (hen, quail, etc.) in facet B. Index the part of egg (whole, yolk, white) in facet C. Index in facet H the types of manufacturers treatment the product has undergone (filled, flavoured, salted), in facet E its physical form (sliced), and in facet F any heat treatment (cooked). Index Food Quality/Food Assurance Claim in facet P.</rdfs:comment>
	<oboInOwl:hasDbXref>LANGUAL:A1039</oboInOwl:hasDbXref>
</owl:Class>

<owl:Class rdf:about="&obo;FOODON_03401040">
	<rdfs:label xml:lang="en">10000031 - eggs/eggs substitutes (perishable) (gs1 gpc)</rdfs:label>
	<rdfs:subClassOf rdf:resource="&obo;FOODON_03401038"/>
	<obo:IAO_0000412>http://langual.org</obo:IAO_0000412>
	<obo:IAO_0000115 xml:lang="en">Includes any products that can be described/observed as an egg produced by female fowl of various shell sizes and colours or an egg substitute that is specifically labelled and marketed to replicate natural eggs. These products can be/must be refrigerated to extend their consumable life. Products include chicken, duck and quail eggs. Excludes products such as Shelf Stable and Frozen Eggs and Eggs Substitutes and Egg-Based Meals.</obo:IAO_0000115>
	<obo:IAO_0000114 rdf:resource="&obo;IAO_0000428"/>
	<rdfs:comment xml:lang="en">LanguaL curation note: Index the source of the product (hen, quail, etc.) in facet B. Index the part of egg (whole, yolk, white) in facet C. Index in facet H the types of manufacturers treatment the product has undergone (filled, flavoured, salted), in facet E its physical form (sliced), and in facet F any heat treatment (cooked). Index Food Quality/Food Assurance Claim in facet P. Index preservation method (refrigeration) in facet J.</rdfs:comment>
	<oboInOwl:hasDbXref>LANGUAL:A1040</oboInOwl:hasDbXref>
</owl:Class>

<owl:Class rdf:about="&obo;FOODON_03401041">
	<rdfs:label xml:lang="en">10000032 - eggs/eggs substitutes (shelf stable) (gs1 gpc)</rdfs:label>
	<rdfs:subClassOf rdf:resource="&obo;FOODON_03401038"/>
	<obo:IAO_0000412>http://langual.org</obo:IAO_0000412>
	<obo:IAO_0000115 xml:lang="en">Includes any products that can be described/observed as any egg produced by female fowl or an egg substitute that is specifically labelled and marketed to replicate natural eggs. These products have been treated or packaged in such a way as to extend their consumable life. Includes dried and pickled eggs. Excludes products such as Frozen and Perishable Eggs and Eggs Substitutes and Egg-Based Meals.</obo:IAO_0000115>
	<obo:IAO_0000114 rdf:resource="&obo;IAO_0000428"/>
	<rdfs:comment xml:lang="en">LanguaL curation note: Index the source of the product (hen, quail, etc.) in facet B. Index the part of egg (whole, yolk, white) in facet C. Index in facet H the types of manufacturers treatment the product has undergone (filled, flavoured, salted), in facet E its physical form (sliced), and in facet F any heat treatment (cooked). Index preservation method (pasteurised) in facet J and packing medium (oil, vinegar) in facet K.</rdfs:comment>
	<oboInOwl:hasDbXref>LANGUAL:A1041</oboInOwl:hasDbXref>
</owl:Class>

<owl:Class rdf:about="&obo;FOODON_03401042">
	<rdfs:label xml:lang="en">50131700 - milk/milk substitutes (gs1 gpc)</rdfs:label>
	<rdfs:subClassOf rdf:resource="&obo;FOODON_03401025"/>
	<obo:IAO_0000412>http://langual.org</obo:IAO_0000412>
	<obo:IAO_0000114 rdf:resource="&obo;IAO_0000428"/>
	<oboInOwl:hasDbXref>LANGUAL:A1042</oboInOwl:hasDbXref>
</owl:Class>

<owl:Class rdf:about="&obo;FOODON_03401043">
	<rdfs:label xml:lang="en">10000027 - milk/milk substitutes (frozen) (gs1 gpc)</rdfs:label>
	<rdfs:subClassOf rdf:resource="&obo;FOODON_03401042"/>
	<obo:IAO_0000412>http://langual.org</obo:IAO_0000412>
	<obo:IAO_0000115 xml:lang="en">Includes any products that can be described/observed as frozen unflavoured milk derived from animals, such as cow, goat and buffalo, and vegetable-based milk, naturally derived from fruit or vegetables, such as coconut milk and almond milk or vegetable proteins such as soya milk. These products must be frozen to extend their consumable life. Products include those that have been homogenized and pasteurized, but not to artificially extend their shelf life. Specifically excludes all fermented milk (or milk substitute) based beverages. Excludes products such as Shelf Stable and Perishable Milk and Milk Substitutes and Baby and Infant Specialized Beverages and Formula.</obo:IAO_0000115>
	<obo:IAO_0000114 rdf:resource="&obo;IAO_0000428"/>
	<rdfs:comment xml:lang="en">LanguaL curation note: Index the source of the product (cow,soy) in facet B. Index in facet H the types of manufacturers treatment the product has undergone (dehydrated, condensed). Index the manufacturer's fat claim (full fat, reduced fat, low fat) and organic claim in facet P.</rdfs:comment>
	<oboInOwl:hasDbXref>LANGUAL:A1043</oboInOwl:hasDbXref>
</owl:Class>

<owl:Class rdf:about="&obo;FOODON_03401044">
	<rdfs:label xml:lang="en">10000025 - milk/milk substitutes (perishable) (gs1 gpc)</rdfs:label>
	<rdfs:subClassOf rdf:resource="&obo;FOODON_03401042"/>
	<obo:IAO_0000412>http://langual.org</obo:IAO_0000412>
	<obo:IAO_0000115 xml:lang="en">Includes any products that can be described/observed as unflavoured milk derived from animals, such as cow, goat and buffalo, and vegetable-based milk, naturally derived from fruit or vegetables, such as coconut milk and almond milk or vegetable proteins such as soya milk. Products include those, which have been inoculated with live acidophilus and bifidus bacteria, but have been kept at the temperature which is too cool for such bacteria to develop, and have not therefore been fermented and retain the flavour of natural milk. These products must be refrigerated to extend their consumable life. Specifically excludes all fermented milk (or milk substitute) based beverages. Excludes products such as Frozen and Shelf Stable Milk and Milk Substitutes and Baby and Infant Specialized Beverage and Formula.</obo:IAO_0000115>
	<obo:IAO_0000114 rdf:resource="&obo;IAO_0000428"/>
	<rdfs:comment xml:lang="en">LanguaL curation note: Index the source of the product (cow,soy) in facet B. Index in facet H the types of manufacturers treatment the product has undergone (dehydrated, condensed). Index the manufacturer's fat claim (full fat, reduced fat, low fat) probiotic claim and organic claim in facet P. Index preservation method (refrigeration) in facet J.</rdfs:comment>
	<oboInOwl:hasDbXref>LANGUAL:A1044</oboInOwl:hasDbXref>
</owl:Class>

<owl:Class rdf:about="&obo;FOODON_03401045">
	<rdfs:label xml:lang="en">10000026 - milk/milk substitutes (shelf stable) (gs1 gpc)</rdfs:label>
	<rdfs:subClassOf rdf:resource="&obo;FOODON_03401042"/>
	<obo:IAO_0000412>http://langual.org</obo:IAO_0000412>
	<obo:IAO_0000115 xml:lang="en">Includes any products that can be described/observed as unflavoured milk derived from animals, such as cow, goat and buffalo, and vegetable-based milk, naturally derived from fruit or vegetables, such as coconut milk and almond milk or vegetable proteins such as soy milk. These products have been treated or packaged in such a way as to extend their consumable life. Products include evaporated milk, condensed milk and UHT treated milk. Specifically excludes all fermented milk (or milk substitute) based beverages. Excludes products such as Frozen and Perishable Milk and Milk Substitutes and Baby and Infant Specialised Beverages and Formula.</obo:IAO_0000115>
	<obo:IAO_0000114 rdf:resource="&obo;IAO_0000428"/>
	<rdfs:comment xml:lang="en">LanguaL curation note: Index the source of the product (cow,soy) in facet B. Index in facet H the types of manufacturers treatment (condensed, dehydrated) the product has undergone. Index the manufacturer's fat claim (full fat, reduced fat, low fat) probiotic claim and organic claim in facet P. Index preservation method (UHT, dehydrated) in facet J.</rdfs:comment>
	<oboInOwl:hasDbXref>LANGUAL:A1045</oboInOwl:hasDbXref>
</owl:Class>

<owl:Class rdf:about="&obo;FOODON_03401046">
	<rdfs:label xml:lang="en">50132100 - yoghurt/yoghurt substitutes (gs1 gpc)</rdfs:label>
	<rdfs:subClassOf rdf:resource="&obo;FOODON_03401025"/>
	<obo:IAO_0000412>http://langual.org</obo:IAO_0000412>
	<obo:IAO_0000114 rdf:resource="&obo;IAO_0000428"/>
	<oboInOwl:hasDbXref>LANGUAL:A1046</oboInOwl:hasDbXref>
</owl:Class>

<owl:Class rdf:about="&obo;FOODON_03401047">
	<rdfs:label xml:lang="en">10000277 - yoghurt/yoghurt substitutes (frozen) (gs1 gpc)</rdfs:label>
	<rdfs:subClassOf rdf:resource="&obo;FOODON_03401046"/>
	<obo:IAO_0000412>http://langual.org</obo:IAO_0000412>
	<obo:IAO_0000115 xml:lang="en">Includes any products that can be described/observed as a frozen food made from animal milk or non-animal milk, thickened by fermentation with lactic bacteria. Products include spoonable yogurt and fromage frais. These products must be frozen to extend their consumable life. Products include yogurt derived from an animal and yogurt derived from a plant, soy, almond, coconut. Also include yogurt flavoured with fruit, vanilla, nuts and honey, or packaged with a small amount of fruit preserve, nuts, or other accompaniment. Excludes products such as Drinking Yogurt, Shelf Stable and Perishable Yogurt and Yogurt Substitutes, Dairy and Dairy Substitute Drinks and Desserts.</obo:IAO_0000115>
	<obo:IAO_0000114 rdf:resource="&obo;IAO_0000428"/>
	<rdfs:comment xml:lang="en">LanguaL curation note: Index source of product (dairy, non dairy) in facet B. Index added ingredients (cereals, fruit pulp, sugar, flavouring) in facet H. Index fat claim (full fat, reduced fat, low fat) and organic claim in Facet P.</rdfs:comment>
	<oboInOwl:hasDbXref>LANGUAL:A1047</oboInOwl:hasDbXref>
</owl:Class>

<owl:Class rdf:about="&obo;FOODON_03401048">
	<rdfs:label xml:lang="en">10000278 - yoghurt/yoghurt substitutes (perishable) (gs1 gpc)</rdfs:label>
	<rdfs:subClassOf rdf:resource="&obo;FOODON_03401046"/>
	<obo:IAO_0000412>http://langual.org</obo:IAO_0000412>
	<obo:IAO_0000115 xml:lang="en">Includes any products that can be described/observed as a prepared food made from animal milk or non-animal milk, thickened by fermentation with lactic bacteria. Products include spoonable yogurt and fromage frais. These products must be refrigerated to extend their consumable life. Products include yogurt derived from an animal and yogurt derived from a plant, soy, almond, coconut. Also include yogurt flavoured with fruit, vanilla, nuts and honey, or packaged with a small amount of fruit preserve, nuts, or other accompaniment. Excludes products such as Drinking Yogurt, Frozen and Shelf Stable Yogurt and Yogurt Substitutes, Dairy and Dairy Substitute Drinks and Desserts.</obo:IAO_0000115>
	<obo:IAO_0000114 rdf:resource="&obo;IAO_0000428"/>
	<rdfs:comment xml:lang="en">LanguaL curation note: Index source of product (dairy, non dairy) in facet B. Index added ingredients (cereals, fruit pulp, sugar, flavouring) in facet H. Index fat claim (full fat, reduced fat, low fat), probiotic claim and organic claim in Facet P. Index preservation method (refrigeration) in facet J.</rdfs:comment>
	<oboInOwl:hasDbXref>LANGUAL:A1048</oboInOwl:hasDbXref>
</owl:Class>

<owl:Class rdf:about="&obo;FOODON_03401049">
	<rdfs:label xml:lang="en">10000279 - yoghurt/yoghurt substitutes (shelf stable) (gs1 gpc)</rdfs:label>
	<rdfs:subClassOf rdf:resource="&obo;FOODON_03401046"/>
	<obo:IAO_0000412>http://langual.org</obo:IAO_0000412>
	<obo:IAO_0000115 xml:lang="en">Includes any products that can be described/observed as a prepared food made from animal milk and non-animal milk, thickened by fermentation with lactic bacteria. Products include spoonable yogurt and fromage frais. These products have been treated or packaged in such a way as to extend their consumable life. Products include yogurt derived from an animal and yogurt derived from a plant, soya, almond, coconut. Also include yogurt flavoured with fruit, vanilla, nuts and honey, or packaged with a small amount of fruit preserve, nuts, or other accompaniment. Excludes products such as Drinking Yogurt, Frozen and Perishable Yogurt and Yogurt Substitutes, Dairy and Dairy Substitute Drinks and Desserts.</obo:IAO_0000115>
	<obo:IAO_0000114 rdf:resource="&obo;IAO_0000428"/>
	<rdfs:comment xml:lang="en">LanguaL curation note: Index source of product (dairy, non dairy) in facet B. Index added ingredients (cereals, fruit pulp, sugar, flavouring) in facet H. Index fat claim (full fat, reduced fat, low fat) and organic claim in Facet P. Index preservation method (dehydrated, UHT) in facet J.</rdfs:comment>
	<oboInOwl:hasDbXref>LANGUAL:A1049</oboInOwl:hasDbXref>
</owl:Class>

<owl:Class rdf:about="&obo;FOODON_03401050">
	<rdfs:label xml:lang="en">50132200 - milk/butter/cream/yoghurts/cheese/eggs/substitutes variety packs (gs1 gpc)</rdfs:label>
	<rdfs:subClassOf rdf:resource="&obo;FOODON_03401025"/>
	<obo:IAO_0000412>http://langual.org</obo:IAO_0000412>
	<obo:IAO_0000115 xml:lang="en">Includes any products that can be described/observed as two or more distinct Milk, Butter, Cream, Yogurt, Cheese, Egg or Substitute products sold together which exist within the schema but belong to different classes, that is two or more products contained within the same pack which cross classes within the Milk, Butter, Cream, Yogurts, Cheese, Eggs and Substitutes Family. Includes products such as Yogurts with Cream variety packs. Items that are received free with purchases should be removed from the classification decision-making process. Excludes products such as Strawberries and Cream variety packs.</obo:IAO_0000115>
	<obo:IAO_0000114 rdf:resource="&obo;IAO_0000428"/>
	<oboInOwl:hasDbXref>LANGUAL:A1050</oboInOwl:hasDbXref>
</owl:Class>

<owl:Class rdf:about="&obo;FOODON_03401051">
	<rdfs:label xml:lang="en">50150000 - oils/fats edible (gs1 gpc)</rdfs:label>
	<rdfs:subClassOf rdf:resource="&obo;FOODON_03400874"/>
	<obo:IAO_0000412>http://langual.org</obo:IAO_0000412>
	<obo:IAO_0000114 rdf:resource="&obo;IAO_0000428"/>
	<oboInOwl:hasDbXref>LANGUAL:A1051</oboInOwl:hasDbXref>
</owl:Class>

<owl:Class rdf:about="&obo;FOODON_03401052">
	<rdfs:label xml:lang="en">50151600 - fats edible (gs1 gpc)</rdfs:label>
	<rdfs:subClassOf rdf:resource="&obo;FOODON_03401051"/>
	<obo:IAO_0000412>http://langual.org</obo:IAO_0000412>
	<obo:IAO_0000114 rdf:resource="&obo;IAO_0000428"/>
	<oboInOwl:hasDbXref>LANGUAL:A1052</oboInOwl:hasDbXref>
</owl:Class>

<owl:Class rdf:about="&obo;FOODON_03401053">
	<rdfs:label xml:lang="en">10000041 - fats edible - animal (perishable) (gs1 gpc)</rdfs:label>
	<rdfs:subClassOf rdf:resource="&obo;FOODON_03401052"/>
	<obo:IAO_0000412>http://langual.org</obo:IAO_0000412>
	<obo:IAO_0000115 xml:lang="en">Includes any products that can be described/observed as a solid made from melting animal fat, purified and then allowed to solidify upon cooling. These products are designed for cooking and baking. These products can be/must be refrigerated to extend their consumable life. Products include lard, dripping, shortening and tallow. Excludes products such as Vegetable Cooking Fats, Margarine and Butter or Butter Based Spreads.</obo:IAO_0000115>
	<obo:IAO_0000114 rdf:resource="&obo;IAO_0000428"/>
	<rdfs:comment xml:lang="en">LanguaL curation note: If an industry recognized organic certification is claimed, index ORGANIC FOOD CLAIM OR USE in facet P. Index preservation method (refrigeration) in facet J.</rdfs:comment>
	<oboInOwl:hasDbXref>LANGUAL:A1053</oboInOwl:hasDbXref>
</owl:Class>

<owl:Class rdf:about="&obo;FOODON_03401054">
	<rdfs:label xml:lang="en">10000574 - fats edible - animal (shelf stable) (gs1 gpc)</rdfs:label>
	<rdfs:subClassOf rdf:resource="&obo;FOODON_03401052"/>
	<obo:IAO_0000412>http://langual.org</obo:IAO_0000412>
	<obo:IAO_0000115 xml:lang="en">Includes any product that can be described/observed as flakes or granules made from shredding/grating hard animal fat and treated and packaged in such a way as to extend their consumable life. These products are designed for cooking and baking. Products include derivatives of beef fat and mutton fat. Excludes products such as Vegetable Cooking Fats, Margarine and Butter or Butter Based Spreads.</obo:IAO_0000115>
	<obo:IAO_0000114 rdf:resource="&obo;IAO_0000428"/>
	<rdfs:comment xml:lang="en">LanguaL curation note: If an industry recognized organic certification is claimed, index ORGANIC FOOD CLAIM OR USE in facet P. Index physical form (grated, powder) in facet E.</rdfs:comment>
	<oboInOwl:hasDbXref>LANGUAL:A1054</oboInOwl:hasDbXref>
</owl:Class>

<owl:Class rdf:about="&obo;FOODON_03401055">
	<rdfs:label xml:lang="en">10000585 - fats edible - vegetable or plant (perishable) (gs1 gpc)</rdfs:label>
	<rdfs:subClassOf rdf:resource="&obo;FOODON_03401052"/>
	<obo:IAO_0000412>http://langual.org</obo:IAO_0000412>
	<obo:IAO_0000115 xml:lang="en">Includes any products that can be described/observed as a solid made from artificially hardened vegetable oils for baking and cooking. These products can be/must be refrigerated to extend their consumable life. Products include vegetable shortening specifically designed for baking and cooking. Excludes products such as Butter and Butter Based Spreads and Margarine, Cooking Animal Fats and Shelf Stable Vegetable Fats and Oils.</obo:IAO_0000115>
	<obo:IAO_0000114 rdf:resource="&obo;IAO_0000428"/>
	<rdfs:comment xml:lang="en">LanguaL curation note: Index plant in facet B. Index use claim (vegan) or organic claim in facet P. Index preservation method (refrigeration) in facet J.</rdfs:comment>
	<oboInOwl:hasDbXref>LANGUAL:A1055</oboInOwl:hasDbXref>
</owl:Class>

<owl:Class rdf:about="&obo;FOODON_03401056">
	<rdfs:label xml:lang="en">10000042 - fats edible - vegetable or plant (shelf stable) (gs1 gpc)</rdfs:label>
	<rdfs:subClassOf rdf:resource="&obo;FOODON_03401052"/>
	<obo:IAO_0000412>http://langual.org</obo:IAO_0000412>
	<obo:IAO_0000115 xml:lang="en">Includes any products that can be described/observed as a solid made from artificially hardened vegetable oils for baking and cooking. These products have been treated or packaged in such a way as to extend their consumable life. Products include vegetable shortening specifically designed for baking and cooking. Excludes products such as Butter and Butter Based Spreads and Margarine, Cooking Animal Fats and Vegetable Oils.</obo:IAO_0000115>
	<obo:IAO_0000114 rdf:resource="&obo;IAO_0000428"/>
	<rdfs:comment xml:lang="en">LanguaL curation note: Index plant in facet B. Index use claim (vegan) or organic claim in facet P.</rdfs:comment>
	<oboInOwl:hasDbXref>LANGUAL:A1056</oboInOwl:hasDbXref>
</owl:Class>

<owl:Class rdf:about="&obo;FOODON_03401057">
	<rdfs:label xml:lang="en">10000608 - fats edible variety packs (gs1 gpc)</rdfs:label>
	<rdfs:subClassOf rdf:resource="&obo;FOODON_03401052"/>
	<obo:IAO_0000412>http://langual.org</obo:IAO_0000412>
	<obo:IAO_0000115 xml:lang="en">Includes any products that can be described/observed as two or more distinct Edible Fats sold together, which exist within the schema belonging to different bricks but to the same class, that is two or more products contained within the same pack which cross bricks within the Fats Edible class. Includes products such as Lard and Dripping sold together. Items that are received free with purchases should be removed from the classification decision-making process. Excludes products such as Margarine and Vegetable Oil variety packs.</obo:IAO_0000115>
	<obo:IAO_0000114 rdf:resource="&obo;IAO_0000428"/>
	<oboInOwl:hasDbXref>LANGUAL:A1057</oboInOwl:hasDbXref>
</owl:Class>

<owl:Class rdf:about="&obo;FOODON_03401058">
	<rdfs:label xml:lang="en">50151500 - oils edible (gs1 gpc)</rdfs:label>
	<rdfs:subClassOf rdf:resource="&obo;FOODON_03401051"/>
	<obo:IAO_0000412>http://langual.org</obo:IAO_0000412>
	<obo:IAO_0000114 rdf:resource="&obo;IAO_0000428"/>
	<oboInOwl:hasDbXref>LANGUAL:A1058</oboInOwl:hasDbXref>
</owl:Class>

<owl:Class rdf:about="&obo;FOODON_03401059">
	<rdfs:label xml:lang="en">10000040 - oils edible - vegetable or plant (shelf stable) (gs1 gpc)</rdfs:label>
	<rdfs:subClassOf rdf:resource="&obo;FOODON_03401058"/>
	<obo:IAO_0000412>http://langual.org</obo:IAO_0000412>
	<obo:IAO_0000115 xml:lang="en">Includes any products that can be described/observed as any edible liquid oil derived from the following: grains, nuts, olives, palms, palm kernels, seeds, corn, maize, fruit pulp, beans or combination of these, that can be poured or dispensed as a spray, intended for cooking or for use as a dressing for salads. Products can include added flavouring, such as chilli and herbs. Excludes products such as health supplement based oils, such as Cod Liver, and non-edible oils, such as Linseed Oil.</obo:IAO_0000115>
	<obo:IAO_0000114 rdf:resource="&obo;IAO_0000428"/>
	<rdfs:comment xml:lang="en">LanguaL curation note: Index plant (almond, walnut) in facet B. If flavoured or added ingredients, index in facet H. If an industry recognized organic certification is claimed, index ORGANIC FOOD CLAIM OR USE in facet P.</rdfs:comment>
	<oboInOwl:hasDbXref>LANGUAL:A1059</oboInOwl:hasDbXref>
</owl:Class>

<owl:Class rdf:about="&obo;FOODON_03401060">
	<rdfs:label xml:lang="en">50151700 - oils/fats edible variety packs (gs1 gpc)</rdfs:label>
	<rdfs:subClassOf rdf:resource="&obo;FOODON_03401051"/>
	<obo:IAO_0000412>http://langual.org</obo:IAO_0000412>
	<obo:IAO_0000115 xml:lang="en">Includes any products that can be described/observed as two or more distinct Edible Fats sold together, which exist within the schema belonging to different bricks but to the same class, that is two or more products contained within the same pack which cross bricks within the Fats Edible class. Includes products such as Lard and Dripping sold together. Items that are received free with purchases should be removed from the classification decision-making process. Excludes products such as Margarine and Vegetable Oil variety packs.</obo:IAO_0000115>
	<obo:IAO_0000114 rdf:resource="&obo;IAO_0000428"/>
	<oboInOwl:hasDbXref>LANGUAL:A1060</oboInOwl:hasDbXref>
</owl:Class>

<owl:Class rdf:about="&obo;FOODON_03401061">
	<rdfs:label xml:lang="en">50190000 - prepared/preserved foods (gs1 gpc)</rdfs:label>
	<rdfs:subClassOf rdf:resource="&obo;FOODON_03400874"/>
	<obo:IAO_0000412>http://langual.org</obo:IAO_0000412>
	<obo:IAO_0000114 rdf:resource="&obo;IAO_0000428"/>
	<oboInOwl:hasDbXref>LANGUAL:A1061</oboInOwl:hasDbXref>
</owl:Class>

<owl:Class rdf:about="&obo;FOODON_03401062">
	<rdfs:label xml:lang="en">50193000 - baby/infant - foods/beverages (gs1 gpc)</rdfs:label>
	<rdfs:subClassOf rdf:resource="&obo;FOODON_03401061"/>
	<obo:IAO_0000412>http://langual.org</obo:IAO_0000412>
	<obo:IAO_0000114 rdf:resource="&obo;IAO_0000428"/>
	<oboInOwl:hasDbXref>LANGUAL:A1062</oboInOwl:hasDbXref>
</owl:Class>

<owl:Class rdf:about="&obo;FOODON_03401063">
	<rdfs:label xml:lang="en">10000575 - baby/infant - formula (shelf stable) (gs1 gpc)</rdfs:label>
	<rdfs:subClassOf rdf:resource="&obo;FOODON_03401062"/>
	<obo:IAO_0000412>http://langual.org</obo:IAO_0000412>
	<obo:IAO_0000115 xml:lang="en">Includes any product that can be described/observed as a food specifically labelled and marketed for a baby or infant. It is typically a powdered and ready to drink formula designed as a replacement for breast milk during nursing and is intended to provide a healthy, balanced diet for babies and infants of all ages. These products have been treated or packaged in such a way as to extend their consumable life. Excludes products such as Baby and Infant Beverages and adult variants of food formulas.</obo:IAO_0000115>
	<obo:IAO_0000114 rdf:resource="&obo;IAO_0000428"/>
	<rdfs:comment xml:lang="en">LanguaL curation note: Index age group (0-3 months, 6-12 months) the food is intended for. Index use claims (gluten free, lactose free) and organic claim in facet P. Index source (cow, soy) in facet B.</rdfs:comment>
	<oboInOwl:hasDbXref>LANGUAL:A1063</oboInOwl:hasDbXref>
</owl:Class>

<owl:Class rdf:about="&obo;FOODON_03401064">
	<rdfs:label xml:lang="en">10000105 - baby/infant - specialised beverages (shelf stable) (gs1 gpc)</rdfs:label>
	<rdfs:subClassOf rdf:resource="&obo;FOODON_03401062"/>
	<obo:IAO_0000412>http://langual.org</obo:IAO_0000412>
	<obo:IAO_0000115 xml:lang="en">Includes any products that can be described/observed as a beverage specifically labelled and marketed for a baby or infant. These products have been treated or packaged in such a way as to extend their consumable life. Includes juice, juice drinks, nursery water and dairy based drinks. Excludes products such as Formula, Baby and Infant Food, Adult variants of the above.</obo:IAO_0000115>
	<obo:IAO_0000114 rdf:resource="&obo;IAO_0000428"/>
	<rdfs:comment xml:lang="en">LanguaL curation note: Index age group (0-3 months, 6-12 months) the food is intended for. Index physical form (powder, liquid) in facet E.  E244If an industry recognized organic certification is claimed, index ORGANIC FOOD CLAIM OR USE in facet P.</rdfs:comment>
	<oboInOwl:hasDbXref>LANGUAL:A1064</oboInOwl:hasDbXref>
</owl:Class>

<owl:Class rdf:about="&obo;FOODON_03401065">
	<rdfs:label xml:lang="en">10000104 - baby/infant - specialised foods (shelf stable) (gs1 gpc)</rdfs:label>
	<rdfs:subClassOf rdf:resource="&obo;FOODON_03401062"/>
	<obo:IAO_0000412>http://langual.org</obo:IAO_0000412>
	<obo:IAO_0000115 xml:lang="en">Includes any products that can be described/observed as food specifically labelled and marketed for a baby or infant, which is typically intended to provide a healthy, balanced diet for Infants and babies of all ages. These products have been treated or packaged in such a way as to extend their consumable life. Excludes products such as Baby and Infant Beverages, powdered and ready to drink formula specifically designed for use as a replacement for breast milk during nursing. Adult variants of the above.</obo:IAO_0000115>
	<obo:IAO_0000114 rdf:resource="&obo;IAO_0000428"/>
	<rdfs:comment xml:lang="en">LanguaL curation note: Index age group (0-3 months, 6-12 months) the food is intended for. Index the base ingredient (fruit, poultry) in facets B and C (meat, egg). If an industry recognized organic certification is claimed, index ORGANIC FOOD CLAIM OR USE in facet P.</rdfs:comment>
	<oboInOwl:hasDbXref>LANGUAL:A1065</oboInOwl:hasDbXref>
</owl:Class>

<owl:Class rdf:about="&obo;FOODON_03401066">
	<rdfs:label xml:lang="en">10000610 - baby/infant - foods/beverages variety packs (gs1 gpc)</rdfs:label>
	<rdfs:subClassOf rdf:resource="&obo;FOODON_03401062"/>
	<obo:IAO_0000412>http://langual.org</obo:IAO_0000412>
	<obo:IAO_0000115 xml:lang="en">Includes any products that can be described/observed as two or more distinct Baby and Infant Foods or Beverages sold together, which exist within the schema belonging to different bricks but to the same class, that is two or more products contained within the same pack which cross bricks within the Baby and Infant - Foods and Beverages class. Includes products such as Baby Formula and jars of Baby Food sold together. Items that are received free with purchases should be removed from the classification decision-making process. Excludes products such as Baby Formula and Milk variety packs.</obo:IAO_0000115>
	<obo:IAO_0000114 rdf:resource="&obo;IAO_0000428"/>
	<oboInOwl:hasDbXref>LANGUAL:A1066</oboInOwl:hasDbXref>
</owl:Class>

<owl:Class rdf:about="&obo;FOODON_03401067">
	<rdfs:label xml:lang="en">50193500 - dairy/egg based products (gs1 gpc)</rdfs:label>
	<rdfs:subClassOf rdf:resource="&obo;FOODON_03401061"/>
	<obo:IAO_0000412>http://langual.org</obo:IAO_0000412>
	<obo:IAO_0000114 rdf:resource="&obo;IAO_0000428"/>
	<oboInOwl:hasDbXref>LANGUAL:A1067</oboInOwl:hasDbXref>
</owl:Class>

<owl:Class rdf:about="&obo;FOODON_03401068">
	<rdfs:label xml:lang="en">10005224 - dairy/egg based products - not ready to eat (frozen) (gs1 gpc)</rdfs:label>
	<rdfs:subClassOf rdf:resource="&obo;FOODON_03401067"/>
	<obo:IAO_0000412>http://langual.org</obo:IAO_0000412>
	<obo:IAO_0000115 xml:lang="en">Includes any products that can be described/observed as a dairy or egg based not ready to eat, prepared product, such as eggs or cheese in combination with other ingredients, such as another protein or vegetables. These ingredients form a valuable part of the product, rather than just serve as a seasoning or flavouring, such as ham in a ham and cheese omelette. These products must not include any dough or grain based products. They may or may not contain a sauce. These products require cooking prior to consumption. These products must be frozen to extend their consumable life. Specifically excludes all eggs and cheese to which no recipe has been applied. Excludes products such as Shelf Stable and Perishable Not Ready to Eat and Ready to Eat Dairy and Egg Based Products.</obo:IAO_0000115>
	<obo:IAO_0000114 rdf:resource="&obo;IAO_0000428"/>
	<rdfs:comment xml:lang="en">LanguaL curation note: Index the main ingredient (fish, fruit) in facets B and C (meat, dairy). Index packing medium (sauce) in facet K. Index fat claim (low fat, reduced fat) and organic claim in facet P.</rdfs:comment>
	<oboInOwl:hasDbXref>LANGUAL:A1068</oboInOwl:hasDbXref>
</owl:Class>

<owl:Class rdf:about="&obo;FOODON_03401069">
	<rdfs:label xml:lang="en">10005225 - dairy/egg based products - not ready to eat (perishable) (gs1 gpc)</rdfs:label>
	<rdfs:subClassOf rdf:resource="&obo;FOODON_03401067"/>
	<obo:IAO_0000412>http://langual.org</obo:IAO_0000412>
	<obo:IAO_0000115 xml:lang="en">Includes any products that can be described/observed as a dairy or egg based not ready to eat, prepared product, such as eggs or cheese in combination with other ingredients, such as another protein or vegetables. These ingredients form a valuable part of the product, rather than just serve as a seasoning or flavouring, such as ham in a ham and cheese omelette. These products must not include any dough or grain based products. They may or may not contain a sauce. These products require cooking prior to consumption. These products must be refrigerated to extend their consumable life. Specifically excludes all eggs and cheese to which no recipe has been applied. Excludes products such as Shelf Stable and Frozen Not Ready to Eat and Ready to Eat Dairy and Egg Based Products.</obo:IAO_0000115>
	<obo:IAO_0000114 rdf:resource="&obo;IAO_0000428"/>
	<rdfs:comment xml:lang="en">LanguaL curation note: Index the main ingredient (fish, fruit) in facets B and C (meat, dairy). Index packing medium (sauce) in facet K. Index fat claim (low fat, reduced fat) and organic claim in facet P. Index preservation method (refrigeration) in facet J.</rdfs:comment>
	<oboInOwl:hasDbXref>LANGUAL:A1069</oboInOwl:hasDbXref>
</owl:Class>

<owl:Class rdf:about="&obo;FOODON_03401070">
	<rdfs:label xml:lang="en">10005226 - dairy/egg based products - not ready to eat (shelf stable) (gs1 gpc)</rdfs:label>
	<rdfs:subClassOf rdf:resource="&obo;FOODON_03401067"/>
	<obo:IAO_0000412>http://langual.org</obo:IAO_0000412>
	<obo:IAO_0000115 xml:lang="en">Includes any products that can be described/observed as a dairy or egg based not ready to eat, prepared product, such as eggs or cheese in combination with other ingredients, such as another protein or vegetables. These ingredients form a valuable part of the product, rather than just serve as a seasoning or flavouring, such as ham in a ham and cheese omelette. These products must not include any dough or grain based products. They may or may not contain a sauce. These products require cooking prior to consumption. These products have been treated or packaged in such a way as to extend their consumable life. Specifically excludes all eggs and cheese to which no recipe has been applied. Excludes products such as Perishable and Frozen Not Ready to Eat and Ready to Eat Dairy and Egg Based Products.</obo:IAO_0000115>
	<obo:IAO_0000114 rdf:resource="&obo;IAO_0000428"/>
	<rdfs:comment xml:lang="en">LanguaL curation note: Index the main ingredient (fish, fruit) in facets B and C (meat, dairy). Index packing medium (sauce) in facet K. Index fat claim (low fat, reduced fat) and organic claim in facet P.</rdfs:comment>
	<oboInOwl:hasDbXref>LANGUAL:A1070</oboInOwl:hasDbXref>
</owl:Class>

<owl:Class rdf:about="&obo;FOODON_03401071">
	<rdfs:label xml:lang="en">10005227 - dairy/egg based products - ready to eat (perishable) (gs1 gpc)</rdfs:label>
	<rdfs:subClassOf rdf:resource="&obo;FOODON_03401067"/>
	<obo:IAO_0000412>http://langual.org</obo:IAO_0000412>
	<obo:IAO_0000115 xml:lang="en">Includes any products that can be described/observed as a dairy or egg based ready to eat, prepared product, such as eggs or cheese in combination with other ingredients, such as another protein or vegetables. These ingredients form a valuable part of the product, rather than just serve as a seasoning or flavouring, such as the salad in an egg salad. These products must not include any dough or grain based products. They may or may not contain a sauce. These products do not require cooking prior to consumption, but some products can be eaten hot after reheating. These products must be refrigerated to extend their consumable life. Specifically excludes all eggs and cheese to which no recipe has been applied. Excludes products such as Shelf Stable Ready to Eat and Not Ready to Eat Dairy and Egg Based Products.</obo:IAO_0000115>
	<obo:IAO_0000114 rdf:resource="&obo;IAO_0000428"/>
	<rdfs:comment xml:lang="en">LanguaL curation note: Index the main ingredient (fish, fruit) in facets B and C (meat, dairy). Index packing medium (sauce) in facet K. Index fat claim (low fat, reduced fat) and organic claim in facet P. Index preservation method (refrigeration) in facet J.</rdfs:comment>
	<oboInOwl:hasDbXref>LANGUAL:A1071</oboInOwl:hasDbXref>
</owl:Class>

<owl:Class rdf:about="&obo;FOODON_03401072">
	<rdfs:label xml:lang="en">10005228 - dairy/egg based products - ready to eat (shelf stable) (gs1 gpc)</rdfs:label>
	<rdfs:subClassOf rdf:resource="&obo;FOODON_03401067"/>
	<obo:IAO_0000412>http://langual.org</obo:IAO_0000412>
	<obo:IAO_0000115 xml:lang="en">Includes any products that can be described/observed as a dairy or egg based ready to eat, prepared product, such as eggs or cheese in combination with other ingredients, such as another protein or vegetables. These ingredients form a valuable part of the product, rather than just serve as a seasoning or flavouring, such as the salad in an egg salad. These products must not include any dough or grain based products. They may or may not contain a sauce. These products do not require cooking prior to consumption, but some products can be eaten hot after reheating. These products have been treated or packaged in such a way as to extend their consumable life. Specifically excludes all eggs and cheese to which no recipe has been applied. Excludes products such as Perishable Ready to Eat and Not Ready to Eat Dairy and Egg Based Products.</obo:IAO_0000115>
	<obo:IAO_0000114 rdf:resource="&obo;IAO_0000428"/>
	<rdfs:comment xml:lang="en">LanguaL curation note: Index the main ingredient (fish, fruit) in facets B and C (meat, dairy). Index packing medium (sauce) in facet K. Index fat claim (low fat, reduced fat) and organic claim in facet P.</rdfs:comment>
	<oboInOwl:hasDbXref>LANGUAL:A1072</oboInOwl:hasDbXref>
</owl:Class>

<owl:Class rdf:about="&obo;FOODON_03401073">
	<rdfs:label xml:lang="en">50192300 - desserts/dessert sauces/toppings (gs1 gpc)</rdfs:label>
	<rdfs:subClassOf rdf:resource="&obo;FOODON_03401061"/>
	<obo:IAO_0000412>http://langual.org</obo:IAO_0000412>
	<obo:IAO_0000114 rdf:resource="&obo;IAO_0000428"/>
	<oboInOwl:hasDbXref>LANGUAL:A1073</oboInOwl:hasDbXref>
</owl:Class>

<owl:Class rdf:about="&obo;FOODON_03401074">
	<rdfs:label xml:lang="en">10000193 - dessert sauces/toppings/fillings (frozen) (gs1 gpc)</rdfs:label>
	<rdfs:subClassOf rdf:resource="&obo;FOODON_03401073"/>
	<obo:IAO_0000412>http://langual.org</obo:IAO_0000412>
	<obo:IAO_0000115 xml:lang="en">Includes any products that can be described/observed as a flavoured topping/filling or a sweetened liquid typically intended for consumption as an accompaniment to a dessert. Includes products such as cream pie fillings. These products must be frozen to extend their consumable life. Excludes products such as Perishable and Shelf Stable Dessert Sauces and Toppings.</obo:IAO_0000115>
	<obo:IAO_0000114 rdf:resource="&obo;IAO_0000428"/>
	<rdfs:comment xml:lang="en">LanguaL curation note: Index main ingredient (fruit, chocolate) in facet B. Index use claim (diabetic) and fat claim (low fat, reduced fat) in facet P.</rdfs:comment>
	<oboInOwl:hasDbXref>LANGUAL:A1074</oboInOwl:hasDbXref>
</owl:Class>

<owl:Class rdf:about="&obo;FOODON_03401075">
	<rdfs:label xml:lang="en">10000194 - dessert sauces/toppings/fillings (perishable) (gs1 gpc)</rdfs:label>
	<rdfs:subClassOf rdf:resource="&obo;FOODON_03401073"/>
	<obo:IAO_0000412>http://langual.org</obo:IAO_0000412>
	<obo:IAO_0000115 xml:lang="en">Includes any products that can be described/observed as a flavoured topping/filling or a sweetened liquid typically intended for consumption as an accompaniment to a dessert. Includes products such as cream pie fillings. These products must be refrigerated to extend their consumable life. Excludes products such as Frozen and Shelf Stable Dessert Sauces and Toppings.</obo:IAO_0000115>
	<obo:IAO_0000114 rdf:resource="&obo;IAO_0000428"/>
	<rdfs:comment xml:lang="en">LanguaL curation note: Index main ingredient (fruit, chocolate) in facet B. Index use claim (diabetic) and fat claim (low fat, reduced fat) in facet P. Index preservation method (refrigeration) in facet J.</rdfs:comment>
	<oboInOwl:hasDbXref>LANGUAL:A1075</oboInOwl:hasDbXref>
</owl:Class>

<owl:Class rdf:about="&obo;FOODON_03401076">
	<rdfs:label xml:lang="en">10000195 - dessert sauces/toppings/fillings (shelf stable) (gs1 gpc)</rdfs:label>
	<rdfs:subClassOf rdf:resource="&obo;FOODON_03401073"/>
	<obo:IAO_0000412>http://langual.org</obo:IAO_0000412>
	<obo:IAO_0000115 xml:lang="en">Includes any products that can be described/observed as a flavoured topping/filling or a sweetened liquid typically intended for consumption as an accompaniment to a dessert. Includes products such as cream pie fillings. These products have been packaged in such a way as to extend their consumable life. Excludes products such as Perishable and Frozen Desserts, Ice Cream, Pastries and Cakes, Yogurt.</obo:IAO_0000115>
	<obo:IAO_0000114 rdf:resource="&obo;IAO_0000428"/>
	<rdfs:comment xml:lang="en">LanguaL curation note: Index main ingredient (fruit, chocolate) in facet B. Index use claim (diabetic) and fat claim (low fat, reduced fat) in facet P.</rdfs:comment>
	<oboInOwl:hasDbXref>LANGUAL:A1076</oboInOwl:hasDbXref>
</owl:Class>

<owl:Class rdf:about="&obo;FOODON_03401077">
	<rdfs:label xml:lang="en">10000196 - desserts (frozen) (gs1 gpc)</rdfs:label>
	<rdfs:subClassOf rdf:resource="&obo;FOODON_03401073"/>
	<obo:IAO_0000412>http://langual.org</obo:IAO_0000412>
	<obo:IAO_0000115 xml:lang="en">Includes any products that can be described/observed as a prepared food normally consumed as the last course of a meal. These products must be frozen to extend their consumable life. Products include desserts that are biscuit based, bread based, cake/sponge based, dairy based, pastry based and rice based. Excludes products such as Perishable and Shelf Stable Desserts, Ice Cream, Pastries and Cakes, Yogurt.</obo:IAO_0000115>
	<obo:IAO_0000114 rdf:resource="&obo;IAO_0000428"/>
	<rdfs:comment xml:lang="en">LanguaL curation note: Index main ingredient in facets B (fruit, cereal) and C (egg, milk). Index added ingredients (alcohol, nut) in facet H. Index use claim (diabetic) and fat claim (low fat, reduced fat) in facet P.</rdfs:comment>
	<oboInOwl:hasDbXref>LANGUAL:A1077</oboInOwl:hasDbXref>
</owl:Class>

<owl:Class rdf:about="&obo;FOODON_03401078">
	<rdfs:label xml:lang="en">10000197 - desserts (perishable) (gs1 gpc)</rdfs:label>
	<rdfs:subClassOf rdf:resource="&obo;FOODON_03401073"/>
	<obo:IAO_0000412>http://langual.org</obo:IAO_0000412>
	<obo:IAO_0000115 xml:lang="en">Includes any products that can be described/observed as a prepared food normally consumed as the last course of a meal. These products must be refrigerated to extend their consumable life. Products include desserts that are biscuit based, bread based, cake/sponge based, dairy based, pastry based and rice based. Excludes products such as Frozen and Shelf Stable Desserts, Ice Cream Pastries, Cakes and Yogurt.</obo:IAO_0000115>
	<obo:IAO_0000114 rdf:resource="&obo;IAO_0000428"/>
	<rdfs:comment xml:lang="en">LanguaL curation note: Index main ingredient in facets B (fruit, cereal) and C (egg, milk). Index added ingredients (alcohol, nut) in facet H. Index use claim (diabetic) and fat claim (low fat, reduced fat) in facet P. Index preservation method (refrigeration) in facet J.</rdfs:comment>
	<oboInOwl:hasDbXref>LANGUAL:A1078</oboInOwl:hasDbXref>
</owl:Class>

<owl:Class rdf:about="&obo;FOODON_03401079">
	<rdfs:label xml:lang="en">10000312 - desserts (shelf stable) (gs1 gpc)</rdfs:label>
	<rdfs:subClassOf rdf:resource="&obo;FOODON_03401073"/>
	<obo:IAO_0000412>http://langual.org</obo:IAO_0000412>
	<obo:IAO_0000115 xml:lang="en">Includes any products that can be described/observed as a prepared food normally consumed as the last course of a meal. These products have been packaged in such a way as to extend their consumable life. Products include desserts that are biscuit based, bread based, cake/sponge based, dairy based, pastry based and rice based. Excludes products such as Perishable and Frozen Desserts, Ice Cream, Pastries and Cakes, Yogurt.</obo:IAO_0000115>
	<obo:IAO_0000114 rdf:resource="&obo;IAO_0000428"/>
	<rdfs:comment xml:lang="en">LanguaL curation note: Index main ingredient in facets B (fruit, cereal) and C (egg, milk). Index added ingredients (alcohol, nut) in facet H. Index use claim (diabetic) and fat claim (low fat, reduced fat) in facet P. Index the manufacturer's cooking process the product has undergone (fried, baked) in facet G.</rdfs:comment>
	<oboInOwl:hasDbXref>LANGUAL:A1079</oboInOwl:hasDbXref>
</owl:Class>

<owl:Class rdf:about="&obo;FOODON_03401080">
	<rdfs:label xml:lang="en">10000215 - ice cream/ice novelties (frozen) (gs1 gpc)</rdfs:label>
	<rdfs:subClassOf rdf:resource="&obo;FOODON_03401073"/>
	<obo:IAO_0000412>http://langual.org</obo:IAO_0000412>
	<obo:IAO_0000115 xml:lang="en">Includes any products that can be described/observed as a sweet prepared food made from animal milk, milk substitute or water, which is frozen, sweetened and often flavoured by the addition of other ingredients, such as chocolate, vanilla and fruit. These products must be frozen to extend their consumable life. Includes ice cream novelties, ice cream cakes and ice cream in various forms such as containers, filled ice cream cones, iced lollies and Popsicles. Excludes products such as Shelf Stable Ice Cream and Ice Cream Novelties, and Ice Cream Based Desserts.</obo:IAO_0000115>
	<obo:IAO_0000114 rdf:resource="&obo;IAO_0000428"/>
	<rdfs:comment xml:lang="en">LanguaL curation note: Index the level of fat claim (low fat, reduced fat, full fat) in facet P.</rdfs:comment>
	<oboInOwl:hasDbXref>LANGUAL:A1080</oboInOwl:hasDbXref>
</owl:Class>

<owl:Class rdf:about="&obo;FOODON_03401081">
	<rdfs:label xml:lang="en">10000216 - ice cream/ice novelties (shelf stable) (gs1 gpc)</rdfs:label>
	<rdfs:subClassOf rdf:resource="&obo;FOODON_03401073"/>
	<obo:IAO_0000412>http://langual.org</obo:IAO_0000412>
	<obo:IAO_0000115 xml:lang="en">Includes any products that can be described/observed as a sweet prepared food made from animal milk, milk substitute or water, which is sweetened and often flavoured by the addition of other ingredients, such as chocolate, vanilla and fruit. Includes ice cream mixes, novelties and ice cream in various formats, such as containers, filled ice cream cones, iced lollies and Popsicles, which are sold in a shelf stable form but are designed to be frozen before consumption. These products have been treated or packaged in such a way as to extend their consumable life. Excludes products such as Frozen Ice Cream and Ice Cream Novelties, and Ice Cream Based Desserts.</obo:IAO_0000115>
	<obo:IAO_0000114 rdf:resource="&obo;IAO_0000428"/>
	<rdfs:comment xml:lang="en">LanguaL curation note: Index the level of fat claim (low fat, reduced fat, full fat) in facet P.</rdfs:comment>
	<oboInOwl:hasDbXref>LANGUAL:A1081</oboInOwl:hasDbXref>
</owl:Class>

<owl:Class rdf:about="&obo;FOODON_03401082">
	<rdfs:label xml:lang="en">10000611 - desserts/dessert toppings variety packs (gs1 gpc)</rdfs:label>
	<rdfs:subClassOf rdf:resource="&obo;FOODON_03401073"/>
	<obo:IAO_0000412>http://langual.org</obo:IAO_0000412>
	<obo:IAO_0000115 xml:lang="en">Includes any products that can be described/observed as two or more distinct Desserts or Dessert Sauces/Toppings sold together, which exist within the schema belonging to different bricks but to the same class, that is two or more products contained within the same pack which cross bricks within the Desserts and Dessert Toppings class. Includes products such as Ice Cream and Dessert Sauce sold together. Items that are received free with purchases should be removed from the classification decision-making process. Excludes products such as Ice Cream and Wafer variety packs and Ice Cream and Chicken Korma variety packs.</obo:IAO_0000115>
	<obo:IAO_0000114 rdf:resource="&obo;IAO_0000428"/>
	<oboInOwl:hasDbXref>LANGUAL:A1082</oboInOwl:hasDbXref>
</owl:Class>

<owl:Class rdf:about="&obo;FOODON_03401083">
	<rdfs:label xml:lang="en">50193300 - dough based products (gs1 gpc)</rdfs:label>
	<rdfs:subClassOf rdf:resource="&obo;FOODON_03401061"/>
	<obo:IAO_0000412>http://langual.org</obo:IAO_0000412>
	<obo:IAO_0000114 rdf:resource="&obo;IAO_0000428"/>
	<oboInOwl:hasDbXref>LANGUAL:A1083</oboInOwl:hasDbXref>
</owl:Class>

<owl:Class rdf:about="&obo;FOODON_03401084">
	<rdfs:label xml:lang="en">10000301 - dough based products - not ready to eat - savoury (frozen) (gs1 gpc)</rdfs:label>
	<rdfs:subClassOf rdf:resource="&obo;FOODON_03401083"/>
	<obo:IAO_0000412>http://langual.org</obo:IAO_0000412>
	<obo:IAO_0000115 xml:lang="en">Includes any products that can be described/observed as a savoury dough-based not ready to eat, prepared product, such as Pasta, Gnocchi, Noodles or Batter, in combination with other ingredients, such as meat, eggs, fish or vegetables. These ingredients form a valuable part of the product rather than just serve as a seasoning or flavouring, such as the meat/tomato sauce in Spaghetti Bolognaise. These products can include dairy based ingredients. They may or may not contain a sauce. These products are not ready to eat and require cooking prior to consumption. These products must be frozen to extend their consumable life. Specifically excludes pizza and savoury pies, quiches, pastries and bread products Excludes products such as Shelf Stable and Perishable Not Ready to Eat and Ready to Eat Dough-Based Prepared Products, Pasta and Noodles Unprepared.</obo:IAO_0000115>
	<obo:IAO_0000114 rdf:resource="&obo;IAO_0000428"/>
	<rdfs:comment xml:lang="en">LanguaL curation note: Index main ingredient in facets B (fruit, poultry) and C (egg, milk). Index added ingredients in facet H. Index packing medium (sauce) in facet K. Index fat claim (full fat, reduced fat, low fat) and organic claim in Facet P.</rdfs:comment>
	<oboInOwl:hasDbXref>LANGUAL:A1084</oboInOwl:hasDbXref>
</owl:Class>

<owl:Class rdf:about="&obo;FOODON_03401085">
	<rdfs:label xml:lang="en">10000300 - dough based products - not ready to eat - savoury (perishable) (gs1 gpc)</rdfs:label>
	<rdfs:subClassOf rdf:resource="&obo;FOODON_03401083"/>
	<obo:IAO_0000412>http://langual.org</obo:IAO_0000412>
	<obo:IAO_0000115 xml:lang="en">Includes any products that can be described/observed as a savoury dough-based not ready to eat, prepared product, such as Pasta, Gnocchi, Noodles or Batter in combination with other ingredients, such as meat, eggs, fish or vegetables. These ingredients form a valuable part of the product rather than just serve as a seasoning or flavouring, such as the meat/tomato sauce in Spaghetti Bolognaise. These products can include dairy based ingredients. They may or may not contain a sauce. These products are not ready to eat and require cooking prior to consumption. These products must be refrigerated to extend their consumable life. Specifically excludes pizza, savoury pies, quiches, pastries and bread products. Excludes products such as Shelf Stable and Frozen Not Ready to Eat and Ready to Eat Dough-Based Prepared Products, Pasta and Noodles Unprepared.</obo:IAO_0000115>
	<obo:IAO_0000114 rdf:resource="&obo;IAO_0000428"/>
	<rdfs:comment xml:lang="en">LanguaL curation note: Index main ingredient in facets B (fruit, poultry) and C (egg, milk). Index added ingredients in facet H. Index packing medium (sauce) in facet K. Index fat claim (full fat, reduced fat, low fat) and organic claim in Facet P. Index preservation method (refrigeration) in facet J.</rdfs:comment>
	<oboInOwl:hasDbXref>LANGUAL:A1085</oboInOwl:hasDbXref>
</owl:Class>

<owl:Class rdf:about="&obo;FOODON_03401086">
	<rdfs:label xml:lang="en">10000302 - dough based products - not ready to eat - savoury (shelf stable) (gs1 gpc)</rdfs:label>
	<rdfs:subClassOf rdf:resource="&obo;FOODON_03401083"/>
	<obo:IAO_0000412>http://langual.org</obo:IAO_0000412>
	<obo:IAO_0000115 xml:lang="en">Includes any products that can be described/observed as a savoury dough-based not ready to eat, prepared product, such as Pasta, Gnocchi, Noodles or Batter in combination with other ingredients, such as meat, eggs, fish or vegetables. These ingredients form a valuable part of the product rather than just serve as a seasoning or flavouring, such as the meat/tomato sauce in Spaghetti Bolognaise. These products can include dairy based ingredients. They may or may not contain a sauce. These products are not ready to eat and require cooking prior to consumption. These products have been specially treated or packaged to extend their consumable life. Specifically excludes pizza, savoury pies, quiches, pastries and bread products. Excludes products such as Frozen and Perishable Not Ready to Eat and Ready to Eat Dough-Based Prepared Products, Unprepared Pasta and Noodles.</obo:IAO_0000115>
	<obo:IAO_0000114 rdf:resource="&obo;IAO_0000428"/>
	<rdfs:comment xml:lang="en">LanguaL curation note: Index main ingredient in facets B (fruit, poultry) and C (egg, milk). Index added ingredients in facet H. Index packing medium (sauce) in facet K. Index fat claim (full fat, reduced fat, low fat) and organic claim in Facet P.</rdfs:comment>
	<oboInOwl:hasDbXref>LANGUAL:A1086</oboInOwl:hasDbXref>
</owl:Class>

<owl:Class rdf:about="&obo;FOODON_03401087">
	<rdfs:label xml:lang="en">10000298 - dough based products - ready to eat - savoury (perishable) (gs1 gpc)</rdfs:label>
	<rdfs:subClassOf rdf:resource="&obo;FOODON_03401083"/>
	<obo:IAO_0000412>http://langual.org</obo:IAO_0000412>
	<obo:IAO_0000115 xml:lang="en">Includes any products that can be described/observed as a savoury dough-based ready to eat, prepared product, such as Pasta, Gnocchi or Noodles in combination with other ingredients, such as meat, eggs, fish or vegetables. These ingredients form a valuable part of the product rather than just serve as a seasoning or flavouring, such as Pasta with a Roasted Vegetable Salad. These products can include dairy based ingredients. They may or may not contain a sauce. These products do not require cooking prior to consumption, but some products can be eaten hot after reheating. These products must be refrigerated to extend their consumable life. Specifically excludes pizza, savoury pies, quiches, pastries and bread products. Excludes products such as Shelf Stable Ready to Eat and Not Ready to Eat Dough-Based Prepared Product, Unprepared Pasta and Noodles.</obo:IAO_0000115>
	<obo:IAO_0000114 rdf:resource="&obo;IAO_0000428"/>
	<rdfs:comment xml:lang="en">LanguaL curation note: Index main ingredient in facets B (fruit, poultry) and C (egg, milk). Index added ingredients in facet H. Index packing medium (sauce) in facet K. Index fat claim (full fat, reduced fat, low fat) and organic claim in Facet P. Index preservation method (refrigeration) in facet J.</rdfs:comment>
	<oboInOwl:hasDbXref>LANGUAL:A1087</oboInOwl:hasDbXref>
</owl:Class>

<owl:Class rdf:about="&obo;FOODON_03401088">
	<rdfs:label xml:lang="en">10000299 - dough based products - ready to eat - savoury (shelf stable) (gs1 gpc)</rdfs:label>
	<rdfs:subClassOf rdf:resource="&obo;FOODON_03401083"/>
	<obo:IAO_0000412>http://langual.org</obo:IAO_0000412>
	<obo:IAO_0000115 xml:lang="en">Includes any products that can be described/observed as a savoury dough-based ready to eat, prepared product, such as Pasta, Gnocchi or Noodles, in combination with other ingredients, such as meat, eggs, fish or vegetables. These ingredients form a valuable part of the product, rather than just serve as a seasoning or flavouring, such as tuna and salad in a Tuna Pasta Salad. These products can include dairy based ingredients. They may or may not contain a sauce. These products do not require cooking prior to consumption, but some products can be eaten hot after reheating. These products have been treated or packaged in such a way as to extend their consumable life. Specifically excludes pizza, savoury pies, pastries, quiches and bread products. Excludes products such as Perishable Ready to Eat and Not Ready to Eat Dough Based Prepared Products, Unprepared Pasta and Noodles, Dried Pasta and Noodles.</obo:IAO_0000115>
	<obo:IAO_0000114 rdf:resource="&obo;IAO_0000428"/>
	<rdfs:comment xml:lang="en">LanguaL curation note: Index main ingredient in facets B (fruit, poultry) and C (egg, milk). Index added ingredients in facet H. Index packing medium (sauce) in facet K. Index fat claim (full fat, reduced fat, low fat) and organic claim in Facet P.</rdfs:comment>
	<oboInOwl:hasDbXref>LANGUAL:A1088</oboInOwl:hasDbXref>
</owl:Class>

<owl:Class rdf:about="&obo;FOODON_03401089">
	<rdfs:label xml:lang="en">50193200 - grain based products (gs1 gpc)</rdfs:label>
	<rdfs:subClassOf rdf:resource="&obo;FOODON_03401061"/>
	<obo:IAO_0000412>http://langual.org</obo:IAO_0000412>
	<obo:IAO_0000114 rdf:resource="&obo;IAO_0000428"/>
	<oboInOwl:hasDbXref>LANGUAL:A1089</oboInOwl:hasDbXref>
</owl:Class>

<owl:Class rdf:about="&obo;FOODON_03401090">
	<rdfs:label xml:lang="en">10000296 - grain based products - not ready to eat - savoury (frozen) (gs1 gpc)</rdfs:label>
	<rdfs:subClassOf rdf:resource="&obo;FOODON_03401089"/>
	<obo:IAO_0000412>http://langual.org</obo:IAO_0000412>
	<obo:IAO_0000115 xml:lang="en">Includes any products that can be described/observed as a savoury grain-based not ready to eat, prepared product, such as Rice, Polenta or Couscous in combination with other ingredients, such as meat, eggs, fish or vegetables. These ingredients form a valuable part of the product, rather than just serve as a seasoning or flavouring, such as Chicken Tandoori with Pilau Rice. These products must not include any dough-based products. They may or may not contain a sauce. These products require cooking prior to consumption. These products must be frozen to extend their consumable life. Specifically excludes all unprepared dried rice. Excludes products such as Shelf Stable and Perishable Not Ready to Eat and Ready to Eat Grain-Based Prepared Products, Unprepared Grains.</obo:IAO_0000115>
	<obo:IAO_0000114 rdf:resource="&obo;IAO_0000428"/>
	<rdfs:comment xml:lang="en">LanguaL curation note: Index main ingredient in facets B (fruit, poultry) and C (egg, milk). Index added ingredients in facet H. Index packing medium (sauce) in facet K. Index fat claim (full fat, reduced fat, low fat) and organic claim in Facet P.</rdfs:comment>
	<oboInOwl:hasDbXref>LANGUAL:A1090</oboInOwl:hasDbXref>
</owl:Class>

<owl:Class rdf:about="&obo;FOODON_03401091">
	<rdfs:label xml:lang="en">10000295 - grain based products - not ready to eat - savoury (perishable) (gs1 gpc)</rdfs:label>
	<rdfs:subClassOf rdf:resource="&obo;FOODON_03401089"/>
	<obo:IAO_0000412>http://langual.org</obo:IAO_0000412>
	<obo:IAO_0000115 xml:lang="en">Includes any products that can be described/observed as a savoury grain-based not ready to eat, prepared product, such as Rice, Polenta or Couscous in combination with other ingredients, such as meat, eggs, fish or vegetables. These ingredients form a valuable part of the product, rather than just serve as a seasoning or flavouring, such as Chicken Tandoori with Pilau Rice. These products must not include any dough-based products. They may or may not contain a sauce. These products require cooking prior to consumption. These products must be refrigerated to extend their consumable life. Specifically excludes all unprepared dried rice. Excludes products such as Shelf Stable and Frozen Not Ready-to-Eat and Ready-to-Eat Grain-Based Prepared Products, Unprepared Grains.</obo:IAO_0000115>
	<obo:IAO_0000114 rdf:resource="&obo;IAO_0000428"/>
	<rdfs:comment xml:lang="en">LanguaL curation note: Index main ingredient in facets B (fruit, poultry) and C (egg, milk). Index added ingredients in facet H. Index packing medium (sauce) in facet K. Index fat claim (full fat, reduced fat, low fat) and organic claim in Facet P. Index preservation method (refrigeration) in facet J.</rdfs:comment>
	<oboInOwl:hasDbXref>LANGUAL:A1091</oboInOwl:hasDbXref>
</owl:Class>

<owl:Class rdf:about="&obo;FOODON_03401092">
	<rdfs:label xml:lang="en">10000297 - grain based products - not ready to eat - savoury (shelf stable) (gs1 gpc)</rdfs:label>
	<rdfs:subClassOf rdf:resource="&obo;FOODON_03401089"/>
	<obo:IAO_0000412>http://langual.org</obo:IAO_0000412>
	<obo:IAO_0000115 xml:lang="en">Includes any products that can be described/observed as a savoury grain-based not ready to eat, prepared product, such as Rice, Polenta or Couscous in combination with other ingredients, such as meat, eggs, fish or vegetables. These ingredients form a valuable part of the product, rather than just serve as a seasoning or flavouring, such as Chicken Tandoori with Pilau Rice. These products must not include any dough-based products. They may or may not contain a sauce. These products require cooking prior to consumption. These products have been treated or packaged in such a way as to extend their consumable life. Specifically excludes all unprepared dried rice. Excludes products such as Frozen and Perishable Ready to Eat and Not Ready to Eat Grain Based Prepared Products, Unprepared Grains.</obo:IAO_0000115>
	<obo:IAO_0000114 rdf:resource="&obo;IAO_0000428"/>
	<rdfs:comment xml:lang="en">LanguaL curation note: Index main ingredient in facets B (fruit, poultry) and C (egg, milk). Index added ingredients in facet H. Index packing medium (sauce) in facet K. Index fat claim (full fat, reduced fat, low fat) and organic claim in Facet P.</rdfs:comment>
	<oboInOwl:hasDbXref>LANGUAL:A1092</oboInOwl:hasDbXref>
</owl:Class>

<owl:Class rdf:about="&obo;FOODON_03401093">
	<rdfs:label xml:lang="en">10000293 - grain based products - ready to eat - savoury (perishable) (gs1 gpc)</rdfs:label>
	<rdfs:subClassOf rdf:resource="&obo;FOODON_03401089"/>
	<obo:IAO_0000412>http://langual.org</obo:IAO_0000412>
	<obo:IAO_0000115 xml:lang="en">Includes any products that can be described/observed as a savoury grain-based ready to eat, prepared product, such as Rice, Polenta or Couscous in combination with other ingredients, such as meat, eggs, fish or vegetables. These ingredients form a valuable part of the product, rather than just serve as a seasoning or flavouring, such as Couscous with Fish Salad. These products must not include any dough-based products. They may or may not contain a sauce. These products do not require cooking prior to consumption, but some products can be eaten hot after reheating. These products must be refrigerated to extend their consumable life. Specifically excludes all unprepared dried rice. Excludes products such as Shelf Stable Ready to Eat and all Not Ready to Eat Grain-Based Prepared Products, Unprepared Grains.</obo:IAO_0000115>
	<obo:IAO_0000114 rdf:resource="&obo;IAO_0000428"/>
	<rdfs:comment xml:lang="en">LanguaL curation note: Index main ingredient in facets B (fruit, poultry) and C (egg, milk). Index added ingredients in facet H. Index packing medium (sauce) in facet K. Index fat claim (full fat, reduced fat, low fat) and organic claim in Facet P. Index preservation method (refrigeration) in facet J.</rdfs:comment>
	<oboInOwl:hasDbXref>LANGUAL:A1093</oboInOwl:hasDbXref>
</owl:Class>

<owl:Class rdf:about="&obo;FOODON_03401094">
	<rdfs:label xml:lang="en">10000294 - grain based products - ready to eat - savoury (shelf stable) (gs1 gpc)</rdfs:label>
	<rdfs:subClassOf rdf:resource="&obo;FOODON_03401089"/>
	<obo:IAO_0000412>http://langual.org</obo:IAO_0000412>
	<obo:IAO_0000115 xml:lang="en">Includes any products that can be described/observed as a savoury grain-based ready to eat, prepared product, such as Rice, Polenta or Couscous in combination with other ingredients, such as meat, eggs, fish or vegetables. These ingredients form a valuable part of the product, rather than just serve as a seasoning or flavouring, such as Tuna with Rice. These products must not include any dough-based products. They may or may not contain a sauce. These products do not require cooking prior to consumption, but some products can be eaten hot after reheating. These products have been treated or packaged in such a way as to extend their consumable life. Specifically excludes all unprepared dried rice. Excludes products such as Perishable Ready to Eat and Not Ready to Eat Grain Based Prepared Products and Unprepared Grains.</obo:IAO_0000115>
	<obo:IAO_0000114 rdf:resource="&obo;IAO_0000428"/>
	<rdfs:comment xml:lang="en">LanguaL curation note: Index main ingredient in facets B (fruit, poultry) and C (egg, milk). Index added ingredients in facet H. Index packing medium (sauce) in facet K. Index fat claim (full fat, reduced fat, low fat) and organic claim in Facet P.</rdfs:comment>
	<oboInOwl:hasDbXref>LANGUAL:A1094</oboInOwl:hasDbXref>
</owl:Class>

<owl:Class rdf:about="&obo;FOODON_03401095">
	<rdfs:label xml:lang="en">50192900 - pasta/noodles  (gs1 gpc)</rdfs:label>
	<rdfs:subClassOf rdf:resource="&obo;FOODON_03401061"/>
	<obo:IAO_0000412>http://langual.org</obo:IAO_0000412>
	<obo:IAO_0000114 rdf:resource="&obo;IAO_0000428"/>
	<oboInOwl:hasDbXref>LANGUAL:A1095</oboInOwl:hasDbXref>
</owl:Class>

<owl:Class rdf:about="&obo;FOODON_03401096">
	<rdfs:label xml:lang="en">10000318 - pasta/noodles - not ready to eat (frozen) (gs1 gpc)</rdfs:label>
	<rdfs:subClassOf rdf:resource="&obo;FOODON_03401095"/>
	<obo:IAO_0000412>http://langual.org</obo:IAO_0000412>
	<obo:IAO_0000115 xml:lang="en">Includes any products that can be described/observed, as a savoury pasta, noodle or gnocchi not ready to eat product. These products must not include any additional ingredients such as vegetables, protein or a sauce, and must not be part of a recipe prior to sale. These products are not ready to eat and require cooking prior to consumption. These products must be frozen to extend their consumable life. Specifically excludes all dough based prepared products such as Spaghetti Bolognaise. Excludes products such as Perishable and Shelf Not Ready to Eat and all Ready to Eat Pasta and Noodles and all Dough Based Prepared Recipe Products.</obo:IAO_0000115>
	<obo:IAO_0000114 rdf:resource="&obo;IAO_0000428"/>
	<rdfs:comment xml:lang="en">LanguaL curation note: Index country of origin in facet R. Index cereal in facets B (durumm wheat) and C (whole wheat). If flavoured or added ingredient, index in facet H. Index use claims (gluten free, vegetarians/vegans) in facet P.</rdfs:comment>
	<oboInOwl:hasDbXref>LANGUAL:A1096</oboInOwl:hasDbXref>
</owl:Class>

<owl:Class rdf:about="&obo;FOODON_03401097">
	<rdfs:label xml:lang="en">10000317 - pasta/noodles - not ready to eat (perishable) (gs1 gpc)</rdfs:label>
	<rdfs:subClassOf rdf:resource="&obo;FOODON_03401095"/>
	<obo:IAO_0000412>http://langual.org</obo:IAO_0000412>
	<obo:IAO_0000115 xml:lang="en">Includes any products that can be described/observed, as a savoury pasta, noodle or gnocchi not ready to eat product. These products must not include any additional ingredients such as vegetables, protein or a sauce, and must not be part of a recipe prior to sale. These products are not ready to eat and require cooking prior to consumption. These products must be refrigerated to extend their consumable life. Specifically excludes all dough based prepared products such as Spaghetti Bolognaise. Excludes products such as Frozen and Shelf Not Ready to Eat and all Ready to Eat Pasta and Noodles and all Dough Based Prepared Recipe Products.</obo:IAO_0000115>
	<obo:IAO_0000114 rdf:resource="&obo;IAO_0000428"/>
	<rdfs:comment xml:lang="en">LanguaL curation note: Index country of origin in facet R. Index cereal in facets B (durumm wheat) and C (whole wheat). If flavoured or added ingredient, index in facet H. Index use claims (gluten free, vegetarians/vegans) in facet P. Index preservation method (refrigeration) in facet J.</rdfs:comment>
	<oboInOwl:hasDbXref>LANGUAL:A1097</oboInOwl:hasDbXref>
</owl:Class>

<owl:Class rdf:about="&obo;FOODON_03401098">
	<rdfs:label xml:lang="en">10000242 - pasta/noodles - not ready to eat (shelf stable) (gs1 gpc)</rdfs:label>
	<rdfs:subClassOf rdf:resource="&obo;FOODON_03401095"/>
	<obo:IAO_0000412>http://langual.org</obo:IAO_0000412>
	<obo:IAO_0000115 xml:lang="en">Includes any products that can be described/observed as a savoury pasta, noodle or gnocchi not ready to eat product. These products must not include any additional ingredients such as vegetables, protein or a sauce, and must not be part of a recipe prior to sale. These products are not ready to eat and require cooking prior to consumption. These products have been treated or packaged in such a way to extend their consumable life. Specifically excludes all dough based prepared products such as Spaghetti Bolognaise. Excludes products such as Perishable and Frozen Not Ready to Eat and all Ready to Eat Pasta, Noodles and Gnocchi and all Dough Based Prepared Recipe Products.</obo:IAO_0000115>
	<obo:IAO_0000114 rdf:resource="&obo;IAO_0000428"/>
	<rdfs:comment xml:lang="en">LanguaL curation note: Index country of origin in facet R. Index cereal in facets B (durumm wheat) and C (whole wheat). If flavoured or added ingredient, index in facet H. Index use claims (gluten free, vegetarians/vegans) in facet P.</rdfs:comment>
	<oboInOwl:hasDbXref>LANGUAL:A1098</oboInOwl:hasDbXref>
</owl:Class>

<owl:Class rdf:about="&obo;FOODON_03401099">
	<rdfs:label xml:lang="en">10000240 - pasta/noodles - ready to eat (perishable) (gs1 gpc)</rdfs:label>
	<rdfs:subClassOf rdf:resource="&obo;FOODON_03401095"/>
	<obo:IAO_0000412>http://langual.org</obo:IAO_0000412>
	<obo:IAO_0000115 xml:lang="en">Includes any products that can be described/observed as a savoury pasta, noodle or gnocchi ready to eat product. These products must not include any additional ingredients such as vegetables, protein or a sauce, and must not be part of a recipe prior to sale. These products do not require cooking prior to consumption, but some products can be reheated. These products must be refrigerated to extend their consumable life. Specifically excludes all dough based prepared products such as Tuna Pasta Salad. Excludes products such as Shelf Stable Ready to Eat, and Not Ready to Eat Pasta and Noodles and all Prepared Dough Based Recipe Products.</obo:IAO_0000115>
	<obo:IAO_0000114 rdf:resource="&obo;IAO_0000428"/>
	<rdfs:comment xml:lang="en">LanguaL curation note: Index cereal in facets B (durumm wheat) and C (whole wheat). If flavoured or added ingredient, index in facet H. Index use claims (gluten free, vegetarians/vegans) and organic claim in facet P. Index preservation method (refrigeration) in facet J.</rdfs:comment>
	<oboInOwl:hasDbXref>LANGUAL:A1099</oboInOwl:hasDbXref>
</owl:Class>

<owl:Class rdf:about="&obo;FOODON_03401100">
	<rdfs:label xml:lang="en">10000241 - pasta/noodles - ready to eat (shelf stable) (gs1 gpc)</rdfs:label>
	<rdfs:subClassOf rdf:resource="&obo;FOODON_03401095"/>
	<obo:IAO_0000412>http://langual.org</obo:IAO_0000412>
	<obo:IAO_0000115 xml:lang="en">Includes any products that can be described/observed as a savoury pasta, noodle or gnocchi ready to eat product. These products must not include any additional ingredients such as vegetables, protein or a sauce, and must not be part of a recipe prior to sale. These products do not require cooking prior to consumption, but some products can be reheated. These products have been treated or packaged in such a way to extend their consumable life. Specifically excludes all dough based prepared products such as Tuna Pasta Salad. Excludes products such as Perishable Ready to Eat and Not Ready to Eat Pasta and Noodles and all Dough Based Prepared Recipe Products.</obo:IAO_0000115>
	<obo:IAO_0000114 rdf:resource="&obo;IAO_0000428"/>
	<rdfs:comment xml:lang="en">LanguaL curation note: Index cereal in facets B (durumm wheat) and C (whole wheat). If flavoured or added ingredient, index in facet H. Index use claims (gluten free, vegetarians/vegans) and organic claim in facet P.</rdfs:comment>
	<oboInOwl:hasDbXref>LANGUAL:A1100</oboInOwl:hasDbXref>
</owl:Class>

<owl:Class rdf:about="&obo;FOODON_03401101">
	<rdfs:label xml:lang="en">50191500 - prepared soups (gs1 gpc)</rdfs:label>
	<rdfs:subClassOf rdf:resource="&obo;FOODON_03401061"/>
	<obo:IAO_0000412>http://langual.org</obo:IAO_0000412>
	<obo:IAO_0000114 rdf:resource="&obo;IAO_0000428"/>
	<oboInOwl:hasDbXref>LANGUAL:A1101</oboInOwl:hasDbXref>
</owl:Class>

<owl:Class rdf:about="&obo;FOODON_03401102">
	<rdfs:label xml:lang="en">10000260 - soups - prepared (frozen) (gs1 gpc)</rdfs:label>
	<rdfs:subClassOf rdf:resource="&obo;FOODON_03401101"/>
	<obo:IAO_0000412>http://langual.org</obo:IAO_0000412>
	<obo:IAO_0000115 xml:lang="en">Includes any products that can be described/observed as a liquid food made from the stock of meat, fish and/or vegetables, which may also contain some small solid pieces of meat, fish and/or vegetables. These products must be frozen to extend their consumable life. Excludes products such as Shelf Stable and Perishable Prepared Soups.</obo:IAO_0000115>
	<obo:IAO_0000114 rdf:resource="&obo;IAO_0000428"/>
	<rdfs:comment xml:lang="en">LanguaL curation note: Index use claims (vegetarians/vegans) and organic claim in facet P. If condensed, index in facet H.</rdfs:comment>
	<oboInOwl:hasDbXref>LANGUAL:A1102</oboInOwl:hasDbXref>
</owl:Class>

<owl:Class rdf:about="&obo;FOODON_03401103">
	<rdfs:label xml:lang="en">10000261 - soups - prepared (perishable) (gs1 gpc)</rdfs:label>
	<rdfs:subClassOf rdf:resource="&obo;FOODON_03401101"/>
	<obo:IAO_0000412>http://langual.org</obo:IAO_0000412>
	<obo:IAO_0000115 xml:lang="en">Includes any products that can be described/observed as liquid food made from the stock of meat, fish and/or vegetables, which may also contain some small solid pieces of meat, fish and/or vegetables. These products must be refrigerated to extend their consumable life. Includes only Prepared Soups. Excludes products such as Shelf Stable and Frozen Prepared Soups.</obo:IAO_0000115>
	<obo:IAO_0000114 rdf:resource="&obo;IAO_0000428"/>
	<rdfs:comment xml:lang="en">LanguaL curation note: Index use claims (vegetarians/vegans) and organic claim in facet P. If condensed, index in facet H. Index preservation method (refrigeration) in facet J.</rdfs:comment>
	<oboInOwl:hasDbXref>LANGUAL:A1103</oboInOwl:hasDbXref>
</owl:Class>

<owl:Class rdf:about="&obo;FOODON_03401104">
	<rdfs:label xml:lang="en">10000262 - soups - prepared (shelf stable) (gs1 gpc)</rdfs:label>
	<rdfs:subClassOf rdf:resource="&obo;FOODON_03401101"/>
	<obo:IAO_0000412>http://langual.org</obo:IAO_0000412>
	<obo:IAO_0000115 xml:lang="en">Includes any products that can be described/observed as food made from the stock of meat, fish and/or vegetables, which may also contain some small solid pieces of meat, fish and/or vegetables. These products have been treated or packaged in such a way as to extend their consumable life. Includes also instant soups. Excludes products such as Perishable and Frozen Prepared Soups.</obo:IAO_0000115>
	<obo:IAO_0000114 rdf:resource="&obo;IAO_0000428"/>
	<rdfs:comment xml:lang="en">LanguaL curation note: Index physical form (liquid, powder) in facet E. Index use claims (vegetarians/vegans) and organic claim in facet P. If instant or condensed, index in facet H.</rdfs:comment>
	<oboInOwl:hasDbXref>LANGUAL:A1104</oboInOwl:hasDbXref>
</owl:Class>

<owl:Class rdf:about="&obo;FOODON_03401105">
	<rdfs:label xml:lang="en">50192500 - sandwiches/filled rolls/wraps (gs1 gpc)</rdfs:label>
	<rdfs:subClassOf rdf:resource="&obo;FOODON_03401061"/>
	<obo:IAO_0000412>http://langual.org</obo:IAO_0000412>
	<obo:IAO_0000114 rdf:resource="&obo;IAO_0000428"/>
	<oboInOwl:hasDbXref>LANGUAL:A1105</oboInOwl:hasDbXref>
</owl:Class>

<owl:Class rdf:about="&obo;FOODON_03401106">
	<rdfs:label xml:lang="en">10000254 - sandwiches/filled rolls/wraps (frozen) (gs1 gpc)</rdfs:label>
	<rdfs:subClassOf rdf:resource="&obo;FOODON_03401105"/>
	<obo:IAO_0000412>http://langual.org</obo:IAO_0000412>
	<obo:IAO_0000115 xml:lang="en">Includes any products that can be described/observed as a frozen leavened or unleavened, baked bread product from which slices, or the whole loaf, may be used to wrap or enclose a combination of one or more ingredients. These products must be frozen to extend their consumable life. Includes ready to eat products and products eaten hot or cold, once thawed. Excludes products such as Perishable Sandwiches, Filled Rolls and Wraps.</obo:IAO_0000115>
	<obo:IAO_0000114 rdf:resource="&obo;IAO_0000428"/>
	<rdfs:comment xml:lang="en">LanguaL curation note: Index use claims (vegetarians/vegans), fat level claims (low fat, reduced fat) and organic claim in facet P.</rdfs:comment>
	<oboInOwl:hasDbXref>LANGUAL:A1106</oboInOwl:hasDbXref>
</owl:Class>

<owl:Class rdf:about="&obo;FOODON_03401107">
	<rdfs:label xml:lang="en">10000255 - sandwiches/filled rolls/wraps (perishable) (gs1 gpc)</rdfs:label>
	<rdfs:subClassOf rdf:resource="&obo;FOODON_03401105"/>
	<obo:IAO_0000412>http://langual.org</obo:IAO_0000412>
	<obo:IAO_0000115 xml:lang="en">Includes any products that can be described/observed as a leavened or unleavened, baked bread product from which slices, or the whole loaf, may be used to wrap or enclose one or more ingredients. These products must be refrigerated to extend their consumable life. Includes ready to eat products and products eaten hot or cold. Excludes products such as Frozen Sandwiches Filled Rolls and Wraps.</obo:IAO_0000115>
	<obo:IAO_0000114 rdf:resource="&obo;IAO_0000428"/>
	<rdfs:comment xml:lang="en">LanguaL curation note: Index use claims (vegetarians/vegans), fat level claims (low fat, reduced fat) and organic claim in facet P. Index preservation method (refrigeration) in facet J.</rdfs:comment>
	<oboInOwl:hasDbXref>LANGUAL:A1107</oboInOwl:hasDbXref>
</owl:Class>

<owl:Class rdf:about="&obo;FOODON_03401108">
	<rdfs:label xml:lang="en">50192100 - snacks (gs1 gpc)</rdfs:label>
	<rdfs:subClassOf rdf:resource="&obo;FOODON_03401061"/>
	<obo:IAO_0000412>http://langual.org</obo:IAO_0000412>
	<obo:IAO_0000114 rdf:resource="&obo;IAO_0000428"/>
	<oboInOwl:hasDbXref>LANGUAL:A1108</oboInOwl:hasDbXref>
</owl:Class>

<owl:Class rdf:about="&obo;FOODON_03401109">
	<rdfs:label xml:lang="en">10000177 - chips/crisps/snack mixes - natural/extruded (shelf stable) (gs1 gpc)</rdfs:label>
	<rdfs:subClassOf rdf:resource="&obo;FOODON_03401108"/>
	<obo:IAO_0000412>http://langual.org</obo:IAO_0000412>
	<obo:IAO_0000115 xml:lang="en">Includes any products that can be described/observed as a type of food usually consumed between meals. They can contain, extracts from potatoes or other vegetables, gram flour products, rice, pulses and fruit, which are blended with other ingredients, reconstituted, and pressed into bite size shapes, or sliced products, which are fried in oil or oven-baked. These products are usually packaged in airtight bags, tubes, or plastic containers. Includes products such as Bombay Mix. Excludes products such as Popcorn, Prepared and Processed Vegetables and Prepared and Processed Meat, Poultry and Game and hot snacks.</obo:IAO_0000115>
	<obo:IAO_0000114 rdf:resource="&obo;IAO_0000428"/>
	<rdfs:comment xml:lang="en">LanguaL curation note: Index fat level claims (low fat, reduced fat) and organic claim in facet P. Index type of chips/snacks (maize, potato) in facet B. Index Manufacturers Treatment/Cooking Process in facets H (salted, seasoned) and G (fried, baked).</rdfs:comment>
	<oboInOwl:hasDbXref>LANGUAL:A1109</oboInOwl:hasDbXref>
</owl:Class>

<owl:Class rdf:about="&obo;FOODON_03401110">
	<rdfs:label xml:lang="en">10000252 - popcorn (shelf stable) (gs1 gpc)</rdfs:label>
	<rdfs:subClassOf rdf:resource="&obo;FOODON_03401108"/>
	<obo:IAO_0000412>http://langual.org</obo:IAO_0000412>
	<obo:IAO_0000115 xml:lang="en">Includes any products that can be described/observed as a type of food usually consumed between meals, made from maize (corn). Includes both unpopped corn that requires heating and popped corn that has been heated until it bursts and puffs out. Excludes products such as Other Grain Based Snacks, and Not Ready to Eat Cereals.</obo:IAO_0000115>
	<obo:IAO_0000114 rdf:resource="&obo;IAO_0000428"/>
	<rdfs:comment xml:lang="en">LanguaL curation note: Index added flavour or ingredients (sugar, salt) in facet H. Index fat level claims (low fat, reduced fat) and organic claim in facet P.</rdfs:comment>
	<oboInOwl:hasDbXref>LANGUAL:A1110</oboInOwl:hasDbXref>
</owl:Class>

<owl:Class rdf:about="&obo;FOODON_03401111">
	<rdfs:label xml:lang="en">10000612 - snacks variety packs (gs1 gpc)</rdfs:label>
	<rdfs:subClassOf rdf:resource="&obo;FOODON_03401108"/>
	<obo:IAO_0000412>http://langual.org</obo:IAO_0000412>
	<obo:IAO_0000115 xml:lang="en">Includes any products that can be described/observed as two or more distinct Snacks sold together, which exist within the schema belonging to different bricks but to the same class, that is two or more products contained within the same pack which cross bricks within the Snacks class. Includes products such as Crisps and Popcorn sold together. Items that are received free with purchases should be removed from the classification decision-making process. Excludes products such as Chips and Dips variety packs.</obo:IAO_0000115>
	<obo:IAO_0000114 rdf:resource="&obo;IAO_0000428"/>
	<oboInOwl:hasDbXref>LANGUAL:A1111</oboInOwl:hasDbXref>
</owl:Class>

<owl:Class rdf:about="&obo;FOODON_03401112">
	<rdfs:label xml:lang="en">50192400 - sweet spreads (gs1 gpc)</rdfs:label>
	<rdfs:subClassOf rdf:resource="&obo;FOODON_03401061"/>
	<obo:IAO_0000412>http://langual.org</obo:IAO_0000412>
	<obo:IAO_0000114 rdf:resource="&obo;IAO_0000428"/>
	<oboInOwl:hasDbXref>LANGUAL:A1112</oboInOwl:hasDbXref>
</owl:Class>

<owl:Class rdf:about="&obo;FOODON_03401113">
	<rdfs:label xml:lang="en">10000187 - confectionery based spreads (shelf stable) (gs1 gpc)</rdfs:label>
	<rdfs:subClassOf rdf:resource="&obo;FOODON_03401112"/>
	<obo:IAO_0000412>http://langual.org</obo:IAO_0000412>
	<obo:IAO_0000115 xml:lang="en">Includes any products that can be described/observed as spreadable liquid confection specifically intended for use as a filling for sandwiches and cakes, or to be spread on toast, croissants and biscuits. These products have been treated or packaged in such a way as to extend their consumable life. Includes nut based, chocolate based and combination based spreads. Excludes products such as Jams, Marmalades and Confitures and Honey Spreads.</obo:IAO_0000115>
	<obo:IAO_0000114 rdf:resource="&obo;IAO_0000428"/>
	<rdfs:comment xml:lang="en">LanguaL curation note: Index use claim (diabetic), calorie claims (low calorie), fat level claims (low fat, reduced fat) and organic claim in facet P. Index main ingredient (chocolate, nut) in facet B and additional ingredients (milk) in facet H.</rdfs:comment>
	<oboInOwl:hasDbXref>LANGUAL:A1113</oboInOwl:hasDbXref>
</owl:Class>

<owl:Class rdf:about="&obo;FOODON_03401114">
	<rdfs:label xml:lang="en">10000213 - honey (shelf stable) (gs1 gpc)</rdfs:label>
	<rdfs:subClassOf rdf:resource="&obo;FOODON_03401112"/>
	<obo:IAO_0000412>http://langual.org</obo:IAO_0000412>
	<obo:IAO_0000115 xml:lang="en">Includes any products that can be described/observed as a sweet spreadable liquid made by honey bees from the nectar of flowers. Includes dried honey, honey spreads, honey with added ingredients and other honey bee products, such as honey bee pollen. Excludes products such as Jams, Marmalades, Confitures and Confectionery Based Spreads.</obo:IAO_0000115>
	<obo:IAO_0000114 rdf:resource="&obo;IAO_0000428"/>
	<rdfs:comment xml:lang="en">LanguaL curation note: Index added ingredients in facet H. Index country of origin in facet R. If an industry recognized organic certification is claimed, index ORGANIC FOOD CLAIM OR USE in facet P. Index physical form (liquid, solid) in facet E. Index origin of honey (acacia, thyme) in facet B.</rdfs:comment>
	<oboInOwl:hasDbXref>LANGUAL:A1114</oboInOwl:hasDbXref>
</owl:Class>

<owl:Class rdf:about="&obo;FOODON_03401115">
	<rdfs:label xml:lang="en">10000217 - jams/marmalades/confiture (shelf stable) (gs1 gpc)</rdfs:label>
	<rdfs:subClassOf rdf:resource="&obo;FOODON_03401112"/>
	<obo:IAO_0000412>http://langual.org</obo:IAO_0000412>
	<obo:IAO_0000115 xml:lang="en">Includes any products that can be described/observed as a sweet semi firm liquid, usually used as a spread, made by cooking and preserving crushed fruit in sugar, and allowing the mixture to set, often with the addition of setting agents. Includes jams, jellies, marmalades and confitures. Excludes products such as Confectionery Based Spreads and Honey.</obo:IAO_0000115>
	<obo:IAO_0000114 rdf:resource="&obo;IAO_0000428"/>
	<rdfs:comment xml:lang="en">LanguaL curation note: Index use claim (diabetic), calorie claims (low calorie), and organic claim in facet P. Index added flavours and ingredients in facet H.</rdfs:comment>
	<oboInOwl:hasDbXref>LANGUAL:A1115</oboInOwl:hasDbXref>
</owl:Class>

<owl:Class rdf:about="&obo;FOODON_03401116">
	<rdfs:label xml:lang="en">10000621 - sweet spreads variety packs (gs1 gpc)</rdfs:label>
	<rdfs:subClassOf rdf:resource="&obo;FOODON_03401112"/>
	<obo:IAO_0000412>http://langual.org</obo:IAO_0000412>
	<obo:IAO_0000115 xml:lang="en">Includes any products that can be described/observed as two or more distinct Sweet Spreads sold together, which exist within the schema belonging to different bricks but to the same class, that is two or more products contained within the same pack which cross bricks within the Sweet Spreads class. Includes products such as Chocolate Spread and Jam sold together. Items that are received free with purchases should be removed from the classification decision-making process. Excludes products such as Jam and Tea variety packs.</obo:IAO_0000115>
	<obo:IAO_0000114 rdf:resource="&obo;IAO_0000428"/>
	<oboInOwl:hasDbXref>LANGUAL:A1116</oboInOwl:hasDbXref>
</owl:Class>

<owl:Class rdf:about="&obo;FOODON_03401117">
	<rdfs:label xml:lang="en">50193100 - vegetable based products (gs1 gpc)</rdfs:label>
	<rdfs:subClassOf rdf:resource="&obo;FOODON_03401061"/>
	<obo:IAO_0000412>http://langual.org</obo:IAO_0000412>
	<obo:IAO_0000114 rdf:resource="&obo;IAO_0000428"/>
	<oboInOwl:hasDbXref>LANGUAL:A1117</oboInOwl:hasDbXref>
</owl:Class>

<owl:Class rdf:about="&obo;FOODON_03401118">
	<rdfs:label xml:lang="en">10000291 - vegetable based products - not ready to eat (frozen) (gs1 gpc)</rdfs:label>
	<rdfs:subClassOf rdf:resource="&obo;FOODON_03401117"/>
	<obo:IAO_0000412>http://langual.org</obo:IAO_0000412>
	<obo:IAO_0000115 xml:lang="en">Includes any products that can be described/observed as a vegetable based not ready to eat, prepared product, such as Potato, Cabbage, Eggplant or any other vegetable in combination with other ingredients, such as meat, poultry or fish. These ingredients form a valuable part of the product rather than just serve as a seasoning or flavouring, such as Chicken Breast with Steamed Vegetables. These products must not include any dough, grain, dairy or egg based products. They may or may not contain a sauce. These products require cooking prior to consumption. These products must be frozen to extend their consumable life. Specifically excludes all prepared and processed and unprepared and unprocessed vegetables to which no recipe has been applied. Excludes products such as Shelf Stable and Perishable Not Ready to Eat and Ready to Eat Vegetable-Based Prepared Products and all Prepared and Processed Vegetables.</obo:IAO_0000115>
	<obo:IAO_0000114 rdf:resource="&obo;IAO_0000428"/>
	<rdfs:comment xml:lang="en">LanguaL curation note: Index main ingredient in facets B (fruit, poultry) and C (egg, milk). Index added ingredients in facet H. Index packing medium (sauce) in facet K. Index fat claim (full fat, reduced fat, low fat) and organic claim in Facet P.</rdfs:comment>
	<oboInOwl:hasDbXref>LANGUAL:A1118</oboInOwl:hasDbXref>
</owl:Class>

<owl:Class rdf:about="&obo;FOODON_03401119">
	<rdfs:label xml:lang="en">10000290 - vegetable based products - not ready to eat (perishable) (gs1 gpc)</rdfs:label>
	<rdfs:subClassOf rdf:resource="&obo;FOODON_03401117"/>
	<obo:IAO_0000412>http://langual.org</obo:IAO_0000412>
	<obo:IAO_0000115 xml:lang="en">Includes any products that can be described/observed as a vegetable based not ready to eat, prepared product, such as Potato, Cabbage, Eggplant or any other vegetable in combination with other ingredients, such as meat, poultry or fish. These ingredients form a valuable part of the product rather than just serve as a seasoning or flavouring, such as Chicken Breast with Steamed Vegetables. These products must not include any dough, grain, dairy or egg based products. They may or may not contain a sauce. These products require cooking prior to consumption. These products must be refrigerated to extend their consumable life. Specifically excludes all prepared and processed and unprepared and unprocessed vegetables to which no recipe has been applied. Excludes products such as Shelf Stable and Frozen Not Ready to Eat and Ready to Eat Vegetable-Based Prepared Products and all Prepared and Processed Vegetables.</obo:IAO_0000115>
	<obo:IAO_0000114 rdf:resource="&obo;IAO_0000428"/>
	<rdfs:comment xml:lang="en">LanguaL curation note: Index main ingredient in facets B (fruit, poultry) and C (egg, milk). Index added ingredients in facet H. Index packing medium (sauce) in facet K. Index fat claim (full fat, reduced fat, low fat) and organic claim in Facet P. Index preservation method (refrigeration) in facet J.</rdfs:comment>
	<oboInOwl:hasDbXref>LANGUAL:A1119</oboInOwl:hasDbXref>
</owl:Class>

<owl:Class rdf:about="&obo;FOODON_03401120">
	<rdfs:label xml:lang="en">10000292 - vegetable based products - not ready to eat (shelf stable) (gs1 gpc)</rdfs:label>
	<rdfs:subClassOf rdf:resource="&obo;FOODON_03401117"/>
	<obo:IAO_0000412>http://langual.org</obo:IAO_0000412>
	<obo:IAO_0000115 xml:lang="en">Includes any products that can be described/observed as a vegetable based not ready to eat, prepared product, such as Potato, Cabbage, Eggplant or any other vegetable in combination with other ingredients, such as meat, poultry or fish. These ingredients form a valuable part of the product rather than just serve as a seasoning or flavouring, such as minced beef in a Shepherds Pie. These products must not include any dough, grain, dairy or egg based products. They may or may not contain a sauce. These products require cooking prior to consumption. These products have been specially treated or packaged to extend their consumable life. Specifically excludes all prepared and processed and unprepared and unprocessed vegetables to which no recipe has been applied. Excludes products such as Frozen and Perishable Not Ready to Eat and Ready to Eat Vegetable-Based Prepared Products and all Prepared and Processed Vegetables.</obo:IAO_0000115>
	<obo:IAO_0000114 rdf:resource="&obo;IAO_0000428"/>
	<rdfs:comment xml:lang="en">LanguaL curation note: Index main ingredient in facets B (fruit, poultry) and C (egg, milk). Index added ingredients in facet H. Index packing medium (sauce) in facet K. Index fat claim (full fat, reduced fat, low fat) and organic claim in Facet P.</rdfs:comment>
	<oboInOwl:hasDbXref>LANGUAL:A1120</oboInOwl:hasDbXref>
</owl:Class>

<owl:Class rdf:about="&obo;FOODON_03401121">
	<rdfs:label xml:lang="en">10000289 - vegetable based products - ready to eat (perishable) (gs1 gpc)</rdfs:label>
	<rdfs:subClassOf rdf:resource="&obo;FOODON_03401117"/>
	<obo:IAO_0000412>http://langual.org</obo:IAO_0000412>
	<obo:IAO_0000115 xml:lang="en">Includes any products that can be described/observed as a vegetable based ready to eat, prepared product, such as Potato, Cabbage, Eggplant or any other vegetable in combination with other ingredients, such as meat, poultry or fish. These ingredients form a valuable part of the product rather than just serve as a seasoning or flavouring, such as tuna in a Tuna Salad. These products must not include any dough, grain, dairy or egg based products. They may or may not contain a sauce. These products do not require cooking prior to consumption, but some products can be eaten hot after reheating. These products must be refrigerated to extend their consumable life. Specifically excludes all prepared and processed and unprepared and unprocessed vegetables to which no recipe has been applied. Excludes products such as Shelf Stable Ready to Eat and all Not Ready to Eat Vegetable-Based Prepared Products and all Prepared and Processed Vegetables.</obo:IAO_0000115>
	<obo:IAO_0000114 rdf:resource="&obo;IAO_0000428"/>
	<rdfs:comment xml:lang="en">LanguaL curation note: Index main ingredient in facets B (fruit, poultry) and C (egg, milk). Index added ingredients in facet H. Index packing medium (sauce) in facet K. Index fat claim (full fat, reduced fat, low fat) and organic claim in Facet P. Index preservation method (refrigeration) in facet J.</rdfs:comment>
	<oboInOwl:hasDbXref>LANGUAL:A1121</oboInOwl:hasDbXref>
</owl:Class>

<owl:Class rdf:about="&obo;FOODON_03401122">
	<rdfs:label xml:lang="en">10000288 - vegetable based products - ready to eat (shelf stable) (gs1 gpc)</rdfs:label>
	<rdfs:subClassOf rdf:resource="&obo;FOODON_03401117"/>
	<obo:IAO_0000412>http://langual.org</obo:IAO_0000412>
	<obo:IAO_0000115 xml:lang="en">Includes any products that can be described/observed as a vegetable based ready to eat, prepared product, such as Potato, Cabbage, Eggplant or any other vegetable in combination with other ingredients, such as meat, poultry or fish. These ingredients form a valuable part of the product rather than just serve as a seasoning or flavouring, such as tuna in a Tuna Salad. These products must not include any dough, grain, dairy or egg based products. They may or may not contain a sauce. Products include ready to eat salads where the main ingredient is any type of vegetable. These products do not require cooking prior to consumption, but some products can be eaten hot after reheating. These products have been treated or packaged in such a way as to extend their consumable life. Specifically excludes all prepared and processed and unprepared and unprocessed vegetables to which no recipe has been applied. Excludes products such as Perishable Ready to Eat and Not Ready to Eat Vegetable Based Prepared Products and all Prepared and Processed Vegetables.</obo:IAO_0000115>
	<obo:IAO_0000114 rdf:resource="&obo;IAO_0000428"/>
	<rdfs:comment xml:lang="en">LanguaL curation note: Index main ingredient in facets B (fruit, poultry) and C (egg, milk). Index added ingredients in facet H. Index packing medium (sauce) in facet K. Index fat claim (full fat, reduced fat, low fat) and organic claim in Facet P.</rdfs:comment>
	<oboInOwl:hasDbXref>LANGUAL:A1122</oboInOwl:hasDbXref>
</owl:Class>

<owl:Class rdf:about="&obo;FOODON_03401123">
	<rdfs:label xml:lang="en">50193400 - prepared/preserved foods variety packs (gs1 gpc)</rdfs:label>
	<rdfs:subClassOf rdf:resource="&obo;FOODON_03401061"/>
	<obo:IAO_0000412>http://langual.org</obo:IAO_0000412>
	<obo:IAO_0000115 xml:lang="en">Includes any products that can be described/observed as two or more distinct Prepared and Preserved Foods sold together which exist within the schema but belong to different classes, that is two or more products contained within the same pack which cross classes within the Prepared and Preserved Foods Family. Includes products such as Chicken Korma and Ice Cream variety packs. Items that are received free with purchases should be removed from the classification decision-making process. Excludes products such as Jam and Chocolate Spread variety packs and Chips and Dips variety packs.</obo:IAO_0000115>
	<obo:IAO_0000114 rdf:resource="&obo;IAO_0000428"/>
	<oboInOwl:hasDbXref>LANGUAL:A1123</oboInOwl:hasDbXref>
</owl:Class>

<owl:Class rdf:about="&obo;FOODON_03401124">
	<rdfs:label xml:lang="en">50120000 - seafood (gs1 gpc)</rdfs:label>
	<rdfs:subClassOf rdf:resource="&obo;FOODON_03400874"/>
	<obo:IAO_0000412>http://langual.org</obo:IAO_0000412>
	<obo:IAO_0000114 rdf:resource="&obo;IAO_0000428"/>
	<oboInOwl:hasDbXref>LANGUAL:A1124</oboInOwl:hasDbXref>
</owl:Class>

<owl:Class rdf:about="&obo;FOODON_03401125">
	<rdfs:label xml:lang="en">50122000 - aquatic invertebrates - prepared/processed (gs1 gpc)</rdfs:label>
	<rdfs:subClassOf rdf:resource="&obo;FOODON_03401124"/>
	<obo:IAO_0000412>http://langual.org</obo:IAO_0000412>
	<obo:IAO_0000114 rdf:resource="&obo;IAO_0000428"/>
	<oboInOwl:hasDbXref>LANGUAL:A1125</oboInOwl:hasDbXref>
</owl:Class>

<owl:Class rdf:about="&obo;FOODON_03401126">
	<rdfs:label xml:lang="en">10000145 - aquatic invertebrates - prepared/processed (frozen) (gs1 gpc)</rdfs:label>
	<rdfs:subClassOf rdf:resource="&obo;FOODON_03401125"/>
	<obo:IAO_0000412>http://langual.org</obo:IAO_0000412>
	<obo:IAO_0000115 xml:lang="en">Includes any products that can be described/observed as any frozen edible animal, such as an insect or mollusc that lacks a backbone or spinal column and has no external shell, that lives in, on or near the water, that has gone through further manufacturing processes, such as reformed, cooked, dried and salted, however these products can also be coated, in sauce, stuffed or filled. Specifically excludes products that have added ingredients included such as vegetables, rice, couscous and pasta. These products must be frozen to extend their consumable life. Excludes products such as Aquatic Invertebrates with additional vegetables, dough or grains, Shelf Stable and Perishable Prepared and Processed Aquatic Invertebrates, all Unprepared and Unprocessed Aquatic Invertebrates.</obo:IAO_0000115>
	<obo:IAO_0000114 rdf:resource="&obo;IAO_0000428"/>
	<rdfs:comment xml:lang="en">LanguaL curation note: Index type of Aquatic Invertebrate (octopus, sea urchin) in facet B. If an industry recognized organic certification is claimed, index ORGANIC FOOD CLAIM OR USE in facet P. Index Manufacturers Treatment/Cooking Process in facets H (dried, salted) and F (cooked).</rdfs:comment>
	<oboInOwl:hasDbXref>LANGUAL:A1126</oboInOwl:hasDbXref>
</owl:Class>

<owl:Class rdf:about="&obo;FOODON_03401127">
	<rdfs:label xml:lang="en">10000146 - aquatic invertebrates - prepared/processed (perishable) (gs1 gpc)</rdfs:label>
	<rdfs:subClassOf rdf:resource="&obo;FOODON_03401125"/>
	<obo:IAO_0000412>http://langual.org</obo:IAO_0000412>
	<obo:IAO_0000115 xml:lang="en">Includes any products that can be described/observed as any edible animal, such as an insect or mollusc that lacks a backbone or spinal column and has no external shell, that lives in, on or near the water, that has gone through further manufacturing processes, such as reformed, cooked, dried and salted, however these products can also be coated, in sauce, stuffed or filled. Specifically excludes products that have added ingredients included such as vegetables, rice, couscous and pasta. These products must be refrigerated to extend their consumable life. Excludes products such as Aquatic Invertebrates with additional vegetables, dough or grains, Frozen and Shelf Stable Prepared and Processed Aquatic Invertebrates, all Unprepared and Unprocessed Aquatic Invertebrates.</obo:IAO_0000115>
	<obo:IAO_0000114 rdf:resource="&obo;IAO_0000428"/>
	<rdfs:comment xml:lang="en">LanguaL curation note: Index type of Aquatic Invertebrate (octopus, sea urchin) in facet B. If an industry recognized organic certification is claimed, index ORGANIC FOOD CLAIM OR USE in facet P. Index Manufacturers Treatment/Cooking Process in facets H (dried, salted) and F (cooked). Index preservation method (refrigeration) in facet J.</rdfs:comment>
	<oboInOwl:hasDbXref>LANGUAL:A1127</oboInOwl:hasDbXref>
</owl:Class>

<owl:Class rdf:about="&obo;FOODON_03401128">
	<rdfs:label xml:lang="en">10000147 - aquatic invertebrates - prepared/processed (shelf stable) (gs1 gpc)</rdfs:label>
	<rdfs:subClassOf rdf:resource="&obo;FOODON_03401125"/>
	<obo:IAO_0000412>http://langual.org</obo:IAO_0000412>
	<obo:IAO_0000115 xml:lang="en">Includes any products that can be described/observed as any edible animal, such as an insect or mollusc that lacks a backbone or spinal column and has no external shell, that lives in, on or near the water, that has gone through further manufacturing processes, such as reformed, cooked, dried and salted, however these products can also be coated, in sauce, stuffed or filled. Specifically excludes products that have added ingredients included such as vegetables, rice, couscous and pasta. These products have been treated or packaged in such a way as to extend their consumable life. Excludes products such as Aquatic Invertebrates with additional vegetables, dough or grains, Frozen and Perishable prepared and Processed Aquatic Invertebrates, all Unprepared and Unprocessed Aquatic Invertebrates.</obo:IAO_0000115>
	<obo:IAO_0000114 rdf:resource="&obo;IAO_0000428"/>
	<rdfs:comment xml:lang="en">LanguaL curation note: Index type of Aquatic Invertebrate (octopus, sea urchin) in facet B. If an industry recognized organic certification is claimed, index ORGANIC FOOD CLAIM OR USE in facet P. Index Manufacturers Treatment/Cooking Process in facets H (dried, salted) and F (cooked).</rdfs:comment>
	<oboInOwl:hasDbXref>LANGUAL:A1128</oboInOwl:hasDbXref>
</owl:Class>

<owl:Class rdf:about="&obo;FOODON_03401129">
	<rdfs:label xml:lang="en">50122300 - aquatic invertebrates - unprepared/unprocessed (gs1 gpc)</rdfs:label>
	<rdfs:subClassOf rdf:resource="&obo;FOODON_03401124"/>
	<obo:IAO_0000412>http://langual.org</obo:IAO_0000412>
	<obo:IAO_0000114 rdf:resource="&obo;IAO_0000428"/>
	<oboInOwl:hasDbXref>LANGUAL:A1129</oboInOwl:hasDbXref>
</owl:Class>

<owl:Class rdf:about="&obo;FOODON_03401130">
	<rdfs:label xml:lang="en">10000148 - aquatic invertebrates - unprepared/unprocessed (frozen) (gs1 gpc)</rdfs:label>
	<rdfs:subClassOf rdf:resource="&obo;FOODON_03401129"/>
	<obo:IAO_0000412>http://langual.org</obo:IAO_0000412>
	<obo:IAO_0000115 xml:lang="en">Includes any products that can be described/observed as any frozen edible animal, such as an insect or mollusc that lacks a backbone or spinal column and has no external shell, that lives in, on or near the water, that has not gone through any further manufacturing processes, such as reformed, cooked, dried and salted, however these products can be coated, in sauce, stuffed or filled. Specifically excludes products that have added ingredients included such as vegetables, rice, couscous and pasta. These products must be frozen to extend their consumable life. Excludes products such as Aquatic Invertebrates with additional vegetables, dough or grains, Shelf Stable and Perishable Unprepared and Unprocessed Aquatic Invertebrates, all Prepared and Processed Aquatic Invertebrates.</obo:IAO_0000115>
	<obo:IAO_0000114 rdf:resource="&obo;IAO_0000428"/>
	<rdfs:comment xml:lang="en">LanguaL curation note: Index type of Aquatic Invertebrate (octopus, sea urchin) in facet B. If an industry recognized organic certification is claimed, index ORGANIC FOOD CLAIM OR USE in facet P.</rdfs:comment>
	<oboInOwl:hasDbXref>LANGUAL:A1130</oboInOwl:hasDbXref>
</owl:Class>

<owl:Class rdf:about="&obo;FOODON_03401131">
	<rdfs:label xml:lang="en">10000149 - aquatic invertebrates - unprepared/unprocessed (perishable) (gs1 gpc)</rdfs:label>
	<rdfs:subClassOf rdf:resource="&obo;FOODON_03401129"/>
	<obo:IAO_0000412>http://langual.org</obo:IAO_0000412>
	<obo:IAO_0000115 xml:lang="en">Includes any products that can be described/observed as any fresh edible animal, such as an insect or mollusc that lacks a backbone or spinal column and has no external shell, that lives in, on or near the water, that has not gone through any further manufacturing processes, such as reformed, cooked, dried and salted, however these products can be coated, in sauce, stuffed or filled. Specifically excludes products that have added ingredients included such as vegetables, rice, couscous and pasta. These products must be refrigerated to extend their consumable life. Excludes products such as Aquatic Invertebrates with additional vegetables, dough or grains, Shelf Stable and Frozen Unprepared and Unprocessed Aquatic Invertebrates, all Prepared and Processed Aquatic Invertebrates.</obo:IAO_0000115>
	<obo:IAO_0000114 rdf:resource="&obo;IAO_0000428"/>
	<rdfs:comment xml:lang="en">LanguaL curation note: Index type of Aquatic Invertebrate (octopus, sea urchin) in facet B. If an industry recognized organic certification is claimed, index ORGANIC FOOD CLAIM OR USE in facet P. Index preservation method (refrigeration) in facet J.</rdfs:comment>
	<oboInOwl:hasDbXref>LANGUAL:A1131</oboInOwl:hasDbXref>
</owl:Class>

<owl:Class rdf:about="&obo;FOODON_03401132">
	<rdfs:label xml:lang="en">10000150 - aquatic invertebrates - unprepared/unprocessed (shelf stable) (gs1 gpc)</rdfs:label>
	<rdfs:subClassOf rdf:resource="&obo;FOODON_03401129"/>
	<obo:IAO_0000412>http://langual.org</obo:IAO_0000412>
	<obo:IAO_0000115 xml:lang="en">Includes any products that can be described/observed as any edible animal, such as an insect or mollusc that lacks a backbone or spinal column and has no external shell, that lives in, on or near the water, that has not gone through any further manufacturing processes, such as reformed, cooked, dried and salted, however these products can be coated, in sauce, stuffed or filled. Specifically excludes products that have added ingredients included such as vegetables, rice, couscous and pasta. These products have been treated or packaged in such a way as to extend their consumable life. Excludes products such as Aquatic Invertebrates with additional vegetables, dough or grains, Frozen and Perishable Unprepared and Unprocessed Aquatic Invertebrates, all Prepared and Processed Aquatic Invertebrates.</obo:IAO_0000115>
	<obo:IAO_0000114 rdf:resource="&obo;IAO_0000428"/>
	<rdfs:comment xml:lang="en">LanguaL curation note: Index type of Aquatic Invertebrate (octopus, sea urchin) in facet B. If an industry recognized organic certification is claimed, index ORGANIC FOOD CLAIM OR USE in facet P.</rdfs:comment>
	<oboInOwl:hasDbXref>LANGUAL:A1132</oboInOwl:hasDbXref>
</owl:Class>

<owl:Class rdf:about="&obo;FOODON_03401133">
	<rdfs:label xml:lang="en">50122500 - aquatic invertebrates/fish/shellfish/seafood combination (gs1 gpc)</rdfs:label>
	<rdfs:subClassOf rdf:resource="&obo;FOODON_03401124"/>
	<obo:IAO_0000412>http://langual.org</obo:IAO_0000412>
	<obo:IAO_0000114 rdf:resource="&obo;IAO_0000428"/>
	<oboInOwl:hasDbXref>LANGUAL:A1133</oboInOwl:hasDbXref>
</owl:Class>

<owl:Class rdf:about="&obo;FOODON_03401134">
	<rdfs:label xml:lang="en">10000626 - aquatic invertebrates/fish/shellfish/seafood mixes - prepared/processed (frozen) (gs1 gpc)</rdfs:label>
	<rdfs:subClassOf rdf:resource="&obo;FOODON_03401133"/>
	<obo:IAO_0000412>http://langual.org</obo:IAO_0000412>
	<obo:IAO_0000115 xml:lang="en">Includes any products that can be described/observed as a mix of any variety of Aquatic Invertebrate, Fish, Shellfish or Seafood, that has gone through further manufacturing processes, such as reformed, cooked, dried and salted, however these products can also be coated, in sauce, stuffed or filled. Specifically excludes products that have added ingredients included such as vegetables, rice, couscous and pasta. These products must be frozen to extend their consumable life. Excludes products such as Aquatic Invertebrates, Fish, Shellfish and Seafood Mixes with additional vegetables, dough or grains, Shelf Stable and Perishable Prepared and Processed Aquatic Invertebrates, Fish, Shellfish and Seafood Mixes, all Unprepared and Unprocessed Aquatic Invertebrates, Fish, Shellfish and Seafood Mixes.</obo:IAO_0000115>
	<obo:IAO_0000114 rdf:resource="&obo;IAO_0000428"/>
	<rdfs:comment xml:lang="en">LanguaL curation note: Index types of seafood in facets B and H (fish or shelfish added). If an industry recognized organic certification is claimed, index ORGANIC FOOD CLAIM OR USE in facet P. Index Manufacturers Treatment/Cooking Process in facets H (dried, salted) and F (cooked).</rdfs:comment>
	<oboInOwl:hasDbXref>LANGUAL:A1134</oboInOwl:hasDbXref>
</owl:Class>

<owl:Class rdf:about="&obo;FOODON_03401135">
	<rdfs:label xml:lang="en">10000627 - aquatic invertebrates/fish/shellfish/seafood mixes - prepared/processed (perishable) (gs1 gpc)</rdfs:label>
	<rdfs:subClassOf rdf:resource="&obo;FOODON_03401133"/>
	<obo:IAO_0000412>http://langual.org</obo:IAO_0000412>
	<obo:IAO_0000115 xml:lang="en">Includes any products that can be described/observed as a mix of any variety of Aquatic Invertebrate, Fish, shellfish or Seafood, that has gone through further manufacturing processes, such as reformed, cooked, dried and salted, however these products can also be coated, in sauce, stuffed or filled. Specifically excludes products that have added ingredients included such as vegetables, rice, couscous and pasta. These products must be refrigerated to extend their consumable life. Excludes products such as Aquatic Invertebrates, Fish, Shellfish and Seafood Mixes with additional vegetables, dough or grains, Shelf Stable and Frozen Prepared and Processed Aquatic Invertebrates, Fish, Shellfish and Seafood Mixes, all Unprepared and Unprocessed Aquatic Invertebrates, Fish, Shellfish and Seafood Mixes.</obo:IAO_0000115>
	<obo:IAO_0000114 rdf:resource="&obo;IAO_0000428"/>
	<rdfs:comment xml:lang="en">LanguaL curation note: Index types of seafood in facets B and H (fish or shelfish added). If an industry recognized organic certification is claimed, index ORGANIC FOOD CLAIM OR USE in facet P. Index Manufacturers Treatment/Cooking Process in facets H (dried, salted) and F (cooked). Index preservation method (refrigeration) in facet J.</rdfs:comment>
	<oboInOwl:hasDbXref>LANGUAL:A1135</oboInOwl:hasDbXref>
</owl:Class>

<owl:Class rdf:about="&obo;FOODON_03401136">
	<rdfs:label xml:lang="en">10000628 - aquatic invertebrates/fish/shellfish/seafood mixes - prepared/processed (shelf stable) (gs1 gpc)</rdfs:label>
	<rdfs:subClassOf rdf:resource="&obo;FOODON_03401133"/>
	<obo:IAO_0000412>http://langual.org</obo:IAO_0000412>
	<obo:IAO_0000115 xml:lang="en">Includes any products that can be described/observed as a mix of any variety of Aquatic Invertebrate, Fish, Shellfish or Seafood, that has gone through further manufacturing processes, such as reformed, cooked, dried and salted, however these products can also be coated, in sauce, stuffed or filled. Specifically excludes products that have added ingredients included such as vegetables, rice, couscous and pasta. These products have been specially treated or packaged to extend their consumable life. Excludes products such as Aquatic Invertebrates, Fish, Shellfish and Seafood Mixes with additional vegetables, dough or grains, Frozen and Perishable Prepared and Processed Aquatic Invertebrates, Fish, Shellfish and Seafood Mixes, all Unprepared and Unprocessed Aquatic Invertebrates, Fish, Shellfish and Seafood Mixes.</obo:IAO_0000115>
	<obo:IAO_0000114 rdf:resource="&obo;IAO_0000428"/>
	<rdfs:comment xml:lang="en">LanguaL curation note: Index types of seafood in facets B and H (fish or shelfish added). If an industry recognized organic certification is claimed, index ORGANIC FOOD CLAIM OR USE in facet P. Index Manufacturers Treatment/Cooking Process in facets H (dried, salted) and F (cooked).</rdfs:comment>
	<oboInOwl:hasDbXref>LANGUAL:A1136</oboInOwl:hasDbXref>
</owl:Class>

<owl:Class rdf:about="&obo;FOODON_03401137">
	<rdfs:label xml:lang="en">10000629 - aquatic invertebrates/fish/shellfish/seafood mixes - unprepared/unprocessed (frozen) (gs1 gpc)</rdfs:label>
	<rdfs:subClassOf rdf:resource="&obo;FOODON_03401133"/>
	<obo:IAO_0000412>http://langual.org</obo:IAO_0000412>
	<obo:IAO_0000115 xml:lang="en">Includes any products that can be described/observed as a mix of any variety of Aquatic Invertebrate, Fish, Shellfish or Seafood, that has not gone through further manufacturing processes such as reformed, cooked, dried and salted, however these products can be coated, in sauce, stuffed or filled. Specifically excludes products that have added ingredients included such as vegetables, rice, couscous and pasta. These products must be frozen to extend their consumable life. Excludes products such as Aquatic Invertebrates, Fish, Shellfish and Seafood Mixes with additional vegetables, dough or grains, Shelf Stable and Perishable Unprepared and Unprocessed Aquatic Invertebrates, Fish, Shellfish and Seafood Mixes, all Prepared and Processed Aquatic Invertebrates, Fish, Shellfish and Seafood Mixes.</obo:IAO_0000115>
	<obo:IAO_0000114 rdf:resource="&obo;IAO_0000428"/>
	<rdfs:comment xml:lang="en">LanguaL curation note: Index types of seafood in facets B and H (fish or shelfish added). If an industry recognized organic certification is claimed, index ORGANIC FOOD CLAIM OR USE in facet P.</rdfs:comment>
	<oboInOwl:hasDbXref>LANGUAL:A1137</oboInOwl:hasDbXref>
</owl:Class>

<owl:Class rdf:about="&obo;FOODON_03401138">
	<rdfs:label xml:lang="en">10000630 - aquatic invertebrates/fish/shellfish/seafood mixes - unprepared/unprocessed (perishable) (gs1 gpc)</rdfs:label>
	<rdfs:subClassOf rdf:resource="&obo;FOODON_03401133"/>
	<obo:IAO_0000412>http://langual.org</obo:IAO_0000412>
	<obo:IAO_0000115 xml:lang="en">Includes any products that can be described/observed as a mix of any variety of Aquatic Invertebrate, Fish, shellfish or Seafood, that has not gone through further manufacturing processes, such as reformed, cooked, dried and salted, however these products can be coated, in sauce, stuffed or filled. Specifically excludes products that have added ingredients included such as vegetables, rice, couscous and pasta. These products must be refrigerated to extend their consumable life. Excludes products such as Aquatic Invertebrates, Fish, Shellfish and Seafood Mixes with additional vegetables, dough or grains, Shelf Stable and Frozen Unprepared and Unprocessed Aquatic Invertebrates, Fish, Shellfish and Seafood Mixes, all Prepared and Processed Aquatic Invertebrates, Fish, Shellfish and Seafood Mixes.</obo:IAO_0000115>
	<obo:IAO_0000114 rdf:resource="&obo;IAO_0000428"/>
	<rdfs:comment xml:lang="en">LanguaL curation note: Index types of seafood in facets B and H (fish or shelfish added). If an industry recognized organic certification is claimed, index ORGANIC FOOD CLAIM OR USE in facet P. Index preservation method (refrigeration) in facet J.</rdfs:comment>
	<oboInOwl:hasDbXref>LANGUAL:A1138</oboInOwl:hasDbXref>
</owl:Class>

<owl:Class rdf:about="&obo;FOODON_03401139">
	<rdfs:label xml:lang="en">10000631 - aquatic invertebrates/fish/shellfish/seafood mixes - unprepared/unprocessed (shelf stable) (gs1 gpc)</rdfs:label>
	<rdfs:subClassOf rdf:resource="&obo;FOODON_03401133"/>
	<obo:IAO_0000412>http://langual.org</obo:IAO_0000412>
	<obo:IAO_0000115 xml:lang="en">Includes any products that can be described/observed as a mix of any variety of Aquatic Invertebrate, Fish, Shellfish or Seafood, that has not gone through further manufacturing processes, such as reformed, cooked, dried and salted, however these products can be coated, in sauce, stuffed or filled. Specifically excludes products that have added ingredients included such as vegetables, rice, couscous and pasta. These products have been specially treated or packaged to extend their consumable life. Excludes products such as Aquatic Invertebrates, Fish, Shellfish and Seafood Mixes with additional vegetables, dough or grains, Frozen and Perishable Unprepared and Unprocessed Aquatic Invertebrates, Fish, Shellfish and Seafood Mixes, all Prepared and Processed Aquatic Invertebrates, Fish, Shellfish and Seafood Mixes.</obo:IAO_0000115>
	<obo:IAO_0000114 rdf:resource="&obo;IAO_0000428"/>
	<rdfs:comment xml:lang="en">LanguaL curation note: Index types of seafood in facets B and H (fish or shelfish added). If an industry recognized organic certification is claimed, index ORGANIC FOOD CLAIM OR USE in facet P.</rdfs:comment>
	<oboInOwl:hasDbXref>LANGUAL:A1139</oboInOwl:hasDbXref>
</owl:Class>

<owl:Class rdf:about="&obo;FOODON_03401140">
	<rdfs:label xml:lang="en">50121900 - fish - prepared/processed (gs1 gpc)</rdfs:label>
	<rdfs:subClassOf rdf:resource="&obo;FOODON_03401124"/>
	<obo:IAO_0000412>http://langual.org</obo:IAO_0000412>
	<obo:IAO_0000114 rdf:resource="&obo;IAO_0000428"/>
	<oboInOwl:hasDbXref>LANGUAL:A1140</oboInOwl:hasDbXref>
</owl:Class>

<owl:Class rdf:about="&obo;FOODON_03401141">
	<rdfs:label xml:lang="en">10000017 - fish - prepared/processed (frozen) (gs1 gpc)</rdfs:label>
	<rdfs:subClassOf rdf:resource="&obo;FOODON_03401140"/>
	<obo:IAO_0000412>http://langual.org</obo:IAO_0000412>
	<obo:IAO_0000115 xml:lang="en">Includes any products that can be described/observed as any variety of fish or a combination of fish, that has gone through further manufacturing processes, such as reformed, cooked, dried and salted, however these products can also be coated, in sauce, stuffed or filled. Specifically excludes products that have added ingredients included such as rice, couscous and pasta. However products may contain a small quantity of vegetables such as those in a sauce or stuffing/filling. These products must be frozen to extend their consumable life. Excludes products such as Fish with additional vegetables, dough or grains, Shelf Stable and Perishable Prepared and Processed Fish, all Unprepared and Unprocessed Fish.</obo:IAO_0000115>
	<obo:IAO_0000114 rdf:resource="&obo;IAO_0000428"/>
	<rdfs:comment xml:lang="en">LanguaL curation note: Index type of fish (anchovy, tuna) in facet B and part of fish (half, tail, egg) in facet C. Index Manufacturers Treatment/Cooking Process in facets H (dried, salted) and F (cooked). Index coating and stuffing in facet H. Index packing medium in facet K.</rdfs:comment>
	<oboInOwl:hasDbXref>LANGUAL:A1141</oboInOwl:hasDbXref>
</owl:Class>

<owl:Class rdf:about="&obo;FOODON_03401142">
	<rdfs:label xml:lang="en">10000016 - fish - prepared/processed (perishable) (gs1 gpc)</rdfs:label>
	<rdfs:subClassOf rdf:resource="&obo;FOODON_03401140"/>
	<obo:IAO_0000412>http://langual.org</obo:IAO_0000412>
	<obo:IAO_0000115 xml:lang="en">Includes any products that can be described/observed as any variety of fish or a combination of fish, that has gone through further manufacturing processes, such as reformed, cooked, dried and salted, however these products can also be coated, in sauce, stuffed or filled. Specifically excludes products that have added ingredients included such as rice, couscous and pasta. However products may contain a small quantity of vegetables such as those in a sauce or stuffing/filling. These products must be refrigerated to extend their consumable life. Excludes products such as Fish with additional vegetables, dough or grains, Frozen and Shelf Stable Prepared and Processed Fish, all Unprepared and Unprocessed Fish.</obo:IAO_0000115>
	<obo:IAO_0000114 rdf:resource="&obo;IAO_0000428"/>
	<rdfs:comment xml:lang="en">LanguaL curation note: Index type of fish (anchovy, tuna) in facet B and part of fish (half, tail, egg) in facet C. Index Manufacturers Treatment/Cooking Process in facets H (dried, salted) and F (cooked). Index coating and stuffing in facet H. Index packing medium in facet K. Index preservation method (refrigeration) in facet J.</rdfs:comment>
	<oboInOwl:hasDbXref>LANGUAL:A1142</oboInOwl:hasDbXref>
</owl:Class>

<owl:Class rdf:about="&obo;FOODON_03401143">
	<rdfs:label xml:lang="en">10000018 - fish - prepared/processed (shelf stable) (gs1 gpc)</rdfs:label>
	<rdfs:subClassOf rdf:resource="&obo;FOODON_03401140"/>
	<obo:IAO_0000412>http://langual.org</obo:IAO_0000412>
	<obo:IAO_0000115 xml:lang="en">Includes any products that can be described/observed as any variety of fish or a combination of fish, that has gone through further manufacturing processes, such as reformed, cooked, dried and salted, however these products can also be coated, in sauce, stuffed or filled. Specifically excludes products that have added ingredients included such as rice, couscous and pasta. However products may contain a small quantity of vegetables such as those in a sauce or stuffing/filling. These products have been treated or packaged in such a way as to extend their consumable life. Excludes products such as Fish with additional vegetables, dough or grains, Frozen and Perishable Prepared and Processed Fish, all Unprepared and Unprocessed Fish.</obo:IAO_0000115>
	<obo:IAO_0000114 rdf:resource="&obo;IAO_0000428"/>
	<rdfs:comment xml:lang="en">LanguaL curation note: Index type of fish (anchovy, tuna) in facet B and part of fish (with or without bone) in facet C. Index Manufacturers Treatment/Cooking Process in facets H (dried, salted) and F (cooked). Index coating and stuffing in facet H. Index packing medium in facet K. Index organic claim in facet P.</rdfs:comment>
	<oboInOwl:hasDbXref>LANGUAL:A1143</oboInOwl:hasDbXref>
</owl:Class>

<owl:Class rdf:about="&obo;FOODON_03401144">
	<rdfs:label xml:lang="en">50121500 - fish - unprepared/unprocessed (gs1 gpc)</rdfs:label>
	<rdfs:subClassOf rdf:resource="&obo;FOODON_03401124"/>
	<obo:IAO_0000412>http://langual.org</obo:IAO_0000412>
	<obo:IAO_0000114 rdf:resource="&obo;IAO_0000428"/>
	<oboInOwl:hasDbXref>LANGUAL:A1144</oboInOwl:hasDbXref>
</owl:Class>

<owl:Class rdf:about="&obo;FOODON_03401145">
	<rdfs:label xml:lang="en">10000281 - fish - unprepared/unprocessed (frozen) (gs1 gpc)</rdfs:label>
	<rdfs:subClassOf rdf:resource="&obo;FOODON_03401144"/>
	<obo:IAO_0000412>http://langual.org</obo:IAO_0000412>
	<obo:IAO_0000115 xml:lang="en">Includes any products that can be described/observed as any variety of fish, or a combination of fish, which has not gone through any further manufacturing processes, such as reformed, cooked, dried and salted, however these products can be coated, in sauce, stuffed or filled. Specifically excludes products that have added ingredients included such as rice, couscous and pasta. However products may contain a small quantity of vegetables such as those in a sauce or stuffing/filling. These products must be frozen to extend their consumable life. Excludes products such as Fish with additional vegetables, dough or grains, Shelf Stable and Perishable Unprepared and Unprocessed Fish, all Prepared and Processed Fish.</obo:IAO_0000115>
	<obo:IAO_0000114 rdf:resource="&obo;IAO_0000428"/>
	<rdfs:comment xml:lang="en">LanguaL curation note: Index type of fish (anchovy, tuna) in facet B and part of fish (with or without bone) in facet C. Index organic claim in facet P.</rdfs:comment>
	<oboInOwl:hasDbXref>LANGUAL:A1145</oboInOwl:hasDbXref>
</owl:Class>

<owl:Class rdf:about="&obo;FOODON_03401146">
	<rdfs:label xml:lang="en">10000282 - fish - unprepared/unprocessed (perishable) (gs1 gpc)</rdfs:label>
	<rdfs:subClassOf rdf:resource="&obo;FOODON_03401144"/>
	<obo:IAO_0000412>http://langual.org</obo:IAO_0000412>
	<obo:IAO_0000115 xml:lang="en">Includes any products that can be described/observed as any variety of fish or a combination of fish, which has not gone through any further manufacturing processes, such as reformed, cooked, dried and salted, however these products can be coated, in sauce, stuffed or filled. Specifically excludes products that have added ingredients included such as rice, couscous and pasta. However products may contain a small quantity of vegetables such as those in a sauce or stuffing/filling. These products must be refrigerated to extend their consumable life. Excludes products such as Fish with additional vegetables, dough or grains, Shelf Stable and Frozen Unprepared and Unprocessed Fish, all Prepared and Processed Fish.</obo:IAO_0000115>
	<obo:IAO_0000114 rdf:resource="&obo;IAO_0000428"/>
	<rdfs:comment xml:lang="en">LanguaL curation note: Index type of fish (anchovy, tuna) in facet B and part of fish (with or without bone) in facet C. Index organic claim in facet P. Index preservation method (refrigeration) in facet J.</rdfs:comment>
	<oboInOwl:hasDbXref>LANGUAL:A1146</oboInOwl:hasDbXref>
</owl:Class>

<owl:Class rdf:about="&obo;FOODON_03401147">
	<rdfs:label xml:lang="en">10000283 - fish - unprepared/unprocessed (shelf stable) (gs1 gpc)</rdfs:label>
	<rdfs:subClassOf rdf:resource="&obo;FOODON_03401144"/>
	<obo:IAO_0000412>http://langual.org</obo:IAO_0000412>
	<obo:IAO_0000115 xml:lang="en">Includes any products that can be described/observed as any variety of fish or a combination of fish, which has not gone through any further manufacturing processes, such as reformed, cooked, dried and salted, however these products can be coated, in sauce, stuffed or filled. Specifically excludes products that have added ingredients included such as rice, couscous and pasta. However products may contain a small quantity of vegetables such as those in a sauce or stuffing/filling. These products have been treated or packaged in such a way as to extend their consumable life. Excludes products such as Fish with additional vegetables, dough or grains, Frozen and Perishable Unprepared and Unprocessed Fish, all Prepared and Processed Fish.</obo:IAO_0000115>
	<obo:IAO_0000114 rdf:resource="&obo;IAO_0000428"/>
	<rdfs:comment xml:lang="en">LanguaL curation note: Index type of fish (anchovy, tuna) in facet B and part of fish (with or without bone) in facet C. Index organic claim in facet P.</rdfs:comment>
	<oboInOwl:hasDbXref>LANGUAL:A1147</oboInOwl:hasDbXref>
</owl:Class>

<owl:Class rdf:about="&obo;FOODON_03401148">
	<rdfs:label xml:lang="en">50122100 - shellfish prepared/processed (gs1 gpc)</rdfs:label>
	<rdfs:subClassOf rdf:resource="&obo;FOODON_03401124"/>
	<obo:IAO_0000412>http://langual.org</obo:IAO_0000412>
	<obo:IAO_0000114 rdf:resource="&obo;IAO_0000428"/>
	<oboInOwl:hasDbXref>LANGUAL:A1148</oboInOwl:hasDbXref>
</owl:Class>

<owl:Class rdf:about="&obo;FOODON_03401149">
	<rdfs:label xml:lang="en">10000256 - shellfish prepared/processed (frozen) (gs1 gpc)</rdfs:label>
	<rdfs:subClassOf rdf:resource="&obo;FOODON_03401148"/>
	<obo:IAO_0000412>http://langual.org</obo:IAO_0000412>
	<obo:IAO_0000115 xml:lang="en">Includes any products that can be described/observed as an aquatic animal whose external covering consists of a shell, as in oysters, clams, lobsters and crabs, that has gone through further manufacturing processes, such as reformed, cooked, dried and salted, however these products can also be coated, in sauce, stuffed or filled. Products include sea snails and molluscs but specifically exclude products that have added ingredients included such as rice, couscous and pasta. However products may contain a small quantity of vegetables such as those in a sauce or stuffing/filling. These products must be frozen to extend their consumable life. Excludes products such as Shellfish with additional vegetables, dough or grains, Shelf Stable and Perishable Prepared and Processed Shellfish, all Unprepared and Unprocessed Shellfish.</obo:IAO_0000115>
	<obo:IAO_0000114 rdf:resource="&obo;IAO_0000428"/>
	<rdfs:comment xml:lang="en">LanguaL curation note: Index type of shellfish (abalone, winkle) in facet B and fish part (shelled, whole, piece) in facet C. Index Manufacturers Treatment/Cooking Process in facets H (smoked, salted) and F (cooked). Index organic claim in facet P.</rdfs:comment>
	<oboInOwl:hasDbXref>LANGUAL:A1149</oboInOwl:hasDbXref>
</owl:Class>

<owl:Class rdf:about="&obo;FOODON_03401150">
	<rdfs:label xml:lang="en">10000257 - shellfish prepared/processed (perishable) (gs1 gpc)</rdfs:label>
	<rdfs:subClassOf rdf:resource="&obo;FOODON_03401148"/>
	<obo:IAO_0000412>http://langual.org</obo:IAO_0000412>
	<obo:IAO_0000115 xml:lang="en">Includes any products that can be described/observed as an aquatic animal whose external covering consists of a shell, as in oysters, clams, lobsters and crabs, that has gone through further manufacturing processes, such as reformed, cooked, dried and salted, however these products can also be coated, in sauce, stuffed or filled. Products include sea snails and molluscs but specifically exclude products that have added ingredients included such as rice, couscous and pasta. However products may contain a small quantity of vegetables such as those in a sauce or stuffing/filling. These products must be refrigerated to extend their consumable life. Excludes products such as Shellfish with additional vegetables, dough or grains, Frozen and Shelf Stable Prepared and Processed Shellfish, all Unprepared and Unprocessed Shellfish.</obo:IAO_0000115>
	<obo:IAO_0000114 rdf:resource="&obo;IAO_0000428"/>
	<rdfs:comment xml:lang="en">LanguaL curation note: Index type of shellfish (abalone, winkle) in facet B and fish part (shelled, whole, piece) in facet C. Index Manufacturers Treatment/Cooking Process in facets H (smoked, salted) and F (cooked). Index organic claim in facet P. Index preservation method (refrigeration) in facet J.</rdfs:comment>
	<oboInOwl:hasDbXref>LANGUAL:A1150</oboInOwl:hasDbXref>
</owl:Class>

<owl:Class rdf:about="&obo;FOODON_03401151">
	<rdfs:label xml:lang="en">10000258 - shellfish prepared/processed (shelf stable) (gs1 gpc)</rdfs:label>
	<rdfs:subClassOf rdf:resource="&obo;FOODON_03401148"/>
	<obo:IAO_0000412>http://langual.org</obo:IAO_0000412>
	<obo:IAO_0000115 xml:lang="en">Includes any products that can be described/observed as any aquatic animal whose external covering consists of a shell, as in oysters, clams, lobsters and crabs, that has gone through further manufacturing processes, such as reformed, cooked, dried and salted, however these products can also be coated, in sauce, stuffed or filled. Products include sea snails and molluscs but specifically exclude products that have added ingredients included such as rice, couscous and pasta. However products may contain a small quantity of vegetables such as those in a sauce or stuffing/filling. These products have been treated or packaged in such a way as to extend their consumable life. Excludes products such as Shellfish with additional vegetables, dough or grains, Frozen and Perishable Prepared and Processed Shellfish, all Unprepared and Unprocessed Shellfish.</obo:IAO_0000115>
	<obo:IAO_0000114 rdf:resource="&obo;IAO_0000428"/>
	<rdfs:comment xml:lang="en">LanguaL curation note: Index type of shellfish (abalone, winkle) in facet B and fish part (shelled, whole, piece) in facet C. Index Manufacturers Treatment/Cooking Process in facets H (smoked, salted) and F (cooked). Index organic claim in facet P.</rdfs:comment>
	<oboInOwl:hasDbXref>LANGUAL:A1151</oboInOwl:hasDbXref>
</owl:Class>

<owl:Class rdf:about="&obo;FOODON_03401152">
	<rdfs:label xml:lang="en">50121700 - shellfish unprepared/unprocessed (gs1 gpc)</rdfs:label>
	<rdfs:subClassOf rdf:resource="&obo;FOODON_03401124"/>
	<obo:IAO_0000412>http://langual.org</obo:IAO_0000412>
	<obo:IAO_0000114 rdf:resource="&obo;IAO_0000428"/>
	<oboInOwl:hasDbXref>LANGUAL:A1152</oboInOwl:hasDbXref>
</owl:Class>

<owl:Class rdf:about="&obo;FOODON_03401153">
	<rdfs:label xml:lang="en">10000020 - shellfish - unprepared/unprocessed (frozen) (gs1 gpc)</rdfs:label>
	<rdfs:subClassOf rdf:resource="&obo;FOODON_03401152"/>
	<obo:IAO_0000412>http://langual.org</obo:IAO_0000412>
	<obo:IAO_0000115 xml:lang="en">Includes any products that can be described/observed as aquatic animal whose external covering consists of a shell, as in oysters, clams, lobsters and crabs, that has not gone through any further manufacturing processes, such as reformed, cooked, dried and salted, however these products can be coated, in sauce, stuffed or filled. Products include sea snails and molluscs but specifically exclude products that have added ingredients included such as rice, couscous and pasta. However products may contain a small quantity of vegetables such as those in a sauce or stuffing/filling. These products must be refrigerated to extend their consumable life. Excludes products such as Shellfish with additional vegetables, dough or grains, Shelf Stable and Frozen Unprepared and Unprocessed Shellfish, all Prepared and Processed Shellfish.</obo:IAO_0000115>
	<obo:IAO_0000114 rdf:resource="&obo;IAO_0000428"/>
	<rdfs:comment xml:lang="en">LanguaL curation note: Index type of shellfish (abalone, winkle) in facet B and fish part (shelled, whole, piece) in facet C. Index organic claim in facet P.</rdfs:comment>
	<oboInOwl:hasDbXref>LANGUAL:A1153</oboInOwl:hasDbXref>
</owl:Class>

<owl:Class rdf:about="&obo;FOODON_03401154">
	<rdfs:label xml:lang="en">10000019 - shellfish - unprepared/unprocessed (perishable) (gs1 gpc)</rdfs:label>
	<rdfs:subClassOf rdf:resource="&obo;FOODON_03401152"/>
	<obo:IAO_0000412>http://langual.org</obo:IAO_0000412>
	<obo:IAO_0000115 xml:lang="en">Includes any products that can be described/observed as an aquatic animal whose external covering consists of a shell, as in oysters, clams, lobsters and crabs, that has not gone through any further manufacturing processes, such as reformed, cooked, dried and salted, however these products can be coated, in sauce, stuffed or filled. Products include sea snails and molluscs but specifically exclude products that have added ingredients included such as rice, couscous and pasta. However products may contain a small quantity of vegetables such as those in a sauce or stuffing/filling. These products must be frozen to extend their consumable life. Excludes products such as Shellfish with additional vegetables, dough or grains, Shelf Stable and Perishable Unprepared and Unprocessed Shellfish, all Prepared and Processed Shellfish.</obo:IAO_0000115>
	<obo:IAO_0000114 rdf:resource="&obo;IAO_0000428"/>
	<rdfs:comment xml:lang="en">LanguaL curation note: Index type of shellfish (abalone, winkle) in facet B and fish part (shelled, whole, piece) in facet C. Index organic claim in facet P. Index preservation method (refrigeration) in facet J.</rdfs:comment>
	<oboInOwl:hasDbXref>LANGUAL:A1154</oboInOwl:hasDbXref>
</owl:Class>

<owl:Class rdf:about="&obo;FOODON_03401155">
	<rdfs:label xml:lang="en">10000021 - shellfish - unprepared/unprocessed (shelf stable) (gs1 gpc)</rdfs:label>
	<rdfs:subClassOf rdf:resource="&obo;FOODON_03401152"/>
	<obo:IAO_0000412>http://langual.org</obo:IAO_0000412>
	<obo:IAO_0000115 xml:lang="en">Includes any products that can be described/observed as an aquatic animal whose external covering consists of a shell, as in oysters, clams, lobsters and crabs, that has not gone through any further manufacturing processes, such as reformed, cooked, dried and salted, however these products can be coated, in sauce, stuffed or filled. Products include sea snails and molluscs but specifically exclude products that have added ingredients included such as rice, couscous and pasta. However products may contain a small quantity of vegetables such as those in a sauce or stuffing/filling. These products have been treated or packaged in such a way as to extend their consumable life. Excludes products such as Shellfish with additional vegetables, dough or grains, Frozen and Perishable Unprepared and Unprocessed Shellfish, all Prepared and Processed Shellfish.</obo:IAO_0000115>
	<obo:IAO_0000114 rdf:resource="&obo;IAO_0000428"/>
	<rdfs:comment xml:lang="en">LanguaL curation note: Index type of shellfish (abalone, winkle) in facet B and fish part (shelled, whole, piece) in facet C. Index organic claim in facet P.</rdfs:comment>
	<oboInOwl:hasDbXref>LANGUAL:A1155</oboInOwl:hasDbXref>
</owl:Class>

<owl:Class rdf:about="&obo;FOODON_03401156">
	<rdfs:label xml:lang="en">50122200 - aquatic plants prepared/processed (gs1 gpc)</rdfs:label>
	<rdfs:subClassOf rdf:resource="&obo;FOODON_03401124"/>
	<obo:IAO_0000412>http://langual.org</obo:IAO_0000412>
	<obo:IAO_0000114 rdf:resource="&obo;IAO_0000428"/>
	<oboInOwl:hasDbXref>LANGUAL:A1156</oboInOwl:hasDbXref>
</owl:Class>

<owl:Class rdf:about="&obo;FOODON_03401157">
	<rdfs:label xml:lang="en">10000151 - aquatic plants prepared/processed (frozen) (gs1 gpc)</rdfs:label>
	<rdfs:subClassOf rdf:resource="&obo;FOODON_03401156"/>
	<obo:IAO_0000412>http://langual.org</obo:IAO_0000412>
	<obo:IAO_0000115 xml:lang="en">Includes any products that can be described/observed as an edible plant that grows in or on the water, that has gone through further manufacturing processes, such as reformed, cooked, dried and salted, however these products can also be coated, in sauce, stuffed or filled. Specifically excludes products that have added ingredients included such as vegetables, rice, couscous and pasta. These products must be frozen to extend their consumable life. Excludes products such as Aquatic Plants with additional vegetables, dough or grains, Shelf Stable and Perishable Prepared and Processed Aquatic Plants, all Unprepared and Unprocessed Aquatic Plants.</obo:IAO_0000115>
	<obo:IAO_0000114 rdf:resource="&obo;IAO_0000428"/>
	<rdfs:comment xml:lang="en">LanguaL curation note: Index type of aquatic plant (agar, watercress) in facet B. If an industry recognized organic certification is claimed, index ORGANIC FOOD CLAIM OR USE in facet P. Index physical form (chopped, whole) in facet E. Index Manufacturers Treatment/Cooking Process in facets H (dried, salted) and F (cooked).</rdfs:comment>
	<oboInOwl:hasDbXref>LANGUAL:A1157</oboInOwl:hasDbXref>
</owl:Class>

<owl:Class rdf:about="&obo;FOODON_03401158">
	<rdfs:label xml:lang="en">10000152 - aquatic plants prepared/processed (perishable) (gs1 gpc)</rdfs:label>
	<rdfs:subClassOf rdf:resource="&obo;FOODON_03401156"/>
	<obo:IAO_0000412>http://langual.org</obo:IAO_0000412>
	<obo:IAO_0000115 xml:lang="en">Includes any products that can be described/observed as an edible plant that grows in or on the water, that has gone through further manufacturing processes, such as reformed, cooked, dried and salted, however these products can also be coated, in sauce, stuffed or filled. Specifically excludes products that have added ingredients included such as vegetables, rice, couscous and pasta. These products must be refrigerated to extend their consumable life. Excludes products such as Aquatic Plants with additional vegetables, dough or grains, Shelf Stable and Frozen Prepared and Processed Aquatic Plants, all Unprepared and Unprocessed Aquatic Plants.</obo:IAO_0000115>
	<obo:IAO_0000114 rdf:resource="&obo;IAO_0000428"/>
	<rdfs:comment xml:lang="en">LanguaL curation note: Index type of aquatic plant (agar, watercress) in facet B. If an industry recognized organic certification is claimed, index ORGANIC FOOD CLAIM OR USE in facet P. Index physical form (chopped, whole) in facet E. Index Manufacturers Treatment/Cooking Process in facets H (dried, salted) and F (cooked). Index preservation method (refrigeration) in facet J.</rdfs:comment>
	<oboInOwl:hasDbXref>LANGUAL:A1158</oboInOwl:hasDbXref>
</owl:Class>

<owl:Class rdf:about="&obo;FOODON_03401159">
	<rdfs:label xml:lang="en">10000153 - aquatic plants prepared/processed (shelf stable) (gs1 gpc)</rdfs:label>
	<rdfs:subClassOf rdf:resource="&obo;FOODON_03401156"/>
	<obo:IAO_0000412>http://langual.org</obo:IAO_0000412>
	<obo:IAO_0000115 xml:lang="en">Includes any products that can be described/observed as an edible plant that grows in or on the water, that has gone through further manufacturing processes, such as reformed, cooked, dried and salted, however these products can also be coated, in sauce, stuffed or filled. Specifically excludes products that have added ingredients included such as vegetables, rice, couscous and pasta. These products have been treated or packaged in such a way as to extend their consumable life. Excludes products such as Aquatic Plants with additional vegetables, dough or grains, Frozen and Perishable Prepared and Processed Aquatic Plants, all Unprepared and Unprocessed Aquatic Plants.</obo:IAO_0000115>
	<obo:IAO_0000114 rdf:resource="&obo;IAO_0000428"/>
	<rdfs:comment xml:lang="en">LanguaL curation note: Index type of aquatic plant (agar, watercress) in facet B. If an industry recognized organic certification is claimed, index ORGANIC FOOD CLAIM OR USE in facet P. Index physical form (chopped, whole) in facet E. Index Manufacturers Treatment/Cooking Process in facets H (dried, salted) and F (cooked).</rdfs:comment>
	<oboInOwl:hasDbXref>LANGUAL:A1159</oboInOwl:hasDbXref>
</owl:Class>

<owl:Class rdf:about="&obo;FOODON_03401160">
	<rdfs:label xml:lang="en">50121800 - aquatic plants unprepared/unprocessed (gs1 gpc)</rdfs:label>
	<rdfs:subClassOf rdf:resource="&obo;FOODON_03401124"/>
	<obo:IAO_0000412>http://langual.org</obo:IAO_0000412>
	<obo:IAO_0000114 rdf:resource="&obo;IAO_0000428"/>
	<oboInOwl:hasDbXref>LANGUAL:A1160</oboInOwl:hasDbXref>
</owl:Class>

<owl:Class rdf:about="&obo;FOODON_03401161">
	<rdfs:label xml:lang="en">10000138 - aquatic plants unprepared/unprocessed (frozen) (gs1 gpc)</rdfs:label>
	<rdfs:subClassOf rdf:resource="&obo;FOODON_03401160"/>
	<obo:IAO_0000412>http://langual.org</obo:IAO_0000412>
	<obo:IAO_0000115 xml:lang="en">Includes any products that can be described/observed as an edible plant that grows in or on the water, that has not gone through any further manufacturing processes, such as reformed, cooked, dried and salted, however these products can be coated, in sauce, stuffed or filled. Specifically excludes products that have added ingredients included such as vegetables, rice, couscous and pasta. These products must be frozen to extend their consumable life. Excludes products such as Aquatic Plants with additional vegetables, dough or grains, Shelf Stable and Perishable Unprepared and Unprocessed Aquatic Plants, all Prepared and Processed Aquatic Plants</obo:IAO_0000115>
	<obo:IAO_0000114 rdf:resource="&obo;IAO_0000428"/>
	<rdfs:comment xml:lang="en">LanguaL curation note: Index type of aquatic plant (agar, watercress) in facet B. If an industry recognized organic certification is claimed, index ORGANIC FOOD CLAIM OR USE in facet P. Index physical form (chopped, whole) in facet E.</rdfs:comment>
	<oboInOwl:hasDbXref>LANGUAL:A1161</oboInOwl:hasDbXref>
</owl:Class>

<owl:Class rdf:about="&obo;FOODON_03401162">
	<rdfs:label xml:lang="en">10000137 - aquatic plants unprepared/unprocessed (perishable) (gs1 gpc)</rdfs:label>
	<rdfs:subClassOf rdf:resource="&obo;FOODON_03401160"/>
	<obo:IAO_0000412>http://langual.org</obo:IAO_0000412>
	<obo:IAO_0000115 xml:lang="en">Includes any products that can be described/observed as any fresh edible plant that grows in or on the water, that has not gone through any further manufacturing processes, such as reformed, cooked, dried and salted, however these products can be coated, in sauce, stuffed or filled. Specifically excludes products that have added ingredients included such as vegetables, rice, couscous and pasta. These products have to be refrigerated to extend their consumable life. Excludes products such as Aquatic Plants with additional vegetables, dough or grains, Shelf Stable and Frozen Unprepared and Unprocessed Aquatic Plants, all Prepared and Processed Aquatic Plants.</obo:IAO_0000115>
	<obo:IAO_0000114 rdf:resource="&obo;IAO_0000428"/>
	<rdfs:comment xml:lang="en">LanguaL curation note: Index type of aquatic plant (agar, watercress) in facet B. If an industry recognized organic certification is claimed, index ORGANIC FOOD CLAIM OR USE in facet P. Index physical form (chopped, whole) in facet E. Index preservation method (refrigeration) in facet J.</rdfs:comment>
	<oboInOwl:hasDbXref>LANGUAL:A1162</oboInOwl:hasDbXref>
</owl:Class>

<owl:Class rdf:about="&obo;FOODON_03401163">
	<rdfs:label xml:lang="en">10000139 - aquatic plants unprepared/unprocessed (shelf stable) (gs1 gpc)</rdfs:label>
	<rdfs:subClassOf rdf:resource="&obo;FOODON_03401160"/>
	<obo:IAO_0000412>http://langual.org</obo:IAO_0000412>
	<obo:IAO_0000115 xml:lang="en">Includes any products that can be described/observed as any edible plant that grows in or on the water, that has not gone through any further manufacturing processes, such as reformed, cooked, dried and salted, however these products can be coated, in sauce, stuffed or filled. Specifically excludes products that have added ingredients included such as vegetables, rice, couscous and pasta. These products have been treated or packaged in such a way as to extend their consumable life. Excludes products such as Aquatic Plants with additional vegetables, dough or grains, Frozen and Perishable Unprepared and Unprocessed Aquatic Plants, all Prepared and Processed Aquatic Plants.</obo:IAO_0000115>
	<obo:IAO_0000114 rdf:resource="&obo;IAO_0000428"/>
	<rdfs:comment xml:lang="en">LanguaL curation note: Index type of aquatic plant (agar, watercress) in facet B. If an industry recognized organic certification is claimed, index ORGANIC FOOD CLAIM OR USE in facet P. Index physical form (chopped, whole) in facet E.</rdfs:comment>
	<oboInOwl:hasDbXref>LANGUAL:A1163</oboInOwl:hasDbXref>
</owl:Class>

<owl:Class rdf:about="&obo;FOODON_03401164">
	<rdfs:label xml:lang="en">50122400 - seafood variety packs (gs1 gpc)</rdfs:label>
	<rdfs:subClassOf rdf:resource="&obo;FOODON_03401124"/>
	<obo:IAO_0000412>http://langual.org</obo:IAO_0000412>
	<obo:IAO_0000115 xml:lang="en">Includes any products that can be described/observed as two or more distinct Seafood Products sold together which exist within the schema but belong to different classes, that is two or more products contained within the same pack which cross classes within the Seafood Family. Includes products such as Shrimp and Cod variety packs and Crabsticks and Herring variety packs. Items that are received free with purchases should be removed from the classification decision-making process. Excludes products such as Fish and Tartar Sauce variety packs and cockles and mussels variety packs.</obo:IAO_0000115>
	<obo:IAO_0000114 rdf:resource="&obo;IAO_0000428"/>
	<oboInOwl:hasDbXref>LANGUAL:A1164</oboInOwl:hasDbXref>
</owl:Class>

<owl:Class rdf:about="&obo;FOODON_03401165">
	<rdfs:label xml:lang="en">50170000 - seasonings/preservatives/extracts (gs1 gpc)</rdfs:label>
	<rdfs:subClassOf rdf:resource="&obo;FOODON_03400874"/>
	<obo:IAO_0000412>http://langual.org</obo:IAO_0000412>
	<obo:IAO_0000114 rdf:resource="&obo;IAO_0000428"/>
	<oboInOwl:hasDbXref>LANGUAL:A1165</oboInOwl:hasDbXref>
</owl:Class>

<owl:Class rdf:about="&obo;FOODON_03401166">
	<rdfs:label xml:lang="en">50171500 - herbs/spices/extracts (gs1 gpc)</rdfs:label>
	<rdfs:subClassOf rdf:resource="&obo;FOODON_03401165"/>
	<obo:IAO_0000412>http://langual.org</obo:IAO_0000412>
	<obo:IAO_0000114 rdf:resource="&obo;IAO_0000428"/>
	<oboInOwl:hasDbXref>LANGUAL:A1166</oboInOwl:hasDbXref>
</owl:Class>

<owl:Class rdf:about="&obo;FOODON_03401167">
	<rdfs:label xml:lang="en">10000050 - extracts/salt/meat tenderisers (shelf stable) (gs1 gpc)</rdfs:label>
	<rdfs:subClassOf rdf:resource="&obo;FOODON_03401166"/>
	<obo:IAO_0000412>http://langual.org</obo:IAO_0000412>
	<obo:IAO_0000115 xml:lang="en">Includes any products that can be described/observed as a liquid, paste, powder, granules or solid made from evaporation or refinement of meat, vegetable, yeast or sodium chloride that is added to season and flavour food, and in specific cases to tenderise meat. Products specifically include refined and unrefined Salt and Monosodium Glutamate, Bouillon, as well as a powdered form of Meat Tenderiser. These products have been treated or packaged in such a way as to extend their consumable life. Excludes products such as single or pure Perishable or Shelf Stable Herbs and Spices, Gravy Browning, Soup Mixes.</obo:IAO_0000115>
	<obo:IAO_0000114 rdf:resource="&obo;IAO_0000428"/>
	<rdfs:comment xml:lang="en">LanguaL curation note: Index physical form (liquid, powder) in facet E. Index level of salt claim (low salt, no salt) and organic claim in facet P. Index the main ingredient (fish, salt) in facet B.</rdfs:comment>
	<oboInOwl:hasDbXref>LANGUAL:A1167</oboInOwl:hasDbXref>
</owl:Class>

<owl:Class rdf:about="&obo;FOODON_03401168">
	<rdfs:label xml:lang="en">10000212 - herbs/spices (frozen) (gs1 gpc)</rdfs:label>
	<rdfs:subClassOf rdf:resource="&obo;FOODON_03401166"/>
	<obo:IAO_0000412>http://langual.org</obo:IAO_0000412>
	<obo:IAO_0000115 xml:lang="en">Includes any products that can be described/observed as an aromatic or richly flavoured vegetable or plant or its derivative that is typically added to season or give additional flavour to foods. These products include aromatic seasonings which are obtained from the bark, buds, fruit, roots, seeds or stems of various plant and known as spices, and those, which are obtained from the leafy part of a plant and known as herbs. Products include unprocessed and processed frozen herbs and/or spices or a combination of frozen herbs and spices. These products must be frozen to extend their consumable life. Excludes products such as Perishable Herbs and Spices, Salt and Extracts.</obo:IAO_0000115>
	<obo:IAO_0000114 rdf:resource="&obo;IAO_0000428"/>
	<rdfs:comment xml:lang="en">LanguaL curation note: Index the herb/spice in facets B (basil, white pepper) and C (bark, leaf). If an industry recognized organic certification is claimed, index ORGANIC FOOD CLAIM OR USE in facet P. Index Manufacturers Treatment/Cooking Process in facets H (dried, salted) and F (cooked). Index physical form (chopped, powder) in facet E.</rdfs:comment>
	<oboInOwl:hasDbXref>LANGUAL:A1168</oboInOwl:hasDbXref>
</owl:Class>

<owl:Class rdf:about="&obo;FOODON_03401169">
	<rdfs:label xml:lang="en">10000048 - herbs/spices (perishable) (gs1 gpc)</rdfs:label>
	<rdfs:subClassOf rdf:resource="&obo;FOODON_03401166"/>
	<obo:IAO_0000412>http://langual.org</obo:IAO_0000412>
	<obo:IAO_0000115 xml:lang="en">Includes any products that can be described/observed as an aromatic or richly flavoured vegetable or plant or its derivative that is typically added to season or give additional flavour to foods. These products include aromatic seasonings which are obtained from the bark, buds, fruit, roots, seeds or stems of various plant and known as spices, and those, which are obtained from the leafy part of a plant and known as herbs. These products can be/must be refrigerated to extend their consumable life. Products include growing, potted plants, unprocessed herbs and spices in their natural state and a combination of herbs and spices. Excludes products such as Shelf Stable Herbs and Spices, Salt and Extracts.</obo:IAO_0000115>
	<obo:IAO_0000114 rdf:resource="&obo;IAO_0000428"/>
	<rdfs:comment xml:lang="en">LanguaL curation note: Index the herb/spice in facets B (basil, white pepper) and C (bark, leaf). If an industry recognized organic certification is claimed, index ORGANIC FOOD CLAIM OR USE in facet P. Index Manufacturers Treatment/Cooking Process in facets H (dried, salted) and F (cooked). Index physical form (chopped, powder) in facet E. Index preservation method (refrigeration) in facet J.</rdfs:comment>
	<oboInOwl:hasDbXref>LANGUAL:A1169</oboInOwl:hasDbXref>
</owl:Class>

<owl:Class rdf:about="&obo;FOODON_03401170">
	<rdfs:label xml:lang="en">10000049 - herbs/spices (shelf stable) (gs1 gpc)</rdfs:label>
	<rdfs:subClassOf rdf:resource="&obo;FOODON_03401166"/>
	<obo:IAO_0000412>http://langual.org</obo:IAO_0000412>
	<obo:IAO_0000115 xml:lang="en">Includes any products that can be described/observed as an aromatic or richly flavoured vegetable or plant or its derivative that is typically added to season or give additional flavour to foods. These products include aromatic seasonings which are obtained from the bark, buds, fruit, roots, seeds or stems of various plant and known as spices, and those, which are obtained from the leafy part of a plant and known as herbs. These products have been treated or packaged in such a way as to extend their consumable life. Products include unprocessed and processed herbs or spices or a combination of herbs and spices. Excludes products such as Perishable Herbs and Spices, Salt and Extracts.</obo:IAO_0000115>
	<obo:IAO_0000114 rdf:resource="&obo;IAO_0000428"/>
	<rdfs:comment xml:lang="en">LanguaL curation note: Index the herb/spice in facets B (basil, white pepper) and C (bark, leaf). If an industry recognized organic certification is claimed, index ORGANIC FOOD CLAIM OR USE in facet P. Index Manufacturers Treatment/Cooking Process in facets H (dried, salted) and F (cooked). Index physical form (chopped, powder) in facet E.</rdfs:comment>
	<oboInOwl:hasDbXref>LANGUAL:A1170</oboInOwl:hasDbXref>
</owl:Class>

<owl:Class rdf:about="&obo;FOODON_03401171">
	<rdfs:label xml:lang="en">10000580 - stock liquid/bones (frozen) (gs1 gpc)</rdfs:label>
	<rdfs:subClassOf rdf:resource="&obo;FOODON_03401166"/>
	<obo:IAO_0000412>http://langual.org</obo:IAO_0000412>
	<obo:IAO_0000115 xml:lang="en">Includes any products that can be described/observed as a frozen substance, which, upon defrosting, returns to its original consistency of a liquid extract resulting from boiling meat or fish and/or vegetables. The product can be presented as purely a liquid or a combination of liquid and bones. The liquid extract is added to season or give a defined flavour to a particular food or recipe. Excludes products such as Shelf Stable and Perishable Stock Liquid/Bones; Shelf Stable Extracts; Perishable or Shelf Stable Herbs and Spices; Gravy Browning; Soup Mixes.</obo:IAO_0000115>
	<obo:IAO_0000114 rdf:resource="&obo;IAO_0000428"/>
	<rdfs:comment xml:lang="en">LanguaL curation note: If an industry recognized organic certification is claimed, index ORGANIC FOOD CLAIM OR USE in facet P.Index the main ingredient (fish, salt) in facet B.</rdfs:comment>
	<oboInOwl:hasDbXref>LANGUAL:A1171</oboInOwl:hasDbXref>
</owl:Class>

<owl:Class rdf:about="&obo;FOODON_03401172">
	<rdfs:label xml:lang="en">10000579 - stock liquid/bones (perishable) (gs1 gpc)</rdfs:label>
	<rdfs:subClassOf rdf:resource="&obo;FOODON_03401166"/>
	<obo:IAO_0000412>http://langual.org</obo:IAO_0000412>
	<obo:IAO_0000115 xml:lang="en">Includes any products that can be described/observed as a liquid extract resulting from boiling meat or fish and/or vegetables. The product can be presented as purely a liquid or a combination of liquid and bones. The liquid extract is added to season or give a defined flavour to a particular food or recipe. These products must be refrigerated to extend their consumable life. Excludes products such as Shelf Stable and Frozen Stock Liquid/Bones; Shelf Stable Extracts; Perishable or Shelf Stable Herbs and Spices; Gravy Browning; Soup Mixes.</obo:IAO_0000115>
	<obo:IAO_0000114 rdf:resource="&obo;IAO_0000428"/>
	<rdfs:comment xml:lang="en">LanguaL curation note: If an industry recognized organic certification is claimed, index ORGANIC FOOD CLAIM OR USE in facet P.Index the main ingredient (fish, salt) in facet B. Index preservation method (refrigeration) in facet J.</rdfs:comment>
	<oboInOwl:hasDbXref>LANGUAL:A1172</oboInOwl:hasDbXref>
</owl:Class>

<owl:Class rdf:about="&obo;FOODON_03401173">
	<rdfs:label xml:lang="en">10000578 - stock liquid/bones (shelf stable) (gs1 gpc)</rdfs:label>
	<rdfs:subClassOf rdf:resource="&obo;FOODON_03401166"/>
	<obo:IAO_0000412>http://langual.org</obo:IAO_0000412>
	<obo:IAO_0000115 xml:lang="en">Includes any products that can be described/observed as a liquid extract resulting from boiling meat or fish and/or vegetables. The product can be presented as purely a liquid or a combination of liquid and bones. The liquid extract is added to season or give a defined flavour to a particular food or recipe. These products have been treated or packaged in such a way as to extend their consumable life. Excludes products such as Perishable and Frozen Stock Liquid/Bones; Shelf Stable Extracts; Perishable or Shelf Stable Herbs and Spices; Gravy Browning; Soup Mixes.</obo:IAO_0000115>
	<obo:IAO_0000114 rdf:resource="&obo;IAO_0000428"/>
	<rdfs:comment xml:lang="en">LanguaL curation note: If an industry recognized organic certification is claimed, index ORGANIC FOOD CLAIM OR USE in facet P.Index the main ingredient (fish, salt) in facet B.</rdfs:comment>
	<oboInOwl:hasDbXref>LANGUAL:A1173</oboInOwl:hasDbXref>
</owl:Class>

<owl:Class rdf:about="&obo;FOODON_03401174">
	<rdfs:label xml:lang="en">10000615 - herbs/spices/extracts variety packs (gs1 gpc)</rdfs:label>
	<rdfs:subClassOf rdf:resource="&obo;FOODON_03401166"/>
	<obo:IAO_0000412>http://langual.org</obo:IAO_0000412>
	<obo:IAO_0000115 xml:lang="en">Includes any products that can be described/observed as two or more distinct Herbs, Spices or Extracts sold together, which exist within the schema belonging to different bricks but to the same class, that is two or more products contained within the same pack which cross bricks within the Herbs, Spices and Extracts class. Includes products such as Salt and Pepper sold together. Items that are received free with purchases should be removed from the classification decision-making process. Excludes products such as Marinades and Spices variety packs.</obo:IAO_0000115>
	<obo:IAO_0000114 rdf:resource="&obo;IAO_0000428"/>
	<oboInOwl:hasDbXref>LANGUAL:A1174</oboInOwl:hasDbXref>
</owl:Class>

<owl:Class rdf:about="&obo;FOODON_03401175">
	<rdfs:label xml:lang="en">50171900 - pickles/relishes/chutneys/olives (gs1 gpc)</rdfs:label>
	<rdfs:subClassOf rdf:resource="&obo;FOODON_03401165"/>
	<obo:IAO_0000412>http://langual.org</obo:IAO_0000412>
	<obo:IAO_0000114 rdf:resource="&obo;IAO_0000428"/>
	<oboInOwl:hasDbXref>LANGUAL:A1175</oboInOwl:hasDbXref>
</owl:Class>

<owl:Class rdf:about="&obo;FOODON_03401176">
	<rdfs:label xml:lang="en">10000586 - chutneys/relishes (frozen) (gs1 gpc)</rdfs:label>
	<rdfs:subClassOf rdf:resource="&obo;FOODON_03401175"/>
	<obo:IAO_0000412>http://langual.org</obo:IAO_0000412>
	<obo:IAO_0000115 xml:lang="en">Includes any products that can be described as a spoonable substance, usually served as a spread or as an accompaniment to savoury foods, containing chopped or minced fruit of vegetables, with herbs, spices and seasonings. These products are usually sweet, but can also be savoury or spicy. These products must be frozen to extend their consumable life Includes products such as tomato chutney and mango chutney. Specifically excludes pickles and piccalilli. Excludes products such as Whole Pickled Vegetables, Canned Vegetables and Sandwich Spread., Shelf Stable and Perishable Chutneys and Relishes.</obo:IAO_0000115>
	<obo:IAO_0000114 rdf:resource="&obo;IAO_0000428"/>
	<rdfs:comment xml:lang="en">LanguaL curation note: Index physical form (sliced, pureed) in facet E. Index use claim (vegetarians/vegans), level of salt claim (low salt, no salt) and organic claim in facet P. Index the main ingredient (mango, tomato) in facet B.</rdfs:comment>
	<oboInOwl:hasDbXref>LANGUAL:A1176</oboInOwl:hasDbXref>
</owl:Class>

<owl:Class rdf:about="&obo;FOODON_03401177">
	<rdfs:label xml:lang="en">10000587 - chutneys/relishes (perishable) (gs1 gpc)</rdfs:label>
	<rdfs:subClassOf rdf:resource="&obo;FOODON_03401175"/>
	<obo:IAO_0000412>http://langual.org</obo:IAO_0000412>
	<obo:IAO_0000115 xml:lang="en">Includes any products that can be described as a spoonable substance, usually served as a spread or as an accompaniment to savoury foods, containing chopped or minced fruit of vegetables, with herbs, spices and seasonings. These products are usually sweet, but can also be savoury or spicy. These products must be refrigerated to extend their consumable life. Includes products such as tomato chutney and mango chutney. Specifically excludes pickles and piccalilli. Excludes products such as Whole Pickled Vegetables, Canned Vegetables and Sandwich Spread., Shelf Stable and Frozen Chutneys and Relishes.</obo:IAO_0000115>
	<obo:IAO_0000114 rdf:resource="&obo;IAO_0000428"/>
	<rdfs:comment xml:lang="en">LanguaL curation note: Index physical form (sliced, pureed) in facet E. Index use claim (vegetarians/vegans), level of salt claim (low salt, no salt) and organic claim in facet P. Index the main ingredient (mango, tomato) in facet B. Index preservation method (refrigeration) in facet J.</rdfs:comment>
	<oboInOwl:hasDbXref>LANGUAL:A1177</oboInOwl:hasDbXref>
</owl:Class>

<owl:Class rdf:about="&obo;FOODON_03401178">
	<rdfs:label xml:lang="en">10000180 - chutneys/relishes (shelf stable) (gs1 gpc)</rdfs:label>
	<rdfs:subClassOf rdf:resource="&obo;FOODON_03401175"/>
	<obo:IAO_0000412>http://langual.org</obo:IAO_0000412>
	<obo:IAO_0000115 xml:lang="en">Includes any products that can be described as a spoonable substance, usually served as a spread or as an accompaniment to savoury foods, containing chopped or minced fruit of vegetables, with herbs, spices and seasonings. These products are usually sweet, but can also be savoury or spicy. These products have been treated or packaged in such a way as to extend their consumable life. Includes products such as tomato chutney and mango chutney. Specifically excludes pickles and piccalilli. Excludes products such as Whole Pickled Vegetables, Canned Vegetables and Sandwich Spread., Frozen and Perishable Chutneys and Relishes</obo:IAO_0000115>
	<obo:IAO_0000114 rdf:resource="&obo;IAO_0000428"/>
	<rdfs:comment xml:lang="en">LanguaL curation note: Index physical form (sliced, pureed) in facet E. Index use claim (vegetarians/vegans), level of salt claim (low salt, no salt) and organic claim in facet P. Index the main ingredient (mango, tomato) in facet B.</rdfs:comment>
	<oboInOwl:hasDbXref>LANGUAL:A1178</oboInOwl:hasDbXref>
</owl:Class>

<owl:Class rdf:about="&obo;FOODON_03401179">
	<rdfs:label xml:lang="en">10000238 - olives (perishable) (gs1 gpc)</rdfs:label>
	<rdfs:subClassOf rdf:resource="&obo;FOODON_03401175"/>
	<obo:IAO_0000412>http://langual.org</obo:IAO_0000412>
	<obo:IAO_0000115 xml:lang="en">Includes any products that can be described/observed as any variety of olive from the olive tree, such as Sevillana, Manzanilla and Ascolane, that have no added ingredients or flavourings and can be in various forms, whole, diced, sliced or cut. These products can be/must be refrigerated to extend their consumable life. Excludes products such as Pickles and Shelf Stable Olives.</obo:IAO_0000115>
	<obo:IAO_0000114 rdf:resource="&obo;IAO_0000428"/>
	<rdfs:comment xml:lang="en">LanguaL curation note: Index type of olive (black, green) in facet B and whether pittet/stoned in facet C. Index level of salt claim (low salt, no salt) and organic claim in facet P. Index preservation method (refrigeration) in facet J.</rdfs:comment>
	<oboInOwl:hasDbXref>LANGUAL:A1179</oboInOwl:hasDbXref>
</owl:Class>

<owl:Class rdf:about="&obo;FOODON_03401180">
	<rdfs:label xml:lang="en">10000239 - olives (shelf stable) (gs1 gpc)</rdfs:label>
	<rdfs:subClassOf rdf:resource="&obo;FOODON_03401175"/>
	<obo:IAO_0000412>http://langual.org</obo:IAO_0000412>
	<obo:IAO_0000115 xml:lang="en">Includes any products that can be described/observed as any variety of olive from the olive tree, such as Sevillana, Manzanilla and Ascolane, that may have been prepared by removing the stone. These products can be in a sauce - tomato, curry, BBQ or Cream and have added ingredients or flavourings that may fill (pimento, anchovies) or cover (herbs, sauces) the olive. These products have been treated or packaged in such a way as to extend their consumable life. Excludes products such as Pickles and Perishable Olives.</obo:IAO_0000115>
	<obo:IAO_0000114 rdf:resource="&obo;IAO_0000428"/>
	<rdfs:comment xml:lang="en">LanguaL curation note: Index type of olive (black, green) in facet B and whether pittet/stoned in facet C. Index level of salt claim (low salt, no salt) and organic claim in facet P. Index packing medium (brine, oil) in facet K.</rdfs:comment>
	<oboInOwl:hasDbXref>LANGUAL:A1180</oboInOwl:hasDbXref>
</owl:Class>

<owl:Class rdf:about="&obo;FOODON_03401181">
	<rdfs:label xml:lang="en">10000244 - pickles (gs1 gpc)</rdfs:label>
	<rdfs:subClassOf rdf:resource="&obo;FOODON_03401175"/>
	<obo:IAO_0000412>http://langual.org</obo:IAO_0000412>
	<obo:IAO_0000115 xml:lang="en">Includes any products that can be described/observed as chopped or whole vegetables, preserved in vinegar, oil or brine, with added ingredients such as herbs, spices and mustard, commonly used as a condiment for meats, cheese and bread. Products include pickled tomatoes, gherkins, onions and capers. These products have been treated or packaged in such a way as to extend their consumable life. Excludes products such as Canned Vegetables and Vegetable Spreads, Chutneys, Relishes and Olives and Pickled Eggs.</obo:IAO_0000115>
	<obo:IAO_0000114 rdf:resource="&obo;IAO_0000428"/>
	<rdfs:comment xml:lang="en">LanguaL curation note: Index type of piclke (cucumber, pepper) in facet B. Index physical form (chopped, whole) in facet E. Index use claim (vegetarians/vegans), level of salt claim (low salt, no salt) and organic claim in facet P. Index packing medium (brine, oil) in facet K.</rdfs:comment>
	<oboInOwl:hasDbXref>LANGUAL:A1181</oboInOwl:hasDbXref>
</owl:Class>

<owl:Class rdf:about="&obo;FOODON_03401182">
	<rdfs:label xml:lang="en">10000616 - pickles/relishes/chutneys/olives variety packs (gs1 gpc)</rdfs:label>
	<rdfs:subClassOf rdf:resource="&obo;FOODON_03401175"/>
	<obo:IAO_0000412>http://langual.org</obo:IAO_0000412>
	<obo:IAO_0000115 xml:lang="en">Includes any products that can be described/observed as two or more distinct Pickles, Relish, Chutney or Olives sold together, which exist within the schema belonging to different bricks but to the same class, that is two or more products contained within the same pack which cross bricks within the Pickles, Relishes, Chutneys and Olives class. Includes products such as Pickles and Relishes sold together. Items that are received free with purchases should be removed from the classification decision-making process. Excludes products such as Mango Chutney and Poppadom variety packs.</obo:IAO_0000115>
	<obo:IAO_0000114 rdf:resource="&obo;IAO_0000428"/>
	<oboInOwl:hasDbXref>LANGUAL:A1182</oboInOwl:hasDbXref>
</owl:Class>

<owl:Class rdf:about="&obo;FOODON_03401183">
	<rdfs:label xml:lang="en">50171800 - sauces/spreads/dips/condiments (gs1 gpc)</rdfs:label>
	<rdfs:subClassOf rdf:resource="&obo;FOODON_03401165"/>
	<obo:IAO_0000412>http://langual.org</obo:IAO_0000412>
	<obo:IAO_0000114 rdf:resource="&obo;IAO_0000428"/>
	<oboInOwl:hasDbXref>LANGUAL:A1183</oboInOwl:hasDbXref>
</owl:Class>

<owl:Class rdf:about="&obo;FOODON_03401184">
	<rdfs:label xml:lang="en">10000583 - dressing/dips (frozen) (gs1 gpc)</rdfs:label>
	<rdfs:subClassOf rdf:resource="&obo;FOODON_03401183"/>
	<obo:IAO_0000412>http://langual.org</obo:IAO_0000412>
	<obo:IAO_0000115 xml:lang="en">Includes any products that can be described/observed as a frozen substance, which, upon defrosting, returns to its original soft consistency and can be served as an accompaniment to snacks or starters, such as crisps, tortilla chips, raw vegetables and pappadums, or poured cold over salads and vegetables. Products include dairy or mayonnaise based dressings, garlic and herb dip, cheese dip and taramasalata. Excludes products such as Shelf Stable and Perishable Dressings and Dips, and Sauces, Condiments, Savoury Toppings, Savoury Spreads and Marinades.</obo:IAO_0000115>
	<obo:IAO_0000114 rdf:resource="&obo;IAO_0000428"/>
	<rdfs:comment xml:lang="en">LanguaL curation note: Index main ingredient in facet B and added ingredients in facet H. Index manufacturer's treatments (homogenized) in facet H. Index physical form (liquid, puree) in facet E. Index use claims (vegetarian/vegan), fat level claim (low fat, reduced fat) and organic claim in facet P.</rdfs:comment>
	<oboInOwl:hasDbXref>LANGUAL:A1184</oboInOwl:hasDbXref>
</owl:Class>

<owl:Class rdf:about="&obo;FOODON_03401185">
	<rdfs:label xml:lang="en">10000199 - dressings/dips (perishable) (gs1 gpc)</rdfs:label>
	<rdfs:subClassOf rdf:resource="&obo;FOODON_03401183"/>
	<obo:IAO_0000412>http://langual.org</obo:IAO_0000412>
	<obo:IAO_0000115 xml:lang="en">Includes any products that can be described/observed as a pourable or spoonable substance, usually served as an accompaniment to snacks or starters, such as crisps, tortilla chips, raw vegetables and pappadums, or poured cold over salads or vegetables. Products include dairy or mayonnaise based dressings, garlic and herb dip, cheese dip and taramasalata. These products must be refrigerated to extend their consumable life. Excludes products such as Frozen and Shelf Stable Dressings and Dips, and Sauces, Condiments, Savoury Toppings, Savoury Spreads and Marinades.</obo:IAO_0000115>
	<obo:IAO_0000114 rdf:resource="&obo;IAO_0000428"/>
	<rdfs:comment xml:lang="en">LanguaL curation note: Index main ingredient in facet B and added ingredients in facet H. Index manufacturer's treatments (homogenized) in facet H. Index physical form (liquid, puree) in facet E. Index use claims (vegetarian/vegan), fat level claim (low fat, reduced fat) and organic claim in facet P. Index preservation method (refrigeration) in facet J.</rdfs:comment>
	<oboInOwl:hasDbXref>LANGUAL:A1185</oboInOwl:hasDbXref>
</owl:Class>

<owl:Class rdf:about="&obo;FOODON_03401186">
	<rdfs:label xml:lang="en">10000200 - dressings/dips (shelf stable) (gs1 gpc)</rdfs:label>
	<rdfs:subClassOf rdf:resource="&obo;FOODON_03401183"/>
	<obo:IAO_0000412>http://langual.org</obo:IAO_0000412>
	<obo:IAO_0000115 xml:lang="en">Includes any products that can be described/observed as a pourable or spoonable substance, or a dehydrated combination of ingredients to which water or milk can be added to form a liquid. These products are usually served as an accompaniment to snacks or starters, such as crisps, tortilla chips, raw vegetables and pappadums, or poured cold over salads or vegetables. Products include dairy or mayonnaise based dressings, garlic and herb dips, cheese dips and taramasalata. These products have been treated or packaged in such a way as to extend their consumable life. Excludes products such as, Frozen and Perishable Dressings and Dips and Sauces, Condiments, Savoury Toppings, Savoury Spreads and Marinades.</obo:IAO_0000115>
	<obo:IAO_0000114 rdf:resource="&obo;IAO_0000428"/>
	<rdfs:comment xml:lang="en">LanguaL curation note: Index main ingredient in facet B and added ingredients in facet H. Index manufacturer's treatments (homogenized) in facet H. Index physical form (liquid, puree) in facet E. Index use claims (vegetarian/vegan), fat level claim (low fat, reduced fat) and organic claim in facet P.</rdfs:comment>
	<oboInOwl:hasDbXref>LANGUAL:A1186</oboInOwl:hasDbXref>
</owl:Class>

<owl:Class rdf:about="&obo;FOODON_03401187">
	<rdfs:label xml:lang="en">10000581 - food glazes (shelf stable) (gs1 gpc)</rdfs:label>
	<rdfs:subClassOf rdf:resource="&obo;FOODON_03401183"/>
	<obo:IAO_0000412>http://langual.org</obo:IAO_0000412>
	<obo:IAO_0000115 xml:lang="en">Includes any products that can be described/observed as a liquid that can be used to create a smooth, shiny surface on food, which is then decorated in various ways. It may be stock or gravy reduced to the thickness of jelly, a fruit based jelly or a thin sugar syrup to cover meat or confectionary. These products have been treated or packaged in such a way as to extend their consumable life. Excludes products such as Sauces Cooking; Sauces Dipping, Condiments, Savoury Toppings, Savoury Spreads and Marinades.</obo:IAO_0000115>
	<obo:IAO_0000114 rdf:resource="&obo;IAO_0000428"/>
	<rdfs:comment xml:lang="en">LanguaL curation note: Index the type of principal food product from which the glaze is made (fruit, meat) in facet B.</rdfs:comment>
	<oboInOwl:hasDbXref>LANGUAL:A1187</oboInOwl:hasDbXref>
</owl:Class>

<owl:Class rdf:about="&obo;FOODON_03401188">
	<rdfs:label xml:lang="en">10000576 - pate (frozen) (gs1 gpc)</rdfs:label>
	<rdfs:subClassOf rdf:resource="&obo;FOODON_03401183"/>
	<obo:IAO_0000412>http://langual.org</obo:IAO_0000412>
	<obo:IAO_0000115 xml:lang="en">Includes any products that can be described/observed as a frozen substance, which, upon defrosting, returns to its original consistency of a thick savoury mixture made from fish, meat, mushrooms or vegetables. Products may be coarsely textured or fine/smooth. Excludes products such as Sandwich Fillings, Pastes and Spreads; Dressings and Dips; Savoury Spreads and Toppings, Perishable and Shelf Stable Pate.</obo:IAO_0000115>
	<obo:IAO_0000114 rdf:resource="&obo;IAO_0000428"/>
	<rdfs:comment xml:lang="en">LanguaL curation note: Index the type of pate (beef, vegetable) in facet B. Index added ingredients (dairy, spices) in facet H. Index use claims (vegetarian/vegan), fat level claim (low fat, reduced fat) and organic claim in facet P.</rdfs:comment>
	<oboInOwl:hasDbXref>LANGUAL:A1188</oboInOwl:hasDbXref>
</owl:Class>

<owl:Class rdf:about="&obo;FOODON_03401189">
	<rdfs:label xml:lang="en">10000064 - pate (perishable) (gs1 gpc)</rdfs:label>
	<rdfs:subClassOf rdf:resource="&obo;FOODON_03401183"/>
	<obo:IAO_0000412>http://langual.org</obo:IAO_0000412>
	<obo:IAO_0000115 xml:lang="en">Includes any products that can be described/observed as a thick savoury mixture made from fish, meat, mushrooms or vegetables. Products may be coarsely textured or smooth. These products must be refrigerated to extend their consumable life. Excludes products such as Sandwich Fillings, Pastes and Spreads, Frozen and Shelf Stable Pate.</obo:IAO_0000115>
	<obo:IAO_0000114 rdf:resource="&obo;IAO_0000428"/>
	<rdfs:comment xml:lang="en">LanguaL curation note: Index the type of pate (beef, vegetable) in facet B. Index added ingredients (dairy, spices) in facet H. Index use claims (vegetarian/vegan), fat level claim (low fat, reduced fat) and organic claim in facet P. Index preservation method (refrigeration) in facet J.</rdfs:comment>
	<oboInOwl:hasDbXref>LANGUAL:A1189</oboInOwl:hasDbXref>
</owl:Class>

<owl:Class rdf:about="&obo;FOODON_03401190">
	<rdfs:label xml:lang="en">10000306 - pate (shelf stable) (gs1 gpc)</rdfs:label>
	<rdfs:subClassOf rdf:resource="&obo;FOODON_03401183"/>
	<obo:IAO_0000412>http://langual.org</obo:IAO_0000412>
	<obo:IAO_0000115 xml:lang="en">Includes any products that can be described/observed as a thick savoury mixture made from fish, meat, mushrooms or vegetables. Products may be coarsely textured or smooth. These products have been treated or packaged in such a way as to extend their consumable life. Excludes products such as Sandwich Fillings, Pastes and Spreads, Frozen and Perishable Pate.</obo:IAO_0000115>
	<obo:IAO_0000114 rdf:resource="&obo;IAO_0000428"/>
	<rdfs:comment xml:lang="en">LanguaL curation note: Index the type of pate (beef, vegetable) in facet B. Index added ingredients (dairy, spices) in facet H. Index use claims (vegetarian/vegan), fat level claim (low fat, reduced fat) and organic claim in facet P.</rdfs:comment>
	<oboInOwl:hasDbXref>LANGUAL:A1190</oboInOwl:hasDbXref>
</owl:Class>

<owl:Class rdf:about="&obo;FOODON_03401191">
	<rdfs:label xml:lang="en">10000056 - sauces - cooking (frozen) (gs1 gpc)</rdfs:label>
	<rdfs:subClassOf rdf:resource="&obo;FOODON_03401183"/>
	<obo:IAO_0000412>http://langual.org</obo:IAO_0000412>
	<obo:IAO_0000115 xml:lang="en">Includes any products that can be described/observed as a frozen substance, which can be heated and combined with other ingredients, such as pasta, rice and chicken, to produce a specific recipe, such as Bolognese, Carbonara, Chicken Korma or Thai Curry. Excludes products such as Sauces Dipping and Condiments and Savoury Spreads and Marinades, Perishable and Shelf Stable Sauces Cooking.</obo:IAO_0000115>
	<obo:IAO_0000114 rdf:resource="&obo;IAO_0000428"/>
	<rdfs:comment xml:lang="en">LanguaL curation note: Index use claims (vegetarian/vegan) and organic claim in facet P. Index added ingredients in facet H.</rdfs:comment>
	<oboInOwl:hasDbXref>LANGUAL:A1191</oboInOwl:hasDbXref>
</owl:Class>

<owl:Class rdf:about="&obo;FOODON_03401192">
	<rdfs:label xml:lang="en">10000055 - sauces - cooking (perishable) (gs1 gpc)</rdfs:label>
	<rdfs:subClassOf rdf:resource="&obo;FOODON_03401183"/>
	<obo:IAO_0000412>http://langual.org</obo:IAO_0000412>
	<obo:IAO_0000115 xml:lang="en">Includes any products that can be described/observed as a substance, which can be heated and combined with other ingredients, such as pasta, rice and chicken, to produce a specific recipe, such as Bolognese, Carbonara, Chicken Korma or Thai Curry. These products must be refrigerated to extend their consumable life. Excludes products such as Dipping Sauces and Condiments and Savoury Spreads and Marinades, Shelf Stable and Frozen Sauces Cooking.</obo:IAO_0000115>
	<obo:IAO_0000114 rdf:resource="&obo;IAO_0000428"/>
	<rdfs:comment xml:lang="en">LanguaL curation note: Index use claims (vegetarian/vegan) and organic claim in facet P. Index added ingredients in facet H. Index preservation method (refrigeration) in facet J.</rdfs:comment>
	<oboInOwl:hasDbXref>LANGUAL:A1192</oboInOwl:hasDbXref>
</owl:Class>

<owl:Class rdf:about="&obo;FOODON_03401193">
	<rdfs:label xml:lang="en">10000057 - sauces - cooking (shelf stable) (gs1 gpc)</rdfs:label>
	<rdfs:subClassOf rdf:resource="&obo;FOODON_03401183"/>
	<obo:IAO_0000412>http://langual.org</obo:IAO_0000412>
	<obo:IAO_0000115 xml:lang="en">Includes any products that can be described/observed as a liquid, or as a dehydrated combination of ingredients, which can be mixed with water, milk or stock, to form a liquid, which can be heated and combined with other ingredients, such as pasta, rice and chicken, to produce a specific recipe, such as Bolognese, Carbonara, Chicken Korma or Thai Curry. These products have been treated or packaged in such a way as to extend their consumable life. Excludes products such as Sauces Dipping and Condiments and Savoury Spreads and Marinades, Perishable and Frozen Sauces Cooking.</obo:IAO_0000115>
	<obo:IAO_0000114 rdf:resource="&obo;IAO_0000428"/>
	<rdfs:comment xml:lang="en">LanguaL curation note: Index use claims (vegetarian/vegan) and organic claim in facet P. Index added ingredients in facet H.</rdfs:comment>
	<oboInOwl:hasDbXref>LANGUAL:A1193</oboInOwl:hasDbXref>
</owl:Class>

<owl:Class rdf:about="&obo;FOODON_03401194">
	<rdfs:label xml:lang="en">10000577 - sauces dipping/condiments/savoury toppings/savoury spreads/marinades (frozen) (gs1 gpc)</rdfs:label>
	<rdfs:subClassOf rdf:resource="&obo;FOODON_03401183"/>
	<obo:IAO_0000412>http://langual.org</obo:IAO_0000412>
	<obo:IAO_0000115 xml:lang="en">Includes any products that can be described/observed as a frozen substance, which, upon defrosting, returns to its original consistency of a savoury liquid, paste, spread or granulated substance, which is usually used to enhance the flavour, appearance and texture of savoury foods. These products can be blended with other ingredients. Products include combinations of fish, meat, mushrooms, seafood, vegetables, herbs and spices. Excludes products such as Cooking Sauces; Dressings and Dips; Shelf Stable and Perishable Sauces Dipping, Condiments, Savoury Toppings, Savoury Spreads and Marinades.</obo:IAO_0000115>
	<obo:IAO_0000114 rdf:resource="&obo;IAO_0000428"/>
	<rdfs:comment xml:lang="en">LanguaL curation note: Index use claims (vegetarian/vegan) and organic claim in facet P. Index physical form (liquid, puree) in facet E. Index added ingredients (cheese, herbs) in facet H.</rdfs:comment>
	<oboInOwl:hasDbXref>LANGUAL:A1194</oboInOwl:hasDbXref>
</owl:Class>

<owl:Class rdf:about="&obo;FOODON_03401195">
	<rdfs:label xml:lang="en">10000054 - sauces dipping/condiments/savoury toppings/savoury spreads/marinades (perishable) (gs1 gpc)</rdfs:label>
	<rdfs:subClassOf rdf:resource="&obo;FOODON_03401183"/>
	<obo:IAO_0000412>http://langual.org</obo:IAO_0000412>
	<obo:IAO_0000115 xml:lang="en">Includes any products that can be described/observed as a savoury liquid, paste, spread or granulated substance, which is usually served as an accompaniment to savoury foods. These products can be blended with other ingredients. These products must be refrigerated to extend their consumable life. Products include liquids and spreads flavoured with, but not necessarily made from fish, meat, mushrooms, sea food or vegetables. Excludes products such as Cooking Sauces, Frozen and Shelf Stable Sauces Dipping, Condiments, Savoury Toppings, Savoury Spreads and Marinades.</obo:IAO_0000115>
	<obo:IAO_0000114 rdf:resource="&obo;IAO_0000428"/>
	<rdfs:comment xml:lang="en">LanguaL curation note: Index use claims (vegetarian/vegan) and organic claim in facet P. Index physical form (liquid, puree) in facet E. Index added ingredients (cheese, herbs) in facet H. Index preservation method (refrigeration) in facet J.</rdfs:comment>
	<oboInOwl:hasDbXref>LANGUAL:A1195</oboInOwl:hasDbXref>
</owl:Class>

<owl:Class rdf:about="&obo;FOODON_03401196">
	<rdfs:label xml:lang="en">10000280 - sauces dipping/condiments/savoury toppings/savoury spreads/marinades (shelf stable) (gs1 gpc)</rdfs:label>
	<rdfs:subClassOf rdf:resource="&obo;FOODON_03401183"/>
	<obo:IAO_0000412>http://langual.org</obo:IAO_0000412>
	<obo:IAO_0000115 xml:lang="en">Includes any products that can be described/observed as a savoury liquid, paste, spread or granulated substance, which is usually served as an accompaniment to savoury foods. These products can be blended with other ingredients. These products have been treated or packaged in such a way as to extend their consumable life. Products include liquids, spreads and granules flavoured with, but not necessarily made from fish, meat, mushrooms, seafood or vegetables. Excludes products such as Cooking Sauces, Frozen and Perishable Sauces Dipping, Condiments, Savoury Toppings, Savoury Spreads and Marinades.</obo:IAO_0000115>
	<obo:IAO_0000114 rdf:resource="&obo;IAO_0000428"/>
	<rdfs:comment xml:lang="en">LanguaL curation note: Index use claims (vegetarian/vegan) and organic claim in facet P. Index physical form (liquid, puree) in facet E. Index added ingredients (cheese, herbs) in facet H.</rdfs:comment>
	<oboInOwl:hasDbXref>LANGUAL:A1196</oboInOwl:hasDbXref>
</owl:Class>

<owl:Class rdf:about="&obo;FOODON_03401197">
	<rdfs:label xml:lang="en">10000617 - sauces/spreads/dips/condiments variety packs (gs1 gpc)</rdfs:label>
	<rdfs:subClassOf rdf:resource="&obo;FOODON_03401183"/>
	<obo:IAO_0000412>http://langual.org</obo:IAO_0000412>
	<obo:IAO_0000115 xml:lang="en">Includes any products that can be described/observed as two or more distinct Sauces, Spreads, Dips or Condiments sold together, which exist within the schema belonging to different bricks but to the same class, that is two or more products contained within the same pack which cross bricks within the Sauces, Spreads, Dips and Condiments class. Includes products such as Salad Dressings and Crunchy Savoury Toppings sold together. Items that are received free with purchases should be removed from the classification decision-making process. Excludes products such as Salad Dressing and Salad variety packs.</obo:IAO_0000115>
	<obo:IAO_0000114 rdf:resource="&obo;IAO_0000428"/>
	<oboInOwl:hasDbXref>LANGUAL:A1197</oboInOwl:hasDbXref>
</owl:Class>

<owl:Class rdf:about="&obo;FOODON_03401198">
	<rdfs:label xml:lang="en">50171700 - vinegars/cooking wines (gs1 gpc)</rdfs:label>
	<rdfs:subClassOf rdf:resource="&obo;FOODON_03401165"/>
	<obo:IAO_0000412>http://langual.org</obo:IAO_0000412>
	<obo:IAO_0000114 rdf:resource="&obo;IAO_0000428"/>
	<oboInOwl:hasDbXref>LANGUAL:A1198</oboInOwl:hasDbXref>
</owl:Class>

<owl:Class rdf:about="&obo;FOODON_03401199">
	<rdfs:label xml:lang="en">10000052 - cooking wines (gs1 gpc)</rdfs:label>
	<rdfs:subClassOf rdf:resource="&obo;FOODON_03401198"/>
	<obo:IAO_0000412>http://langual.org</obo:IAO_0000412>
	<obo:IAO_0000115 xml:lang="en">Includes any products that can be described/observed as a typically inferior variety of wine to Drinking Wine, sometimes adulterated with salt, which is used in cooking to enhance the flavour or colour of a prepared recipe. These products are specifically labelled and marketed as cooking wine, and their alcohol content ensures that they do not need to be refrigerated. Excludes products such as Wine or Sherry Alcoholic Beverages, and any alcohol not specifically used for cooking.</obo:IAO_0000115>
	<obo:IAO_0000114 rdf:resource="&obo;IAO_0000428"/>
	<rdfs:comment xml:lang="en">LanguaL curation note: If an industry recognized organic certification is claimed, index ORGANIC FOOD CLAIM OR USE in facet P. Index added ingredients (fruit, sugar) in facet H.</rdfs:comment>
	<oboInOwl:hasDbXref>LANGUAL:A1199</oboInOwl:hasDbXref>
</owl:Class>

<owl:Class rdf:about="&obo;FOODON_03401200">
	<rdfs:label xml:lang="en">10000051 - vinegars (gs1 gpc)</rdfs:label>
	<rdfs:subClassOf rdf:resource="&obo;FOODON_03401198"/>
	<obo:IAO_0000412>http://langual.org</obo:IAO_0000412>
	<obo:IAO_0000115 xml:lang="en">Includes any products that can be described/observed as a liquid, made from acetic acid derived from the fermentation of alcohol, mixed with water, and used as a flavouring, preservative, or condiment for savoury foods. Products include all varieties of vinegar, such as malt, red wine, white wine and balsamic. Excludes products such as Cooking Wines.</obo:IAO_0000115>
	<obo:IAO_0000114 rdf:resource="&obo;IAO_0000428"/>
	<rdfs:comment xml:lang="en">LanguaL curation note: If an industry recognized organic certification is claimed, index ORGANIC FOOD CLAIM OR USE in facet P. Index added ingredients (fruit, sugar) in facet H.</rdfs:comment>
	<oboInOwl:hasDbXref>LANGUAL:A1200</oboInOwl:hasDbXref>
</owl:Class>

<owl:Class rdf:about="&obo;FOODON_03401201">
	<rdfs:label xml:lang="en">10000618 - vinegars/cooking wines variety packs (gs1 gpc)</rdfs:label>
	<rdfs:subClassOf rdf:resource="&obo;FOODON_03401198"/>
	<obo:IAO_0000412>http://langual.org</obo:IAO_0000412>
	<obo:IAO_0000115 xml:lang="en">Includes any products that can be described/observed as two or more distinct Vinegars and Cooking Wines sold together, which exist within the schema belonging to different bricks but to the same class, that is two or more products contained within the same pack which cross bricks within the Vinegars and Cooking Wines class. Includes products such as Balsamic Vinegar and Cooking Wine sold together. Items that are received free with purchases should be removed from the classification decision-making process. Excludes products such as Balsamic Vinegar and Salad variety packs.</obo:IAO_0000115>
	<obo:IAO_0000114 rdf:resource="&obo;IAO_0000428"/>
	<oboInOwl:hasDbXref>LANGUAL:A1201</oboInOwl:hasDbXref>
</owl:Class>

<owl:Class rdf:about="&obo;FOODON_03401202">
	<rdfs:label xml:lang="en">50172000 - seasonings/preservatives/extracts variety packs (gs1 gpc)</rdfs:label>
	<rdfs:subClassOf rdf:resource="&obo;FOODON_03401165"/>
	<obo:IAO_0000412>http://langual.org</obo:IAO_0000412>
	<obo:IAO_0000115 xml:lang="en">Includes any products that can be described/observed as two or more distinct Seasonings, Preservatives or Extracts sold together which exist within the schema but belong to different classes, that is two or more products contained within the same pack which cross classes within the Seasonings, Preservatives and Extracts Family. Includes products such as Salt and Vinegar variety packs. Items that are received free with purchases should be removed from the classification decision-making process. Excludes products such as Salt and Pepper variety packs and Salad Dressing and Salad variety packs.</obo:IAO_0000115>
	<obo:IAO_0000114 rdf:resource="&obo;IAO_0000428"/>
	<oboInOwl:hasDbXref>LANGUAL:A1202</oboInOwl:hasDbXref>
</owl:Class>

<owl:Class rdf:about="&obo;FOODON_03401203">
	<rdfs:label xml:lang="en">sandwich (eurofir)</rdfs:label>
	<rdfs:subClassOf rdf:resource="&obo;FOODON_03400861"/>
	<obo:IAO_0000412>http://langual.org</obo:IAO_0000412>
	<obo:IAO_0000115 xml:lang="en">A sandwich is a food item made of two or more slices of leavened bread with one or more layers of filling, typically meat or cheese, with the addition of vegetables or salad. The bread can be used as is, or it can be coated with butter, oil, mustard or other condiments to enhance flavor and texture. (Wikipedia)</obo:IAO_0000115>
	<obo:IAO_0000114 rdf:resource="&obo;IAO_0000428"/>
	<oboInOwl:hasDbXref>LANGUAL:A1203</oboInOwl:hasDbXref>
</owl:Class>

<owl:Class rdf:about="&obo;FOODON_03401204">
	<rdfs:label xml:lang="en">pasta dish (eurofir)</rdfs:label>
	<rdfs:subClassOf rdf:resource="&obo;FOODON_03400822"/>
	<obo:IAO_0000412>http://langual.org</obo:IAO_0000412>
	<obo:IAO_0000114 rdf:resource="&obo;IAO_0000428"/>
	<oboInOwl:hasDbXref>LANGUAL:A1204</oboInOwl:hasDbXref>
</owl:Class>

<owl:Class rdf:about="&obo;FOODON_03401205">
	<rdfs:label xml:lang="en">food for weight reduction</rdfs:label>
	<rdfs:subClassOf rdf:resource="&obo;FOODON_03400871"/>
	<obo:IAO_0000412>http://langual.org</obo:IAO_0000412>
	<obo:IAO_0000114 rdf:resource="&obo;IAO_0000428"/>
	<oboInOwl:hasSynonym xml:lang="en">food intended for use in energy-restricted diets for weight reduction</oboInOwl:hasSynonym>
	<oboInOwl:hasDbXref>LANGUAL:A1205</oboInOwl:hasDbXref>
</owl:Class>

<owl:Class rdf:about="&obo;FOODON_03401206">
	<rdfs:label xml:lang="en">sports food</rdfs:label>
	<rdfs:subClassOf rdf:resource="&obo;FOODON_03400871"/>
	<obo:IAO_0000412>http://langual.org</obo:IAO_0000412>
	<obo:IAO_0000114 rdf:resource="&obo;IAO_0000428"/>
	<oboInOwl:hasSynonym xml:lang="en">food for sports people</oboInOwl:hasSynonym>
	<oboInOwl:hasSynonym xml:lang="en">food intended to meet the expenditure of intense muscular effort</oboInOwl:hasSynonym>
	<oboInOwl:hasDbXref>LANGUAL:A1206</oboInOwl:hasDbXref>
</owl:Class>

<owl:Class rdf:about="&obo;FOODON_03401207">
	<rdfs:label xml:lang="en">general standard for cheese (codex alimentarius)</rdfs:label>
	<rdfs:subClassOf rdf:resource="&obo;FOODON_03400352"/>
	<obo:IAO_0000412>http://langual.org</obo:IAO_0000412>
	<obo:IAO_0000115 xml:lang="en">CODEX STAN A-6-1978, Rev.1-1999, Amended 2006.</obo:IAO_0000115>
	<obo:IAO_0000114 rdf:resource="&obo;IAO_0000428"/>
	<rdfs:comment xml:lang="en">LanguaL curation note: This term is for CLASSIFICATION ONLY; DO NOT USE term in indexing. Use a more precise narrower term.</rdfs:comment>
	<oboInOwl:hasDbXref>LANGUAL:A1207</oboInOwl:hasDbXref>
</owl:Class>

<owl:Class rdf:about="&obo;FOODON_03401208">
	<rdfs:label xml:lang="en">designation according to principle cheese ripening characteristics (codex)</rdfs:label>
	<rdfs:subClassOf rdf:resource="&obo;FOODON_03401207"/>
	<obo:IAO_0000412>http://langual.org</obo:IAO_0000412>
	<obo:IAO_0000114 rdf:resource="&obo;IAO_0000428"/>
	<rdfs:comment xml:lang="en">LanguaL curation note: This term is for CLASSIFICATION ONLY; DO NOT USE term in indexing. Use a more precise narrower term.</rdfs:comment>
	<oboInOwl:hasDbXref>LANGUAL:A1208</oboInOwl:hasDbXref>
</owl:Class>

<owl:Class rdf:about="&obo;FOODON_03401209">
	<rdfs:label xml:lang="en">ripened (codex)</rdfs:label>
	<rdfs:subClassOf rdf:resource="&obo;FOODON_03401208"/>
	<obo:IAO_0000412>http://langual.org</obo:IAO_0000412>
	<obo:IAO_0000114 rdf:resource="&obo;IAO_0000428"/>
	<oboInOwl:hasSynonym xml:lang="en">matured cheese</oboInOwl:hasSynonym>
	<oboInOwl:hasDbXref>LANGUAL:A1209</oboInOwl:hasDbXref>
</owl:Class>

<owl:Class rdf:about="&obo;FOODON_03401210">
	<rdfs:label xml:lang="en">mould ripened (codex)</rdfs:label>
	<rdfs:subClassOf rdf:resource="&obo;FOODON_03401208"/>
	<obo:IAO_0000412>http://langual.org</obo:IAO_0000412>
	<obo:IAO_0000114 rdf:resource="&obo;IAO_0000428"/>
	<oboInOwl:hasDbXref>LANGUAL:A1210</oboInOwl:hasDbXref>
</owl:Class>

<owl:Class rdf:about="&obo;FOODON_03401211">
	<rdfs:label xml:lang="en">unripened (codex)</rdfs:label>
	<rdfs:subClassOf rdf:resource="&obo;FOODON_03401208"/>
	<obo:IAO_0000412>http://langual.org</obo:IAO_0000412>
	<obo:IAO_0000114 rdf:resource="&obo;IAO_0000428"/>
	<oboInOwl:hasSynonym xml:lang="en">fresh cheese</oboInOwl:hasSynonym>
	<oboInOwl:hasDbXref>LANGUAL:A1211</oboInOwl:hasDbXref>
</owl:Class>

<owl:Class rdf:about="&obo;FOODON_03401212">
	<rdfs:label xml:lang="en">in brine</rdfs:label>
	<rdfs:subClassOf rdf:resource="&obo;FOODON_03401208"/>
	<obo:IAO_0000412>http://langual.org</obo:IAO_0000412>
	<obo:IAO_0000114 rdf:resource="&obo;IAO_0000428"/>
	<oboInOwl:hasDbXref>LANGUAL:A1212</oboInOwl:hasDbXref>
</owl:Class>

<owl:Class rdf:about="&obo;FOODON_03401213">
	<rdfs:label xml:lang="en">designation according to milk fat content</rdfs:label>
	<rdfs:subClassOf rdf:resource="&obo;FOODON_03401207"/>
	<obo:IAO_0000412>http://langual.org</obo:IAO_0000412>
	<obo:IAO_0000114 rdf:resource="&obo;IAO_0000428"/>
	<rdfs:comment xml:lang="en">LanguaL curation note: This term is for CLASSIFICATION ONLY; DO NOT USE term in indexing. Use a more precise narrower term.</rdfs:comment>
	<oboInOwl:hasDbXref>LANGUAL:A1213</oboInOwl:hasDbXref>
</owl:Class>

<owl:Class rdf:about="&obo;FOODON_03401214">
	<rdfs:label xml:lang="en">high fat cheese (codex)</rdfs:label>
	<rdfs:subClassOf rdf:resource="&obo;FOODON_03401213"/>
	<obo:IAO_0000412>http://langual.org</obo:IAO_0000412>
	<obo:IAO_0000114 rdf:resource="&obo;IAO_0000428"/>
	<rdfs:comment xml:lang="en">LanguaL curation note: Used when the percentage of fat in dry matter is more than 60% [CODEX STAN A-6-1978, Rev.1-1999, Amended 2006]</rdfs:comment>
	<oboInOwl:hasDbXref>LANGUAL:A1214</oboInOwl:hasDbXref>
</owl:Class>

<owl:Class rdf:about="&obo;FOODON_03401215">
	<rdfs:label xml:lang="en">full fat cheese (codex)</rdfs:label>
	<rdfs:subClassOf rdf:resource="&obo;FOODON_03401213"/>
	<obo:IAO_0000412>http://langual.org</obo:IAO_0000412>
	<obo:IAO_0000114 rdf:resource="&obo;IAO_0000428"/>
	<rdfs:comment xml:lang="en">LanguaL curation note: Used when the percentage of fat in dry matter is above or equal to 45% and less than 60% [CODEX STAN A-6-1978, Rev.1-1999, Amended 2006].</rdfs:comment>
	<oboInOwl:hasDbXref>LANGUAL:A1215</oboInOwl:hasDbXref>
</owl:Class>

<owl:Class rdf:about="&obo;FOODON_03401216">
	<rdfs:label xml:lang="en">medium fat cheese (codex)</rdfs:label>
	<rdfs:subClassOf rdf:resource="&obo;FOODON_03401213"/>
	<obo:IAO_0000412>http://langual.org</obo:IAO_0000412>
	<obo:IAO_0000114 rdf:resource="&obo;IAO_0000428"/>
	<rdfs:comment xml:lang="en">LanguaL curation note: Used when the percentage of fat in dry matter is above or equal to 25% and less than 45% [CODEX STAN A-6-1978, Rev.1-1999, Amended 2006].</rdfs:comment>
	<oboInOwl:hasDbXref>LANGUAL:A1216</oboInOwl:hasDbXref>
</owl:Class>

<owl:Class rdf:about="&obo;FOODON_03401217">
	<rdfs:label xml:lang="en">partially skimmed cheese (codex)</rdfs:label>
	<rdfs:subClassOf rdf:resource="&obo;FOODON_03401213"/>
	<obo:IAO_0000412>http://langual.org</obo:IAO_0000412>
	<obo:IAO_0000114 rdf:resource="&obo;IAO_0000428"/>
	<rdfs:comment xml:lang="en">LanguaL curation note: Used when the percentage of fat in dry matter is above or equal to 10% and less than 25% [CODEX STAN A-6-1978, Rev.1-1999, Amended 2006].</rdfs:comment>
	<oboInOwl:hasDbXref>LANGUAL:A1217</oboInOwl:hasDbXref>
</owl:Class>

<owl:Class rdf:about="&obo;FOODON_03401218">
	<rdfs:label xml:lang="en">skim cheese (codex)</rdfs:label>
	<rdfs:subClassOf rdf:resource="&obo;FOODON_03401213"/>
	<obo:IAO_0000412>http://langual.org</obo:IAO_0000412>
	<obo:IAO_0000114 rdf:resource="&obo;IAO_0000428"/>
	<rdfs:comment xml:lang="en">LanguaL curation note: Used when the percentage of fat in dry matter is less than 10% [CODEX STAN A-6-1978, Rev.1-1999, Amended 2006].</rdfs:comment>
	<oboInOwl:hasDbXref>LANGUAL:A1218</oboInOwl:hasDbXref>
</owl:Class>

<owl:Class rdf:about="&obo;FOODON_03401219">
	<rdfs:label xml:lang="en">semisoft part skim cheese (us cfr)</rdfs:label>
	<rdfs:subClassOf rdf:resource="&obo;FOODON_03400316"/>
	<obo:IAO_0000412>http://langual.org</obo:IAO_0000412>
	<obo:IAO_0000114 rdf:resource="&obo;IAO_0000428"/>
	<rdfs:comment xml:lang="en">LanguaL curation note: Used for cheeses, which contain not more than 50 percent of moisture, and their solids contain more than 45, but less than 50 percent, of milkfat [21 CFR Ch. I (4-1-99 Edition)]</rdfs:comment>
	<oboInOwl:hasDbXref>LANGUAL:A1219</oboInOwl:hasDbXref>
</owl:Class>

<owl:Class rdf:about="&obo;FOODON_03401220">
	<rdfs:label xml:lang="en">classification of products of plant and animal origin, european community</rdfs:label>
	<rdfs:subClassOf rdf:resource="&obo;FOODON_03400356"/>
	<obo:IAO_0000412>http://langual.org</obo:IAO_0000412>
	<obo:IAO_0000115 xml:lang="en">Top level classes as defined in COMMISSION REGULATION (EC) No 178/2006 of 1 February 2006 amending Regulation (EC) No 396/2005 of the European Parliament and of the Council to establish Annex I listing the food and feed products to which maximum levels for pesticide residues apply. Further ammended and updated by COMMISSION REGULATION (EU) No 600/2010 of 8 July 2010.[http://eur-lex.europa.eu/LexUriServ/LexUriServ.do?uri=OJ:L:2010:174:0018:0039:EN:PDF]</obo:IAO_0000115>
	<obo:IAO_0000114 rdf:resource="&obo;IAO_0000428"/>
	<rdfs:comment xml:lang="en">LanguaL curation note: This term is for CLASSIFICATION ONLY; DO NOT USE term in indexing. Use a more precise narrower term.</rdfs:comment>
	<oboInOwl:hasDbXref>LANGUAL:A1220</oboInOwl:hasDbXref>
</owl:Class>

<owl:Class rdf:about="&obo;FOODON_03401221">
	<rdfs:label xml:lang="en">0100000 - 1. fruit fresh or frozen; nuts (ec)</rdfs:label>
	<rdfs:subClassOf rdf:resource="&obo;FOODON_03401220"/>
	<obo:IAO_0000412>http://langual.org</obo:IAO_0000412>
	<obo:IAO_0000115 xml:lang="en">COMMISSION REGULATION (EC) No 178/2006 of 1 February 2006 amending Regulation (EC) No 396/2005 of the European Parliament and of the Council.</obo:IAO_0000115>
	<obo:IAO_0000114 rdf:resource="&obo;IAO_0000428"/>
	<oboInOwl:hasDbXref>LANGUAL:A1221</oboInOwl:hasDbXref>
</owl:Class>

<owl:Class rdf:about="&obo;FOODON_03401222">
	<rdfs:label xml:lang="en">0110000 - citrus fruit (ec)</rdfs:label>
	<rdfs:subClassOf rdf:resource="&obo;FOODON_03401221"/>
	<obo:IAO_0000412>http://langual.org</obo:IAO_0000412>
	<obo:IAO_0000115 xml:lang="en">COMMISSION REGULATION (EC) No 178/2006 of 1 February 2006 amending Regulation (EC) No 396/2005 of the European Parliament and of the Council.</obo:IAO_0000115>
	<obo:IAO_0000114 rdf:resource="&obo;IAO_0000428"/>
	<oboInOwl:hasDbXref>LANGUAL:A1222</oboInOwl:hasDbXref>
</owl:Class>

<owl:Class rdf:about="&obo;FOODON_03401223">
	<rdfs:label xml:lang="en">0120000 - tree nuts (shelled or unshelled) (ec)</rdfs:label>
	<rdfs:subClassOf rdf:resource="&obo;FOODON_03401221"/>
	<obo:IAO_0000412>http://langual.org</obo:IAO_0000412>
	<obo:IAO_0000115 xml:lang="en">COMMISSION REGULATION (EC) No 178/2006 of 1 February 2006 amending Regulation (EC) No 396/2005 of the European Parliament and of the Council.</obo:IAO_0000115>
	<obo:IAO_0000114 rdf:resource="&obo;IAO_0000428"/>
	<oboInOwl:hasDbXref>LANGUAL:A1223</oboInOwl:hasDbXref>
</owl:Class>

<owl:Class rdf:about="&obo;FOODON_03401224">
	<rdfs:label xml:lang="en">0130000 - pome fruit (ec)</rdfs:label>
	<rdfs:subClassOf rdf:resource="&obo;FOODON_03401221"/>
	<obo:IAO_0000412>http://langual.org</obo:IAO_0000412>
	<obo:IAO_0000115 xml:lang="en">COMMISSION REGULATION (EC) No 178/2006 of 1 February 2006 amending Regulation (EC) No 396/2005 of the European Parliament and of the Council.</obo:IAO_0000115>
	<obo:IAO_0000114 rdf:resource="&obo;IAO_0000428"/>
	<oboInOwl:hasDbXref>LANGUAL:A1224</oboInOwl:hasDbXref>
</owl:Class>

<owl:Class rdf:about="&obo;FOODON_03401225">
	<rdfs:label xml:lang="en">0140000 - stone fruit (ec)</rdfs:label>
	<rdfs:subClassOf rdf:resource="&obo;FOODON_03401221"/>
	<obo:IAO_0000412>http://langual.org</obo:IAO_0000412>
	<obo:IAO_0000115 xml:lang="en">COMMISSION REGULATION (EC) No 178/2006 of 1 February 2006 amending Regulation (EC) No 396/2005 of the European Parliament and of the Council.</obo:IAO_0000115>
	<obo:IAO_0000114 rdf:resource="&obo;IAO_0000428"/>
	<oboInOwl:hasDbXref>LANGUAL:A1225</oboInOwl:hasDbXref>
</owl:Class>

<owl:Class rdf:about="&obo;FOODON_03401226">
	<rdfs:label xml:lang="en">0150000 - berries and small fruit (ec)</rdfs:label>
	<rdfs:subClassOf rdf:resource="&obo;FOODON_03401221"/>
	<obo:IAO_0000412>http://langual.org</obo:IAO_0000412>
	<obo:IAO_0000115 xml:lang="en">COMMISSION REGULATION (EC) No 178/2006 of 1 February 2006 amending Regulation (EC) No 396/2005 of the European Parliament and of the Council.</obo:IAO_0000115>
	<obo:IAO_0000114 rdf:resource="&obo;IAO_0000428"/>
	<oboInOwl:hasDbXref>LANGUAL:A1226</oboInOwl:hasDbXref>
</owl:Class>

<owl:Class rdf:about="&obo;FOODON_03401227">
	<rdfs:label xml:lang="en">0200000 - 2. vegetables fresh or frozen (ec)</rdfs:label>
	<rdfs:subClassOf rdf:resource="&obo;FOODON_03401220"/>
	<obo:IAO_0000412>http://langual.org</obo:IAO_0000412>
	<obo:IAO_0000115 xml:lang="en">COMMISSION REGULATION (EC) No 178/2006 of 1 February 2006 amending Regulation (EC) No 396/2005 of the European Parliament and of the Council.</obo:IAO_0000115>
	<obo:IAO_0000114 rdf:resource="&obo;IAO_0000428"/>
	<oboInOwl:hasDbXref>LANGUAL:A1227</oboInOwl:hasDbXref>
</owl:Class>

<owl:Class rdf:about="&obo;FOODON_03401228">
	<rdfs:label xml:lang="en">0210000 - root and tuber vegetables (ec)</rdfs:label>
	<rdfs:subClassOf rdf:resource="&obo;FOODON_03401227"/>
	<obo:IAO_0000412>http://langual.org</obo:IAO_0000412>
	<obo:IAO_0000115 xml:lang="en">COMMISSION REGULATION (EC) No 178/2006 of 1 February 2006 amending Regulation (EC) No 396/2005 of the European Parliament and of the Council.</obo:IAO_0000115>
	<obo:IAO_0000114 rdf:resource="&obo;IAO_0000428"/>
	<oboInOwl:hasDbXref>LANGUAL:A1228</oboInOwl:hasDbXref>
</owl:Class>

<owl:Class rdf:about="&obo;FOODON_03401229">
	<rdfs:label xml:lang="en">0220000 - bulb vegetables (ec)</rdfs:label>
	<rdfs:subClassOf rdf:resource="&obo;FOODON_03401227"/>
	<obo:IAO_0000412>http://langual.org</obo:IAO_0000412>
	<obo:IAO_0000115 xml:lang="en">COMMISSION REGULATION (EC) No 178/2006 of 1 February 2006 amending Regulation (EC) No 396/2005 of the European Parliament and of the Council.</obo:IAO_0000115>
	<obo:IAO_0000114 rdf:resource="&obo;IAO_0000428"/>
	<oboInOwl:hasDbXref>LANGUAL:A1229</oboInOwl:hasDbXref>
</owl:Class>

<owl:Class rdf:about="&obo;FOODON_03401230">
	<rdfs:label xml:lang="en">0230000 - fruiting vegetables (ec)</rdfs:label>
	<rdfs:subClassOf rdf:resource="&obo;FOODON_03401227"/>
	<obo:IAO_0000412>http://langual.org</obo:IAO_0000412>
	<obo:IAO_0000115 xml:lang="en">COMMISSION REGULATION (EC) No 178/2006 of 1 February 2006 amending Regulation (EC) No 396/2005 of the European Parliament and of the Council.</obo:IAO_0000115>
	<obo:IAO_0000114 rdf:resource="&obo;IAO_0000428"/>
	<oboInOwl:hasDbXref>LANGUAL:A1230</oboInOwl:hasDbXref>
</owl:Class>

<owl:Class rdf:about="&obo;FOODON_03401231">
	<rdfs:label xml:lang="en">0240000 - brassica vegetables (ec)</rdfs:label>
	<rdfs:subClassOf rdf:resource="&obo;FOODON_03401227"/>
	<obo:IAO_0000412>http://langual.org</obo:IAO_0000412>
	<obo:IAO_0000115 xml:lang="en">COMMISSION REGULATION (EC) No 178/2006 of 1 February 2006 amending Regulation (EC) No 396/2005 of the European Parliament and of the Council.</obo:IAO_0000115>
	<obo:IAO_0000114 rdf:resource="&obo;IAO_0000428"/>
	<oboInOwl:hasDbXref>LANGUAL:A1231</oboInOwl:hasDbXref>
</owl:Class>

<owl:Class rdf:about="&obo;FOODON_03401232">
	<rdfs:label xml:lang="en">0250000 - leaf vegetables and herbs (ec)</rdfs:label>
	<rdfs:subClassOf rdf:resource="&obo;FOODON_03401227"/>
	<obo:IAO_0000412>http://langual.org</obo:IAO_0000412>
	<obo:IAO_0000115 xml:lang="en">COMMISSION REGULATION (EC) No 178/2006 of 1 February 2006 amending Regulation (EC) No 396/2005 of the European Parliament and of the Council.</obo:IAO_0000115>
	<obo:IAO_0000114 rdf:resource="&obo;IAO_0000428"/>
	<oboInOwl:hasDbXref>LANGUAL:A1232</oboInOwl:hasDbXref>
</owl:Class>

<owl:Class rdf:about="&obo;FOODON_03401233">
	<rdfs:label xml:lang="en">0260000 - legume vegetables (ec)</rdfs:label>
	<rdfs:subClassOf rdf:resource="&obo;FOODON_03401227"/>
	<obo:IAO_0000412>http://langual.org</obo:IAO_0000412>
	<obo:IAO_0000115 xml:lang="en">COMMISSION REGULATION (EC) No 178/2006 of 1 February 2006 amending Regulation (EC) No 396/2005 of the European Parliament and of the Council.</obo:IAO_0000115>
	<obo:IAO_0000114 rdf:resource="&obo;IAO_0000428"/>
	<oboInOwl:hasDbXref>LANGUAL:A1233</oboInOwl:hasDbXref>
</owl:Class>

<owl:Class rdf:about="&obo;FOODON_03401234">
	<rdfs:label xml:lang="en">0270000 - stem vegetables (ec)</rdfs:label>
	<rdfs:subClassOf rdf:resource="&obo;FOODON_03401227"/>
	<obo:IAO_0000412>http://langual.org</obo:IAO_0000412>
	<obo:IAO_0000115 xml:lang="en">COMMISSION REGULATION (EC) No 178/2006 of 1 February 2006 amending Regulation (EC) No 396/2005 of the European Parliament and of the Council.</obo:IAO_0000115>
	<obo:IAO_0000114 rdf:resource="&obo;IAO_0000428"/>
	<oboInOwl:hasDbXref>LANGUAL:A1234</oboInOwl:hasDbXref>
</owl:Class>

<owl:Class rdf:about="&obo;FOODON_03401235">
	<rdfs:label xml:lang="en">0280000 - fungi (ec)</rdfs:label>
	<rdfs:subClassOf rdf:resource="&obo;FOODON_03401227"/>
	<obo:IAO_0000412>http://langual.org</obo:IAO_0000412>
	<obo:IAO_0000115 xml:lang="en">COMMISSION REGULATION (EC) No 178/2006 of 1 February 2006 amending Regulation (EC) No 396/2005 of the European Parliament and of the Council.</obo:IAO_0000115>
	<obo:IAO_0000114 rdf:resource="&obo;IAO_0000428"/>
	<oboInOwl:hasDbXref>LANGUAL:A1235</oboInOwl:hasDbXref>
</owl:Class>

<owl:Class rdf:about="&obo;FOODON_03401236">
	<rdfs:label xml:lang="en">0300000 - 3. pulses, dry (ec)</rdfs:label>
	<rdfs:subClassOf rdf:resource="&obo;FOODON_03401220"/>
	<obo:IAO_0000412>http://langual.org</obo:IAO_0000412>
	<obo:IAO_0000115 xml:lang="en">COMMISSION REGULATION (EC) No 178/2006 of 1 February 2006 amending Regulation (EC) No 396/2005 of the European Parliament and of the Council.</obo:IAO_0000115>
	<obo:IAO_0000114 rdf:resource="&obo;IAO_0000428"/>
	<oboInOwl:hasDbXref>LANGUAL:A1236</oboInOwl:hasDbXref>
</owl:Class>

<owl:Class rdf:about="&obo;FOODON_03401237">
	<rdfs:label xml:lang="en">0400000 - 4. oilseeds and oilfruits (ec)</rdfs:label>
	<rdfs:subClassOf rdf:resource="&obo;FOODON_03401220"/>
	<obo:IAO_0000412>http://langual.org</obo:IAO_0000412>
	<obo:IAO_0000115 xml:lang="en">COMMISSION REGULATION (EC) No 178/2006 of 1 February 2006 amending Regulation (EC) No 396/2005 of the European Parliament and of the Council.</obo:IAO_0000115>
	<obo:IAO_0000114 rdf:resource="&obo;IAO_0000428"/>
	<oboInOwl:hasDbXref>LANGUAL:A1237</oboInOwl:hasDbXref>
</owl:Class>

<owl:Class rdf:about="&obo;FOODON_03401238">
	<rdfs:label xml:lang="en">0401000 - oilseeds (ec)</rdfs:label>
	<rdfs:subClassOf rdf:resource="&obo;FOODON_03401237"/>
	<obo:IAO_0000412>http://langual.org</obo:IAO_0000412>
	<obo:IAO_0000115 xml:lang="en">COMMISSION REGULATION (EC) No 178/2006 of 1 February 2006 amending Regulation (EC) No 396/2005 of the European Parliament and of the Council.</obo:IAO_0000115>
	<obo:IAO_0000114 rdf:resource="&obo;IAO_0000428"/>
	<oboInOwl:hasDbXref>LANGUAL:A1238</oboInOwl:hasDbXref>
</owl:Class>

<owl:Class rdf:about="&obo;FOODON_03401239">
	<rdfs:label xml:lang="en">0402000 - oilfruits (ec)</rdfs:label>
	<rdfs:subClassOf rdf:resource="&obo;FOODON_03401237"/>
	<obo:IAO_0000412>http://langual.org</obo:IAO_0000412>
	<obo:IAO_0000115 xml:lang="en">COMMISSION REGULATION (EC) No 178/2006 of 1 February 2006 amending Regulation (EC) No 396/2005 of the European Parliament and of the Council.</obo:IAO_0000115>
	<obo:IAO_0000114 rdf:resource="&obo;IAO_0000428"/>
	<oboInOwl:hasDbXref>LANGUAL:A1239</oboInOwl:hasDbXref>
</owl:Class>

<owl:Class rdf:about="&obo;FOODON_03401240">
	<rdfs:label xml:lang="en">0500000 - 5. cereals (ec)</rdfs:label>
	<rdfs:subClassOf rdf:resource="&obo;FOODON_03401220"/>
	<obo:IAO_0000412>http://langual.org</obo:IAO_0000412>
	<obo:IAO_0000115 xml:lang="en">COMMISSION REGULATION (EC) No 178/2006 of 1 February 2006 amending Regulation (EC) No 396/2005 of the European Parliament and of the Council.</obo:IAO_0000115>
	<obo:IAO_0000114 rdf:resource="&obo;IAO_0000428"/>
	<oboInOwl:hasDbXref>LANGUAL:A1240</oboInOwl:hasDbXref>
</owl:Class>

<owl:Class rdf:about="&obo;FOODON_03401241">
	<rdfs:label xml:lang="en">0600000 - 6. tea, coffee, herbal infusions and cocoa (ec)</rdfs:label>
	<rdfs:subClassOf rdf:resource="&obo;FOODON_03401220"/>
	<obo:IAO_0000412>http://langual.org</obo:IAO_0000412>
	<obo:IAO_0000115 xml:lang="en">COMMISSION REGULATION (EC) No 178/2006 of 1 February 2006 amending Regulation (EC) No 396/2005 of the European Parliament and of the Council.</obo:IAO_0000115>
	<obo:IAO_0000114 rdf:resource="&obo;IAO_0000428"/>
	<oboInOwl:hasDbXref>LANGUAL:A1241</oboInOwl:hasDbXref>
</owl:Class>

<owl:Class rdf:about="&obo;FOODON_03401242">
	<rdfs:label xml:lang="en">0610000 - tea (ec)</rdfs:label>
	<rdfs:subClassOf rdf:resource="&obo;FOODON_03401241"/>
	<obo:IAO_0000412>http://langual.org</obo:IAO_0000412>
	<obo:IAO_0000115 xml:lang="en">COMMISSION REGULATION (EC) No 178/2006 of 1 February 2006 amending Regulation (EC) No 396/2005 of the European Parliament and of the Council.</obo:IAO_0000115>
	<obo:IAO_0000114 rdf:resource="&obo;IAO_0000428"/>
	<rdfs:comment xml:lang="en">LanguaL curation note: Include dried leaves and stalks, fermented or otherwise of Camellia sinensis.</rdfs:comment>
	<oboInOwl:hasDbXref>LANGUAL:A1242</oboInOwl:hasDbXref>
</owl:Class>

<owl:Class rdf:about="&obo;FOODON_03401243">
	<rdfs:label xml:lang="en">0620000 - coffee beans (ec)</rdfs:label>
	<rdfs:subClassOf rdf:resource="&obo;FOODON_03401241"/>
	<obo:IAO_0000412>http://langual.org</obo:IAO_0000412>
	<obo:IAO_0000115 xml:lang="en">COMMISSION REGULATION (EC) No 178/2006 of 1 February 2006 amending Regulation (EC) No 396/2005 of the European Parliament and of the Council.</obo:IAO_0000115>
	<obo:IAO_0000114 rdf:resource="&obo;IAO_0000428"/>
	<oboInOwl:hasDbXref>LANGUAL:A1243</oboInOwl:hasDbXref>
</owl:Class>

<owl:Class rdf:about="&obo;FOODON_03401244">
	<rdfs:label xml:lang="en">0630000 - herbal infusions (ec)</rdfs:label>
	<rdfs:subClassOf rdf:resource="&obo;FOODON_03401241"/>
	<obo:IAO_0000412>http://langual.org</obo:IAO_0000412>
	<obo:IAO_0000115 xml:lang="en">COMMISSION REGULATION (EC) No 178/2006 of 1 February 2006 amending Regulation (EC) No 396/2005 of the European Parliament and of the Council.</obo:IAO_0000115>
	<obo:IAO_0000114 rdf:resource="&obo;IAO_0000428"/>
	<oboInOwl:hasDbXref>LANGUAL:A1244</oboInOwl:hasDbXref>
</owl:Class>

<owl:Class rdf:about="&obo;FOODON_03401245">
	<rdfs:label xml:lang="en">0640000 - cocoa (ec)</rdfs:label>
	<rdfs:subClassOf rdf:resource="&obo;FOODON_03401241"/>
	<obo:IAO_0000412>http://langual.org</obo:IAO_0000412>
	<obo:IAO_0000115 xml:lang="en">COMMISSION REGULATION (EC) No 178/2006 of 1 February 2006 amending Regulation (EC) No 396/2005 of the European Parliament and of the Council.</obo:IAO_0000115>
	<obo:IAO_0000114 rdf:resource="&obo;IAO_0000428"/>
	<oboInOwl:hasDbXref>LANGUAL:A1245</oboInOwl:hasDbXref>
</owl:Class>

<owl:Class rdf:about="&obo;FOODON_03401246">
	<rdfs:label xml:lang="en">0650000 - carob (ec)</rdfs:label>
	<rdfs:subClassOf rdf:resource="&obo;FOODON_03401241"/>
	<obo:IAO_0000412>http://langual.org</obo:IAO_0000412>
	<obo:IAO_0000115 xml:lang="en">COMMISSION REGULATION (EC) No 178/2006 of 1 February 2006 amending Regulation (EC) No 396/2005 of the European Parliament and of the Council.</obo:IAO_0000115>
	<obo:IAO_0000114 rdf:resource="&obo;IAO_0000428"/>
	<oboInOwl:hasSynonym xml:lang="en">st johns bread</oboInOwl:hasSynonym>
	<oboInOwl:hasDbXref>LANGUAL:A1246</oboInOwl:hasDbXref>
</owl:Class>

<owl:Class rdf:about="&obo;FOODON_03401247">
	<rdfs:label xml:lang="en">0700000 - hops (dried) (ec)</rdfs:label>
	<rdfs:subClassOf rdf:resource="&obo;FOODON_03401220"/>
	<obo:IAO_0000412>http://langual.org</obo:IAO_0000412>
	<obo:IAO_0000115 xml:lang="en">COMMISSION REGULATION (EC) No 178/2006 of 1 February 2006 amending Regulation (EC) No 396/2005 of the European Parliament and of the Council.</obo:IAO_0000115>
	<obo:IAO_0000114 rdf:resource="&obo;IAO_0000428"/>
	<rdfs:comment xml:lang="en">LanguaL curation note: Including hop pellets and unconcentrated powder.</rdfs:comment>
	<oboInOwl:hasDbXref>LANGUAL:A1247</oboInOwl:hasDbXref>
</owl:Class>

<owl:Class rdf:about="&obo;FOODON_03401248">
	<rdfs:label xml:lang="en">0800000 - spices (ec)</rdfs:label>
	<rdfs:subClassOf rdf:resource="&obo;FOODON_03401220"/>
	<obo:IAO_0000412>http://langual.org</obo:IAO_0000412>
	<obo:IAO_0000115 xml:lang="en">COMMISSION REGULATION (EC) No 178/2006 of 1 February 2006 amending Regulation (EC) No 396/2005 of the European Parliament and of the Council.</obo:IAO_0000115>
	<obo:IAO_0000114 rdf:resource="&obo;IAO_0000428"/>
	<oboInOwl:hasDbXref>LANGUAL:A1248</oboInOwl:hasDbXref>
</owl:Class>

<owl:Class rdf:about="&obo;FOODON_03401249">
	<rdfs:label xml:lang="en">0810000 - spices, seeds (ec)</rdfs:label>
	<rdfs:subClassOf rdf:resource="&obo;FOODON_03401248"/>
	<obo:IAO_0000412>http://langual.org</obo:IAO_0000412>
	<obo:IAO_0000115 xml:lang="en">COMMISSION REGULATION (EC) No 178/2006 of 1 February 2006 amending Regulation (EC) No 396/2005 of the European Parliament and of the Council.</obo:IAO_0000115>
	<obo:IAO_0000114 rdf:resource="&obo;IAO_0000428"/>
	<oboInOwl:hasDbXref>LANGUAL:A1249</oboInOwl:hasDbXref>
</owl:Class>

<owl:Class rdf:about="&obo;FOODON_03401250">
	<rdfs:label xml:lang="en">0820000 - spices, fruits and berries (ec)</rdfs:label>
	<rdfs:subClassOf rdf:resource="&obo;FOODON_03401248"/>
	<obo:IAO_0000412>http://langual.org</obo:IAO_0000412>
	<obo:IAO_0000115 xml:lang="en">COMMISSION REGULATION (EC) No 178/2006 of 1 February 2006 amending Regulation (EC) No 396/2005 of the European Parliament and of the Council.</obo:IAO_0000115>
	<obo:IAO_0000114 rdf:resource="&obo;IAO_0000428"/>
	<oboInOwl:hasDbXref>LANGUAL:A1250</oboInOwl:hasDbXref>
</owl:Class>

<owl:Class rdf:about="&obo;FOODON_03401251">
	<rdfs:label xml:lang="en">0830000 - spices, bark (ec)</rdfs:label>
	<rdfs:subClassOf rdf:resource="&obo;FOODON_03401248"/>
	<obo:IAO_0000412>http://langual.org</obo:IAO_0000412>
	<obo:IAO_0000115 xml:lang="en">COMMISSION REGULATION (EC) No 178/2006 of 1 February 2006 amending Regulation (EC) No 396/2005 of the European Parliament and of the Council.</obo:IAO_0000115>
	<obo:IAO_0000114 rdf:resource="&obo;IAO_0000428"/>
	<oboInOwl:hasDbXref>LANGUAL:A1251</oboInOwl:hasDbXref>
</owl:Class>

<owl:Class rdf:about="&obo;FOODON_03401252">
	<rdfs:label xml:lang="en">0840000 - spices, roots or rhizome (ec)</rdfs:label>
	<rdfs:subClassOf rdf:resource="&obo;FOODON_03401248"/>
	<obo:IAO_0000412>http://langual.org</obo:IAO_0000412>
	<obo:IAO_0000115 xml:lang="en">COMMISSION REGULATION (EC) No 178/2006 of 1 February 2006 amending Regulation (EC) No 396/2005 of the European Parliament and of the Council.</obo:IAO_0000115>
	<obo:IAO_0000114 rdf:resource="&obo;IAO_0000428"/>
	<oboInOwl:hasDbXref>LANGUAL:A1252</oboInOwl:hasDbXref>
</owl:Class>

<owl:Class rdf:about="&obo;FOODON_03401253">
	<rdfs:label xml:lang="en">0850000 - spices, buds (ec)</rdfs:label>
	<rdfs:subClassOf rdf:resource="&obo;FOODON_03401248"/>
	<obo:IAO_0000412>http://langual.org</obo:IAO_0000412>
	<obo:IAO_0000115 xml:lang="en">COMMISSION REGULATION (EC) No 178/2006 of 1 February 2006 amending Regulation (EC) No 396/2005 of the European Parliament and of the Council.</obo:IAO_0000115>
	<obo:IAO_0000114 rdf:resource="&obo;IAO_0000428"/>
	<oboInOwl:hasDbXref>LANGUAL:A1253</oboInOwl:hasDbXref>
</owl:Class>

<owl:Class rdf:about="&obo;FOODON_03401254">
	<rdfs:label xml:lang="en">0860000 - spices, flower stigma (ec)</rdfs:label>
	<rdfs:subClassOf rdf:resource="&obo;FOODON_03401248"/>
	<obo:IAO_0000412>http://langual.org</obo:IAO_0000412>
	<obo:IAO_0000115 xml:lang="en">COMMISSION REGULATION (EC) No 178/2006 of 1 February 2006 amending Regulation (EC) No 396/2005 of the European Parliament and of the Council.</obo:IAO_0000115>
	<obo:IAO_0000114 rdf:resource="&obo;IAO_0000428"/>
	<oboInOwl:hasDbXref>LANGUAL:A1254</oboInOwl:hasDbXref>
</owl:Class>

<owl:Class rdf:about="&obo;FOODON_03401255">
	<rdfs:label xml:lang="en">0870000 - spices, aril (ec)</rdfs:label>
	<rdfs:subClassOf rdf:resource="&obo;FOODON_03401248"/>
	<obo:IAO_0000412>http://langual.org</obo:IAO_0000412>
	<obo:IAO_0000115 xml:lang="en">COMMISSION REGULATION (EC) No 178/2006 of 1 February 2006 amending Regulation (EC) No 396/2005 of the European Parliament and of the Council.</obo:IAO_0000115>
	<obo:IAO_0000114 rdf:resource="&obo;IAO_0000428"/>
	<oboInOwl:hasDbXref>LANGUAL:A1255</oboInOwl:hasDbXref>
</owl:Class>

<owl:Class rdf:about="&obo;FOODON_03401256">
	<rdfs:label xml:lang="en">0900000 - 9. sugar plants (ec)</rdfs:label>
	<rdfs:subClassOf rdf:resource="&obo;FOODON_03401220"/>
	<obo:IAO_0000412>http://langual.org</obo:IAO_0000412>
	<obo:IAO_0000115 xml:lang="en">COMMISSION REGULATION (EC) No 178/2006 of 1 February 2006 amending Regulation (EC) No 396/2005 of the European Parliament and of the Council.</obo:IAO_0000115>
	<obo:IAO_0000114 rdf:resource="&obo;IAO_0000428"/>
	<oboInOwl:hasDbXref>LANGUAL:A1256</oboInOwl:hasDbXref>
</owl:Class>

<owl:Class rdf:about="&obo;FOODON_03401257">
	<rdfs:label xml:lang="en">1000000 - 10. products of animal origin - terrestrial animals (ec)</rdfs:label>
	<rdfs:subClassOf rdf:resource="&obo;FOODON_03401220"/>
	<obo:IAO_0000412>http://langual.org</obo:IAO_0000412>
	<obo:IAO_0000115 xml:lang="en">COMMISSION REGULATION (EC) No 178/2006 of 1 February 2006 amending Regulation (EC) No 396/2005 of the European Parliament and of the Council.</obo:IAO_0000115>
	<obo:IAO_0000114 rdf:resource="&obo;IAO_0000428"/>
	<oboInOwl:hasDbXref>LANGUAL:A1257</oboInOwl:hasDbXref>
</owl:Class>

<owl:Class rdf:about="&obo;FOODON_03401258">
	<rdfs:label xml:lang="en">1010000 - meat (ec)</rdfs:label>
	<rdfs:subClassOf rdf:resource="&obo;FOODON_03401257"/>
	<obo:IAO_0000412>http://langual.org</obo:IAO_0000412>
	<obo:IAO_0000115 xml:lang="en">COMMISSION REGULATION (EC) No 178/2006 of 1 February 2006 amending Regulation (EC) No 396/2005 of the European Parliament and of the Council.</obo:IAO_0000115>
	<obo:IAO_0000114 rdf:resource="&obo;IAO_0000428"/>
	<rdfs:comment xml:lang="en">LanguaL curation note: Includes meat, preparations of meat, offals, blood, animal fats; fresh, chilled or frozen, salted, in brine, dried or smoked or processed as flours or meals; other processed products such as sausages and food
preparations based on these.</rdfs:comment>
	<oboInOwl:hasDbXref>LANGUAL:A1258</oboInOwl:hasDbXref>
</owl:Class>

<owl:Class rdf:about="&obo;FOODON_03401259">
	<rdfs:label xml:lang="en">1020000 - milk and milk products (ec)</rdfs:label>
	<rdfs:subClassOf rdf:resource="&obo;FOODON_03401257"/>
	<obo:IAO_0000412>http://langual.org</obo:IAO_0000412>
	<obo:IAO_0000115 xml:lang="en">COMMISSION REGULATION (EC) No 178/2006 of 1 February 2006 amending Regulation (EC) No 396/2005 of the European Parliament and of the Council.</obo:IAO_0000115>
	<obo:IAO_0000114 rdf:resource="&obo;IAO_0000428"/>
	<rdfs:comment xml:lang="en">LanguaL curation note: Include milk and cream, not concentrated, nor containing added sugar or sweetening matter, butter and other fats derived from milk, cheese and curd.</rdfs:comment>
	<oboInOwl:hasDbXref>LANGUAL:A1259</oboInOwl:hasDbXref>
</owl:Class>

<owl:Class rdf:about="&obo;FOODON_03401260">
	<rdfs:label xml:lang="en">1030000 - birds eggs (ec)</rdfs:label>
	<rdfs:subClassOf rdf:resource="&obo;FOODON_03401257"/>
	<obo:IAO_0000412>http://langual.org</obo:IAO_0000412>
	<obo:IAO_0000115 xml:lang="en">COMMISSION REGULATION (EC) No 178/2006 of 1 February 2006 amending Regulation (EC) No 396/2005 of the European Parliament and of the Council.</obo:IAO_0000115>
	<obo:IAO_0000114 rdf:resource="&obo;IAO_0000428"/>
	<rdfs:comment xml:lang="en">LanguaL curation note: Include birds eggs, fresh preserved or cooked; shelled eggs and egg yolks fresh, dried, cooked by steaming or boiling in water, moulded, frozen or otherwise preserved whether or not containing added sugar or sweetening matter.</rdfs:comment>
	<oboInOwl:hasDbXref>LANGUAL:A1260</oboInOwl:hasDbXref>
</owl:Class>

<owl:Class rdf:about="&obo;FOODON_03401261">
	<rdfs:label xml:lang="en">1040000 - honey (ec)</rdfs:label>
	<rdfs:subClassOf rdf:resource="&obo;FOODON_03401257"/>
	<obo:IAO_0000412>http://langual.org</obo:IAO_0000412>
	<obo:IAO_0000115 xml:lang="en">COMMISSION REGULATION (EC) No 178/2006 of 1 February 2006 amending Regulation (EC) No 396/2005 of the European Parliament and of the Council.</obo:IAO_0000115>
	<obo:IAO_0000114 rdf:resource="&obo;IAO_0000428"/>
	<oboInOwl:hasDbXref>LANGUAL:A1261</oboInOwl:hasDbXref>
</owl:Class>

<owl:Class rdf:about="&obo;FOODON_03401262">
	<rdfs:label xml:lang="en">1050000 - amphibians and reptiles (ec)</rdfs:label>
	<rdfs:subClassOf rdf:resource="&obo;FOODON_03401257"/>
	<obo:IAO_0000412>http://langual.org</obo:IAO_0000412>
	<obo:IAO_0000115 xml:lang="en">COMMISSION REGULATION (EC) No 178/2006 of 1 February 2006 amending Regulation (EC) No 396/2005 of the European Parliament and of the Council.</obo:IAO_0000115>
	<obo:IAO_0000114 rdf:resource="&obo;IAO_0000428"/>
	<oboInOwl:hasDbXref>LANGUAL:A1262</oboInOwl:hasDbXref>
</owl:Class>

<owl:Class rdf:about="&obo;FOODON_03401263">
	<rdfs:label xml:lang="en">1060000 - snails (ec)</rdfs:label>
	<rdfs:subClassOf rdf:resource="&obo;FOODON_03401257"/>
	<obo:IAO_0000412>http://langual.org</obo:IAO_0000412>
	<obo:IAO_0000115 xml:lang="en">COMMISSION REGULATION (EC) No 178/2006 of 1 February 2006 amending Regulation (EC) No 396/2005 of the European Parliament and of the Council.</obo:IAO_0000115>
	<obo:IAO_0000114 rdf:resource="&obo;IAO_0000428"/>
	<oboInOwl:hasDbXref>LANGUAL:A1263</oboInOwl:hasDbXref>
</owl:Class>

<owl:Class rdf:about="&obo;FOODON_03401264">
	<rdfs:label xml:lang="en">1070000 - other terrestrial animal products (ec)</rdfs:label>
	<rdfs:subClassOf rdf:resource="&obo;FOODON_03401257"/>
	<obo:IAO_0000412>http://langual.org</obo:IAO_0000412>
	<obo:IAO_0000115 xml:lang="en">COMMISSION REGULATION (EC) No 178/2006 of 1 February 2006 amending Regulation (EC) No 396/2005 of the European Parliament and of the Council.</obo:IAO_0000115>
	<obo:IAO_0000114 rdf:resource="&obo;IAO_0000428"/>
	<oboInOwl:hasDbXref>LANGUAL:A1264</oboInOwl:hasDbXref>
</owl:Class>

<owl:Class rdf:about="&obo;FOODON_03401265">
	<rdfs:label xml:lang="en">1100000 - 11. fish, fish products, shell fish, molluscs and other marine and freshwater food products (ec)</rdfs:label>
	<rdfs:subClassOf rdf:resource="&obo;FOODON_03401220"/>
	<obo:IAO_0000412>http://langual.org</obo:IAO_0000412>
	<obo:IAO_0000115 xml:lang="en">COMMISSION REGULATION (EC) No 178/2006 of 1 February 2006 amending Regulation (EC) No 396/2005 of the European Parliament and of the Council.</obo:IAO_0000115>
	<obo:IAO_0000114 rdf:resource="&obo;IAO_0000428"/>
	<oboInOwl:hasDbXref>LANGUAL:A1265</oboInOwl:hasDbXref>
</owl:Class>

<owl:Class rdf:about="&obo;FOODON_03401266">
	<rdfs:label xml:lang="en">1200000 - crops exclusively for animal feed (ec)</rdfs:label>
	<rdfs:subClassOf rdf:resource="&obo;FOODON_03401220"/>
	<obo:IAO_0000412>http://langual.org</obo:IAO_0000412>
	<obo:IAO_0000115 xml:lang="en">COMMISSION REGULATION (EC) No 178/2006 of 1 February 2006 amending Regulation (EC) No 396/2005 of the European Parliament and of the Council.</obo:IAO_0000115>
	<obo:IAO_0000114 rdf:resource="&obo;IAO_0000428"/>
	<oboInOwl:hasDbXref>LANGUAL:A1266</oboInOwl:hasDbXref>
</owl:Class>

<owl:Class rdf:about="&obo;FOODON_03401267">
	<rdfs:label xml:lang="en">0160000 - miscellaneous fruit (ec)</rdfs:label>
	<rdfs:subClassOf rdf:resource="&obo;FOODON_03401221"/>
	<obo:IAO_0000412>http://langual.org</obo:IAO_0000412>
	<obo:IAO_0000115 xml:lang="en">COMMISSION REGULATION (EC) No 178/2006 of 1 February 2006 amending Regulation (EC) No 396/2005 of the European Parliament and of the Council.</obo:IAO_0000115>
	<obo:IAO_0000114 rdf:resource="&obo;IAO_0000428"/>
	<oboInOwl:hasDbXref>LANGUAL:A1267</oboInOwl:hasDbXref>
</owl:Class>

<owl:Class rdf:about="&obo;FOODON_03401268">
	<rdfs:label xml:lang="en">0290000 - sea weeds (ec)</rdfs:label>
	<rdfs:subClassOf rdf:resource="&obo;FOODON_03401227"/>
	<obo:IAO_0000412>http://langual.org</obo:IAO_0000412>
	<obo:IAO_0000115 xml:lang="en">COMMISSION REGULATION (EC) No 178/2006 of 1 February 2006 amending Regulation (EC) No 396/2005 of the European Parliament and of the Council.</obo:IAO_0000115>
	<obo:IAO_0000114 rdf:resource="&obo;IAO_0000428"/>
	<oboInOwl:hasDbXref>LANGUAL:A1268</oboInOwl:hasDbXref>
</owl:Class>

<owl:Class rdf:about="&obo;FOODON_03401269">
	<rdfs:label xml:lang="en">product type, usda standard reference</rdfs:label>
	<rdfs:subClassOf rdf:resource="&obo;FOODON_03400289"/>
	<obo:IAO_0000412>http://langual.org</obo:IAO_0000412>
	<obo:IAO_0000115 xml:lang="en">Food classification according to the USDA National Nutrient Database for Standard Reference.</obo:IAO_0000115>
	<obo:IAO_0000114 rdf:resource="&obo;IAO_0000428"/>
	<rdfs:comment xml:lang="en">LanguaL curation note: This term is for CLASSIFICATION ONLY; DO NOT USE term in indexing. Use a more precise narrower term.</rdfs:comment>
	<oboInOwl:hasDbXref>LANGUAL:A1269</oboInOwl:hasDbXref>
</owl:Class>

<owl:Class rdf:about="&obo;FOODON_03401270">
	<rdfs:label xml:lang="en">product type,  u.s. code of federal regulations, title 21</rdfs:label>
	<rdfs:subClassOf rdf:resource="&obo;FOODON_03400289"/>
	<obo:IAO_0000412>http://langual.org</obo:IAO_0000412>
	<obo:IAO_0000115 xml:lang="en">Food and Drugs, title 21, Code of Federal Regulations. Original  food classification in LanguaL.</obo:IAO_0000115>
	<obo:IAO_0000114 rdf:resource="&obo;IAO_0000428"/>
	<rdfs:comment xml:lang="en">LanguaL curation note: This term is for CLASSIFICATION ONLY; DO NOT USE term in indexing. Use a more precise narrower term.</rdfs:comment>
	<oboInOwl:hasDbXref>LANGUAL:A1270</oboInOwl:hasDbXref>
</owl:Class>

<owl:Class rdf:about="&obo;FOODON_03401271">
	<rdfs:label xml:lang="en">0100 dairy and egg products (usda sr)</rdfs:label>
	<rdfs:subClassOf rdf:resource="&obo;FOODON_03401269"/>
	<obo:IAO_0000412>http://langual.org</obo:IAO_0000412>
	<obo:IAO_0000114 rdf:resource="&obo;IAO_0000428"/>
	<oboInOwl:hasDbXref>LANGUAL:A1271</oboInOwl:hasDbXref>
</owl:Class>

<owl:Class rdf:about="&obo;FOODON_03401272">
	<rdfs:label xml:lang="en">0200 spices and herbs (usda sr)</rdfs:label>
	<rdfs:subClassOf rdf:resource="&obo;FOODON_03401269"/>
	<obo:IAO_0000412>http://langual.org</obo:IAO_0000412>
	<obo:IAO_0000114 rdf:resource="&obo;IAO_0000428"/>
	<oboInOwl:hasDbXref>LANGUAL:A1272</oboInOwl:hasDbXref>
</owl:Class>

<owl:Class rdf:about="&obo;FOODON_03401273">
	<rdfs:label xml:lang="en">0300 baby foods (usda sr)</rdfs:label>
	<rdfs:subClassOf rdf:resource="&obo;FOODON_03401269"/>
	<obo:IAO_0000412>http://langual.org</obo:IAO_0000412>
	<obo:IAO_0000114 rdf:resource="&obo;IAO_0000428"/>
	<oboInOwl:hasDbXref>LANGUAL:A1273</oboInOwl:hasDbXref>
</owl:Class>

<owl:Class rdf:about="&obo;FOODON_03401274">
	<rdfs:label xml:lang="en">0400 fats and oils (usda sr)</rdfs:label>
	<rdfs:subClassOf rdf:resource="&obo;FOODON_03401269"/>
	<obo:IAO_0000412>http://langual.org</obo:IAO_0000412>
	<obo:IAO_0000114 rdf:resource="&obo;IAO_0000428"/>
	<oboInOwl:hasDbXref>LANGUAL:A1274</oboInOwl:hasDbXref>
</owl:Class>

<owl:Class rdf:about="&obo;FOODON_03401275">
	<rdfs:label xml:lang="en">0500 poultry products (usda sr)</rdfs:label>
	<rdfs:subClassOf rdf:resource="&obo;FOODON_03401269"/>
	<obo:IAO_0000412>http://langual.org</obo:IAO_0000412>
	<obo:IAO_0000114 rdf:resource="&obo;IAO_0000428"/>
	<oboInOwl:hasDbXref>LANGUAL:A1275</oboInOwl:hasDbXref>
</owl:Class>

<owl:Class rdf:about="&obo;FOODON_03401276">
	<rdfs:label xml:lang="en">0600 soups, sauces, and gravies (usda sr)</rdfs:label>
	<rdfs:subClassOf rdf:resource="&obo;FOODON_03401269"/>
	<obo:IAO_0000412>http://langual.org</obo:IAO_0000412>
	<obo:IAO_0000114 rdf:resource="&obo;IAO_0000428"/>
	<oboInOwl:hasDbXref>LANGUAL:A1276</oboInOwl:hasDbXref>
</owl:Class>

<owl:Class rdf:about="&obo;FOODON_03401277">
	<rdfs:label xml:lang="en">0700 sausages and luncheon meats (usda sr)</rdfs:label>
	<rdfs:subClassOf rdf:resource="&obo;FOODON_03401269"/>
	<obo:IAO_0000412>http://langual.org</obo:IAO_0000412>
	<obo:IAO_0000114 rdf:resource="&obo;IAO_0000428"/>
	<oboInOwl:hasDbXref>LANGUAL:A1277</oboInOwl:hasDbXref>
</owl:Class>

<owl:Class rdf:about="&obo;FOODON_03401278">
	<rdfs:label xml:lang="en">0800 breakfast cereals (usda sr)</rdfs:label>
	<rdfs:subClassOf rdf:resource="&obo;FOODON_03401269"/>
	<obo:IAO_0000412>http://langual.org</obo:IAO_0000412>
	<obo:IAO_0000114 rdf:resource="&obo;IAO_0000428"/>
	<oboInOwl:hasDbXref>LANGUAL:A1278</oboInOwl:hasDbXref>
</owl:Class>

<owl:Class rdf:about="&obo;FOODON_03401279">
	<rdfs:label xml:lang="en">0900 fruits and fruit juices (usda sr)</rdfs:label>
	<rdfs:subClassOf rdf:resource="&obo;FOODON_03401269"/>
	<obo:IAO_0000412>http://langual.org</obo:IAO_0000412>
	<obo:IAO_0000114 rdf:resource="&obo;IAO_0000428"/>
	<oboInOwl:hasDbXref>LANGUAL:A1279</oboInOwl:hasDbXref>
</owl:Class>

<owl:Class rdf:about="&obo;FOODON_03401280">
	<rdfs:label xml:lang="en">1000 pork products (usda sr)</rdfs:label>
	<rdfs:subClassOf rdf:resource="&obo;FOODON_03401269"/>
	<obo:IAO_0000412>http://langual.org</obo:IAO_0000412>
	<obo:IAO_0000114 rdf:resource="&obo;IAO_0000428"/>
	<oboInOwl:hasDbXref>LANGUAL:A1280</oboInOwl:hasDbXref>
</owl:Class>

<owl:Class rdf:about="&obo;FOODON_03401281">
	<rdfs:label xml:lang="en">1100 vegetables and vegetable products (usda sr)</rdfs:label>
	<rdfs:subClassOf rdf:resource="&obo;FOODON_03401269"/>
	<obo:IAO_0000412>http://langual.org</obo:IAO_0000412>
	<obo:IAO_0000114 rdf:resource="&obo;IAO_0000428"/>
	<oboInOwl:hasDbXref>LANGUAL:A1281</oboInOwl:hasDbXref>
</owl:Class>

<owl:Class rdf:about="&obo;FOODON_03401282">
	<rdfs:label xml:lang="en">1200 nut and seed products (usda sr)</rdfs:label>
	<rdfs:subClassOf rdf:resource="&obo;FOODON_03401269"/>
	<obo:IAO_0000412>http://langual.org</obo:IAO_0000412>
	<obo:IAO_0000114 rdf:resource="&obo;IAO_0000428"/>
	<oboInOwl:hasDbXref>LANGUAL:A1282</oboInOwl:hasDbXref>
</owl:Class>

<owl:Class rdf:about="&obo;FOODON_03401283">
	<rdfs:label xml:lang="en">1300 beef products (usda sr)</rdfs:label>
	<rdfs:subClassOf rdf:resource="&obo;FOODON_03401269"/>
	<obo:IAO_0000412>http://langual.org</obo:IAO_0000412>
	<obo:IAO_0000114 rdf:resource="&obo;IAO_0000428"/>
	<oboInOwl:hasDbXref>LANGUAL:A1283</oboInOwl:hasDbXref>
</owl:Class>

<owl:Class rdf:about="&obo;FOODON_03401284">
	<rdfs:label xml:lang="en">1400 beverages (usda sr)</rdfs:label>
	<rdfs:subClassOf rdf:resource="&obo;FOODON_03401269"/>
	<obo:IAO_0000412>http://langual.org</obo:IAO_0000412>
	<obo:IAO_0000114 rdf:resource="&obo;IAO_0000428"/>
	<oboInOwl:hasDbXref>LANGUAL:A1284</oboInOwl:hasDbXref>
</owl:Class>

<owl:Class rdf:about="&obo;FOODON_03401285">
	<rdfs:label xml:lang="en">1500 finfish and shellfish products (usda sr)</rdfs:label>
	<rdfs:subClassOf rdf:resource="&obo;FOODON_03401269"/>
	<obo:IAO_0000412>http://langual.org</obo:IAO_0000412>
	<obo:IAO_0000114 rdf:resource="&obo;IAO_0000428"/>
	<oboInOwl:hasDbXref>LANGUAL:A1285</oboInOwl:hasDbXref>
</owl:Class>

<owl:Class rdf:about="&obo;FOODON_03401286">
	<rdfs:label xml:lang="en">1600 legumes and legume products (usda sr)</rdfs:label>
	<rdfs:subClassOf rdf:resource="&obo;FOODON_03401269"/>
	<obo:IAO_0000412>http://langual.org</obo:IAO_0000412>
	<obo:IAO_0000114 rdf:resource="&obo;IAO_0000428"/>
	<oboInOwl:hasDbXref>LANGUAL:A1286</oboInOwl:hasDbXref>
</owl:Class>

<owl:Class rdf:about="&obo;FOODON_03401287">
	<rdfs:label xml:lang="en">1700 lamb, veal, and game products (usda sr)</rdfs:label>
	<rdfs:subClassOf rdf:resource="&obo;FOODON_03401269"/>
	<obo:IAO_0000412>http://langual.org</obo:IAO_0000412>
	<obo:IAO_0000114 rdf:resource="&obo;IAO_0000428"/>
	<oboInOwl:hasDbXref>LANGUAL:A1287</oboInOwl:hasDbXref>
</owl:Class>

<owl:Class rdf:about="&obo;FOODON_03401288">
	<rdfs:label xml:lang="en">1800 baked products (usda sr)</rdfs:label>
	<rdfs:subClassOf rdf:resource="&obo;FOODON_03401269"/>
	<obo:IAO_0000412>http://langual.org</obo:IAO_0000412>
	<obo:IAO_0000114 rdf:resource="&obo;IAO_0000428"/>
	<oboInOwl:hasDbXref>LANGUAL:A1288</oboInOwl:hasDbXref>
</owl:Class>

<owl:Class rdf:about="&obo;FOODON_03401289">
	<rdfs:label xml:lang="en">1900 sweets (usda sr)</rdfs:label>
	<rdfs:subClassOf rdf:resource="&obo;FOODON_03401269"/>
	<obo:IAO_0000412>http://langual.org</obo:IAO_0000412>
	<obo:IAO_0000114 rdf:resource="&obo;IAO_0000428"/>
	<oboInOwl:hasDbXref>LANGUAL:A1289</oboInOwl:hasDbXref>
</owl:Class>

<owl:Class rdf:about="&obo;FOODON_03401290">
	<rdfs:label xml:lang="en">2000 cereal grains and pasta (usda sr)</rdfs:label>
	<rdfs:subClassOf rdf:resource="&obo;FOODON_03401269"/>
	<obo:IAO_0000412>http://langual.org</obo:IAO_0000412>
	<obo:IAO_0000114 rdf:resource="&obo;IAO_0000428"/>
	<oboInOwl:hasDbXref>LANGUAL:A1290</oboInOwl:hasDbXref>
</owl:Class>

<owl:Class rdf:about="&obo;FOODON_03401291">
	<rdfs:label xml:lang="en">2100 fast foods (usda sr)</rdfs:label>
	<rdfs:subClassOf rdf:resource="&obo;FOODON_03401269"/>
	<obo:IAO_0000412>http://langual.org</obo:IAO_0000412>
	<obo:IAO_0000114 rdf:resource="&obo;IAO_0000428"/>
	<oboInOwl:hasDbXref>LANGUAL:A1291</oboInOwl:hasDbXref>
</owl:Class>

<owl:Class rdf:about="&obo;FOODON_03401292">
	<rdfs:label xml:lang="en">2200 meals, entrees, and sidedishes (usda sr)</rdfs:label>
	<rdfs:subClassOf rdf:resource="&obo;FOODON_03401269"/>
	<obo:IAO_0000412>http://langual.org</obo:IAO_0000412>
	<obo:IAO_0000114 rdf:resource="&obo;IAO_0000428"/>
	<oboInOwl:hasDbXref>LANGUAL:A1292</oboInOwl:hasDbXref>
</owl:Class>

<owl:Class rdf:about="&obo;FOODON_03401293">
	<rdfs:label xml:lang="en">2500 snacks (usda sr)</rdfs:label>
	<rdfs:subClassOf rdf:resource="&obo;FOODON_03401269"/>
	<obo:IAO_0000412>http://langual.org</obo:IAO_0000412>
	<obo:IAO_0000114 rdf:resource="&obo;IAO_0000428"/>
	<oboInOwl:hasDbXref>LANGUAL:A1293</oboInOwl:hasDbXref>
</owl:Class>

<owl:Class rdf:about="&obo;FOODON_03401294">
	<rdfs:label xml:lang="en">3500 ethnic foods (usda sr)</rdfs:label>
	<rdfs:subClassOf rdf:resource="&obo;FOODON_03401269"/>
	<obo:IAO_0000412>http://langual.org</obo:IAO_0000412>
	<obo:IAO_0000114 rdf:resource="&obo;IAO_0000428"/>
	<oboInOwl:hasDbXref>LANGUAL:A1294</oboInOwl:hasDbXref>
</owl:Class>

<owl:Class rdf:about="&obo;FOODON_03401295">
	<rdfs:label xml:lang="en">3600 restaurant foods (usda sr)</rdfs:label>
	<rdfs:subClassOf rdf:resource="&obo;FOODON_03401269"/>
	<obo:IAO_0000412>http://langual.org</obo:IAO_0000412>
	<obo:IAO_0000114 rdf:resource="&obo;IAO_0000428"/>
	<oboInOwl:hasDbXref>LANGUAL:A1295</oboInOwl:hasDbXref>
</owl:Class>

<owl:Class rdf:about="&obo;FOODON_03401296">
	<rdfs:label xml:lang="en">pie, unsweetened, or pizza (eurofir)</rdfs:label>
	<rdfs:subClassOf rdf:resource="&obo;FOODON_03400822"/>
	<obo:IAO_0000412>http://langual.org</obo:IAO_0000412>
	<obo:IAO_0000114 rdf:resource="&obo;IAO_0000428"/>
	<rdfs:comment xml:lang="en">LanguaL curation note: Used only for unsweetened products; sweetened pies are indexed under * FINE BAKERY WARE (EUROFIR) [A0821]*. Pizza crust should be indexed as *UNLEAVENED BREAD (EUROFIR)* [A0819]</rdfs:comment>
	<oboInOwl:hasSynonym xml:lang="en">pizza</oboInOwl:hasSynonym>
	<oboInOwl:hasSynonym xml:lang="en">unsweetened pie</oboInOwl:hasSynonym>
	<oboInOwl:hasDbXref>LANGUAL:A1296</oboInOwl:hasDbXref>
</owl:Class>

<owl:Class rdf:about="&obo;FOODON_03401297">
	<rdfs:label xml:lang="en">pancake or waffle (eurofir)</rdfs:label>
	<rdfs:subClassOf rdf:resource="&obo;FOODON_03400821"/>
	<obo:IAO_0000412>http://langual.org</obo:IAO_0000412>
	<obo:IAO_0000115 xml:lang="en">A thin, bakery product griddled or cooked in a heated mould.</obo:IAO_0000115>
	<obo:IAO_0000114 rdf:resource="&obo;IAO_0000428"/>
	<rdfs:comment xml:lang="en">LanguaL curation note: If sweetened, index also * SUGAR OR SUGAR SYRUP ADDED* [H0136] or narrower term.  If filled, use * PREPARED FOOD PRODUCT (EUROFIR)* [A0861] or narrower term.</rdfs:comment>
	<oboInOwl:hasDbXref>LANGUAL:A1297</oboInOwl:hasDbXref>
</owl:Class>

<owl:Class rdf:about="&obo;FOODON_03401298">
	<rdfs:label xml:lang="en">dietary supplement</rdfs:label>
	<rdfs:subClassOf rdf:resource="&obo;FOODON_03400361"/>
	<obo:IAO_0000412>http://langual.org</obo:IAO_0000412>
	<obo:IAO_0000115 xml:lang="en">Index dietary/food supplements according to legal and market definitions.

The United States defines dietary supplements in the Dietary Supplement Health and Education Act of 1994 (DSHEA). Pub L 103-417, 108 STAT. 4235, (Oct. 25, 1994): A dietary supplement is a product taken by mouth that contains a "dietary ingredient" intended to supplement the diet. The "dietary ingredients" in these products may include: vitamins, minerals, herbs or other botanicals, amino acids, and substances such as enzymes, organ tissues, glandulars, and metabolites. Dietary supplements can also be extracts or concentrates, and may be found in many forms such as tablets, capsules, softgels, gelcaps, liquids, or powders.

In the European Union, food supplements are framed by two kinds of regulations: 
- the EU vertical regulation relating to food supplements, composed with the directive 2002/46/CE  (essentially for the definition of food supplements) and the regulation 1170/2009 (which lists the vitamins and minerals, and the chemical forms of the substances allowed in food supplements); 
- the EU transversal regulation relating to foodstuffs and especially the 2006/1924 regulation concerning nutrition and health claims, and the EU labeling transversal regulations, 90/496/EC and 2008/100/EC.
The EU regulation 2002/46/CE defines food supplements as "foodstuffs the purpose of which is to supplement the normal diet and which are concentrated sources of nutrients or other substances with a nutritional or physiological effect, alone or in combination, marketed in dose form, namely forms such as capsules, pastilles, tablets, pills and other similar forms, sachets of powder, ampoules of liquids, drop dispensing bottles, and other similar forms of liquids and powders designed to be taken in measured small unit quantities". [Directive 2002/46/EC]

Codex Alimentarius also includes supplements containing vitamins or dietary minerals [http://www.codexalimentarius.net/download/standards/10206/cxg_055e.pdf]</obo:IAO_0000115>
	<obo:IAO_0000114 rdf:resource="&obo;IAO_0000428"/>
	<rdfs:comment xml:lang="en">LanguaL curation note: This term is for CLASSIFICATION ONLY; DO NOT USE term in indexing. Use a more precise narrower term.</rdfs:comment>
	<oboInOwl:hasSynonym xml:lang="en">food supplement</oboInOwl:hasSynonym>
	<oboInOwl:hasSynonym xml:lang="en">nutritional supplement</oboInOwl:hasSynonym>
	<oboInOwl:hasDbXref>LANGUAL:A1298</oboInOwl:hasDbXref>
</owl:Class>

<owl:Class rdf:about="&obo;FOODON_03401299">
	<rdfs:label xml:lang="en">dietary supplement, mineral</rdfs:label>
	<rdfs:subClassOf rdf:resource="&obo;FOODON_03401298"/>
	<obo:IAO_0000412>http://langual.org</obo:IAO_0000412>
	<obo:IAO_0000114 rdf:resource="&obo;IAO_0000428"/>
	<oboInOwl:hasSynonym xml:lang="en">mineral supplement</oboInOwl:hasSynonym>
	<oboInOwl:hasDbXref>LANGUAL:A1299</oboInOwl:hasDbXref>
</owl:Class>

<owl:Class rdf:about="&obo;FOODON_03401300">
	<rdfs:label xml:lang="en">multi-mineral supplement</rdfs:label>
	<rdfs:subClassOf rdf:resource="&obo;FOODON_03401299"/>
	<obo:IAO_0000412>http://langual.org</obo:IAO_0000412>
	<obo:IAO_0000115 xml:lang="en">A multi-mineral supplement contains more than one mineral, e.g. calcium-magnesium supplement.</obo:IAO_0000115>
	<obo:IAO_0000114 rdf:resource="&obo;IAO_0000428"/>
	<rdfs:comment xml:lang="en">LanguaL curation note: Currently not used in US classification of dietary supplements.</rdfs:comment>
	<oboInOwl:hasDbXref>LANGUAL:A1300</oboInOwl:hasDbXref>
</owl:Class>

<owl:Class rdf:about="&obo;FOODON_03401301">
	<rdfs:label xml:lang="en">single mineral supplement</rdfs:label>
	<rdfs:subClassOf rdf:resource="&obo;FOODON_03401299"/>
	<obo:IAO_0000412>http://langual.org</obo:IAO_0000412>
	<obo:IAO_0000115 xml:lang="en">A single mineral supplement is defined as containing one mineral, e.g. calcium supplement.</obo:IAO_0000115>
	<obo:IAO_0000114 rdf:resource="&obo;IAO_0000428"/>
	<rdfs:comment xml:lang="en">LanguaL curation note: Currently not used in US classification of dietary supplements.</rdfs:comment>
	<oboInOwl:hasDbXref>LANGUAL:A1301</oboInOwl:hasDbXref>
</owl:Class>

<owl:Class rdf:about="&obo;FOODON_03401302">
	<rdfs:label xml:lang="en">dietary supplement, vitamin</rdfs:label>
	<rdfs:subClassOf rdf:resource="&obo;FOODON_03401298"/>
	<obo:IAO_0000412>http://langual.org</obo:IAO_0000412>
	<obo:IAO_0000114 rdf:resource="&obo;IAO_0000428"/>
	<oboInOwl:hasSynonym xml:lang="en">vitamin supplement</oboInOwl:hasSynonym>
	<oboInOwl:hasDbXref>LANGUAL:A1302</oboInOwl:hasDbXref>
</owl:Class>

<owl:Class rdf:about="&obo;FOODON_03401303">
	<rdfs:label xml:lang="en">multi-vitamin supplement</rdfs:label>
	<rdfs:subClassOf rdf:resource="&obo;FOODON_03401302"/>
	<obo:IAO_0000412>http://langual.org</obo:IAO_0000412>
	<obo:IAO_0000115 xml:lang="en">A multi-vitamin supplement contains more than one vitamin, e.g. vitamin B complex supplement.</obo:IAO_0000115>
	<obo:IAO_0000114 rdf:resource="&obo;IAO_0000428"/>
	<rdfs:comment xml:lang="en">LanguaL curation note: Currently not used in US classification of dietary supplements.</rdfs:comment>
	<oboInOwl:hasDbXref>LANGUAL:A1303</oboInOwl:hasDbXref>
</owl:Class>

<owl:Class rdf:about="&obo;FOODON_03401304">
	<rdfs:label xml:lang="en">single vitamin supplement</rdfs:label>
	<rdfs:subClassOf rdf:resource="&obo;FOODON_03401302"/>
	<obo:IAO_0000412>http://langual.org</obo:IAO_0000412>
	<obo:IAO_0000115 xml:lang="en">A single vitamin supplement is defined as containing one vitamin, e.g. vitamin C supplement.</obo:IAO_0000115>
	<obo:IAO_0000114 rdf:resource="&obo;IAO_0000428"/>
	<rdfs:comment xml:lang="en">LanguaL curation note: Currently not used in US classification of dietary supplements.</rdfs:comment>
	<oboInOwl:hasDbXref>LANGUAL:A1304</oboInOwl:hasDbXref>
</owl:Class>

<owl:Class rdf:about="&obo;FOODON_03401305">
	<rdfs:label xml:lang="en">dietary supplement, amino acid or protein</rdfs:label>
	<rdfs:subClassOf rdf:resource="&obo;FOODON_03401298"/>
	<obo:IAO_0000412>http://langual.org</obo:IAO_0000412>
	<obo:IAO_0000114 rdf:resource="&obo;IAO_0000428"/>
	<oboInOwl:hasSynonym xml:lang="en">protein supplement</oboInOwl:hasSynonym>
	<oboInOwl:hasDbXref>LANGUAL:A1305</oboInOwl:hasDbXref>
</owl:Class>

<owl:Class rdf:about="&obo;FOODON_03401306">
	<rdfs:label xml:lang="en">dietary supplement, herbal or botanical</rdfs:label>
	<rdfs:subClassOf rdf:resource="&obo;FOODON_03401298"/>
	<obo:IAO_0000412>http://langual.org</obo:IAO_0000412>
	<obo:IAO_0000115 xml:lang="en">Yeast, algae, or fungus based dietary supplement.</obo:IAO_0000115>
	<obo:IAO_0000114 rdf:resource="&obo;IAO_0000428"/>
	<rdfs:comment xml:lang="en">LanguaL curation note: Use for supplements based on plants, yeast, algae, and fungi (index in facet B).
If the supplement also contains vitamins or minerals use the appropriate descriptor under * DIETARY SUPPLEMENT, COMBINATION*.</rdfs:comment>
	<oboInOwl:hasDbXref>LANGUAL:A1306</oboInOwl:hasDbXref>
</owl:Class>

<owl:Class rdf:about="&obo;FOODON_03401307">
	<rdfs:label xml:lang="en">yeast supplement</rdfs:label>
	<rdfs:subClassOf rdf:resource="&obo;FOODON_03401306"/>
	<obo:IAO_0000412>http://langual.org</obo:IAO_0000412>
	<obo:IAO_0000115 xml:lang="en">Nutritional yeast is a source of protein and vitamins, especially the B-complex vitamins and is a complete protein. [http://en.wikipedia.org/wiki/Nutritional_yeast]</obo:IAO_0000115>
	<obo:IAO_0000119>WIKIPEDIA:Nutritional_yeast</obo:IAO_0000119>
	<obo:IAO_0000114 rdf:resource="&obo;IAO_0000428"/>
	<rdfs:comment xml:lang="en">LanguaL curation note: Currently not used in US classification of dietary supplements.</rdfs:comment>
	<oboInOwl:hasDbXref>LANGUAL:A1307</oboInOwl:hasDbXref>
</owl:Class>

<owl:Class rdf:about="&obo;FOODON_03401308">
	<rdfs:label xml:lang="en">probiotic or bacteria supplement</rdfs:label>
	<rdfs:subClassOf rdf:resource="&obo;FOODON_03401309"/>
	<obo:IAO_0000412>http://langual.org</obo:IAO_0000412>
	<obo:IAO_0000115 xml:lang="en">Probiotics are live microorganisms thought to be healthy for the host organism. According to the currently adopted definition by FAO/WHO, probiotics are selected "live microorganisms which when administered in adequate amounts confer a health benefit on the host".[FAO/WHO (2001) Health and Nutritional Properties of Probiotics in Food including Powder Milk with Live Lactic Acid Bacteria. Report of a Joint FAO/WHO Expert Consultation on Evaluation of Health and Nutritional Properties of Probiotics in Food Including Powder Milk with Live Lactic Acid Bacteria]  
Lactic acid bacteria (LAB) and bifidobacteria are the most common types of microbes used as probiotics; but also certain yeasts and bacilli are available. [http://en.wikipedia.org/wiki/Probiotics]</obo:IAO_0000115>
	<obo:IAO_0000119>WIKIPEDIA:Probiotics</obo:IAO_0000119>
	<obo:IAO_0000114 rdf:resource="&obo;IAO_0000428"/>
	<rdfs:comment xml:lang="en">LanguaL curation note: Currently not used in US classification of dietary supplements.</rdfs:comment>
	<oboInOwl:hasDbXref>LANGUAL:A1308</oboInOwl:hasDbXref>
</owl:Class>

<owl:Class rdf:about="&obo;FOODON_03401309">
	<rdfs:label xml:lang="en">dietary supplement, non-nutrient/non-botanical supplement</rdfs:label>
	<rdfs:subClassOf rdf:resource="&obo;FOODON_03401298"/>
	<obo:IAO_0000412>http://langual.org</obo:IAO_0000412>
	<obo:IAO_0000115 xml:lang="en">Includes hormone precursors; steroid precursors; 7-dehydrocholesterol, lutein, omega-3's, CoQ10</obo:IAO_0000115>
	<obo:IAO_0000114 rdf:resource="&obo;IAO_0000428"/>
	<oboInOwl:hasDbXref>LANGUAL:A1309</oboInOwl:hasDbXref>
</owl:Class>

<owl:Class rdf:about="&obo;FOODON_03401310">
	<rdfs:label xml:lang="en">fatty acid or fat/oil supplement</rdfs:label>
	<rdfs:subClassOf rdf:resource="&obo;FOODON_03401326"/>
	<obo:IAO_0000412>http://langual.org</obo:IAO_0000412>
	<obo:IAO_0000115 xml:lang="en">Includes omega-3 supplements, fish oil capsules, evening primrose capsules.</obo:IAO_0000115>
	<obo:IAO_0000114 rdf:resource="&obo;IAO_0000428"/>
	<rdfs:comment xml:lang="en">LanguaL curation note: Currently not used in US classification of dietary supplements.</rdfs:comment>
	<oboInOwl:hasDbXref>LANGUAL:A1310</oboInOwl:hasDbXref>
</owl:Class>

<owl:Class rdf:about="&obo;FOODON_03401311">
	<rdfs:label xml:lang="en">enzyme supplement</rdfs:label>
	<rdfs:subClassOf rdf:resource="&obo;FOODON_03401309"/>
	<obo:IAO_0000412>http://langual.org</obo:IAO_0000412>
	<obo:IAO_0000115 xml:lang="en">Plant and animal enzymes are used to facilitate the digestive process and improve the body's ability to maintain balanced metabolism. Enzyme supplements are extracted from plants like pineapple and papaya and from the organs of cows and pigs. The supplements are typically given in tablet or capsule form. Pancreatic enzymes may also be given by injection. The dosage varies with the condition being treated. For nondigestive ailments, the supplements are taken in the hour before meals so that they can be quickly absorbed into the blood. For digestive ailments, the supplements are taken immediately before meals accompanied by a large glass of fluids. Pancreatic enzymes may be accompanied by doses of vitamin A.[http://medical-dictionary.thefreedictionary.com/enzyme+therapy]</obo:IAO_0000115>
	<obo:IAO_0000114 rdf:resource="&obo;IAO_0000428"/>
	<rdfs:comment xml:lang="en">LanguaL curation note: Currently not used in US classification of dietary supplements.</rdfs:comment>
	<oboInOwl:hasDbXref>LANGUAL:A1311</oboInOwl:hasDbXref>
</owl:Class>

<owl:Class rdf:about="&obo;FOODON_03401312">
	<rdfs:label xml:lang="en">phytoestrogen supplement</rdfs:label>
	<rdfs:subClassOf rdf:resource="&obo;FOODON_03401309"/>
	<obo:IAO_0000412>http://langual.org</obo:IAO_0000412>
	<obo:IAO_0000115 xml:lang="en">Phytoestrogens are weak estrogens found concentrated in soybeans. Extracted phytoestrogens are marketed in numerous forms as dietary supplements. Consumers of phytoestrogen supplements tend to be peri- and postmenopausal women looking for an alternative to hormone therapy.</obo:IAO_0000115>
	<obo:IAO_0000114 rdf:resource="&obo;IAO_0000428"/>
	<rdfs:comment xml:lang="en">LanguaL curation note: Currently not used in US classification of dietary supplements.</rdfs:comment>
	<oboInOwl:hasDbXref>LANGUAL:A1312</oboInOwl:hasDbXref>
</owl:Class>

<owl:Class rdf:about="&obo;FOODON_03401313">
	<rdfs:label xml:lang="en">dietary supplement, combination</rdfs:label>
	<rdfs:subClassOf rdf:resource="&obo;FOODON_03401298"/>
	<obo:IAO_0000412>http://langual.org</obo:IAO_0000412>
	<obo:IAO_0000114 rdf:resource="&obo;IAO_0000428"/>
	<rdfs:comment xml:lang="en">LanguaL curation note: Use to index a dietary supplement that is a combination of any of the other supplement types. Whenever possible, use a more precise narrower term.</rdfs:comment>
	<oboInOwl:hasDbXref>LANGUAL:A1313</oboInOwl:hasDbXref>
</owl:Class>

<owl:Class rdf:about="&obo;FOODON_03401314">
	<rdfs:label xml:lang="en">dietary supplement, multi-vitamin/mineral</rdfs:label>
	<rdfs:subClassOf rdf:resource="&obo;FOODON_03401313"/>
	<obo:IAO_0000412>http://langual.org</obo:IAO_0000412>
	<obo:IAO_0000115 xml:lang="en">A multivitamin/mineral supplement is defined in the United States as a supplement containing 3 or more vitamins and minerals but does not include herbs, hormones, or drugs, with each nutrient at a dose below the tolerable upper level determined by the Food and Drug Board and the maximum daily intake to not cause a risk for adverse health effects. (National Institutes of Health State-of-the-Science Panel. National Institutes of Health State-of-the-Science Conference Statement: multivitamin/mineral supplements and chronic disease prevention. Am J Clin Nutr 2007;85:257S-64S) [http://en.wikipedia.org/wiki/Multivitamin]

In Europe, a supplement containing 2 or more vitamins and minerals is defined as vitamin-mineral combination supplement.</obo:IAO_0000115>
	<obo:IAO_0000119>WIKIPEDIA:Multivitamin</obo:IAO_0000119>
	<obo:IAO_0000114 rdf:resource="&obo;IAO_0000428"/>
	<oboInOwl:hasDbXref>LANGUAL:A1314</oboInOwl:hasDbXref>
</owl:Class>

<owl:Class rdf:about="&obo;FOODON_03401315">
	<rdfs:label xml:lang="en">multi-vitamin and multi-mineral supplement</rdfs:label>
	<rdfs:subClassOf rdf:resource="&obo;FOODON_03401314"/>
	<obo:IAO_0000412>http://langual.org</obo:IAO_0000412>
	<obo:IAO_0000115 xml:lang="en">Defined as containing several vitamins and several minerals.</obo:IAO_0000115>
	<obo:IAO_0000114 rdf:resource="&obo;IAO_0000428"/>
	<rdfs:comment xml:lang="en">LanguaL curation note: Currently not used in US classification of dietary supplements.</rdfs:comment>
	<oboInOwl:hasDbXref>LANGUAL:A1315</oboInOwl:hasDbXref>
</owl:Class>

<owl:Class rdf:about="&obo;FOODON_03401316">
	<rdfs:label xml:lang="en">single vitamin and single mineral supplement</rdfs:label>
	<rdfs:subClassOf rdf:resource="&obo;FOODON_03401314"/>
	<obo:IAO_0000412>http://langual.org</obo:IAO_0000412>
	<obo:IAO_0000115 xml:lang="en">Defined as containing one vitamin and one mineral.</obo:IAO_0000115>
	<obo:IAO_0000114 rdf:resource="&obo;IAO_0000428"/>
	<rdfs:comment xml:lang="en">LanguaL curation note: Currently not used in US classification of dietary supplements.</rdfs:comment>
	<oboInOwl:hasDbXref>LANGUAL:A1316</oboInOwl:hasDbXref>
</owl:Class>

<owl:Class rdf:about="&obo;FOODON_03401317">
	<rdfs:label xml:lang="en">botanical supplement with vitamin/mineral</rdfs:label>
	<rdfs:subClassOf rdf:resource="&obo;FOODON_03401313"/>
	<obo:IAO_0000412>http://langual.org</obo:IAO_0000412>
	<obo:IAO_0000115 xml:lang="en">Botanical dietary supplement with mineral(s) and/or vitamin(s).</obo:IAO_0000115>
	<obo:IAO_0000114 rdf:resource="&obo;IAO_0000428"/>
	<rdfs:comment xml:lang="en">LanguaL curation note: For US supplement classification, use narrower term.</rdfs:comment>
	<oboInOwl:hasDbXref>LANGUAL:A1317</oboInOwl:hasDbXref>
</owl:Class>

<owl:Class rdf:about="&obo;FOODON_03401318">
	<rdfs:label xml:lang="en">botanical supplement with mineral(s)</rdfs:label>
	<rdfs:subClassOf rdf:resource="&obo;FOODON_03401317"/>
	<obo:IAO_0000412>http://langual.org</obo:IAO_0000412>
	<obo:IAO_0000114 rdf:resource="&obo;IAO_0000428"/>
	<oboInOwl:hasDbXref>LANGUAL:A1318</oboInOwl:hasDbXref>
</owl:Class>

<owl:Class rdf:about="&obo;FOODON_03401319">
	<rdfs:label xml:lang="en">botanical supplement with multi-vitamin/mineral</rdfs:label>
	<rdfs:subClassOf rdf:resource="&obo;FOODON_03401317"/>
	<obo:IAO_0000412>http://langual.org</obo:IAO_0000412>
	<obo:IAO_0000114 rdf:resource="&obo;IAO_0000428"/>
	<oboInOwl:hasDbXref>LANGUAL:A1319</oboInOwl:hasDbXref>
</owl:Class>

<owl:Class rdf:about="&obo;FOODON_03401320">
	<rdfs:label xml:lang="en">botanical supplement with vitamin(s)</rdfs:label>
	<rdfs:subClassOf rdf:resource="&obo;FOODON_03401317"/>
	<obo:IAO_0000412>http://langual.org</obo:IAO_0000412>
	<obo:IAO_0000114 rdf:resource="&obo;IAO_0000428"/>
	<oboInOwl:hasDbXref>LANGUAL:A1320</oboInOwl:hasDbXref>
</owl:Class>

<owl:Class rdf:about="&obo;FOODON_03401321">
	<rdfs:label xml:lang="en">dietary supplement, multi-vitamin/mineral and amino acids</rdfs:label>
	<rdfs:subClassOf rdf:resource="&obo;FOODON_03401313"/>
	<obo:IAO_0000412>http://langual.org</obo:IAO_0000412>
	<obo:IAO_0000114 rdf:resource="&obo;IAO_0000428"/>
	<oboInOwl:hasDbXref>LANGUAL:A1321</oboInOwl:hasDbXref>
</owl:Class>

<owl:Class rdf:about="&obo;FOODON_03401322">
	<rdfs:label xml:lang="en">single vitamin and multi-mineral supplement</rdfs:label>
	<rdfs:subClassOf rdf:resource="&obo;FOODON_03401314"/>
	<obo:IAO_0000412>http://langual.org</obo:IAO_0000412>
	<obo:IAO_0000115 xml:lang="en">Defined as containing one vitamin and several minerals.</obo:IAO_0000115>
	<obo:IAO_0000114 rdf:resource="&obo;IAO_0000428"/>
	<rdfs:comment xml:lang="en">LanguaL curation note: Currently not used in US classification of dietary supplements.</rdfs:comment>
	<oboInOwl:hasDbXref>LANGUAL:A1322</oboInOwl:hasDbXref>
</owl:Class>

<owl:Class rdf:about="&obo;FOODON_03401323">
	<rdfs:label xml:lang="en">multi-vitamin and single mineral supplement</rdfs:label>
	<rdfs:subClassOf rdf:resource="&obo;FOODON_03401314"/>
	<obo:IAO_0000412>http://langual.org</obo:IAO_0000412>
	<obo:IAO_0000115 xml:lang="en">Defined as containing several vitamins and one mineral.</obo:IAO_0000115>
	<obo:IAO_0000114 rdf:resource="&obo;IAO_0000428"/>
	<rdfs:comment xml:lang="en">LanguaL curation note: Currently not used in US classification of dietary supplements.</rdfs:comment>
	<oboInOwl:hasDbXref>LANGUAL:A1323</oboInOwl:hasDbXref>
</owl:Class>

<owl:Class rdf:about="&obo;FOODON_03401324">
	<rdfs:label xml:lang="en">dietary supplement, vitamin(s) and fatty acids</rdfs:label>
	<rdfs:subClassOf rdf:resource="&obo;FOODON_03401313"/>
	<obo:IAO_0000412>http://langual.org</obo:IAO_0000412>
	<obo:IAO_0000114 rdf:resource="&obo;IAO_0000428"/>
	<oboInOwl:hasDbXref>LANGUAL:A1324</oboInOwl:hasDbXref>
</owl:Class>

<owl:Class rdf:about="&obo;FOODON_03401325">
	<rdfs:label xml:lang="en">dietary supplement, combination, other</rdfs:label>
	<rdfs:subClassOf rdf:resource="&obo;FOODON_03401313"/>
	<obo:IAO_0000412>http://langual.org</obo:IAO_0000412>
	<owl:deprecated rdf:datatype="&xsd;boolean">true</owl:deprecated>
	<obo:IAO_0000114 rdf:resource="&obo;IAO_0000122"/>
	<oboInOwl:hasDbXref>LANGUAL:A1325</oboInOwl:hasDbXref>
</owl:Class>

<owl:Class rdf:about="&obo;FOODON_03401326">
	<rdfs:label xml:lang="en">dietary supplement, other nutritive supplement</rdfs:label>
	<rdfs:subClassOf rdf:resource="&obo;FOODON_03401298"/>
	<obo:IAO_0000412>http://langual.org</obo:IAO_0000412>
	<obo:IAO_0000115 xml:lang="en">Includes other dietary substance to supplement the diet (fiber, electrolytes).</obo:IAO_0000115>
	<obo:IAO_0000114 rdf:resource="&obo;IAO_0000428"/>
	<rdfs:comment xml:lang="en">LanguaL curation note: Use only if needed to index other combination dietary supplements.</rdfs:comment>
	<oboInOwl:hasDbXref>LANGUAL:A1326</oboInOwl:hasDbXref>
</owl:Class>

<owl:Class rdf:about="&obo;FOODON_03401327">
	<rdfs:label xml:lang="en">dietary supplement, electrolyte</rdfs:label>
	<rdfs:subClassOf rdf:resource="&obo;FOODON_03401326"/>
	<obo:IAO_0000412>http://langual.org</obo:IAO_0000412>
	<obo:IAO_0000115 xml:lang="en">Electrolyte supplements are a varied group of prescription and nonprescription preparations used to correct imbalances in the body's electrolyte levels. Electrolyte supplements are intended to prevent or treat electrolyte imbalances in very different situations or groups of patients. They range from sports drinks and other supplements used by amateur or professional athletes to prevent muscle cramps and improve athletic performance, to liquids used at home to prevent dehydration in children with diarrhea, to injections administered as part of enteral (feeding through a tube or stoma directly into the small intestine) or parenteral nutrition (intravenous feeding that bypasses the digestive tract). [http://medical-dictionary.thefreedictionary.com/Electrolyte+Supplements]</obo:IAO_0000115>
	<obo:IAO_0000114 rdf:resource="&obo;IAO_0000428"/>
	<oboInOwl:hasDbXref>LANGUAL:A1327</oboInOwl:hasDbXref>
</owl:Class>

<owl:Class rdf:about="&obo;FOODON_03401328">
	<rdfs:label xml:lang="en">dietary supplement, fibre</rdfs:label>
	<rdfs:subClassOf rdf:resource="&obo;FOODON_03401326"/>
	<obo:IAO_0000412>http://langual.org</obo:IAO_0000412>
	<obo:IAO_0000115 xml:lang="en">Fibre supplements (or fiber supplements) are considered to be a form of a subgroup of functional dietary fibre, and in the United States are defined by the Institute of Medicine (IOM). According to the IOM, functional fibre "consists of isolated, non-digestible carbohydrates that have beneficial physiological effects in humans".
Fibre supplements are widely available, and can be found in forms such as powders, tablets and capsules. Consumption of fibre supplements may be for: improving dietary intake, lowering blood cholesterol, alleviating irritable bowel syndrome, reducing the risk of colon cancer, and increasing feelings of satiety. [http://en.wikipedia.org/wiki/Fibre_supplements]</obo:IAO_0000115>
	<obo:IAO_0000119>WIKIPEDIA:Fibre_supplements</obo:IAO_0000119>
	<obo:IAO_0000114 rdf:resource="&obo;IAO_0000428"/>
	<oboInOwl:hasSynonym xml:lang="en">fibre supplement</oboInOwl:hasSynonym>
	<oboInOwl:hasDbXref>LANGUAL:A1328</oboInOwl:hasDbXref>
</owl:Class>

<owl:Class rdf:about="&obo;FOODON_03401329">
	<rdfs:label xml:lang="en">dietary supplement, not specified</rdfs:label>
	<rdfs:subClassOf rdf:resource="&obo;FOODON_03401298"/>
	<obo:IAO_0000412>http://langual.org</obo:IAO_0000412>
	<obo:IAO_0000114 rdf:resource="&obo;IAO_0000428"/>
	<rdfs:comment xml:lang="en">LanguaL curation note: Use only when no supplement type is evident from the product name.</rdfs:comment>
	<oboInOwl:hasDbXref>LANGUAL:A1329</oboInOwl:hasDbXref>
</owl:Class>

<owl:Class rdf:about="&obo;FOODON_03401330">
	<rdfs:label xml:lang="en">cereal bar (eurofir)</rdfs:label>
	<rdfs:subClassOf rdf:resource="&obo;FOODON_03400816"/>
	<obo:IAO_0000412>http://langual.org</obo:IAO_0000412>
	<obo:IAO_0000114 rdf:resource="&obo;IAO_0000428"/>
	<oboInOwl:hasSynonym xml:lang="en">flapjack bar</oboInOwl:hasSynonym>
	<oboInOwl:hasSynonym xml:lang="en">granola bar</oboInOwl:hasSynonym>
	<oboInOwl:hasSynonym xml:lang="en">muesli bar</oboInOwl:hasSynonym>
	<oboInOwl:hasDbXref>LANGUAL:A1330</oboInOwl:hasDbXref>
</owl:Class>

<owl:Class rdf:about="&obo;FOODON_03401331">
	<rdfs:label xml:lang="en">biscuits, sweet and semi-sweet (eurofir)</rdfs:label>
	<rdfs:subClassOf rdf:resource="&obo;FOODON_03400821"/>
	<obo:IAO_0000412>http://langual.org</obo:IAO_0000412>
	<obo:IAO_0000115 xml:lang="en">Sweetened bakery product baked in individual portions that are usually smal and flat.[US CFR 21]</obo:IAO_0000115>
	<obo:IAO_0000114 rdf:resource="&obo;IAO_0000428"/>
	<oboInOwl:hasSynonym xml:lang="en">cookie</oboInOwl:hasSynonym>
	<oboInOwl:hasDbXref>LANGUAL:A1331</oboInOwl:hasDbXref>
</owl:Class>

<owl:Class rdf:about="&obo;FOODON_03401332">
	<rdfs:label xml:lang="en">pastries and cakes (eurofir)</rdfs:label>
	<rdfs:subClassOf rdf:resource="&obo;FOODON_03400821"/>
	<obo:IAO_0000412>http://langual.org</obo:IAO_0000412>
	<obo:IAO_0000114 rdf:resource="&obo;IAO_0000428"/>
	<oboInOwl:hasDbXref>LANGUAL:A1332</oboInOwl:hasDbXref>
</owl:Class>

<owl:Class rdf:about="&obo;FOODON_03401333">
	<rdfs:label xml:lang="en">cake (eurofir)</rdfs:label>
	<rdfs:subClassOf rdf:resource="&obo;FOODON_03401332"/>
	<obo:IAO_0000412>http://langual.org</obo:IAO_0000412>
	<obo:IAO_0000114 rdf:resource="&obo;IAO_0000428"/>
	<oboInOwl:hasDbXref>LANGUAL:A1333</oboInOwl:hasDbXref>
</owl:Class>

<owl:Class rdf:about="&obo;FOODON_03401334">
	<rdfs:label xml:lang="en">pie, sweetened (eurofir)</rdfs:label>
	<rdfs:subClassOf rdf:resource="&obo;FOODON_03401332"/>
	<obo:IAO_0000412>http://langual.org</obo:IAO_0000412>
	<obo:IAO_0000114 rdf:resource="&obo;IAO_0000428"/>
	<oboInOwl:hasDbXref>LANGUAL:A1334</oboInOwl:hasDbXref>
</owl:Class>

<owl:Class rdf:about="&obo;FOODON_03401335">
	<rdfs:label xml:lang="en">mushroom dish (eurofir)</rdfs:label>
	<rdfs:subClassOf rdf:resource="&obo;FOODON_03400828"/>
	<obo:IAO_0000412>http://langual.org</obo:IAO_0000412>
	<obo:IAO_0000114 rdf:resource="&obo;IAO_0000428"/>
	<oboInOwl:hasDbXref>LANGUAL:A1335</oboInOwl:hasDbXref>
</owl:Class></rdf:RDF>